@prefix ddhub: <http://ddhub.no/>.
@prefix owl: <http://www.w3.org/2002/07/owl#>.
@prefix rdf: <http://www.w3.org/1999/02/22-rdf-syntax-ns#>.
@prefix rdfs: <http://www.w3.org/2000/01/rdf-schema#>.
@prefix xsd: <http://www.w3.org/2001/XMLSchema#>.
@base <https://rdfsharp.codeplex.com/>.

ddhub:Aangstroem a owl:Class; 
                 rdfs:comment """[v] = a * [SI]
where
[v] is the value in ångstrøm
[SI] is the value in SI
a = 1.0/Angstrom, i.e., 10000000000
and
Angstrom = 1e-10
"""@EN; 
                 rdfs:subClassOf ddhub:Unit. 
ddhub:Abampere a owl:Class; 
               rdfs:comment """[v] = a * [SI]
where
[v] is the value in abampere
[SI] is the value in SI
a = 1.0/Deca, i.e., 0.1
and
Deca = 10.0
"""@EN; 
               rdfs:subClassOf ddhub:Unit. 
ddhub:AbnormalAxialOscillation a owl:Class; 
                               rdfs:comment """This Noun is used to refer to abnormal axial oscillations.
"""@EN; 
                               rdfs:subClassOf ddhub:AbnormalOscillation. 
ddhub:AbnormalLateralOscillation a owl:Class; 
                                 rdfs:comment """This Noun is used to refer to abnormal lateral oscillations.
"""@EN; 
                                 rdfs:subClassOf ddhub:AbnormalOscillation. 
ddhub:AbnormalOscillation a owl:Class; 
                          rdfs:comment """This Noun represents abnormal oscillations along the drill-stem.
"""@EN; 
                          rdfs:subClassOf ddhub:DrillingIncident. 
ddhub:AbnormalTorsionalOscillation a owl:Class; 
                                   rdfs:comment """This Noun is used to refer to abnormal torsional oscillations.
"""@EN; 
                                   rdfs:subClassOf ddhub:AbnormalOscillation. 
ddhub:AbscissaReferenceLocation a owl:Class; 
                                rdfs:comment ""@EN; 
                                rdfs:subClassOf ddhub:Location. 
ddhub:AbsolutePressureReference a owl:Class; 
                                rdfs:comment ""@EN; 
                                rdfs:subClassOf ddhub:PressureReference. 
ddhub:AbsoluteTimeReference a owl:Class; 
                            rdfs:comment ""@EN; 
                            rdfs:subClassOf ddhub:TimeReference. 
ddhub:AccelerationDrillingQuantity a owl:Class; 
                                   rdfs:comment """**Acceleration** is defined as the rate of change of velocity with respect to time. Velocity itself is the rate of change of displacement (or position) with respect to time. Therefore, acceleration is the rate of change of displacement twice with respect to time.
Let's break this down:
1. **Displacement** (or position) has the dimension of **Length(L)**.
2. **Velocity** is displacement per unit time:
$$\\text{Velocity} = \\frac{\\text{Length}}{\\text{Time}} = \\frac{L}{T}$$
So, the dimension of velocity is **$[L T^{ -1}]$**.
3. **Acceleration** is the rate of change of velocity with respect to time:
$$\\text{Acceleration} = \\frac{\\text{Velocity}}{\\text{Time}} = \\frac{L T^{ -1}}{T} = L T ^{-2}$$
Therefore, the dimension of acceleration is $[LT^{-2}]$.
The SI unit for **acceleration** is: metre per second squared with the associated unit label $\\frac{m}{s^{2}}$
The meaningful precision of acceleration in the drilling context is typically: 0.001 m/s²
"""@EN; 
                                   rdfs:subClassOf ddhub:MeasurableQuantity. 
ddhub:AccelerationQuantity a owl:Class; 
                           rdfs:comment """**Acceleration** is defined as the rate of change of velocity with respect to time. Velocity itself is the rate of change of displacement (or position) with respect to time. Therefore, acceleration is the rate of change of displacement twice with respect to time.
Let's break this down:
1. **Displacement** (or position) has the dimension of **Length(L)**.
2. **Velocity** is displacement per unit time:
$$\\text{Velocity} = \\frac{\\text{Length}}{\\text{Time}} = \\frac{L}{T}$$
So, the dimension of velocity is **$[L T^{ -1}]$**.
3. **Acceleration** is the rate of change of velocity with respect to time:
$$\\text{Acceleration} = \\frac{\\text{Velocity}}{\\text{Time}} = \\frac{L T^{ -1}}{T} = L T ^{-2}$$
Therefore, the dimension of acceleration is $[LT^{-2}]$.
The SI unit for **acceleration** is: metre per second squared with the associated unit label $\\frac{m}{s^{2}}$
"""@EN; 
                           rdfs:subClassOf ddhub:Quantity. 
ddhub:Accelerator a owl:Class; 
                  rdfs:comment ""@EN; 
                  rdfs:subClassOf ddhub:JarringAssembly. 
ddhub:AccountsFor a owl:ObjectProperty; 
                  rdfs:comment """This verb is used to indicate something accounts for a drilling management feature.
"""@EN; 
                  rdfs:domain ddhub:DWISNoun; 
                  rdfs:range ddhub:DrillingManagementFeature; 
                  rdfs:subPropertyOf ddhub:DWISVerb. 
ddhub:Accumulator a owl:Class; 
                  rdfs:comment ""@EN; 
                  rdfs:subClassOf ddhub:WellControlSystem. 
ddhub:Accuracy a owl:DatatypeProperty, owl:FunctionalProperty; 
               rdfs:comment """The standard deviation of the systematic bias component of the uncertainty of the sensor. The assumed mean value of the attached Gaussian distribution is the measured value. The value is expected to be in the same physical quantity as the sensor value.
"""@EN; 
               rdfs:domain ddhub:SensorUncertainty; 
               rdfs:range xsd:double. 
ddhub:Acoustic a owl:Class; 
               rdfs:comment ""@EN; 
               rdfs:subClassOf ddhub:EquipmentTelemetry. 
ddhub:AcousticTelemetry a owl:Class; 
                        rdfs:comment """A method that allows transfer of downhole data to the surface via acoustic waves along the drill-string.
"""@EN; 
                        rdfs:subClassOf ddhub:DownHoleTelemetry. 
ddhub:Acre a owl:Class; 
           rdfs:comment """[v] = a * [SI]
where
[v] is the value in acre
[SI] is the value in SI
a = 1.0/Acre, i.e., 0.0002471053814671654
and
Acre = SurveyorChain * Furlong reference: https://en.wikipedia.org/wiki/Acre
SurveyorChain = 22.0 * Yard reference: https://www.britannica.com/technology/surveyors-chain
Furlong = 660.0 * Foot reference: https://www.britannica.com/science/furlong
Yard = 3.0 * Foot
Foot = 12.0 * Inch
Inch = 0.0254 reference: https://www.nist.gov/pml/owm/si-units-length
"""@EN; 
           rdfs:subClassOf ddhub:Unit. 
ddhub:Action a owl:Class; 
             rdfs:comment ""@EN; 
             rdfs:subClassOf ddhub:PistonMudPump. 
ddhub:ActionStep a owl:Class; 
                 rdfs:comment """An action step is at the second level of a rig action plan.
"""@EN; 
                 rdfs:subClassOf ddhub:OperationalStep. 
ddhub:ActivableFunction a owl:Class; 
                        rdfs:comment """An `ActivableFunction` is an ADCS function that can be activated. Here activation means that the
function may run immediately or that it is enabled and can trigger if some conditions are respected.
"""@EN; 
                        rdfs:subClassOf ddhub:DWISNoun. 
ddhub:ActivationState a owl:Class; 
                      rdfs:comment ""@EN; 
                      rdfs:subClassOf ddhub:ProceduralState. 
ddhub:ActiveDrillingSystem a owl:Class; 
                           rdfs:comment ""@EN; 
                           rdfs:subClassOf ddhub:MudPits. 
ddhub:ActiveLine a owl:Class; 
                 rdfs:comment ""@EN; 
                 rdfs:subClassOf ddhub:DrillLine. 
ddhub:ActiveVibrationTools a owl:Class; 
                           rdfs:comment ""@EN; 
                           rdfs:subClassOf ddhub:DrillingEquipment. 
ddhub:ActiveVolume a owl:Class; 
                   rdfs:comment ""@EN; 
                   rdfs:subClassOf ddhub:PrototypeData. 
ddhub:AdapterSpool a owl:Class; 
                   rdfs:comment ""@EN; 
                   rdfs:subClassOf ddhub:WellControlSystem. 
ddhub:AdjustableKickoffSub a owl:Class; 
                           rdfs:comment ""@EN; 
                           rdfs:subClassOf ddhub:DrillingEquipment. 
ddhub:Advice a owl:Class; 
             rdfs:comment ""@EN; 
             rdfs:subClassOf ddhub:ProcessData. 
ddhub:AdviceType a owl:DatatypeProperty, owl:FunctionalProperty; 
                 rdfs:comment """
"""@EN; 
                 rdfs:domain ddhub:Advisor; 
                 rdfs:range xsd:string. 
ddhub:AdvisedMaximum a owl:Class; 
                     rdfs:comment ""@EN; 
                     rdfs:subClassOf ddhub:Advice. 
ddhub:AdvisedMinimum a owl:Class; 
                     rdfs:comment ""@EN; 
                     rdfs:subClassOf ddhub:Advice. 
ddhub:AdvisedTarget a owl:Class; 
                    rdfs:comment ""@EN; 
                    rdfs:subClassOf ddhub:Advice. 
ddhub:Advisor a owl:Class; 
              rdfs:comment """An advisor is a computation unit that produces an advice on how to control a process. Its output is typically
an AdvisorySystemAdvice.
"""@EN; 
              rdfs:subClassOf ddhub:ComputationUnit. 
ddhub:AdvisorySystemAdvice a owl:Class; 
                           rdfs:comment """An advisory system provides one or several advices. These advices are structured data that are stored as a JSon
string. 
"""@EN; 
                           rdfs:subClassOf ddhub:JSonDataType. 
ddhub:AfmAutofluidMeasSkid a owl:Class; 
                           rdfs:comment ""@EN; 
                           rdfs:subClassOf ddhub:CirculationSystem. 
ddhub:Aggregation a owl:Class; 
                  rdfs:comment ""@EN; 
                  rdfs:subClassOf ddhub:DirectTransformation. 
ddhub:AlgebraicModel a owl:Class; 
                     rdfs:comment """A model that uses algebraic equations.
"""@EN; 
                     rdfs:subClassOf ddhub:MathematicalFormulation. 
ddhub:AllowEnablementSignalFor a owl:ObjectProperty; 
                               rdfs:comment """This verb is used to define a `DrillingDataPoint` tells if it is allowed or not to enable or
disable an activable function. It is expected that the `DrillingDataPoint` is a Boolean value. If the signal is true,
then it is possible to enable or disable the function using the signal associated with `IsEnablingSignalFor`. If it is
false, it is not allowed to enable or disable the `ActivableFunction`, meaning that the signal associated with `IsEnablingSignalFor`
is ignored.
"""@EN; 
                               rdfs:domain ddhub:DrillingDataPoint; 
                               rdfs:range ddhub:ActivableFunction; 
                               rdfs:subPropertyOf ddhub:DWISVerb. 
ddhub:AmountSubstanceQuantity a owl:Class; 
                              rdfs:comment """The **amount of substance** refers to the quantity of entities (such as atoms, molecules, ions, or other particles) in a system.The standard unit used to measure the amount of substance is the **mole** (mol). One mole corresponds to $6.022×10^{23}$ entities (Avogadro's number) of the given substance.
This is one of the nine fundamental dimensions in the International System of Units (SI).A fundamental quantity does not depend on any combinations of other fundamental dimensions.It is denoted $[N]$.
The SI unit for **amount substance** is: mole with the associated unit label $mol$
"""@EN; 
                              rdfs:subClassOf ddhub:Quantity. 
ddhub:Ampere a owl:Class; 
             rdfs:comment """No conversion necessary as the unit choice is SI
"""@EN; 
             rdfs:subClassOf ddhub:Unit. 
ddhub:Anchors a owl:Class; 
              rdfs:comment ""@EN; 
              rdfs:subClassOf ddhub:MooringSystem. 
ddhub:AngleGradientPerLengthDrillingQuantity a owl:Class; 
                                             rdfs:comment """Consider a situation where you have a length $L$ along which an angle $\\theta$ changes. The angle variation gradient is defined as the **rate of change of the angle** per unit change in length. Mathematically, it can be expressed as: 
$$\\text{ Angle Variation Gradient} = \\frac{ d\\theta}{ dL}$$
where: 
"""@EN; 
                                             rdfs:subClassOf ddhub:MeasurableQuantity. 
ddhub:AngleGradientPerLengthQuantity a owl:Class; 
                                     rdfs:comment """Consider a situation where you have a length $L$ along which an angle $\\theta$ changes. The angle variation gradient is defined as the **rate of change of the angle** per unit change in length. Mathematically, it can be expressed as: 
$$\\text{ Angle Variation Gradient} = \\frac{ d\\theta}{ dL}$$
where: 
"""@EN; 
                                     rdfs:subClassOf ddhub:Quantity. 
ddhub:AngleMagneticFluxDensityQuantity a owl:Class; 
                                       rdfs:comment """The **angle magnetic flux density** is the product of an angle by a magnetic flux density. Let's break it down step by step:
1. Magnetic Flux Density
The **magnetic flux density** $\\mathbf{B}$ is a measure of the strength and direction of the magnetic field at a particular point in space. It represents the amount of magnetic flux passing through a unit area perpendicular to the direction of the magnetic field. In simpler terms, it describes how dense or concentrated the magnetic field lines are in a given region.It can be expressed in terms of the fundamental dimensions as:
$$[M][T]^{-2}[I]^{-1}$$
Where:
"""@EN; 
                                       rdfs:subClassOf ddhub:Quantity. 
ddhub:AngleMagneticFluxDensitySurveyInstrumentDrillingQuantity a owl:Class; 
                                                               rdfs:comment """The **angle magnetic flux density** is the product of an angle by a magnetic flux density. Let's break it down step by step:
1. Magnetic Flux Density
The **magnetic flux density** $\\mathbf{B}$ is a measure of the strength and direction of the magnetic field at a particular point in space. It represents the amount of magnetic flux passing through a unit area perpendicular to the direction of the magnetic field. In simpler terms, it describes how dense or concentrated the magnetic field lines are in a given region.It can be expressed in terms of the fundamental dimensions as:
$$[M][T]^{-2}[I]^{-1}$$
Where:
"""@EN; 
                                                               rdfs:subClassOf ddhub:MeasurableQuantity. 
ddhub:AngleReferenceFrame a owl:Class; 
                          rdfs:comment ""@EN; 
                          rdfs:subClassOf ddhub:OneDimensionalReferenceFrame. 
ddhub:AngleReferenceLocation a owl:Class; 
                             rdfs:comment ""@EN; 
                             rdfs:subClassOf ddhub:Location. 
ddhub:AngularAccelerationDrillingQuantity a owl:Class; 
                                          rdfs:comment """An angular acceleration is the second derivative compared to time of a plan angle: $\\frac{d^2\\theta}{dt^2}$.
The dimension of angular acceleration is:
$$[{\\theta}T^{-2}]$$.
The SI unit for **angular acceleration** is: radian per second squared with the associated unit label $\\frac{rad}{s^{2}}$
The meaningful precision of angular acceleration in the drilling context is typically: 0.01 rad/s²
"""@EN; 
                                          rdfs:subClassOf ddhub:MeasurableQuantity. 
ddhub:AngularAccelerationQuantity a owl:Class; 
                                  rdfs:comment """An angular acceleration is the second derivative compared to time of a plan angle: $\\frac{d^2\\theta}{dt^2}$.
The dimension of angular acceleration is:
$$[{\\theta}T^{-2}]$$.
The SI unit for **angular acceleration** is: radian per second squared with the associated unit label $\\frac{rad}{s^{2}}$
"""@EN; 
                                  rdfs:subClassOf ddhub:Quantity. 
ddhub:AngularLateralModelling a owl:Class; 
                              rdfs:comment """The model accounts for the angular lateral movement of some parts of the physical system.
"""@EN; 
                              rdfs:subClassOf ddhub:LateralModelling. 
ddhub:AngularVelocityDrillingQuantity a owl:Class; 
                                      rdfs:comment """An angular velocity is the first derivative compared to time of a plan angle: $\\frac{d\\theta}{dt}$.
The dimension of angular velocity is:
$$[{\\theta}T^{-1}]$$.
The SI unit for **angular velocity** is: radian per second with the associated unit label $\\frac{rad}{s}$
The meaningful precision of angular velocity in the drilling context is typically: 0.01 rad/s
"""@EN; 
                                      rdfs:subClassOf ddhub:MeasurableQuantity. 
ddhub:AngularVelocityQuantity a owl:Class; 
                              rdfs:comment """An angular velocity is the first derivative compared to time of a plan angle: $\\frac{d\\theta}{dt}$.
The dimension of angular velocity is:
$$[{\\theta}T^{-1}]$$.
The SI unit for **angular velocity** is: radian per second with the associated unit label $\\frac{rad}{s}$
"""@EN; 
                              rdfs:subClassOf ddhub:Quantity. 
ddhub:AngularVelocitySurveyInstrumentDrillingQuantity a owl:Class; 
                                                      rdfs:comment """An angular velocity is the first derivative compared to time of a plan angle: $\\frac{d\\theta}{dt}$.
The dimension of angular velocity is:
$$[{\\theta}T^{-1}]$$.
The SI unit for **angular velocity** is: radian per second with the associated unit label $\\frac{rad}{s}$
The meaningful precision of angular velocity related to survey instrument performance models in the drilling context is typically: 1E-07 rad•T
"""@EN; 
                                                      rdfs:subClassOf ddhub:MeasurableQuantity. 
ddhub:Annular a owl:Class; 
              rdfs:comment ""@EN; 
              rdfs:subClassOf ddhub:HydraulicBranch. 
ddhub:AnnularPreventer a owl:Class; 
                       rdfs:comment ""@EN; 
                       rdfs:subClassOf ddhub:BopElement. 
ddhub:ArcMinute a owl:Class; 
                rdfs:comment """[v] = a * [SI]
where
[v] is the value in arc minute
[SI] is the value in SI
a = 60.0*Degree, i.e., 3437.746770784939
and
Degree = 180.0 / System.Math.PI
"""@EN; 
                rdfs:subClassOf ddhub:Unit. 
ddhub:ArcSecond a owl:Class; 
                rdfs:comment """[v] = a * [SI]
where
[v] is the value in arc second
[SI] is the value in SI
a = 60.0*60.0*Degree, i.e., 206264.80624709636
and
Degree = 180.0 / System.Math.PI
"""@EN; 
                rdfs:subClassOf ddhub:Unit. 
ddhub:AreaDrillingQuantity a owl:Class; 
                           rdfs:comment """Area is the measure of the extent of a surface or the size of a two-dimensional shape.
The dimension of area is:
$$[L^{2}]$$.
The SI unit for **area** is: square metre with the associated unit label $m^{2}$
The meaningful precision of area in the drilling context is typically: 1E-06 m²
"""@EN; 
                           rdfs:subClassOf ddhub:MeasurableQuantity. 
ddhub:AreaQuantity a owl:Class; 
                   rdfs:comment """Area is the measure of the extent of a surface or the size of a two-dimensional shape.
The dimension of area is:
$$[L^{2}]$$.
The SI unit for **area** is: square metre with the associated unit label $m^{2}$
"""@EN; 
                   rdfs:subClassOf ddhub:Quantity. 
ddhub:AssociatesMeasurableQuantity a owl:ObjectProperty; 
                                   rdfs:comment """This `Verb` is typically used when defining a `UnitSystem`. It allows to associate a
`MeasurableQuantityUnitAssociation` with a `MeasurableQuantity`.
"""@EN; 
                                   rdfs:domain ddhub:MeasurableQuantityUnitAssociation; 
                                   rdfs:range ddhub:MeasurableQuantity; 
                                   rdfs:subPropertyOf ddhub:DWISVerb. 
ddhub:AssociatesUnit a owl:ObjectProperty; 
                     rdfs:comment """This `Verb` is typically used when defining a `UnitSystem`. It allows to associate a
`MeasurableQuantityUnitAssociation` with a `Unit`.
"""@EN; 
                     rdfs:domain ddhub:MeasurableQuantityUnitAssociation; 
                     rdfs:range ddhub:Unit; 
                     rdfs:subPropertyOf ddhub:DWISVerb. 
ddhub:AstronomicalUnit a owl:Class; 
                       rdfs:comment """[v] = a * [SI]
where
[v] is the value in astronomical unit
[SI] is the value in SI
a = 1.0/AstronomicalUnit, i.e., 6.684587122268445E-12
and
AstronomicalUnit = 149597870700.0 reference: https://www.iau.org/static/resolutions/IAU2012_English.pdf
"""@EN; 
                       rdfs:subClassOf ddhub:Unit. 
ddhub:AtomMassUnit a owl:Class; 
                   rdfs:comment """[v] = a * [SI]
where
[v] is the value in atom mass unit
[SI] is the value in SI
a = 1.0/AtomicMass, i.e., 6.022140762081123E+26
and
AtomicMass = 1.66053906660e-27 reference: https://en.wikipedia.org/wiki/Atomic_mass
"""@EN; 
                   rdfs:subClassOf ddhub:Unit. 
ddhub:Attowatt a owl:Class; 
               rdfs:comment """[v] = a * [SI]
where
[v] is the value in attowatt
[SI] is the value in SI
a = 1.0/Atto, i.e., 9.999999999999999E+17
and
Atto = 1e-18
"""@EN; 
               rdfs:subClassOf ddhub:Unit. 
ddhub:AverageDelayByRepeater a owl:DatatypeProperty, owl:FunctionalProperty; 
                             rdfs:comment """The average delay caused by each repeater. The physical quantity is Time and the unit is second.
"""@EN; 
                             rdfs:domain ddhub:Telemetry; 
                             rdfs:range xsd:double. 
ddhub:AxialModelling a owl:Class; 
                     rdfs:comment """The model accounts for the axial movement of some parts of the physical system.
"""@EN; 
                     rdfs:subClassOf ddhub:ModelledDegreeOfFreedom. 
ddhub:AxialMotionType a owl:Class; 
                      rdfs:comment ""@EN; 
                      rdfs:subClassOf ddhub:MotionType. 
ddhub:AxialReferenceLocation a owl:Class; 
                             rdfs:comment ""@EN; 
                             rdfs:subClassOf ddhub:Location. 
ddhub:AxialVelocityDrillingQuantity a owl:Class; 
                                    rdfs:comment """A velocity is the time derivative of a position or a displacement: $\\frac{dx}{dt}$, where $x$ is a position and $t$ is time.
The dimension of velocity is:
$$[LT^{-1}]$$.
The SI unit for **velocity** is: metre per second with the associated unit label $\\frac{m}{s}$
The meaningful precision of velocity in the drilling context is typically: 0.01 m/s
"""@EN; 
                                    rdfs:subClassOf ddhub:MeasurableQuantity. 
ddhub:AxialVelocityLimit a owl:Class; 
                         rdfs:comment """This Noun is used to refer to an axial velocity limit.
"""@EN; 
                         rdfs:subClassOf ddhub:DrillingLimit. 
ddhub:Azimuth a owl:Class; 
              rdfs:comment ""@EN; 
              rdfs:subClassOf ddhub:PrototypeData. 
ddhub:AzimuthalTools a owl:Class; 
                     rdfs:comment ""@EN; 
                     rdfs:subClassOf ddhub:LoggingWhileDrillingTools. 
ddhub:AzimuthReferenceLocation a owl:Class; 
                               rdfs:comment ""@EN; 
                               rdfs:subClassOf ddhub:Location. 
ddhub:BackPressurePump a owl:Class; 
                       rdfs:comment ""@EN; 
                       rdfs:subClassOf ddhub:CirculationSystem. 
ddhub:BackPressurePumpPressure a owl:Class; 
                               rdfs:comment ""@EN; 
                               rdfs:subClassOf ddhub:PrototypeData. 
ddhub:BackwardWhirl a owl:Class; 
                    rdfs:comment """This Noun is used to refer to backward whirl.
"""@EN; 
                    rdfs:subClassOf ddhub:Whirling. 
ddhub:BallastSystem a owl:Class; 
                    rdfs:comment ""@EN; 
                    rdfs:subClassOf ddhub:MarineSystem. 
ddhub:BallJoint a owl:Class; 
                rdfs:comment ""@EN; 
                rdfs:subClassOf ddhub:DrillingRiser. 
ddhub:BandPassFilter a owl:Class; 
                     rdfs:comment ""@EN; 
                     rdfs:subClassOf ddhub:Filter. 
ddhub:Bar a owl:Class; 
          rdfs:comment """[v] = a * [SI]
where
[v] is the value in bar
[SI] is the value in SI
a = 1.0/Bar, i.e., 1E-05
and
Bar = 1e5 reference: https://en.wikipedia.org/wiki/Bar_(unit)
"""@EN; 
          rdfs:subClassOf ddhub:Unit. 
ddhub:BarPerHour a owl:Class; 
                 rdfs:comment """[v] = a * [SI]
where
[v] is the value in bar per hour
[SI] is the value in SI
a = Hour/Bar, i.e., 0.036
and
Hour = 60.0 * Minute
Bar = 1e5 reference: https://en.wikipedia.org/wiki/Bar_(unit)
Minute = 60.0
"""@EN; 
                 rdfs:subClassOf ddhub:Unit. 
ddhub:BarPerMetre a owl:Class; 
                  rdfs:comment """[v] = a * [SI]
where
[v] is the value in bar per metre
[SI] is the value in SI
a = 1.0/Bar, i.e., 1E-05
and
Bar = 1e5 reference: https://en.wikipedia.org/wiki/Bar_(unit)
"""@EN; 
                  rdfs:subClassOf ddhub:Unit. 
ddhub:BarPerMinute a owl:Class; 
                   rdfs:comment """[v] = a * [SI]
where
[v] is the value in bar per minute
[SI] is the value in SI
a = Minute/Bar, i.e., 0.0006
and
Minute = 60.0
Bar = 1e5 reference: https://en.wikipedia.org/wiki/Bar_(unit)
"""@EN; 
                   rdfs:subClassOf ddhub:Unit. 
ddhub:BarPerSecond a owl:Class; 
                   rdfs:comment """[v] = a * [SI]
where
[v] is the value in bar per second
[SI] is the value in SI
a = 1.0/Bar, i.e., 1E-05
and
Bar = 1e5 reference: https://en.wikipedia.org/wiki/Bar_(unit)
"""@EN; 
                   rdfs:subClassOf ddhub:Unit. 
ddhub:Barrel a owl:Class; 
             rdfs:comment """[v] = a * [SI]
where
[v] is the value in barrel
[SI] is the value in SI
a = 1.0/Barrel, i.e., 6.289810770432106
and
Barrel = 42.0 * GallonUS reference: https://en.wikipedia.org/wiki/Barrel_(unit)
GallonUS = 231.0 * Inch * Inch * Inch reference: https://en.wikipedia.org/wiki/Gallon
Inch = 0.0254 reference: https://www.nist.gov/pml/owm/si-units-length
"""@EN; 
             rdfs:subClassOf ddhub:Unit. 
ddhub:BarrelPerDay a owl:Class; 
                   rdfs:comment """[v] = a * [SI]
where
[v] is the value in barrel per day
[SI] is the value in SI
a = Day / Barrel, i.e., 543439.6505653339
and
Day = 24.0 * Hour
Barrel = 42.0 * GallonUS reference: https://en.wikipedia.org/wiki/Barrel_(unit)
Hour = 60.0 * Minute
GallonUS = 231.0 * Inch * Inch * Inch reference: https://en.wikipedia.org/wiki/Gallon
Minute = 60.0
Inch = 0.0254 reference: https://www.nist.gov/pml/owm/si-units-length
"""@EN; 
                   rdfs:subClassOf ddhub:Unit. 
ddhub:BarrelPerHour a owl:Class; 
                    rdfs:comment """[v] = a * [SI]
where
[v] is the value in barrel per hour
[SI] is the value in SI
a = Hour/ Barrel, i.e., 22643.31877355558
and
Hour = 60.0 * Minute
Barrel = 42.0 * GallonUS reference: https://en.wikipedia.org/wiki/Barrel_(unit)
Minute = 60.0
GallonUS = 231.0 * Inch * Inch * Inch reference: https://en.wikipedia.org/wiki/Gallon
Inch = 0.0254 reference: https://www.nist.gov/pml/owm/si-units-length
"""@EN; 
                    rdfs:subClassOf ddhub:Unit. 
ddhub:BarrelPerMinute a owl:Class; 
                      rdfs:comment """[v] = a * [SI]
where
[v] is the value in barrel per minute
[SI] is the value in SI
a = Minute /Barrel, i.e., 377.3886462259263
and
Minute = 60.0
Barrel = 42.0 * GallonUS reference: https://en.wikipedia.org/wiki/Barrel_(unit)
GallonUS = 231.0 * Inch * Inch * Inch reference: https://en.wikipedia.org/wiki/Gallon
Inch = 0.0254 reference: https://www.nist.gov/pml/owm/si-units-length
"""@EN; 
                      rdfs:subClassOf ddhub:Unit. 
ddhub:BarrelPerSecond a owl:Class; 
                      rdfs:comment """[v] = a * [SI]
where
[v] is the value in barrel per second
[SI] is the value in SI
a = 1.0/Barrel, i.e., 6.289810770432106
and
Barrel = 42.0 * GallonUS reference: https://en.wikipedia.org/wiki/Barrel_(unit)
GallonUS = 231.0 * Inch * Inch * Inch reference: https://en.wikipedia.org/wiki/Gallon
Inch = 0.0254 reference: https://www.nist.gov/pml/owm/si-units-length
"""@EN; 
                      rdfs:subClassOf ddhub:Unit. 
ddhub:BarrelPerYear a owl:Class; 
                    rdfs:comment """[v] = a * [SI]
where
[v] is the value in barrel per year
[SI] is the value in SI
a = YearJulian /Barrel, i.e., 198491332.36898822
and
YearJulian = 365.25 * Day
Barrel = 42.0 * GallonUS reference: https://en.wikipedia.org/wiki/Barrel_(unit)
Day = 24.0 * Hour
GallonUS = 231.0 * Inch * Inch * Inch reference: https://en.wikipedia.org/wiki/Gallon
Hour = 60.0 * Minute
Inch = 0.0254 reference: https://www.nist.gov/pml/owm/si-units-length
Minute = 60.0
"""@EN; 
                    rdfs:subClassOf ddhub:Unit. 
ddhub:Beacons a owl:Class; 
              rdfs:comment ""@EN; 
              rdfs:subClassOf ddhub:MarineSystem. 
ddhub:BellNipple a owl:Class; 
                 rdfs:comment ""@EN; 
                 rdfs:subClassOf ddhub:WellControlSystem. 
ddhub:BelongsToClass a owl:ObjectProperty; 
                     rdfs:comment """The verb is used between a node and a Noun, i.e., a class. Semantically it can be considered as a synonym to `rdf:type`. It has been introduced to overcome limitations from OPC-UA that does not allow for multiple inheritance. Note that the same node can be in relation using `BelongsToClass` to several classes.
"""@EN; 
                     rdfs:domain ddhub:DWISNoun; 
                     rdfs:range ddhub:DWISNoun; 
                     rdfs:subPropertyOf ddhub:DWISVerb. 
ddhub:BelongsToSynchronizationGroup a owl:ObjectProperty; 
                                    rdfs:comment ""@EN; 
                                    rdfs:domain ddhub:Resampling; 
                                    rdfs:range ddhub:SynchronizationGroup; 
                                    rdfs:subPropertyOf ddhub:DWISVerb. 
ddhub:BerlinerLichteinheit a owl:Class; 
                           rdfs:comment """[v] = a * [SI]
where
[v] is the value in berliner lichteinheit
[SI] is the value in SI
a = 1.0/ Hefnerkerze, i.e., 1.0869565217391304
and
Hefnerkerze = 0.92 reference: https://en.wikipedia.org/wiki/Hefner_lamp
"""@EN; 
                           rdfs:subClassOf ddhub:Unit. 
ddhub:BHAAnnular a owl:Class; 
                 rdfs:comment ""@EN; 
                 rdfs:subClassOf ddhub:Annular. 
ddhub:BHAInner a owl:Class; 
               rdfs:comment ""@EN; 
               rdfs:subClassOf ddhub:Pipe. 
ddhub:BhaVibrationDampers a owl:Class; 
                          rdfs:comment ""@EN; 
                          rdfs:subClassOf ddhub:ActiveVibrationTools. 
ddhub:BicenterReamerBit a owl:Class; 
                        rdfs:comment ""@EN; 
                        rdfs:subClassOf ddhub:Reamers. 
ddhub:Biot a owl:Class; 
           rdfs:comment """[v] = a * [SI]
where
[v] is the value in biot
[SI] is the value in SI
a = 1.0/Deca, i.e., 0.1
and
Deca = 10.0
"""@EN; 
           rdfs:subClassOf ddhub:Unit. 
ddhub:BitDepth a owl:Class; 
               rdfs:comment """Curvilinear abscissa of the bottom of the bit, in the reference frame centered in the wellbore.
"""@EN; 
               rdfs:subClassOf ddhub:PrototypeData. 
ddhub:BlackBoxModel a owl:Class; 
                    rdfs:comment """The internal workings of the model are unknown or not interpretable, focusing only on the input-output relationship.
"""@EN; 
                    rdfs:subClassOf ddhub:ModelTransparency. 
ddhub:BladeDiameter a owl:Class; 
                    rdfs:comment ""@EN; 
                    rdfs:subClassOf ddhub:Stabilizers. 
ddhub:BladeLength a owl:Class; 
                  rdfs:comment ""@EN; 
                  rdfs:subClassOf ddhub:Stabilizers. 
ddhub:BladeShape a owl:Class; 
                 rdfs:comment ""@EN; 
                 rdfs:subClassOf ddhub:Stabilizers. 
ddhub:BladeType a owl:Class; 
                rdfs:comment ""@EN; 
                rdfs:subClassOf ddhub:Stabilizers. 
ddhub:BladeTypeWelded a owl:Class; 
                      rdfs:comment ""@EN; 
                      rdfs:subClassOf ddhub:BladeType. 
ddhub:BlindRam a owl:Class; 
               rdfs:comment ""@EN; 
               rdfs:subClassOf ddhub:BopElement. 
ddhub:BlockVelocityDrillingQuantity a owl:Class; 
                                    rdfs:comment """A velocity is the time derivative of a position or a displacement: $\\frac{dx}{dt}$, where $x$ is a position and $t$ is time.
The dimension of velocity is:
$$[LT^{-1}]$$.
The SI unit for **velocity** is: metre per second with the associated unit label $\\frac{m}{s}$
The meaningful precision of block velocity in the drilling context is typically: 0.01 m/s
"""@EN; 
                                    rdfs:subClassOf ddhub:MeasurableQuantity. 
ddhub:BooleanDataType a owl:Class; 
                      rdfs:comment ""@EN; 
                      rdfs:subClassOf ddhub:EnumerationDataType. 
ddhub:BoosterLine a owl:Class; 
                  rdfs:comment ""@EN; 
                  rdfs:subClassOf ddhub:MarineSystem. 
ddhub:BoosterPump a owl:Class; 
                  rdfs:comment ""@EN; 
                  rdfs:subClassOf ddhub:CirculationSystem. 
ddhub:BOPControlSystem a owl:Class; 
                       rdfs:comment ""@EN; 
                       rdfs:subClassOf ddhub:ControlSystem. 
ddhub:BopElement a owl:Class; 
                 rdfs:comment ""@EN; 
                 rdfs:subClassOf ddhub:WellControlSystem. 
ddhub:BOPOpening a owl:Class; 
                 rdfs:comment ""@EN; 
                 rdfs:subClassOf ddhub:PrototypeData. 
ddhub:BOPPressure a owl:Class; 
                  rdfs:comment ""@EN; 
                  rdfs:subClassOf ddhub:PrototypeData. 
ddhub:BopStack a owl:Class; 
               rdfs:comment ""@EN; 
               rdfs:subClassOf ddhub:WellControlSystem. 
ddhub:BottomholeAssembly a owl:Class; 
                         rdfs:comment ""@EN; 
                         rdfs:subClassOf ddhub:DrillString. 
ddhub:BottomOfStringReferenceLocation a owl:Class; 
                                      rdfs:comment ""@EN; 
                                      rdfs:subClassOf ddhub:AbscissaReferenceLocation. 
ddhub:BottomShoulderAxialLocation a owl:Class; 
                                  rdfs:comment ""@EN; 
                                  rdfs:subClassOf ddhub:AxialReferenceLocation. 
ddhub:BoundaryDiscretization a owl:Class; 
                             rdfs:comment """A model only considers the bounds of the physical system and does not apply any intermediate discretization.
"""@EN; 
                             rdfs:subClassOf ddhub:ModellingDiscretization. 
ddhub:Box a owl:Class; 
          rdfs:comment ""@EN; 
          rdfs:subClassOf ddhub:Connection. 
ddhub:Boxbox a owl:Class; 
             rdfs:comment ""@EN; 
             rdfs:subClassOf ddhub:TubularConfiguration. 
ddhub:BritishThermalUnit a owl:Class; 
                         rdfs:comment """[v] = a * [SI]
where
[v] is the value in british thermal unit
[SI] is the value in SI
a = 1.0/BTU, i.e., 0.0009484516526770049
and
BTU = 1054.35 reference: https://en.wikipedia.org/wiki/British_thermal_unit
"""@EN; 
                         rdfs:subClassOf ddhub:Unit. 
ddhub:BritishThermalUnitInchPerHourSquareFootDegreeFahrenheit a owl:Class; 
                                                              rdfs:comment """[v] = a * [SI]
where
[v] is the value in british thermal unit inch per hour square foot degree fahrenheit
[SI] is the value in SI
a = Hour*Foot*Foot*FahrenheitSlope/(BTU*Inch), i.e., 6.938113529662824
and
Hour = 60.0 * Minute
Foot = 12.0 * Inch
FahrenheitSlope = 5.0 / 9.0 reference: https://nn.wikipedia.org/wiki/Fahrenheit
BTU = 1054.35 reference: https://en.wikipedia.org/wiki/British_thermal_unit
Inch = 0.0254 reference: https://www.nist.gov/pml/owm/si-units-length
Minute = 60.0
"""@EN; 
                                                              rdfs:subClassOf ddhub:Unit. 
ddhub:BritishThermalUnitInchPerHourSquareFootDegreeFahrenheitSquared a owl:Class; 
                                                                     rdfs:comment """[v] = a * [SI]
where
[v] is the value in british thermal unit inch per hour square foot degree fahrenheit squared
[SI] is the value in SI
a = Hour*Foot*Foot*FahrenheitSlope*FahrenheitSlope/(BTU*Inch), i.e., 3.8545075164793468
and
Hour = 60.0 * Minute
Foot = 12.0 * Inch
FahrenheitSlope = 5.0 / 9.0 reference: https://nn.wikipedia.org/wiki/Fahrenheit
BTU = 1054.35 reference: https://en.wikipedia.org/wiki/British_thermal_unit
Inch = 0.0254 reference: https://www.nist.gov/pml/owm/si-units-length
Minute = 60.0
"""@EN; 
                                                                     rdfs:subClassOf ddhub:Unit. 
ddhub:BritishThermalUnitPerCubicFoot a owl:Class; 
                                     rdfs:comment """[v] = a * [SI]
where
[v] is the value in british thermal unit per cubic foot
[SI] is the value in SI
a = Foot * Foot * Foot / BTU, i.e., 2.6857159948783606E-05
and
Foot = 12.0 * Inch
BTU = 1054.35 reference: https://en.wikipedia.org/wiki/British_thermal_unit
Inch = 0.0254 reference: https://www.nist.gov/pml/owm/si-units-length
"""@EN; 
                                     rdfs:subClassOf ddhub:Unit. 
ddhub:BritishThermalUnitPerCubicInch a owl:Class; 
                                     rdfs:comment """[v] = a * [SI]
where
[v] is the value in british thermal unit per cubic inch
[SI] is the value in SI
a = Inch*Inch*Inch/BTU, i.e., 1.554233793332385E-08
and
Inch = 0.0254 reference: https://www.nist.gov/pml/owm/si-units-length
BTU = 1054.35 reference: https://en.wikipedia.org/wiki/British_thermal_unit
"""@EN; 
                                     rdfs:subClassOf ddhub:Unit. 
ddhub:BritishThermalUnitPerCubicMetre a owl:Class; 
                                      rdfs:comment """[v] = a * [SI]
where
[v] is the value in british thermal unit per cubic metre
[SI] is the value in SI
a = 1.0/BTU, i.e., 0.0009484516526770049
and
BTU = 1054.35 reference: https://en.wikipedia.org/wiki/British_thermal_unit
"""@EN; 
                                      rdfs:subClassOf ddhub:Unit. 
ddhub:BritishThermalUnitPerGallonUk a owl:Class; 
                                    rdfs:comment """[v] = a * [SI]
where
[v] is the value in british thermal unit per gallon (UK)
[SI] is the value in SI
a = GallonUK / BTU, i.e., 4.311746573718405E-06
and
GallonUK = 4.54609e-3 reference: https://en.wikipedia.org/wiki/Gallon
BTU = 1054.35 reference: https://en.wikipedia.org/wiki/British_thermal_unit
"""@EN; 
                                    rdfs:subClassOf ddhub:Unit. 
ddhub:BritishThermalUnitPerGallonUs a owl:Class; 
                                    rdfs:comment """[v] = a * [SI]
where
[v] is the value in british thermal unit per gallon (US)
[SI] is the value in SI
a = GallonUS / BTU, i.e., 3.5902800625978092E-06
and
GallonUS = 231.0 * Inch * Inch * Inch reference: https://en.wikipedia.org/wiki/Gallon
BTU = 1054.35 reference: https://en.wikipedia.org/wiki/British_thermal_unit
Inch = 0.0254 reference: https://www.nist.gov/pml/owm/si-units-length
"""@EN; 
                                    rdfs:subClassOf ddhub:Unit. 
ddhub:BritishThermalUnitPerHourFootDegreeFahrenheit a owl:Class; 
                                                    rdfs:comment """[v] = a * [SI]
where
[v] is the value in british thermal unit per hour foot degree fahrenheit
[SI] is the value in SI
a = Hour*Foot*FahrenheitSlope/BTU, i.e., 0.5781761274719021
and
Hour = 60.0 * Minute
Foot = 12.0 * Inch
FahrenheitSlope = 5.0 / 9.0 reference: https://nn.wikipedia.org/wiki/Fahrenheit
BTU = 1054.35 reference: https://en.wikipedia.org/wiki/British_thermal_unit
Minute = 60.0
Inch = 0.0254 reference: https://www.nist.gov/pml/owm/si-units-length
"""@EN; 
                                                    rdfs:subClassOf ddhub:Unit. 
ddhub:BritishThermalUnitPerHourFootDegreeFahrenheitSquared a owl:Class; 
                                                           rdfs:comment """[v] = a * [SI]
where
[v] is the value in british thermal unit per hour foot degree fahrenheit squared
[SI] is the value in SI
a = Hour*Foot*FahrenheitSlope*FahrenheitSlope/BTU, i.e., 0.3212089597066123
and
Hour = 60.0 * Minute
Foot = 12.0 * Inch
FahrenheitSlope = 5.0 / 9.0 reference: https://nn.wikipedia.org/wiki/Fahrenheit
BTU = 1054.35 reference: https://en.wikipedia.org/wiki/British_thermal_unit
Minute = 60.0
Inch = 0.0254 reference: https://www.nist.gov/pml/owm/si-units-length
"""@EN; 
                                                           rdfs:subClassOf ddhub:Unit. 
ddhub:BritishThermalUnitPerHourPerSquareFootPerDegreeFahrenheit a owl:Class; 
                                                                rdfs:comment """[v] = a * [SI]
where
[v] is the value in british thermal unit per hour per square foot per degree fahrenheit
[SI] is the value in SI
a = Hour * Foot*Foot * FahrenheitSlope / BTU, i.e., 0.17622808365343573
and
Hour = 60.0 * Minute
Foot = 12.0 * Inch
FahrenheitSlope = 5.0 / 9.0 reference: https://nn.wikipedia.org/wiki/Fahrenheit
BTU = 1054.35 reference: https://en.wikipedia.org/wiki/British_thermal_unit
Minute = 60.0
Inch = 0.0254 reference: https://www.nist.gov/pml/owm/si-units-length
"""@EN; 
                                                                rdfs:subClassOf ddhub:Unit. 
ddhub:BritishThermalUnitPerLitre a owl:Class; 
                                 rdfs:comment """[v] = a * [SI]
where
[v] is the value in british thermal unit per litre
[SI] is the value in SI
a = Litre/BTU, i.e., 9.484516526770049E-07
and
Litre = 0.001
BTU = 1054.35 reference: https://en.wikipedia.org/wiki/British_thermal_unit
"""@EN; 
                                 rdfs:subClassOf ddhub:Unit. 
ddhub:BritishThermalUnitPerPoundDegreeFahrenheit a owl:Class; 
                                                 rdfs:comment """[v] = a * [SI]
where
[v] is the value in british thermal unit per pound degree fahrenheit
[SI] is the value in SI
a = Pound*FahrenheitSlope/BTU, i.e., 0.0002390057960934331
and
Pound = 0.45359237 reference: https://en.wikipedia.org/wiki/Pound_(mass)
FahrenheitSlope = 5.0 / 9.0 reference: https://nn.wikipedia.org/wiki/Fahrenheit
BTU = 1054.35 reference: https://en.wikipedia.org/wiki/British_thermal_unit
"""@EN; 
                                                 rdfs:subClassOf ddhub:Unit. 
ddhub:BritishThermalUnitPerPoundSquaredDegreeFahrenheit a owl:Class; 
                                                        rdfs:comment """[v] = a * [SI]
where
[v] is the value in british thermal unit per pound squared degree fahrenheit 
[SI] is the value in SI
a = Pound*FahrenheitSlope*FahrenheitSlope/BTU, i.e., 0.00013278099782968505
and
Pound = 0.45359237 reference: https://en.wikipedia.org/wiki/Pound_(mass)
FahrenheitSlope = 5.0 / 9.0 reference: https://nn.wikipedia.org/wiki/Fahrenheit
BTU = 1054.35 reference: https://en.wikipedia.org/wiki/British_thermal_unit
"""@EN; 
                                                        rdfs:subClassOf ddhub:Unit. 
ddhub:Buffering a owl:Class; 
                rdfs:comment ""@EN; 
                rdfs:subClassOf ddhub:TimeBasedTransformation. 
ddhub:BufferingInterval a owl:DatatypeProperty, owl:FunctionalProperty; 
                        rdfs:comment """
"""@EN; 
                        rdfs:domain ddhub:Buffering; 
                        rdfs:range xsd:double. 
ddhub:BulkTank a owl:Class; 
               rdfs:comment ""@EN; 
               rdfs:subClassOf ddhub:MudPits. 
ddhub:BullNose a owl:Class; 
               rdfs:comment ""@EN; 
               rdfs:subClassOf ddhub:DrillstemTerminator. 
ddhub:CableDiameterDrillingQuantity a owl:Class; 
                                    rdfs:comment """Length is a measure of distance.
The dimension of length is:
$$[L]$$.
The SI unit for **length** is: metre with the associated unit label $m$
The meaningful precision of small length is typically: 0.0005 m
The meaningful precision of a cable diameter in the drilling context is typically: 0.0005 m
"""@EN; 
                                    rdfs:subClassOf ddhub:MeasurableQuantity. 
ddhub:CalibrationModel a owl:Class; 
                       rdfs:comment """A model that focuses on adjusting parameters to improve alignment with observed data.
"""@EN; 
                       rdfs:subClassOf ddhub:ModelingObjective. 
ddhub:Calorie a owl:Class; 
              rdfs:comment """[v] = a * [SI]
where
[v] is the value in calorie
[SI] is the value in SI
a = 1.0/Calorie, i.e., 0.2390057361376673
and
Calorie = 4.184 reference: https://en.wikipedia.org/wiki/Calorie
"""@EN; 
              rdfs:subClassOf ddhub:Unit. 
ddhub:CaloriePerCentimetreSecondDegreeCelsius a owl:Class; 
                                              rdfs:comment """[v] = a * [SI]
where
[v] is the value in calorie per centimetre second degree celsius
[SI] is the value in SI
a = Centi/Calorie, i.e., 0.002390057361376673
and
Centi = 0.01
Calorie = 4.184 reference: https://en.wikipedia.org/wiki/Calorie
"""@EN; 
                                              rdfs:subClassOf ddhub:Unit. 
ddhub:CaloriePerCentimetreSecondDegreeCelsiusSquared a owl:Class; 
                                                     rdfs:comment """[v] = a * [SI]
where
[v] is the value in calorie per centimetre second degree celsius squared
[SI] is the value in SI
a = Centi/Calorie, i.e., 0.002390057361376673
and
Centi = 0.01
Calorie = 4.184 reference: https://en.wikipedia.org/wiki/Calorie
"""@EN; 
                                                     rdfs:subClassOf ddhub:Unit. 
ddhub:CaloriePerCubicFoot a owl:Class; 
                          rdfs:comment """[v] = a * [SI]
where
[v] is the value in calorie per cubic foot
[SI] is the value in SI
a = Foot * Foot * Foot / Calorie, i.e., 0.006767888764818353
and
Foot = 12.0 * Inch
Calorie = 4.184 reference: https://en.wikipedia.org/wiki/Calorie
Inch = 0.0254 reference: https://www.nist.gov/pml/owm/si-units-length
"""@EN; 
                          rdfs:subClassOf ddhub:Unit. 
ddhub:CaloriePerCubicInch a owl:Class; 
                          rdfs:comment """[v] = a * [SI]
where
[v] is the value in calorie per cubic inch
[SI] is the value in SI
a = Inch*Inch*Inch/Calorie, i.e., 3.916602294455067E-06
and
Inch = 0.0254 reference: https://www.nist.gov/pml/owm/si-units-length
Calorie = 4.184 reference: https://en.wikipedia.org/wiki/Calorie
"""@EN; 
                          rdfs:subClassOf ddhub:Unit. 
ddhub:CaloriePerCubicMetre a owl:Class; 
                           rdfs:comment """[v] = a * [SI]
where
[v] is the value in calorie per cubic metre
[SI] is the value in SI
a = 1.0/Calorie, i.e., 0.2390057361376673
and
Calorie = 4.184 reference: https://en.wikipedia.org/wiki/Calorie
"""@EN; 
                           rdfs:subClassOf ddhub:Unit. 
ddhub:CaloriePerGallonUk a owl:Class; 
                         rdfs:comment """[v] = a * [SI]
where
[v] is the value in calorie per gallon (UK)
[SI] is the value in SI
a = GallonUK / Calorie, i.e., 0.0010865415869980878
and
GallonUK = 4.54609e-3 reference: https://en.wikipedia.org/wiki/Gallon
Calorie = 4.184 reference: https://en.wikipedia.org/wiki/Calorie
"""@EN; 
                         rdfs:subClassOf ddhub:Unit. 
ddhub:CaloriePerGallonUs a owl:Class; 
                         rdfs:comment """[v] = a * [SI]
where
[v] is the value in calorie per gallon (US)
[SI] is the value in SI
a = GallonUS / Calorie, i.e., 0.0009047351300191204
and
GallonUS = 231.0 * Inch * Inch * Inch reference: https://en.wikipedia.org/wiki/Gallon
Calorie = 4.184 reference: https://en.wikipedia.org/wiki/Calorie
Inch = 0.0254 reference: https://www.nist.gov/pml/owm/si-units-length
"""@EN; 
                         rdfs:subClassOf ddhub:Unit. 
ddhub:CaloriePerGramDegreeCelsius a owl:Class; 
                                  rdfs:comment """[v] = a * [SI]
where
[v] is the value in calorie per gram degree celsius
[SI] is the value in SI
a = Milli/Calorie, i.e., 0.0002390057361376673
and
Milli = 0.001
Calorie = 4.184 reference: https://en.wikipedia.org/wiki/Calorie
"""@EN; 
                                  rdfs:subClassOf ddhub:Unit. 
ddhub:CaloriePerGramDegreeSquaredCelsius a owl:Class; 
                                         rdfs:comment """[v] = a * [SI]
where
[v] is the value in calorie per gram degree squared celsius
[SI] is the value in SI
a = Milli/Calorie, i.e., 0.0002390057361376673
and
Milli = 0.001
Calorie = 4.184 reference: https://en.wikipedia.org/wiki/Calorie
"""@EN; 
                                         rdfs:subClassOf ddhub:Unit. 
ddhub:CaloriePerLitre a owl:Class; 
                      rdfs:comment """[v] = a * [SI]
where
[v] is the value in calorie per litre
[SI] is the value in SI
a = Litre/Calorie, i.e., 0.0002390057361376673
and
Litre = 0.001
Calorie = 4.184 reference: https://en.wikipedia.org/wiki/Calorie
"""@EN; 
                      rdfs:subClassOf ddhub:Unit. 
ddhub:CaloriePerMetreSecondDegreeCelsius a owl:Class; 
                                         rdfs:comment """[v] = a * [SI]
where
[v] is the value in calorie per metre second degree celsius
[SI] is the value in SI
a = 1.0/Calorie, i.e., 0.2390057361376673
and
Calorie = 4.184 reference: https://en.wikipedia.org/wiki/Calorie
"""@EN; 
                                         rdfs:subClassOf ddhub:Unit. 
ddhub:CaloriePerMetreSecondDegreeCelsiusSquared a owl:Class; 
                                                rdfs:comment """[v] = a * [SI]
where
[v] is the value in calorie per metre second degree celsius squared
[SI] is the value in SI
a = 1.0/Calorie, i.e., 0.2390057361376673
and
Calorie = 4.184 reference: https://en.wikipedia.org/wiki/Calorie
"""@EN; 
                                                rdfs:subClassOf ddhub:Unit. 
ddhub:Candela a owl:Class; 
              rdfs:comment """No conversion necessary as the unit choice is SI
"""@EN; 
              rdfs:subClassOf ddhub:Unit. 
ddhub:CapillaryPressureDrillingQuantity a owl:Class; 
                                        rdfs:comment """Pressure is the force applied per unit area on a surface.
The dimension of pressure is:
$$[ML^{-1}T^{-2}]$$.
The SI unit for **pressure** is: pascal with the associated unit label $Pa$
The meaningful precision of capilary pressure in the drilling context is typically: 0.1 Pa
"""@EN; 
                                        rdfs:subClassOf ddhub:MeasurableQuantity. 
ddhub:Carcel a owl:Class; 
             rdfs:comment """[v] = a * [SI]
where
[v] is the value in carcel
[SI] is the value in SI
a = 1.0/Carcel, i.e., 0.1026694045174538
and
Carcel = 9.74 reference: https://en.wikipedia.org/wiki/Carcel
"""@EN; 
             rdfs:subClassOf ddhub:Unit. 
ddhub:CartesianFourDimensionalReferenceFrame a owl:Class; 
                                             rdfs:comment ""@EN; 
                                             rdfs:subClassOf ddhub:FourDimensionalReferenceFrame. 
ddhub:CartesianThreeDimensionalReferenceFrame a owl:Class; 
                                              rdfs:comment ""@EN; 
                                              rdfs:subClassOf ddhub:ThreeDimensionalReferenceFrame. 
ddhub:CartesianTwoDimensionalReferenceFrame a owl:Class; 
                                            rdfs:comment ""@EN; 
                                            rdfs:subClassOf ddhub:TwoDimensionalReferenceFrame. 
ddhub:CasedHoleTools a owl:Class; 
                     rdfs:comment ""@EN; 
                     rdfs:subClassOf ddhub:WirelineLoggingTools. 
ddhub:Casing a owl:Class; 
             rdfs:comment ""@EN; 
             rdfs:subClassOf ddhub:CasingString. 
ddhub:CasingCollarLocator a owl:Class; 
                          rdfs:comment ""@EN; 
                          rdfs:subClassOf ddhub:WirelineLoggingTools. 
ddhub:CasingCutter a owl:Class; 
                   rdfs:comment ""@EN; 
                   rdfs:subClassOf ddhub:CasingEquipment. 
ddhub:CasingEquipment a owl:Class; 
                      rdfs:comment ""@EN; 
                      rdfs:subClassOf ddhub:DownholeEquipment. 
ddhub:CasingFlangeVerticalLocation a owl:Class; 
                                   rdfs:comment ""@EN; 
                                   rdfs:subClassOf ddhub:VerticalReferenceLocation. 
ddhub:CasingHanger a owl:Class; 
                   rdfs:comment ""@EN; 
                   rdfs:subClassOf ddhub:Hangers. 
ddhub:CasingHead a owl:Class; 
                 rdfs:comment ""@EN; 
                 rdfs:subClassOf ddhub:CasingEquipment. 
ddhub:CasingLinerEquipment a owl:Class; 
                           rdfs:comment ""@EN; 
                           rdfs:subClassOf ddhub:CasingEquipment. 
ddhub:CasingMillingTools a owl:Class; 
                         rdfs:comment ""@EN; 
                         rdfs:subClassOf ddhub:CasingEquipment. 
ddhub:CasingShoe a owl:Class; 
                 rdfs:comment ""@EN; 
                 rdfs:subClassOf ddhub:CasingEquipment. 
ddhub:CasingString a owl:Class; 
                   rdfs:comment ""@EN; 
                   rdfs:subClassOf ddhub:Tubulars. 
ddhub:CasingStringDescription a owl:Class; 
                              rdfs:comment """A casing string is a drill-stem that is used to complete a section. It is composed of casing joints and a shoe track.
"""@EN; 
                              rdfs:subClassOf ddhub:DrillStemDescription. 
ddhub:CasingTongs a owl:Class; 
                  rdfs:comment ""@EN; 
                  rdfs:subClassOf ddhub:DrillPipeTongs. 
ddhub:Casingwhiledrilling a owl:Class; 
                          rdfs:comment ""@EN; 
                          rdfs:subClassOf ddhub:DrillingEquipment. 
ddhub:CavingsComponent a owl:Class; 
                       rdfs:comment ""@EN; 
                       rdfs:subClassOf ddhub:FormationSolidComponent. 
ddhub:Celsius a owl:Class; 
              rdfs:comment """[v] = a * [SI] + b
where
[v] is the value in celsius
[SI] is the value in SI
a = Unit, i.e., 1
b = -ZeroCelsius, i.e., -273.15
and
Unit = 1.0
ZeroCelsius = 273.15 reference: https://www.nist.gov/pml/owm/si-units-temperature
"""@EN; 
              rdfs:subClassOf ddhub:Unit. 
ddhub:CelsiusPer100Foot a owl:Class; 
                        rdfs:comment """[v] = a * [SI]
where
[v] is the value in celsius per 100 foot
[SI] is the value in SI
a = 100.0*Foot/Unit, i.e., 30.479999999999997
and
Foot = 12.0 * Inch
Unit = 1.0
Inch = 0.0254 reference: https://www.nist.gov/pml/owm/si-units-length
"""@EN; 
                        rdfs:subClassOf ddhub:Unit. 
ddhub:CelsiusPer100Metre a owl:Class; 
                         rdfs:comment """[v] = a * [SI]
where
[v] is the value in celsius per 100 metre
[SI] is the value in SI
a = Hecto/Unit, i.e., 100
and
Hecto = 100.0
Unit = 1.0
"""@EN; 
                         rdfs:subClassOf ddhub:Unit. 
ddhub:CelsiusPer10Metre a owl:Class; 
                        rdfs:comment """[v] = a * [SI]
where
[v] is the value in celsius per 10 metre
[SI] is the value in SI
a = Deca/Unit, i.e., 10
and
Deca = 10.0
Unit = 1.0
"""@EN; 
                        rdfs:subClassOf ddhub:Unit. 
ddhub:CelsiusPer30Foot a owl:Class; 
                       rdfs:comment """[v] = a * [SI]
where
[v] is the value in celsius per 30 foot
[SI] is the value in SI
a = 30.0*Foot/Unit, i.e., 9.143999999999998
and
Foot = 12.0 * Inch
Unit = 1.0
Inch = 0.0254 reference: https://www.nist.gov/pml/owm/si-units-length
"""@EN; 
                       rdfs:subClassOf ddhub:Unit. 
ddhub:CelsiusPer30Metre a owl:Class; 
                        rdfs:comment """[v] = a * [SI]
where
[v] is the value in celsius per 30 metre
[SI] is the value in SI
a = 3.0*Deca/Unit, i.e., 30
and
Deca = 10.0
Unit = 1.0
"""@EN; 
                        rdfs:subClassOf ddhub:Unit. 
ddhub:CelsiusPerFoot a owl:Class; 
                     rdfs:comment """[v] = a * [SI]
where
[v] is the value in celsius per foot
[SI] is the value in SI
a = Foot/Unit, i.e., 0.30479999999999996
and
Foot = 12.0 * Inch
Unit = 1.0
Inch = 0.0254 reference: https://www.nist.gov/pml/owm/si-units-length
"""@EN; 
                     rdfs:subClassOf ddhub:Unit. 
ddhub:CelsiusPerMetre a owl:Class; 
                      rdfs:comment """[v] = a * [SI]
where
[v] is the value in celsius per metre
[SI] is the value in SI
a = 1.0/Unit, i.e., 1
and
Unit = 1.0
"""@EN; 
                      rdfs:subClassOf ddhub:Unit. 
ddhub:CementBondLoggingTools a owl:Class; 
                             rdfs:comment ""@EN; 
                             rdfs:subClassOf ddhub:WirelineLoggingTools. 
ddhub:CementFluidDescription a owl:Class; 
                             rdfs:comment """Cement fluid contains information about the density, rheological behavior and chemical characteristics of fluids
used during a cementing operation, e.g., cement slurry but also spacer.
"""@EN; 
                             rdfs:subClassOf ddhub:FluidDescription. 
ddhub:CementHead a owl:Class; 
                 rdfs:comment ""@EN; 
                 rdfs:subClassOf ddhub:CementingEquipment. 
ddhub:CementingEquipment a owl:Class; 
                         rdfs:comment ""@EN; 
                         rdfs:subClassOf ddhub:RigEquipment. 
ddhub:CementingFeature a owl:Class; 
                       rdfs:comment """A cementing feature indicates that something accounts for displacing a train of drilling fluids and cement slurries to perform
a cement operation.
"""@EN; 
                       rdfs:subClassOf ddhub:DrillingFluidDisplacementFeature. 
ddhub:CementingProcedure a owl:Class; 
                         rdfs:comment """The cementing procedure is used to displace the correct amount of cement at the right position while cleaning the borehole
to ensure good conditions for the cement setting.
"""@EN; 
                         rdfs:subClassOf ddhub:DrillingProcedure. 
ddhub:CementingServiceCompany a owl:Class; 
                              rdfs:comment ""@EN; 
                              rdfs:subClassOf ddhub:ServiceCompany. 
ddhub:CementLines a owl:Class; 
                  rdfs:comment ""@EN; 
                  rdfs:subClassOf ddhub:CementingEquipment. 
ddhub:CementManifold a owl:Class; 
                     rdfs:comment ""@EN; 
                     rdfs:subClassOf ddhub:CementingEquipment. 
ddhub:CementPump a owl:Class; 
                 rdfs:comment ""@EN; 
                 rdfs:subClassOf ddhub:CementingEquipment. 
ddhub:CementSlurry a owl:Class; 
                   rdfs:comment ""@EN; 
                   rdfs:subClassOf ddhub:CementingEquipment. 
ddhub:CementSpacer a owl:Class; 
                   rdfs:comment ""@EN; 
                   rdfs:subClassOf ddhub:CementingEquipment. 
ddhub:CementStand a owl:Class; 
                  rdfs:comment ""@EN; 
                  rdfs:subClassOf ddhub:CementingEquipment. 
ddhub:CementStinger a owl:Class; 
                    rdfs:comment ""@EN; 
                    rdfs:subClassOf ddhub:CementingEquipment. 
ddhub:CementUnit a owl:Class; 
                 rdfs:comment ""@EN; 
                 rdfs:subClassOf ddhub:CementingEquipment. 
ddhub:Centiampere a owl:Class; 
                  rdfs:comment """[v] = a * [SI]
where
[v] is the value in centiampere
[SI] is the value in SI
a = 1.0/Centi, i.e., 100
and
Centi = 0.01
"""@EN; 
                  rdfs:subClassOf ddhub:Unit. 
ddhub:Centigram a owl:Class; 
                rdfs:comment """[v] = a * [SI]
where
[v] is the value in centigram
[SI] is the value in SI
a = 1.0/(0.1*Milli), i.e., 10000
and
Milli = 0.001
"""@EN; 
                rdfs:subClassOf ddhub:Unit. 
ddhub:Centilitre a owl:Class; 
                 rdfs:comment """[v] = a * [SI]
where
[v] is the value in centilitre
[SI] is the value in SI
a = 1.0/(Centi*Milli), i.e., 99999.99999999999
and
Centi = 0.01
Milli = 0.001
"""@EN; 
                 rdfs:subClassOf ddhub:Unit. 
ddhub:Centimetre a owl:Class; 
                 rdfs:comment """[v] = a * [SI]
where
[v] is the value in centimetre
[SI] is the value in SI
a = 1.0/Centi, i.e., 100
and
Centi = 0.01
"""@EN; 
                 rdfs:subClassOf ddhub:Unit. 
ddhub:CentimetreMercuryAtZeroDegreeCelsius a owl:Class; 
                                           rdfs:comment """[v] = a * [SI]
where
[v] is the value in centimetre mercury at zero degree celsius
[SI] is the value in SI
a = 1.0/(Deca*MillimetreMercury), i.e., 0.0007500615758456563
and
Deca = 10.0
MillimetreMercury = 133.322387415 reference: https://en.wikipedia.org/wiki/Millimetre_of_mercury
"""@EN; 
                                           rdfs:subClassOf ddhub:Unit. 
ddhub:CentimetreMercuryAtZeroDegreeCelsiusPerHour a owl:Class; 
                                                  rdfs:comment """[v] = a * [SI]
where
[v] is the value in centimetre mercury at zero degree celsius per hour
[SI] is the value in SI
a = Hour/(Deca*MillimetreMercury), i.e., 2.700221673044363
and
Hour = 60.0 * Minute
Deca = 10.0
MillimetreMercury = 133.322387415 reference: https://en.wikipedia.org/wiki/Millimetre_of_mercury
Minute = 60.0
"""@EN; 
                                                  rdfs:subClassOf ddhub:Unit. 
ddhub:CentimetreMercuryAtZeroDegreeCelsiusPerMinute a owl:Class; 
                                                    rdfs:comment """[v] = a * [SI]
where
[v] is the value in centimetre mercury at zero degree celsius per minute
[SI] is the value in SI
a = Minute/(Deca*MillimetreMercury), i.e., 0.04500369455073938
and
Minute = 60.0
Deca = 10.0
MillimetreMercury = 133.322387415 reference: https://en.wikipedia.org/wiki/Millimetre_of_mercury
"""@EN; 
                                                    rdfs:subClassOf ddhub:Unit. 
ddhub:CentimetreMercuryAtZeroDegreeCelsiusPerSecond a owl:Class; 
                                                    rdfs:comment """[v] = a * [SI]
where
[v] is the value in centimetre mercury at zero degree celsius per second
[SI] is the value in SI
a = 1.0/(Deca*MillimetreMercury), i.e., 0.0007500615758456563
and
Deca = 10.0
MillimetreMercury = 133.322387415 reference: https://en.wikipedia.org/wiki/Millimetre_of_mercury
"""@EN; 
                                                    rdfs:subClassOf ddhub:Unit. 
ddhub:CentimetrePerDay a owl:Class; 
                       rdfs:comment """[v] = a * [SI]
where
[v] is the value in centimetre per day
[SI] is the value in SI
a = Day/Centi, i.e., 8640000
and
Day = 24.0 * Hour
Centi = 0.01
Hour = 60.0 * Minute
Minute = 60.0
"""@EN; 
                       rdfs:subClassOf ddhub:Unit. 
ddhub:CentimetrePerHour a owl:Class; 
                        rdfs:comment """[v] = a * [SI]
where
[v] is the value in centimetre per hour
[SI] is the value in SI
a = Hour/Centi, i.e., 360000
and
Hour = 60.0 * Minute
Centi = 0.01
Minute = 60.0
"""@EN; 
                        rdfs:subClassOf ddhub:Unit. 
ddhub:CentimetrePerHourPerSecond a owl:Class; 
                                 rdfs:comment """[v] = a * [SI]
where
[v] is the value in centimetre per hour per second
[SI] is the value in SI
a = Hour/Centi, i.e., 360000
and
Hour = 60.0 * Minute
Centi = 0.01
Minute = 60.0
"""@EN; 
                                 rdfs:subClassOf ddhub:Unit. 
ddhub:CentimetrePerKilometre a owl:Class; 
                             rdfs:comment """[v] = a * [SI]
where
[v] is the value in centimetre per kilometre
[SI] is the value in SI
a = Kilo / Centi, i.e., 100000
and
Kilo = 1000.0
Centi = 0.01
"""@EN; 
                             rdfs:subClassOf ddhub:Unit. 
ddhub:CentimetrePerMetre a owl:Class; 
                         rdfs:comment """[v] = a * [SI]
where
[v] is the value in centimetre per metre
[SI] is the value in SI
a = 1.0 / Centi, i.e., 100
and
Centi = 0.01
"""@EN; 
                         rdfs:subClassOf ddhub:Unit. 
ddhub:CentimetrePerMinute a owl:Class; 
                          rdfs:comment """[v] = a * [SI]
where
[v] is the value in centimetre per minute
[SI] is the value in SI
a = Minute/Centi, i.e., 6000
and
Minute = 60.0
Centi = 0.01
"""@EN; 
                          rdfs:subClassOf ddhub:Unit. 
ddhub:CentimetrePerMinutePerSecond a owl:Class; 
                                   rdfs:comment """[v] = a * [SI]
where
[v] is the value in centimetre per minute per second
[SI] is the value in SI
a = Minute/Centi, i.e., 6000
and
Minute = 60.0
Centi = 0.01
"""@EN; 
                                   rdfs:subClassOf ddhub:Unit. 
ddhub:CentimetrePerSecond a owl:Class; 
                          rdfs:comment """[v] = a * [SI]
where
[v] is the value in centimetre per second
[SI] is the value in SI
a = Unit/Centi, i.e., 100
and
Unit = 1.0
Centi = 0.01
"""@EN; 
                          rdfs:subClassOf ddhub:Unit. 
ddhub:CentimetrePerSecondSquared a owl:Class; 
                                 rdfs:comment """[v] = a * [SI]
where
[v] is the value in centimetre per second squared
[SI] is the value in SI
a = 1.0/Centi, i.e., 100
and
Centi = 0.01
"""@EN; 
                                 rdfs:subClassOf ddhub:Unit. 
ddhub:CentimetreWaterAt4DegreeCelsius a owl:Class; 
                                      rdfs:comment """[v] = a * [SI]
where
[v] is the value in centimetre water at 4 degree celsius
[SI] is the value in SI
a = 1.0/(Deca*MillimetreWater4degC), i.e., 0.010104429276573386
and
Deca = 10.0
MillimetreWater4degC = 9.89665 reference: https://en.wikipedia.org/wiki/Centimetre_or_millimetre_of_water
"""@EN; 
                                      rdfs:subClassOf ddhub:Unit. 
ddhub:CentimetreWaterAt4DegreeCelsiusPerHour a owl:Class; 
                                             rdfs:comment """[v] = a * [SI]
where
[v] is the value in centimetre water at 4 degree celsius per hour
[SI] is the value in SI
a = Hour/(Deca*MillimetreWater4degC), i.e., 36.37594539566419
and
Hour = 60.0 * Minute
Deca = 10.0
MillimetreWater4degC = 9.89665 reference: https://en.wikipedia.org/wiki/Centimetre_or_millimetre_of_water
Minute = 60.0
"""@EN; 
                                             rdfs:subClassOf ddhub:Unit. 
ddhub:CentimetreWaterAt4DegreeCelsiusPerMinute a owl:Class; 
                                               rdfs:comment """[v] = a * [SI]
where
[v] is the value in centimetre water at 4 degree celsius per minute
[SI] is the value in SI
a = Minute/(Deca*MillimetreWater4degC), i.e., 0.6062657565944032
and
Minute = 60.0
Deca = 10.0
MillimetreWater4degC = 9.89665 reference: https://en.wikipedia.org/wiki/Centimetre_or_millimetre_of_water
"""@EN; 
                                               rdfs:subClassOf ddhub:Unit. 
ddhub:CentimetreWaterAt4DegreeCelsiusPerSecond a owl:Class; 
                                               rdfs:comment """[v] = a * [SI]
where
[v] is the value in centimetre water at 4 degree celsius per second
[SI] is the value in SI
a = 1.0/(Deca*MillimetreWater4degC), i.e., 0.010104429276573386
and
Deca = 10.0
MillimetreWater4degC = 9.89665 reference: https://en.wikipedia.org/wiki/Centimetre_or_millimetre_of_water
"""@EN; 
                                               rdfs:subClassOf ddhub:Unit. 
ddhub:Centimole a owl:Class; 
                rdfs:comment """[v] = a * [SI]
where
[v] is the value in centimole
[SI] is the value in SI
a = 1.0/Centi, i.e., 100
and
Centi = 0.01
"""@EN; 
                rdfs:subClassOf ddhub:Unit. 
ddhub:Centipoise a owl:Class; 
                 rdfs:comment """[v] = a * [SI]
where
[v] is the value in centipoise
[SI] is the value in SI
a = 1.0/(Centi * Poise), i.e., 1000
and
Centi = 0.01
Poise = 0.1 reference: https://en.wikipedia.org/wiki/Poise_(unit)
"""@EN; 
                 rdfs:subClassOf ddhub:Unit. 
ddhub:Centivolt a owl:Class; 
                rdfs:comment """[v] = a * [SI]
where
[v] is the value in centivolt
[SI] is the value in SI
a = 1.0/Centi, i.e., 100
and
Centi = 0.01
"""@EN; 
                rdfs:subClassOf ddhub:Unit. 
ddhub:Centiwatt a owl:Class; 
                rdfs:comment """[v] = a * [SI]
where
[v] is the value in centiwatt
[SI] is the value in SI
a = 1.0/Centi, i.e., 100
and
Centi = 0.01
"""@EN; 
                rdfs:subClassOf ddhub:Unit. 
ddhub:Centralizers a owl:Class; 
                   rdfs:comment ""@EN; 
                   rdfs:subClassOf ddhub:CasingString. 
ddhub:CentrifugalDegasser a owl:Class; 
                          rdfs:comment ""@EN; 
                          rdfs:subClassOf ddhub:Degasser. 
ddhub:CentrifugalMudPump a owl:Class; 
                         rdfs:comment ""@EN; 
                         rdfs:subClassOf ddhub:MudPump. 
ddhub:Centrifuge a owl:Class; 
                 rdfs:comment ""@EN; 
                 rdfs:subClassOf ddhub:CirculationSystem. 
ddhub:Century a owl:Class; 
              rdfs:comment """[v] = a * [SI]
where
[v] is the value in century
[SI] is the value in SI
a = 1.0/Century, i.e., 3.168808781402895E-10
and
Century = 10.0 * Decade
Decade = 10.0 * YearJulian
YearJulian = 365.25 * Day
Day = 24.0 * Hour
Hour = 60.0 * Minute
Minute = 60.0
"""@EN; 
              rdfs:subClassOf ddhub:Unit. 
ddhub:ChaoticWhirl a owl:Class; 
                   rdfs:comment """This Noun is used to refer to chaotic whirl.
"""@EN; 
                   rdfs:subClassOf ddhub:Whirling. 
ddhub:ChemicalTank a owl:Class; 
                   rdfs:comment ""@EN; 
                   rdfs:subClassOf ddhub:MudPits. 
ddhub:ChokeLine a owl:Class; 
                rdfs:comment ""@EN; 
                rdfs:subClassOf ddhub:WellControlSystem. 
ddhub:ChokeManifold a owl:Class; 
                    rdfs:comment ""@EN; 
                    rdfs:subClassOf ddhub:WellControlSystem. 
ddhub:ChokeValve a owl:Class; 
                 rdfs:comment ""@EN; 
                 rdfs:subClassOf ddhub:ChokeManifold. 
ddhub:ChokeValveGatevalve a owl:Class; 
                          rdfs:comment ""@EN; 
                          rdfs:subClassOf ddhub:ChokeValve. 
ddhub:Circle a owl:Class; 
             rdfs:comment """[v] = a * [SI]
where
[v] is the value in circle
[SI] is the value in SI
a = 1.0/(2.0*PI), i.e., 0.15915494309189535
"""@EN; 
             rdfs:subClassOf ddhub:Unit. 
ddhub:CirculationControlSystem a owl:Class; 
                               rdfs:comment ""@EN; 
                               rdfs:subClassOf ddhub:ControlSystem. 
ddhub:CirculationFeature a owl:Class; 
                         rdfs:comment """A circulation feature indicates that something accounts for circulation.
"""@EN; 
                         rdfs:subClassOf ddhub:DrillingManagementFeature. 
ddhub:CirculationStartupProcedure a owl:Class; 
                                  rdfs:comment """The circulation stop procedure defines how to stop the mud pumps in a way that limit potential bull-heading effects
that could result in undesired downhole pressure conditions with regards to the geo-pressure window.
"""@EN; 
                                  rdfs:subClassOf ddhub:DrillingProcedure. 
ddhub:CirculationStopProcedure a owl:Class; 
                               rdfs:comment """The rotation startup procedure controls the steps to start the rotation of the drill-stem to reach a target rotational
speed while attempting to avoid having too large torsional oscillations.
"""@EN; 
                               rdfs:subClassOf ddhub:DrillingProcedure. 
ddhub:CirculationSub a owl:Class; 
                     rdfs:comment ""@EN; 
                     rdfs:subClassOf ddhub:DrillingEquipment. 
ddhub:CirculationSystem a owl:Class; 
                        rdfs:comment ""@EN; 
                        rdfs:subClassOf ddhub:RigEquipment. 
ddhub:Clampon a owl:Class; 
              rdfs:comment ""@EN; 
              rdfs:subClassOf ddhub:BladeType. 
ddhub:Clock a owl:Class; 
            rdfs:comment """Represents a clock
"""@EN; 
            rdfs:subClassOf ddhub:DWISNoun. 
ddhub:ClusterPositionLocation a owl:Class; 
                              rdfs:comment ""@EN; 
                              rdfs:subClassOf ddhub:PositionReferenceLocation. 
ddhub:CoiledTubingEquipment a owl:Class; 
                            rdfs:comment ""@EN; 
                            rdfs:subClassOf ddhub:Equipment. 
ddhub:CoiledTubingReel a owl:Class; 
                       rdfs:comment ""@EN; 
                       rdfs:subClassOf ddhub:CoiledTubingEquipment. 
ddhub:CollapsePressure a owl:Class; 
                       rdfs:comment ""@EN; 
                       rdfs:subClassOf ddhub:PrototypeData. 
ddhub:CollapsePressureGradient a owl:Class; 
                               rdfs:comment ""@EN; 
                               rdfs:subClassOf ddhub:PrototypeData. 
ddhub:Command a owl:Class; 
              rdfs:comment ""@EN; 
              rdfs:subClassOf ddhub:ProcessData. 
ddhub:CompletionFluidDescription a owl:Class; 
                                 rdfs:comment """Completion fluid contains information about the density, rheological behavior and chemical characteristics of a
fluid used during a completion operation.
"""@EN; 
                                 rdfs:subClassOf ddhub:FluidDescription. 
ddhub:CompletionServiceCompany a owl:Class; 
                               rdfs:comment ""@EN; 
                               rdfs:subClassOf ddhub:ServiceCompany. 
ddhub:CompletionWorkoverRiser a owl:Class; 
                              rdfs:comment ""@EN; 
                              rdfs:subClassOf ddhub:MarineSystem. 
ddhub:CompressibilityDrillingQuantity a owl:Class; 
                                      rdfs:comment """Compressibility is the measure of how much a substance's volume decreases under pressure. It indicates how easily a material or fluid can be compressed and is typically expressed as a change in volume per unit change in pressure.
The dimension of compressibility is:
$$[T^{2}LM^{-1}]$$.
The SI unit for **compressibility** is: inverse pascal with the associated unit label $\\frac{1}{Pa}$
The meaningful precision of compressibility in the drilling context is typically: 1E-13 1/Pa
"""@EN; 
                                      rdfs:subClassOf ddhub:MeasurableQuantity. 
ddhub:CompressibilityQuantity a owl:Class; 
                              rdfs:comment """Compressibility is the measure of how much a substance's volume decreases under pressure. It indicates how easily a material or fluid can be compressed and is typically expressed as a change in volume per unit change in pressure.
The dimension of compressibility is:
$$[T^{2}LM^{-1}]$$.
The SI unit for **compressibility** is: inverse pascal with the associated unit label $\\frac{1}{Pa}$
"""@EN; 
                              rdfs:subClassOf ddhub:Quantity. 
ddhub:CompressiveDrillPipe a owl:Class; 
                           rdfs:comment ""@EN; 
                           rdfs:subClassOf ddhub:DrillString. 
ddhub:ComputationUnit a owl:Class; 
                      rdfs:comment """Denotes a complex computation unit, typically based on advanced numerical modeling
"""@EN; 
                      rdfs:subClassOf ddhub:DataFlowNode. 
ddhub:ComputedData a owl:Class; 
                   rdfs:comment ""@EN; 
                   rdfs:subClassOf ddhub:PhysicalData. 
ddhub:ComputedState a owl:Class; 
                    rdfs:comment """A state represents the current configuation of a system.
"""@EN; 
                    rdfs:subClassOf ddhub:ComputationUnit. 
ddhub:ConcernsAFluidComponent a owl:ObjectProperty; 
                              rdfs:comment ""@EN; 
                              rdfs:domain ddhub:DrillingDataPoint; 
                              rdfs:range ddhub:FluidComponent; 
                              rdfs:subPropertyOf ddhub:DWISVerb. 
ddhub:ConductorDrivePipe a owl:Class; 
                         rdfs:comment ""@EN; 
                         rdfs:subClassOf ddhub:CasingString. 
ddhub:ConductorTensioners a owl:Class; 
                          rdfs:comment ""@EN; 
                          rdfs:subClassOf ddhub:MarineSystem. 
ddhub:ConfigurationData a owl:Class; 
                        rdfs:comment """Configuration data is used to configure a computation unit.
"""@EN; 
                        rdfs:subClassOf ddhub:ContextualData. 
ddhub:ConnectedCondition a owl:Class; 
                         rdfs:comment ""@EN; 
                         rdfs:subClassOf ddhub:ValidityCondition. 
ddhub:Connection a owl:Class; 
                 rdfs:comment ""@EN; 
                 rdfs:subClassOf ddhub:CasingString. 
ddhub:ConnectionWelded a owl:Class; 
                       rdfs:comment ""@EN; 
                       rdfs:subClassOf ddhub:Connection. 
ddhub:ConsistencyIndexRheologyQuantity a owl:Class; 
                                       rdfs:comment """Dynamic viscosity is a measure of a fluid's resistance to shear or flow when a force is applied. It quantifies how thick or thin the fluid is.
The dimension of dynamic viscosity is:
$$[ML^{-1}T^{-1}]$$.
The SI unit for **dynamic viscosity** is: pascal second with the associated unit label $Pa \\cdot s$
The consistency index in rheology measures a fluid's resistance to flow; it quantifies the fluid's viscosity and how it changes with shear rate.
The meaningful precision of a consistency index in rheology is typically: 0.0001 Pa•s
"""@EN; 
                                       rdfs:subClassOf ddhub:MeasurableQuantity. 
ddhub:Context a owl:Class; 
              rdfs:comment """A context is at the fourth level of a rig action plan.
"""@EN; 
              rdfs:subClassOf ddhub:OperationalStep. 
ddhub:ContextualData a owl:Class; 
                     rdfs:comment """Contextual data are structured objects stored in a JSon string.
"""@EN; 
                     rdfs:subClassOf ddhub:JSonDataType. 
ddhub:ContinuousDataType a owl:Class; 
                         rdfs:comment ""@EN; 
                         rdfs:subClassOf ddhub:DataType. 
ddhub:ContinuousProportional a owl:Class; 
                             rdfs:comment ""@EN; 
                             rdfs:subClassOf ddhub:RotarySteerableSystems. 
ddhub:ControlAndMonitoringEquipment a owl:Class; 
                                    rdfs:comment ""@EN; 
                                    rdfs:subClassOf ddhub:ControlConsole. 
ddhub:ControlConsole a owl:Class; 
                     rdfs:comment ""@EN; 
                     rdfs:subClassOf ddhub:CoiledTubingEquipment. 
ddhub:Controller a owl:Class; 
                 rdfs:comment ""@EN; 
                 rdfs:subClassOf ddhub:DataFlowNode. 
ddhub:ControllerFunction a owl:Class; 
                         rdfs:comment """A `ControllerFunction` is a `RunnableFunction` that executes a feedback control loop to follow as closely
as possible one or several desired values. A typical example of `ControllerFunction` is the `AutoDriller`. An `AutoDriller` 
follows as closely as possible, for instance, a desired `WOB`.
"""@EN; 
                         rdfs:subClassOf ddhub:RunnableFunction. 
ddhub:ControlLines a owl:Class; 
                   rdfs:comment ""@EN; 
                   rdfs:subClassOf ddhub:WellControlSystem. 
ddhub:ControlManifold a owl:Class; 
                      rdfs:comment ""@EN; 
                      rdfs:subClassOf ddhub:WellControlSystem. 
ddhub:ControlModel a owl:Class; 
                   rdfs:comment """A model that regulate or steer a system's behavior toward a desired outcome through inputs.
"""@EN; 
                   rdfs:subClassOf ddhub:ModelingObjective. 
ddhub:Controls a owl:ObjectProperty; 
               rdfs:comment ""@EN; 
               rdfs:domain ddhub:DWISNoun; 
               rdfs:range ddhub:DWISNoun; 
               rdfs:subPropertyOf ddhub:DWISVerb. 
ddhub:ControlSystem a owl:Class; 
                    rdfs:comment ""@EN; 
                    rdfs:subClassOf ddhub:DataFlowNode. 
ddhub:ConventionalDerrick a owl:Class; 
                          rdfs:comment ""@EN; 
                          rdfs:subClassOf ddhub:Derrick. 
ddhub:ConversionFactorA a owl:DatatypeProperty, owl:FunctionalProperty; 
                        rdfs:comment """Unit conversion from SI unit is performed as:
ConvertedValue = ConversionFactorA + SIValue * ConversionFactorB
"""@EN; 
                        rdfs:domain ddhub:Unit; 
                        rdfs:range xsd:double. 
ddhub:ConversionFactorB a owl:DatatypeProperty, owl:FunctionalProperty; 
                        rdfs:comment """Unit conversion from SI unit is performed as:
ConvertedValue = ConversionFactorA + SIValue * ConversionFactorB
"""@EN; 
                        rdfs:domain ddhub:Unit; 
                        rdfs:range xsd:double. 
ddhub:CoringTool a owl:Class; 
                 rdfs:comment ""@EN; 
                 rdfs:subClassOf ddhub:DrillingEquipment. 
ddhub:CorrectedMeasurement a owl:Class; 
                           rdfs:comment ""@EN; 
                           rdfs:subClassOf ddhub:Measurement. 
ddhub:CoulombPerSecond a owl:Class; 
                       rdfs:comment """[v] = a * [SI]
where
[v] is the value in coulomb per second
[SI] is the value in SI
a = 1.0/Unit, i.e., 1
and
Unit = 1.0
"""@EN; 
                       rdfs:subClassOf ddhub:Unit. 
ddhub:CoulombPerVolt a owl:Class; 
                     rdfs:comment """[v] = a * [SI]
where
[v] is the value in coulomb per volt
[SI] is the value in SI
a = 1.0/Unit, i.e., 1
and
Unit = 1.0
"""@EN; 
                     rdfs:subClassOf ddhub:Unit. 
ddhub:Crossover a owl:Class; 
                rdfs:comment ""@EN; 
                rdfs:subClassOf ddhub:CasingString. 
ddhub:CrownBlock a owl:Class; 
                 rdfs:comment ""@EN; 
                 rdfs:subClassOf ddhub:MechanicalBlock. 
ddhub:CrownValveVerticalLocation a owl:Class; 
                                 rdfs:comment ""@EN; 
                                 rdfs:subClassOf ddhub:VerticalReferenceLocation. 
ddhub:CtBhaComponents a owl:Class; 
                      rdfs:comment ""@EN; 
                      rdfs:subClassOf ddhub:CoiledTubingEquipment. 
ddhub:CubicFoot a owl:Class; 
                rdfs:comment """[v] = a * [SI]
where
[v] is the value in cubic foot
[SI] is the value in SI
a = 1.0/(Foot*Foot*Foot), i.e., 35.3146667214886
and
Foot = 12.0 * Inch
Inch = 0.0254 reference: https://www.nist.gov/pml/owm/si-units-length
"""@EN; 
                rdfs:subClassOf ddhub:Unit. 
ddhub:CubicFootPerDay a owl:Class; 
                      rdfs:comment """[v] = a * [SI]
where
[v] is the value in cubic foot per day
[SI] is the value in SI
a = Day / (Foot*Foot*Foot), i.e., 3051187.204736615
and
Day = 24.0 * Hour
Foot = 12.0 * Inch
Hour = 60.0 * Minute
Inch = 0.0254 reference: https://www.nist.gov/pml/owm/si-units-length
Minute = 60.0
"""@EN; 
                      rdfs:subClassOf ddhub:Unit. 
ddhub:CubicFootPerHour a owl:Class; 
                       rdfs:comment """[v] = a * [SI]
where
[v] is the value in cubic foot per hour
[SI] is the value in SI
a = Hour / (Foot*Foot*Foot), i.e., 127132.80019735897
and
Hour = 60.0 * Minute
Foot = 12.0 * Inch
Minute = 60.0
Inch = 0.0254 reference: https://www.nist.gov/pml/owm/si-units-length
"""@EN; 
                       rdfs:subClassOf ddhub:Unit. 
ddhub:CubicFootPerMinute a owl:Class; 
                         rdfs:comment """[v] = a * [SI]
where
[v] is the value in cubic foot per minute
[SI] is the value in SI
a = Minute / (Foot*Foot*Foot), i.e., 2118.880003289316
and
Minute = 60.0
Foot = 12.0 * Inch
Inch = 0.0254 reference: https://www.nist.gov/pml/owm/si-units-length
"""@EN; 
                         rdfs:subClassOf ddhub:Unit. 
ddhub:CubicFootPerSecond a owl:Class; 
                         rdfs:comment """[v] = a * [SI]
where
[v] is the value in cubic foot per second
[SI] is the value in SI
a = 1.0/(Foot*Foot*Foot), i.e., 35.3146667214886
and
Foot = 12.0 * Inch
Inch = 0.0254 reference: https://www.nist.gov/pml/owm/si-units-length
"""@EN; 
                         rdfs:subClassOf ddhub:Unit. 
ddhub:CubicFootPerYear a owl:Class; 
                       rdfs:comment """[v] = a * [SI]
where
[v] is the value in cubic foot per year
[SI] is the value in SI
a = YearJulian / (Foot*Foot*Foot), i.e., 1114446126.5300486
and
YearJulian = 365.25 * Day
Foot = 12.0 * Inch
Day = 24.0 * Hour
Inch = 0.0254 reference: https://www.nist.gov/pml/owm/si-units-length
Hour = 60.0 * Minute
Minute = 60.0
"""@EN; 
                       rdfs:subClassOf ddhub:Unit. 
ddhub:CubicInch a owl:Class; 
                rdfs:comment """[v] = a * [SI]
where
[v] is the value in cubic inch
[SI] is the value in SI
a = 1.0/(Inch*Inch*Inch), i.e., 61023.74409473229
and
Inch = 0.0254 reference: https://www.nist.gov/pml/owm/si-units-length
"""@EN; 
                rdfs:subClassOf ddhub:Unit. 
ddhub:CubicMetre a owl:Class; 
                 rdfs:comment """No conversion necessary as the unit choice is SI
"""@EN; 
                 rdfs:subClassOf ddhub:Unit. 
ddhub:CubicMetrePerDay a owl:Class; 
                       rdfs:comment """[v] = a * [SI]
where
[v] is the value in cubic metre per day
[SI] is the value in SI
a = Day / Unit, i.e., 86400
and
Day = 24.0 * Hour
Unit = 1.0
Hour = 60.0 * Minute
Minute = 60.0
"""@EN; 
                       rdfs:subClassOf ddhub:Unit. 
ddhub:CubicMetrePerHour a owl:Class; 
                        rdfs:comment """[v] = a * [SI]
where
[v] is the value in cubic metre per hour
[SI] is the value in SI
a = Hour/ Unit, i.e., 3600
and
Hour = 60.0 * Minute
Unit = 1.0
Minute = 60.0
"""@EN; 
                        rdfs:subClassOf ddhub:Unit. 
ddhub:CubicMetrePerMinute a owl:Class; 
                          rdfs:comment """[v] = a * [SI]
where
[v] is the value in cubic metre per minute
[SI] is the value in SI
a = Minute / Unit, i.e., 60
and
Minute = 60.0
Unit = 1.0
"""@EN; 
                          rdfs:subClassOf ddhub:Unit. 
ddhub:CubicMetrePerSecond a owl:Class; 
                          rdfs:comment """No conversion necessary as the unit choice is SI
"""@EN; 
                          rdfs:subClassOf ddhub:Unit. 
ddhub:CubicMetrePerSecondSquared a owl:Class; 
                                 rdfs:comment """No conversion necessary as the unit choice is SI
"""@EN; 
                                 rdfs:subClassOf ddhub:Unit. 
ddhub:CubicMetrePerYear a owl:Class; 
                        rdfs:comment """[v] = a * [SI]
where
[v] is the value in cubic metre per year
[SI] is the value in SI
a = YearJulian/Unit, i.e., 31557600
and
YearJulian = 365.25 * Day
Unit = 1.0
Day = 24.0 * Hour
Hour = 60.0 * Minute
Minute = 60.0
"""@EN; 
                        rdfs:subClassOf ddhub:Unit. 
ddhub:Current a owl:Class; 
              rdfs:comment """Current characterizes that the wellbore data is the currently selected one as the official one.
"""@EN; 
              rdfs:subClassOf ddhub:WellBoreDataCharateristic. 
ddhub:CurvatureDrillingQuantity a owl:Class; 
                                rdfs:comment """A curvature is the second derivative of a position compared to the curvilinear abscissa: $\\frac{d^2x}{ds^2}$, where $x$ is the position and $s$ is the curvilinear abscissa.
The dimension of curvature is:
$$[{\\theta}L^{-1}]$$.
The SI unit for **curvature** is: radian per metre with the associated unit label $\\frac{rad}{m}$
The meaningful precision of curvature in the drilling context is typically: 5.817764173314432E-06 rad/m
"""@EN; 
                                rdfs:subClassOf ddhub:MeasurableQuantity. 
ddhub:CurvatureQuantity a owl:Class; 
                        rdfs:comment """A curvature is the second derivative of a position compared to the curvilinear abscissa: $\\frac{d^2x}{ds^2}$, where $x$ is the position and $s$ is the curvilinear abscissa.
The dimension of curvature is:
$$[{\\theta}L^{-1}]$$.
The SI unit for **curvature** is: radian per metre with the associated unit label $\\frac{rad}{m}$
"""@EN; 
                        rdfs:subClassOf ddhub:Quantity. 
ddhub:CutOffFrequency a owl:DatatypeProperty, owl:FunctionalProperty; 
                      rdfs:comment """
"""@EN; 
                      rdfs:domain ddhub:HighPassFilter, ddhub:LowPassFilter; 
                      rdfs:range xsd:double. 
ddhub:CuttingsAnalysisEquipmnet a owl:Class; 
                                rdfs:comment ""@EN; 
                                rdfs:subClassOf ddhub:MudLoggingEquipment. 
ddhub:CuttingsBedLocation a owl:Class; 
                          rdfs:comment ""@EN; 
                          rdfs:subClassOf ddhub:AbscissaReferenceLocation. 
ddhub:CuttingsComponent a owl:Class; 
                        rdfs:comment ""@EN; 
                        rdfs:subClassOf ddhub:FormationSolidComponent. 
ddhub:CuttingsSamplingEquipment a owl:Class; 
                                rdfs:comment ""@EN; 
                                rdfs:subClassOf ddhub:MudLoggingEquipment. 
ddhub:CuttingsTransportFeature a owl:Class; 
                               rdfs:comment """A cuttings transport feature indicates that something accounts for cuttings transport while circulating.
"""@EN; 
                               rdfs:subClassOf ddhub:CirculationFeature. 
ddhub:Cylinders a owl:Class; 
                rdfs:comment ""@EN; 
                rdfs:subClassOf ddhub:PistonMudPump. 
ddhub:CylindricalReferenceFrame a owl:Class; 
                                rdfs:comment ""@EN; 
                                rdfs:subClassOf ddhub:ThreeDimensionalReferenceFrame. 
ddhub:Darcy a owl:Class; 
            rdfs:comment """[v] = a * [SI]
where
[v] is the value in darcy
[SI] is the value in SI
a = 1.0/Darcy, i.e., 1013250000000
and
Darcy = 0.0000001 / Atmosphere reference: https://en.wikipedia.org/wiki/Darcy_(unit)
Atmosphere = 101325.0 reference: https://en.wikipedia.org/wiki/Atmospheric_pressure
"""@EN; 
            rdfs:subClassOf ddhub:Unit. 
ddhub:DataAnalysisServiceCompany a owl:Class; 
                                 rdfs:comment """A data analysis service company is an entity that analyses measured data and provide new information from these measurements.
"""@EN; 
                                 rdfs:subClassOf ddhub:ServiceCompany. 
ddhub:DataEndPoint a owl:Class; 
                   rdfs:comment ""@EN; 
                   rdfs:subClassOf ddhub:DWISNoun. 
ddhub:DataFlowNode a owl:Class; 
                   rdfs:comment """A data flow node is a generic term for any node in the data flow graph.
"""@EN; 
                   rdfs:subClassOf ddhub:DWISNoun. 
ddhub:DataIntegrationStrategy a owl:Class; 
                              rdfs:comment """A classification of a model with regards to its strategy for integrating data.
"""@EN; 
                              rdfs:subClassOf ddhub:DWISNoun. 
ddhub:DataLevelIntegationModel a owl:Class; 
                               rdfs:comment """A model that integrates data at a low-level like direct merging, using data transforms or filtering.
"""@EN; 
                               rdfs:subClassOf ddhub:DataIntegrationStrategy. 
ddhub:DataProvider a owl:Class; 
                   rdfs:comment """A data provider is any sources for data.
"""@EN; 
                   rdfs:subClassOf ddhub:DWISNoun. 
ddhub:DataType a owl:Class; 
               rdfs:comment ""@EN; 
               rdfs:subClassOf ddhub:DWISNoun. 
ddhub:Day a owl:Class; 
          rdfs:comment """[v] = a * [SI]
where
[v] is the value in day
[SI] is the value in SI
a = 1.0/Day, i.e., 1.1574074074074073E-05
and
Day = 24.0 * Hour
Hour = 60.0 * Minute
Minute = 60.0
"""@EN; 
          rdfs:subClassOf ddhub:Unit. 
ddhub:DeadLine a owl:Class; 
               rdfs:comment ""@EN; 
               rdfs:subClassOf ddhub:DrillLine. 
ddhub:DeadLineAnchor a owl:Class; 
                     rdfs:comment ""@EN; 
                     rdfs:subClassOf ddhub:DrillLineFastener. 
ddhub:Decade a owl:Class; 
             rdfs:comment """[v] = a * [SI]
where
[v] is the value in decade
[SI] is the value in SI
a = 1.0/Decade, i.e., 3.168808781402895E-09
and
Decade = 10.0 * YearJulian
YearJulian = 365.25 * Day
Day = 24.0 * Hour
Hour = 60.0 * Minute
Minute = 60.0
"""@EN; 
             rdfs:subClassOf ddhub:Unit. 
ddhub:Decagram a owl:Class; 
               rdfs:comment """[v] = a * [SI]
where
[v] is the value in decagram
[SI] is the value in SI
a = 1.0/Centi, i.e., 100
and
Centi = 0.01
"""@EN; 
               rdfs:subClassOf ddhub:Unit. 
ddhub:Decametre a owl:Class; 
                rdfs:comment """[v] = a * [SI]
where
[v] is the value in decametre
[SI] is the value in SI
a = 1.0/Deca, i.e., 0.1
and
Deca = 10.0
"""@EN; 
                rdfs:subClassOf ddhub:Unit. 
ddhub:Decanewton a owl:Class; 
                 rdfs:comment """[v] = a * [SI]
where
[v] is the value in decanewton
[SI] is the value in SI
a = 1.0/(Deca), i.e., 0.1
and
Deca = 10.0
"""@EN; 
                 rdfs:subClassOf ddhub:Unit. 
ddhub:DecanewtonMetre a owl:Class; 
                      rdfs:comment """[v] = a * [SI]
where
[v] is the value in decanewton metre
[SI] is the value in SI
a = 1.0/(Deca), i.e., 0.1
and
Deca = 10.0
"""@EN; 
                      rdfs:subClassOf ddhub:Unit. 
ddhub:DecanewtonMetrePerCentimetre a owl:Class; 
                                   rdfs:comment """[v] = a * [SI]
where
[v] is the value in decanewton metre per centimetre
[SI] is the value in SI
a = Centi/(Deca), i.e., 0.001
and
Centi = 0.01
Deca = 10.0
"""@EN; 
                                   rdfs:subClassOf ddhub:Unit. 
ddhub:DecanewtonMetrePerDecimetre a owl:Class; 
                                  rdfs:comment """[v] = a * [SI]
where
[v] is the value in decanewton metre per decimetre
[SI] is the value in SI
a = Deci/Deca, i.e., 0.01
and
Deci = 0.1
Deca = 10.0
"""@EN; 
                                  rdfs:subClassOf ddhub:Unit. 
ddhub:DecanewtonMetrePerFoot a owl:Class; 
                             rdfs:comment """[v] = a * [SI]
where
[v] is the value in decanewton metre per foot
[SI] is the value in SI
a = Foot/(Deca), i.e., 0.030479999999999997
and
Foot = 12.0 * Inch
Deca = 10.0
Inch = 0.0254 reference: https://www.nist.gov/pml/owm/si-units-length
"""@EN; 
                             rdfs:subClassOf ddhub:Unit. 
ddhub:DecanewtonMetrePerHour a owl:Class; 
                             rdfs:comment """[v] = a * [SI]
where
[v] is the value in decanewton metre per hour
[SI] is the value in SI
a = Hour/(Deca), i.e., 360
and
Hour = 60.0 * Minute
Deca = 10.0
Minute = 60.0
"""@EN; 
                             rdfs:subClassOf ddhub:Unit. 
ddhub:DecanewtonMetrePerInch a owl:Class; 
                             rdfs:comment """[v] = a * [SI]
where
[v] is the value in decanewton metre per inch
[SI] is the value in SI
a = Inch/Deca, i.e., 0.0025399999999999997
and
Inch = 0.0254 reference: https://www.nist.gov/pml/owm/si-units-length
Deca = 10.0
"""@EN; 
                             rdfs:subClassOf ddhub:Unit. 
ddhub:DecanewtonMetrePerMetre a owl:Class; 
                              rdfs:comment """[v] = a * [SI]
where
[v] is the value in decanewton metre per metre
[SI] is the value in SI
a = Unit/Deca, i.e., 0.1
and
Unit = 1.0
Deca = 10.0
"""@EN; 
                              rdfs:subClassOf ddhub:Unit. 
ddhub:DecanewtonMetrePerMillimetre a owl:Class; 
                                   rdfs:comment """[v] = a * [SI]
where
[v] is the value in decanewton metre per millimetre
[SI] is the value in SI
a = Milli/(Deca), i.e., 0.0001
and
Milli = 0.001
Deca = 10.0
"""@EN; 
                                   rdfs:subClassOf ddhub:Unit. 
ddhub:DecanewtonMetrePerMinute a owl:Class; 
                               rdfs:comment """[v] = a * [SI]
where
[v] is the value in decanewton metre per minute
[SI] is the value in SI
a = Minute/(Deca), i.e., 6
and
Minute = 60.0
Deca = 10.0
"""@EN; 
                               rdfs:subClassOf ddhub:Unit. 
ddhub:DecanewtonMetrePerSecond a owl:Class; 
                               rdfs:comment """[v] = a * [SI]
where
[v] is the value in decanewton metre per second
[SI] is the value in SI
a = 1.0/(Deca), i.e., 0.1
and
Deca = 10.0
"""@EN; 
                               rdfs:subClassOf ddhub:Unit. 
ddhub:DecanewtonPer10Metre a owl:Class; 
                           rdfs:comment """[v] = a * [SI]
where
[v] is the value in decanewton per 10 metre
[SI] is the value in SI
a = Deca/Deca, i.e., 1
and
Deca = 10.0
"""@EN; 
                           rdfs:subClassOf ddhub:Unit. 
ddhub:DecanewtonPer30Metre a owl:Class; 
                           rdfs:comment """[v] = a * [SI]
where
[v] is the value in decanewton per 30 metre
[SI] is the value in SI
a = 3*Deca/Deca, i.e., 3
and
Deca = 10.0
"""@EN; 
                           rdfs:subClassOf ddhub:Unit. 
ddhub:DecanewtonPerCentimetre a owl:Class; 
                              rdfs:comment """[v] = a * [SI]
where
[v] is the value in decanewton per centimetre
[SI] is the value in SI
a = Centi/Deca, i.e., 0.001
and
Centi = 0.01
Deca = 10.0
"""@EN; 
                              rdfs:subClassOf ddhub:Unit. 
ddhub:DecanewtonPerDecimetre a owl:Class; 
                             rdfs:comment """[v] = a * [SI]
where
[v] is the value in decanewton per decimetre
[SI] is the value in SI
a = Deci/Deca, i.e., 0.01
and
Deci = 0.1
Deca = 10.0
"""@EN; 
                             rdfs:subClassOf ddhub:Unit. 
ddhub:DecanewtonPerHour a owl:Class; 
                        rdfs:comment """[v] = a * [SI]
where
[v] is the value in decanewton per hour
[SI] is the value in SI
a = Hour/(Deca), i.e., 360
and
Hour = 60.0 * Minute
Deca = 10.0
Minute = 60.0
"""@EN; 
                        rdfs:subClassOf ddhub:Unit. 
ddhub:DecanewtonPerMetre a owl:Class; 
                         rdfs:comment """[v] = a * [SI]
where
[v] is the value in decanewton per metre
[SI] is the value in SI
a = 1.0/Deca, i.e., 0.1
and
Deca = 10.0
"""@EN; 
                         rdfs:subClassOf ddhub:Unit. 
ddhub:DecanewtonPerMillimetre a owl:Class; 
                              rdfs:comment """[v] = a * [SI]
where
[v] is the value in decanewton per millimetre
[SI] is the value in SI
a = Milli/Deca, i.e., 0.0001
and
Milli = 0.001
Deca = 10.0
"""@EN; 
                              rdfs:subClassOf ddhub:Unit. 
ddhub:DecanewtonPerMinute a owl:Class; 
                          rdfs:comment """[v] = a * [SI]
where
[v] is the value in decanewton per minute
[SI] is the value in SI
a = Minute/(Deca), i.e., 6
and
Minute = 60.0
Deca = 10.0
"""@EN; 
                          rdfs:subClassOf ddhub:Unit. 
ddhub:DecanewtonPerSecond a owl:Class; 
                          rdfs:comment """[v] = a * [SI]
where
[v] is the value in decanewton per second
[SI] is the value in SI
a = 1.0/(Deca), i.e., 0.1
and
Deca = 10.0
"""@EN; 
                          rdfs:subClassOf ddhub:Unit. 
ddhub:Decawatt a owl:Class; 
               rdfs:comment """[v] = a * [SI]
where
[v] is the value in decawatt
[SI] is the value in SI
a = 1.0/Deca, i.e., 0.1
and
Deca = 10.0
"""@EN; 
               rdfs:subClassOf ddhub:Unit. 
ddhub:Deciampere a owl:Class; 
                 rdfs:comment """[v] = a * [SI]
where
[v] is the value in deciampere
[SI] is the value in SI
a = 1.0/Deci, i.e., 10
and
Deci = 0.1
"""@EN; 
                 rdfs:subClassOf ddhub:Unit. 
ddhub:Decilitre a owl:Class; 
                rdfs:comment """[v] = a * [SI]
where
[v] is the value in decilitre
[SI] is the value in SI
a = 1.0/(Deci*Milli), i.e., 10000
and
Deci = 0.1
Milli = 0.001
"""@EN; 
                rdfs:subClassOf ddhub:Unit. 
ddhub:DecimalCandle a owl:Class; 
                    rdfs:comment """[v] = a * [SI]
where
[v] is the value in decimal candle
[SI] is the value in SI
a = 1.0 / Unit, i.e., 1
and
Unit = 1.0
"""@EN; 
                    rdfs:subClassOf ddhub:Unit. 
ddhub:Decimetre a owl:Class; 
                rdfs:comment """[v] = a * [SI]
where
[v] is the value in decimetre
[SI] is the value in SI
a = 1.0/Deci, i.e., 10
and
Deci = 0.1
"""@EN; 
                rdfs:subClassOf ddhub:Unit. 
ddhub:DecimetrePerDay a owl:Class; 
                      rdfs:comment """[v] = a * [SI]
where
[v] is the value in decimetre per day
[SI] is the value in SI
a = Day/Deci, i.e., 864000
and
Day = 24.0 * Hour
Deci = 0.1
Hour = 60.0 * Minute
Minute = 60.0
"""@EN; 
                      rdfs:subClassOf ddhub:Unit. 
ddhub:DecimetrePerHour a owl:Class; 
                       rdfs:comment """[v] = a * [SI]
where
[v] is the value in decimetre per hour
[SI] is the value in SI
a = Hour/Deci, i.e., 36000
and
Hour = 60.0 * Minute
Deci = 0.1
Minute = 60.0
"""@EN; 
                       rdfs:subClassOf ddhub:Unit. 
ddhub:DecimetrePerKilometre a owl:Class; 
                            rdfs:comment """[v] = a * [SI]
where
[v] is the value in decimetre per kilometre
[SI] is the value in SI
a = Kilo / Deci, i.e., 10000
and
Kilo = 1000.0
Deci = 0.1
"""@EN; 
                            rdfs:subClassOf ddhub:Unit. 
ddhub:DecimetrePerMetre a owl:Class; 
                        rdfs:comment """[v] = a * [SI]
where
[v] is the value in decimetre per metre
[SI] is the value in SI
a = 1.0 / Deci, i.e., 10
and
Deci = 0.1
"""@EN; 
                        rdfs:subClassOf ddhub:Unit. 
ddhub:DecimetrePerMinute a owl:Class; 
                         rdfs:comment """[v] = a * [SI]
where
[v] is the value in decimetre per minute
[SI] is the value in SI
a = Minute/Deci, i.e., 600
and
Minute = 60.0
Deci = 0.1
"""@EN; 
                         rdfs:subClassOf ddhub:Unit. 
ddhub:DecimetrePerSecond a owl:Class; 
                         rdfs:comment """[v] = a * [SI]
where
[v] is the value in decimetre per second
[SI] is the value in SI
a = Unit/Deci, i.e., 10
and
Unit = 1.0
Deci = 0.1
"""@EN; 
                         rdfs:subClassOf ddhub:Unit. 
ddhub:Decimole a owl:Class; 
               rdfs:comment """[v] = a * [SI]
where
[v] is the value in decimole
[SI] is the value in SI
a = 1.0/Deci, i.e., 10
and
Deci = 0.1
"""@EN; 
               rdfs:subClassOf ddhub:Unit. 
ddhub:DecisionLevelIntegationModel a owl:Class; 
                                   rdfs:comment """A model that integrates data at a high-level like using majority voting, ensemble methods, Bayesian decision fusion,
Dempster-Shafer theory.
"""@EN; 
                                   rdfs:subClassOf ddhub:DataIntegrationStrategy. 
ddhub:Deciwatt a owl:Class; 
               rdfs:comment """[v] = a * [SI]
where
[v] is the value in deciwatt
[SI] is the value in SI
a = 1.0/Deci, i.e., 10
and
Deci = 0.1
"""@EN; 
               rdfs:subClassOf ddhub:Unit. 
ddhub:Degasser a owl:Class; 
               rdfs:comment ""@EN; 
               rdfs:subClassOf ddhub:CirculationSystem. 
ddhub:Degree a owl:Class; 
             rdfs:comment """[v] = a * [SI]
where
[v] is the value in degree
[SI] is the value in SI
a = Degree, i.e., 57.29577951308232
and
Degree = 180.0 / System.Math.PI
"""@EN; 
             rdfs:subClassOf ddhub:Unit. 
ddhub:DegreeGauss a owl:Class; 
                  rdfs:comment """[v] = a * [SI]
where
[v] is the value in degree gauss
[SI] is the value in SI
a = Degree/Gauss, i.e., 572957.7951308232
and
Degree = 180.0 / System.Math.PI
Gauss = 1e-4 reference: https://en.wikipedia.org/wiki/Gauss_(unit)
"""@EN; 
                  rdfs:subClassOf ddhub:Unit. 
ddhub:DegreeMaxwellPerSquareCentimetre a owl:Class; 
                                       rdfs:comment """[v] = a * [SI]
where
[v] is the value in degree maxwell per square centimetre
[SI] is the value in SI
a = Degree/(Centi*Centi), i.e., 572957.7951308232
and
Degree = 180.0 / System.Math.PI
Centi = 0.01
"""@EN; 
                                       rdfs:subClassOf ddhub:Unit. 
ddhub:DegreeMicrotesla a owl:Class; 
                       rdfs:comment """[v] = a * [SI]
where
[v] is the value in degree microtesla
[SI] is the value in SI
a = Degree/Micro, i.e., 57295779.513082325
and
Degree = 180.0 / System.Math.PI
Micro = 1e-6
"""@EN; 
                       rdfs:subClassOf ddhub:Unit. 
ddhub:DegreeMilligauss a owl:Class; 
                       rdfs:comment """[v] = a * [SI]
where
[v] is the value in degree milligauss
[SI] is the value in SI
a = Degree/(Milli*Gauss), i.e., 572957795.1308231
and
Degree = 180.0 / System.Math.PI
Milli = 0.001
Gauss = 1e-4 reference: https://en.wikipedia.org/wiki/Gauss_(unit)
"""@EN; 
                       rdfs:subClassOf ddhub:Unit. 
ddhub:DegreeMillitesla a owl:Class; 
                       rdfs:comment """[v] = a * [SI]
where
[v] is the value in degree millitesla
[SI] is the value in SI
a = Degree/Milli, i.e., 57295.77951308232
and
Degree = 180.0 / System.Math.PI
Milli = 0.001
"""@EN; 
                       rdfs:subClassOf ddhub:Unit. 
ddhub:DegreeNanotesla a owl:Class; 
                      rdfs:comment """[v] = a * [SI]
where
[v] is the value in degree nanotesla
[SI] is the value in SI
a = Degree/Nano, i.e., 57295779513.08232
and
Degree = 180.0 / System.Math.PI
Nano = 1e-9
"""@EN; 
                      rdfs:subClassOf ddhub:Unit. 
ddhub:DegreePer100ft a owl:Class; 
                     rdfs:comment """[v] = a * [SI]
where
[v] is the value in degree per 100ft
[SI] is the value in SI
a = Degree*100.0*Foot, i.e., 1746.375359558749
and
Degree = 180.0 / System.Math.PI
Foot = 12.0 * Inch
Inch = 0.0254 reference: https://www.nist.gov/pml/owm/si-units-length
"""@EN; 
                     rdfs:subClassOf ddhub:Unit. 
ddhub:DegreePer10m a owl:Class; 
                   rdfs:comment """[v] = a * [SI]
where
[v] is the value in degree per 10m
[SI] is the value in SI
a = Degree*10.0, i.e., 572.9577951308232
and
Degree = 180.0 / System.Math.PI
"""@EN; 
                   rdfs:subClassOf ddhub:Unit. 
ddhub:DegreePer30ft a owl:Class; 
                    rdfs:comment """[v] = a * [SI]
where
[v] is the value in degree per 30ft
[SI] is the value in SI
a = Degree*30.0*Foot, i.e., 523.9126078676246
and
Degree = 180.0 / System.Math.PI
Foot = 12.0 * Inch
Inch = 0.0254 reference: https://www.nist.gov/pml/owm/si-units-length
"""@EN; 
                    rdfs:subClassOf ddhub:Unit. 
ddhub:DegreePer30m a owl:Class; 
                   rdfs:comment """[v] = a * [SI]
where
[v] is the value in degree per 30m
[SI] is the value in SI
a = Degree*30.0, i.e., 1718.8733853924696
and
Degree = 180.0 / System.Math.PI
"""@EN; 
                   rdfs:subClassOf ddhub:Unit. 
ddhub:DegreePerCentimeter a owl:Class; 
                          rdfs:comment """[v] = a * [SI]
where
[v] is the value in degree per centimeter
[SI] is the value in SI
a = Degree*Centi, i.e., 0.5729577951308232
and
Degree = 180.0 / System.Math.PI
Centi = 0.01
"""@EN; 
                          rdfs:subClassOf ddhub:Unit. 
ddhub:DegreePerCentimetre a owl:Class; 
                          rdfs:comment """[v] = a * [SI]
where
[v] is the value in degree per centimetre
[SI] is the value in SI
a = Degree*Centi, i.e., 0.5729577951308232
and
Degree = 180.0 / System.Math.PI
Centi = 0.01
"""@EN; 
                          rdfs:subClassOf ddhub:Unit. 
ddhub:DegreePerDay a owl:Class; 
                   rdfs:comment """[v] = a * [SI]
where
[v] is the value in degree per day
[SI] is the value in SI
a = Degree*Day, i.e., 4950355.3499303125
and
Degree = 180.0 / System.Math.PI
Day = 24.0 * Hour
Hour = 60.0 * Minute
Minute = 60.0
"""@EN; 
                   rdfs:subClassOf ddhub:Unit. 
ddhub:DegreePerDayPerHour a owl:Class; 
                          rdfs:comment """[v] = a * [SI]
where
[v] is the value in degree per day per hour
[SI] is the value in SI
a = Day*Hour*Degree, i.e., 17821279259.749126
and
Day = 24.0 * Hour
Hour = 60.0 * Minute
Degree = 180.0 / System.Math.PI
Minute = 60.0
"""@EN; 
                          rdfs:subClassOf ddhub:Unit. 
ddhub:DegreePerDayPerMinute a owl:Class; 
                            rdfs:comment """[v] = a * [SI]
where
[v] is the value in degree per day per minute
[SI] is the value in SI
a = Day*Minute*Degree, i.e., 297021320.99581873
and
Day = 24.0 * Hour
Minute = 60.0
Degree = 180.0 / System.Math.PI
Hour = 60.0 * Minute
"""@EN; 
                            rdfs:subClassOf ddhub:Unit. 
ddhub:DegreePerDayPerSecond a owl:Class; 
                            rdfs:comment """[v] = a * [SI]
where
[v] is the value in degree per day per second
[SI] is the value in SI
a = Day*Degree, i.e., 4950355.3499303125
and
Day = 24.0 * Hour
Degree = 180.0 / System.Math.PI
Hour = 60.0 * Minute
Minute = 60.0
"""@EN; 
                            rdfs:subClassOf ddhub:Unit. 
ddhub:DegreePerDaySquared a owl:Class; 
                          rdfs:comment """[v] = a * [SI]
where
[v] is the value in degree per day squared
[SI] is the value in SI
a = Day*Day*Degree, i.e., 427710702233.979
and
Day = 24.0 * Hour
Degree = 180.0 / System.Math.PI
Hour = 60.0 * Minute
Minute = 60.0
"""@EN; 
                          rdfs:subClassOf ddhub:Unit. 
ddhub:DegreePerDecameter a owl:Class; 
                         rdfs:comment """[v] = a * [SI]
where
[v] is the value in degree per decameter
[SI] is the value in SI
a = Degree*Deca, i.e., 572.9577951308232
and
Degree = 180.0 / System.Math.PI
Deca = 10.0
"""@EN; 
                         rdfs:subClassOf ddhub:Unit. 
ddhub:DegreePerDecimeter a owl:Class; 
                         rdfs:comment """[v] = a * [SI]
where
[v] is the value in degree per decimeter
[SI] is the value in SI
a = Degree*Deci, i.e., 5.729577951308233
and
Degree = 180.0 / System.Math.PI
Deci = 0.1
"""@EN; 
                         rdfs:subClassOf ddhub:Unit. 
ddhub:DegreePerDecimetre a owl:Class; 
                         rdfs:comment """[v] = a * [SI]
where
[v] is the value in degree per decimetre
[SI] is the value in SI
a = Degree*Deci, i.e., 5.729577951308233
and
Degree = 180.0 / System.Math.PI
Deci = 0.1
"""@EN; 
                         rdfs:subClassOf ddhub:Unit. 
ddhub:DegreePerFoot a owl:Class; 
                    rdfs:comment """[v] = a * [SI]
where
[v] is the value in degree per foot
[SI] is the value in SI
a = Degree*Foot, i.e., 17.46375359558749
and
Degree = 180.0 / System.Math.PI
Foot = 12.0 * Inch
Inch = 0.0254 reference: https://www.nist.gov/pml/owm/si-units-length
"""@EN; 
                    rdfs:subClassOf ddhub:Unit. 
ddhub:DegreePerHectometer a owl:Class; 
                          rdfs:comment """[v] = a * [SI]
where
[v] is the value in degree per hectometer
[SI] is the value in SI
a = Degree*Hecto, i.e., 5729.5779513082325
and
Degree = 180.0 / System.Math.PI
Hecto = 100.0
"""@EN; 
                          rdfs:subClassOf ddhub:Unit. 
ddhub:DegreePerHour a owl:Class; 
                    rdfs:comment """[v] = a * [SI]
where
[v] is the value in degree per hour
[SI] is the value in SI
a = Degree*Hour, i.e., 206264.80624709636
and
Degree = 180.0 / System.Math.PI
Hour = 60.0 * Minute
Minute = 60.0
"""@EN; 
                    rdfs:subClassOf ddhub:Unit. 
ddhub:DegreePerHourPerDay a owl:Class; 
                          rdfs:comment """[v] = a * [SI]
where
[v] is the value in degree per hour per day
[SI] is the value in SI
a = Hour*Day*Degree, i.e., 17821279259.749126
and
Hour = 60.0 * Minute
Day = 24.0 * Hour
Degree = 180.0 / System.Math.PI
Minute = 60.0
"""@EN; 
                          rdfs:subClassOf ddhub:Unit. 
ddhub:DegreePerHourPerMinute a owl:Class; 
                             rdfs:comment """[v] = a * [SI]
where
[v] is the value in degree per hour per minute
[SI] is the value in SI
a = Hour*Minute*Degree, i.e., 12375888.374825781
and
Hour = 60.0 * Minute
Minute = 60.0
Degree = 180.0 / System.Math.PI
"""@EN; 
                             rdfs:subClassOf ddhub:Unit. 
ddhub:DegreePerHourPerSecond a owl:Class; 
                             rdfs:comment """[v] = a * [SI]
where
[v] is the value in degree per hour per second
[SI] is the value in SI
a = Hour*Degree, i.e., 206264.80624709636
and
Hour = 60.0 * Minute
Degree = 180.0 / System.Math.PI
Minute = 60.0
"""@EN; 
                             rdfs:subClassOf ddhub:Unit. 
ddhub:DegreePerHourSquared a owl:Class; 
                           rdfs:comment """[v] = a * [SI]
where
[v] is the value in degree per hour squared
[SI] is the value in SI
a = Hour*Hour*Degree, i.e., 742553302.4895469
and
Hour = 60.0 * Minute
Degree = 180.0 / System.Math.PI
Minute = 60.0
"""@EN; 
                           rdfs:subClassOf ddhub:Unit. 
ddhub:DegreePerInch a owl:Class; 
                    rdfs:comment """[v] = a * [SI]
where
[v] is the value in degree per inch
[SI] is the value in SI
a = Degree*Inch, i.e., 1.455312799632291
and
Degree = 180.0 / System.Math.PI
Inch = 0.0254 reference: https://www.nist.gov/pml/owm/si-units-length
"""@EN; 
                    rdfs:subClassOf ddhub:Unit. 
ddhub:DegreePerKilometer a owl:Class; 
                         rdfs:comment """[v] = a * [SI]
where
[v] is the value in degree per kilometer
[SI] is the value in SI
a = Degree*Kilo, i.e., 57295.77951308232
and
Degree = 180.0 / System.Math.PI
Kilo = 1000.0
"""@EN; 
                         rdfs:subClassOf ddhub:Unit. 
ddhub:DegreePerMetre a owl:Class; 
                     rdfs:comment """[v] = a * [SI]
where
[v] is the value in degree per metre
[SI] is the value in SI
a = Degree, i.e., 57.29577951308232
and
Degree = 180.0 / System.Math.PI
"""@EN; 
                     rdfs:subClassOf ddhub:Unit. 
ddhub:DegreePerMicrometer a owl:Class; 
                          rdfs:comment """[v] = a * [SI]
where
[v] is the value in degree per micrometer
[SI] is the value in SI
a = Degree*Micro, i.e., 5.729577951308232E-05
and
Degree = 180.0 / System.Math.PI
Micro = 1e-6
"""@EN; 
                          rdfs:subClassOf ddhub:Unit. 
ddhub:DegreePerMile a owl:Class; 
                    rdfs:comment """[v] = a * [SI]
where
[v] is the value in degree per mile
[SI] is the value in SI
a = Degree*Mile, i.e., 92208.61898470194
and
Degree = 180.0 / System.Math.PI
Mile = 1760.0 * Yard reference: https://dictionary.cambridge.org/dictionary/english/mile
Yard = 3.0 * Foot
Foot = 12.0 * Inch
Inch = 0.0254 reference: https://www.nist.gov/pml/owm/si-units-length
"""@EN; 
                    rdfs:subClassOf ddhub:Unit. 
ddhub:DegreePerMillimeter a owl:Class; 
                          rdfs:comment """[v] = a * [SI]
where
[v] is the value in degree per millimeter
[SI] is the value in SI
a = Degree*Milli, i.e., 0.057295779513082325
and
Degree = 180.0 / System.Math.PI
Milli = 0.001
"""@EN; 
                          rdfs:subClassOf ddhub:Unit. 
ddhub:DegreePerMillimetre a owl:Class; 
                          rdfs:comment """[v] = a * [SI]
where
[v] is the value in degree per millimetre
[SI] is the value in SI
a = Degree*Milli, i.e., 0.057295779513082325
and
Degree = 180.0 / System.Math.PI
Milli = 0.001
"""@EN; 
                          rdfs:subClassOf ddhub:Unit. 
ddhub:DegreePerMinute a owl:Class; 
                      rdfs:comment """[v] = a * [SI]
where
[v] is the value in degree per minute
[SI] is the value in SI
a = Degree*Minute, i.e., 3437.746770784939
and
Degree = 180.0 / System.Math.PI
Minute = 60.0
"""@EN; 
                      rdfs:subClassOf ddhub:Unit. 
ddhub:DegreePerMinutePerDay a owl:Class; 
                            rdfs:comment """[v] = a * [SI]
where
[v] is the value in degree per minute per day
[SI] is the value in SI
a = Minute*Day*Degree, i.e., 297021320.99581873
and
Minute = 60.0
Day = 24.0 * Hour
Degree = 180.0 / System.Math.PI
Hour = 60.0 * Minute
"""@EN; 
                            rdfs:subClassOf ddhub:Unit. 
ddhub:DegreePerMinutePerHour a owl:Class; 
                             rdfs:comment """[v] = a * [SI]
where
[v] is the value in degree per minute per hour
[SI] is the value in SI
a = Minute*Hour*Degree, i.e., 12375888.374825781
and
Minute = 60.0
Hour = 60.0 * Minute
Degree = 180.0 / System.Math.PI
"""@EN; 
                             rdfs:subClassOf ddhub:Unit. 
ddhub:DegreePerMinutePerSecond a owl:Class; 
                               rdfs:comment """[v] = a * [SI]
where
[v] is the value in degree per minute per second
[SI] is the value in SI
a = Minute*Degree, i.e., 3437.746770784939
and
Minute = 60.0
Degree = 180.0 / System.Math.PI
"""@EN; 
                               rdfs:subClassOf ddhub:Unit. 
ddhub:DegreePerMinuteSquared a owl:Class; 
                             rdfs:comment """[v] = a * [SI]
where
[v] is the value in degree per minute squared
[SI] is the value in SI
a = Minute*Minute*Degree, i.e., 206264.80624709636
and
Minute = 60.0
Degree = 180.0 / System.Math.PI
"""@EN; 
                             rdfs:subClassOf ddhub:Unit. 
ddhub:DegreePerNanometer a owl:Class; 
                         rdfs:comment """[v] = a * [SI]
where
[v] is the value in degree per nanometer
[SI] is the value in SI
a = Degree*Nano, i.e., 5.7295779513082324E-08
and
Degree = 180.0 / System.Math.PI
Nano = 1e-9
"""@EN; 
                         rdfs:subClassOf ddhub:Unit. 
ddhub:DegreePerSecond a owl:Class; 
                      rdfs:comment """[v] = a * [SI]
where
[v] is the value in degree per second
[SI] is the value in SI
a = Degree, i.e., 57.29577951308232
and
Degree = 180.0 / System.Math.PI
"""@EN; 
                      rdfs:subClassOf ddhub:Unit. 
ddhub:DegreePerSecondPerDay a owl:Class; 
                            rdfs:comment """[v] = a * [SI]
where
[v] is the value in degree per second per day
[SI] is the value in SI
a = Degree*Unit*Day, i.e., 4950355.3499303125
and
Degree = 180.0 / System.Math.PI
Unit = 1.0
Day = 24.0 * Hour
Hour = 60.0 * Minute
Minute = 60.0
"""@EN; 
                            rdfs:subClassOf ddhub:Unit. 
ddhub:DegreePerSecondPerHour a owl:Class; 
                             rdfs:comment """[v] = a * [SI]
where
[v] is the value in degree per second per hour
[SI] is the value in SI
a = Unit*Hour*Degree, i.e., 206264.80624709636
and
Unit = 1.0
Hour = 60.0 * Minute
Degree = 180.0 / System.Math.PI
Minute = 60.0
"""@EN; 
                             rdfs:subClassOf ddhub:Unit. 
ddhub:DegreePerSecondPerMinute a owl:Class; 
                               rdfs:comment """[v] = a * [SI]
where
[v] is the value in degree per second per minute
[SI] is the value in SI
a = Unit * Minute * Degree, i.e., 3437.746770784939
and
Unit = 1.0
Minute = 60.0
Degree = 180.0 / System.Math.PI
"""@EN; 
                               rdfs:subClassOf ddhub:Unit. 
ddhub:DegreePerSecondSquared a owl:Class; 
                             rdfs:comment """[v] = a * [SI]
where
[v] is the value in degree per second squared
[SI] is the value in SI
a = Degree, i.e., 57.29577951308232
and
Degree = 180.0 / System.Math.PI
"""@EN; 
                             rdfs:subClassOf ddhub:Unit. 
ddhub:DegreePerSquareRootDay a owl:Class; 
                             rdfs:comment """[v] = a * [SI]
where
[v] is the value in degree per square root day
[SI] is the value in SI
a = Sqrt(Day)*Degree, i.e., 16841.450906647406
and
Day = 24.0 * Hour
Degree = 180.0 / System.Math.PI
Hour = 60.0 * Minute
Minute = 60.0
"""@EN; 
                             rdfs:subClassOf ddhub:Unit. 
ddhub:DegreePerSquareRootHour a owl:Class; 
                              rdfs:comment """[v] = a * [SI]
where
[v] is the value in degree per square root hour
[SI] is the value in SI
a = Sqrt(Hour)*Degree, i.e., 3437.746770784939
and
Hour = 60.0 * Minute
Degree = 180.0 / System.Math.PI
Minute = 60.0
"""@EN; 
                              rdfs:subClassOf ddhub:Unit. 
ddhub:DegreePerSquareRootMinute a owl:Class; 
                                rdfs:comment """[v] = a * [SI]
where
[v] is the value in degree per square root minute
[SI] is the value in SI
a = Sqrt(Minute)*Degree, i.e., 443.8111997242799
and
Minute = 60.0
Degree = 180.0 / System.Math.PI
"""@EN; 
                                rdfs:subClassOf ddhub:Unit. 
ddhub:DegreePerSquareRootSecond a owl:Class; 
                                rdfs:comment """[v] = a * [SI]
where
[v] is the value in degree per square root second
[SI] is the value in SI
a = Degree, i.e., 57.29577951308232
and
Degree = 180.0 / System.Math.PI
"""@EN; 
                                rdfs:subClassOf ddhub:Unit. 
ddhub:DegreePerYard a owl:Class; 
                    rdfs:comment """[v] = a * [SI]
where
[v] is the value in degree per yard
[SI] is the value in SI
a = Degree*Yard, i.e., 52.391260786762466
and
Degree = 180.0 / System.Math.PI
Yard = 3.0 * Foot
Foot = 12.0 * Inch
Inch = 0.0254 reference: https://www.nist.gov/pml/owm/si-units-length
"""@EN; 
                    rdfs:subClassOf ddhub:Unit. 
ddhub:DegreeSquared a owl:Class; 
                    rdfs:comment """[v] = a * [SI]
where
[v] is the value in degree squared
[SI] is the value in SI
a = (180.0*180.0)/(PI*PI), i.e., 3282.806350011744
"""@EN; 
                    rdfs:subClassOf ddhub:Unit. 
ddhub:DegreeTesla a owl:Class; 
                  rdfs:comment """[v] = a * [SI]
where
[v] is the value in degree tesla
[SI] is the value in SI
a = Degree/Unit, i.e., 57.29577951308232
and
Degree = 180.0 / System.Math.PI
Unit = 1.0
"""@EN; 
                  rdfs:subClassOf ddhub:Unit. 
ddhub:DegreeWeberPerSquareMetre a owl:Class; 
                                rdfs:comment """[v] = a * [SI]
where
[v] is the value in degree weber per square metre
[SI] is the value in SI
a = Degree/Unit, i.e., 57.29577951308232
and
Degree = 180.0 / System.Math.PI
Unit = 1.0
"""@EN; 
                                rdfs:subClassOf ddhub:Unit. 
ddhub:DensityIn a owl:Class; 
                rdfs:comment ""@EN; 
                rdfs:subClassOf ddhub:PrototypeData. 
ddhub:DensityOut a owl:Class; 
                 rdfs:comment ""@EN; 
                 rdfs:subClassOf ddhub:PrototypeData. 
ddhub:DepthAndAngleFrame a owl:Class; 
                         rdfs:comment ""@EN; 
                         rdfs:subClassOf ddhub:ReferenceFrame. 
ddhub:DepthDrillingQuantity a owl:Class; 
                            rdfs:comment """Length is a measure of distance.
The dimension of length is:
$$[L]$$.
The SI unit for **length** is: metre with the associated unit label $m$
The meaningful precision of depth in the drilling context is typically: 0.001 m
"""@EN; 
                            rdfs:subClassOf ddhub:MeasurableQuantity. 
ddhub:Derivation a owl:Class; 
                 rdfs:comment ""@EN; 
                 rdfs:subClassOf ddhub:TimeBasedTransformation. 
ddhub:DerivedMeasurement a owl:Class; 
                         rdfs:comment ""@EN; 
                         rdfs:subClassOf ddhub:Measurement. 
ddhub:Derrick a owl:Class; 
              rdfs:comment ""@EN; 
              rdfs:subClassOf ddhub:HoistingSystem. 
ddhub:DerrickFloorVerticalLocation a owl:Class; 
                                   rdfs:comment ""@EN; 
                                   rdfs:subClassOf ddhub:VerticalReferenceLocation. 
ddhub:DescriptiveModel a owl:Class; 
                       rdfs:comment """A model that seeks to explain or describe a system's behavior or underlying mechanisms.
"""@EN; 
                       rdfs:subClassOf ddhub:ModelingObjective. 
ddhub:DeterministicModel a owl:Class; 
                         rdfs:comment ""@EN; 
                         rdfs:subClassOf ddhub:ModelType. 
ddhub:DiameterPipeDrillingQuantity a owl:Class; 
                                   rdfs:comment """Length is a measure of distance.
The dimension of length is:
$$[L]$$.
The SI unit for **length** is: metre with the associated unit label $m$
The meaningful precision of small length is typically: 0.0001 m
The meaningful precision of pipe diameter in the drilling context is typically: 0.0001 m
"""@EN; 
                                   rdfs:subClassOf ddhub:MeasurableQuantity. 
ddhub:DiameterPoreDrillingQuantity a owl:Class; 
                                   rdfs:comment """Length is a measure of distance.
The dimension of length is:
$$[L]$$.
The SI unit for **length** is: metre with the associated unit label $m$
The meaningful precision of small length is typically: 1E-07 m
The meaningful precision of pore diameter in the drilling context is typically: 1E-07 m
"""@EN; 
                                   rdfs:subClassOf ddhub:MeasurableQuantity. 
ddhub:DiameterSmallQuantity a owl:Class; 
                            rdfs:comment """Length is a measure of distance.
The dimension of length is:
$$[L]$$.
The SI unit for **length** is: metre with the associated unit label $m$
The meaningful precision of small diameter is typically: 0.0001 m
"""@EN; 
                            rdfs:subClassOf ddhub:MeasurableQuantity. 
ddhub:Diamond a owl:Class; 
              rdfs:comment ""@EN; 
              rdfs:subClassOf ddhub:FixedCutter. 
ddhub:DiamondCore a owl:Class; 
                  rdfs:comment ""@EN; 
                  rdfs:subClassOf ddhub:FixedCutter. 
ddhub:DiaphragmMudPump a owl:Class; 
                       rdfs:comment ""@EN; 
                       rdfs:subClassOf ddhub:MudPump. 
ddhub:DieselElectricalDrawworks a owl:Class; 
                                rdfs:comment ""@EN; 
                                rdfs:subClassOf ddhub:Drawworks. 
ddhub:DifferentiallyStuck a owl:Class; 
                          rdfs:comment """This Noun is used to refer to a situation during which the drill-stem is stuck because of differential sticking.
"""@EN; 
                          rdfs:subClassOf ddhub:StuckPipe. 
ddhub:DifferentialPressureLimit a owl:Class; 
                                rdfs:comment """This Noun is used to refer to a differential pressure limit.
"""@EN; 
                                rdfs:subClassOf ddhub:DrillingLimit. 
ddhub:DifferentialStickingLocation a owl:Class; 
                                   rdfs:comment ""@EN; 
                                   rdfs:subClassOf ddhub:AbscissaReferenceLocation. 
ddhub:DigitalTwinAdvice a owl:Class; 
                        rdfs:comment """A digital twin simulates the drilling operation using the boundary conditions applied to the drilling system.
It provides information about the plausible values that can be expected anywhere along the drilling system. These results
are stored in a DigitalTwinAdvice.
"""@EN; 
                        rdfs:subClassOf ddhub:AdvisorySystemAdvice. 
ddhub:Dimensionless a owl:Class; 
                    rdfs:comment """No conversion necessary as the unit choice is SI
"""@EN; 
                    rdfs:subClassOf ddhub:Unit. 
ddhub:DimensionlessQuantity a owl:Class; 
                            rdfs:comment """As its name indicates, a dimensionless quantity has no dimension:
"""@EN; 
                            rdfs:subClassOf ddhub:Quantity. 
ddhub:DimensionLessStandardQuantity a owl:Class; 
                                    rdfs:comment """As its name indicates, a dimensionless quantity has no dimension:
The meaningful precision of standard dimensionless values is typically: 0.001 
"""@EN; 
                                    rdfs:subClassOf ddhub:MeasurableQuantity. 
ddhub:DipmeterAndImagingTools a owl:Class; 
                              rdfs:comment ""@EN; 
                              rdfs:subClassOf ddhub:WirelineLoggingTools. 
ddhub:DirectionalCasingWhileDrilling a owl:Class; 
                                     rdfs:comment ""@EN; 
                                     rdfs:subClassOf ddhub:Casingwhiledrilling. 
ddhub:DirectionalServiceCompany a owl:Class; 
                                rdfs:comment """A directional service company is an entity that provides services for downhole directional drilling and downhole measurements.
"""@EN; 
                                rdfs:subClassOf ddhub:ServiceCompany. 
ddhub:DirectionalTool a owl:Class; 
                      rdfs:comment ""@EN; 
                      rdfs:subClassOf ddhub:MeasurementWhileDrillingTools. 
ddhub:DirectTransformation a owl:Class; 
                           rdfs:comment """Direct transformations are performed using only the current value of their inputs, time is not involved
"""@EN; 
                           rdfs:subClassOf ddhub:Transformation. 
ddhub:DiscreteDataType a owl:Class; 
                       rdfs:comment ""@EN; 
                       rdfs:subClassOf ddhub:DataType. 
ddhub:DistanceBetweenRepeaters a owl:DatatypeProperty, owl:FunctionalProperty; 
                               rdfs:comment """The average distance between two repeaters. The physical quantity is Length and the unit is metre.
"""@EN; 
                               rdfs:domain ddhub:Telemetry; 
                               rdfs:range xsd:double. 
ddhub:Diverter a owl:Class; 
               rdfs:comment ""@EN; 
               rdfs:subClassOf ddhub:WellControlSystem. 
ddhub:DiverterLine a owl:Class; 
                   rdfs:comment ""@EN; 
                   rdfs:subClassOf ddhub:Diverter. 
ddhub:DiverterLineHanger a owl:Class; 
                         rdfs:comment ""@EN; 
                         rdfs:subClassOf ddhub:Diverter. 
ddhub:DogHouse a owl:Class; 
               rdfs:comment ""@EN; 
               rdfs:subClassOf ddhub:DrillFloorStructure. 
ddhub:Dolly a owl:Class; 
            rdfs:comment ""@EN; 
            rdfs:subClassOf ddhub:DrillFloorEquipment. 
ddhub:DollyRail a owl:Class; 
                rdfs:comment ""@EN; 
                rdfs:subClassOf ddhub:DrillFloorEquipment. 
ddhub:DotPerInch a owl:Class; 
                 rdfs:comment """[v] = a * [SI]
where
[v] is the value in dot per inch
[SI] is the value in SI
a = Inch, i.e., 0.0254
and
Inch = 0.0254 reference: https://www.nist.gov/pml/owm/si-units-length
"""@EN; 
                 rdfs:subClassOf ddhub:Unit. 
ddhub:DotPerMetre a owl:Class; 
                  rdfs:comment """No conversion necessary as the unit choice is SI
"""@EN; 
                  rdfs:subClassOf ddhub:Unit. 
ddhub:DotPerMicrometre a owl:Class; 
                       rdfs:comment """[v] = a * [SI]
where
[v] is the value in dot per micrometre
[SI] is the value in SI
a = Micro, i.e., 1E-06
and
Micro = 1e-6
"""@EN; 
                       rdfs:subClassOf ddhub:Unit. 
ddhub:DotPerMillimetre a owl:Class; 
                       rdfs:comment """[v] = a * [SI]
where
[v] is the value in dot per millimetre
[SI] is the value in SI
a = Milli, i.e., 0.001
and
Milli = 0.001
"""@EN; 
                       rdfs:subClassOf ddhub:Unit. 
ddhub:Doubles a owl:Class; 
              rdfs:comment ""@EN; 
              rdfs:subClassOf ddhub:Grouping. 
ddhub:DoubleStandDerrick a owl:Class; 
                         rdfs:comment ""@EN; 
                         rdfs:subClassOf ddhub:Derrick. 
ddhub:DownholeAlternator a owl:Class; 
                         rdfs:comment ""@EN; 
                         rdfs:subClassOf ddhub:PowerSystems. 
ddhub:DownholeBatteries a owl:Class; 
                        rdfs:comment ""@EN; 
                        rdfs:subClassOf ddhub:PowerSystems. 
ddhub:DownholeCtConnectors a owl:Class; 
                           rdfs:comment ""@EN; 
                           rdfs:subClassOf ddhub:CoiledTubingEquipment. 
ddhub:DownholeECD a owl:Class; 
                  rdfs:comment ""@EN; 
                  rdfs:subClassOf ddhub:PrototypeData. 
ddhub:DownholeEquipment a owl:Class; 
                        rdfs:comment ""@EN; 
                        rdfs:subClassOf ddhub:Equipment. 
ddhub:DownholeHydraulicNetwork a owl:Class; 
                               rdfs:comment ""@EN; 
                               rdfs:subClassOf ddhub:HydraulicNetwork. 
ddhub:DownholeMotor a owl:Class; 
                    rdfs:comment ""@EN; 
                    rdfs:subClassOf ddhub:DrillingEquipment. 
ddhub:DownholePressure a owl:Class; 
                       rdfs:comment ""@EN; 
                       rdfs:subClassOf ddhub:PrototypeData. 
ddhub:DownholePressureFeature a owl:Class; 
                              rdfs:comment """A downhole pressure feature indicates that something accounts for downhole pressure.
"""@EN; 
                              rdfs:subClassOf ddhub:DrillingManagementFeature. 
ddhub:DownholeRPM a owl:Class; 
                  rdfs:comment ""@EN; 
                  rdfs:subClassOf ddhub:PrototypeData. 
ddhub:DownHoleTelemetry a owl:Class; 
                        rdfs:comment """Technology that allows transfer of downhole data to the surface.
"""@EN; 
                        rdfs:subClassOf ddhub:Telemetry. 
ddhub:DownholeTemperature a owl:Class; 
                          rdfs:comment ""@EN; 
                          rdfs:subClassOf ddhub:PrototypeData. 
ddhub:DownholeTorque a owl:Class; 
                     rdfs:comment ""@EN; 
                     rdfs:subClassOf ddhub:PrototypeData. 
ddhub:DownholeValveAssembly a owl:Class; 
                            rdfs:comment ""@EN; 
                            rdfs:subClassOf ddhub:CasingEquipment. 
ddhub:DownlinkingProcedure a owl:Class; 
                           rdfs:comment """The downlinking procedure is used to manipulate the flowrate/pressure or rotational speed to send a coded message to
the rotary steerable system.
"""@EN; 
                           rdfs:subClassOf ddhub:DrillingProcedure. 
ddhub:Drawworks a owl:Class; 
                rdfs:comment ""@EN; 
                rdfs:subClassOf ddhub:HoistingSystem. 
ddhub:DrillCollars a owl:Class; 
                   rdfs:comment ""@EN; 
                   rdfs:subClassOf ddhub:DrillString. 
ddhub:DrillersConsole a owl:Class; 
                      rdfs:comment ""@EN; 
                      rdfs:subClassOf ddhub:DrillFloorEquipment. 
ddhub:DrillFloorEquipment a owl:Class; 
                          rdfs:comment ""@EN; 
                          rdfs:subClassOf ddhub:DrillFloorSystems. 
ddhub:DrillFloorStructure a owl:Class; 
                          rdfs:comment ""@EN; 
                          rdfs:subClassOf ddhub:DrillFloorSystems. 
ddhub:DrillFloorSubstructure a owl:Class; 
                             rdfs:comment ""@EN; 
                             rdfs:subClassOf ddhub:DrillFloorStructure. 
ddhub:DrillFloorSystems a owl:Class; 
                        rdfs:comment ""@EN; 
                        rdfs:subClassOf ddhub:RigEquipment. 
ddhub:DrillingBit a owl:Class; 
                  rdfs:comment ""@EN; 
                  rdfs:subClassOf ddhub:DrillstemTerminator. 
ddhub:DrillingContractor a owl:Class; 
                         rdfs:comment ""@EN; 
                         rdfs:subClassOf ddhub:DataProvider. 
ddhub:DrillingControlAdvice a owl:Class; 
                            rdfs:comment """A drilling control advisor provides information on how to control a part of the drilling process to stay as close
as possible to one or several desired values.
"""@EN; 
                            rdfs:subClassOf ddhub:AdvisorySystemAdvice. 
ddhub:DrillingDataPoint a owl:Class; 
                        rdfs:comment """Main type of DDHub data. Represents a drilling signal.
Can be a dynamic signal (linked to a ValueNode) or a static parameter. 
"""@EN; 
                        rdfs:subClassOf ddhub:DWISNoun. 
ddhub:DrillingEquipment a owl:Class; 
                        rdfs:comment ""@EN; 
                        rdfs:subClassOf ddhub:DownholeEquipment. 
ddhub:DrillingFaultDetectionIsolationAndRecoveryAdvice a owl:Class; 
                                                       rdfs:comment """A fault detection, isolation and recovery (FDIR) advisor provides information on how to detect an drilling incident
and parameters to procedure that is executed when a drilling incident is detected in order to first to isolate the drilling incident
and then possibly recover from that incident.
"""@EN; 
                                                       rdfs:subClassOf ddhub:AdvisorySystemAdvice. 
ddhub:DrillingFluid a owl:Class; 
                    rdfs:comment ""@EN; 
                    rdfs:subClassOf ddhub:CirculationSystem. 
ddhub:DrillingFluidDescription a owl:Class; 
                               rdfs:comment """A drilling fluid is a fluid that is used well
used during a drilling operation.
"""@EN; 
                               rdfs:subClassOf ddhub:FluidDescription. 
ddhub:DrillingFluidDisplacementFeature a owl:Class; 
                                       rdfs:comment """A drilling fluid displacement feature indicates that something accounts for displacing a drilling fluid with another.
"""@EN; 
                                       rdfs:subClassOf ddhub:CirculationFeature. 
ddhub:DrillingFluidGasComponent a owl:Class; 
                                rdfs:comment ""@EN; 
                                rdfs:subClassOf ddhub:GasComponent. 
ddhub:DrillingFluidLiquidComponent a owl:Class; 
                                   rdfs:comment ""@EN; 
                                   rdfs:subClassOf ddhub:LiquidComponent. 
ddhub:DrillingFluidOilComponent a owl:Class; 
                                rdfs:comment ""@EN; 
                                rdfs:subClassOf ddhub:DrillingFluidLiquidComponent. 
ddhub:DrillingFluidProvider a owl:Class; 
                            rdfs:comment """A drilling fluid provider is a company that provides and maintains the drilling fluids during well construction.
"""@EN; 
                            rdfs:subClassOf ddhub:ServiceCompany. 
ddhub:DrillingFluidSolidComponent a owl:Class; 
                                  rdfs:comment ""@EN; 
                                  rdfs:subClassOf ddhub:SolidComponent. 
ddhub:DrillingFluidSweepFeature a owl:Class; 
                                rdfs:comment """A drilling fluid sweep feature indicates that something accounts for sweeping the borehole with one or several fluids of
different densities and/or viscosities.
"""@EN; 
                                rdfs:subClassOf ddhub:CirculationFeature. 
ddhub:DrillingFluidWaterComponent a owl:Class; 
                                  rdfs:comment ""@EN; 
                                  rdfs:subClassOf ddhub:DrillingFluidLiquidComponent. 
ddhub:DrillingIncident a owl:Class; 
                       rdfs:comment """This is the parent class for drilling incidents. A drilling incident is often detectable by an abnormal value of a process variable, i.e., a variable that is influenced
by the drilling process.
"""@EN; 
                       rdfs:subClassOf ddhub:DWISNoun. 
ddhub:DrillingLimit a owl:Class; 
                    rdfs:comment """This is the parent class for drilling limits. A limit applies typically on a desired value as controlled by a controller.
"""@EN; 
                    rdfs:subClassOf ddhub:DWISNoun. 
ddhub:DrillingManagementFeature a owl:Class; 
                                rdfs:comment """A drilling management feature is a drilling management characteristic that is supported by something. For instance
an advisory system may provide ROP management parameters accounting for cuttings transport.
"""@EN; 
                                rdfs:subClassOf ddhub:DWISNoun. 
ddhub:DrillingObjective a owl:Class; 
                        rdfs:comment """This is the parent class for drilling objectives.
"""@EN; 
                        rdfs:subClassOf ddhub:DWISNoun. 
ddhub:DrillingProcedure a owl:Class; 
                        rdfs:comment """This is the parent class for drilling procedures.
"""@EN; 
                        rdfs:subClassOf ddhub:DWISNoun. 
ddhub:DrillingProgram a owl:Class; 
                      rdfs:comment """A drilling program is a set of procedures that are necessary to construct a well.
"""@EN; 
                      rdfs:subClassOf ddhub:Plan. 
ddhub:DrillingProgramFeature a owl:Class; 
                             rdfs:comment """A drilling program feature indicates that something accounts for the drilling program.
"""@EN; 
                             rdfs:subClassOf ddhub:DrillingManagementFeature. 
ddhub:DrillingRiser a owl:Class; 
                    rdfs:comment ""@EN; 
                    rdfs:subClassOf ddhub:MarineSystem. 
ddhub:DrillingSafeOperatingEnvelopeAdvice a owl:Class; 
                                          rdfs:comment """A safe operating envelope (SOE) advisor provides information on the limits that shall be used when controlling the drilling
process to avoid possible drilling incidents.
"""@EN; 
                                          rdfs:subClassOf ddhub:AdvisorySystemAdvice. 
ddhub:DrillingSignal a owl:Class; 
                     rdfs:comment """Data structure used to store the streaming drilling data.
"""@EN; 
                     rdfs:subClassOf ddhub:DWISNoun. 
ddhub:DrillingStandardProcedureAdvice a owl:Class; 
                                      rdfs:comment """A drilling standard procedure advisor provides parameters for a standard procedure like starting the mud pumps or
running a friction test.
"""@EN; 
                                      rdfs:subClassOf ddhub:AdvisorySystemAdvice. 
ddhub:DrillLine a owl:Class; 
                rdfs:comment ""@EN; 
                rdfs:subClassOf ddhub:HoistingSystem. 
ddhub:DrillLineFastener a owl:Class; 
                        rdfs:comment ""@EN; 
                        rdfs:subClassOf ddhub:HoistingSystem. 
ddhub:DrillPipe a owl:Class; 
                rdfs:comment ""@EN; 
                rdfs:subClassOf ddhub:DrillString. 
ddhub:DrillPipeElevator a owl:Class; 
                        rdfs:comment ""@EN; 
                        rdfs:subClassOf ddhub:DrillFloorEquipment. 
ddhub:DrillPipesAnnular a owl:Class; 
                        rdfs:comment ""@EN; 
                        rdfs:subClassOf ddhub:Annular. 
ddhub:DrillPipesInner a owl:Class; 
                      rdfs:comment ""@EN; 
                      rdfs:subClassOf ddhub:Pipe. 
ddhub:DrillPipeTongs a owl:Class; 
                     rdfs:comment ""@EN; 
                     rdfs:subClassOf ddhub:DrillFloorEquipment. 
ddhub:DrillStemAxialImpedimentFeature a owl:Class; 
                                      rdfs:comment """A drill-stem axial impediment feature indicates that something accounts for drill-stem axial impediment.
"""@EN; 
                                      rdfs:subClassOf ddhub:StuckPipeFeature. 
ddhub:DrillStemAxialMovementFeature a owl:Class; 
                                    rdfs:comment """A drill-stem axial movement feature indicates that something accounts for drill-stem axial movement.
"""@EN; 
                                    rdfs:subClassOf ddhub:DrillStemMovementFeature. 
ddhub:DrillStemAxialStickSlipFeature a owl:Class; 
                                     rdfs:comment """A drill-stem axial stick-slip feature indicates that something acconts for in particular axial stick-slip drill-stem vibrations.
"""@EN; 
                                     rdfs:subClassOf ddhub:DrillStemAxialVibrationFeature. 
ddhub:DrillStemAxialVibrationFeature a owl:Class; 
                                     rdfs:comment """A drill-stem axial vibration feature indicates that something accounts for in particular axial drill-stem vibrations.
"""@EN; 
                                     rdfs:subClassOf ddhub:DrillStemVibrationFeature. 
ddhub:DrillStemBackwardWhirlingFeature a owl:Class; 
                                       rdfs:comment """A drill-stem backward whirling feature indicates that something accounts for in particular drill-stem backward whirling.
"""@EN; 
                                       rdfs:subClassOf ddhub:DrillStemWhirlingFeature. 
ddhub:DrillStemBucklingFeature a owl:Class; 
                               rdfs:comment """A drill-stem buckling feature indicates that something accounts for drill-stem buckling.
"""@EN; 
                               rdfs:subClassOf ddhub:DrillingManagementFeature. 
ddhub:DrillStemChaoticWhirlingFeature a owl:Class; 
                                      rdfs:comment """A drill-stem chaotic whirling feature indicates that something accounts for in particular drill-stem chaotic whirling.
"""@EN; 
                                      rdfs:subClassOf ddhub:DrillStemWhirlingFeature. 
ddhub:DrillStemDescription a owl:Class; 
                           rdfs:comment """A dill-stem is a generic term for all strings that are run in a borehole. The drill-stem describes the geometrical
and mechanical characteristics of such a string. 
"""@EN; 
                           rdfs:subClassOf ddhub:WellBoreData. 
ddhub:DrillStemForwardWhirlingFeature a owl:Class; 
                                      rdfs:comment """A drill-stem forward whirling feature indicates that something accounts for in particular drill-stem forward whirling.
"""@EN; 
                                      rdfs:subClassOf ddhub:DrillStemWhirlingFeature. 
ddhub:DrillStemLateralVibrationFeature a owl:Class; 
                                       rdfs:comment """A drill-stem lateral vibration feature indicates that something accounts for in particular lateral drill-stem vibrations.
"""@EN; 
                                       rdfs:subClassOf ddhub:DrillStemVibrationFeature. 
ddhub:DrillStemMaterialStrengthDrillingQuantity a owl:Class; 
                                                rdfs:comment """Material strength refers to the ability of a material to withstand an applied force or load without failing or deforming. It measures how much stress a material can endure before it breaks, bends, or permanently deforms, often categorized into types like tensile, compressive, and shear strength.
The dimension of material strength is:
$$[ML^{-1}T^{-2}]$$.
The SI unit for **material strength** is: pascal with the associated unit label $Pa$
The meaningful precision of drill stem material strength in the drilling context is typically: 10000 Pa
"""@EN; 
                                                rdfs:subClassOf ddhub:MeasurableQuantity. 
ddhub:DrillStemMechanicalModel a owl:Class; 
                               rdfs:comment """A mechanical model for a drill-stem. Another standard name for drill-stem mechanical models is a torque and drag model.
"""@EN; 
                               rdfs:subClassOf ddhub:ModelType. 
ddhub:DrillStemMovementFeature a owl:Class; 
                               rdfs:comment """A drill-stem movement feature indicates that something accounts for the drill-stem movement.
"""@EN; 
                               rdfs:subClassOf ddhub:DrillingManagementFeature. 
ddhub:DrillStemRotationalMovementFeature a owl:Class; 
                                         rdfs:comment """A drill-stem rotational movement feature indicates that something accounts for drill-stem rotational movement.
"""@EN; 
                                         rdfs:subClassOf ddhub:DrillStemMovementFeature. 
ddhub:DrillstemTerminator a owl:Class; 
                          rdfs:comment ""@EN; 
                          rdfs:subClassOf ddhub:DrillingEquipment. 
ddhub:DrillStemTorsionalStickSlipFeature a owl:Class; 
                                         rdfs:comment """A drill-stem torsional stick-slip feature indicates that something acconts for in particular torsional stick-slip drill-stem vibrations.
"""@EN; 
                                         rdfs:subClassOf ddhub:DrillStemTorsionalVibrationFeature. 
ddhub:DrillStemTorsionalVibrationFeature a owl:Class; 
                                         rdfs:comment """A drill-stem torsional vibration feature indicates that something acconts for in particular torsional drill-stem vibrations.
"""@EN; 
                                         rdfs:subClassOf ddhub:DrillStemVibrationFeature. 
ddhub:DrillStemVibrationFeature a owl:Class; 
                                rdfs:comment """A drill-stem vibration feature indicates that something accounts for drill-stem vibrations.
"""@EN; 
                                rdfs:subClassOf ddhub:DrillStemMovementFeature. 
ddhub:DrillStemWhirlingFeature a owl:Class; 
                               rdfs:comment """A drill-stem whirling feature indicates that something accounts for in particular drill-stem whirling.
"""@EN; 
                               rdfs:subClassOf ddhub:DrillStemLateralVibrationFeature. 
ddhub:DrillSteRotationalImpedimentFeature a owl:Class; 
                                          rdfs:comment """A drill-stem rotational impediment feature indicates that something accounts for drill-stem rotational impediment.
"""@EN; 
                                          rdfs:subClassOf ddhub:StuckPipeFeature. 
ddhub:DrillString a owl:Class; 
                  rdfs:comment ""@EN; 
                  rdfs:subClassOf ddhub:Tubulars. 
ddhub:DrillStringCenterLineFrame a owl:Class; 
                                 rdfs:comment ""@EN; 
                                 rdfs:subClassOf ddhub:OneDimensionalCurviLinearReferenceFrame. 
ddhub:DrillStringDescription a owl:Class; 
                             rdfs:comment """A drill-string is a drill-stem that is used during a drilling operation. It is composed of drill-pipes, drill-collars,
BHA elements and is terminated either by a bit, a bull-nose, or other special elements such as fishing equipment, etc.
"""@EN; 
                             rdfs:subClassOf ddhub:DrillStemDescription. 
ddhub:DrillStringMagneticFluxDrillingQuantity a owl:Class; 
                                              rdfs:comment """Magnetic flux is the measure of the total magnetic field passing through a given area. It quantifies the strength and distribution of a magnetic field over a surface.
The dimension of magnetic flux is:
$$[L^{2}MI^{-1}T^{-2}]$$.
The SI unit for **magnetic flux** is: weber with the associated unit label $Wb$
The meaningful precision of magnetic flux in the drilling context is typically: 1E-07 Wb
"""@EN; 
                                              rdfs:subClassOf ddhub:MeasurableQuantity. 
ddhub:DrillWater a owl:Class; 
                 rdfs:comment ""@EN; 
                 rdfs:subClassOf ddhub:DrillingFluid. 
ddhub:DualActing a owl:Class; 
                 rdfs:comment ""@EN; 
                 rdfs:subClassOf ddhub:Action. 
ddhub:DurationDrillingQuantity a owl:Class; 
                               rdfs:comment """Time is a continuous, measurable progression in which events occur, from the past through the present to the future.
The dimension of time is:
$$[T]$$.
The SI unit for **time** is: second with the associated unit label $s$
The meaningful precision of time in the drilling context is typically: 0.001 s
"""@EN; 
                               rdfs:subClassOf ddhub:MeasurableQuantity. 
ddhub:DvwgCandle a owl:Class; 
                 rdfs:comment """[v] = a * [SI]
where
[v] is the value in DVWG candle
[SI] is the value in SI
a = 1.0/DVGWCandle, i.e., 0.9354186934071691
and
DVGWCandle = 1.162 * Hefnerkerze reference: https://fr.wikipedia.org/wiki/Bougie_(unit%C3%A9)
Hefnerkerze = 0.92 reference: https://en.wikipedia.org/wiki/Hefner_lamp
"""@EN; 
                 rdfs:subClassOf ddhub:Unit. 
ddhub:DWISADCSCapabilityDescriptor a owl:Class; 
                                   rdfs:comment ""@EN; 
                                   rdfs:subClassOf ddhub:DWISInternalService. 
ddhub:DWISADCSInterface a owl:Class; 
                        rdfs:comment ""@EN; 
                        rdfs:subClassOf ddhub:DWISInternalService. 
ddhub:DWISAdviceComposer a owl:Class; 
                         rdfs:comment ""@EN; 
                         rdfs:subClassOf ddhub:DWISInternalService. 
ddhub:DWISAttributeCardinalityRestriction a owl:Class, owl:Restriction; 
                                          owl:onClass ddhub:RunnableFunction, ddhub:Advisor, ddhub:BandPassFilter, ddhub:HighPassFilter, ddhub:LowPassFilter, ddhub:NumberOfSampleMovingAverage, ddhub:TimeWindowMovingAverage, ddhub:Buffering, ddhub:NumberOfItemsRangeExtraction, ddhub:TimeWindowRangeExtraction, ddhub:Resampling, ddhub:DataProvider, ddhub:OperatingCompany, ddhub:ServiceCompany, ddhub:DirectionalServiceCompany, ddhub:DrillingFluidProvider, ddhub:LoggingServiceCompany, ddhub:CementingServiceCompany, ddhub:CompletionServiceCompany, ddhub:DataAnalysisServiceCompany, ddhub:DrillingContractor, ddhub:DWISInternalService, ddhub:Telemetry, ddhub:DrillingDataPoint, ddhub:DrillingSignal, ddhub:DynamicDrillingSignal, ddhub:DataEndPoint, ddhub:WitsMLTimeBasedLogEndPoint, ddhub:EndPointMapping, ddhub:HydraulicConnectedState, ddhub:HydraulicJunction, ddhub:MeasurableQuantity, ddhub:MechanicalElementState, ddhub:OneDimensionalReferenceFrame, ddhub:Quantity, ddhub:Unit, ddhub:Clock, ddhub:SynchronizationGroup, ddhub:FullScaleUncertainty, ddhub:SensorUncertainty; 
                                          owl:onProperty ddhub:IsAuxiliary, ddhub:AdviceType, ddhub:MinFrequency, ddhub:MaxFrequency, ddhub:CutOffFrequency, ddhub:NumberOfSamples, ddhub:TimeWindow, ddhub:BufferingInterval, ddhub:NumberOfItems, ddhub:ResamplingRate, ddhub:ResamplingDelay, ddhub:Validity, ddhub:ProviderName, ddhub:NumberOfRepeaters, ddhub:DistanceBetweenRepeaters, ddhub:AverageDelayByRepeater, ddhub:IsValid, ddhub:Value, ddhub:TimeStampAtSource, ddhub:TimeStampAcquisition, ddhub:EndPointDescription, ddhub:WellUID, ddhub:WellName, ddhub:WellboreUID, ddhub:WellboreName, ddhub:LogUID, ddhub:LogName, ddhub:Mnemonic, ddhub:FixedIndices, ddhub:ValuesIndices, ddhub:MeasurementIndex, ddhub:LeftToRight, ddhub:RightToLeft, ddhub:MeaningfulPrecision, ddhub:PostiveUpward, ddhub:L, ddhub:M, ddhub:T, ddhub:I, ddhub:ThT, ddhub:N, ddhub:J, ddhub:Theta, ddhub:Omega, ddhub:SIUnit, ddhub:Symbol, ddhub:ConversionFactorA, ddhub:ConversionFactorB, ddhub:LeapSeconds, ddhub:Stratum, ddhub:NetworkSynchronizationLatencyAverage, ddhub:NetworkSynchronizationLatencyStandardDeviation, ddhub:Resolution, ddhub:MaximumFluctuations, ddhub:SynchronizationDelay, ddhub:SamplingRate, ddhub:FullScale, ddhub:ProportionError, ddhub:Accuracy, ddhub:Precision; 
                                          owl:qualifiedCardinality "1"^^xsd:nonNegativeInteger. 
ddhub:DWISBlackboard a owl:Class; 
                     rdfs:comment ""@EN; 
                     rdfs:subClassOf ddhub:DWISInternalService. 
ddhub:DWISContextualDataBuilder a owl:Class; 
                                rdfs:comment ""@EN; 
                                rdfs:subClassOf ddhub:DWISInternalService. 
ddhub:DWISDrillingProcessStateInterpreter a owl:Class; 
                                          rdfs:comment ""@EN; 
                                          rdfs:subClassOf ddhub:DWISInternalService. 
ddhub:DWISInternalService a owl:Class; 
                          rdfs:comment """A DWIS internal service is an internal component of the DWIS infrastructure that generates information that can be used by any systems connected to the DWIS infrastructure.
"""@EN; 
                          rdfs:subClassOf ddhub:DataProvider. 
ddhub:DWISLogger a owl:Class; 
                 rdfs:comment ""@EN; 
                 rdfs:subClassOf ddhub:DWISInternalService. 
ddhub:DWISNoun a owl:Class; 
               rdfs:comment """Nouns refer to the nature of a node in the graph. Implicitely a noun refers to a "is a" relation between the instance node and the noun. This is the root class for all the nouns defined in the DWIS vocabulary.
"""@EN. 
ddhub:DWISScheduler a owl:Class; 
                    rdfs:comment ""@EN; 
                    rdfs:subClassOf ddhub:DWISInternalService. 
ddhub:DWISVerb a owl:ObjectProperty; 
               rdfs:comment """This is the root class for all verbs defined in the DWIS vocabulary. It is used to define a relation between a subject, which can be of any `DWISNoun` and an object, also of any type of `DWISNoun`.
"""@EN; 
               rdfs:domain ddhub:DWISNoun; 
               rdfs:range ddhub:DWISNoun. 
ddhub:DWISVocabulary a owl:Ontology; 
                     rdfs:comment "This is the ontology generated by the D-WIS WG1: Semantics of Real-time signals. It has been automatically generated from the vocabulary defined at https://github.com/D-WIS/DDHub-Semantic-Interoperability/tree/main/docs/vocabulary_development/auto-generated"@EN; 
                     rdfs:isDefinedBy "D-WIS WG1: Semantics of Real-time signals"^^xsd:string; 
                     rdfs:label "D-WIS vocabulary"^^xsd:string; 
                     owl:versionInfo "0.1"^^xsd:string; 
                     owl:versionIRI "https://github.com/D-WIS/DDHub-Semantic-Interoperability/tree/main/docs/vocabulary_development/auto-generated/dwis.owl"^^xsd:anyURI. 
ddhub:Dynamic a owl:Class; 
              rdfs:comment ""@EN; 
              rdfs:subClassOf ddhub:BladeShape. 
ddhub:DynamicDrillingSignal a owl:Class; 
                            rdfs:comment ""@EN; 
                            rdfs:subClassOf ddhub:DrillingSignal. 
ddhub:DynamicViscosityDrillingQuantity a owl:Class; 
                                       rdfs:comment """Dynamic viscosity is a measure of a fluid's resistance to shear or flow when a force is applied. It quantifies how thick or thin the fluid is.
The dimension of dynamic viscosity is:
$$[ML^{-1}T^{-1}]$$.
The SI unit for **dynamic viscosity** is: pascal second with the associated unit label $Pa \\cdot s$
The meaningful precision of dynamic viscosity in the drilling context is typically: 0.0001 Pa•s
"""@EN; 
                                       rdfs:subClassOf ddhub:MeasurableQuantity. 
ddhub:DynamicViscosityQuantity a owl:Class; 
                               rdfs:comment """Dynamic viscosity is a measure of a fluid's resistance to shear or flow when a force is applied. It quantifies how thick or thin the fluid is.
The dimension of dynamic viscosity is:
$$[ML^{-1}T^{-1}]$$.
The SI unit for **dynamic viscosity** is: pascal second with the associated unit label $Pa \\cdot s$
"""@EN; 
                               rdfs:subClassOf ddhub:Quantity. 
ddhub:DynePerCentimetre a owl:Class; 
                        rdfs:comment """[v] = a * [SI]
where
[v] is the value in dyne per centimetre
[SI] is the value in SI
a = Centi/Dyne, i.e., 999.9999999999999
and
Centi = 0.01
Dyne = 1e-5 reference: https://en.wikipedia.org/wiki/Dyne
"""@EN; 
                        rdfs:subClassOf ddhub:Unit. 
ddhub:DynePerSquareCentimetre a owl:Class; 
                              rdfs:comment """[v] = a * [SI]
where
[v] is the value in dyne per square centimetre
[SI] is the value in SI
a = Centi*Centi/Dyne, i.e., 10
and
Centi = 0.01
Dyne = 1e-5 reference: https://en.wikipedia.org/wiki/Dyne
"""@EN; 
                              rdfs:subClassOf ddhub:Unit. 
ddhub:DynePerSquareCentimetrePerHour a owl:Class; 
                                     rdfs:comment """[v] = a * [SI]
where
[v] is the value in dyne per square centimetre per hour
[SI] is the value in SI
a = Hour*Centi*Centi/Dyne, i.e., 35999.99999999999
and
Hour = 60.0 * Minute
Centi = 0.01
Dyne = 1e-5 reference: https://en.wikipedia.org/wiki/Dyne
Minute = 60.0
"""@EN; 
                                     rdfs:subClassOf ddhub:Unit. 
ddhub:DynePerSquareCentimetrePerMinute a owl:Class; 
                                       rdfs:comment """[v] = a * [SI]
where
[v] is the value in dyne per square centimetre per minute
[SI] is the value in SI
a = Minute*Centi*Centi/Dyne, i.e., 600
and
Minute = 60.0
Centi = 0.01
Dyne = 1e-5 reference: https://en.wikipedia.org/wiki/Dyne
"""@EN; 
                                       rdfs:subClassOf ddhub:Unit. 
ddhub:DynePerSquareCentimetrePerSecond a owl:Class; 
                                       rdfs:comment """[v] = a * [SI]
where
[v] is the value in dyne per square centimetre per second
[SI] is the value in SI
a = Centi*Centi/Dyne, i.e., 10
and
Centi = 0.01
Dyne = 1e-5 reference: https://en.wikipedia.org/wiki/Dyne
"""@EN; 
                                       rdfs:subClassOf ddhub:Unit. 
ddhub:DyneSecondPerSquareCentimetre a owl:Class; 
                                    rdfs:comment """[v] = a * [SI]
where
[v] is the value in dyne second per square centimetre
[SI] is the value in SI
a = 1.0/Poise, i.e., 10
and
Poise = 0.1 reference: https://en.wikipedia.org/wiki/Poise_(unit)
"""@EN; 
                                    rdfs:subClassOf ddhub:Unit. 
ddhub:EarthMagneticFluxDensityQuantity a owl:Class; 
                                       rdfs:comment """Magnetic flux density is the measure of the strength of a magnetic field per unit area through which the magnetic flux passes. It indicates how concentrated the magnetic field is.
The dimension of magnetic flux density is:
$$[MI^{-1}T^{-2}]$$.
The SI unit for **magnetic flux density** is: tesla with the associated unit label $T$
Earth's magnetic flux density refers to the strength and direction of the Earth's magnetic field at a specific location.
The meaningful precision of earth magnetic flux density is: 1E-09 T
"""@EN; 
                                       rdfs:subClassOf ddhub:MeasurableQuantity. 
ddhub:EarthMass a owl:Class; 
                rdfs:comment """[v] = a * [SI]
where
[v] is the value in earth mass
[SI] is the value in SI
a = 1.0/EarthMass, i.e., 1.6744248350691536E-25
and
EarthMass = 5.9722e24 reference: https://en.wikipedia.org/wiki/Earth_mass
"""@EN; 
                rdfs:subClassOf ddhub:Unit. 
ddhub:ElasticModulusQuantity a owl:Class; 
                             rdfs:comment """Pressure is the force applied per unit area on a surface.
The dimension of pressure is:
$$[ML^{-1}T^{-2}]$$.
The SI unit for **pressure** is: pascal with the associated unit label $Pa$
Elastic modulus is a measure of a material's ability to resist deformation under stress. It quantifies the ratio of stress to strain in the material's elastic region
The meaningful precision of an elastic modulus is typically: 10000 Pa
"""@EN; 
                             rdfs:subClassOf ddhub:MeasurableQuantity. 
ddhub:ElectricalControlSystem a owl:Class; 
                              rdfs:comment ""@EN; 
                              rdfs:subClassOf ddhub:PowerGenerationSystem. 
ddhub:ElectricCapacitanceQuantity a owl:Class; 
                                  rdfs:comment """lectric capacitance is the ability of a capacitor or a component to store electrical charge per unit voltage applied across it.
The dimension of electric capacitance is:
$$[T^{4}I^{2}M^{-1}L^{-2}]$$.
The SI unit for **electric capacitance** is: farad with the associated unit label $F$
"""@EN; 
                                  rdfs:subClassOf ddhub:Quantity. 
ddhub:ElectricCurrentQuantity a owl:Class; 
                              rdfs:comment """Electric current is the flow of electric charge through a conductor or circuit.
The dimension of electric current is:
$$[I]$$.
The SI unit for **electric current** is: ampere with the associated unit label $A$
"""@EN; 
                              rdfs:subClassOf ddhub:Quantity. 
ddhub:ElectricResistivityQuantity a owl:Class; 
                                  rdfs:comment """Electric resistivity is a material's inherent property that measures how strongly it resists the flow of electric current.
The dimension of resistivity is:
$$[L^{3}MI^{-2}T^{-3}]$$.
The SI unit for **electric resistivity** is: ohm metre with the associated unit label $\\Omega \\cdot m$
"""@EN; 
                                  rdfs:subClassOf ddhub:Quantity. 
ddhub:ElectricTensionQuantity a owl:Class; 
                              rdfs:comment """Electric tension is the difference in electric potential between two points.In a static electric field, it corresponds to the work needed per unit of charge to move a positive test charge from the first point to the second point.
The dimension of electric tension is:
$$[L^{2}MI^{-1}T^{-3}]$$.
The SI unit for **electric tension** is: volt with the associated unit label $V$
"""@EN; 
                              rdfs:subClassOf ddhub:MeasurableQuantity. 
ddhub:Electromagnetic a owl:Class; 
                      rdfs:comment ""@EN; 
                      rdfs:subClassOf ddhub:EquipmentTelemetry. 
ddhub:ElectromagneticCouplingDownholeTelemetry a owl:Class; 
                                               rdfs:comment """A method that allows transfer of downhole data to the surface via electromagnetic coupling between pipes along the drill-string.
"""@EN; 
                                               rdfs:subClassOf ddhub:WiredPipeTelemetry. 
ddhub:ElectromagneticTelemetry a owl:Class; 
                               rdfs:comment """A method that allows transfer of downhole data to the surface via electromagnetic waves sent through the drilling formation.
"""@EN; 
                               rdfs:subClassOf ddhub:DownHoleTelemetry. 
ddhub:ElevatorBailsLinks a owl:Class; 
                         rdfs:comment ""@EN; 
                         rdfs:subClassOf ddhub:DrillFloorEquipment. 
ddhub:ElongationGradientPerLengthDrillingQuantity a owl:Class; 
                                                  rdfs:comment """An elongation gradient per length is the first derivative of an elongation compared to a distance: $\\frac{d\\epsilon}{ds}$, where $\\epsilon$ is an elongation and $s$ is a distance.
It is dimensionless.
The SI unit for **elongation gradient per length** is: metre per metre with the associated unit label $\\frac{m}{m}$
The meaningful precision of elongation gradient per length in the drilling context is typically: 1E-05 m/m
"""@EN; 
                                                  rdfs:subClassOf ddhub:MeasurableQuantity. 
ddhub:ElongationGradientPerLengthQuantity a owl:Class; 
                                          rdfs:comment """An elongation gradient per length is the first derivative of an elongation compared to a distance: $\\frac{d\\epsilon}{ds}$, where $\\epsilon$ is an elongation and $s$ is a distance.
It is dimensionless.
The SI unit for **elongation gradient per length** is: metre per metre with the associated unit label $\\frac{m}{m}$
"""@EN; 
                                          rdfs:subClassOf ddhub:Quantity. 
ddhub:EmpiricalModel a owl:Class; 
                     rdfs:comment """A model that heavily rely on data without using explicitly physical laws.
"""@EN; 
                     rdfs:subClassOf ddhub:ModelingParadigm. 
ddhub:EnablementState a owl:Class; 
                      rdfs:comment ""@EN; 
                      rdfs:subClassOf ddhub:ProceduralState. 
ddhub:EndPointDescription a owl:DatatypeProperty, owl:FunctionalProperty; 
                          rdfs:comment """
"""@EN; 
                          rdfs:domain ddhub:DataEndPoint; 
                          rdfs:range xsd:string. 
ddhub:EndPointMapping a owl:Class; 
                      rdfs:comment ""@EN; 
                      rdfs:subClassOf ddhub:DWISNoun. 
ddhub:EndsHydraulicBranchDecomposition a owl:ObjectProperty; 
                                       rdfs:comment ""@EN; 
                                       rdfs:domain ddhub:HydraulicBranch; 
                                       rdfs:range ddhub:HydraulicBranch; 
                                       rdfs:subPropertyOf ddhub:DWISVerb. 
ddhub:EnergyDensityDrillingQuantity a owl:Class; 
                                    rdfs:comment """Energy density is the amount of energy stored per unit volume or mass of a substance or system.
The dimension of energy density is:
$$[ML^{-1}T^{-2}]$$.
The SI unit for **energy density** is: joule per cubic metre with the associated unit label $\\frac{J}{m^{3}}$
The meaningful precision of energy density in the drilling context is typically: 0.01 J/m³
"""@EN; 
                                    rdfs:subClassOf ddhub:MeasurableQuantity. 
ddhub:EnergyDensityQuantity a owl:Class; 
                            rdfs:comment """Energy density is the amount of energy stored per unit volume or mass of a substance or system.
The dimension of energy density is:
$$[ML^{-1}T^{-2}]$$.
The SI unit for **energy density** is: joule per cubic metre with the associated unit label $\\frac{J}{m^{3}}$
"""@EN; 
                            rdfs:subClassOf ddhub:Quantity. 
ddhub:EnergyQuantity a owl:Class; 
                     rdfs:comment """Energy is the quantitative property that is transferred to a body or to a physical system, recognizable in the performance of work and in the form of heat and light. Energy is a conserved quantity—the law of conservation of energy states that energy can be converted in form, but not created or destroyed; matter and energy may also be converted to one another.
The dimension of energy is:
$$[L^{2}MT^{-2}]$$.
The SI unit for **energy** is: joule with the associated unit label $J$
"""@EN; 
                     rdfs:subClassOf ddhub:Quantity. 
ddhub:EnumerationDataType a owl:Class; 
                          rdfs:comment ""@EN; 
                          rdfs:subClassOf ddhub:DiscreteDataType. 
ddhub:EQ a owl:Class; 
         rdfs:comment ""@EN; 
         rdfs:subClassOf ddhub:ValidityCondition. 
ddhub:Equipment a owl:Class; 
                rdfs:comment ""@EN; 
                rdfs:subClassOf ddhub:DWISNoun. 
ddhub:EquipmentTelemetry a owl:Class; 
                         rdfs:comment ""@EN; 
                         rdfs:subClassOf ddhub:LoggingEquipment. 
ddhub:Exawatt a owl:Class; 
              rdfs:comment """[v] = a * [SI]
where
[v] is the value in exawatt
[SI] is the value in SI
a = 1.0/Exa, i.e., 1E-18
and
Exa = 1e18
"""@EN; 
              rdfs:subClassOf ddhub:Unit. 
ddhub:ExpandableReamers a owl:Class; 
                        rdfs:comment ""@EN; 
                        rdfs:subClassOf ddhub:Reamers. 
ddhub:Expandables a owl:Class; 
                  rdfs:comment ""@EN; 
                  rdfs:subClassOf ddhub:Tubulars. 
ddhub:ExtendFrame a owl:Class; 
                  rdfs:comment ""@EN; 
                  rdfs:subClassOf ddhub:TopDrive. 
ddhub:Extrapolated a owl:Class; 
                   rdfs:comment """Extrapolated characterizes that the wellbore data is being partially measured/observed and also extended to
positions that have not been measured/observed yet.
"""@EN; 
                   rdfs:subClassOf ddhub:WellBoreDataCharateristic. 
ddhub:Fahrenheit a owl:Class; 
                 rdfs:comment """[v] = a * [SI] + b
where
[v] is the value in fahrenheit
[SI] is the value in SI
a = 1.0/FahrenheitSlope, i.e., 1.7999999999999998
b = -FahrenheitBias, i.e., -459.67
and
FahrenheitSlope = 5.0 / 9.0 reference: https://nn.wikipedia.org/wiki/Fahrenheit
FahrenheitBias = 459.67 reference: https://nn.wikipedia.org/wiki/Fahrenheit
"""@EN; 
                 rdfs:subClassOf ddhub:Unit. 
ddhub:FahrenheitPer100Foot a owl:Class; 
                           rdfs:comment """[v] = a * [SI]
where
[v] is the value in fahrenheit per 100 foot
[SI] is the value in SI
a = 100.0*Foot/FahrenheitSlope, i.e., 54.86399999999999
and
Foot = 12.0 * Inch
FahrenheitSlope = 5.0 / 9.0 reference: https://nn.wikipedia.org/wiki/Fahrenheit
Inch = 0.0254 reference: https://www.nist.gov/pml/owm/si-units-length
"""@EN; 
                           rdfs:subClassOf ddhub:Unit. 
ddhub:FahrenheitPer30Foot a owl:Class; 
                          rdfs:comment """[v] = a * [SI]
where
[v] is the value in fahrenheit per 30 foot
[SI] is the value in SI
a = 30.0*Foot/FahrenheitSlope, i.e., 16.459199999999996
and
Foot = 12.0 * Inch
FahrenheitSlope = 5.0 / 9.0 reference: https://nn.wikipedia.org/wiki/Fahrenheit
Inch = 0.0254 reference: https://www.nist.gov/pml/owm/si-units-length
"""@EN; 
                          rdfs:subClassOf ddhub:Unit. 
ddhub:FahrenheitPerFoot a owl:Class; 
                        rdfs:comment """[v] = a * [SI]
where
[v] is the value in fahrenheit per foot
[SI] is the value in SI
a = Foot/FahrenheitSlope, i.e., 0.5486399999999999
and
Foot = 12.0 * Inch
FahrenheitSlope = 5.0 / 9.0 reference: https://nn.wikipedia.org/wiki/Fahrenheit
Inch = 0.0254 reference: https://www.nist.gov/pml/owm/si-units-length
"""@EN; 
                        rdfs:subClassOf ddhub:Unit. 
ddhub:Farad a owl:Class; 
            rdfs:comment """No conversion necessary as the unit choice is SI
"""@EN; 
            rdfs:subClassOf ddhub:Unit. 
ddhub:Fathom a owl:Class; 
             rdfs:comment """[v] = a * [SI]
where
[v] is the value in fathom
[SI] is the value in SI
a = 1.0/Fathom, i.e., 0.546806649168854
and
Fathom = 6.0 * Foot reference: https://www.britannica.com/science/fathom
Foot = 12.0 * Inch
Inch = 0.0254 reference: https://www.nist.gov/pml/owm/si-units-length
"""@EN; 
             rdfs:subClassOf ddhub:Unit. 
ddhub:FDIRFunction a owl:Class; 
                   rdfs:comment """A `FDIRFunction` is a `ProtectionFunction` that reacts to a particular state of the drilling process. FDIR
stands for Fault Detection, Isolation and Recovery. An FDIR protects the drilling process by looking at its outputs.
When that state is detected, then an isolation procedure is run, and if successful and defined, a recovery procedure is
thereafter executed. In case of success of the recovery procedure, the drilling process is resumed. In all other cases,
the system returns in manual mode, usually using the safe mode management procedure. An example of `FDIRFunction` is an
packoff detection and reaction procedure.
"""@EN; 
                   rdfs:subClassOf ddhub:ProtectionFunction. 
ddhub:FeatureLevelIntegationModel a owl:Class; 
                                  rdfs:comment """A model that integrates data at a medium-level like using feature extraction and merging, reducing dimensionality,
weighting features, or correlating features.
"""@EN; 
                                  rdfs:subClassOf ddhub:DataIntegrationStrategy. 
ddhub:Femtowatt a owl:Class; 
                rdfs:comment """[v] = a * [SI]
where
[v] is the value in femtowatt
[SI] is the value in SI
a = 1.0/Femto, i.e., 999999999999999.9
and
Femto = 1e-15
"""@EN; 
                rdfs:subClassOf ddhub:Unit. 
ddhub:FillPump a owl:Class; 
               rdfs:comment ""@EN; 
               rdfs:subClassOf ddhub:CirculationSystem. 
ddhub:Filter a owl:Class; 
             rdfs:comment ""@EN; 
             rdfs:subClassOf ddhub:SignalProcessingUnit. 
ddhub:FireSafetySystems a owl:Class; 
                        rdfs:comment ""@EN; 
                        rdfs:subClassOf ddhub:SafetyEquipment. 
ddhub:FishingTools a owl:Class; 
                   rdfs:comment ""@EN; 
                   rdfs:subClassOf ddhub:DrillingEquipment. 
ddhub:FixedBlade a owl:Class; 
                 rdfs:comment ""@EN; 
                 rdfs:subClassOf ddhub:HoleOpener. 
ddhub:FixedBladeReamers a owl:Class; 
                        rdfs:comment ""@EN; 
                        rdfs:subClassOf ddhub:Reamers. 
ddhub:FixedCutter a owl:Class; 
                  rdfs:comment ""@EN; 
                  rdfs:subClassOf ddhub:DrillingBit. 
ddhub:FixedIndices a owl:DatatypeProperty, owl:FunctionalProperty; 
                   rdfs:comment """
"""@EN; 
                   rdfs:domain ddhub:EndPointMapping; 
                   rdfs:range <http://www.w3.org/2001/XMLSchema#int[]>. 
ddhub:Flange a owl:Class; 
             rdfs:comment ""@EN; 
             rdfs:subClassOf ddhub:Connection. 
ddhub:FlapperFloatValvesG a owl:Class; 
                          rdfs:comment ""@EN; 
                          rdfs:subClassOf ddhub:FloatValveNonreturnValve. 
ddhub:FloatCollar a owl:Class; 
                  rdfs:comment ""@EN; 
                  rdfs:subClassOf ddhub:CasingEquipment. 
ddhub:FloatShoe a owl:Class; 
                rdfs:comment ""@EN; 
                rdfs:subClassOf ddhub:CasingEquipment. 
ddhub:FloatValveNonreturnValve a owl:Class; 
                               rdfs:comment ""@EN; 
                               rdfs:subClassOf ddhub:WellControlSystem. 
ddhub:FlowAnalysisEquipment a owl:Class; 
                            rdfs:comment ""@EN; 
                            rdfs:subClassOf ddhub:MudLoggingEquipment. 
ddhub:FlowCheckProcedure a owl:Class; 
                         rdfs:comment """The flow-check procedure is used to check the well is stable (no influx of formation fluids) while ensuring that the
drill-stem will not get stuck during the test.
"""@EN; 
                         rdfs:subClassOf ddhub:DrillingProcedure. 
ddhub:FlowLine a owl:Class; 
               rdfs:comment ""@EN; 
               rdfs:subClassOf ddhub:MudLines. 
ddhub:FlowmeterTools a owl:Class; 
                     rdfs:comment ""@EN; 
                     rdfs:subClassOf ddhub:WirelineLoggingTools. 
ddhub:FlowRateIn a owl:Class; 
                 rdfs:comment ""@EN; 
                 rdfs:subClassOf ddhub:PrototypeData. 
ddhub:FlowrateLimit a owl:Class; 
                    rdfs:comment """This Noun is used to refer to a flowrate limit.
"""@EN; 
                    rdfs:subClassOf ddhub:DrillingLimit. 
ddhub:FlowRateOut a owl:Class; 
                  rdfs:comment ""@EN; 
                  rdfs:subClassOf ddhub:PrototypeData. 
ddhub:FluidComponent a owl:Class; 
                     rdfs:comment ""@EN; 
                     rdfs:subClassOf ddhub:DWISNoun. 
ddhub:FluidDensityTools a owl:Class; 
                        rdfs:comment ""@EN; 
                        rdfs:subClassOf ddhub:WirelineLoggingTools. 
ddhub:FluidDescription a owl:Class; 
                       rdfs:comment """Drilling fluid contains information about the density, rheological behavior, thermo-physical and chemical characteristics of a fluid
used during a drilling operation.
"""@EN; 
                       rdfs:subClassOf ddhub:WellBoreData. 
ddhub:FluidShearRateQuantity a owl:Class; 
                             rdfs:comment """Frequency is the number of occurrences of a repeating event per unit of time.
The dimension of frequency is:
$$[T^{-1}]$$.
The SI unit for **frequency** is: hertz with the associated unit label $Hz$
Shear rate in a fluid is the rate at which adjacent layers of the fluid move relative to each other, typically expressed as the change in velocity per unit distance between the layers. It measures how quickly the fluid is being deformed by shear stress.
The meaningful precision of a shear rate for a fluid is typically: 0.01 Hz
"""@EN; 
                             rdfs:subClassOf ddhub:MeasurableQuantity. 
ddhub:FluidShearStressQuantity a owl:Class; 
                               rdfs:comment """Pressure is the force applied per unit area on a surface.
The dimension of pressure is:
$$[ML^{-1}T^{-2}]$$.
The SI unit for **pressure** is: pascal with the associated unit label $Pa$
Shear stress in a fluid is the force per unit area exerted parallel to the fluid's surface, causing layers of the fluid to slide relative to each other. It measures the fluid's resistance to this shearing action.
The meaningful precision of a shear stress for a fluid is typically: 0.0001 Pa
"""@EN; 
                               rdfs:subClassOf ddhub:MeasurableQuantity. 
ddhub:FluidVelocityDrillingQuantity a owl:Class; 
                                    rdfs:comment """A velocity is the time derivative of a position or a displacement: $\\frac{dx}{dt}$, where $x$ is a position and $t$ is time.
The dimension of velocity is:
$$[LT^{-1}]$$.
The SI unit for **velocity** is: metre per second with the associated unit label $\\frac{m}{s}$
The meaningful precision of fluid velocity in the drilling context is typically: 0.01 m/s
"""@EN; 
                                    rdfs:subClassOf ddhub:MeasurableQuantity. 
ddhub:Foot a owl:Class; 
           rdfs:comment """[v] = a * [SI]
where
[v] is the value in foot
[SI] is the value in SI
a = 1.0/Foot, i.e., 3.280839895013124
and
Foot = 12.0 * Inch
Inch = 0.0254 reference: https://www.nist.gov/pml/owm/si-units-length
"""@EN; 
           rdfs:subClassOf ddhub:Unit. 
ddhub:FootPerDay a owl:Class; 
                 rdfs:comment """[v] = a * [SI]
where
[v] is the value in foot per day
[SI] is the value in SI
a = Day/Foot, i.e., 283464.5669291339
and
Day = 24.0 * Hour
Foot = 12.0 * Inch
Hour = 60.0 * Minute
Inch = 0.0254 reference: https://www.nist.gov/pml/owm/si-units-length
Minute = 60.0
"""@EN; 
                 rdfs:subClassOf ddhub:Unit. 
ddhub:FootPerFoot a owl:Class; 
                  rdfs:comment """[v] = a * [SI]
where
[v] is the value in foot per foot
[SI] is the value in SI
a = Foot / Foot, i.e., 1
and
Foot = 12.0 * Inch
Inch = 0.0254 reference: https://www.nist.gov/pml/owm/si-units-length
"""@EN; 
                  rdfs:subClassOf ddhub:Unit. 
ddhub:FootPerHour a owl:Class; 
                  rdfs:comment """[v] = a * [SI]
where
[v] is the value in foot per hour
[SI] is the value in SI
a = Hour/Foot, i.e., 11811.023622047245
and
Hour = 60.0 * Minute
Foot = 12.0 * Inch
Minute = 60.0
Inch = 0.0254 reference: https://www.nist.gov/pml/owm/si-units-length
"""@EN; 
                  rdfs:subClassOf ddhub:Unit. 
ddhub:FootPerHourPerSecond a owl:Class; 
                           rdfs:comment """[v] = a * [SI]
where
[v] is the value in foot per hour per second
[SI] is the value in SI
a = Hour/Foot, i.e., 11811.023622047245
and
Hour = 60.0 * Minute
Foot = 12.0 * Inch
Minute = 60.0
Inch = 0.0254 reference: https://www.nist.gov/pml/owm/si-units-length
"""@EN; 
                           rdfs:subClassOf ddhub:Unit. 
ddhub:FootPerMile a owl:Class; 
                  rdfs:comment """[v] = a * [SI]
where
[v] is the value in foot per mile
[SI] is the value in SI
a = Mile / Foot, i.e., 5280
and
Mile = 1760.0 * Yard reference: https://dictionary.cambridge.org/dictionary/english/mile
Foot = 12.0 * Inch
Yard = 3.0 * Foot
Inch = 0.0254 reference: https://www.nist.gov/pml/owm/si-units-length
"""@EN; 
                  rdfs:subClassOf ddhub:Unit. 
ddhub:FootPerMinute a owl:Class; 
                    rdfs:comment """[v] = a * [SI]
where
[v] is the value in foot per minute
[SI] is the value in SI
a = Minute/Foot, i.e., 196.85039370078744
and
Minute = 60.0
Foot = 12.0 * Inch
Inch = 0.0254 reference: https://www.nist.gov/pml/owm/si-units-length
"""@EN; 
                    rdfs:subClassOf ddhub:Unit. 
ddhub:FootPerMinutePerSecond a owl:Class; 
                             rdfs:comment """[v] = a * [SI]
where
[v] is the value in foot per minute per second
[SI] is the value in SI
a = Minute/Foot, i.e., 196.85039370078744
and
Minute = 60.0
Foot = 12.0 * Inch
Inch = 0.0254 reference: https://www.nist.gov/pml/owm/si-units-length
"""@EN; 
                             rdfs:subClassOf ddhub:Unit. 
ddhub:FootPerSecond a owl:Class; 
                    rdfs:comment """[v] = a * [SI]
where
[v] is the value in foot per second
[SI] is the value in SI
a = Unit/Foot, i.e., 3.280839895013124
and
Unit = 1.0
Foot = 12.0 * Inch
Inch = 0.0254 reference: https://www.nist.gov/pml/owm/si-units-length
"""@EN; 
                    rdfs:subClassOf ddhub:Unit. 
ddhub:FootPerSecondSquared a owl:Class; 
                           rdfs:comment """[v] = a * [SI]
where
[v] is the value in foot per second squared
[SI] is the value in SI
a = 1.0/Foot, i.e., 3.280839895013124
and
Foot = 12.0 * Inch
Inch = 0.0254 reference: https://www.nist.gov/pml/owm/si-units-length
"""@EN; 
                           rdfs:subClassOf ddhub:Unit. 
ddhub:FootPerYard a owl:Class; 
                  rdfs:comment """[v] = a * [SI]
where
[v] is the value in foot per yard
[SI] is the value in SI
a = Yard / Foot, i.e., 3
and
Yard = 3.0 * Foot
Foot = 12.0 * Inch
Inch = 0.0254 reference: https://www.nist.gov/pml/owm/si-units-length
"""@EN; 
                  rdfs:subClassOf ddhub:Unit. 
ddhub:FootPound a owl:Class; 
                rdfs:comment """[v] = a * [SI]
where
[v] is the value in foot pound
[SI] is the value in SI
a = 1.0/(Foot*PoundForce), i.e., 0.7375621492772655
and
Foot = 12.0 * Inch
PoundForce = Pound * G reference: https://en.wikipedia.org/wiki/Pound_(force)
Inch = 0.0254 reference: https://www.nist.gov/pml/owm/si-units-length
Pound = 0.45359237 reference: https://en.wikipedia.org/wiki/Pound_(mass)
G = 9.80665 reference: https://en.wikipedia.org/wiki/Gravity_of_Earth
"""@EN; 
                rdfs:subClassOf ddhub:Unit. 
ddhub:FootPoundPerCentimetre a owl:Class; 
                             rdfs:comment """[v] = a * [SI]
where
[v] is the value in foot pound per centimetre
[SI] is the value in SI
a = Centi/(Foot*PoundForce), i.e., 0.007375621492772655
and
Centi = 0.01
Foot = 12.0 * Inch
PoundForce = Pound * G reference: https://en.wikipedia.org/wiki/Pound_(force)
Inch = 0.0254 reference: https://www.nist.gov/pml/owm/si-units-length
Pound = 0.45359237 reference: https://en.wikipedia.org/wiki/Pound_(mass)
G = 9.80665 reference: https://en.wikipedia.org/wiki/Gravity_of_Earth
"""@EN; 
                             rdfs:subClassOf ddhub:Unit. 
ddhub:FootPoundPerDecimetre a owl:Class; 
                            rdfs:comment """[v] = a * [SI]
where
[v] is the value in foot pound per decimetre
[SI] is the value in SI
a = Deci/(Foot*PoundForce), i.e., 0.07375621492772655
and
Deci = 0.1
Foot = 12.0 * Inch
PoundForce = Pound * G reference: https://en.wikipedia.org/wiki/Pound_(force)
Inch = 0.0254 reference: https://www.nist.gov/pml/owm/si-units-length
Pound = 0.45359237 reference: https://en.wikipedia.org/wiki/Pound_(mass)
G = 9.80665 reference: https://en.wikipedia.org/wiki/Gravity_of_Earth
"""@EN; 
                            rdfs:subClassOf ddhub:Unit. 
ddhub:FootPoundPerFoot a owl:Class; 
                       rdfs:comment """[v] = a * [SI]
where
[v] is the value in foot pound per foot
[SI] is the value in SI
a = Foot/(Foot*PoundForce), i.e., 0.2248089430997105
and
Foot = 12.0 * Inch
PoundForce = Pound * G reference: https://en.wikipedia.org/wiki/Pound_(force)
Inch = 0.0254 reference: https://www.nist.gov/pml/owm/si-units-length
Pound = 0.45359237 reference: https://en.wikipedia.org/wiki/Pound_(mass)
G = 9.80665 reference: https://en.wikipedia.org/wiki/Gravity_of_Earth
"""@EN; 
                       rdfs:subClassOf ddhub:Unit. 
ddhub:FootPoundPerHour a owl:Class; 
                       rdfs:comment """[v] = a * [SI]
where
[v] is the value in foot pound per hour
[SI] is the value in SI
a = Hour/(Foot*PoundForce), i.e., 2655.2237373981557
and
Hour = 60.0 * Minute
Foot = 12.0 * Inch
PoundForce = Pound * G reference: https://en.wikipedia.org/wiki/Pound_(force)
Minute = 60.0
Inch = 0.0254 reference: https://www.nist.gov/pml/owm/si-units-length
Pound = 0.45359237 reference: https://en.wikipedia.org/wiki/Pound_(mass)
G = 9.80665 reference: https://en.wikipedia.org/wiki/Gravity_of_Earth
"""@EN; 
                       rdfs:subClassOf ddhub:Unit. 
ddhub:FootPoundPerInch a owl:Class; 
                       rdfs:comment """[v] = a * [SI]
where
[v] is the value in foot pound per inch
[SI] is the value in SI
a = Inch/(Foot*PoundForce), i.e., 0.018734078591642542
and
Inch = 0.0254 reference: https://www.nist.gov/pml/owm/si-units-length
Foot = 12.0 * Inch
PoundForce = Pound * G reference: https://en.wikipedia.org/wiki/Pound_(force)
Pound = 0.45359237 reference: https://en.wikipedia.org/wiki/Pound_(mass)
G = 9.80665 reference: https://en.wikipedia.org/wiki/Gravity_of_Earth
"""@EN; 
                       rdfs:subClassOf ddhub:Unit. 
ddhub:FootPoundPerMetre a owl:Class; 
                        rdfs:comment """[v] = a * [SI]
where
[v] is the value in foot pound per metre
[SI] is the value in SI
a = Unit/(PoundForce*Foot), i.e., 0.7375621492772655
and
Unit = 1.0
PoundForce = Pound * G reference: https://en.wikipedia.org/wiki/Pound_(force)
Foot = 12.0 * Inch
Pound = 0.45359237 reference: https://en.wikipedia.org/wiki/Pound_(mass)
G = 9.80665 reference: https://en.wikipedia.org/wiki/Gravity_of_Earth
Inch = 0.0254 reference: https://www.nist.gov/pml/owm/si-units-length
"""@EN; 
                        rdfs:subClassOf ddhub:Unit. 
ddhub:FootPoundPerMillimetre a owl:Class; 
                             rdfs:comment """[v] = a * [SI]
where
[v] is the value in foot pound per millimetre
[SI] is the value in SI
a = Milli/(Foot*PoundForce), i.e., 0.0007375621492772656
and
Milli = 0.001
Foot = 12.0 * Inch
PoundForce = Pound * G reference: https://en.wikipedia.org/wiki/Pound_(force)
Inch = 0.0254 reference: https://www.nist.gov/pml/owm/si-units-length
Pound = 0.45359237 reference: https://en.wikipedia.org/wiki/Pound_(mass)
G = 9.80665 reference: https://en.wikipedia.org/wiki/Gravity_of_Earth
"""@EN; 
                             rdfs:subClassOf ddhub:Unit. 
ddhub:FootPoundPerMinute a owl:Class; 
                         rdfs:comment """[v] = a * [SI]
where
[v] is the value in foot pound per minute
[SI] is the value in SI
a = Minute/(Foot*PoundForce), i.e., 44.25372895663593
and
Minute = 60.0
Foot = 12.0 * Inch
PoundForce = Pound * G reference: https://en.wikipedia.org/wiki/Pound_(force)
Inch = 0.0254 reference: https://www.nist.gov/pml/owm/si-units-length
Pound = 0.45359237 reference: https://en.wikipedia.org/wiki/Pound_(mass)
G = 9.80665 reference: https://en.wikipedia.org/wiki/Gravity_of_Earth
"""@EN; 
                         rdfs:subClassOf ddhub:Unit. 
ddhub:FootPoundPerSecond a owl:Class; 
                         rdfs:comment """[v] = a * [SI]
where
[v] is the value in foot pound per second
[SI] is the value in SI
a = 1.0/(Foot*PoundForce), i.e., 0.7375621492772655
and
Foot = 12.0 * Inch
PoundForce = Pound * G reference: https://en.wikipedia.org/wiki/Pound_(force)
Inch = 0.0254 reference: https://www.nist.gov/pml/owm/si-units-length
Pound = 0.45359237 reference: https://en.wikipedia.org/wiki/Pound_(mass)
G = 9.80665 reference: https://en.wikipedia.org/wiki/Gravity_of_Earth
"""@EN; 
                         rdfs:subClassOf ddhub:Unit. 
ddhub:FootWaterAt4DegreeCelsius a owl:Class; 
                                rdfs:comment """[v] = a * [SI]
where
[v] is the value in foot water at 4 degree celsius
[SI] is the value in SI
a = 1.0/FootWater4degC, i.e., 0.0003345525543589354
and
FootWater4degC = 2989.067 reference: https://en.wikipedia.org/wiki/Inch_of_water
"""@EN; 
                                rdfs:subClassOf ddhub:Unit. 
ddhub:FootWaterAt4DegreeCelsiusPerHour a owl:Class; 
                                       rdfs:comment """[v] = a * [SI]
where
[v] is the value in foot water at 4 degree celsius per hour
[SI] is the value in SI
a = Hour/FootWater4degC, i.e., 1.2043891956921675
and
Hour = 60.0 * Minute
FootWater4degC = 2989.067 reference: https://en.wikipedia.org/wiki/Inch_of_water
Minute = 60.0
"""@EN; 
                                       rdfs:subClassOf ddhub:Unit. 
ddhub:FootWaterAt4DegreeCelsiusPerMinute a owl:Class; 
                                         rdfs:comment """[v] = a * [SI]
where
[v] is the value in foot water at 4 degree celsius per minute
[SI] is the value in SI
a = Minute/FootWater4degC, i.e., 0.020073153261536126
and
Minute = 60.0
FootWater4degC = 2989.067 reference: https://en.wikipedia.org/wiki/Inch_of_water
"""@EN; 
                                         rdfs:subClassOf ddhub:Unit. 
ddhub:FootWaterAt4DegreeCelsiusPerSecond a owl:Class; 
                                         rdfs:comment """[v] = a * [SI]
where
[v] is the value in foot water at 4 degree celsius per second
[SI] is the value in SI
a = 1.0/FootWater4degC, i.e., 0.0003345525543589354
and
FootWater4degC = 2989.067 reference: https://en.wikipedia.org/wiki/Inch_of_water
"""@EN; 
                                         rdfs:subClassOf ddhub:Unit. 
ddhub:ForceDrillingQuantity a owl:Class; 
                            rdfs:comment """A force is an influence that can cause an object to change its velocity unless counterbalanced by other forces.
The dimension of force is:
$$[LMT^{-2}]$$.
The SI unit for **force** is: newton with the associated unit label $N$
The meaningful precision of force in the drilling context is typically: 0.1 N
"""@EN; 
                            rdfs:subClassOf ddhub:MeasurableQuantity. 
ddhub:ForceFromLoadPinsTransformation a owl:Class; 
                                      rdfs:comment ""@EN; 
                                      rdfs:subClassOf ddhub:DirectTransformation. 
ddhub:ForceGradientPerLengthDrillingQuantity a owl:Class; 
                                             rdfs:comment """A force gradient per length is the first derivative compared to a distance of a force: $\\frac{dF}{ds}$ where $F$ is a force and $s$ is a distance.
The dimension of force gradient per length is:
$$[MT^{-2}]$$.
The SI unit for **force gradient per length** is: newton per metre with the associated unit label $\\frac{N}{m}$
The meaningful precision of force gradient per length in the drilling context is typically: 1 N/m
"""@EN; 
                                             rdfs:subClassOf ddhub:MeasurableQuantity. 
ddhub:ForceGradientPerLengthQuantity a owl:Class; 
                                     rdfs:comment """A force gradient per length is the first derivative compared to a distance of a force: $\\frac{dF}{ds}$ where $F$ is a force and $s$ is a distance.
The dimension of force gradient per length is:
$$[MT^{-2}]$$.
The SI unit for **force gradient per length** is: newton per metre with the associated unit label $\\frac{N}{m}$
"""@EN; 
                                     rdfs:subClassOf ddhub:Quantity. 
ddhub:ForceQuantity a owl:Class; 
                    rdfs:comment """A force is an influence that can cause an object to change its velocity unless counterbalanced by other forces.
The dimension of force is:
$$[LMT^{-2}]$$.
The SI unit for **force** is: newton with the associated unit label $N$
"""@EN; 
                    rdfs:subClassOf ddhub:Quantity. 
ddhub:ForceRateOfChangeDrillingQuantity a owl:Class; 
                                        rdfs:comment """A force rate of change is the time derivative of a force: $\\frac{dF}{dt}$, where $F$ is the mass density and $t$ is time.
The dimension of force rate of change is:
$$[LMT^{-3}]$$.
The SI unit for **force rate of change** is: Newton per second with the associated unit label $\\frac{N}{s}$
The meaningful precision of force rate of change in the drilling context is typically: 0.1 N/s
"""@EN; 
                                        rdfs:subClassOf ddhub:MeasurableQuantity. 
ddhub:ForceRateOfChangeQuantity a owl:Class; 
                                rdfs:comment """A force rate of change is the time derivative of a force: $\\frac{dF}{dt}$, where $F$ is the mass density and $t$ is time.
The dimension of force rate of change is:
$$[LMT^{-3}]$$.
The SI unit for **force rate of change** is: Newton per second with the associated unit label $\\frac{N}{s}$
"""@EN; 
                                rdfs:subClassOf ddhub:Quantity. 
ddhub:ForceToLoadTransformation a owl:Class; 
                                rdfs:comment ""@EN; 
                                rdfs:subClassOf ddhub:DirectTransformation. 
ddhub:FormationCollapseFeature a owl:Class; 
                               rdfs:comment """A formation collapse feature indicates that something accounts for formation collapse limits.
"""@EN; 
                               rdfs:subClassOf ddhub:DownholePressureFeature. 
ddhub:FormationCollapseLocation a owl:Class; 
                                rdfs:comment ""@EN; 
                                rdfs:subClassOf ddhub:AbscissaReferenceLocation. 
ddhub:FormationFluidTransferLocation a owl:Class; 
                                     rdfs:comment ""@EN; 
                                     rdfs:subClassOf ddhub:AbscissaReferenceLocation. 
ddhub:FormationFracturingFeature a owl:Class; 
                                 rdfs:comment """A formation fracturing feature indicates that something accounts for formation fracturing limits.
"""@EN; 
                                 rdfs:subClassOf ddhub:DownholePressureFeature. 
ddhub:FormationGasComponent a owl:Class; 
                            rdfs:comment ""@EN; 
                            rdfs:subClassOf ddhub:GasComponent. 
ddhub:FormationLiquidComponent a owl:Class; 
                               rdfs:comment ""@EN; 
                               rdfs:subClassOf ddhub:LiquidComponent. 
ddhub:FormationResistivityDrillingQuantity a owl:Class; 
                                           rdfs:comment """Electric resistivity is a material's inherent property that measures how strongly it resists the flow of electric current.
The dimension of resistivity is:
$$[L^{3}MI^{-2}T^{-3}]$$.
The SI unit for **electric resistivity** is: ohm metre with the associated unit label $\\Omega \\cdot m$
The meaningful precision of formation electric resistivity in the drilling context is typically: 0.01 Ω•m
"""@EN; 
                                           rdfs:subClassOf ddhub:MeasurableQuantity. 
ddhub:FormationSolidComponent a owl:Class; 
                              rdfs:comment ""@EN; 
                              rdfs:subClassOf ddhub:SolidComponent. 
ddhub:FormationStrengthDescription a owl:Class; 
                                   rdfs:comment """The formation strength data structure describes the formation strength and internal friction angle of the formation
encountered along the wellbore.
"""@EN; 
                                   rdfs:subClassOf ddhub:WellBoreData. 
ddhub:FormationStrengthDrillingQuantity a owl:Class; 
                                        rdfs:comment """Material strength refers to the ability of a material to withstand an applied force or load without failing or deforming. It measures how much stress a material can endure before it breaks, bends, or permanently deforms, often categorized into types like tensile, compressive, and shear strength.
The dimension of material strength is:
$$[ML^{-1}T^{-2}]$$.
The SI unit for **material strength** is: pascal with the associated unit label $Pa$
The meaningful precision of formation strength in the drilling context is typically: 10000 Pa
"""@EN; 
                                        rdfs:subClassOf ddhub:MeasurableQuantity. 
ddhub:FormationTestingAndSampling a owl:Class; 
                                  rdfs:comment ""@EN; 
                                  rdfs:subClassOf ddhub:WirelineLoggingTools. 
ddhub:FormationTestTools a owl:Class; 
                         rdfs:comment ""@EN; 
                         rdfs:subClassOf ddhub:LoggingWhileDrillingTools. 
ddhub:FormationWashout a owl:Class; 
                       rdfs:comment """This Noun is used to refer to a situation during which the formation is being washed out.
"""@EN; 
                       rdfs:subClassOf ddhub:DrillingIncident. 
ddhub:FormationWashoutFeature a owl:Class; 
                              rdfs:comment """A formation washout feature indicates that something accounts for formation washout while circulating.
"""@EN; 
                              rdfs:subClassOf ddhub:CirculationFeature. 
ddhub:FormationWashoutLocation a owl:Class; 
                               rdfs:comment ""@EN; 
                               rdfs:subClassOf ddhub:AbscissaReferenceLocation. 
ddhub:Fortnight a owl:Class; 
                rdfs:comment """[v] = a * [SI]
where
[v] is the value in fortnight
[SI] is the value in SI
a = 1.0/Fortnight, i.e., 8.267195767195768E-07
and
Fortnight = 14.0 * Day
Day = 24.0 * Hour
Hour = 60.0 * Minute
Minute = 60.0
"""@EN; 
                rdfs:subClassOf ddhub:Unit. 
ddhub:ForwardModel a owl:Class; 
                   rdfs:comment """For a forward model, the inputs are used to predict outputs.
"""@EN; 
                   rdfs:subClassOf ddhub:ModelingApproach. 
ddhub:ForwardWhirl a owl:Class; 
                   rdfs:comment """This Noun is used to refer to forward whirl.
"""@EN; 
                   rdfs:subClassOf ddhub:Whirling. 
ddhub:FourDimensionalReferenceFrame a owl:Class; 
                                    rdfs:comment ""@EN; 
                                    rdfs:subClassOf ddhub:ReferenceFrame. 
ddhub:FracturingPressure a owl:Class; 
                         rdfs:comment ""@EN; 
                         rdfs:subClassOf ddhub:PrototypeData. 
ddhub:FracturingPressureGradient a owl:Class; 
                                 rdfs:comment ""@EN; 
                                 rdfs:subClassOf ddhub:PrototypeData. 
ddhub:FrenetSerretReferenceFrame a owl:Class; 
                                 rdfs:comment ""@EN; 
                                 rdfs:subClassOf ddhub:ThreeDimensionalReferenceFrame. 
ddhub:FrequencyQuantity a owl:Class; 
                        rdfs:comment """Frequency is the number of occurrences of a repeating event per unit of time.
The dimension of frequency is:
$$[T^{-1}]$$.
The SI unit for **frequency** is: hertz with the associated unit label $Hz$
"""@EN; 
                        rdfs:subClassOf ddhub:Quantity. 
ddhub:FrequencyRateOfChangeQuantity a owl:Class; 
                                    rdfs:comment """A frequency rate of change is the time derivative of a frequency: $\\frac{df}{dt}$, where $f$ is a frequency and $t$ is time.
The dimension of frequency rate of change is:
$$[T^{-2}]$$.
The SI unit for **frequency rate of change** is: hertz per second with the associated unit label $\\frac{Hz}{s}$
"""@EN; 
                                    rdfs:subClassOf ddhub:Quantity. 
ddhub:FrictionTestProcedure a owl:Class; 
                            rdfs:comment """A friction test procedure is used to measure the free rotating weight and torque and the pick-up and slack-off weights.
"""@EN; 
                            rdfs:subClassOf ddhub:DrillingProcedure. 
ddhub:FullScale a owl:DatatypeProperty, owl:FunctionalProperty; 
                rdfs:comment """The total range of measurement of the signal, i.e., $\\left| max - min \\right|$. The value is expected to be in the same physical quantity as the sensor value.
"""@EN; 
                rdfs:domain ddhub:FullScaleUncertainty; 
                rdfs:range xsd:double. 
ddhub:FullScaleUncertainty a owl:Class; 
                           rdfs:comment """The uncertainty on the signal is described as a Gaussian distribution with a standard deviation that is calculated using a proportion of the maximum range of the signal. The `Fullscale` or `ProportionError` can either be defined as attribute values, for example when they have fixed values, or using facts utilizing the verbs `HasFullScale` or repectively `HasProportionError` when these values may change through time.
"""@EN; 
                           rdfs:subClassOf ddhub:GaussianUncertainty. 
ddhub:Furlong a owl:Class; 
              rdfs:comment """[v] = a * [SI]
where
[v] is the value in furlong
[SI] is the value in SI
a = 1.0/Furlong, i.e., 0.004970969537898672
and
Furlong = 660.0 * Foot reference: https://www.britannica.com/science/furlong
Foot = 12.0 * Inch
Inch = 0.0254 reference: https://www.nist.gov/pml/owm/si-units-length
"""@EN; 
              rdfs:subClassOf ddhub:Unit. 
ddhub:FurlongPerFortnight a owl:Class; 
                          rdfs:comment """[v] = a * [SI]
where
[v] is the value in furlong per fortnight
[SI] is the value in SI
a = Fortnight/Furlong, i.e., 6012.884753042234
and
Fortnight = 14.0 * Day
Furlong = 660.0 * Foot reference: https://www.britannica.com/science/furlong
Day = 24.0 * Hour
Foot = 12.0 * Inch
Hour = 60.0 * Minute
Inch = 0.0254 reference: https://www.nist.gov/pml/owm/si-units-length
Minute = 60.0
"""@EN; 
                          rdfs:subClassOf ddhub:Unit. 
ddhub:Galileo a owl:Class; 
              rdfs:comment """[v] = a * [SI]
where
[v] is the value in galileo
[SI] is the value in SI
a = 1.0/Centi, i.e., 100
and
Centi = 0.01
"""@EN; 
              rdfs:subClassOf ddhub:Unit. 
ddhub:GalvanicCouplingDownholeTelemetry a owl:Class; 
                                        rdfs:comment """A method that allows transfer of downhole data to the surface via galvanic coupling between pipes along the drill-string.
"""@EN; 
                                        rdfs:subClassOf ddhub:WiredPipeTelemetry. 
ddhub:GammaRayIndexDrillingQuantity a owl:Class; 
                                    rdfs:comment """The Gamma Ray API is a unit used in the petroleum industry to measure the natural gamma radiation of formations. Specifically, the Gamma Ray Index (GRI) is used in well logging to measure the gamma ray activity of the rock surrounding the borehole.
Gamma rays are a form of electromagnetic radiation, and in well logging, they are used to assess the radioactive content of the formations, which helps in identifying rock types (shales, sandstones, etc.).
Since the Gamma Ray API is a measure of gamma radiation intensity, let's break down its physical nature:
"""@EN; 
                                    rdfs:subClassOf ddhub:MeasurableQuantity. 
ddhub:GasAbsorptionFeature a owl:Class; 
                           rdfs:comment """A gas absorption feature indicates that something accounts for conditions by which gas can be absorbed by the drilling fluid.
"""@EN; 
                           rdfs:subClassOf ddhub:DownholePressureFeature. 
ddhub:GasAnalysisEquipment a owl:Class; 
                           rdfs:comment ""@EN; 
                           rdfs:subClassOf ddhub:MudLoggingEquipment. 
ddhub:GasComponent a owl:Class; 
                   rdfs:comment ""@EN; 
                   rdfs:subClassOf ddhub:FluidComponent. 
ddhub:GasFlowRate a owl:Class; 
                  rdfs:comment ""@EN; 
                  rdfs:subClassOf ddhub:PrototypeData. 
ddhub:GasSafetySystems a owl:Class; 
                       rdfs:comment ""@EN; 
                       rdfs:subClassOf ddhub:SafetyEquipment. 
ddhub:GasShowDrillingQuantity a owl:Class; 
                              rdfs:comment """A proportion is the ratio of two quantities with the same dimension. It represents how one quantity compares to another in relative terms.
A proportion is dimensionless:
The meaningful precision of gas show in the drilling context is typically: 1E-07 
"""@EN; 
                              rdfs:subClassOf ddhub:MeasurableQuantity. 
ddhub:GasVolumetricFlowRateDrillingQuantity a owl:Class; 
                                            rdfs:comment """A volumetric flowrate is the volume of fluid that passes per unit time: $\\frac{dV}{dt}$, where $V$ is a volume and $t$ is time.
The dimension of volumetric flowrate is:
$$[L^{3}T^{-1}]$$.
The SI unit for **volumetric flow rate** is: cubic metre per second with the associated unit label $\\frac{m^{3}}{s}$
The meaningful precision of gas volumetric flowrate in the drilling context is typically: 0.01 m³/s
"""@EN; 
                                            rdfs:subClassOf ddhub:MeasurableQuantity. 
ddhub:GaugePressureReference a owl:Class; 
                             rdfs:comment ""@EN; 
                             rdfs:subClassOf ddhub:RelativePressureReference. 
ddhub:Gauss a owl:Class; 
            rdfs:comment """[v] = a * [SI]
where
[v] is the value in gauss
[SI] is the value in SI
a = 1.0/Gauss, i.e., 10000
and
Gauss = 1e-4 reference: https://en.wikipedia.org/wiki/Gauss_(unit)
"""@EN; 
            rdfs:subClassOf ddhub:Unit. 
ddhub:GaussianUncertainty a owl:Class; 
                          rdfs:comment """The uncertainty is represented by a Gaussian distribution, i.e., with a `Mean` and a `StandardDeviation`, $\\mathcal{N}(\\overline{x},{\\sigma_{x}}^2)$ where $\\overline{x}$ is the `Mean` value and $\\sigma_{x}$ is the `StandardDeviation`.
"""@EN; 
                          rdfs:subClassOf ddhub:SignalUncertainty. 
ddhub:GaussSquareCentimetre a owl:Class; 
                            rdfs:comment """[v] = a * [SI]
where
[v] is the value in gauss square centimetre
[SI] is the value in SI
a = 1.0/(Gauss *Centi*Centi), i.e., 99999999.99999999
and
Gauss = 1e-4 reference: https://en.wikipedia.org/wiki/Gauss_(unit)
Centi = 0.01
"""@EN; 
                            rdfs:subClassOf ddhub:Unit. 
ddhub:GeneralModel a owl:Class; 
                   rdfs:comment """A model with a broad range of application across various systems or phenomena.
"""@EN; 
                   rdfs:subClassOf ddhub:ModelScope. 
ddhub:GenericEquipment a owl:Class; 
                       rdfs:comment ""@EN; 
                       rdfs:subClassOf ddhub:Equipment. 
ddhub:GenericEquipmentGatevalve a owl:Class; 
                                rdfs:comment ""@EN; 
                                rdfs:subClassOf ddhub:GenericEquipment. 
ddhub:GenericUncertainty a owl:Class; 
                         rdfs:comment """The uncertainty is represented by a `Histogram`.
"""@EN; 
                         rdfs:subClassOf ddhub:SignalUncertainty. 
ddhub:GeoPressuresDescription a owl:Class; 
                              rdfs:comment """The geo-pressure data structure describes the pore pressure, collapse pressure, min horizontal stress, fracturing pressure
along the wellbore.
"""@EN; 
                              rdfs:subClassOf ddhub:WellBoreData. 
ddhub:GeoThermalDescription a owl:Class; 
                            rdfs:comment """The geothermal data structure describes the temperature and thermophysical properties of the formation encountered
along the wellbore.
"""@EN; 
                            rdfs:subClassOf ddhub:WellBoreData. 
ddhub:Gigaampere a owl:Class; 
                 rdfs:comment """[v] = a * [SI]
where
[v] is the value in gigaampere
[SI] is the value in SI
a = 1.0/Giga, i.e., 1E-09
and
Giga = 1e9
"""@EN; 
                 rdfs:subClassOf ddhub:Unit. 
ddhub:Gigahertz a owl:Class; 
                rdfs:comment """[v] = a * [SI]
where
[v] is the value in gigahertz
[SI] is the value in SI
a = 1.0/Giga, i.e., 1E-09
and
Giga = 1e9
"""@EN; 
                rdfs:subClassOf ddhub:Unit. 
ddhub:GigaHertzPerDay a owl:Class; 
                      rdfs:comment """[v] = a * [SI]
where
[v] is the value in giga hertz per day
[SI] is the value in SI
a = Day/Giga, i.e., 8.64E-05
and
Day = 24.0 * Hour
Giga = 1e9
Hour = 60.0 * Minute
Minute = 60.0
"""@EN; 
                      rdfs:subClassOf ddhub:Unit. 
ddhub:GigaHertzPerHour a owl:Class; 
                       rdfs:comment """[v] = a * [SI]
where
[v] is the value in giga hertz per hour
[SI] is the value in SI
a = Hour/Giga, i.e., 3.6E-06
and
Hour = 60.0 * Minute
Giga = 1e9
Minute = 60.0
"""@EN; 
                       rdfs:subClassOf ddhub:Unit. 
ddhub:GigaHertzPerMinute a owl:Class; 
                         rdfs:comment """[v] = a * [SI]
where
[v] is the value in giga hertz per minute
[SI] is the value in SI
a = Minute/Giga, i.e., 6E-08
and
Minute = 60.0
Giga = 1e9
"""@EN; 
                         rdfs:subClassOf ddhub:Unit. 
ddhub:GigaHertzPerSecond a owl:Class; 
                         rdfs:comment """[v] = a * [SI]
where
[v] is the value in giga hertz per second
[SI] is the value in SI
a = 1.0/Giga, i.e., 1E-09
and
Giga = 1e9
"""@EN; 
                         rdfs:subClassOf ddhub:Unit. 
ddhub:GigaHertzPerYear a owl:Class; 
                       rdfs:comment """[v] = a * [SI]
where
[v] is the value in giga hertz per year
[SI] is the value in SI
a = YearJulian/Giga, i.e., 0.0315576
and
YearJulian = 365.25 * Day
Giga = 1e9
Day = 24.0 * Hour
Hour = 60.0 * Minute
Minute = 60.0
"""@EN; 
                       rdfs:subClassOf ddhub:Unit. 
ddhub:Gigajoule a owl:Class; 
                rdfs:comment """[v] = a * [SI]
where
[v] is the value in gigajoule
[SI] is the value in SI
a = 1.0/Giga, i.e., 1E-09
and
Giga = 1e9
"""@EN; 
                rdfs:subClassOf ddhub:Unit. 
ddhub:GigajoulePerCubicFoot a owl:Class; 
                            rdfs:comment """[v] = a * [SI]
where
[v] is the value in gigajoule per cubic foot
[SI] is the value in SI
a = Foot * Foot * Foot / Giga, i.e., 2.831684659199999E-11
and
Foot = 12.0 * Inch
Giga = 1e9
Inch = 0.0254 reference: https://www.nist.gov/pml/owm/si-units-length
"""@EN; 
                            rdfs:subClassOf ddhub:Unit. 
ddhub:GigajoulePerCubicInch a owl:Class; 
                            rdfs:comment """[v] = a * [SI]
where
[v] is the value in gigajoule per cubic inch
[SI] is the value in SI
a = Inch*Inch*Inch/Giga, i.e., 1.6387064E-14
and
Inch = 0.0254 reference: https://www.nist.gov/pml/owm/si-units-length
Giga = 1e9
"""@EN; 
                            rdfs:subClassOf ddhub:Unit. 
ddhub:GigajoulePerCubicMetre a owl:Class; 
                             rdfs:comment """[v] = a * [SI]
where
[v] is the value in gigajoule per cubic metre
[SI] is the value in SI
a = 1.0/Giga, i.e., 1E-09
and
Giga = 1e9
"""@EN; 
                             rdfs:subClassOf ddhub:Unit. 
ddhub:GigajoulePerGallonUk a owl:Class; 
                           rdfs:comment """[v] = a * [SI]
where
[v] is the value in gigajoule per gallon (UK)
[SI] is the value in SI
a = GallonUK / Giga, i.e., 4.54609E-12
and
GallonUK = 4.54609e-3 reference: https://en.wikipedia.org/wiki/Gallon
Giga = 1e9
"""@EN; 
                           rdfs:subClassOf ddhub:Unit. 
ddhub:GigajoulePerGallonUs a owl:Class; 
                           rdfs:comment """[v] = a * [SI]
where
[v] is the value in gigajoule per gallon (US)
[SI] is the value in SI
a = GallonUS / Giga, i.e., 3.785411784E-12
and
GallonUS = 231.0 * Inch * Inch * Inch reference: https://en.wikipedia.org/wiki/Gallon
Giga = 1e9
Inch = 0.0254 reference: https://www.nist.gov/pml/owm/si-units-length
"""@EN; 
                           rdfs:subClassOf ddhub:Unit. 
ddhub:GigajoulePerLitre a owl:Class; 
                        rdfs:comment """[v] = a * [SI]
where
[v] is the value in gigajoule per litre
[SI] is the value in SI
a = Litre/Giga, i.e., 1E-12
and
Litre = 0.001
Giga = 1e9
"""@EN; 
                        rdfs:subClassOf ddhub:Unit. 
ddhub:GigaOhmMetre a owl:Class; 
                   rdfs:comment """[v] = a * [SI]
where
[v] is the value in giga ohm metre
[SI] is the value in SI
a = 1.0/Giga, i.e., 1E-09
and
Giga = 1e9
"""@EN; 
                   rdfs:subClassOf ddhub:Unit. 
ddhub:Gigapascal a owl:Class; 
                 rdfs:comment """[v] = a * [SI]
where
[v] is the value in gigapascal
[SI] is the value in SI
a = 1.0/Giga, i.e., 1E-09
and
Giga = 1e9
"""@EN; 
                 rdfs:subClassOf ddhub:Unit. 
ddhub:GigapascalPerHour a owl:Class; 
                        rdfs:comment """[v] = a * [SI]
where
[v] is the value in gigapascal per hour
[SI] is the value in SI
a = Hour/Giga, i.e., 3.6E-06
and
Hour = 60.0 * Minute
Giga = 1e9
Minute = 60.0
"""@EN; 
                        rdfs:subClassOf ddhub:Unit. 
ddhub:GigapascalPerMinute a owl:Class; 
                          rdfs:comment """[v] = a * [SI]
where
[v] is the value in gigapascal per minute
[SI] is the value in SI
a = Minute/Giga, i.e., 6E-08
and
Minute = 60.0
Giga = 1e9
"""@EN; 
                          rdfs:subClassOf ddhub:Unit. 
ddhub:GigapascalPerSecond a owl:Class; 
                          rdfs:comment """[v] = a * [SI]
where
[v] is the value in gigapascal per second
[SI] is the value in SI
a = 1.0/Giga, i.e., 1E-09
and
Giga = 1e9
"""@EN; 
                          rdfs:subClassOf ddhub:Unit. 
ddhub:Gigatonne a owl:Class; 
                rdfs:comment """[v] = a * [SI]
where
[v] is the value in gigatonne
[SI] is the value in SI
a = 1.0/Tera, i.e., 1E-12
and
Tera = 1e12
"""@EN; 
                rdfs:subClassOf ddhub:Unit. 
ddhub:Gigavolt a owl:Class; 
               rdfs:comment """[v] = a * [SI]
where
[v] is the value in gigavolt
[SI] is the value in SI
a = 1.0/Giga, i.e., 1E-09
and
Giga = 1e9
"""@EN; 
               rdfs:subClassOf ddhub:Unit. 
ddhub:Gigawatt a owl:Class; 
               rdfs:comment """[v] = a * [SI]
where
[v] is the value in gigawatt
[SI] is the value in SI
a = 1.0/Giga, i.e., 1E-09
and
Giga = 1e9
"""@EN; 
               rdfs:subClassOf ddhub:Unit. 
ddhub:Gon a owl:Class; 
          rdfs:comment """[v] = a * [SI]
where
[v] is the value in gon
[SI] is the value in SI
a = Grad, i.e., 63.66197723675813
and
Grad = 200.0 / System.Math.PI
"""@EN; 
          rdfs:subClassOf ddhub:Unit. 
ddhub:Gooseneck a owl:Class; 
                rdfs:comment ""@EN; 
                rdfs:subClassOf ddhub:MudLines. 
ddhub:GPSReference a owl:Class; 
                   rdfs:comment ""@EN; 
                   rdfs:subClassOf ddhub:TimeReference. 
ddhub:Grad a owl:Class; 
           rdfs:comment """[v] = a * [SI]
where
[v] is the value in grad
[SI] is the value in SI
a = Grad, i.e., 63.66197723675813
and
Grad = 200.0 / System.Math.PI
"""@EN; 
           rdfs:subClassOf ddhub:Unit. 
ddhub:Grain a owl:Class; 
            rdfs:comment """[v] = a * [SI]
where
[v] is the value in grain
[SI] is the value in SI
a = 1.0/Grain, i.e., 15432.358352941428
and
Grain = (1.0 / 7000.0) * Pound reference: https://en.wikipedia.org/wiki/Grain_(unit)
Pound = 0.45359237 reference: https://en.wikipedia.org/wiki/Pound_(mass)
"""@EN; 
            rdfs:subClassOf ddhub:Unit. 
ddhub:Gram a owl:Class; 
           rdfs:comment """[v] = a * [SI]
where
[v] is the value in gram
[SI] is the value in SI
a = 1.0/Milli, i.e., 1000
and
Milli = 0.001
"""@EN; 
           rdfs:subClassOf ddhub:Unit. 
ddhub:GramPerCubicCentimetre a owl:Class; 
                             rdfs:comment """[v] = a * [SI]
where
[v] is the value in gram per cubic centimetre
[SI] is the value in SI
a = Centi*Centi*Centi / Milli, i.e., 0.0010000000000000002
and
Centi = 0.01
Milli = 0.001
"""@EN; 
                             rdfs:subClassOf ddhub:Unit. 
ddhub:GramPerCubicCentimetrePer100Metre a owl:Class; 
                                        rdfs:comment """[v] = a * [SI]
where
[v] is the value in gram per cubic centimetre per 100 metre
[SI] is the value in SI
a = Centi*Centi*Centi*Hecto/Milli, i.e., 0.10000000000000002
and
Centi = 0.01
Hecto = 100.0
Milli = 0.001
"""@EN; 
                                        rdfs:subClassOf ddhub:Unit. 
ddhub:GramPerCubicCentimetrePer10Metre a owl:Class; 
                                       rdfs:comment """[v] = a * [SI]
where
[v] is the value in gram per cubic centimetre per 10 metre
[SI] is the value in SI
a = Centi*Centi*Centi*Deca/Milli, i.e., 0.010000000000000002
and
Centi = 0.01
Deca = 10.0
Milli = 0.001
"""@EN; 
                                       rdfs:subClassOf ddhub:Unit. 
ddhub:GramPerCubicCentimetrePer30Metre a owl:Class; 
                                       rdfs:comment """[v] = a * [SI]
where
[v] is the value in gram per cubic centimetre per 30 metre
[SI] is the value in SI
a = Centi*Centi*Centi*3.0*Deca/Milli, i.e., 0.030000000000000002
and
Centi = 0.01
Deca = 10.0
Milli = 0.001
"""@EN; 
                                       rdfs:subClassOf ddhub:Unit. 
ddhub:GramPerCubicCentimetrePerCelsius a owl:Class; 
                                       rdfs:comment """[v] = a * [SI]
where
[v] is the value in gram per cubic centimetre per celsius
[SI] is the value in SI
a = Centi*Centi*Centi/Milli, i.e., 0.0010000000000000002
and
Centi = 0.01
Milli = 0.001
"""@EN; 
                                       rdfs:subClassOf ddhub:Unit. 
ddhub:GramPerCubicCentimetrePerHour a owl:Class; 
                                    rdfs:comment """[v] = a * [SI]
where
[v] is the value in gram per cubic centimetre per hour
[SI] is the value in SI
a = Hour *Milli, i.e., 3.6
and
Hour = 60.0 * Minute
Milli = 0.001
Minute = 60.0
"""@EN; 
                                    rdfs:subClassOf ddhub:Unit. 
ddhub:GramPerCubicCentimetrePerMetre a owl:Class; 
                                     rdfs:comment """[v] = a * [SI]
where
[v] is the value in gram per cubic centimetre per metre
[SI] is the value in SI
a = Centi*Centi*Centi/Milli, i.e., 0.0010000000000000002
and
Centi = 0.01
Milli = 0.001
"""@EN; 
                                     rdfs:subClassOf ddhub:Unit. 
ddhub:GramPerCubicCentimetrePerMinute a owl:Class; 
                                      rdfs:comment """[v] = a * [SI]
where
[v] is the value in gram per cubic centimetre per minute
[SI] is the value in SI
a = Minute * Milli, i.e., 0.06
and
Minute = 60.0
Milli = 0.001
"""@EN; 
                                      rdfs:subClassOf ddhub:Unit. 
ddhub:GramPerCubicCentimetrePerSecond a owl:Class; 
                                      rdfs:comment """[v] = a * [SI]
where
[v] is the value in gram per cubic centimetre per second
[SI] is the value in SI
a = Milli, i.e., 0.001
and
Milli = 0.001
"""@EN; 
                                      rdfs:subClassOf ddhub:Unit. 
ddhub:GramPerCubicMetre a owl:Class; 
                        rdfs:comment """[v] = a * [SI]
where
[v] is the value in gram per cubic metre
[SI] is the value in SI
a = 1.0/Milli, i.e., 1000
and
Milli = 0.001
"""@EN; 
                        rdfs:subClassOf ddhub:Unit. 
ddhub:GramPerMetre a owl:Class; 
                   rdfs:comment """[v] = a * [SI]
where
[v] is the value in gram per metre
[SI] is the value in SI
a = 1.0/Milli, i.e., 1000
and
Milli = 0.001
"""@EN; 
                   rdfs:subClassOf ddhub:Unit. 
ddhub:GravitationalLoadQuantity a owl:Class; 
                                rdfs:comment """Mass can be experimentally defined as a measure of the body's inertia, meaning the resistance to acceleration (change of velocity) when a net force is applied. The object's mass also determines the strength of its gravitational attraction to other bodies.
The dimension of mass is:
$$[M]$$.
The SI unit for **mass** is: kilogram with the associated unit label $kg$
"""@EN; 
                                rdfs:subClassOf ddhub:Quantity. 
ddhub:GravityHighSideAngleLocation a owl:Class; 
                                   rdfs:comment ""@EN; 
                                   rdfs:subClassOf ddhub:AngleReferenceLocation. 
ddhub:GravityStandard a owl:Class; 
                      rdfs:comment """[v] = a * [SI]
where
[v] is the value in gravity standard
[SI] is the value in SI
a = 1.0/G, i.e., 0.10197162129779283
and
G = 9.80665 reference: https://en.wikipedia.org/wiki/Gravity_of_Earth
"""@EN; 
                      rdfs:subClassOf ddhub:Unit. 
ddhub:GrayBoxModel a owl:Class; 
                   rdfs:comment """The model combines both data-drive and mechanistic models offering a partial transparency.
"""@EN; 
                   rdfs:subClassOf ddhub:ModelTransparency. 
ddhub:GridNorthAzimuthLocation a owl:Class; 
                               rdfs:comment ""@EN; 
                               rdfs:subClassOf ddhub:AzimuthReferenceLocation. 
ddhub:GroundLevelVerticalLocation a owl:Class; 
                                  rdfs:comment ""@EN; 
                                  rdfs:subClassOf ddhub:VerticalReferenceLocation. 
ddhub:Grouping a owl:Class; 
               rdfs:comment ""@EN; 
               rdfs:subClassOf ddhub:DrillString. 
ddhub:GT a owl:Class; 
         rdfs:comment ""@EN; 
         rdfs:subClassOf ddhub:ValidityCondition. 
ddhub:HammerAssembly a owl:Class; 
                     rdfs:comment ""@EN; 
                     rdfs:subClassOf ddhub:DrillingEquipment. 
ddhub:Hand a owl:Class; 
           rdfs:comment """[v] = a * [SI]
where
[v] is the value in hand
[SI] is the value in SI
a = 1.0/Hand, i.e., 9.84251968503937
and
Hand = 4.0 * Inch reference: https://en.wikipedia.org/wiki/Hand_(unit)
Inch = 0.0254 reference: https://www.nist.gov/pml/owm/si-units-length
"""@EN; 
           rdfs:subClassOf ddhub:Unit. 
ddhub:Hangers a owl:Class; 
              rdfs:comment ""@EN; 
              rdfs:subClassOf ddhub:CasingEquipment. 
ddhub:HasAcquisitionClock a owl:ObjectProperty; 
                          rdfs:comment ""@EN; 
                          rdfs:domain ddhub:DrillingDataPoint; 
                          rdfs:range ddhub:Clock; 
                          rdfs:subPropertyOf ddhub:DWISVerb. 
ddhub:HasAcquisitionTime a owl:ObjectProperty; 
                         rdfs:comment ""@EN; 
                         rdfs:domain ddhub:DrillingDataPoint; 
                         rdfs:range ddhub:DrillingDataPoint; 
                         rdfs:subPropertyOf ddhub:DWISVerb. 
ddhub:HasBranchComponent a owl:ObjectProperty; 
                         rdfs:comment ""@EN; 
                         rdfs:domain ddhub:HydraulicNetwork; 
                         rdfs:range ddhub:HydraulicBranch; 
                         rdfs:subPropertyOf ddhub:DWISVerb. 
ddhub:HasBranchCoordinateSystem a owl:ObjectProperty; 
                                rdfs:comment ""@EN; 
                                rdfs:domain ddhub:HydraulicBranch; 
                                rdfs:range ddhub:ReferenceFrame; 
                                rdfs:subPropertyOf ddhub:DWISVerb. 
ddhub:HasControlLimit a owl:ObjectProperty; 
                      rdfs:comment """This Verb is used to indicate that a drilling data point has a control limit.
"""@EN; 
                      rdfs:domain ddhub:DrillingDataPoint; 
                      rdfs:range ddhub:DrillingLimit; 
                      rdfs:subPropertyOf ddhub:IsRelatedToDrillingLimit. 
ddhub:HasCoordinates a owl:ObjectProperty; 
                     rdfs:comment ""@EN; 
                     rdfs:domain ddhub:Location; 
                     rdfs:range ddhub:DrillingDataPoint; 
                     rdfs:subPropertyOf ddhub:DWISVerb. 
ddhub:HasDomain a owl:ObjectProperty; 
                rdfs:comment ""@EN; 
                rdfs:domain ddhub:DrillingDataPoint; 
                rdfs:range ddhub:DrillingDataPoint; 
                rdfs:subPropertyOf ddhub:DWISVerb. 
ddhub:HasDynamicValue a owl:ObjectProperty; 
                      rdfs:comment ""@EN; 
                      rdfs:domain ddhub:DrillingDataPoint; 
                      rdfs:range ddhub:DynamicDrillingSignal; 
                      rdfs:subPropertyOf ddhub:HasValue. 
ddhub:HasElevationReference a owl:ObjectProperty; 
                            rdfs:comment """This verb is a specialization of `IsDependentOn` and refers to the specific dependence on an elevation reference.
"""@EN; 
                            rdfs:domain ddhub:DrillingDataPoint; 
                            rdfs:range ddhub:Location; 
                            rdfs:subPropertyOf ddhub:IsDependentOn. 
ddhub:HasEndJunction a owl:ObjectProperty; 
                     rdfs:comment ""@EN; 
                     rdfs:domain ddhub:HydraulicBranch; 
                     rdfs:range ddhub:HydraulicJunction; 
                     rdfs:subPropertyOf ddhub:IsHydraulicConnectedTo. 
ddhub:HasEndPoint a owl:ObjectProperty; 
                  rdfs:comment ""@EN; 
                  rdfs:domain ddhub:DrillingSignal; 
                  rdfs:range ddhub:DataEndPoint; 
                  rdfs:subPropertyOf ddhub:DWISVerb. 
ddhub:HasFullScale a owl:ObjectProperty; 
                   rdfs:comment """This verb is used to associate a `DrillingDataPoint` as the `FullScale` value of a `FullScaleUncertainty`
"""@EN; 
                   rdfs:domain ddhub:FullScaleUncertainty; 
                   rdfs:range ddhub:DrillingDataPoint; 
                   rdfs:subPropertyOf ddhub:DWISVerb. 
ddhub:HasFunction a owl:ObjectProperty; 
                  rdfs:comment ""@EN; 
                  rdfs:domain ddhub:DrillingDataPoint; 
                  rdfs:range ddhub:DataFlowNode; 
                  rdfs:subPropertyOf ddhub:DWISVerb. 
ddhub:HasHydraulicState a owl:ObjectProperty; 
                        rdfs:comment ""@EN; 
                        rdfs:domain ddhub:HydraulicJunction; 
                        rdfs:range ddhub:HydraulicElementState; 
                        rdfs:subPropertyOf ddhub:DWISVerb. 
ddhub:HasHydraulicStateValueFrom a owl:ObjectProperty; 
                                 rdfs:comment ""@EN; 
                                 rdfs:domain ddhub:DWISNoun; 
                                 rdfs:range ddhub:DWISNoun; 
                                 rdfs:subPropertyOf ddhub:DWISVerb. 
ddhub:HasLeftBranch a owl:ObjectProperty; 
                    rdfs:comment ""@EN; 
                    rdfs:domain ddhub:HydraulicJunction; 
                    rdfs:range ddhub:HydraulicBranch; 
                    rdfs:subPropertyOf ddhub:IsHydraulicConnectedTo. 
ddhub:HasLeftBranchCoordinates a owl:ObjectProperty; 
                               rdfs:comment ""@EN; 
                               rdfs:domain ddhub:HydraulicJunction; 
                               rdfs:range ddhub:DrillingDataPoint; 
                               rdfs:subPropertyOf ddhub:DWISVerb. 
ddhub:HasMeasurableQuantity a owl:ObjectProperty; 
                            rdfs:comment """This `Verb` is used to define the reciprocal relationship of `IsOfBaseQuantity`, i.e., to relate
a `Quantity` with a `MeasureableQuantity`.
"""@EN; 
                            rdfs:domain ddhub:Quantity; 
                            rdfs:range ddhub:MeasurableQuantity; 
                            rdfs:subPropertyOf ddhub:DWISVerb. 
ddhub:HasMechanicalState a owl:ObjectProperty; 
                         rdfs:comment ""@EN; 
                         rdfs:domain ddhub:MechanicalLogicalElement; 
                         rdfs:range ddhub:MechanicalElementState; 
                         rdfs:subPropertyOf ddhub:DWISVerb. 
ddhub:HasMechanicalStateValueFrom a owl:ObjectProperty; 
                                  rdfs:comment ""@EN; 
                                  rdfs:domain ddhub:MechanicalElementState; 
                                  rdfs:range ddhub:DrillingDataPoint; 
                                  rdfs:subPropertyOf ddhub:DWISVerb. 
ddhub:HasMotionType a owl:ObjectProperty; 
                    rdfs:comment ""@EN; 
                    rdfs:domain ddhub:MechanicalLogicalElement; 
                    rdfs:range ddhub:MotionType; 
                    rdfs:subPropertyOf ddhub:DWISVerb. 
ddhub:HasOperationalStep a owl:ObjectProperty; 
                         rdfs:comment """this Verb is used to relate an operational step to a rig action plan.
"""@EN; 
                         rdfs:domain ddhub:OperationalStep; 
                         rdfs:range ddhub:OperationalStep; 
                         rdfs:subPropertyOf ddhub:DWISVerb. 
ddhub:HasPressureReference a owl:ObjectProperty; 
                           rdfs:comment """This verb is a specialization of `IsDependentOn` and refers to the specific dependence on a pressure reference.
"""@EN; 
                           rdfs:domain ddhub:DrillingDataPoint; 
                           rdfs:range ddhub:DrillingDataPoint; 
                           rdfs:subPropertyOf ddhub:IsDependentOn. 
ddhub:HasPressureReferenceType a owl:ObjectProperty; 
                               rdfs:comment ""@EN; 
                               rdfs:domain ddhub:DrillingDataPoint; 
                               rdfs:range ddhub:PressureReference; 
                               rdfs:subPropertyOf ddhub:DWISVerb. 
ddhub:HasProportionError a owl:ObjectProperty; 
                         rdfs:comment """This verb is used to associate a `DrillingDataPoint` as the `ProportionError` value of a `FullScaleUncertainty`
"""@EN; 
                         rdfs:domain ddhub:FullScaleUncertainty; 
                         rdfs:range ddhub:DrillingDataPoint; 
                         rdfs:subPropertyOf ddhub:DWISVerb. 
ddhub:HasReferenceFrame a owl:ObjectProperty; 
                        rdfs:comment ""@EN; 
                        rdfs:domain ddhub:DrillingDataPoint; 
                        rdfs:range ddhub:ReferenceFrame; 
                        rdfs:subPropertyOf ddhub:DWISVerb. 
ddhub:HasReferenceFrameOrigin a owl:ObjectProperty; 
                              rdfs:comment ""@EN; 
                              rdfs:domain ddhub:ReferenceFrame; 
                              rdfs:range ddhub:Location; 
                              rdfs:subPropertyOf ddhub:DWISVerb. 
ddhub:HasRightBranch a owl:ObjectProperty; 
                     rdfs:comment ""@EN; 
                     rdfs:domain ddhub:HydraulicJunction; 
                     rdfs:range ddhub:HydraulicBranch; 
                     rdfs:subPropertyOf ddhub:IsHydraulicConnectedTo. 
ddhub:HasRightBranchCoordinates a owl:ObjectProperty; 
                                rdfs:comment ""@EN; 
                                rdfs:domain ddhub:HydraulicJunction; 
                                rdfs:range ddhub:DrillingDataPoint; 
                                rdfs:subPropertyOf ddhub:DWISVerb. 
ddhub:HasSIUnit a owl:ObjectProperty; 
                rdfs:comment """This `verb` is used to be define a relation between a `Quantity` and a `Unit`.
"""@EN; 
                rdfs:domain ddhub:Quantity; 
                rdfs:range ddhub:Unit; 
                rdfs:subPropertyOf ddhub:DWISVerb. 
ddhub:HasSourceClock a owl:ObjectProperty; 
                     rdfs:comment ""@EN; 
                     rdfs:domain ddhub:DrillingDataPoint; 
                     rdfs:range ddhub:Clock; 
                     rdfs:subPropertyOf ddhub:DWISVerb. 
ddhub:HasSourceTime a owl:ObjectProperty; 
                    rdfs:comment ""@EN; 
                    rdfs:domain ddhub:DrillingDataPoint; 
                    rdfs:range ddhub:DrillingDataPoint; 
                    rdfs:subPropertyOf ddhub:DWISVerb. 
ddhub:HasStartJunction a owl:ObjectProperty; 
                       rdfs:comment ""@EN; 
                       rdfs:domain ddhub:HydraulicBranch; 
                       rdfs:range ddhub:HydraulicJunction; 
                       rdfs:subPropertyOf ddhub:IsHydraulicConnectedTo. 
ddhub:HasStaticValue a owl:ObjectProperty; 
                     rdfs:comment ""@EN; 
                     rdfs:domain ddhub:DrillingDataPoint; 
                     rdfs:range ddhub:DrillingSignal; 
                     rdfs:subPropertyOf ddhub:HasValue. 
ddhub:HasTemperatureReference a owl:ObjectProperty; 
                              rdfs:comment """This verb is a specialization of `IsDependentOn` and refers to the specific dependence on a temperature reference.
"""@EN; 
                              rdfs:domain ddhub:DrillingDataPoint; 
                              rdfs:range ddhub:DrillingDataPoint; 
                              rdfs:subPropertyOf ddhub:IsDependentOn. 
ddhub:HasTimeIntervalDomain a owl:ObjectProperty; 
                            rdfs:comment ""@EN; 
                            rdfs:domain ddhub:DrillingDataPoint; 
                            rdfs:range ddhub:DrillingDataPoint; 
                            rdfs:subPropertyOf ddhub:HasDomain. 
ddhub:HasTimeReference a owl:ObjectProperty; 
                       rdfs:comment ""@EN; 
                       rdfs:domain ddhub:DrillingDataPoint; 
                       rdfs:range ddhub:TimeReference; 
                       rdfs:subPropertyOf ddhub:DWISVerb. 
ddhub:HasTransmissionDelay a owl:ObjectProperty; 
                           rdfs:comment ""@EN; 
                           rdfs:domain ddhub:DrillingDataPoint; 
                           rdfs:range ddhub:DrillingDataPoint; 
                           rdfs:subPropertyOf ddhub:DWISVerb. 
ddhub:HasUncertainty a owl:ObjectProperty; 
                     rdfs:comment """This verb allows to associate a `SignalUncertainty` to a `DrillingDataPoint`.
"""@EN; 
                     rdfs:domain ddhub:DrillingDataPoint; 
                     rdfs:range ddhub:SignalUncertainty; 
                     rdfs:subPropertyOf ddhub:DWISVerb. 
ddhub:HasUncertaintyAccuracy a owl:ObjectProperty; 
                             rdfs:comment """This verb allows to associate a `DrillingDataPoint` as the `Accuracy` of a `SensorUncertainty`
"""@EN; 
                             rdfs:domain ddhub:SensorUncertainty; 
                             rdfs:range ddhub:DrillingDataPoint; 
                             rdfs:subPropertyOf ddhub:DWISVerb. 
ddhub:HasUncertaintyHistogram a owl:ObjectProperty; 
                              rdfs:comment """This verb is used to associated a `DrillingDataPoint` as the `Histogram` value of a `GenericUncertainty`
"""@EN; 
                              rdfs:domain ddhub:GenericUncertainty; 
                              rdfs:range ddhub:DrillingDataPoint; 
                              rdfs:subPropertyOf ddhub:DWISVerb. 
ddhub:HasUncertaintyMax a owl:ObjectProperty; 
                        rdfs:comment """This verb is used to associate a `DrillingDataPoint` as the `Max` value of a `MinMaxUncertainty`
"""@EN; 
                        rdfs:domain ddhub:MinMaxUncertainty; 
                        rdfs:range ddhub:DrillingDataPoint; 
                        rdfs:subPropertyOf ddhub:DWISVerb. 
ddhub:HasUncertaintyMean a owl:ObjectProperty; 
                         rdfs:comment """This verb is used to associate a `DrillingDataPoint` as the `Mean` value of a `GaussianUncertainty`
"""@EN; 
                         rdfs:domain ddhub:GaussianUncertainty; 
                         rdfs:range ddhub:DrillingDataPoint; 
                         rdfs:subPropertyOf ddhub:DWISVerb. 
ddhub:HasUncertaintyMin a owl:ObjectProperty; 
                        rdfs:comment """This verb is used to associate a `DrillingDataPoint` as the `Min` value of `MinMaxUncertainty`
"""@EN; 
                        rdfs:domain ddhub:MinMaxUncertainty; 
                        rdfs:range ddhub:DrillingDataPoint; 
                        rdfs:subPropertyOf ddhub:DWISVerb. 
ddhub:HasUncertaintyPrecision a owl:ObjectProperty; 
                              rdfs:comment """This verb is used to associate a `DrillingDataPoint` as the `Precision` of a `SensorUncertainty`
"""@EN; 
                              rdfs:domain ddhub:SensorUncertainty; 
                              rdfs:range ddhub:DrillingDataPoint; 
                              rdfs:subPropertyOf ddhub:DWISVerb. 
ddhub:HasUncertaintyStandardDeviation a owl:ObjectProperty; 
                                      rdfs:comment """This verb is used to associate a `DrillingDataPoint` as the `StandardDeviation` value of a `GaussianUncertainty`
"""@EN; 
                                      rdfs:domain ddhub:GaussianUncertainty; 
                                      rdfs:range ddhub:DrillingDataPoint; 
                                      rdfs:subPropertyOf ddhub:DWISVerb. 
ddhub:HasUnitAssociation a owl:ObjectProperty; 
                         rdfs:comment """This `Verb` is typically used when defining a `UnitSystem`. It allows to associate a
`UnitSystem` with a `MeasurableQuantityUnitAssociation`.
"""@EN; 
                         rdfs:domain ddhub:UnitSystem; 
                         rdfs:range ddhub:MeasurableQuantityUnitAssociation; 
                         rdfs:subPropertyOf ddhub:DWISVerb. 
ddhub:HasUnitOfMeasure a owl:ObjectProperty; 
                       rdfs:comment ""@EN; 
                       rdfs:domain ddhub:DrillingSignal; 
                       rdfs:range ddhub:Unit; 
                       rdfs:subPropertyOf ddhub:DWISVerb. 
ddhub:HasValue a owl:ObjectProperty; 
               rdfs:comment ""@EN; 
               rdfs:domain ddhub:DrillingDataPoint; 
               rdfs:range ddhub:DrillingSignal; 
               rdfs:subPropertyOf ddhub:DWISVerb. 
ddhub:HeatTransferCoefficientDrillingQuantity a owl:Class; 
                                              rdfs:comment """Heat transfer coefficient is a measure of the efficiency with which heat is transferred between a solid surface and a fluid (or between two fluids) per unit area and temperature difference.
The dimension of heat transfer coefficient is:
$$[MK^{-1}T^{-3}]$$.
The SI unit for **heat transfer coefficient** is: watt per square metre per kelvin with the associated unit label $\\frac{W}{m^{2} \\cdot K}$
The meaningful precision of heat transfer coefficient in the drilling context is typically: 0.0001 W/m²/K
"""@EN; 
                                              rdfs:subClassOf ddhub:MeasurableQuantity. 
ddhub:HeatTransferCoefficientQuantity a owl:Class; 
                                      rdfs:comment """Heat transfer coefficient is a measure of the efficiency with which heat is transferred between a solid surface and a fluid (or between two fluids) per unit area and temperature difference.
The dimension of heat transfer coefficient is:
$$[MK^{-1}T^{-3}]$$.
The SI unit for **heat transfer coefficient** is: watt per square metre per kelvin with the associated unit label $\\frac{W}{m^{2} \\cdot K}$
"""@EN; 
                                      rdfs:subClassOf ddhub:Quantity. 
ddhub:HeatTransferFeature a owl:Class; 
                          rdfs:comment """A heat transfer feature indicates that something accounts for heat transfer.
"""@EN; 
                          rdfs:subClassOf ddhub:DrillingManagementFeature. 
ddhub:HeaveCompensationSystem a owl:Class; 
                              rdfs:comment ""@EN; 
                              rdfs:subClassOf ddhub:MarineSystem. 
ddhub:Heavyweight a owl:Class; 
                  rdfs:comment ""@EN; 
                  rdfs:subClassOf ddhub:DrillString. 
ddhub:Hectare a owl:Class; 
              rdfs:comment """[v] = a * [SI]
where
[v] is the value in hectare
[SI] is the value in SI
a = 1.0/(Hecto*Hecto), i.e., 0.0001
and
Hecto = 100.0
"""@EN; 
              rdfs:subClassOf ddhub:Unit. 
ddhub:Hectogram a owl:Class; 
                rdfs:comment """[v] = a * [SI]
where
[v] is the value in hectogram
[SI] is the value in SI
a = 1.0/Deci, i.e., 10
and
Deci = 0.1
"""@EN; 
                rdfs:subClassOf ddhub:Unit. 
ddhub:Hectometre a owl:Class; 
                 rdfs:comment """[v] = a * [SI]
where
[v] is the value in hectometre
[SI] is the value in SI
a = 1.0/Hecto, i.e., 0.01
and
Hecto = 100.0
"""@EN; 
                 rdfs:subClassOf ddhub:Unit. 
ddhub:Hectowatt a owl:Class; 
                rdfs:comment """[v] = a * [SI]
where
[v] is the value in hectowatt
[SI] is the value in SI
a = 1.0/Hecto, i.e., 0.01
and
Hecto = 100.0
"""@EN; 
                rdfs:subClassOf ddhub:Unit. 
ddhub:Hefnerkerze a owl:Class; 
                  rdfs:comment """[v] = a * [SI]
where
[v] is the value in hefnerkerze
[SI] is the value in SI
a = 1.0/Hefnerkerze, i.e., 1.0869565217391304
and
Hefnerkerze = 0.92 reference: https://en.wikipedia.org/wiki/Hefner_lamp
"""@EN; 
                  rdfs:subClassOf ddhub:Unit. 
ddhub:HeightDrillingQuantity a owl:Class; 
                             rdfs:comment """Length is a measure of distance.
The dimension of length is:
$$[L]$$.
The SI unit for **length** is: metre with the associated unit label $m$
The meaningful precision of height in the drilling context is typically: 0.001 m
"""@EN; 
                             rdfs:subClassOf ddhub:MeasurableQuantity. 
ddhub:Hertz a owl:Class; 
            rdfs:comment """No conversion necessary as the unit choice is SI
"""@EN; 
            rdfs:subClassOf ddhub:Unit. 
ddhub:HertzPerDay a owl:Class; 
                  rdfs:comment """[v] = a * [SI]
where
[v] is the value in hertz per day
[SI] is the value in SI
a = Day/Unit, i.e., 86400
and
Day = 24.0 * Hour
Unit = 1.0
Hour = 60.0 * Minute
Minute = 60.0
"""@EN; 
                  rdfs:subClassOf ddhub:Unit. 
ddhub:HertzPerHour a owl:Class; 
                   rdfs:comment """[v] = a * [SI]
where
[v] is the value in hertz per hour
[SI] is the value in SI
a = Hour/Unit, i.e., 3600
and
Hour = 60.0 * Minute
Unit = 1.0
Minute = 60.0
"""@EN; 
                   rdfs:subClassOf ddhub:Unit. 
ddhub:HertzPerMinute a owl:Class; 
                     rdfs:comment """[v] = a * [SI]
where
[v] is the value in hertz per minute
[SI] is the value in SI
a = Minute/Unit, i.e., 60
and
Minute = 60.0
Unit = 1.0
"""@EN; 
                     rdfs:subClassOf ddhub:Unit. 
ddhub:HertzPerSecond a owl:Class; 
                     rdfs:comment """No conversion necessary as the unit choice is SI
"""@EN; 
                     rdfs:subClassOf ddhub:Unit. 
ddhub:HertzPerYear a owl:Class; 
                   rdfs:comment """[v] = a * [SI]
where
[v] is the value in hertz per year
[SI] is the value in SI
a = YearJulian/Unit, i.e., 31557600
and
YearJulian = 365.25 * Day
Unit = 1.0
Day = 24.0 * Hour
Hour = 60.0 * Minute
Minute = 60.0
"""@EN; 
                   rdfs:subClassOf ddhub:Unit. 
ddhub:HFTO a owl:Class; 
           rdfs:comment """This Noun is used to refer to high frequency torsional oscillations.
"""@EN; 
           rdfs:subClassOf ddhub:AbnormalTorsionalOscillation. 
ddhub:HighGravitySolidComponent a owl:Class; 
                                rdfs:comment ""@EN; 
                                rdfs:subClassOf ddhub:DrillingFluidSolidComponent. 
ddhub:HighPassFilter a owl:Class; 
                     rdfs:comment ""@EN; 
                     rdfs:subClassOf ddhub:Filter. 
ddhub:HighPressureRiser a owl:Class; 
                        rdfs:comment ""@EN; 
                        rdfs:subClassOf ddhub:SurfaceRiser. 
ddhub:HoistingControlSystem a owl:Class; 
                            rdfs:comment ""@EN; 
                            rdfs:subClassOf ddhub:ControlSystem. 
ddhub:HoistingSystem a owl:Class; 
                     rdfs:comment ""@EN; 
                     rdfs:subClassOf ddhub:RigEquipment. 
ddhub:HoistProcedure a owl:Class; 
                     rdfs:comment """The hoist procedure is used to move the top of the drill-stem from one elevation to another elevation while minimizing
the side effects of swab and surge. 
"""@EN; 
                     rdfs:subClassOf ddhub:DrillingProcedure. 
ddhub:HoleBottomLocation a owl:Class; 
                         rdfs:comment ""@EN; 
                         rdfs:subClassOf ddhub:AbscissaReferenceLocation. 
ddhub:HoleCollapse a owl:Class; 
                   rdfs:comment """This Noun is used to refer to a situation during which there is a hole collapse.
"""@EN; 
                   rdfs:subClassOf ddhub:DrillingIncident. 
ddhub:HoleDepth a owl:Class; 
                rdfs:comment ""@EN; 
                rdfs:subClassOf ddhub:PrototypeData. 
ddhub:HoleOpener a owl:Class; 
                 rdfs:comment ""@EN; 
                 rdfs:subClassOf ddhub:DrillingEquipment. 
ddhub:HoleOpeningFeature a owl:Class; 
                         rdfs:comment """An hole opening feature indicates that something accounts for opening the borehole diameter.
"""@EN; 
                         rdfs:subClassOf ddhub:OnBottomDrillingFeature. 
ddhub:Hook a owl:Class; 
           rdfs:comment ""@EN; 
           rdfs:subClassOf ddhub:HoistingSystem. 
ddhub:HookLoad a owl:Class; 
               rdfs:comment ""@EN; 
               rdfs:subClassOf ddhub:PrototypeData. 
ddhub:HookLoadDrillingQuantity a owl:Class; 
                               rdfs:comment """Mass can be experimentally defined as a measure of the body's inertia, meaning the resistance to acceleration (change of velocity) when a net force is applied. The object's mass also determines the strength of its gravitational attraction to other bodies.
The dimension of mass is:
$$[M]$$.
The SI unit for **mass** is: kilogram with the associated unit label $kg$
The meaningful precision of hook load in the drilling context is typically: 100 kg
"""@EN; 
                               rdfs:subClassOf ddhub:MeasurableQuantity. 
ddhub:HookPosition a owl:Class; 
                   rdfs:comment ""@EN; 
                   rdfs:subClassOf ddhub:PrototypeData. 
ddhub:HookVelocity a owl:Class; 
                   rdfs:comment ""@EN; 
                   rdfs:subClassOf ddhub:PrototypeData. 
ddhub:HorizontalOndulationModelling a owl:Class; 
                                    rdfs:comment """The model accounts for the change of azimuth of some parts of the physical system.
"""@EN; 
                                    rdfs:subClassOf ddhub:TangentialModelling. 
ddhub:Hour a owl:Class; 
           rdfs:comment """[v] = a * [SI]
where
[v] is the value in hour
[SI] is the value in SI
a = 1.0/Hour, i.e., 0.0002777777777777778
and
Hour = 60.0 * Minute
Minute = 60.0
"""@EN; 
           rdfs:subClassOf ddhub:Unit. 
ddhub:HundredWeights a owl:Class; 
                     rdfs:comment """[v] = a * [SI]
where
[v] is the value in hundred weights
[SI] is the value in SI
a = 1.0/(100.0*Pound), i.e., 0.022046226218487758
and
Pound = 0.45359237 reference: https://en.wikipedia.org/wiki/Pound_(mass)
"""@EN; 
                     rdfs:subClassOf ddhub:Unit. 
ddhub:Hybrid a owl:Class; 
             rdfs:comment ""@EN; 
             rdfs:subClassOf ddhub:EquipmentTelemetry. 
ddhub:HybridAnalysisModel a owl:Class; 
                          rdfs:comment """A hybrid analysis model may combine forward and inverse steps in an iterative approach.
"""@EN; 
                          rdfs:subClassOf ddhub:ModelingApproach. 
ddhub:HybridKymera a owl:Class; 
                   rdfs:comment ""@EN; 
                   rdfs:subClassOf ddhub:DrillingBit. 
ddhub:HydraulicBranch a owl:Class; 
                      rdfs:comment ""@EN; 
                      rdfs:subClassOf ddhub:HydraulicLogicalElement. 
ddhub:HydraulicConductivityDrillingQuantity a owl:Class; 
                                            rdfs:comment """A velocity is the time derivative of a position or a displacement: $\\frac{dx}{dt}$, where $x$ is a position and $t$ is time.
The dimension of velocity is:
$$[LT^{-1}]$$.
The SI unit for **velocity** is: metre per second with the associated unit label $\\frac{m}{s}$
The meaningful precision of hydraulic conductivity in the drilling context is typically: 0.001 m/s
"""@EN; 
                                            rdfs:subClassOf ddhub:MeasurableQuantity. 
ddhub:HydraulicConductivityQuantity a owl:Class; 
                                    rdfs:comment """A velocity is the time derivative of a position or a displacement: $\\frac{dx}{dt}$, where $x$ is a position and $t$ is time.
The dimension of velocity is:
$$[LT^{-1}]$$.
The SI unit for **velocity** is: metre per second with the associated unit label $\\frac{m}{s}$
"""@EN; 
                                    rdfs:subClassOf ddhub:Quantity. 
ddhub:HydraulicConnectedState a owl:Class; 
                              rdfs:comment ""@EN; 
                              rdfs:subClassOf ddhub:HydraulicElementState. 
ddhub:HydraulicElementState a owl:Class; 
                            rdfs:comment ""@EN; 
                            rdfs:subClassOf ddhub:DWISNoun. 
ddhub:HydraulicJar a owl:Class; 
                   rdfs:comment ""@EN; 
                   rdfs:subClassOf ddhub:JarringAssembly. 
ddhub:HydraulicJunction a owl:Class; 
                        rdfs:comment ""@EN; 
                        rdfs:subClassOf ddhub:HydraulicLogicalElement. 
ddhub:HydraulicLogicalElement a owl:Class; 
                              rdfs:comment ""@EN; 
                              rdfs:subClassOf ddhub:DWISNoun. 
ddhub:HydraulicMudPump a owl:Class; 
                       rdfs:comment ""@EN; 
                       rdfs:subClassOf ddhub:MudPump. 
ddhub:HydraulicNetwork a owl:Class; 
                       rdfs:comment ""@EN; 
                       rdfs:subClassOf ddhub:HydraulicLogicalElement. 
ddhub:Hydrocyclones a owl:Class; 
                    rdfs:comment ""@EN; 
                    rdfs:subClassOf ddhub:CirculationSystem. 
ddhub:HydromechanicalJar a owl:Class; 
                         rdfs:comment ""@EN; 
                         rdfs:subClassOf ddhub:JarringAssembly. 
ddhub:I a owl:DatatypeProperty, owl:FunctionalProperty; 
        rdfs:comment """Electric current exponent.
SI Unit: Ampere (A)
"""@EN; 
        rdfs:domain ddhub:Quantity; 
        rdfs:range xsd:double. 
ddhub:Ibop a owl:Class; 
           rdfs:comment ""@EN; 
           rdfs:subClassOf ddhub:WellControlSystem. 
ddhub:IdlingState a owl:Class; 
                  rdfs:comment ""@EN; 
                  rdfs:subClassOf ddhub:ProceduralState. 
ddhub:ImageScaleQuantity a owl:Class; 
                         rdfs:comment """Image scale refers to the resolution or level of detail in an image.
The dimension of image scale is:
$$[L^{-1}]$$.
The SI unit for **image scale** is: dot per metre with the associated unit label $dpm$
"""@EN; 
                         rdfs:subClassOf ddhub:MeasurableQuantity. 
ddhub:ImagingTools a owl:Class; 
                   rdfs:comment ""@EN; 
                   rdfs:subClassOf ddhub:LoggingWhileDrillingTools. 
ddhub:ImplementsLimit a owl:ObjectProperty; 
                      rdfs:comment """This Verb is used to indicate that a safe operating envelope function implements a drilling limit.
"""@EN; 
                      rdfs:domain ddhub:SOEFunction; 
                      rdfs:range ddhub:DrillingLimit; 
                      rdfs:subPropertyOf ddhub:DWISVerb. 
ddhub:ImplementsObjective a owl:ObjectProperty; 
                          rdfs:comment """This Verb is used to indicate that a control function implements a drilling objective.
"""@EN; 
                          rdfs:domain ddhub:ControllerFunction; 
                          rdfs:range ddhub:DrillingObjective; 
                          rdfs:subPropertyOf ddhub:DWISVerb. 
ddhub:ImplementsProcedure a owl:ObjectProperty; 
                          rdfs:comment """This Verb is used to indicate that a Procedure Function implements a drilling procedure.
"""@EN; 
                          rdfs:domain ddhub:ProcedureFunction; 
                          rdfs:range ddhub:DrillingProcedure; 
                          rdfs:subPropertyOf ddhub:DWISVerb. 
ddhub:Inch a owl:Class; 
           rdfs:comment """[v] = a * [SI]
where
[v] is the value in inch
[SI] is the value in SI
a = 1.0/Inch, i.e., 39.37007874015748
and
Inch = 0.0254 reference: https://www.nist.gov/pml/owm/si-units-length
"""@EN; 
           rdfs:subClassOf ddhub:Unit. 
ddhub:InchMercuryAt32DegreeFahrenheit a owl:Class; 
                                      rdfs:comment """[v] = a * [SI]
where
[v] is the value in inch mercury at 32 degree fahrenheit
[SI] is the value in SI
a = 1.0/InchMercury32degF, i.e., 3386.3890000000006
and
InchMercury32degF = 1.0/3386.389 reference: https://en.wikipedia.org/wiki/Inch_of_mercury
"""@EN; 
                                      rdfs:subClassOf ddhub:Unit. 
ddhub:InchMercuryAt32DegreeFahrenheitPerHour a owl:Class; 
                                             rdfs:comment """[v] = a * [SI]
where
[v] is the value in inch mercury at 32 degree fahrenheit per hour
[SI] is the value in SI
a = Hour/InchMercury32degF, i.e., 12191000.400000002
and
Hour = 60.0 * Minute
InchMercury32degF = 1.0/3386.389 reference: https://en.wikipedia.org/wiki/Inch_of_mercury
Minute = 60.0
"""@EN; 
                                             rdfs:subClassOf ddhub:Unit. 
ddhub:InchMercuryAt32DegreeFahrenheitPerMinute a owl:Class; 
                                               rdfs:comment """[v] = a * [SI]
where
[v] is the value in inch mercury at 32 degree fahrenheit per minute
[SI] is the value in SI
a = Minute/InchMercury32degF, i.e., 203183.34000000003
and
Minute = 60.0
InchMercury32degF = 1.0/3386.389 reference: https://en.wikipedia.org/wiki/Inch_of_mercury
"""@EN; 
                                               rdfs:subClassOf ddhub:Unit. 
ddhub:InchMercuryAt32DegreeFahrenheitPerSecond a owl:Class; 
                                               rdfs:comment """[v] = a * [SI]
where
[v] is the value in inch mercury at 32 degree fahrenheit per second
[SI] is the value in SI
a = 1.0/InchMercury32degF, i.e., 3386.3890000000006
and
InchMercury32degF = 1.0/3386.389 reference: https://en.wikipedia.org/wiki/Inch_of_mercury
"""@EN; 
                                               rdfs:subClassOf ddhub:Unit. 
ddhub:InchMercuryAt60DegreeFahrenheit a owl:Class; 
                                      rdfs:comment """[v] = a * [SI]
where
[v] is the value in inch mercury at 60 degree fahrenheit
[SI] is the value in SI
a = 1.0/InchMercury60degF, i.e., 3376.85
and
InchMercury60degF = 1.0 / 3376.85 reference: https://en.wikipedia.org/wiki/Inch_of_mercury
"""@EN; 
                                      rdfs:subClassOf ddhub:Unit. 
ddhub:InchMercuryAt60DegreeFahrenheitPerHour a owl:Class; 
                                             rdfs:comment """[v] = a * [SI]
where
[v] is the value in inch mercury at 60 degree fahrenheit per hour
[SI] is the value in SI
a = Hour/InchMercury60degF, i.e., 12156660
and
Hour = 60.0 * Minute
InchMercury60degF = 1.0 / 3376.85 reference: https://en.wikipedia.org/wiki/Inch_of_mercury
Minute = 60.0
"""@EN; 
                                             rdfs:subClassOf ddhub:Unit. 
ddhub:InchMercuryAt60DegreeFahrenheitPerMinute a owl:Class; 
                                               rdfs:comment """[v] = a * [SI]
where
[v] is the value in inch mercury at 60 degree fahrenheit per minute
[SI] is the value in SI
a = Minute/InchMercury60degF, i.e., 202611
and
Minute = 60.0
InchMercury60degF = 1.0 / 3376.85 reference: https://en.wikipedia.org/wiki/Inch_of_mercury
"""@EN; 
                                               rdfs:subClassOf ddhub:Unit. 
ddhub:InchMercuryAt60DegreeFahrenheitPerSecond a owl:Class; 
                                               rdfs:comment """[v] = a * [SI]
where
[v] is the value in inch mercury at 60 degree fahrenheit per second
[SI] is the value in SI
a = 1.0/InchMercury60degF, i.e., 3376.85
and
InchMercury60degF = 1.0 / 3376.85 reference: https://en.wikipedia.org/wiki/Inch_of_mercury
"""@EN; 
                                               rdfs:subClassOf ddhub:Unit. 
ddhub:InchPer32 a owl:Class; 
                rdfs:comment """[v] = a * [SI]
where
[v] is the value in inch per 32
[SI] is the value in SI
a = 1.0/InchPer32, i.e., 1259.8425196850394
and
InchPer32 = Inch / 32.0
Inch = 0.0254 reference: https://www.nist.gov/pml/owm/si-units-length
"""@EN; 
                rdfs:subClassOf ddhub:Unit. 
ddhub:InchPerDay a owl:Class; 
                 rdfs:comment """[v] = a * [SI]
where
[v] is the value in inch per day
[SI] is the value in SI
a = Day/Inch, i.e., 3401574.8031496066
and
Day = 24.0 * Hour
Inch = 0.0254 reference: https://www.nist.gov/pml/owm/si-units-length
Hour = 60.0 * Minute
Minute = 60.0
"""@EN; 
                 rdfs:subClassOf ddhub:Unit. 
ddhub:InchPerFoot a owl:Class; 
                  rdfs:comment """[v] = a * [SI]
where
[v] is the value in inch per foot
[SI] is the value in SI
a = Foot / Inch, i.e., 11.999999999999998
and
Foot = 12.0 * Inch
Inch = 0.0254 reference: https://www.nist.gov/pml/owm/si-units-length
"""@EN; 
                  rdfs:subClassOf ddhub:Unit. 
ddhub:InchPerHour a owl:Class; 
                  rdfs:comment """[v] = a * [SI]
where
[v] is the value in inch per hour
[SI] is the value in SI
a = Hour/Inch, i.e., 141732.28346456692
and
Hour = 60.0 * Minute
Inch = 0.0254 reference: https://www.nist.gov/pml/owm/si-units-length
Minute = 60.0
"""@EN; 
                  rdfs:subClassOf ddhub:Unit. 
ddhub:InchPerHourPerSecond a owl:Class; 
                           rdfs:comment """[v] = a * [SI]
where
[v] is the value in inch per hour per second
[SI] is the value in SI
a = Hour/Inch, i.e., 141732.28346456692
and
Hour = 60.0 * Minute
Inch = 0.0254 reference: https://www.nist.gov/pml/owm/si-units-length
Minute = 60.0
"""@EN; 
                           rdfs:subClassOf ddhub:Unit. 
ddhub:InchPerMile a owl:Class; 
                  rdfs:comment """[v] = a * [SI]
where
[v] is the value in inch per mile
[SI] is the value in SI
a = Mile / Inch, i.e., 63359.99999999999
and
Mile = 1760.0 * Yard reference: https://dictionary.cambridge.org/dictionary/english/mile
Inch = 0.0254 reference: https://www.nist.gov/pml/owm/si-units-length
Yard = 3.0 * Foot
Foot = 12.0 * Inch
"""@EN; 
                  rdfs:subClassOf ddhub:Unit. 
ddhub:InchPerMinute a owl:Class; 
                    rdfs:comment """[v] = a * [SI]
where
[v] is the value in inch per minute
[SI] is the value in SI
a = Minute/Inch, i.e., 2362.2047244094488
and
Minute = 60.0
Inch = 0.0254 reference: https://www.nist.gov/pml/owm/si-units-length
"""@EN; 
                    rdfs:subClassOf ddhub:Unit. 
ddhub:InchPerMinutePerSecond a owl:Class; 
                             rdfs:comment """[v] = a * [SI]
where
[v] is the value in inch per minute per second
[SI] is the value in SI
a = Minute/Inch, i.e., 2362.2047244094488
and
Minute = 60.0
Inch = 0.0254 reference: https://www.nist.gov/pml/owm/si-units-length
"""@EN; 
                             rdfs:subClassOf ddhub:Unit. 
ddhub:InchPerSecond a owl:Class; 
                    rdfs:comment """[v] = a * [SI]
where
[v] is the value in inch per second
[SI] is the value in SI
a = Unit/Inch, i.e., 39.37007874015748
and
Unit = 1.0
Inch = 0.0254 reference: https://www.nist.gov/pml/owm/si-units-length
"""@EN; 
                    rdfs:subClassOf ddhub:Unit. 
ddhub:InchPerSecondSquared a owl:Class; 
                           rdfs:comment """[v] = a * [SI]
where
[v] is the value in inch per second squared
[SI] is the value in SI
a = 1.0/Inch, i.e., 39.37007874015748
and
Inch = 0.0254 reference: https://www.nist.gov/pml/owm/si-units-length
"""@EN; 
                           rdfs:subClassOf ddhub:Unit. 
ddhub:InchPerYard a owl:Class; 
                  rdfs:comment """[v] = a * [SI]
where
[v] is the value in inch per yard
[SI] is the value in SI
a = Yard / Inch, i.e., 36
and
Yard = 3.0 * Foot
Inch = 0.0254 reference: https://www.nist.gov/pml/owm/si-units-length
Foot = 12.0 * Inch
"""@EN; 
                  rdfs:subClassOf ddhub:Unit. 
ddhub:InchPound a owl:Class; 
                rdfs:comment """[v] = a * [SI]
where
[v] is the value in inch pound
[SI] is the value in SI
a = 1.0/(PoundForce*Inch), i.e., 8.850745791327185
and
PoundForce = Pound * G reference: https://en.wikipedia.org/wiki/Pound_(force)
Inch = 0.0254 reference: https://www.nist.gov/pml/owm/si-units-length
Pound = 0.45359237 reference: https://en.wikipedia.org/wiki/Pound_(mass)
G = 9.80665 reference: https://en.wikipedia.org/wiki/Gravity_of_Earth
"""@EN; 
                rdfs:subClassOf ddhub:Unit. 
ddhub:InchPoundPerCentimetre a owl:Class; 
                             rdfs:comment """[v] = a * [SI]
where
[v] is the value in inch pound per centimetre
[SI] is the value in SI
a = Centi/(Inch*PoundForce), i.e., 0.08850745791327186
and
Centi = 0.01
Inch = 0.0254 reference: https://www.nist.gov/pml/owm/si-units-length
PoundForce = Pound * G reference: https://en.wikipedia.org/wiki/Pound_(force)
Pound = 0.45359237 reference: https://en.wikipedia.org/wiki/Pound_(mass)
G = 9.80665 reference: https://en.wikipedia.org/wiki/Gravity_of_Earth
"""@EN; 
                             rdfs:subClassOf ddhub:Unit. 
ddhub:InchPoundPerDecimetre a owl:Class; 
                            rdfs:comment """[v] = a * [SI]
where
[v] is the value in inch pound per decimetre
[SI] is the value in SI
a = Deci/(Inch*PoundForce), i.e., 0.8850745791327186
and
Deci = 0.1
Inch = 0.0254 reference: https://www.nist.gov/pml/owm/si-units-length
PoundForce = Pound * G reference: https://en.wikipedia.org/wiki/Pound_(force)
Pound = 0.45359237 reference: https://en.wikipedia.org/wiki/Pound_(mass)
G = 9.80665 reference: https://en.wikipedia.org/wiki/Gravity_of_Earth
"""@EN; 
                            rdfs:subClassOf ddhub:Unit. 
ddhub:InchPoundPerFoot a owl:Class; 
                       rdfs:comment """[v] = a * [SI]
where
[v] is the value in inch pound per foot
[SI] is the value in SI
a = Foot/(Inch*PoundForce), i.e., 2.697707317196526
and
Foot = 12.0 * Inch
Inch = 0.0254 reference: https://www.nist.gov/pml/owm/si-units-length
PoundForce = Pound * G reference: https://en.wikipedia.org/wiki/Pound_(force)
Pound = 0.45359237 reference: https://en.wikipedia.org/wiki/Pound_(mass)
G = 9.80665 reference: https://en.wikipedia.org/wiki/Gravity_of_Earth
"""@EN; 
                       rdfs:subClassOf ddhub:Unit. 
ddhub:InchPoundPerHour a owl:Class; 
                       rdfs:comment """[v] = a * [SI]
where
[v] is the value in inch pound per hour
[SI] is the value in SI
a = Hour/(PoundForce*Inch), i.e., 31862.68484877787
and
Hour = 60.0 * Minute
PoundForce = Pound * G reference: https://en.wikipedia.org/wiki/Pound_(force)
Inch = 0.0254 reference: https://www.nist.gov/pml/owm/si-units-length
Minute = 60.0
Pound = 0.45359237 reference: https://en.wikipedia.org/wiki/Pound_(mass)
G = 9.80665 reference: https://en.wikipedia.org/wiki/Gravity_of_Earth
"""@EN; 
                       rdfs:subClassOf ddhub:Unit. 
ddhub:InchPoundPerInch a owl:Class; 
                       rdfs:comment """[v] = a * [SI]
where
[v] is the value in inch pound per inch
[SI] is the value in SI
a = Inch/(Inch*PoundForce), i.e., 0.2248089430997105
and
Inch = 0.0254 reference: https://www.nist.gov/pml/owm/si-units-length
PoundForce = Pound * G reference: https://en.wikipedia.org/wiki/Pound_(force)
Pound = 0.45359237 reference: https://en.wikipedia.org/wiki/Pound_(mass)
G = 9.80665 reference: https://en.wikipedia.org/wiki/Gravity_of_Earth
"""@EN; 
                       rdfs:subClassOf ddhub:Unit. 
ddhub:InchPoundPerMetre a owl:Class; 
                        rdfs:comment """[v] = a * [SI]
where
[v] is the value in inch pound per metre
[SI] is the value in SI
a = Unit/(Inch*PoundForce), i.e., 8.850745791327185
and
Unit = 1.0
Inch = 0.0254 reference: https://www.nist.gov/pml/owm/si-units-length
PoundForce = Pound * G reference: https://en.wikipedia.org/wiki/Pound_(force)
Pound = 0.45359237 reference: https://en.wikipedia.org/wiki/Pound_(mass)
G = 9.80665 reference: https://en.wikipedia.org/wiki/Gravity_of_Earth
"""@EN; 
                        rdfs:subClassOf ddhub:Unit. 
ddhub:InchPoundPerMillimetre a owl:Class; 
                             rdfs:comment """[v] = a * [SI]
where
[v] is the value in inch pound per millimetre
[SI] is the value in SI
a = Milli/(Inch*PoundForce), i.e., 0.008850745791327186
and
Milli = 0.001
Inch = 0.0254 reference: https://www.nist.gov/pml/owm/si-units-length
PoundForce = Pound * G reference: https://en.wikipedia.org/wiki/Pound_(force)
Pound = 0.45359237 reference: https://en.wikipedia.org/wiki/Pound_(mass)
G = 9.80665 reference: https://en.wikipedia.org/wiki/Gravity_of_Earth
"""@EN; 
                             rdfs:subClassOf ddhub:Unit. 
ddhub:InchPoundPerMinute a owl:Class; 
                         rdfs:comment """[v] = a * [SI]
where
[v] is the value in inch pound per minute
[SI] is the value in SI
a = Minute/(PoundForce*Inch), i.e., 531.0447474796312
and
Minute = 60.0
PoundForce = Pound * G reference: https://en.wikipedia.org/wiki/Pound_(force)
Inch = 0.0254 reference: https://www.nist.gov/pml/owm/si-units-length
Pound = 0.45359237 reference: https://en.wikipedia.org/wiki/Pound_(mass)
G = 9.80665 reference: https://en.wikipedia.org/wiki/Gravity_of_Earth
"""@EN; 
                         rdfs:subClassOf ddhub:Unit. 
ddhub:InchPoundPerSecond a owl:Class; 
                         rdfs:comment """[v] = a * [SI]
where
[v] is the value in inch pound per second
[SI] is the value in SI
a = 1.0/(PoundForce*Inch), i.e., 8.850745791327185
and
PoundForce = Pound * G reference: https://en.wikipedia.org/wiki/Pound_(force)
Inch = 0.0254 reference: https://www.nist.gov/pml/owm/si-units-length
Pound = 0.45359237 reference: https://en.wikipedia.org/wiki/Pound_(mass)
G = 9.80665 reference: https://en.wikipedia.org/wiki/Gravity_of_Earth
"""@EN; 
                         rdfs:subClassOf ddhub:Unit. 
ddhub:InchWaterAt4DegreeCelsius a owl:Class; 
                                rdfs:comment """[v] = a * [SI]
where
[v] is the value in inch water at 4 degree celsius
[SI] is the value in SI
a = 1.0/InchWater4degC, i.e., 0.00401474213311279
and
InchWater4degC = 249.082 reference: https://en.wikipedia.org/wiki/Inch_of_water
"""@EN; 
                                rdfs:subClassOf ddhub:Unit. 
ddhub:InchWaterAt4DegreeCelsiusPerHour a owl:Class; 
                                       rdfs:comment """[v] = a * [SI]
where
[v] is the value in inch water at 4 degree celsius per hour
[SI] is the value in SI
a = Hour/InchWater4degC, i.e., 14.453071679206046
and
Hour = 60.0 * Minute
InchWater4degC = 249.082 reference: https://en.wikipedia.org/wiki/Inch_of_water
Minute = 60.0
"""@EN; 
                                       rdfs:subClassOf ddhub:Unit. 
ddhub:InchWaterAt4DegreeCelsiusPerMinute a owl:Class; 
                                         rdfs:comment """[v] = a * [SI]
where
[v] is the value in inch water at 4 degree celsius per minute
[SI] is the value in SI
a = Minute/InchWater4degC, i.e., 0.2408845279867674
and
Minute = 60.0
InchWater4degC = 249.082 reference: https://en.wikipedia.org/wiki/Inch_of_water
"""@EN; 
                                         rdfs:subClassOf ddhub:Unit. 
ddhub:InchWaterAt4DegreeCelsiusPerSecond a owl:Class; 
                                         rdfs:comment """[v] = a * [SI]
where
[v] is the value in inch water at 4 degree celsius per second
[SI] is the value in SI
a = 1.0/InchWater4degC, i.e., 0.00401474213311279
and
InchWater4degC = 249.082 reference: https://en.wikipedia.org/wiki/Inch_of_water
"""@EN; 
                                         rdfs:subClassOf ddhub:Unit. 
ddhub:Inclination a owl:Class; 
                  rdfs:comment ""@EN; 
                  rdfs:subClassOf ddhub:PrototypeData. 
ddhub:InductionCouplingDownholeTelemetry a owl:Class; 
                                         rdfs:comment """A method that allows transfer of downhole data to the surface via induction coupling between pipes along the drill-string.
"""@EN; 
                                         rdfs:subClassOf ddhub:WiredPipeTelemetry. 
ddhub:Influx a owl:Class; 
             rdfs:comment """This Noun is used to refer to a situation during which there is an influx of formation fluids in the borehole.
"""@EN; 
             rdfs:subClassOf ddhub:DrillingIncident. 
ddhub:InjectorHead a owl:Class; 
                   rdfs:comment ""@EN; 
                   rdfs:subClassOf ddhub:CoiledTubingEquipment. 
ddhub:InnerBarrel a owl:Class; 
                  rdfs:comment ""@EN; 
                  rdfs:subClassOf ddhub:CoringTool. 
ddhub:InnerString a owl:Class; 
                  rdfs:comment ""@EN; 
                  rdfs:subClassOf ddhub:CasingEquipment. 
ddhub:InsertTci a owl:Class; 
                rdfs:comment ""@EN; 
                rdfs:subClassOf ddhub:RollingCutter. 
ddhub:InstrumentedMotor a owl:Class; 
                        rdfs:comment ""@EN; 
                        rdfs:subClassOf ddhub:DownholeMotor. 
ddhub:Integral a owl:Class; 
               rdfs:comment ""@EN; 
               rdfs:subClassOf ddhub:BladeType. 
ddhub:IntegralModel a owl:Class; 
                    rdfs:comment """A model that uses integral equations.
"""@EN; 
                    rdfs:subClassOf ddhub:MathematicalFormulation. 
ddhub:Integration a owl:Class; 
                  rdfs:comment ""@EN; 
                  rdfs:subClassOf ddhub:TimeBasedTransformation. 
ddhub:InterfacialTensionDrillingQuantity a owl:Class; 
                                         rdfs:comment """Interfacial tension is the force per unit length acting along the boundary between two immiscible liquids, resisting their mixing.
The dimension of interfacial tension is:
$$[MT^{-2}]$$.
The SI unit for **interfacial tension** is: newton per metre with the associated unit label $\\frac{N}{m}$
The meaningful precision of interfacial tension in the drilling context is typically: 0.0001 N/m
"""@EN; 
                                         rdfs:subClassOf ddhub:MeasurableQuantity. 
ddhub:InterfacialTensionQuantity a owl:Class; 
                                 rdfs:comment """Interfacial tension is the force per unit length acting along the boundary between two immiscible liquids, resisting their mixing.
The dimension of interfacial tension is:
$$[MT^{-2}]$$.
The SI unit for **interfacial tension** is: newton per metre with the associated unit label $\\frac{N}{m}$
"""@EN; 
                                 rdfs:subClassOf ddhub:Quantity. 
ddhub:InternationalCandle a owl:Class; 
                          rdfs:comment """[v] = a * [SI]
where
[v] is the value in international candle
[SI] is the value in SI
a = 1.0/InternationalCandle, i.e., 0.9803921568627451
and
InternationalCandle = 1.02
"""@EN; 
                          rdfs:subClassOf ddhub:Unit. 
ddhub:InternationalNauticalMile a owl:Class; 
                                rdfs:comment """[v] = a * [SI]
where
[v] is the value in international nautical mile
[SI] is the value in SI
a = 1.0/InternationalNauticalMile, i.e., 0.0005399568034557236
and
InternationalNauticalMile = 1852.0 reference: https://www.merriam-webster.com/dictionary/nautical%20mile
"""@EN; 
                                rdfs:subClassOf ddhub:Unit. 
ddhub:Interpreter a owl:Class; 
                  rdfs:comment """An interpreter is a computation unit that interprets the state of a process. Its output is typically a
ComputedState.
"""@EN; 
                  rdfs:subClassOf ddhub:ComputationUnit. 
ddhub:InverseAtmosphere a owl:Class; 
                        rdfs:comment """[v] = a * [SI]
where
[v] is the value in inverse atmosphere
[SI] is the value in SI
a = Atmosphere, i.e., 101325
and
Atmosphere = 101325.0 reference: https://en.wikipedia.org/wiki/Atmospheric_pressure
"""@EN; 
                        rdfs:subClassOf ddhub:Unit. 
ddhub:InverseBar a owl:Class; 
                 rdfs:comment """[v] = a * [SI]
where
[v] is the value in inverse bar
[SI] is the value in SI
a = Bar, i.e., 100000
and
Bar = 1e5 reference: https://en.wikipedia.org/wiki/Bar_(unit)
"""@EN; 
                 rdfs:subClassOf ddhub:Unit. 
ddhub:InversePascal a owl:Class; 
                    rdfs:comment """No conversion necessary as the unit choice is SI
"""@EN; 
                    rdfs:subClassOf ddhub:Unit. 
ddhub:InversePoundPerSquareInch a owl:Class; 
                                rdfs:comment """[v] = a * [SI]
where
[v] is the value in inverse pound per square inch
[SI] is the value in SI
a = PSI, i.e., 6894.757293168361
and
PSI = PoundForce / (Inch * Inch) reference: https://en.wikipedia.org/wiki/Pound_per_square_inch
PoundForce = Pound * G reference: https://en.wikipedia.org/wiki/Pound_(force)
Inch = 0.0254 reference: https://www.nist.gov/pml/owm/si-units-length
Pound = 0.45359237 reference: https://en.wikipedia.org/wiki/Pound_(mass)
G = 9.80665 reference: https://en.wikipedia.org/wiki/Gravity_of_Earth
"""@EN; 
                                rdfs:subClassOf ddhub:Unit. 
ddhub:InversionModel a owl:Class; 
                     rdfs:comment """For an inversion model, the outputs are used to infer inputs or parameters.
"""@EN; 
                     rdfs:subClassOf ddhub:ModelingApproach. 
ddhub:IronRoughneck a owl:Class; 
                    rdfs:comment ""@EN; 
                    rdfs:subClassOf ddhub:DrillFloorEquipment. 
ddhub:IsAContextOf a owl:ObjectProperty; 
                   rdfs:comment """this Verb is used to relate a context to its parent task step.
"""@EN; 
                   rdfs:domain ddhub:Context; 
                   rdfs:range ddhub:TaskStep; 
                   rdfs:subPropertyOf ddhub:DWISVerb. 
ddhub:IsActivatedSignalFor a owl:ObjectProperty; 
                           rdfs:comment """This verb is used to define a `DrillingDataPoint` that indicates if the `ActivableFunction` is activated or
not. It is expected that the `DrillingDataPoint` is a Boolean value.
"""@EN; 
                           rdfs:domain ddhub:DrillingDataPoint; 
                           rdfs:range ddhub:ActivableFunction; 
                           rdfs:subPropertyOf ddhub:DWISVerb. 
ddhub:IsAHydraulicRepresentationFor a owl:ObjectProperty; 
                                    rdfs:comment ""@EN; 
                                    rdfs:domain ddhub:HydraulicLogicalElement; 
                                    rdfs:range ddhub:DrillingEquipment; 
                                    rdfs:subPropertyOf ddhub:DWISVerb. 
ddhub:IsAMechanicalRepresentationFor a owl:ObjectProperty; 
                                     rdfs:comment ""@EN; 
                                     rdfs:domain ddhub:MechanicalLogicalElement; 
                                     rdfs:range ddhub:DrillingEquipment; 
                                     rdfs:subPropertyOf ddhub:DWISVerb. 
ddhub:IsAnActionOf a owl:ObjectProperty; 
                   rdfs:comment """this Verb is used to relate an action step to its parent phase step.
"""@EN; 
                   rdfs:domain ddhub:ActionStep; 
                   rdfs:range ddhub:PhaseStep; 
                   rdfs:subPropertyOf ddhub:DWISVerb. 
ddhub:IsArmedSignalFor a owl:ObjectProperty; 
                       rdfs:comment """This verb is used to indicate a `DrillingDataPoint` used by an `FDIRFunction` tells if the FDIR function is armed and operative.
The signal is supposed to be a Boolean value.
The FDIR function may be active, but the current state of the drilling process may imply that the function cannot be
triggered. For instance, a pack-off FDIR may be active but would react only if the flow is supposed to be steady state.
"""@EN; 
                       rdfs:domain ddhub:DrillingDataPoint; 
                       rdfs:range ddhub:FDIRFunction; 
                       rdfs:subPropertyOf ddhub:DWISVerb. 
ddhub:IsATaskOf a owl:ObjectProperty; 
                rdfs:comment """this Verb is used to relate an task step to its parent action step.
"""@EN; 
                rdfs:domain ddhub:TaskStep; 
                rdfs:range ddhub:ActionStep; 
                rdfs:subPropertyOf ddhub:DWISVerb. 
ddhub:IsAuxiliary a owl:DatatypeProperty, owl:FunctionalProperty; 
                  rdfs:comment """This attribute specifies if the function is a main or an auxilary one. A main function impacts
substantially the drilling process while an auxiliary function does not impact or only in limited fashion the
drilling process. Example of a main functions are: Hoist, Tag Bottom, Start Circulation, Start Rotation,
Stop Circulation, Stop Rotation, Drill, Pull Out,Run In, Pull Out With Lubrication, Run In With Lubrication, Ream Up,
Ream Down,Test Friction, Reciprocate, Test Pressure Integrity, Place Cement, .... Example of auxiliary functions
are: Boost Riser Flow, Down Link from ADCS, Rock Pipe, ...
"""@EN; 
                  rdfs:domain ddhub:RunnableFunction; 
                  rdfs:range xsd:boolean. 
ddhub:IsBufferingInput a owl:ObjectProperty; 
                       rdfs:comment ""@EN; 
                       rdfs:domain ddhub:DrillingDataPoint; 
                       rdfs:range ddhub:Buffering; 
                       rdfs:subPropertyOf ddhub:IsTransformationInput. 
ddhub:IsBufferingOutput a owl:ObjectProperty; 
                        rdfs:comment ""@EN; 
                        rdfs:domain ddhub:DrillingDataPoint; 
                        rdfs:range ddhub:Buffering; 
                        rdfs:subPropertyOf ddhub:IsTransformationOutput. 
ddhub:IsCharacterizedBy a owl:ObjectProperty; 
                        rdfs:comment """this Verb is used to state some characteristics of a well bore data.
"""@EN; 
                        rdfs:domain ddhub:WellBoreData; 
                        rdfs:range ddhub:WellBoreDataCharateristic; 
                        rdfs:subPropertyOf ddhub:DWISVerb. 
ddhub:IsCommandFor a owl:ObjectProperty; 
                   rdfs:comment ""@EN; 
                   rdfs:domain ddhub:DrillingDataPoint; 
                   rdfs:range ddhub:DWISNoun; 
                   rdfs:subPropertyOf ddhub:HasFunction. 
ddhub:IsComputationInput a owl:ObjectProperty; 
                         rdfs:comment ""@EN; 
                         rdfs:domain ddhub:DrillingDataPoint; 
                         rdfs:range ddhub:ComputationUnit; 
                         rdfs:subPropertyOf ddhub:HasFunction. 
ddhub:IsComputedBy a owl:ObjectProperty; 
                   rdfs:comment ""@EN; 
                   rdfs:domain ddhub:DWISNoun; 
                   rdfs:range ddhub:DWISNoun; 
                   rdfs:subPropertyOf ddhub:IsGeneratedBy. 
ddhub:IsConditionedBy a owl:ObjectProperty; 
                      rdfs:comment ""@EN; 
                      rdfs:domain ddhub:DrillingDataPoint; 
                      rdfs:range ddhub:ValidityCondition; 
                      rdfs:subPropertyOf ddhub:DWISVerb. 
ddhub:IsConditionInput a owl:ObjectProperty; 
                       rdfs:comment ""@EN; 
                       rdfs:domain ddhub:DrillingDataPoint; 
                       rdfs:range ddhub:ValidityCondition; 
                       rdfs:subPropertyOf ddhub:DWISVerb. 
ddhub:IsConditionLeft a owl:ObjectProperty; 
                      rdfs:comment ""@EN; 
                      rdfs:domain ddhub:DWISNoun; 
                      rdfs:range ddhub:DWISNoun; 
                      rdfs:subPropertyOf ddhub:IsConditionInput. 
ddhub:IsConditionRight a owl:ObjectProperty; 
                       rdfs:comment ""@EN; 
                       rdfs:domain ddhub:DWISNoun; 
                       rdfs:range ddhub:DWISNoun; 
                       rdfs:subPropertyOf ddhub:IsConditionInput. 
ddhub:IsDependentOn a owl:ObjectProperty; 
                    rdfs:comment """This verb is used to describe a general dependence relationship between a `DrillingDataPoint` and something else.
"""@EN; 
                    rdfs:domain ddhub:DrillingDataPoint; 
                    rdfs:range ddhub:DWISNoun; 
                    rdfs:subPropertyOf ddhub:DWISVerb. 
ddhub:IsDerivationInput a owl:ObjectProperty; 
                        rdfs:comment ""@EN; 
                        rdfs:domain ddhub:DWISNoun; 
                        rdfs:range ddhub:DWISNoun; 
                        rdfs:subPropertyOf ddhub:IsTransformationInput. 
ddhub:IsDerivedFrom a owl:ObjectProperty; 
                    rdfs:comment ""@EN; 
                    rdfs:domain ddhub:DWISNoun; 
                    rdfs:range ddhub:DWISNoun; 
                    rdfs:subPropertyOf ddhub:IsTransformationOutput. 
ddhub:IsEnablingSignalFor a owl:ObjectProperty; 
                          rdfs:comment """This verb is used to define a `DrillingDataPoint` that is used to enable or disable an `ActivableFunction`.
It is expected that the `DrillingDataPoint` is a Boolean value.
"""@EN; 
                          rdfs:domain ddhub:DrillingDataPoint; 
                          rdfs:range ddhub:ActivableFunction; 
                          rdfs:subPropertyOf ddhub:DWISVerb. 
ddhub:IsEquivalentCirculationDensityAt a owl:ObjectProperty; 
                                       rdfs:comment ""@EN; 
                                       rdfs:domain ddhub:DrillingDataPoint; 
                                       rdfs:range ddhub:HydraulicLogicalElement; 
                                       rdfs:subPropertyOf ddhub:IsHydraulicallyLocatedAt. 
ddhub:IsFeatureSignalFor a owl:ObjectProperty; 
                         rdfs:comment """This verbs is used to indicate that a `DrillingDataPoint` describes a feature of an `ActivableFunction`
"""@EN; 
                         rdfs:domain ddhub:DrillingDataPoint; 
                         rdfs:range ddhub:ActivableFunction; 
                         rdfs:subPropertyOf ddhub:DWISVerb. 
ddhub:IsFluidDensityAt a owl:ObjectProperty; 
                       rdfs:comment ""@EN; 
                       rdfs:domain ddhub:DrillingDataPoint; 
                       rdfs:range ddhub:HydraulicLogicalElement; 
                       rdfs:subPropertyOf ddhub:IsHydraulicallyLocatedAt. 
ddhub:IsFluidTemperatureAt a owl:ObjectProperty; 
                           rdfs:comment ""@EN; 
                           rdfs:domain ddhub:DrillingDataPoint; 
                           rdfs:range ddhub:HydraulicLogicalElement; 
                           rdfs:subPropertyOf ddhub:IsHydraulicallyLocatedAt. 
ddhub:IsFluidVelocityAt a owl:ObjectProperty; 
                        rdfs:comment ""@EN; 
                        rdfs:domain ddhub:DrillingDataPoint; 
                        rdfs:range ddhub:HydraulicLogicalElement; 
                        rdfs:subPropertyOf ddhub:IsHydraulicallyLocatedAt. 
ddhub:IsForMotionType a owl:ObjectProperty; 
                      rdfs:comment ""@EN; 
                      rdfs:domain ddhub:DrillingDataPoint; 
                      rdfs:range ddhub:MotionType; 
                      rdfs:subPropertyOf ddhub:DWISVerb. 
ddhub:IsGeneratedBy a owl:ObjectProperty; 
                    rdfs:comment ""@EN; 
                    rdfs:domain ddhub:DrillingDataPoint; 
                    rdfs:range ddhub:DataFlowNode; 
                    rdfs:subPropertyOf ddhub:DWISVerb. 
ddhub:IsHydraulicallyLocatedAt a owl:ObjectProperty; 
                               rdfs:comment ""@EN; 
                               rdfs:domain ddhub:DrillingDataPoint; 
                               rdfs:range ddhub:HydraulicLogicalElement; 
                               rdfs:subPropertyOf ddhub:DWISVerb. 
ddhub:IsHydraulicConnectedTo a owl:ObjectProperty; 
                             rdfs:comment ""@EN; 
                             rdfs:domain ddhub:HydraulicLogicalElement; 
                             rdfs:range ddhub:HydraulicLogicalElement; 
                             rdfs:subPropertyOf ddhub:DWISVerb. 
ddhub:IsHydraulicEstimationAt a owl:ObjectProperty; 
                              rdfs:comment ""@EN; 
                              rdfs:domain ddhub:DrillingDataPoint; 
                              rdfs:range ddhub:HydraulicLogicalElement; 
                              rdfs:subPropertyOf ddhub:IsHydraulicallyLocatedAt. 
ddhub:IsHydraulicMaximumAllowedRateOfChangeAt a owl:ObjectProperty; 
                                              rdfs:comment ""@EN; 
                                              rdfs:domain ddhub:DrillingDataPoint; 
                                              rdfs:range ddhub:HydraulicLogicalElement; 
                                              rdfs:subPropertyOf ddhub:IsHydraulicallyLocatedAt. 
ddhub:IsHydraulicMaximumAllowedValueAt a owl:ObjectProperty; 
                                       rdfs:comment ""@EN; 
                                       rdfs:domain ddhub:DrillingDataPoint; 
                                       rdfs:range ddhub:HydraulicLogicalElement; 
                                       rdfs:subPropertyOf ddhub:IsHydraulicallyLocatedAt. 
ddhub:IsHydraulicMeasurementAt a owl:ObjectProperty; 
                               rdfs:comment ""@EN; 
                               rdfs:domain ddhub:DrillingDataPoint; 
                               rdfs:range ddhub:HydraulicLogicalElement; 
                               rdfs:subPropertyOf ddhub:IsHydraulicallyLocatedAt. 
ddhub:IsIdlingAfterTriggeredSignalFor a owl:ObjectProperty; 
                                      rdfs:comment """This verb is used to indicate that a `DrillingDataPoint` tells whether the isolation or the recovery
"""@EN; 
                                      rdfs:domain ddhub:DrillingDataPoint; 
                                      rdfs:range ddhub:FDIRFunction; 
                                      rdfs:subPropertyOf ddhub:DWISVerb. 
ddhub:IsIdlingSignalFor a owl:ObjectProperty; 
                        rdfs:comment """This verb is used to indicate a `DrillingDataPoint` that tells if the function is in an idle state.
A function that is idle must be enabled but does not perform any particular control on the machines. For instance, a 
`ProcedureFunction` that has reached its terminal state or a `ControllerFunction` that cannot control anymore its 
parameter because a limit is reached, e.g., autodriller when reaching the `MinDrillHeightVerticalLocation`, or an FDIR
function when there are no incidents that is detected. A SOE function is in idle state, if the used set-points are
within the limits, but if the limits are applied then the idle state is false, because the function acts on the set-points.
"""@EN; 
                        rdfs:domain ddhub:DrillingDataPoint; 
                        rdfs:range ddhub:RunnableFunction; 
                        rdfs:subPropertyOf ddhub:DWISVerb. 
ddhub:IsImpactDescriptionSignalFor a owl:ObjectProperty; 
                                   rdfs:comment """This verbs is used to indicate that a `DrillingDataPoint` used by an `FDIRFunction` can be used to
describe the impact of the function on the drilling process. This signal is supposed to be string value.
"""@EN; 
                                   rdfs:domain ddhub:DrillingDataPoint; 
                                   rdfs:range ddhub:FDIRFunction; 
                                   rdfs:subPropertyOf ddhub:DWISVerb. 
ddhub:IsIntegratedFrom a owl:ObjectProperty; 
                       rdfs:comment ""@EN; 
                       rdfs:domain ddhub:DWISNoun; 
                       rdfs:range ddhub:DWISNoun; 
                       rdfs:subPropertyOf ddhub:IsTransformationOutput. 
ddhub:IsLimitFor a owl:ObjectProperty; 
                 rdfs:comment ""@EN; 
                 rdfs:domain ddhub:DrillingDataPoint; 
                 rdfs:range ddhub:DWISNoun; 
                 rdfs:subPropertyOf ddhub:HasFunction. 
ddhub:IsMassFlowRateAt a owl:ObjectProperty; 
                       rdfs:comment ""@EN; 
                       rdfs:domain ddhub:DrillingDataPoint; 
                       rdfs:range ddhub:HydraulicLogicalElement; 
                       rdfs:subPropertyOf ddhub:IsHydraulicallyLocatedAt. 
ddhub:IsMaximumLimitFor a owl:ObjectProperty; 
                        rdfs:comment ""@EN; 
                        rdfs:domain ddhub:DrillingDataPoint; 
                        rdfs:range ddhub:DWISNoun; 
                        rdfs:subPropertyOf ddhub:IsLimitFor. 
ddhub:IsMeasuredBy a owl:ObjectProperty; 
                   rdfs:comment ""@EN; 
                   rdfs:domain ddhub:DWISNoun; 
                   rdfs:range ddhub:DWISNoun; 
                   rdfs:subPropertyOf ddhub:IsGeneratedBy. 
ddhub:IsMechanicallyConnectedTo a owl:ObjectProperty; 
                                rdfs:comment ""@EN; 
                                rdfs:domain ddhub:MechanicalLogicalElement; 
                                rdfs:range ddhub:MechanicalLogicalElement; 
                                rdfs:subPropertyOf ddhub:DWISVerb. 
ddhub:IsMechanicallyLocatedAt a owl:ObjectProperty; 
                              rdfs:comment ""@EN; 
                              rdfs:domain ddhub:DrillingDataPoint; 
                              rdfs:range ddhub:MechanicalLogicalElement; 
                              rdfs:subPropertyOf ddhub:DWISVerb. 
ddhub:IsMinimumLimitFor a owl:ObjectProperty; 
                        rdfs:comment ""@EN; 
                        rdfs:domain ddhub:DrillingDataPoint; 
                        rdfs:range ddhub:DWISNoun; 
                        rdfs:subPropertyOf ddhub:IsLimitFor. 
ddhub:IsobaricSpecificHeatCapacityDrillingQuantity a owl:Class; 
                                                   rdfs:comment """Isobaric specific heat capacity is the amount of heat required to raise the temperature of one unit mass of a substance by one unit of temperature at constant pressure. It indicates how much heat energy a material can store.
The dimension of specific heat capacity is:
$$[L^{2}K^{-1}T^{-2}]$$.
The SI unit for **isobaric specific heat capacity** is: joule per kilogram kelvin with the associated unit label $\\frac{J}{kg \\cdot K}$
The meaningful precision of specific heat capacity in the drilling context is typically: 0.01 J/kg•K
"""@EN; 
                                                   rdfs:subClassOf ddhub:MeasurableQuantity. 
ddhub:IsobaricSpecificHeatCapacityGradientPerTemperatureDrillingQuantity a owl:Class; 
                                                                         rdfs:comment """An isobaric specific heat capacity gradient per temperature is the first derivative of an isobaric specific heat capacity compared to temperature: $\\frac{dC_p}{dT}$, where $C_p$ is a isobaric specific heat capacity and $T$ is a temperature.
The dimension of specific heat capacity gradient per temperature is:
$$[L^{2}T^{-2}K^{-2}]$$.
The SI unit for **isobaric specific heat capacity gradient per temperature** is: joule per kilogram squared kelvin with the associated unit label $\\frac{J}{kg \\cdot K^{2}}$
The meaningful precision of isobaric specific heat capacity gradient per temperature in the drilling context is typically: 0.01 J/kg•K²
"""@EN; 
                                                                         rdfs:subClassOf ddhub:MeasurableQuantity. 
ddhub:IsobaricSpecificHeatCapacityGradientPerTemperatureQuantity a owl:Class; 
                                                                 rdfs:comment """An isobaric specific heat capacity gradient per temperature is the first derivative of an isobaric specific heat capacity compared to temperature: $\\frac{dC_p}{dT}$, where $C_p$ is a isobaric specific heat capacity and $T$ is a temperature.
The dimension of specific heat capacity gradient per temperature is:
$$[L^{2}T^{-2}K^{-2}]$$.
The SI unit for **isobaric specific heat capacity gradient per temperature** is: joule per kilogram squared kelvin with the associated unit label $\\frac{J}{kg \\cdot K^{2}}$
"""@EN; 
                                                                 rdfs:subClassOf ddhub:Quantity. 
ddhub:IsobaricSpecificHeatCapacityQuantity a owl:Class; 
                                           rdfs:comment """Isobaric specific heat capacity is the amount of heat required to raise the temperature of one unit mass of a substance by one unit of temperature at constant pressure. It indicates how much heat energy a material can store.
The dimension of specific heat capacity is:
$$[L^{2}K^{-1}T^{-2}]$$.
The SI unit for **isobaric specific heat capacity** is: joule per kilogram kelvin with the associated unit label $\\frac{J}{kg \\cdot K}$
"""@EN; 
                                           rdfs:subClassOf ddhub:Quantity. 
ddhub:IsObservableFrom a owl:ObjectProperty; 
                       rdfs:comment """This `Verb` means that something can be seen, detected, or noticed from a particular
location or perspective. It implies that there is a clear view or means of perception from one point 
to another.
"""@EN; 
                       rdfs:domain ddhub:DWISNoun; 
                       rdfs:range ddhub:DrillingDataPoint; 
                       rdfs:subPropertyOf ddhub:DWISVerb. 
ddhub:IsOfBaseQuantity a owl:ObjectProperty; 
                       rdfs:comment """This `Verb` is used to associate a `MeasurableQuantity` with a `Quantity`. It is the reciprocal
relationship to `HasMeasurableQuantity`. 
"""@EN; 
                       rdfs:domain ddhub:MeasurableQuantity; 
                       rdfs:range ddhub:Quantity; 
                       rdfs:subPropertyOf ddhub:DWISVerb. 
ddhub:IsOfMeasurableQuantity a owl:ObjectProperty; 
                             rdfs:comment """This `verb` is used to relate a `MeasureableQuantity` to a `DrillingDataPoint`.
"""@EN; 
                             rdfs:domain ddhub:DrillingDataPoint; 
                             rdfs:range ddhub:MeasurableQuantity; 
                             rdfs:subPropertyOf ddhub:DWISVerb. 
ddhub:IsOfMechanicalStiffnessType a owl:ObjectProperty; 
                                  rdfs:comment """A relation to describe how the drill-stem mechanical model manage stiffness.
"""@EN; 
                                  rdfs:domain ddhub:DrillStemMechanicalModel; 
                                  rdfs:range ddhub:MechanicalStiffnessType; 
                                  rdfs:subPropertyOf ddhub:DWISVerb. 
ddhub:IsolationSeal a owl:Class; 
                    rdfs:comment ""@EN; 
                    rdfs:subClassOf ddhub:DrillingEquipment. 
ddhub:IsOpeningRatioAt a owl:ObjectProperty; 
                       rdfs:comment ""@EN; 
                       rdfs:domain ddhub:DrillingDataPoint; 
                       rdfs:range ddhub:HydraulicLogicalElement; 
                       rdfs:subPropertyOf ddhub:IsHydraulicallyLocatedAt. 
ddhub:IsPhysicallyLocatedAt a owl:ObjectProperty; 
                            rdfs:comment ""@EN; 
                            rdfs:domain ddhub:DWISNoun; 
                            rdfs:range ddhub:Location; 
                            rdfs:subPropertyOf ddhub:DWISVerb. 
ddhub:IsPressureAt a owl:ObjectProperty; 
                   rdfs:comment ""@EN; 
                   rdfs:domain ddhub:DrillingDataPoint; 
                   rdfs:range ddhub:HydraulicLogicalElement; 
                   rdfs:subPropertyOf ddhub:IsHydraulicallyLocatedAt. 
ddhub:IsPressureGradientAt a owl:ObjectProperty; 
                           rdfs:comment ""@EN; 
                           rdfs:domain ddhub:DrillingDataPoint; 
                           rdfs:range ddhub:HydraulicLogicalElement; 
                           rdfs:subPropertyOf ddhub:IsHydraulicallyLocatedAt. 
ddhub:IsProcessedBy a owl:ObjectProperty; 
                    rdfs:comment ""@EN; 
                    rdfs:domain ddhub:DWISNoun; 
                    rdfs:range ddhub:DWISNoun; 
                    rdfs:subPropertyOf ddhub:DWISVerb. 
ddhub:IsProvidedBy a owl:ObjectProperty; 
                   rdfs:comment ""@EN; 
                   rdfs:domain ddhub:DWISNoun; 
                   rdfs:range ddhub:DataProvider; 
                   rdfs:subPropertyOf ddhub:DWISVerb. 
ddhub:IsProvidedTo a owl:ObjectProperty; 
                   rdfs:comment ""@EN; 
                   rdfs:domain ddhub:DWISNoun; 
                   rdfs:range ddhub:DataProvider; 
                   rdfs:subPropertyOf ddhub:DWISVerb. 
ddhub:IsRecommendedBy a owl:ObjectProperty; 
                      rdfs:comment """Indicates that the AdvisorySystemAdvice is recommended by an Advisor
"""@EN; 
                      rdfs:domain ddhub:AdvisorySystemAdvice; 
                      rdfs:range ddhub:ComputationUnit; 
                      rdfs:subPropertyOf ddhub:DWISVerb. 
ddhub:IsRecommendedFor a owl:ObjectProperty; 
                       rdfs:comment """Indicates that the AdvisorySystemAdvice is recommended for an ADCS Activable Function
"""@EN; 
                       rdfs:domain ddhub:AdvisorySystemAdvice; 
                       rdfs:range ddhub:ActivableFunction; 
                       rdfs:subPropertyOf ddhub:DWISVerb. 
ddhub:IsRecordedFrom a owl:ObjectProperty; 
                     rdfs:comment ""@EN; 
                     rdfs:domain ddhub:DWISNoun; 
                     rdfs:range ddhub:DWISNoun; 
                     rdfs:subPropertyOf ddhub:IsGeneratedBy. 
ddhub:IsRelatedToDrillingIncident a owl:ObjectProperty; 
                                  rdfs:comment """This Verb is used to indicate that a drilling data point is related to a drilling incident.
"""@EN; 
                                  rdfs:domain ddhub:DrillingDataPoint; 
                                  rdfs:range ddhub:DrillingIncident; 
                                  rdfs:subPropertyOf ddhub:DWISVerb. 
ddhub:IsRelatedToDrillingLimit a owl:ObjectProperty; 
                               rdfs:comment """This Verb is used to indicate that a drilling data point is related to a drilling incident.
"""@EN; 
                               rdfs:domain ddhub:DrillingDataPoint; 
                               rdfs:range ddhub:DrillingLimit; 
                               rdfs:subPropertyOf ddhub:DWISVerb. 
ddhub:IsRelatedToDrillingObjective a owl:ObjectProperty; 
                                   rdfs:comment """This Verb is used to indicate that a drilling data point is related to a drilling objective.
"""@EN; 
                                   rdfs:domain ddhub:DrillingDataPoint; 
                                   rdfs:range ddhub:DrillingObjective; 
                                   rdfs:subPropertyOf ddhub:DWISVerb. 
ddhub:IsRelatedToDrillingProcedure a owl:ObjectProperty; 
                                   rdfs:comment """This Verb is used to indicate that a drilling data point is related to a drilling procedure.
"""@EN; 
                                   rdfs:domain ddhub:DrillingDataPoint; 
                                   rdfs:range ddhub:DrillingProcedure; 
                                   rdfs:subPropertyOf ddhub:DWISVerb. 
ddhub:IsResampledBy a owl:ObjectProperty; 
                    rdfs:comment ""@EN; 
                    rdfs:domain ddhub:DrillingDataPoint; 
                    rdfs:range ddhub:Resampling; 
                    rdfs:subPropertyOf ddhub:IsTransformationOutput. 
ddhub:IsResamplingInput a owl:ObjectProperty; 
                        rdfs:comment ""@EN; 
                        rdfs:domain ddhub:DrillingDataPoint; 
                        rdfs:range ddhub:Resampling; 
                        rdfs:subPropertyOf ddhub:IsTransformationInput. 
ddhub:IsSetPointAdviceFor a owl:ObjectProperty; 
                          rdfs:comment ""@EN; 
                          rdfs:domain ddhub:DrillingDataPoint; 
                          rdfs:range ddhub:ControlSystem; 
                          rdfs:subPropertyOf ddhub:HasFunction. 
ddhub:IsSetPointFor a owl:ObjectProperty; 
                    rdfs:comment ""@EN; 
                    rdfs:domain ddhub:DrillingDataPoint; 
                    rdfs:range ddhub:Controller; 
                    rdfs:subPropertyOf ddhub:HasFunction. 
ddhub:IsSetPointMaximumAdviceFor a owl:ObjectProperty; 
                                 rdfs:comment ""@EN; 
                                 rdfs:domain ddhub:DrillingDataPoint; 
                                 rdfs:range ddhub:ControlSystem; 
                                 rdfs:subPropertyOf ddhub:HasFunction. 
ddhub:IsSetPointMaximumRecommendationFor a owl:ObjectProperty; 
                                         rdfs:comment ""@EN; 
                                         rdfs:domain ddhub:DrillingDataPoint; 
                                         rdfs:range ddhub:ControlSystem; 
                                         rdfs:subPropertyOf ddhub:HasFunction. 
ddhub:IsSetPointMinimumAdviceFor a owl:ObjectProperty; 
                                 rdfs:comment ""@EN; 
                                 rdfs:domain ddhub:DrillingDataPoint; 
                                 rdfs:range ddhub:ControlSystem; 
                                 rdfs:subPropertyOf ddhub:HasFunction. 
ddhub:IsSetPointMinimumRecommendationFor a owl:ObjectProperty; 
                                         rdfs:comment ""@EN; 
                                         rdfs:domain ddhub:DrillingDataPoint; 
                                         rdfs:range ddhub:ControlSystem; 
                                         rdfs:subPropertyOf ddhub:HasFunction. 
ddhub:IsSetPointRecommendationFor a owl:ObjectProperty; 
                                  rdfs:comment ""@EN; 
                                  rdfs:domain ddhub:DrillingDataPoint; 
                                  rdfs:range ddhub:ControlSystem; 
                                  rdfs:subPropertyOf ddhub:HasFunction. 
ddhub:IsSubPartOf a owl:ObjectProperty; 
                  rdfs:comment ""@EN; 
                  rdfs:domain ddhub:DrillingEquipment; 
                  rdfs:range ddhub:DrillingEquipment; 
                  rdfs:subPropertyOf ddhub:DWISVerb. 
ddhub:IsSynchronizationGroupInput a owl:ObjectProperty; 
                                  rdfs:comment ""@EN; 
                                  rdfs:domain ddhub:DrillingDataPoint; 
                                  rdfs:range ddhub:SynchronizationGroup; 
                                  rdfs:subPropertyOf ddhub:DWISVerb. 
ddhub:IsSynchronizationGroupOutput a owl:ObjectProperty; 
                                   rdfs:comment ""@EN; 
                                   rdfs:domain ddhub:DrillingDataPoint; 
                                   rdfs:range ddhub:SynchronizationGroup; 
                                   rdfs:subPropertyOf ddhub:DWISVerb. 
ddhub:IsToBeComparedWith a owl:ObjectProperty; 
                         rdfs:comment ""@EN; 
                         rdfs:domain ddhub:DrillingDataPoint; 
                         rdfs:range ddhub:DrillingDataPoint; 
                         rdfs:subPropertyOf ddhub:DWISVerb. 
ddhub:IsToBeDifferentFrom a owl:ObjectProperty; 
                          rdfs:comment ""@EN; 
                          rdfs:domain ddhub:DrillingDataPoint; 
                          rdfs:range ddhub:DrillingDataPoint; 
                          rdfs:subPropertyOf ddhub:IsToBeComparedWith. 
ddhub:IsToBeEqualTo a owl:ObjectProperty; 
                    rdfs:comment ""@EN; 
                    rdfs:domain ddhub:DrillingDataPoint; 
                    rdfs:range ddhub:DrillingDataPoint; 
                    rdfs:subPropertyOf ddhub:IsToBeComparedWith. 
ddhub:IsToBeGreaterOrEqualThan a owl:ObjectProperty; 
                               rdfs:comment ""@EN; 
                               rdfs:domain ddhub:DrillingDataPoint; 
                               rdfs:range ddhub:DrillingDataPoint; 
                               rdfs:subPropertyOf ddhub:IsToBeGreaterThan. 
ddhub:IsToBeGreaterThan a owl:ObjectProperty; 
                        rdfs:comment ""@EN; 
                        rdfs:domain ddhub:DrillingDataPoint; 
                        rdfs:range ddhub:DrillingDataPoint; 
                        rdfs:subPropertyOf ddhub:IsToBeComparedWith. 
ddhub:IsToBeSmallerOrEqualThan a owl:ObjectProperty; 
                               rdfs:comment ""@EN; 
                               rdfs:domain ddhub:DrillingDataPoint; 
                               rdfs:range ddhub:DrillingDataPoint; 
                               rdfs:subPropertyOf ddhub:IsToBeSmallerThan. 
ddhub:IsToBeSmallerThan a owl:ObjectProperty; 
                        rdfs:comment ""@EN; 
                        rdfs:domain ddhub:DrillingDataPoint; 
                        rdfs:range ddhub:DrillingDataPoint; 
                        rdfs:subPropertyOf ddhub:IsToBeComparedWith. 
ddhub:IsToBeStrictlyGreaterThan a owl:ObjectProperty; 
                                rdfs:comment ""@EN; 
                                rdfs:domain ddhub:DrillingDataPoint; 
                                rdfs:range ddhub:DrillingDataPoint; 
                                rdfs:subPropertyOf ddhub:IsToBeGreaterThan. 
ddhub:IsToBeStrictlySmallerThan a owl:ObjectProperty; 
                                rdfs:comment ""@EN; 
                                rdfs:domain ddhub:DrillingDataPoint; 
                                rdfs:range ddhub:DrillingDataPoint; 
                                rdfs:subPropertyOf ddhub:IsToBeSmallerThan. 
ddhub:IsTransformationInput a owl:ObjectProperty; 
                            rdfs:comment ""@EN; 
                            rdfs:domain ddhub:DrillingDataPoint; 
                            rdfs:range ddhub:Transformation; 
                            rdfs:subPropertyOf ddhub:HasFunction. 
ddhub:IsTransformationOutput a owl:ObjectProperty; 
                             rdfs:comment ""@EN; 
                             rdfs:domain ddhub:DrillingDataPoint; 
                             rdfs:range ddhub:DataFlowNode; 
                             rdfs:subPropertyOf ddhub:IsGeneratedBy. 
ddhub:IsTransmissionInput a owl:ObjectProperty; 
                          rdfs:comment ""@EN; 
                          rdfs:domain ddhub:DrillingDataPoint; 
                          rdfs:range ddhub:TransmissionLine; 
                          rdfs:subPropertyOf ddhub:HasFunction. 
ddhub:IsTransmissionOutput a owl:ObjectProperty; 
                           rdfs:comment ""@EN; 
                           rdfs:domain ddhub:DrillingDataPoint; 
                           rdfs:range ddhub:TransmissionLine; 
                           rdfs:subPropertyOf ddhub:IsGeneratedBy. 
ddhub:IsTransmittedBy a owl:ObjectProperty; 
                      rdfs:comment """Expresses that a signal is transmitted by some given telemetry system
"""@EN; 
                      rdfs:domain ddhub:DrillingDataPoint; 
                      rdfs:range ddhub:Telemetry; 
                      rdfs:subPropertyOf ddhub:DWISVerb. 
ddhub:IsTriggeredSignalFor a owl:ObjectProperty; 
                           rdfs:comment """This verb is used to indicate a `DrillingDataPoint` tells whether an `FDIRFunction` has been triggered
or not. This signal is expected to be a Boolean value. The signal is expected to be true from the moment the FDIR has triggered
to the moment it has recovered from the incident, if it has a recovery procedure, or to the moment the control is given
back to the end-user, in case of failure of the recovery procedure or at the end of the isolation procedure.
"""@EN; 
                           rdfs:domain ddhub:DrillingDataPoint; 
                           rdfs:range ddhub:FDIRFunction; 
                           rdfs:subPropertyOf ddhub:DWISVerb. 
ddhub:IsUnitForQuantity a owl:ObjectProperty; 
                        rdfs:comment """This `verb` is used to relate a `Unit` with a `Quantity`.
"""@EN; 
                        rdfs:domain ddhub:Unit; 
                        rdfs:range ddhub:Quantity; 
                        rdfs:subPropertyOf ddhub:DWISVerb. 
ddhub:IsUsedExtraMarginSignalFor a owl:ObjectProperty; 
                                 rdfs:comment """This verb is used to indicate a `DrillingDataPoint` used by an `FDIRFunction` tells whether the
extra margin signal is used or not by the FDIR function. This signal is expected to be a boolean value.
"""@EN; 
                                 rdfs:domain ddhub:DrillingDataPoint; 
                                 rdfs:range ddhub:FDIRFunction; 
                                 rdfs:subPropertyOf ddhub:DWISVerb. 
ddhub:IsUserControllableExtraMarginSignalFor a owl:ObjectProperty; 
                                             rdfs:comment """This verb is used to indicate that a `DrillingDataPoint` used by an `FDIRFunction`, extends the calculated
threshold value for the fault detection by a user-defined amount. The value of this signal is supposed to be interpreted
in absolute value. If it is negative, then it is its magnitude that is used. This allows the end-user to increase the margin for
detection of an incident. 
"""@EN; 
                                             rdfs:domain ddhub:DrillingDataPoint; 
                                             rdfs:range ddhub:FDIRFunction; 
                                             rdfs:subPropertyOf ddhub:DWISVerb. 
ddhub:IsValid a owl:DatatypeProperty, owl:FunctionalProperty; 
              rdfs:comment """
"""@EN; 
              rdfs:domain ddhub:DrillingDataPoint; 
              rdfs:range xsd:bool. 
ddhub:IsValidBy a owl:ObjectProperty; 
                rdfs:comment ""@EN; 
                rdfs:domain ddhub:DWISNoun; 
                rdfs:range ddhub:DWISNoun; 
                rdfs:subPropertyOf ddhub:DWISVerb. 
ddhub:IsVolumeAt a owl:ObjectProperty; 
                 rdfs:comment ""@EN; 
                 rdfs:domain ddhub:DrillingDataPoint; 
                 rdfs:range ddhub:Tank; 
                 rdfs:subPropertyOf ddhub:IsHydraulicallyLocatedAt. 
ddhub:IsVolumetricFlowRateAt a owl:ObjectProperty; 
                             rdfs:comment ""@EN; 
                             rdfs:domain ddhub:DrillingDataPoint; 
                             rdfs:range ddhub:HydraulicLogicalElement; 
                             rdfs:subPropertyOf ddhub:IsHydraulicallyLocatedAt. 
ddhub:J a owl:DatatypeProperty, owl:FunctionalProperty; 
        rdfs:comment """Luminous intensity exponent.
SI Unit: Candela (cd)
"""@EN; 
        rdfs:domain ddhub:Quantity; 
        rdfs:range xsd:double. 
ddhub:JackupLegs a owl:Class; 
                 rdfs:comment ""@EN; 
                 rdfs:subClassOf ddhub:MarineSystem. 
ddhub:JarAction a owl:Class; 
                rdfs:comment ""@EN; 
                rdfs:subClassOf ddhub:JarringAssembly. 
ddhub:JarringAssembly a owl:Class; 
                      rdfs:comment ""@EN; 
                      rdfs:subClassOf ddhub:DrillingEquipment. 
ddhub:JettingAssembly a owl:Class; 
                      rdfs:comment ""@EN; 
                      rdfs:subClassOf ddhub:DrillingEquipment. 
ddhub:Joule a owl:Class; 
            rdfs:comment """No conversion necessary as the unit choice is SI
"""@EN; 
            rdfs:subClassOf ddhub:Unit. 
ddhub:JoulePerCubicFoot a owl:Class; 
                        rdfs:comment """[v] = a * [SI]
where
[v] is the value in joule per cubic foot
[SI] is the value in SI
a = Foot * Foot * Foot / Unit, i.e., 0.02831684659199999
and
Foot = 12.0 * Inch
Unit = 1.0
Inch = 0.0254 reference: https://www.nist.gov/pml/owm/si-units-length
"""@EN; 
                        rdfs:subClassOf ddhub:Unit. 
ddhub:JoulePerCubicInch a owl:Class; 
                        rdfs:comment """[v] = a * [SI]
where
[v] is the value in joule per cubic inch
[SI] is the value in SI
a = Inch*Inch*Inch/Unit, i.e., 1.6387064E-05
and
Inch = 0.0254 reference: https://www.nist.gov/pml/owm/si-units-length
Unit = 1.0
"""@EN; 
                        rdfs:subClassOf ddhub:Unit. 
ddhub:JoulePerCubicMetre a owl:Class; 
                         rdfs:comment """No conversion necessary as the unit choice is SI
"""@EN; 
                         rdfs:subClassOf ddhub:Unit. 
ddhub:JoulePerGallonUk a owl:Class; 
                       rdfs:comment """[v] = a * [SI]
where
[v] is the value in joule per gallon (UK)
[SI] is the value in SI
a = GallonUK / Unit, i.e., 0.00454609
and
GallonUK = 4.54609e-3 reference: https://en.wikipedia.org/wiki/Gallon
Unit = 1.0
"""@EN; 
                       rdfs:subClassOf ddhub:Unit. 
ddhub:JoulePerGallonUs a owl:Class; 
                       rdfs:comment """[v] = a * [SI]
where
[v] is the value in joule per gallon (US)
[SI] is the value in SI
a = GallonUS / Unit, i.e., 0.0037854117839999997
and
GallonUS = 231.0 * Inch * Inch * Inch reference: https://en.wikipedia.org/wiki/Gallon
Unit = 1.0
Inch = 0.0254 reference: https://www.nist.gov/pml/owm/si-units-length
"""@EN; 
                       rdfs:subClassOf ddhub:Unit. 
ddhub:JoulePerGramDegreeCelsius a owl:Class; 
                                rdfs:comment """[v] = a * [SI]
where
[v] is the value in joule per gram degree celsius
[SI] is the value in SI
a = Milli/Unit, i.e., 0.001
and
Milli = 0.001
Unit = 1.0
"""@EN; 
                                rdfs:subClassOf ddhub:Unit. 
ddhub:JoulePerGramDegreeSquaredCelsius a owl:Class; 
                                       rdfs:comment """[v] = a * [SI]
where
[v] is the value in joule per gram degree squared celsius
[SI] is the value in SI
a = Milli, i.e., 0.001
and
Milli = 0.001
"""@EN; 
                                       rdfs:subClassOf ddhub:Unit. 
ddhub:JoulePerGramKelvin a owl:Class; 
                         rdfs:comment """[v] = a * [SI]
where
[v] is the value in joule per gram kelvin
[SI] is the value in SI
a = Milli/Unit, i.e., 0.001
and
Milli = 0.001
Unit = 1.0
"""@EN; 
                         rdfs:subClassOf ddhub:Unit. 
ddhub:JoulePerGramSquaredKelvin a owl:Class; 
                                rdfs:comment """[v] = a * [SI]
where
[v] is the value in joule per gram squared kelvin
[SI] is the value in SI
a = Milli, i.e., 0.001
and
Milli = 0.001
"""@EN; 
                                rdfs:subClassOf ddhub:Unit. 
ddhub:JoulePerKilogramKelvin a owl:Class; 
                             rdfs:comment """No conversion necessary as the unit choice is SI
"""@EN; 
                             rdfs:subClassOf ddhub:Unit. 
ddhub:JoulePerKilogramSquaredKelvin a owl:Class; 
                                    rdfs:comment """No conversion necessary as the unit choice is SI
"""@EN; 
                                    rdfs:subClassOf ddhub:Unit. 
ddhub:JoulePerLitre a owl:Class; 
                    rdfs:comment """[v] = a * [SI]
where
[v] is the value in joule per litre
[SI] is the value in SI
a = Litre/Unit, i.e., 0.001
and
Litre = 0.001
Unit = 1.0
"""@EN; 
                    rdfs:subClassOf ddhub:Unit. 
ddhub:JSonDataType a owl:Class; 
                   rdfs:comment """A string that contained the serialization in Json of an object.
"""@EN; 
                   rdfs:subClassOf ddhub:StringDataType. 
ddhub:JunkBasket a owl:Class; 
                 rdfs:comment ""@EN; 
                 rdfs:subClassOf ddhub:FishingTools. 
ddhub:Kelly a owl:Class; 
            rdfs:comment ""@EN; 
            rdfs:subClassOf ddhub:RotaryTable. 
ddhub:KellyBushing a owl:Class; 
                   rdfs:comment ""@EN; 
                   rdfs:subClassOf ddhub:Kelly. 
ddhub:KellyBushingVerticalLocation a owl:Class; 
                                   rdfs:comment ""@EN; 
                                   rdfs:subClassOf ddhub:VerticalReferenceLocation. 
ddhub:KellyHose a owl:Class; 
                rdfs:comment ""@EN; 
                rdfs:subClassOf ddhub:Kelly. 
ddhub:KellyJoint a owl:Class; 
                 rdfs:comment ""@EN; 
                 rdfs:subClassOf ddhub:Kelly. 
ddhub:KellySwivel a owl:Class; 
                  rdfs:comment ""@EN; 
                  rdfs:subClassOf ddhub:Kelly. 
ddhub:KellyValve a owl:Class; 
                 rdfs:comment ""@EN; 
                 rdfs:subClassOf ddhub:WellControlSystem. 
ddhub:Kelvin a owl:Class; 
             rdfs:comment """No conversion necessary as the unit choice is SI
"""@EN; 
             rdfs:subClassOf ddhub:Unit. 
ddhub:KelvinPerMetre a owl:Class; 
                     rdfs:comment """No conversion necessary as the unit choice is SI
"""@EN; 
                     rdfs:subClassOf ddhub:Unit. 
ddhub:KickOffVerticalLocation a owl:Class; 
                              rdfs:comment ""@EN; 
                              rdfs:subClassOf ddhub:VerticalReferenceLocation. 
ddhub:KillLine a owl:Class; 
               rdfs:comment ""@EN; 
               rdfs:subClassOf ddhub:WellControlSystem. 
ddhub:Kiloampere a owl:Class; 
                 rdfs:comment """[v] = a * [SI]
where
[v] is the value in kiloampere
[SI] is the value in SI
a = 1.0/Kilo, i.e., 0.001
and
Kilo = 1000.0
"""@EN; 
                 rdfs:subClassOf ddhub:Unit. 
ddhub:KiloBritishThermalUnit a owl:Class; 
                             rdfs:comment """[v] = a * [SI]
where
[v] is the value in kilo british thermal unit
[SI] is the value in SI
a = 1.0/(Kilo * BTU), i.e., 9.484516526770048E-07
and
Kilo = 1000.0
BTU = 1054.35 reference: https://en.wikipedia.org/wiki/British_thermal_unit
"""@EN; 
                             rdfs:subClassOf ddhub:Unit. 
ddhub:KiloBritishThermalUnitPerCubicFoot a owl:Class; 
                                         rdfs:comment """[v] = a * [SI]
where
[v] is the value in kilo british thermal unit per cubic foot
[SI] is the value in SI
a = Foot * Foot * Foot / (Kilo * BTU), i.e., 2.6857159948783602E-08
and
Foot = 12.0 * Inch
Kilo = 1000.0
BTU = 1054.35 reference: https://en.wikipedia.org/wiki/British_thermal_unit
Inch = 0.0254 reference: https://www.nist.gov/pml/owm/si-units-length
"""@EN; 
                                         rdfs:subClassOf ddhub:Unit. 
ddhub:KiloBritishThermalUnitPerCubicInch a owl:Class; 
                                         rdfs:comment """[v] = a * [SI]
where
[v] is the value in kilo british thermal unit per cubic inch
[SI] is the value in SI
a = Inch*Inch*Inch/(Kilo * BTU), i.e., 1.5542337933323848E-11
and
Inch = 0.0254 reference: https://www.nist.gov/pml/owm/si-units-length
Kilo = 1000.0
BTU = 1054.35 reference: https://en.wikipedia.org/wiki/British_thermal_unit
"""@EN; 
                                         rdfs:subClassOf ddhub:Unit. 
ddhub:KiloBritishThermalUnitPerCubicMetre a owl:Class; 
                                          rdfs:comment """[v] = a * [SI]
where
[v] is the value in kilo british thermal unit per cubic metre
[SI] is the value in SI
a = 1.0/(Kilo * BTU), i.e., 9.484516526770048E-07
and
Kilo = 1000.0
BTU = 1054.35 reference: https://en.wikipedia.org/wiki/British_thermal_unit
"""@EN; 
                                          rdfs:subClassOf ddhub:Unit. 
ddhub:KiloBritishThermalUnitPerGallonUk a owl:Class; 
                                        rdfs:comment """[v] = a * [SI]
where
[v] is the value in kilo british thermal unit per gallon (UK)
[SI] is the value in SI
a = GallonUK / (Kilo * BTU), i.e., 4.311746573718405E-09
and
GallonUK = 4.54609e-3 reference: https://en.wikipedia.org/wiki/Gallon
Kilo = 1000.0
BTU = 1054.35 reference: https://en.wikipedia.org/wiki/British_thermal_unit
"""@EN; 
                                        rdfs:subClassOf ddhub:Unit. 
ddhub:KiloBritishThermalUnitPerGallonUs a owl:Class; 
                                        rdfs:comment """[v] = a * [SI]
where
[v] is the value in kilo british thermal unit per gallon (US)
[SI] is the value in SI
a = GallonUS / (Kilo * BTU), i.e., 3.5902800625978087E-09
and
GallonUS = 231.0 * Inch * Inch * Inch reference: https://en.wikipedia.org/wiki/Gallon
Kilo = 1000.0
BTU = 1054.35 reference: https://en.wikipedia.org/wiki/British_thermal_unit
Inch = 0.0254 reference: https://www.nist.gov/pml/owm/si-units-length
"""@EN; 
                                        rdfs:subClassOf ddhub:Unit. 
ddhub:KiloBritishThermalUnitPerLitre a owl:Class; 
                                     rdfs:comment """[v] = a * [SI]
where
[v] is the value in kilo british thermal unit per litre
[SI] is the value in SI
a = Litre/(Kilo * BTU), i.e., 9.48451652677005E-10
and
Litre = 0.001
Kilo = 1000.0
BTU = 1054.35 reference: https://en.wikipedia.org/wiki/British_thermal_unit
"""@EN; 
                                     rdfs:subClassOf ddhub:Unit. 
ddhub:Kilocalorie a owl:Class; 
                  rdfs:comment """[v] = a * [SI]
where
[v] is the value in kilocalorie
[SI] is the value in SI
a = 1.0/(Kilo * Calorie), i.e., 0.0002390057361376673
and
Kilo = 1000.0
Calorie = 4.184 reference: https://en.wikipedia.org/wiki/Calorie
"""@EN; 
                  rdfs:subClassOf ddhub:Unit. 
ddhub:KilocaloriePerCubicFoot a owl:Class; 
                              rdfs:comment """[v] = a * [SI]
where
[v] is the value in kilocalorie per cubic foot
[SI] is the value in SI
a = Foot * Foot * Foot / (Kilo * Calorie), i.e., 6.767888764818354E-06
and
Foot = 12.0 * Inch
Kilo = 1000.0
Calorie = 4.184 reference: https://en.wikipedia.org/wiki/Calorie
Inch = 0.0254 reference: https://www.nist.gov/pml/owm/si-units-length
"""@EN; 
                              rdfs:subClassOf ddhub:Unit. 
ddhub:KilocaloriePerCubicInch a owl:Class; 
                              rdfs:comment """[v] = a * [SI]
where
[v] is the value in kilocalorie per cubic inch
[SI] is the value in SI
a = Inch*Inch*Inch/(Kilo * Calorie), i.e., 3.916602294455067E-09
and
Inch = 0.0254 reference: https://www.nist.gov/pml/owm/si-units-length
Kilo = 1000.0
Calorie = 4.184 reference: https://en.wikipedia.org/wiki/Calorie
"""@EN; 
                              rdfs:subClassOf ddhub:Unit. 
ddhub:KilocaloriePerCubicMetre a owl:Class; 
                               rdfs:comment """[v] = a * [SI]
where
[v] is the value in kilocalorie per cubic metre
[SI] is the value in SI
a = 1.0 / (Kilo * Calorie), i.e., 0.0002390057361376673
and
Kilo = 1000.0
Calorie = 4.184 reference: https://en.wikipedia.org/wiki/Calorie
"""@EN; 
                               rdfs:subClassOf ddhub:Unit. 
ddhub:KilocaloriePerGallonUk a owl:Class; 
                             rdfs:comment """[v] = a * [SI]
where
[v] is the value in kilocalorie per gallon (UK)
[SI] is the value in SI
a = GallonUK / (Kilo * Calorie), i.e., 1.086541586998088E-06
and
GallonUK = 4.54609e-3 reference: https://en.wikipedia.org/wiki/Gallon
Kilo = 1000.0
Calorie = 4.184 reference: https://en.wikipedia.org/wiki/Calorie
"""@EN; 
                             rdfs:subClassOf ddhub:Unit. 
ddhub:KilocaloriePerGallonUs a owl:Class; 
                             rdfs:comment """[v] = a * [SI]
where
[v] is the value in kilocalorie per gallon (US)
[SI] is the value in SI
a = GallonUS / (Kilo * Calorie), i.e., 9.047351300191203E-07
and
GallonUS = 231.0 * Inch * Inch * Inch reference: https://en.wikipedia.org/wiki/Gallon
Kilo = 1000.0
Calorie = 4.184 reference: https://en.wikipedia.org/wiki/Calorie
Inch = 0.0254 reference: https://www.nist.gov/pml/owm/si-units-length
"""@EN; 
                             rdfs:subClassOf ddhub:Unit. 
ddhub:KilocaloriePerGramDegreeCelsius a owl:Class; 
                                      rdfs:comment """[v] = a * [SI]
where
[v] is the value in kilocalorie per gram degree celsius
[SI] is the value in SI
a = Milli/(Kilo*Calorie), i.e., 2.390057361376673E-07
and
Milli = 0.001
Kilo = 1000.0
Calorie = 4.184 reference: https://en.wikipedia.org/wiki/Calorie
"""@EN; 
                                      rdfs:subClassOf ddhub:Unit. 
ddhub:KilocaloriePerLitre a owl:Class; 
                          rdfs:comment """[v] = a * [SI]
where
[v] is the value in kilocalorie per litre
[SI] is the value in SI
a = Litre/(Kilo * Calorie), i.e., 2.390057361376673E-07
and
Litre = 0.001
Kilo = 1000.0
Calorie = 4.184 reference: https://en.wikipedia.org/wiki/Calorie
"""@EN; 
                          rdfs:subClassOf ddhub:Unit. 
ddhub:Kilocandela a owl:Class; 
                  rdfs:comment """[v] = a * [SI]
where
[v] is the value in kilocandela
[SI] is the value in SI
a = 1.0/Kilo, i.e., 0.001
and
Kilo = 1000.0
"""@EN; 
                  rdfs:subClassOf ddhub:Unit. 
ddhub:Kilodecanewton a owl:Class; 
                     rdfs:comment """[v] = a * [SI]
where
[v] is the value in kilodecanewton
[SI] is the value in SI
a = 1.0/(Kilo*Deca), i.e., 0.0001
and
Kilo = 1000.0
Deca = 10.0
"""@EN; 
                     rdfs:subClassOf ddhub:Unit. 
ddhub:KilodecanewtonPerHour a owl:Class; 
                            rdfs:comment """[v] = a * [SI]
where
[v] is the value in kilodecanewton per hour
[SI] is the value in SI
a = Hour/(Kilo*Deca), i.e., 0.36
and
Hour = 60.0 * Minute
Kilo = 1000.0
Deca = 10.0
Minute = 60.0
"""@EN; 
                            rdfs:subClassOf ddhub:Unit. 
ddhub:KilodecanewtonPerMinute a owl:Class; 
                              rdfs:comment """[v] = a * [SI]
where
[v] is the value in kilodecanewton per minute
[SI] is the value in SI
a = Minute/(Kilo*Deca), i.e., 0.006
and
Minute = 60.0
Kilo = 1000.0
Deca = 10.0
"""@EN; 
                              rdfs:subClassOf ddhub:Unit. 
ddhub:KilodecanewtonPerSecond a owl:Class; 
                              rdfs:comment """[v] = a * [SI]
where
[v] is the value in kilodecanewton per second
[SI] is the value in SI
a = 1.0/(Kilo*Deca), i.e., 0.0001
and
Kilo = 1000.0
Deca = 10.0
"""@EN; 
                              rdfs:subClassOf ddhub:Unit. 
ddhub:KilofootPound a owl:Class; 
                    rdfs:comment """[v] = a * [SI]
where
[v] is the value in kilofoot pound
[SI] is the value in SI
a = 1.0/(Kilo*Foot*PoundForce), i.e., 0.0007375621492772656
and
Kilo = 1000.0
Foot = 12.0 * Inch
PoundForce = Pound * G reference: https://en.wikipedia.org/wiki/Pound_(force)
Inch = 0.0254 reference: https://www.nist.gov/pml/owm/si-units-length
Pound = 0.45359237 reference: https://en.wikipedia.org/wiki/Pound_(mass)
G = 9.80665 reference: https://en.wikipedia.org/wiki/Gravity_of_Earth
"""@EN; 
                    rdfs:subClassOf ddhub:Unit. 
ddhub:KilofootPoundPerCentimetre a owl:Class; 
                                 rdfs:comment """[v] = a * [SI]
where
[v] is the value in kilofoot pound per centimetre
[SI] is the value in SI
a = Centi/(Kilo*Foot*PoundForce), i.e., 7.3756214927726565E-06
and
Centi = 0.01
Kilo = 1000.0
Foot = 12.0 * Inch
PoundForce = Pound * G reference: https://en.wikipedia.org/wiki/Pound_(force)
Inch = 0.0254 reference: https://www.nist.gov/pml/owm/si-units-length
Pound = 0.45359237 reference: https://en.wikipedia.org/wiki/Pound_(mass)
G = 9.80665 reference: https://en.wikipedia.org/wiki/Gravity_of_Earth
"""@EN; 
                                 rdfs:subClassOf ddhub:Unit. 
ddhub:KilofootPoundPerDecimetre a owl:Class; 
                                rdfs:comment """[v] = a * [SI]
where
[v] is the value in kilofoot pound per decimetre
[SI] is the value in SI
a = Deci/(Kilo*Foot*PoundForce), i.e., 7.375621492772657E-05
and
Deci = 0.1
Kilo = 1000.0
Foot = 12.0 * Inch
PoundForce = Pound * G reference: https://en.wikipedia.org/wiki/Pound_(force)
Inch = 0.0254 reference: https://www.nist.gov/pml/owm/si-units-length
Pound = 0.45359237 reference: https://en.wikipedia.org/wiki/Pound_(mass)
G = 9.80665 reference: https://en.wikipedia.org/wiki/Gravity_of_Earth
"""@EN; 
                                rdfs:subClassOf ddhub:Unit. 
ddhub:KilofootPoundPerFoot a owl:Class; 
                           rdfs:comment """[v] = a * [SI]
where
[v] is the value in kilofoot pound per foot
[SI] is the value in SI
a = Foot/(Kilo*Foot*PoundForce), i.e., 0.00022480894309971053
and
Foot = 12.0 * Inch
Kilo = 1000.0
PoundForce = Pound * G reference: https://en.wikipedia.org/wiki/Pound_(force)
Inch = 0.0254 reference: https://www.nist.gov/pml/owm/si-units-length
Pound = 0.45359237 reference: https://en.wikipedia.org/wiki/Pound_(mass)
G = 9.80665 reference: https://en.wikipedia.org/wiki/Gravity_of_Earth
"""@EN; 
                           rdfs:subClassOf ddhub:Unit. 
ddhub:KilofootPoundPerHour a owl:Class; 
                           rdfs:comment """[v] = a * [SI]
where
[v] is the value in kilofoot pound per hour
[SI] is the value in SI
a = Hour/(Kilo*Foot*PoundForce), i.e., 2.655223737398156
and
Hour = 60.0 * Minute
Kilo = 1000.0
Foot = 12.0 * Inch
PoundForce = Pound * G reference: https://en.wikipedia.org/wiki/Pound_(force)
Minute = 60.0
Inch = 0.0254 reference: https://www.nist.gov/pml/owm/si-units-length
Pound = 0.45359237 reference: https://en.wikipedia.org/wiki/Pound_(mass)
G = 9.80665 reference: https://en.wikipedia.org/wiki/Gravity_of_Earth
"""@EN; 
                           rdfs:subClassOf ddhub:Unit. 
ddhub:KilofootPoundPerInch a owl:Class; 
                           rdfs:comment """[v] = a * [SI]
where
[v] is the value in kilofoot pound per inch
[SI] is the value in SI
a = Inch/(Kilo*Foot*PoundForce), i.e., 1.8734078591642546E-05
and
Inch = 0.0254 reference: https://www.nist.gov/pml/owm/si-units-length
Kilo = 1000.0
Foot = 12.0 * Inch
PoundForce = Pound * G reference: https://en.wikipedia.org/wiki/Pound_(force)
Pound = 0.45359237 reference: https://en.wikipedia.org/wiki/Pound_(mass)
G = 9.80665 reference: https://en.wikipedia.org/wiki/Gravity_of_Earth
"""@EN; 
                           rdfs:subClassOf ddhub:Unit. 
ddhub:KilofootPoundPerMetre a owl:Class; 
                            rdfs:comment """[v] = a * [SI]
where
[v] is the value in kilofoot pound per metre
[SI] is the value in SI
a = Unit/(Kilo*PoundForce*Foot), i.e., 0.0007375621492772654
and
Unit = 1.0
Kilo = 1000.0
PoundForce = Pound * G reference: https://en.wikipedia.org/wiki/Pound_(force)
Foot = 12.0 * Inch
Pound = 0.45359237 reference: https://en.wikipedia.org/wiki/Pound_(mass)
G = 9.80665 reference: https://en.wikipedia.org/wiki/Gravity_of_Earth
Inch = 0.0254 reference: https://www.nist.gov/pml/owm/si-units-length
"""@EN; 
                            rdfs:subClassOf ddhub:Unit. 
ddhub:KilofootPoundPerMillimetre a owl:Class; 
                                 rdfs:comment """[v] = a * [SI]
where
[v] is the value in kilofoot pound per millimetre
[SI] is the value in SI
a = Milli/(Kilo*Foot*PoundForce), i.e., 7.375621492772656E-07
and
Milli = 0.001
Kilo = 1000.0
Foot = 12.0 * Inch
PoundForce = Pound * G reference: https://en.wikipedia.org/wiki/Pound_(force)
Inch = 0.0254 reference: https://www.nist.gov/pml/owm/si-units-length
Pound = 0.45359237 reference: https://en.wikipedia.org/wiki/Pound_(mass)
G = 9.80665 reference: https://en.wikipedia.org/wiki/Gravity_of_Earth
"""@EN; 
                                 rdfs:subClassOf ddhub:Unit. 
ddhub:KilofootPoundPerMinute a owl:Class; 
                             rdfs:comment """[v] = a * [SI]
where
[v] is the value in kilofoot pound per minute
[SI] is the value in SI
a = Minute/(Kilo*Foot*PoundForce), i.e., 0.044253728956635936
and
Minute = 60.0
Kilo = 1000.0
Foot = 12.0 * Inch
PoundForce = Pound * G reference: https://en.wikipedia.org/wiki/Pound_(force)
Inch = 0.0254 reference: https://www.nist.gov/pml/owm/si-units-length
Pound = 0.45359237 reference: https://en.wikipedia.org/wiki/Pound_(mass)
G = 9.80665 reference: https://en.wikipedia.org/wiki/Gravity_of_Earth
"""@EN; 
                             rdfs:subClassOf ddhub:Unit. 
ddhub:KilofootPoundPerSecond a owl:Class; 
                             rdfs:comment """[v] = a * [SI]
where
[v] is the value in kilofoot pound per second
[SI] is the value in SI
a = 1.0/(Kilo*Foot*PoundForce), i.e., 0.0007375621492772656
and
Kilo = 1000.0
Foot = 12.0 * Inch
PoundForce = Pound * G reference: https://en.wikipedia.org/wiki/Pound_(force)
Inch = 0.0254 reference: https://www.nist.gov/pml/owm/si-units-length
Pound = 0.45359237 reference: https://en.wikipedia.org/wiki/Pound_(mass)
G = 9.80665 reference: https://en.wikipedia.org/wiki/Gravity_of_Earth
"""@EN; 
                             rdfs:subClassOf ddhub:Unit. 
ddhub:Kilogram a owl:Class; 
               rdfs:comment """No conversion necessary as the unit choice is SI
"""@EN; 
               rdfs:subClassOf ddhub:Unit. 
ddhub:KilogramForce a owl:Class; 
                    rdfs:comment """[v] = a * [SI]
where
[v] is the value in kilogram force
[SI] is the value in SI
a = 1.0/KilogramForce, i.e., 0.10197162129779283
and
KilogramForce = 1.0 * G reference: https://en.wikipedia.org/wiki/Kilogram-force
G = 9.80665 reference: https://en.wikipedia.org/wiki/Gravity_of_Earth
"""@EN; 
                    rdfs:subClassOf ddhub:Unit. 
ddhub:KilogramForceMetre a owl:Class; 
                         rdfs:comment """[v] = a * [SI]
where
[v] is the value in kilogram force metre
[SI] is the value in SI
a = 1.0/ KilogramForce, i.e., 0.10197162129779283
and
KilogramForce = 1.0 * G reference: https://en.wikipedia.org/wiki/Kilogram-force
G = 9.80665 reference: https://en.wikipedia.org/wiki/Gravity_of_Earth
"""@EN; 
                         rdfs:subClassOf ddhub:Unit. 
ddhub:KilogramForceMetrePerCentimetre a owl:Class; 
                                      rdfs:comment """[v] = a * [SI]
where
[v] is the value in kilogram force metre per centimetre
[SI] is the value in SI
a = Centi/(KilogramForce), i.e., 0.0010197162129779284
and
Centi = 0.01
KilogramForce = 1.0 * G reference: https://en.wikipedia.org/wiki/Kilogram-force
G = 9.80665 reference: https://en.wikipedia.org/wiki/Gravity_of_Earth
"""@EN; 
                                      rdfs:subClassOf ddhub:Unit. 
ddhub:KilogramForceMetrePerDecimetre a owl:Class; 
                                     rdfs:comment """[v] = a * [SI]
where
[v] is the value in kilogram force metre per decimetre
[SI] is the value in SI
a = Deci/(KilogramForce), i.e., 0.010197162129779284
and
Deci = 0.1
KilogramForce = 1.0 * G reference: https://en.wikipedia.org/wiki/Kilogram-force
G = 9.80665 reference: https://en.wikipedia.org/wiki/Gravity_of_Earth
"""@EN; 
                                     rdfs:subClassOf ddhub:Unit. 
ddhub:KilogramForceMetrePerFoot a owl:Class; 
                                rdfs:comment """[v] = a * [SI]
where
[v] is the value in kilogram force metre per foot
[SI] is the value in SI
a = Foot/KilogramForce, i.e., 0.03108095017156725
and
Foot = 12.0 * Inch
KilogramForce = 1.0 * G reference: https://en.wikipedia.org/wiki/Kilogram-force
Inch = 0.0254 reference: https://www.nist.gov/pml/owm/si-units-length
G = 9.80665 reference: https://en.wikipedia.org/wiki/Gravity_of_Earth
"""@EN; 
                                rdfs:subClassOf ddhub:Unit. 
ddhub:KilogramForceMetrePerHour a owl:Class; 
                                rdfs:comment """[v] = a * [SI]
where
[v] is the value in kilogram force metre per hour
[SI] is the value in SI
a = Hour/ KilogramForce, i.e., 367.0978366720542
and
Hour = 60.0 * Minute
KilogramForce = 1.0 * G reference: https://en.wikipedia.org/wiki/Kilogram-force
Minute = 60.0
G = 9.80665 reference: https://en.wikipedia.org/wiki/Gravity_of_Earth
"""@EN; 
                                rdfs:subClassOf ddhub:Unit. 
ddhub:KilogramForceMetrePerInch a owl:Class; 
                                rdfs:comment """[v] = a * [SI]
where
[v] is the value in kilogram force metre per inch
[SI] is the value in SI
a = Inch/KilogramForce, i.e., 0.0025900791809639378
and
Inch = 0.0254 reference: https://www.nist.gov/pml/owm/si-units-length
KilogramForce = 1.0 * G reference: https://en.wikipedia.org/wiki/Kilogram-force
G = 9.80665 reference: https://en.wikipedia.org/wiki/Gravity_of_Earth
"""@EN; 
                                rdfs:subClassOf ddhub:Unit. 
ddhub:KilogramForceMetrePerMetre a owl:Class; 
                                 rdfs:comment """[v] = a * [SI]
where
[v] is the value in kilogram force metre per metre
[SI] is the value in SI
a = Unit/(KilogramForce), i.e., 0.10197162129779283
and
Unit = 1.0
KilogramForce = 1.0 * G reference: https://en.wikipedia.org/wiki/Kilogram-force
G = 9.80665 reference: https://en.wikipedia.org/wiki/Gravity_of_Earth
"""@EN; 
                                 rdfs:subClassOf ddhub:Unit. 
ddhub:KilogramForceMetrePerMillimetre a owl:Class; 
                                      rdfs:comment """[v] = a * [SI]
where
[v] is the value in kilogram force metre per millimetre
[SI] is the value in SI
a = Milli/(KilogramForce), i.e., 0.00010197162129779284
and
Milli = 0.001
KilogramForce = 1.0 * G reference: https://en.wikipedia.org/wiki/Kilogram-force
G = 9.80665 reference: https://en.wikipedia.org/wiki/Gravity_of_Earth
"""@EN; 
                                      rdfs:subClassOf ddhub:Unit. 
ddhub:KilogramForceMetrePerMinute a owl:Class; 
                                  rdfs:comment """[v] = a * [SI]
where
[v] is the value in kilogram force metre per minute
[SI] is the value in SI
a = Minute/ KilogramForce, i.e., 6.11829727786757
and
Minute = 60.0
KilogramForce = 1.0 * G reference: https://en.wikipedia.org/wiki/Kilogram-force
G = 9.80665 reference: https://en.wikipedia.org/wiki/Gravity_of_Earth
"""@EN; 
                                  rdfs:subClassOf ddhub:Unit. 
ddhub:KilogramForceMetrePerSecond a owl:Class; 
                                  rdfs:comment """[v] = a * [SI]
where
[v] is the value in kilogram force metre per second
[SI] is the value in SI
a = 1.0/ KilogramForce, i.e., 0.10197162129779283
and
KilogramForce = 1.0 * G reference: https://en.wikipedia.org/wiki/Kilogram-force
G = 9.80665 reference: https://en.wikipedia.org/wiki/Gravity_of_Earth
"""@EN; 
                                  rdfs:subClassOf ddhub:Unit. 
ddhub:KilogramForcePerHour a owl:Class; 
                           rdfs:comment """[v] = a * [SI]
where
[v] is the value in kilogram force per hour
[SI] is the value in SI
a = Hour/KilogramForce, i.e., 367.0978366720542
and
Hour = 60.0 * Minute
KilogramForce = 1.0 * G reference: https://en.wikipedia.org/wiki/Kilogram-force
Minute = 60.0
G = 9.80665 reference: https://en.wikipedia.org/wiki/Gravity_of_Earth
"""@EN; 
                           rdfs:subClassOf ddhub:Unit. 
ddhub:KilogramForcePerMinute a owl:Class; 
                             rdfs:comment """[v] = a * [SI]
where
[v] is the value in kilogram force per minute
[SI] is the value in SI
a = Minute/KilogramForce, i.e., 6.11829727786757
and
Minute = 60.0
KilogramForce = 1.0 * G reference: https://en.wikipedia.org/wiki/Kilogram-force
G = 9.80665 reference: https://en.wikipedia.org/wiki/Gravity_of_Earth
"""@EN; 
                             rdfs:subClassOf ddhub:Unit. 
ddhub:KilogramForcePerSecond a owl:Class; 
                             rdfs:comment """[v] = a * [SI]
where
[v] is the value in kilogram force per second
[SI] is the value in SI
a = 1.0/KilogramForce, i.e., 0.10197162129779283
and
KilogramForce = 1.0 * G reference: https://en.wikipedia.org/wiki/Kilogram-force
G = 9.80665 reference: https://en.wikipedia.org/wiki/Gravity_of_Earth
"""@EN; 
                             rdfs:subClassOf ddhub:Unit. 
ddhub:KilogramPerCubicMetre a owl:Class; 
                            rdfs:comment """No conversion necessary as the unit choice is SI
"""@EN; 
                            rdfs:subClassOf ddhub:Unit. 
ddhub:KilogramPerCubicMetrePer100Metre a owl:Class; 
                                       rdfs:comment """[v] = a * [SI]
where
[v] is the value in kilogram per cubic metre per 100 metre
[SI] is the value in SI
a = Hecto/Unit, i.e., 100
and
Hecto = 100.0
Unit = 1.0
"""@EN; 
                                       rdfs:subClassOf ddhub:Unit. 
ddhub:KilogramPerCubicMetrePer10Metre a owl:Class; 
                                      rdfs:comment """[v] = a * [SI]
where
[v] is the value in kilogram per cubic metre per 10 metre
[SI] is the value in SI
a = Deca/Unit, i.e., 10
and
Deca = 10.0
Unit = 1.0
"""@EN; 
                                      rdfs:subClassOf ddhub:Unit. 
ddhub:KilogramPerCubicMetrePer30Metre a owl:Class; 
                                      rdfs:comment """[v] = a * [SI]
where
[v] is the value in kilogram per cubic metre per 30 metre
[SI] is the value in SI
a = 3.0 *Deca/Unit, i.e., 30
and
Deca = 10.0
Unit = 1.0
"""@EN; 
                                      rdfs:subClassOf ddhub:Unit. 
ddhub:KilogramPerCubicMetrePerKelvin a owl:Class; 
                                     rdfs:comment """No conversion necessary as the unit choice is SI
"""@EN; 
                                     rdfs:subClassOf ddhub:Unit. 
ddhub:KilogramPerCubicMetrePerMetre a owl:Class; 
                                    rdfs:comment """No conversion necessary as the unit choice is SI
"""@EN; 
                                    rdfs:subClassOf ddhub:Unit. 
ddhub:KilogramPerCubicMetrePerSecond a owl:Class; 
                                     rdfs:comment """No conversion necessary as the unit choice is SI
"""@EN; 
                                     rdfs:subClassOf ddhub:Unit. 
ddhub:KilogramPerHour a owl:Class; 
                      rdfs:comment """[v] = a * [SI]
where
[v] is the value in kilogram per hour
[SI] is the value in SI
a = Hour/Unit, i.e., 3600
and
Hour = 60.0 * Minute
Unit = 1.0
Minute = 60.0
"""@EN; 
                      rdfs:subClassOf ddhub:Unit. 
ddhub:KilogramPerMetre a owl:Class; 
                       rdfs:comment """No conversion necessary as the unit choice is SI
"""@EN; 
                       rdfs:subClassOf ddhub:Unit. 
ddhub:KilogramPerMinute a owl:Class; 
                        rdfs:comment """[v] = a * [SI]
where
[v] is the value in kilogram per minute
[SI] is the value in SI
a = Minute/Unit, i.e., 60
and
Minute = 60.0
Unit = 1.0
"""@EN; 
                        rdfs:subClassOf ddhub:Unit. 
ddhub:KilogramPerSecond a owl:Class; 
                        rdfs:comment """No conversion necessary as the unit choice is SI
"""@EN; 
                        rdfs:subClassOf ddhub:Unit. 
ddhub:KilogramPerYear a owl:Class; 
                      rdfs:comment """[v] = a * [SI]
where
[v] is the value in kilogram per year
[SI] is the value in SI
a = YearJulian/Unit, i.e., 31557600
and
YearJulian = 365.25 * Day
Unit = 1.0
Day = 24.0 * Hour
Hour = 60.0 * Minute
Minute = 60.0
"""@EN; 
                      rdfs:subClassOf ddhub:Unit. 
ddhub:Kilohertz a owl:Class; 
                rdfs:comment """[v] = a * [SI]
where
[v] is the value in kilohertz
[SI] is the value in SI
a = 1.0/Kilo, i.e., 0.001
and
Kilo = 1000.0
"""@EN; 
                rdfs:subClassOf ddhub:Unit. 
ddhub:KiloHertzPerDay a owl:Class; 
                      rdfs:comment """[v] = a * [SI]
where
[v] is the value in kilo hertz per day
[SI] is the value in SI
a = Day/Kilo, i.e., 86.4
and
Day = 24.0 * Hour
Kilo = 1000.0
Hour = 60.0 * Minute
Minute = 60.0
"""@EN; 
                      rdfs:subClassOf ddhub:Unit. 
ddhub:KiloHertzPerHour a owl:Class; 
                       rdfs:comment """[v] = a * [SI]
where
[v] is the value in kilo hertz per hour
[SI] is the value in SI
a = Hour/Kilo, i.e., 3.6
and
Hour = 60.0 * Minute
Kilo = 1000.0
Minute = 60.0
"""@EN; 
                       rdfs:subClassOf ddhub:Unit. 
ddhub:KiloHertzPerMinute a owl:Class; 
                         rdfs:comment """[v] = a * [SI]
where
[v] is the value in kilo hertz per minute
[SI] is the value in SI
a = Minute/Kilo, i.e., 0.06
and
Minute = 60.0
Kilo = 1000.0
"""@EN; 
                         rdfs:subClassOf ddhub:Unit. 
ddhub:KiloHertzPerSecond a owl:Class; 
                         rdfs:comment """[v] = a * [SI]
where
[v] is the value in kilo hertz per second
[SI] is the value in SI
a = 1.0/Kilo, i.e., 0.001
and
Kilo = 1000.0
"""@EN; 
                         rdfs:subClassOf ddhub:Unit. 
ddhub:KiloHertzPerYear a owl:Class; 
                       rdfs:comment """[v] = a * [SI]
where
[v] is the value in kilo hertz per year
[SI] is the value in SI
a = YearJulian/Kilo, i.e., 31557.6
and
YearJulian = 365.25 * Day
Kilo = 1000.0
Day = 24.0 * Hour
Hour = 60.0 * Minute
Minute = 60.0
"""@EN; 
                       rdfs:subClassOf ddhub:Unit. 
ddhub:Kilojoule a owl:Class; 
                rdfs:comment """[v] = a * [SI]
where
[v] is the value in kilojoule
[SI] is the value in SI
a = 1.0/Kilo, i.e., 0.001
and
Kilo = 1000.0
"""@EN; 
                rdfs:subClassOf ddhub:Unit. 
ddhub:KilojoulePerCubicFoot a owl:Class; 
                            rdfs:comment """[v] = a * [SI]
where
[v] is the value in kilojoule per cubic foot
[SI] is the value in SI
a = Foot * Foot * Foot / Kilo, i.e., 2.831684659199999E-05
and
Foot = 12.0 * Inch
Kilo = 1000.0
Inch = 0.0254 reference: https://www.nist.gov/pml/owm/si-units-length
"""@EN; 
                            rdfs:subClassOf ddhub:Unit. 
ddhub:KilojoulePerCubicInch a owl:Class; 
                            rdfs:comment """[v] = a * [SI]
where
[v] is the value in kilojoule per cubic inch
[SI] is the value in SI
a = Inch*Inch*Inch/Kilo, i.e., 1.6387064E-08
and
Inch = 0.0254 reference: https://www.nist.gov/pml/owm/si-units-length
Kilo = 1000.0
"""@EN; 
                            rdfs:subClassOf ddhub:Unit. 
ddhub:KilojoulePerCubicMetre a owl:Class; 
                             rdfs:comment """[v] = a * [SI]
where
[v] is the value in kilojoule per cubic metre
[SI] is the value in SI
a = 1.0/Kilo, i.e., 0.001
and
Kilo = 1000.0
"""@EN; 
                             rdfs:subClassOf ddhub:Unit. 
ddhub:KilojoulePerGallonUk a owl:Class; 
                           rdfs:comment """[v] = a * [SI]
where
[v] is the value in kilojoule per gallon (UK)
[SI] is the value in SI
a = GallonUK / Kilo, i.e., 4.54609E-06
and
GallonUK = 4.54609e-3 reference: https://en.wikipedia.org/wiki/Gallon
Kilo = 1000.0
"""@EN; 
                           rdfs:subClassOf ddhub:Unit. 
ddhub:KilojoulePerGallonUs a owl:Class; 
                           rdfs:comment """[v] = a * [SI]
where
[v] is the value in kilojoule per gallon (US)
[SI] is the value in SI
a = GallonUS / Kilo, i.e., 3.7854117839999998E-06
and
GallonUS = 231.0 * Inch * Inch * Inch reference: https://en.wikipedia.org/wiki/Gallon
Kilo = 1000.0
Inch = 0.0254 reference: https://www.nist.gov/pml/owm/si-units-length
"""@EN; 
                           rdfs:subClassOf ddhub:Unit. 
ddhub:KilojoulePerLitre a owl:Class; 
                        rdfs:comment """[v] = a * [SI]
where
[v] is the value in kilojoule per litre
[SI] is the value in SI
a = Litre/Kilo, i.e., 1E-06
and
Litre = 0.001
Kilo = 1000.0
"""@EN; 
                        rdfs:subClassOf ddhub:Unit. 
ddhub:Kiloline a owl:Class; 
               rdfs:comment """[v] = a * [SI]
where
[v] is the value in kiloline
[SI] is the value in SI
a = 1.0/(Kilo*Line), i.e., 99999.99999999999
and
Kilo = 1000.0
Line = 1e-8 reference: https://en.wikipedia.org/wiki/Maxwell_(unit)
"""@EN; 
               rdfs:subClassOf ddhub:Unit. 
ddhub:Kilometre a owl:Class; 
                rdfs:comment """[v] = a * [SI]
where
[v] is the value in kilometre
[SI] is the value in SI
a = 1.0/Kilo, i.e., 0.001
and
Kilo = 1000.0
"""@EN; 
                rdfs:subClassOf ddhub:Unit. 
ddhub:KilometrePerDay a owl:Class; 
                      rdfs:comment """[v] = a * [SI]
where
[v] is the value in kilometre per day
[SI] is the value in SI
a = Day/Kilo, i.e., 86.4
and
Day = 24.0 * Hour
Kilo = 1000.0
Hour = 60.0 * Minute
Minute = 60.0
"""@EN; 
                      rdfs:subClassOf ddhub:Unit. 
ddhub:KilometrePerHour a owl:Class; 
                       rdfs:comment """[v] = a * [SI]
where
[v] is the value in kilometre per hour
[SI] is the value in SI
a = Hour/Kilo, i.e., 3.6
and
Hour = 60.0 * Minute
Kilo = 1000.0
Minute = 60.0
"""@EN; 
                       rdfs:subClassOf ddhub:Unit. 
ddhub:KilometrePerHourPerSecond a owl:Class; 
                                rdfs:comment """[v] = a * [SI]
where
[v] is the value in kilometre per hour per second
[SI] is the value in SI
a = Hour/Kilo, i.e., 3.6
and
Hour = 60.0 * Minute
Kilo = 1000.0
Minute = 60.0
"""@EN; 
                                rdfs:subClassOf ddhub:Unit. 
ddhub:KilometrePerMinute a owl:Class; 
                         rdfs:comment """[v] = a * [SI]
where
[v] is the value in kilometre per minute
[SI] is the value in SI
a = Minute/Kilo, i.e., 0.06
and
Minute = 60.0
Kilo = 1000.0
"""@EN; 
                         rdfs:subClassOf ddhub:Unit. 
ddhub:KilometrePerMinutePerSecond a owl:Class; 
                                  rdfs:comment """[v] = a * [SI]
where
[v] is the value in kilometre per minute per second
[SI] is the value in SI
a = Minute/Kilo, i.e., 0.06
and
Minute = 60.0
Kilo = 1000.0
"""@EN; 
                                  rdfs:subClassOf ddhub:Unit. 
ddhub:KilometrePerSecond a owl:Class; 
                         rdfs:comment """[v] = a * [SI]
where
[v] is the value in kilometre per second
[SI] is the value in SI
a = Unit/Kilo, i.e., 0.001
and
Unit = 1.0
Kilo = 1000.0
"""@EN; 
                         rdfs:subClassOf ddhub:Unit. 
ddhub:KilometrePerSecondSquared a owl:Class; 
                                rdfs:comment """[v] = a * [SI]
where
[v] is the value in kilometre per second squared
[SI] is the value in SI
a = 1.0/Kilo, i.e., 0.001
and
Kilo = 1000.0
"""@EN; 
                                rdfs:subClassOf ddhub:Unit. 
ddhub:Kilomole a owl:Class; 
               rdfs:comment """[v] = a * [SI]
where
[v] is the value in kilomole
[SI] is the value in SI
a = 1.0/Kilo, i.e., 0.001
and
Kilo = 1000.0
"""@EN; 
               rdfs:subClassOf ddhub:Unit. 
ddhub:Kilonewton a owl:Class; 
                 rdfs:comment """[v] = a * [SI]
where
[v] is the value in kilonewton
[SI] is the value in SI
a = 1.0/Kilo, i.e., 0.001
and
Kilo = 1000.0
"""@EN; 
                 rdfs:subClassOf ddhub:Unit. 
ddhub:KilonewtonMetre a owl:Class; 
                      rdfs:comment """[v] = a * [SI]
where
[v] is the value in kilonewton metre
[SI] is the value in SI
a = 1.0/Kilo, i.e., 0.001
and
Kilo = 1000.0
"""@EN; 
                      rdfs:subClassOf ddhub:Unit. 
ddhub:KilonewtonMetrePerCentimetre a owl:Class; 
                                   rdfs:comment """[v] = a * [SI]
where
[v] is the value in kilonewton metre per centimetre
[SI] is the value in SI
a = Centi/(Kilo), i.e., 1E-05
and
Centi = 0.01
Kilo = 1000.0
"""@EN; 
                                   rdfs:subClassOf ddhub:Unit. 
ddhub:KilonewtonMetrePerDecimetre a owl:Class; 
                                  rdfs:comment """[v] = a * [SI]
where
[v] is the value in kilonewton metre per decimetre
[SI] is the value in SI
a = Deci/(Kilo*Unit), i.e., 0.0001
and
Deci = 0.1
Kilo = 1000.0
Unit = 1.0
"""@EN; 
                                  rdfs:subClassOf ddhub:Unit. 
ddhub:KilonewtonMetrePerFoot a owl:Class; 
                             rdfs:comment """[v] = a * [SI]
where
[v] is the value in kilonewton metre per foot
[SI] is the value in SI
a = Foot/Kilo, i.e., 0.0003048
and
Foot = 12.0 * Inch
Kilo = 1000.0
Inch = 0.0254 reference: https://www.nist.gov/pml/owm/si-units-length
"""@EN; 
                             rdfs:subClassOf ddhub:Unit. 
ddhub:KilonewtonMetrePerHour a owl:Class; 
                             rdfs:comment """[v] = a * [SI]
where
[v] is the value in kilonewton metre per hour
[SI] is the value in SI
a = Hour/Kilo, i.e., 3.6
and
Hour = 60.0 * Minute
Kilo = 1000.0
Minute = 60.0
"""@EN; 
                             rdfs:subClassOf ddhub:Unit. 
ddhub:KilonewtonMetrePerInch a owl:Class; 
                             rdfs:comment """[v] = a * [SI]
where
[v] is the value in kilonewton metre per inch
[SI] is the value in SI
a = Inch/Kilo, i.e., 2.5399999999999997E-05
and
Inch = 0.0254 reference: https://www.nist.gov/pml/owm/si-units-length
Kilo = 1000.0
"""@EN; 
                             rdfs:subClassOf ddhub:Unit. 
ddhub:KilonewtonMetrePerMetre a owl:Class; 
                              rdfs:comment """[v] = a * [SI]
where
[v] is the value in kilonewton metre per metre
[SI] is the value in SI
a = Unit/Kilo, i.e., 0.001
and
Unit = 1.0
Kilo = 1000.0
"""@EN; 
                              rdfs:subClassOf ddhub:Unit. 
ddhub:KilonewtonMetrePerMillimetre a owl:Class; 
                                   rdfs:comment """[v] = a * [SI]
where
[v] is the value in kilonewton metre per millimetre
[SI] is the value in SI
a = Milli/(Kilo), i.e., 1E-06
and
Milli = 0.001
Kilo = 1000.0
"""@EN; 
                                   rdfs:subClassOf ddhub:Unit. 
ddhub:KilonewtonMetrePerMinute a owl:Class; 
                               rdfs:comment """[v] = a * [SI]
where
[v] is the value in kilonewton metre per minute
[SI] is the value in SI
a = Minute/Kilo, i.e., 0.06
and
Minute = 60.0
Kilo = 1000.0
"""@EN; 
                               rdfs:subClassOf ddhub:Unit. 
ddhub:KilonewtonMetrePerSecond a owl:Class; 
                               rdfs:comment """[v] = a * [SI]
where
[v] is the value in kilonewton metre per second
[SI] is the value in SI
a = 1.0/Kilo, i.e., 0.001
and
Kilo = 1000.0
"""@EN; 
                               rdfs:subClassOf ddhub:Unit. 
ddhub:KilonewtonPer10Metre a owl:Class; 
                           rdfs:comment """[v] = a * [SI]
where
[v] is the value in kilonewton per 10 metre
[SI] is the value in SI
a = Deca/Kilo, i.e., 0.01
and
Deca = 10.0
Kilo = 1000.0
"""@EN; 
                           rdfs:subClassOf ddhub:Unit. 
ddhub:KilonewtonPer30Metre a owl:Class; 
                           rdfs:comment """[v] = a * [SI]
where
[v] is the value in kilonewton per 30 metre
[SI] is the value in SI
a = 3*Deca/Kilo, i.e., 0.03
and
Deca = 10.0
Kilo = 1000.0
"""@EN; 
                           rdfs:subClassOf ddhub:Unit. 
ddhub:KilonewtonPerCentimetre a owl:Class; 
                              rdfs:comment """[v] = a * [SI]
where
[v] is the value in kilonewton per centimetre
[SI] is the value in SI
a = Centi/Kilo, i.e., 1E-05
and
Centi = 0.01
Kilo = 1000.0
"""@EN; 
                              rdfs:subClassOf ddhub:Unit. 
ddhub:KilonewtonPerDecimetre a owl:Class; 
                             rdfs:comment """[v] = a * [SI]
where
[v] is the value in kilonewton per decimetre
[SI] is the value in SI
a = Deci/Kilo, i.e., 0.0001
and
Deci = 0.1
Kilo = 1000.0
"""@EN; 
                             rdfs:subClassOf ddhub:Unit. 
ddhub:KilonewtonPerHour a owl:Class; 
                        rdfs:comment """[v] = a * [SI]
where
[v] is the value in kilonewton per hour
[SI] is the value in SI
a = Hour/Kilo, i.e., 3.6
and
Hour = 60.0 * Minute
Kilo = 1000.0
Minute = 60.0
"""@EN; 
                        rdfs:subClassOf ddhub:Unit. 
ddhub:KilonewtonPerMetre a owl:Class; 
                         rdfs:comment """[v] = a * [SI]
where
[v] is the value in kilonewton per metre
[SI] is the value in SI
a = 1.0/Kilo, i.e., 0.001
and
Kilo = 1000.0
"""@EN; 
                         rdfs:subClassOf ddhub:Unit. 
ddhub:KilonewtonPerMillimetre a owl:Class; 
                              rdfs:comment """[v] = a * [SI]
where
[v] is the value in kilonewton per millimetre
[SI] is the value in SI
a = Milli/Kilo, i.e., 1E-06
and
Milli = 0.001
Kilo = 1000.0
"""@EN; 
                              rdfs:subClassOf ddhub:Unit. 
ddhub:KilonewtonPerMinute a owl:Class; 
                          rdfs:comment """[v] = a * [SI]
where
[v] is the value in kilonewton per minute
[SI] is the value in SI
a = Minute/Kilo, i.e., 0.06
and
Minute = 60.0
Kilo = 1000.0
"""@EN; 
                          rdfs:subClassOf ddhub:Unit. 
ddhub:KilonewtonPerSecond a owl:Class; 
                          rdfs:comment """[v] = a * [SI]
where
[v] is the value in kilonewton per second
[SI] is the value in SI
a = 1.0/Kilo, i.e., 0.001
and
Kilo = 1000.0
"""@EN; 
                          rdfs:subClassOf ddhub:Unit. 
ddhub:KilonewtonPerSquareMetre a owl:Class; 
                               rdfs:comment """[v] = a * [SI]
where
[v] is the value in kilonewton per square metre
[SI] is the value in SI
a = 1.0/Kilo, i.e., 0.001
and
Kilo = 1000.0
"""@EN; 
                               rdfs:subClassOf ddhub:Unit. 
ddhub:KilonewtonPerSquareMetrePerHour a owl:Class; 
                                      rdfs:comment """[v] = a * [SI]
where
[v] is the value in kilonewton per square metre per hour
[SI] is the value in SI
a = Hour/Kilo, i.e., 3.6
and
Hour = 60.0 * Minute
Kilo = 1000.0
Minute = 60.0
"""@EN; 
                                      rdfs:subClassOf ddhub:Unit. 
ddhub:KilonewtonPerSquareMetrePerMinute a owl:Class; 
                                        rdfs:comment """[v] = a * [SI]
where
[v] is the value in kilonewton per square metre per minute
[SI] is the value in SI
a = Minute/Kilo, i.e., 0.06
and
Minute = 60.0
Kilo = 1000.0
"""@EN; 
                                        rdfs:subClassOf ddhub:Unit. 
ddhub:KilonewtonPerSquareMetrePerSecond a owl:Class; 
                                        rdfs:comment """[v] = a * [SI]
where
[v] is the value in kilonewton per square metre per second
[SI] is the value in SI
a = 1.0/Kilo, i.e., 0.001
and
Kilo = 1000.0
"""@EN; 
                                        rdfs:subClassOf ddhub:Unit. 
ddhub:KiloOhmMetre a owl:Class; 
                   rdfs:comment """[v] = a * [SI]
where
[v] is the value in kilo ohm metre
[SI] is the value in SI
a = 1.0/Kilo, i.e., 0.001
and
Kilo = 1000.0
"""@EN; 
                   rdfs:subClassOf ddhub:Unit. 
ddhub:Kilopascal a owl:Class; 
                 rdfs:comment """[v] = a * [SI]
where
[v] is the value in kilopascal
[SI] is the value in SI
a = 1.0/Kilo, i.e., 0.001
and
Kilo = 1000.0
"""@EN; 
                 rdfs:subClassOf ddhub:Unit. 
ddhub:KilopascalPerHour a owl:Class; 
                        rdfs:comment """[v] = a * [SI]
where
[v] is the value in kilopascal per hour
[SI] is the value in SI
a = Hour/Kilo, i.e., 3.6
and
Hour = 60.0 * Minute
Kilo = 1000.0
Minute = 60.0
"""@EN; 
                        rdfs:subClassOf ddhub:Unit. 
ddhub:KilopascalPerMinute a owl:Class; 
                          rdfs:comment """[v] = a * [SI]
where
[v] is the value in kilopascal per minute
[SI] is the value in SI
a = Minute/Kilo, i.e., 0.06
and
Minute = 60.0
Kilo = 1000.0
"""@EN; 
                          rdfs:subClassOf ddhub:Unit. 
ddhub:KilopascalPerSecond a owl:Class; 
                          rdfs:comment """[v] = a * [SI]
where
[v] is the value in kilopascal per second
[SI] is the value in SI
a = 1.0/Kilo, i.e., 0.001
and
Kilo = 1000.0
"""@EN; 
                          rdfs:subClassOf ddhub:Unit. 
ddhub:Kilopound a owl:Class; 
                rdfs:comment """[v] = a * [SI]
where
[v] is the value in kilopound
[SI] is the value in SI
a = 1.0/(Kilo * Pound), i.e., 0.002204622621848776
and
Kilo = 1000.0
Pound = 0.45359237 reference: https://en.wikipedia.org/wiki/Pound_(mass)
"""@EN; 
                rdfs:subClassOf ddhub:Unit. 
ddhub:KilopoundForce a owl:Class; 
                     rdfs:comment """[v] = a * [SI]
where
[v] is the value in kilopound force
[SI] is the value in SI
a = 1.0/(Kilo*PoundForce), i.e., 0.0002248089430997105
and
Kilo = 1000.0
PoundForce = Pound * G reference: https://en.wikipedia.org/wiki/Pound_(force)
Pound = 0.45359237 reference: https://en.wikipedia.org/wiki/Pound_(mass)
G = 9.80665 reference: https://en.wikipedia.org/wiki/Gravity_of_Earth
"""@EN; 
                     rdfs:subClassOf ddhub:Unit. 
ddhub:KilopoundForcePerHour a owl:Class; 
                            rdfs:comment """[v] = a * [SI]
where
[v] is the value in kilopound force per hour
[SI] is the value in SI
a = Hour/(Kilo*PoundForce), i.e., 0.8093121951589578
and
Hour = 60.0 * Minute
Kilo = 1000.0
PoundForce = Pound * G reference: https://en.wikipedia.org/wiki/Pound_(force)
Minute = 60.0
Pound = 0.45359237 reference: https://en.wikipedia.org/wiki/Pound_(mass)
G = 9.80665 reference: https://en.wikipedia.org/wiki/Gravity_of_Earth
"""@EN; 
                            rdfs:subClassOf ddhub:Unit. 
ddhub:KilopoundForcePerMinute a owl:Class; 
                              rdfs:comment """[v] = a * [SI]
where
[v] is the value in kilopound force per minute
[SI] is the value in SI
a = Minute/(Kilo*PoundForce), i.e., 0.01348853658598263
and
Minute = 60.0
Kilo = 1000.0
PoundForce = Pound * G reference: https://en.wikipedia.org/wiki/Pound_(force)
Pound = 0.45359237 reference: https://en.wikipedia.org/wiki/Pound_(mass)
G = 9.80665 reference: https://en.wikipedia.org/wiki/Gravity_of_Earth
"""@EN; 
                              rdfs:subClassOf ddhub:Unit. 
ddhub:KilopoundForcePerSecond a owl:Class; 
                              rdfs:comment """[v] = a * [SI]
where
[v] is the value in kilopound force per second
[SI] is the value in SI
a = 1.0/(Kilo*PoundForce), i.e., 0.0002248089430997105
and
Kilo = 1000.0
PoundForce = Pound * G reference: https://en.wikipedia.org/wiki/Pound_(force)
Pound = 0.45359237 reference: https://en.wikipedia.org/wiki/Pound_(mass)
G = 9.80665 reference: https://en.wikipedia.org/wiki/Gravity_of_Earth
"""@EN; 
                              rdfs:subClassOf ddhub:Unit. 
ddhub:KilopoundPer100Foot a owl:Class; 
                          rdfs:comment """[v] = a * [SI]
where
[v] is the value in kilopound per 100 foot
[SI] is the value in SI
a = 100.0*Foot/(Kilo*PoundForce), i.e., 0.006852176585679175
and
Foot = 12.0 * Inch
Kilo = 1000.0
PoundForce = Pound * G reference: https://en.wikipedia.org/wiki/Pound_(force)
Inch = 0.0254 reference: https://www.nist.gov/pml/owm/si-units-length
Pound = 0.45359237 reference: https://en.wikipedia.org/wiki/Pound_(mass)
G = 9.80665 reference: https://en.wikipedia.org/wiki/Gravity_of_Earth
"""@EN; 
                          rdfs:subClassOf ddhub:Unit. 
ddhub:KilopoundPer30Foot a owl:Class; 
                         rdfs:comment """[v] = a * [SI]
where
[v] is the value in kilopound per 30 foot
[SI] is the value in SI
a = 30.0*Foot/(Kilo*PoundForce), i.e., 0.0020556529757037524
and
Foot = 12.0 * Inch
Kilo = 1000.0
PoundForce = Pound * G reference: https://en.wikipedia.org/wiki/Pound_(force)
Inch = 0.0254 reference: https://www.nist.gov/pml/owm/si-units-length
Pound = 0.45359237 reference: https://en.wikipedia.org/wiki/Pound_(mass)
G = 9.80665 reference: https://en.wikipedia.org/wiki/Gravity_of_Earth
"""@EN; 
                         rdfs:subClassOf ddhub:Unit. 
ddhub:KilopoundPerFoot a owl:Class; 
                       rdfs:comment """[v] = a * [SI]
where
[v] is the value in kilopound per foot
[SI] is the value in SI
a = Foot/(Kilo*PoundForce), i.e., 6.852176585679175E-05
and
Foot = 12.0 * Inch
Kilo = 1000.0
PoundForce = Pound * G reference: https://en.wikipedia.org/wiki/Pound_(force)
Inch = 0.0254 reference: https://www.nist.gov/pml/owm/si-units-length
Pound = 0.45359237 reference: https://en.wikipedia.org/wiki/Pound_(mass)
G = 9.80665 reference: https://en.wikipedia.org/wiki/Gravity_of_Earth
"""@EN; 
                       rdfs:subClassOf ddhub:Unit. 
ddhub:KilopoundPerInch a owl:Class; 
                       rdfs:comment """[v] = a * [SI]
where
[v] is the value in kilopound per inch
[SI] is the value in SI
a = Inch/(Kilo*PoundForce), i.e., 5.7101471547326466E-06
and
Inch = 0.0254 reference: https://www.nist.gov/pml/owm/si-units-length
Kilo = 1000.0
PoundForce = Pound * G reference: https://en.wikipedia.org/wiki/Pound_(force)
Pound = 0.45359237 reference: https://en.wikipedia.org/wiki/Pound_(mass)
G = 9.80665 reference: https://en.wikipedia.org/wiki/Gravity_of_Earth
"""@EN; 
                       rdfs:subClassOf ddhub:Unit. 
ddhub:KilopoundPerSquareInch a owl:Class; 
                             rdfs:comment """[v] = a * [SI]
where
[v] is the value in kilopound per square inch
[SI] is the value in SI
a = 1.0/(Kilo*PSI), i.e., 1.4503773773020924E-07
and
Kilo = 1000.0
PSI = PoundForce / (Inch * Inch) reference: https://en.wikipedia.org/wiki/Pound_per_square_inch
PoundForce = Pound * G reference: https://en.wikipedia.org/wiki/Pound_(force)
Inch = 0.0254 reference: https://www.nist.gov/pml/owm/si-units-length
Pound = 0.45359237 reference: https://en.wikipedia.org/wiki/Pound_(mass)
G = 9.80665 reference: https://en.wikipedia.org/wiki/Gravity_of_Earth
"""@EN; 
                             rdfs:subClassOf ddhub:Unit. 
ddhub:KilopoundPerSquareInchPerHour a owl:Class; 
                                    rdfs:comment """[v] = a * [SI]
where
[v] is the value in kilopound per square inch per hour
[SI] is the value in SI
a = Hour/(Kilo*PSI), i.e., 0.0005221358558287532
and
Hour = 60.0 * Minute
Kilo = 1000.0
PSI = PoundForce / (Inch * Inch) reference: https://en.wikipedia.org/wiki/Pound_per_square_inch
Minute = 60.0
PoundForce = Pound * G reference: https://en.wikipedia.org/wiki/Pound_(force)
Inch = 0.0254 reference: https://www.nist.gov/pml/owm/si-units-length
Pound = 0.45359237 reference: https://en.wikipedia.org/wiki/Pound_(mass)
G = 9.80665 reference: https://en.wikipedia.org/wiki/Gravity_of_Earth
"""@EN; 
                                    rdfs:subClassOf ddhub:Unit. 
ddhub:KilopoundPerSquareInchPerMinute a owl:Class; 
                                      rdfs:comment """[v] = a * [SI]
where
[v] is the value in kilopound per square inch per minute
[SI] is the value in SI
a = Minute/(Kilo*PSI), i.e., 8.702264263812555E-06
and
Minute = 60.0
Kilo = 1000.0
PSI = PoundForce / (Inch * Inch) reference: https://en.wikipedia.org/wiki/Pound_per_square_inch
PoundForce = Pound * G reference: https://en.wikipedia.org/wiki/Pound_(force)
Inch = 0.0254 reference: https://www.nist.gov/pml/owm/si-units-length
Pound = 0.45359237 reference: https://en.wikipedia.org/wiki/Pound_(mass)
G = 9.80665 reference: https://en.wikipedia.org/wiki/Gravity_of_Earth
"""@EN; 
                                      rdfs:subClassOf ddhub:Unit. 
ddhub:KilopoundPerSquareInchPerSecond a owl:Class; 
                                      rdfs:comment """[v] = a * [SI]
where
[v] is the value in kilopound per square inch per second
[SI] is the value in SI
a = 1.0/(Kilo*PSI), i.e., 1.4503773773020924E-07
and
Kilo = 1000.0
PSI = PoundForce / (Inch * Inch) reference: https://en.wikipedia.org/wiki/Pound_per_square_inch
PoundForce = Pound * G reference: https://en.wikipedia.org/wiki/Pound_(force)
Inch = 0.0254 reference: https://www.nist.gov/pml/owm/si-units-length
Pound = 0.45359237 reference: https://en.wikipedia.org/wiki/Pound_(mass)
G = 9.80665 reference: https://en.wikipedia.org/wiki/Gravity_of_Earth
"""@EN; 
                                      rdfs:subClassOf ddhub:Unit. 
ddhub:Kilotonne a owl:Class; 
                rdfs:comment """[v] = a * [SI]
where
[v] is the value in kilotonne
[SI] is the value in SI
a = 1.0/Mega, i.e., 1E-06
and
Mega = 1e6
"""@EN; 
                rdfs:subClassOf ddhub:Unit. 
ddhub:Kilovolt a owl:Class; 
               rdfs:comment """[v] = a * [SI]
where
[v] is the value in kilovolt
[SI] is the value in SI
a = 1.0/Kilo, i.e., 0.001
and
Kilo = 1000.0
"""@EN; 
               rdfs:subClassOf ddhub:Unit. 
ddhub:Kilowatt a owl:Class; 
               rdfs:comment """[v] = a * [SI]
where
[v] is the value in kilowatt
[SI] is the value in SI
a = 1.0/Kilo, i.e., 0.001
and
Kilo = 1000.0
"""@EN; 
               rdfs:subClassOf ddhub:Unit. 
ddhub:KnotPerSecond a owl:Class; 
                    rdfs:comment """[v] = a * [SI]
where
[v] is the value in knot per second
[SI] is the value in SI
a = 1.0/Knot, i.e., 1.9438444924406046
and
Knot = 1.852 * Kilo / Hour reference: https://en.wikipedia.org/wiki/Knot_(unit)
Kilo = 1000.0
Hour = 60.0 * Minute
Minute = 60.0
"""@EN; 
                    rdfs:subClassOf ddhub:Unit. 
ddhub:L a owl:DatatypeProperty, owl:FunctionalProperty; 
        rdfs:comment """Length exponent.
SI Unit: metre (m)
"""@EN; 
        rdfs:domain ddhub:Quantity; 
        rdfs:range xsd:double. 
ddhub:LandBop a owl:Class; 
              rdfs:comment ""@EN; 
              rdfs:subClassOf ddhub:BopStack. 
ddhub:LandingJoint a owl:Class; 
                   rdfs:comment ""@EN; 
                   rdfs:subClassOf ddhub:MarineSystem. 
ddhub:LandingString a owl:Class; 
                    rdfs:comment ""@EN; 
                    rdfs:subClassOf ddhub:CasingEquipment. 
ddhub:LastCasingShoeReferenceLocation a owl:Class; 
                                      rdfs:comment ""@EN; 
                                      rdfs:subClassOf ddhub:AbscissaReferenceLocation. 
ddhub:LateralModelling a owl:Class; 
                       rdfs:comment """The model accounts for the lateral movement of some parts of the physical system.
"""@EN; 
                       rdfs:subClassOf ddhub:ModelledDegreeOfFreedom. 
ddhub:LateralMotionType a owl:Class; 
                        rdfs:comment ""@EN; 
                        rdfs:subClassOf ddhub:MotionType. 
ddhub:LeapSeconds a owl:DatatypeProperty, owl:FunctionalProperty; 
                  rdfs:comment """
"""@EN; 
                  rdfs:domain ddhub:Clock; 
                  rdfs:range xsd:int. 
ddhub:LeaseLinePositionLocation a owl:Class; 
                                rdfs:comment ""@EN; 
                                rdfs:subClassOf ddhub:PositionReferenceLocation. 
ddhub:LedgeLocation a owl:Class; 
                    rdfs:comment ""@EN; 
                    rdfs:subClassOf ddhub:AbscissaReferenceLocation. 
ddhub:LeftToRight a owl:DatatypeProperty, owl:FunctionalProperty; 
                  rdfs:comment """Indicates whether the fluid can flow from the left branch to the right branch though the junction
"""@EN; 
                  rdfs:domain ddhub:HydraulicJunction; 
                  rdfs:range xsd:bool. 
ddhub:LengthQuantity a owl:Class; 
                     rdfs:comment """Length is a measure of distance.
The dimension of length is:
$$[L]$$.
The SI unit for **length** is: metre with the associated unit label $m$
"""@EN; 
                     rdfs:subClassOf ddhub:Quantity. 
ddhub:LengthSmallQuantity a owl:Class; 
                          rdfs:comment """Length is a measure of distance.
The dimension of length is:
$$[L]$$.
The SI unit for **length** is: metre with the associated unit label $m$
The meaningful precision of small length is typically: 1E-05 m
"""@EN; 
                          rdfs:subClassOf ddhub:MeasurableQuantity. 
ddhub:LengthStandardQuantity a owl:Class; 
                             rdfs:comment """Length is a measure of distance.
The dimension of length is:
$$[L]$$.
The SI unit for **length** is: metre with the associated unit label $m$
The meaningful precision of a standard length is typically: 0.001 m
"""@EN; 
                             rdfs:subClassOf ddhub:MeasurableQuantity. 
ddhub:LightYear a owl:Class; 
                rdfs:comment """[v] = a * [SI]
where
[v] is the value in light year
[SI] is the value in SI
a = 1.0/LightYear, i.e., 1.0570008340246154E-16
and
LightYear = 9460730472580800.0 reference: https://www.iau.org/public/themes/measuring/
"""@EN; 
                rdfs:subClassOf ddhub:Unit. 
ddhub:Limit a owl:Class; 
            rdfs:comment ""@EN; 
            rdfs:subClassOf ddhub:ProcessData. 
ddhub:Line a owl:Class; 
           rdfs:comment """[v] = a * [SI]
where
[v] is the value in line
[SI] is the value in SI
a = 1.0/Line, i.e., 100000000
and
Line = 1e-8 reference: https://en.wikipedia.org/wiki/Maxwell_(unit)
"""@EN; 
           rdfs:subClassOf ddhub:Unit. 
ddhub:Liner a owl:Class; 
            rdfs:comment ""@EN; 
            rdfs:subClassOf ddhub:PistonMudPump. 
ddhub:LinerDrilling a owl:Class; 
                    rdfs:comment ""@EN; 
                    rdfs:subClassOf ddhub:DrillingEquipment. 
ddhub:LinerHanger a owl:Class; 
                  rdfs:comment ""@EN; 
                  rdfs:subClassOf ddhub:Hangers. 
ddhub:LinerPacker a owl:Class; 
                  rdfs:comment ""@EN; 
                  rdfs:subClassOf ddhub:CasingEquipment. 
ddhub:Liners a owl:Class; 
             rdfs:comment ""@EN; 
             rdfs:subClassOf ddhub:CasingString. 
ddhub:LinerStringDescription a owl:Class; 
                             rdfs:comment """A liner string is a drill-stem that is used to complete a section. It is composed of casing joints, possibly a shoe track
a liner hanger and drill-pipes.
"""@EN; 
                             rdfs:subClassOf ddhub:DrillStemDescription. 
ddhub:LiquidComponent a owl:Class; 
                      rdfs:comment ""@EN; 
                      rdfs:subClassOf ddhub:FluidComponent. 
ddhub:Litre a owl:Class; 
            rdfs:comment """[v] = a * [SI]
where
[v] is the value in litre
[SI] is the value in SI
a = 1.0/Milli, i.e., 1000
and
Milli = 0.001
"""@EN; 
            rdfs:subClassOf ddhub:Unit. 
ddhub:LitrePerDay a owl:Class; 
                  rdfs:comment """[v] = a * [SI]
where
[v] is the value in litre per day
[SI] is the value in SI
a = Day / Milli, i.e., 86400000
and
Day = 24.0 * Hour
Milli = 0.001
Hour = 60.0 * Minute
Minute = 60.0
"""@EN; 
                  rdfs:subClassOf ddhub:Unit. 
ddhub:LitrePerHour a owl:Class; 
                   rdfs:comment """[v] = a * [SI]
where
[v] is the value in litre per hour
[SI] is the value in SI
a = Hour/ Milli, i.e., 3600000
and
Hour = 60.0 * Minute
Milli = 0.001
Minute = 60.0
"""@EN; 
                   rdfs:subClassOf ddhub:Unit. 
ddhub:LitrePerMinute a owl:Class; 
                     rdfs:comment """[v] = a * [SI]
where
[v] is the value in litre per minute
[SI] is the value in SI
a = Minute / Milli, i.e., 60000
and
Minute = 60.0
Milli = 0.001
"""@EN; 
                     rdfs:subClassOf ddhub:Unit. 
ddhub:LitrePerMinutePerSecond a owl:Class; 
                              rdfs:comment """[v] = a * [SI]
where
[v] is the value in litre per minute per second
[SI] is the value in SI
a = Minute/Milli, i.e., 60000
and
Minute = 60.0
Milli = 0.001
"""@EN; 
                              rdfs:subClassOf ddhub:Unit. 
ddhub:LitrePerMinuteSquared a owl:Class; 
                            rdfs:comment """[v] = a * [SI]
where
[v] is the value in litre per minute squared
[SI] is the value in SI
a = Minute*Minute/Milli, i.e., 3600000
and
Minute = 60.0
Milli = 0.001
"""@EN; 
                            rdfs:subClassOf ddhub:Unit. 
ddhub:LitrePerSecond a owl:Class; 
                     rdfs:comment """[v] = a * [SI]
where
[v] is the value in litre per second
[SI] is the value in SI
a = 1.0/Milli, i.e., 1000
and
Milli = 0.001
"""@EN; 
                     rdfs:subClassOf ddhub:Unit. 
ddhub:LitrePerSecondSquared a owl:Class; 
                            rdfs:comment """[v] = a * [SI]
where
[v] is the value in litre per second squared
[SI] is the value in SI
a = 1.0/Milli, i.e., 1000
and
Milli = 0.001
"""@EN; 
                            rdfs:subClassOf ddhub:Unit. 
ddhub:LitrePerYear a owl:Class; 
                   rdfs:comment """[v] = a * [SI]
where
[v] is the value in litre per year
[SI] is the value in SI
a = YearJulian/Milli, i.e., 31557600000
and
YearJulian = 365.25 * Day
Milli = 0.001
Day = 24.0 * Hour
Hour = 60.0 * Minute
Minute = 60.0
"""@EN; 
                   rdfs:subClassOf ddhub:Unit. 
ddhub:LoadNut a owl:Class; 
              rdfs:comment ""@EN; 
              rdfs:subClassOf ddhub:TopDrive. 
ddhub:LocalTimeReference a owl:Class; 
                         rdfs:comment ""@EN; 
                         rdfs:subClassOf ddhub:RelativeTimeReference. 
ddhub:Location a owl:Class; 
               rdfs:comment """Physical location for a signal. Refers to: 1) a reference frame (via the HasReferenceFrame relation), that works as a system of coordinates 2) an origin (of type Location) via the HasReferenceFrameOrigin relation.
 - some coordinates
"""@EN; 
               rdfs:subClassOf ddhub:DWISNoun. 
ddhub:LoggingEquipment a owl:Class; 
                       rdfs:comment ""@EN; 
                       rdfs:subClassOf ddhub:DownholeEquipment. 
ddhub:LoggingServiceCompany a owl:Class; 
                            rdfs:comment """A logging service company is an entity that gathers measured information during well construction.
"""@EN; 
                            rdfs:subClassOf ddhub:ServiceCompany. 
ddhub:LoggingWhileDrillingTools a owl:Class; 
                                rdfs:comment ""@EN; 
                                rdfs:subClassOf ddhub:LoggingEquipment. 
ddhub:LoggingWhileDrillingToolsAcoustictools a owl:Class; 
                                             rdfs:comment ""@EN; 
                                             rdfs:subClassOf ddhub:LoggingWhileDrillingTools. 
ddhub:LoggingWhileDrillingToolsElectricalpropagation a owl:Class; 
                                                     rdfs:comment ""@EN; 
                                                     rdfs:subClassOf ddhub:LoggingWhileDrillingTools. 
ddhub:LoggingWhileDrillingToolsElectricalresistivity a owl:Class; 
                                                     rdfs:comment ""@EN; 
                                                     rdfs:subClassOf ddhub:LoggingWhileDrillingTools. 
ddhub:LoggingWhileDrillingToolsNmrtools a owl:Class; 
                                        rdfs:comment ""@EN; 
                                        rdfs:subClassOf ddhub:LoggingWhileDrillingTools. 
ddhub:LoggingWhileDrillingToolsNucleartools a owl:Class; 
                                            rdfs:comment ""@EN; 
                                            rdfs:subClassOf ddhub:LoggingWhileDrillingTools. 
ddhub:LoggingWhileDrillingToolsSeismictools a owl:Class; 
                                            rdfs:comment ""@EN; 
                                            rdfs:subClassOf ddhub:LoggingWhileDrillingTools. 
ddhub:LogName a owl:DatatypeProperty, owl:FunctionalProperty; 
              rdfs:comment """
"""@EN; 
              rdfs:domain ddhub:WitsMLTimeBasedLogEndPoint; 
              rdfs:range xsd:string. 
ddhub:LogUID a owl:DatatypeProperty, owl:FunctionalProperty; 
             rdfs:comment """
"""@EN; 
             rdfs:domain ddhub:WitsMLTimeBasedLogEndPoint; 
             rdfs:range xsd:string. 
ddhub:LossCirculation a owl:Class; 
                      rdfs:comment """This Noun is used to refer to a situation during which drilling fluid is lost to the formation.
"""@EN; 
                      rdfs:subClassOf ddhub:DrillingIncident. 
ddhub:LowerMarineRiserPackageLmrp a owl:Class; 
                                  rdfs:comment ""@EN; 
                                  rdfs:subClassOf ddhub:MarineSystem. 
ddhub:LowestAstronomicalTideVerticalLocation a owl:Class; 
                                             rdfs:comment ""@EN; 
                                             rdfs:subClassOf ddhub:VerticalReferenceLocation. 
ddhub:LowGravitySolidComponent a owl:Class; 
                               rdfs:comment ""@EN; 
                               rdfs:subClassOf ddhub:DrillingFluidSolidComponent. 
ddhub:LowPassFilter a owl:Class; 
                    rdfs:comment ""@EN; 
                    rdfs:subClassOf ddhub:Filter. 
ddhub:LowPressureRiser a owl:Class; 
                       rdfs:comment ""@EN; 
                       rdfs:subClassOf ddhub:SurfaceRiser. 
ddhub:LT a owl:Class; 
         rdfs:comment ""@EN; 
         rdfs:subClassOf ddhub:ValidityCondition. 
ddhub:LumenPerSteradian a owl:Class; 
                        rdfs:comment """[v] = a * [SI]
where
[v] is the value in lumen per steradian
[SI] is the value in SI
a = 1.0/Unit, i.e., 1
and
Unit = 1.0
"""@EN; 
                        rdfs:subClassOf ddhub:Unit. 
ddhub:LuminousIntensityQuantity a owl:Class; 
                                rdfs:comment """Luminous intensity is the measure of the amount of visible light emitted by a source in a particular direction.
The dimension of luminous intensity is:
$$[J]$$.
The SI unit for **luminous intensity** is: candela with the associated unit label $cd$
"""@EN; 
                                rdfs:subClassOf ddhub:Quantity. 
ddhub:M a owl:DatatypeProperty, owl:FunctionalProperty; 
        rdfs:comment """Mass exponent.
SI Unit: Kilogram (kg)
"""@EN; 
        rdfs:domain ddhub:Quantity; 
        rdfs:range xsd:double. 
ddhub:MagneticFluxDensityQuantity a owl:Class; 
                                  rdfs:comment """Magnetic flux density is the measure of the strength of a magnetic field per unit area through which the magnetic flux passes. It indicates how concentrated the magnetic field is.
The dimension of magnetic flux density is:
$$[MI^{-1}T^{-2}]$$.
The SI unit for **magnetic flux density** is: tesla with the associated unit label $T$
"""@EN; 
                                  rdfs:subClassOf ddhub:Quantity. 
ddhub:MagneticFluxQuantity a owl:Class; 
                           rdfs:comment """Magnetic flux is the measure of the total magnetic field passing through a given area. It quantifies the strength and distribution of a magnetic field over a surface.
The dimension of magnetic flux is:
$$[L^{2}MI^{-1}T^{-2}]$$.
The SI unit for **magnetic flux** is: weber with the associated unit label $Wb$
"""@EN; 
                           rdfs:subClassOf ddhub:Quantity. 
ddhub:MagneticFluxQuantum a owl:Class; 
                          rdfs:comment """[v] = a * [SI]
where
[v] is the value in magnetic flux quantum
[SI] is the value in SI
a = 1.0/MagneticFluxQuantum, i.e., 483597848416983.56
and
MagneticFluxQuantum = PlanckConstant / (2.0*ElectronCharge) reference: https://en.wikipedia.org/wiki/Magnetic_flux_quantum
PlanckConstant = 6.62607015e-34 reference: https://en.wikipedia.org/wiki/Planck_constant
ElectronCharge = 1.602176634e-19 reference: https://en.wikipedia.org/wiki/Elementary_charge
"""@EN; 
                          rdfs:subClassOf ddhub:Unit. 
ddhub:MagneticHighSideAngleLocation a owl:Class; 
                                    rdfs:comment ""@EN; 
                                    rdfs:subClassOf ddhub:AngleReferenceLocation. 
ddhub:MagneticNorthAzimuthLocation a owl:Class; 
                                   rdfs:comment ""@EN; 
                                   rdfs:subClassOf ddhub:AzimuthReferenceLocation. 
ddhub:MainframeAssembly a owl:Class; 
                        rdfs:comment ""@EN; 
                        rdfs:subClassOf ddhub:TopDrive. 
ddhub:ManagedDownholePressureFeature a owl:Class; 
                                     rdfs:comment """A managed downhole pressure feature indicates that something manages downhole pressure.
"""@EN; 
                                     rdfs:subClassOf ddhub:DownholePressureFeature. 
ddhub:ManagesIncident a owl:ObjectProperty; 
                      rdfs:comment """This Verb is used to indicate that a fault detection isolation and recovery function manages a drilling incident.
"""@EN; 
                      rdfs:domain ddhub:FDIRFunction; 
                      rdfs:range ddhub:DrillingIncident; 
                      rdfs:subPropertyOf ddhub:DWISVerb. 
ddhub:Mandrel a owl:Class; 
              rdfs:comment ""@EN; 
              rdfs:subClassOf ddhub:Connection. 
ddhub:ManualPipeTongs a owl:Class; 
                      rdfs:comment ""@EN; 
                      rdfs:subClassOf ddhub:DrillPipeTongs. 
ddhub:ManualSlips a owl:Class; 
                  rdfs:comment ""@EN; 
                  rdfs:subClassOf ddhub:RotarySlips. 
ddhub:MarineFuel a owl:Class; 
                 rdfs:comment ""@EN; 
                 rdfs:subClassOf ddhub:MarineSystem. 
ddhub:MarineRiser a owl:Class; 
                  rdfs:comment ""@EN; 
                  rdfs:subClassOf ddhub:DrillingRiser. 
ddhub:MarineRiserTensionerMrtRing a owl:Class; 
                                  rdfs:comment ""@EN; 
                                  rdfs:subClassOf ddhub:MarineSystem. 
ddhub:MarineSystem a owl:Class; 
                   rdfs:comment ""@EN; 
                   rdfs:subClassOf ddhub:RigEquipment. 
ddhub:MassDensityDrillingQuantity a owl:Class; 
                                  rdfs:comment """Mass density is the amount of mass per unit volume of a substance.
The dimension of mass density is:
$$[ML^{-3}]$$.
The SI unit for **mass density** is: kilogram per cubic metre with the associated unit label $\\frac{kg}{m^{3}}$
The meaningful precision of mass density in the drilling context is typically: 1 kg/m³
"""@EN; 
                                  rdfs:subClassOf ddhub:MeasurableQuantity. 
ddhub:MassDensityGradientPerLengthDrillingQuantity a owl:Class; 
                                                   rdfs:comment """A mass density gradient per length is the first derivative of a mass density compared to a distance: $\\frac{d\\rho}{ds}$, where $\\rho$ is the mass density and $s$ is a distance.
The dimension of mass density gradient per length is:
$$[ML^{-4}]$$.
The SI unit for **mass density gradient per length** is: kilogram per cubic metre per metre with the associated unit label $\\frac{\\frac{kg}{m^{3}}}{m}$
The meaningful precision of mass density gradient per length in the drilling context is typically: 0.001 kg/m³/m
"""@EN; 
                                                   rdfs:subClassOf ddhub:MeasurableQuantity. 
ddhub:MassDensityGradientPerLengthQuantity a owl:Class; 
                                           rdfs:comment """A mass density gradient per length is the first derivative of a mass density compared to a distance: $\\frac{d\\rho}{ds}$, where $\\rho$ is the mass density and $s$ is a distance.
The dimension of mass density gradient per length is:
$$[ML^{-4}]$$.
The SI unit for **mass density gradient per length** is: kilogram per cubic metre per metre with the associated unit label $\\frac{\\frac{kg}{m^{3}}}{m}$
"""@EN; 
                                           rdfs:subClassOf ddhub:Quantity. 
ddhub:MassDensityGradientPerTemperatureDrillingQuantity a owl:Class; 
                                                        rdfs:comment """A mass density gradient per temperature is the first derivative of a mass density compared to temperature: $\\frac{d\\rho}{dT}$, where $\\rho$ is a mass density and $T$ is temperature.
The dimension of mass density gradient per temperature is:
$$[MK^{-1}L^{-3}]$$.
The SI unit for **mass density gradient per temperature** is: kilogram per cubic metre per kelvin with the associated unit label $\\frac{\\frac{kg}{m^{3}}}{K}$
The meaningful precision of mass density gradient per temperature in the drilling context is typically: 0.001 kg/m³/K
"""@EN; 
                                                        rdfs:subClassOf ddhub:MeasurableQuantity. 
ddhub:MassDensityGradientPerTemperatureQuantity a owl:Class; 
                                                rdfs:comment """A mass density gradient per temperature is the first derivative of a mass density compared to temperature: $\\frac{d\\rho}{dT}$, where $\\rho$ is a mass density and $T$ is temperature.
The dimension of mass density gradient per temperature is:
$$[MK^{-1}L^{-3}]$$.
The SI unit for **mass density gradient per temperature** is: kilogram per cubic metre per kelvin with the associated unit label $\\frac{\\frac{kg}{m^{3}}}{K}$
"""@EN; 
                                                rdfs:subClassOf ddhub:Quantity. 
ddhub:MassDensityQuantity a owl:Class; 
                          rdfs:comment """Mass density is the amount of mass per unit volume of a substance.
The dimension of mass density is:
$$[ML^{-3}]$$.
The SI unit for **mass density** is: kilogram per cubic metre with the associated unit label $\\frac{kg}{m^{3}}$
"""@EN; 
                          rdfs:subClassOf ddhub:Quantity. 
ddhub:MassDensityRateOfChangeDrillingQuantity a owl:Class; 
                                              rdfs:comment """A mass density rate of change is the time derivative of a mass density: $\\frac{d\\rho}{dt}$, where $\\rho$ is the mass density and $t$ is time.
The dimension of mass density rate of change is:
$$[MT^{-1}L^{-3}]$$.
The SI unit for **mass density rate of change** is: kilogram per cubic metre per second with the associated unit label $\\frac{\\frac{kg}{m^{3}}}{s}$
The meaningful precision of mass density rate of change in the drilling context is typically: 0.001 kg/m³/s
"""@EN; 
                                              rdfs:subClassOf ddhub:MeasurableQuantity. 
ddhub:MassDensityRateOfChangeQuantity a owl:Class; 
                                      rdfs:comment """A mass density rate of change is the time derivative of a mass density: $\\frac{d\\rho}{dt}$, where $\\rho$ is the mass density and $t$ is time.
The dimension of mass density rate of change is:
$$[MT^{-1}L^{-3}]$$.
The SI unit for **mass density rate of change** is: kilogram per cubic metre per second with the associated unit label $\\frac{\\frac{kg}{m^{3}}}{s}$
"""@EN; 
                                      rdfs:subClassOf ddhub:Quantity. 
ddhub:MassDrillingQuantity a owl:Class; 
                           rdfs:comment """Mass can be experimentally defined as a measure of the body's inertia, meaning the resistance to acceleration (change of velocity) when a net force is applied. The object's mass also determines the strength of its gravitational attraction to other bodies.
The dimension of mass is:
$$[M]$$.
The SI unit for **mass** is: kilogram with the associated unit label $kg$
The meaningful precision of mass density in the drilling context is typically: 0.1 kg
"""@EN; 
                           rdfs:subClassOf ddhub:MeasurableQuantity. 
ddhub:MassGradientPerLengthDrillingQuantity a owl:Class; 
                                            rdfs:comment """A mass gradient per length is the first derivative of a mass compared to a distance: $\\frac{dm}{ds}$, where $m$ is a mass and $s$ is a distance.
The dimension of mass gradient per length is:
$$[ML^{-1}]$$.
The SI unit for **mass gradient per length** is: kilogram per metre with the associated unit label $\\frac{kg}{m}$
The meaningful precision of mass gradient per length in the drilling context is typically: 0.05 kg/m
"""@EN; 
                                            rdfs:subClassOf ddhub:MeasurableQuantity. 
ddhub:MassGradientPerLengthQuantity a owl:Class; 
                                    rdfs:comment """A mass gradient per length is the first derivative of a mass compared to a distance: $\\frac{dm}{ds}$, where $m$ is a mass and $s$ is a distance.
The dimension of mass gradient per length is:
$$[ML^{-1}]$$.
The SI unit for **mass gradient per length** is: kilogram per metre with the associated unit label $\\frac{kg}{m}$
"""@EN; 
                                    rdfs:subClassOf ddhub:Quantity. 
ddhub:MassQuantity a owl:Class; 
                   rdfs:comment """Mass can be experimentally defined as a measure of the body's inertia, meaning the resistance to acceleration (change of velocity) when a net force is applied. The object's mass also determines the strength of its gravitational attraction to other bodies.
The dimension of mass is:
$$[M]$$.
The SI unit for **mass** is: kilogram with the associated unit label $kg$
"""@EN; 
                   rdfs:subClassOf ddhub:Quantity. 
ddhub:MassRateDrillingQuantity a owl:Class; 
                               rdfs:comment """A mass rate is the time derivative of a mass: $\\frac{dm}{dt}$, where $m$ is a mass and $t$ is time.
The dimension of mass rate is:
$$[MT^{-1}]$$.
The SI unit for **mass rate** is: kilogram per second with the associated unit label $\\frac{kg}{s}$
The meaningful precision of mass rate in the drilling context is typically: 0.0001 kg/s
"""@EN; 
                               rdfs:subClassOf ddhub:MeasurableQuantity. 
ddhub:MassRateQuantity a owl:Class; 
                       rdfs:comment """A mass rate is the time derivative of a mass: $\\frac{dm}{dt}$, where $m$ is a mass and $t$ is time.
The dimension of mass rate is:
$$[MT^{-1}]$$.
The SI unit for **mass rate** is: kilogram per second with the associated unit label $\\frac{kg}{s}$
"""@EN; 
                       rdfs:subClassOf ddhub:Quantity. 
ddhub:MassTransferBasedDiscretization a owl:Class; 
                                      rdfs:comment """A model can properly estimate values at the level of mass transfer propagation.
"""@EN; 
                                      rdfs:subClassOf ddhub:ModellingDiscretization. 
ddhub:MaterialStrengthQuantity a owl:Class; 
                               rdfs:comment """Material strength refers to the ability of a material to withstand an applied force or load without failing or deforming. It measures how much stress a material can endure before it breaks, bends, or permanently deforms, often categorized into types like tensile, compressive, and shear strength.
The dimension of material strength is:
$$[ML^{-1}T^{-2}]$$.
The SI unit for **material strength** is: pascal with the associated unit label $Pa$
"""@EN; 
                               rdfs:subClassOf ddhub:Quantity. 
ddhub:MathematicalFormulation a owl:Class; 
                              rdfs:comment """A classification of the mathematical formulation used by a model.
"""@EN; 
                              rdfs:subClassOf ddhub:DWISNoun. 
ddhub:MaxFrequency a owl:DatatypeProperty, owl:FunctionalProperty; 
                   rdfs:comment """
"""@EN; 
                   rdfs:domain ddhub:BandPassFilter; 
                   rdfs:range xsd:double. 
ddhub:MaximumFluctuations a owl:DatatypeProperty, owl:FunctionalProperty; 
                          rdfs:comment """
"""@EN; 
                          rdfs:domain ddhub:Clock; 
                          rdfs:range xsd:double. 
ddhub:MaximumLimit a owl:Class; 
                   rdfs:comment ""@EN; 
                   rdfs:subClassOf ddhub:Limit. 
ddhub:Maxwell a owl:Class; 
              rdfs:comment """[v] = a * [SI]
where
[v] is the value in maxwell
[SI] is the value in SI
a = 1.0/Maxwell, i.e., 100000000
and
Maxwell = 1e-8 reference: https://en.wikipedia.org/wiki/Maxwell_(unit)
"""@EN; 
              rdfs:subClassOf ddhub:Unit. 
ddhub:MaxwellPerSquareCentimetre a owl:Class; 
                                 rdfs:comment """[v] = a * [SI]
where
[v] is the value in maxwell per square centimetre
[SI] is the value in SI
a = Centi*Centi/Unit, i.e., 0.0001
and
Centi = 0.01
Unit = 1.0
"""@EN; 
                                 rdfs:subClassOf ddhub:Unit. 
ddhub:MeanHigherHighWaterVerticalLocation a owl:Class; 
                                          rdfs:comment ""@EN; 
                                          rdfs:subClassOf ddhub:VerticalReferenceLocation. 
ddhub:MeanHighWaterVerticalLocation a owl:Class; 
                                    rdfs:comment ""@EN; 
                                    rdfs:subClassOf ddhub:VerticalReferenceLocation. 
ddhub:MeaningfulPrecision a owl:DatatypeProperty, owl:FunctionalProperty; 
                          rdfs:comment """
"""@EN; 
                          rdfs:domain ddhub:MeasurableQuantity; 
                          rdfs:range xsd:double. 
ddhub:MeanLowerLowWaterVerticalLocation a owl:Class; 
                                        rdfs:comment ""@EN; 
                                        rdfs:subClassOf ddhub:VerticalReferenceLocation. 
ddhub:MeanLowWaterVerticalLocation a owl:Class; 
                                   rdfs:comment ""@EN; 
                                   rdfs:subClassOf ddhub:VerticalReferenceLocation. 
ddhub:MeanSeaLevelVerticalLocation a owl:Class; 
                                   rdfs:comment ""@EN; 
                                   rdfs:subClassOf ddhub:VerticalReferenceLocation. 
ddhub:MeanTideLevelVerticalLocation a owl:Class; 
                                    rdfs:comment ""@EN; 
                                    rdfs:subClassOf ddhub:VerticalReferenceLocation. 
ddhub:MeasurableQuantity a owl:Class; 
                         rdfs:comment """Represents a quantity that allows meaningful comparisons.
A `MeasurableQuantity` is related to a Quantity using the `HasMeasurableQuantity` relation and its reciprocal
relation called `IsOfBaseQuantity`.
Context dependence: for example, Fluid density and Equivalent Circulating Density are represented 
as two different "Measurable quantities", although they both refer to the same base SI quantities. 
Typical sub-types of `MeasurableQuantity` are provided in MeasurableQuantityTypes. These types
can be used in a sort of singleton pattern, i.e., it is not necessary to create an individual to use them
in a relation. Also, if individuals are created with the same characteristics, they are considered as being 
multiple representations of the same `Noun`. The list of `MeasurableQuantity` in MeasurableQuantityTypes is automatically generated
from the `PhysicalQuantities` defined in the Open Source Drilling Community ([OSDC](https://opensourcedrilling.org/)) project called `UnitConversion` 
(see [`OSDC UnitConversion`](https://github.com/Open-Source-Drilling-Community/UnitConversion)). Only the
physical quantities for which a `MeaningfulPrecision` has beed defined are used to generate MeasurableQuantityTypes. 
It is possible to look at all the physical quantities defined in the `OSDC UnitConversion` project by
using the web application hosted here: [`OSDC Physical Quantity Web App`](https://dev.digiwells.no/UnitConversion/webapp/PhysicalQuantity).
"""@EN; 
                         rdfs:subClassOf ddhub:DWISNoun. 
ddhub:MeasurableQuantityUnitAssociation a owl:Class; 
                                        rdfs:comment """This `noun` is typically used to create an association between a `MeasurableQuantity`
and a `Unit` as for example when defining a `UnitSystem`.
"""@EN; 
                                        rdfs:subClassOf ddhub:DWISNoun. 
ddhub:Measured a owl:Class; 
               rdfs:comment """Measured characterizes that the wellbore data has been measured or observed.
"""@EN; 
               rdfs:subClassOf ddhub:WellBoreDataCharateristic. 
ddhub:MeasuredDepth a owl:Class; 
                    rdfs:comment ""@EN; 
                    rdfs:subClassOf ddhub:PrototypeData. 
ddhub:MeasuredDepthToTrueVerticalDepthTransformation a owl:Class; 
                                                     rdfs:comment ""@EN; 
                                                     rdfs:subClassOf ddhub:DirectTransformation. 
ddhub:MeasuredDepthTranslation a owl:Class; 
                               rdfs:comment ""@EN; 
                               rdfs:subClassOf ddhub:DirectTransformation. 
ddhub:Measurement a owl:Class; 
                  rdfs:comment """The noun Measurement represents individuals that are measured by some instrument and which value can be compared with another measurement.
"""@EN; 
                  rdfs:subClassOf ddhub:PhysicalData. 
ddhub:MeasurementDevice a owl:Class; 
                        rdfs:comment """Denotes a physical sensor
"""@EN; 
                        rdfs:subClassOf ddhub:DataFlowNode. 
ddhub:MeasurementIndex a owl:DatatypeProperty, owl:FunctionalProperty; 
                       rdfs:comment """
"""@EN; 
                       rdfs:domain ddhub:EndPointMapping; 
                       rdfs:range xsd:int. 
ddhub:MeasurementWhileDrillingTools a owl:Class; 
                                    rdfs:comment ""@EN; 
                                    rdfs:subClassOf ddhub:LoggingEquipment. 
ddhub:MechanicalBlock a owl:Class; 
                      rdfs:comment ""@EN; 
                      rdfs:subClassOf ddhub:HoistingSystem. 
ddhub:MechanicalDrawworks a owl:Class; 
                          rdfs:comment ""@EN; 
                          rdfs:subClassOf ddhub:Drawworks. 
ddhub:MechanicalElementState a owl:Class; 
                             rdfs:comment ""@EN; 
                             rdfs:subClassOf ddhub:DWISNoun. 
ddhub:MechanicalJar a owl:Class; 
                    rdfs:comment ""@EN; 
                    rdfs:subClassOf ddhub:JarringAssembly. 
ddhub:MechanicalLogicalElement a owl:Class; 
                               rdfs:comment ""@EN; 
                               rdfs:subClassOf ddhub:DWISNoun. 
ddhub:MechanicallyActiveState a owl:Class; 
                              rdfs:comment ""@EN; 
                              rdfs:subClassOf ddhub:MechanicalElementState. 
ddhub:MechanicallyClosedState a owl:Class; 
                              rdfs:comment ""@EN; 
                              rdfs:subClassOf ddhub:MechanicalElementState. 
ddhub:MechanicallyConnectedState a owl:Class; 
                                 rdfs:comment ""@EN; 
                                 rdfs:subClassOf ddhub:MechanicalElementState. 
ddhub:MechanicallyInactiveState a owl:Class; 
                                rdfs:comment ""@EN; 
                                rdfs:subClassOf ddhub:MechanicalElementState. 
ddhub:MechanicallyOpenState a owl:Class; 
                            rdfs:comment ""@EN; 
                            rdfs:subClassOf ddhub:MechanicalElementState. 
ddhub:MechanicalSoftModel a owl:Class; 
                          rdfs:comment """An infinitively soft model assumes that the drill-stem deforms without any resistance when compressive loads are applied.
"""@EN; 
                          rdfs:subClassOf ddhub:MechanicalStiffnessType. 
ddhub:MechanicalSpecificEnergy a owl:Class; 
                               rdfs:comment ""@EN; 
                               rdfs:subClassOf ddhub:PrototypeData. 
ddhub:MechanicalStiffModel a owl:Class; 
                           rdfs:comment """A stiff mechanical model considers that the drill-stem can deform laterally when put in compression.
"""@EN; 
                           rdfs:subClassOf ddhub:MechanicalStiffnessType. 
ddhub:MechanicalStiffModelAssumedContacts a owl:Class; 
                                          rdfs:comment """Such a stiff mechanical model presuposes the position of the contact points.
"""@EN; 
                                          rdfs:subClassOf ddhub:MechanicalStiffModel. 
ddhub:MechanicalStiffModelEstimatedContacts a owl:Class; 
                                            rdfs:comment """Such a stiff mechanical model estimates the position of the contact points.
"""@EN; 
                                            rdfs:subClassOf ddhub:MechanicalStiffModel. 
ddhub:MechanicalStiffnessType a owl:Class; 
                              rdfs:comment """A description of how the drill-stem stiffness is modelled.
"""@EN; 
                              rdfs:subClassOf ddhub:DWISNoun. 
ddhub:MechanicsAndVibrationTools a owl:Class; 
                                 rdfs:comment ""@EN; 
                                 rdfs:subClassOf ddhub:MeasurementWhileDrillingTools. 
ddhub:MechanisticModel a owl:Class; 
                       rdfs:comment """A model that is based on first principles or physical laws.
"""@EN; 
                       rdfs:subClassOf ddhub:ModelingParadigm. 
ddhub:Megaampere a owl:Class; 
                 rdfs:comment """[v] = a * [SI]
where
[v] is the value in megaampere
[SI] is the value in SI
a = 1.0/Mega, i.e., 1E-06
and
Mega = 1e6
"""@EN; 
                 rdfs:subClassOf ddhub:Unit. 
ddhub:MegaBritishThermalUnit a owl:Class; 
                             rdfs:comment """[v] = a * [SI]
where
[v] is the value in mega british thermal unit
[SI] is the value in SI
a = 1.0/(Mega * BTU), i.e., 9.48451652677005E-10
and
Mega = 1e6
BTU = 1054.35 reference: https://en.wikipedia.org/wiki/British_thermal_unit
"""@EN; 
                             rdfs:subClassOf ddhub:Unit. 
ddhub:Megahertz a owl:Class; 
                rdfs:comment """[v] = a * [SI]
where
[v] is the value in megahertz
[SI] is the value in SI
a = 1.0/Mega, i.e., 1E-06
and
Mega = 1e6
"""@EN; 
                rdfs:subClassOf ddhub:Unit. 
ddhub:MegaHertzPerDay a owl:Class; 
                      rdfs:comment """[v] = a * [SI]
where
[v] is the value in mega hertz per day
[SI] is the value in SI
a = Day/Mega, i.e., 0.0864
and
Day = 24.0 * Hour
Mega = 1e6
Hour = 60.0 * Minute
Minute = 60.0
"""@EN; 
                      rdfs:subClassOf ddhub:Unit. 
ddhub:MegaHertzPerHour a owl:Class; 
                       rdfs:comment """[v] = a * [SI]
where
[v] is the value in mega hertz per hour
[SI] is the value in SI
a = Hour/Mega, i.e., 0.0036
and
Hour = 60.0 * Minute
Mega = 1e6
Minute = 60.0
"""@EN; 
                       rdfs:subClassOf ddhub:Unit. 
ddhub:MegaHertzPerMinute a owl:Class; 
                         rdfs:comment """[v] = a * [SI]
where
[v] is the value in mega hertz per minute
[SI] is the value in SI
a = Minute/Mega, i.e., 6E-05
and
Minute = 60.0
Mega = 1e6
"""@EN; 
                         rdfs:subClassOf ddhub:Unit. 
ddhub:MegaHertzPerSecond a owl:Class; 
                         rdfs:comment """[v] = a * [SI]
where
[v] is the value in mega hertz per second
[SI] is the value in SI
a = 1.0/Mega, i.e., 1E-06
and
Mega = 1e6
"""@EN; 
                         rdfs:subClassOf ddhub:Unit. 
ddhub:MegaHertzPerYear a owl:Class; 
                       rdfs:comment """[v] = a * [SI]
where
[v] is the value in mega hertz per year
[SI] is the value in SI
a = YearJulian/Mega, i.e., 31.5576
and
YearJulian = 365.25 * Day
Mega = 1e6
Day = 24.0 * Hour
Hour = 60.0 * Minute
Minute = 60.0
"""@EN; 
                       rdfs:subClassOf ddhub:Unit. 
ddhub:Megajoule a owl:Class; 
                rdfs:comment """[v] = a * [SI]
where
[v] is the value in megajoule
[SI] is the value in SI
a = 1.0/Mega, i.e., 1E-06
and
Mega = 1e6
"""@EN; 
                rdfs:subClassOf ddhub:Unit. 
ddhub:MegajoulePerCubicFoot a owl:Class; 
                            rdfs:comment """[v] = a * [SI]
where
[v] is the value in megajoule per cubic foot
[SI] is the value in SI
a = Foot * Foot * Foot / Mega, i.e., 2.831684659199999E-08
and
Foot = 12.0 * Inch
Mega = 1e6
Inch = 0.0254 reference: https://www.nist.gov/pml/owm/si-units-length
"""@EN; 
                            rdfs:subClassOf ddhub:Unit. 
ddhub:MegajoulePerCubicInch a owl:Class; 
                            rdfs:comment """[v] = a * [SI]
where
[v] is the value in megajoule per cubic inch
[SI] is the value in SI
a = Inch*Inch*Inch/Mega, i.e., 1.6387064E-11
and
Inch = 0.0254 reference: https://www.nist.gov/pml/owm/si-units-length
Mega = 1e6
"""@EN; 
                            rdfs:subClassOf ddhub:Unit. 
ddhub:MegajoulePerCubicMetre a owl:Class; 
                             rdfs:comment """[v] = a * [SI]
where
[v] is the value in megajoule per cubic metre
[SI] is the value in SI
a = 1.0/Mega, i.e., 1E-06
and
Mega = 1e6
"""@EN; 
                             rdfs:subClassOf ddhub:Unit. 
ddhub:MegajoulePerGallonUk a owl:Class; 
                           rdfs:comment """[v] = a * [SI]
where
[v] is the value in megajoule per gallon (UK)
[SI] is the value in SI
a = GallonUK / Mega, i.e., 4.54609E-09
and
GallonUK = 4.54609e-3 reference: https://en.wikipedia.org/wiki/Gallon
Mega = 1e6
"""@EN; 
                           rdfs:subClassOf ddhub:Unit. 
ddhub:MegajoulePerGallonUs a owl:Class; 
                           rdfs:comment """[v] = a * [SI]
where
[v] is the value in megajoule per gallon (US)
[SI] is the value in SI
a = GallonUS / Mega, i.e., 3.7854117839999995E-09
and
GallonUS = 231.0 * Inch * Inch * Inch reference: https://en.wikipedia.org/wiki/Gallon
Mega = 1e6
Inch = 0.0254 reference: https://www.nist.gov/pml/owm/si-units-length
"""@EN; 
                           rdfs:subClassOf ddhub:Unit. 
ddhub:MegajoulePerLitre a owl:Class; 
                        rdfs:comment """[v] = a * [SI]
where
[v] is the value in megajoule per litre
[SI] is the value in SI
a = Litre/Mega, i.e., 1E-09
and
Litre = 0.001
Mega = 1e6
"""@EN; 
                        rdfs:subClassOf ddhub:Unit. 
ddhub:Megaline a owl:Class; 
               rdfs:comment """[v] = a * [SI]
where
[v] is the value in megaline
[SI] is the value in SI
a = 1.0/(Mega*Line), i.e., 100
and
Mega = 1e6
Line = 1e-8 reference: https://en.wikipedia.org/wiki/Maxwell_(unit)
"""@EN; 
               rdfs:subClassOf ddhub:Unit. 
ddhub:MegaOhmMetre a owl:Class; 
                   rdfs:comment """[v] = a * [SI]
where
[v] is the value in mega ohm metre
[SI] is the value in SI
a = 1.0/Mega, i.e., 1E-06
and
Mega = 1e6
"""@EN; 
                   rdfs:subClassOf ddhub:Unit. 
ddhub:Megapascal a owl:Class; 
                 rdfs:comment """[v] = a * [SI]
where
[v] is the value in megapascal
[SI] is the value in SI
a = 1.0/Mega, i.e., 1E-06
and
Mega = 1e6
"""@EN; 
                 rdfs:subClassOf ddhub:Unit. 
ddhub:MegapascalPerHour a owl:Class; 
                        rdfs:comment """[v] = a * [SI]
where
[v] is the value in megapascal per hour
[SI] is the value in SI
a = Hour/Mega, i.e., 0.0036
and
Hour = 60.0 * Minute
Mega = 1e6
Minute = 60.0
"""@EN; 
                        rdfs:subClassOf ddhub:Unit. 
ddhub:MegapascalPerMinute a owl:Class; 
                          rdfs:comment """[v] = a * [SI]
where
[v] is the value in megapascal per minute
[SI] is the value in SI
a = Minute/Mega, i.e., 6E-05
and
Minute = 60.0
Mega = 1e6
"""@EN; 
                          rdfs:subClassOf ddhub:Unit. 
ddhub:MegapascalPerSecond a owl:Class; 
                          rdfs:comment """[v] = a * [SI]
where
[v] is the value in megapascal per second
[SI] is the value in SI
a = 1.0/Mega, i.e., 1E-06
and
Mega = 1e6
"""@EN; 
                          rdfs:subClassOf ddhub:Unit. 
ddhub:MegapoundPerSquareInch a owl:Class; 
                             rdfs:comment """[v] = a * [SI]
where
[v] is the value in megapound per square inch
[SI] is the value in SI
a = 1.0/(Mega*PSI), i.e., 1.4503773773020922E-10
and
Mega = 1e6
PSI = PoundForce / (Inch * Inch) reference: https://en.wikipedia.org/wiki/Pound_per_square_inch
PoundForce = Pound * G reference: https://en.wikipedia.org/wiki/Pound_(force)
Inch = 0.0254 reference: https://www.nist.gov/pml/owm/si-units-length
Pound = 0.45359237 reference: https://en.wikipedia.org/wiki/Pound_(mass)
G = 9.80665 reference: https://en.wikipedia.org/wiki/Gravity_of_Earth
"""@EN; 
                             rdfs:subClassOf ddhub:Unit. 
ddhub:MegapoundPerSquareInchPerHour a owl:Class; 
                                    rdfs:comment """[v] = a * [SI]
where
[v] is the value in megapound per square inch per hour
[SI] is the value in SI
a = Hour*Inch*Inch/(Mega*PoundForce), i.e., 5.221358558287532E-07
and
Hour = 60.0 * Minute
Inch = 0.0254 reference: https://www.nist.gov/pml/owm/si-units-length
Mega = 1e6
PoundForce = Pound * G reference: https://en.wikipedia.org/wiki/Pound_(force)
Minute = 60.0
Pound = 0.45359237 reference: https://en.wikipedia.org/wiki/Pound_(mass)
G = 9.80665 reference: https://en.wikipedia.org/wiki/Gravity_of_Earth
"""@EN; 
                                    rdfs:subClassOf ddhub:Unit. 
ddhub:MegapoundPerSquareInchPerMinute a owl:Class; 
                                      rdfs:comment """[v] = a * [SI]
where
[v] is the value in megapound per square inch per minute
[SI] is the value in SI
a = Minute*Inch*Inch/(Mega*PoundForce), i.e., 8.702264263812553E-09
and
Minute = 60.0
Inch = 0.0254 reference: https://www.nist.gov/pml/owm/si-units-length
Mega = 1e6
PoundForce = Pound * G reference: https://en.wikipedia.org/wiki/Pound_(force)
Pound = 0.45359237 reference: https://en.wikipedia.org/wiki/Pound_(mass)
G = 9.80665 reference: https://en.wikipedia.org/wiki/Gravity_of_Earth
"""@EN; 
                                      rdfs:subClassOf ddhub:Unit. 
ddhub:MegapoundPerSquareInchPerSecond a owl:Class; 
                                      rdfs:comment """[v] = a * [SI]
where
[v] is the value in megapound per square inch per second
[SI] is the value in SI
a = Inch*Inch/(Mega*PoundForce), i.e., 1.4503773773020922E-10
and
Inch = 0.0254 reference: https://www.nist.gov/pml/owm/si-units-length
Mega = 1e6
PoundForce = Pound * G reference: https://en.wikipedia.org/wiki/Pound_(force)
Pound = 0.45359237 reference: https://en.wikipedia.org/wiki/Pound_(mass)
G = 9.80665 reference: https://en.wikipedia.org/wiki/Gravity_of_Earth
"""@EN; 
                                      rdfs:subClassOf ddhub:Unit. 
ddhub:Megatonne a owl:Class; 
                rdfs:comment """[v] = a * [SI]
where
[v] is the value in megatonne
[SI] is the value in SI
a = 1.0/Giga, i.e., 1E-09
and
Giga = 1e9
"""@EN; 
                rdfs:subClassOf ddhub:Unit. 
ddhub:Megavolt a owl:Class; 
               rdfs:comment """[v] = a * [SI]
where
[v] is the value in megavolt
[SI] is the value in SI
a = 1.0/Mega, i.e., 1E-06
and
Mega = 1e6
"""@EN; 
               rdfs:subClassOf ddhub:Unit. 
ddhub:Megawatt a owl:Class; 
               rdfs:comment """[v] = a * [SI]
where
[v] is the value in megawatt
[SI] is the value in SI
a = 1.0/Mega, i.e., 1E-06
and
Mega = 1e6
"""@EN; 
               rdfs:subClassOf ddhub:Unit. 
ddhub:Melon a owl:Class; 
            rdfs:comment ""@EN; 
            rdfs:subClassOf ddhub:BladeShape. 
ddhub:Metre a owl:Class; 
            rdfs:comment """No conversion necessary as the unit choice is SI
"""@EN; 
            rdfs:subClassOf ddhub:Unit. 
ddhub:MetrePerDay a owl:Class; 
                  rdfs:comment """[v] = a * [SI]
where
[v] is the value in metre per day
[SI] is the value in SI
a = Day/Unit, i.e., 86400
and
Day = 24.0 * Hour
Unit = 1.0
Hour = 60.0 * Minute
Minute = 60.0
"""@EN; 
                  rdfs:subClassOf ddhub:Unit. 
ddhub:MetrePerHour a owl:Class; 
                   rdfs:comment """[v] = a * [SI]
where
[v] is the value in metre per hour
[SI] is the value in SI
a = Hour/Unit, i.e., 3600
and
Hour = 60.0 * Minute
Unit = 1.0
Minute = 60.0
"""@EN; 
                   rdfs:subClassOf ddhub:Unit. 
ddhub:MetrePerKilometre a owl:Class; 
                        rdfs:comment """[v] = a * [SI]
where
[v] is the value in metre per kilometre
[SI] is the value in SI
a = Kilo/Unit, i.e., 1000
and
Kilo = 1000.0
Unit = 1.0
"""@EN; 
                        rdfs:subClassOf ddhub:Unit. 
ddhub:MetrePerMetre a owl:Class; 
                    rdfs:comment """No conversion necessary as the unit choice is SI
"""@EN; 
                    rdfs:subClassOf ddhub:Unit. 
ddhub:MetrePerMinute a owl:Class; 
                     rdfs:comment """[v] = a * [SI]
where
[v] is the value in metre per minute
[SI] is the value in SI
a = Minute/Unit, i.e., 60
and
Minute = 60.0
Unit = 1.0
"""@EN; 
                     rdfs:subClassOf ddhub:Unit. 
ddhub:MetrePerSecond a owl:Class; 
                     rdfs:comment """No conversion necessary as the unit choice is SI
"""@EN; 
                     rdfs:subClassOf ddhub:Unit. 
ddhub:MetrePerSecondPerMillisecond a owl:Class; 
                                   rdfs:comment """[v] = a * [SI]
where
[v] is the value in metre per second per millisecond
[SI] is the value in SI
a = Milli /Unit, i.e., 0.001
and
Milli = 0.001
Unit = 1.0
"""@EN; 
                                   rdfs:subClassOf ddhub:Unit. 
ddhub:MetrePerSecondSquared a owl:Class; 
                            rdfs:comment """No conversion necessary as the unit choice is SI
"""@EN; 
                            rdfs:subClassOf ddhub:Unit. 
ddhub:Microampere a owl:Class; 
                  rdfs:comment """[v] = a * [SI]
where
[v] is the value in microampere
[SI] is the value in SI
a = 1.0/Micro, i.e., 1000000
and
Micro = 1e-6
"""@EN; 
                  rdfs:subClassOf ddhub:Unit. 
ddhub:Microbar a owl:Class; 
               rdfs:comment """[v] = a * [SI]
where
[v] is the value in microbar
[SI] is the value in SI
a = 1.0/(Micro*Bar), i.e., 10
and
Micro = 1e-6
Bar = 1e5 reference: https://en.wikipedia.org/wiki/Bar_(unit)
"""@EN; 
               rdfs:subClassOf ddhub:Unit. 
ddhub:MicrobarPerHour a owl:Class; 
                      rdfs:comment """[v] = a * [SI]
where
[v] is the value in microbar per hour
[SI] is the value in SI
a = Hour/(Micro*Bar), i.e., 36000
and
Hour = 60.0 * Minute
Micro = 1e-6
Bar = 1e5 reference: https://en.wikipedia.org/wiki/Bar_(unit)
Minute = 60.0
"""@EN; 
                      rdfs:subClassOf ddhub:Unit. 
ddhub:MicrobarPerMinute a owl:Class; 
                        rdfs:comment """[v] = a * [SI]
where
[v] is the value in microbar per minute
[SI] is the value in SI
a = Minute/(Micro*Bar), i.e., 600
and
Minute = 60.0
Micro = 1e-6
Bar = 1e5 reference: https://en.wikipedia.org/wiki/Bar_(unit)
"""@EN; 
                        rdfs:subClassOf ddhub:Unit. 
ddhub:MicrobarPerSecond a owl:Class; 
                        rdfs:comment """[v] = a * [SI]
where
[v] is the value in microbar per second
[SI] is the value in SI
a = 1.0/(Micro*Bar), i.e., 10
and
Micro = 1e-6
Bar = 1e5 reference: https://en.wikipedia.org/wiki/Bar_(unit)
"""@EN; 
                        rdfs:subClassOf ddhub:Unit. 
ddhub:Microdarcy a owl:Class; 
                 rdfs:comment """[v] = a * [SI]
where
[v] is the value in microdarcy
[SI] is the value in SI
a = 1.0/(Micro*Darcy), i.e., 1.01325E+18
and
Micro = 1e-6
Darcy = 0.0000001 / Atmosphere reference: https://en.wikipedia.org/wiki/Darcy_(unit)
Atmosphere = 101325.0 reference: https://en.wikipedia.org/wiki/Atmospheric_pressure
"""@EN; 
                 rdfs:subClassOf ddhub:Unit. 
ddhub:Microfarad a owl:Class; 
                 rdfs:comment """[v] = a * [SI]
where
[v] is the value in microfarad
[SI] is the value in SI
a = 1.0/Micro, i.e., 1000000
and
Micro = 1e-6
"""@EN; 
                 rdfs:subClassOf ddhub:Unit. 
ddhub:Microgram a owl:Class; 
                rdfs:comment """[v] = a * [SI]
where
[v] is the value in microgram
[SI] is the value in SI
a = 1.0/Nano, i.e., 999999999.9999999
and
Nano = 1e-9
"""@EN; 
                rdfs:subClassOf ddhub:Unit. 
ddhub:Micrometre a owl:Class; 
                 rdfs:comment """[v] = a * [SI]
where
[v] is the value in micrometre
[SI] is the value in SI
a = 1.0/Micro, i.e., 1000000
and
Micro = 1e-6
"""@EN; 
                 rdfs:subClassOf ddhub:Unit. 
ddhub:MicrometrePerKilometre a owl:Class; 
                             rdfs:comment """[v] = a * [SI]
where
[v] is the value in micrometre per kilometre
[SI] is the value in SI
a = Kilo / Micro, i.e., 1000000000
and
Kilo = 1000.0
Micro = 1e-6
"""@EN; 
                             rdfs:subClassOf ddhub:Unit. 
ddhub:MicrometrePerMetre a owl:Class; 
                         rdfs:comment """[v] = a * [SI]
where
[v] is the value in micrometre per metre
[SI] is the value in SI
a = 1.0 / Micro, i.e., 1000000
and
Micro = 1e-6
"""@EN; 
                         rdfs:subClassOf ddhub:Unit. 
ddhub:Micromole a owl:Class; 
                rdfs:comment """[v] = a * [SI]
where
[v] is the value in micromole
[SI] is the value in SI
a = 1.0/Micro, i.e., 1000000
and
Micro = 1e-6
"""@EN; 
                rdfs:subClassOf ddhub:Unit. 
ddhub:MicropascalSecond a owl:Class; 
                        rdfs:comment """[v] = a * [SI]
where
[v] is the value in micropascal second
[SI] is the value in SI
a = 1.0/Micro, i.e., 1000000
and
Micro = 1e-6
"""@EN; 
                        rdfs:subClassOf ddhub:Unit. 
ddhub:Micropoise a owl:Class; 
                 rdfs:comment """[v] = a * [SI]
where
[v] is the value in micropoise
[SI] is the value in SI
a = 1.0/(Micro* Poise), i.e., 10000000
and
Micro = 1e-6
Poise = 0.1 reference: https://en.wikipedia.org/wiki/Poise_(unit)
"""@EN; 
                 rdfs:subClassOf ddhub:Unit. 
ddhub:Microsecond a owl:Class; 
                  rdfs:comment """[v] = a * [SI]
where
[v] is the value in microsecond
[SI] is the value in SI
a = 1.0/Micro, i.e., 1000000
and
Micro = 1e-6
"""@EN; 
                  rdfs:subClassOf ddhub:Unit. 
ddhub:Microtesla a owl:Class; 
                 rdfs:comment """[v] = a * [SI]
where
[v] is the value in microtesla
[SI] is the value in SI
a = 1.0/Micro, i.e., 1000000
and
Micro = 1e-6
"""@EN; 
                 rdfs:subClassOf ddhub:Unit. 
ddhub:Microvolt a owl:Class; 
                rdfs:comment """[v] = a * [SI]
where
[v] is the value in microvolt
[SI] is the value in SI
a = 1.0/Micro, i.e., 1000000
and
Micro = 1e-6
"""@EN; 
                rdfs:subClassOf ddhub:Unit. 
ddhub:Microwatt a owl:Class; 
                rdfs:comment """[v] = a * [SI]
where
[v] is the value in microwatt
[SI] is the value in SI
a = 1.0/Micro, i.e., 1000000
and
Micro = 1e-6
"""@EN; 
                rdfs:subClassOf ddhub:Unit. 
ddhub:Microweber a owl:Class; 
                 rdfs:comment """[v] = a * [SI]
where
[v] is the value in microweber
[SI] is the value in SI
a = 1.0/Micro, i.e., 1000000
and
Micro = 1e-6
"""@EN; 
                 rdfs:subClassOf ddhub:Unit. 
ddhub:Mil a owl:Class; 
          rdfs:comment """[v] = a * [SI]
where
[v] is the value in mil
[SI] is the value in SI
a = 1.0/Mil, i.e., 39370.07874015748
and
Mil = 0.001 * Inch reference: https://en.wikipedia.org/wiki/Thousandth_of_an_inch
Inch = 0.0254 reference: https://www.nist.gov/pml/owm/si-units-length
"""@EN; 
          rdfs:subClassOf ddhub:Unit. 
ddhub:Mile a owl:Class; 
           rdfs:comment """[v] = a * [SI]
where
[v] is the value in mile
[SI] is the value in SI
a = 1.0/Mile, i.e., 0.000621371192237334
and
Mile = 1760.0 * Yard reference: https://dictionary.cambridge.org/dictionary/english/mile
Yard = 3.0 * Foot
Foot = 12.0 * Inch
Inch = 0.0254 reference: https://www.nist.gov/pml/owm/si-units-length
"""@EN; 
           rdfs:subClassOf ddhub:Unit. 
ddhub:MilePerDay a owl:Class; 
                 rdfs:comment """[v] = a * [SI]
where
[v] is the value in mile per day
[SI] is the value in SI
a = Day/Mile, i.e., 53.68647100930566
and
Day = 24.0 * Hour
Mile = 1760.0 * Yard reference: https://dictionary.cambridge.org/dictionary/english/mile
Hour = 60.0 * Minute
Yard = 3.0 * Foot
Minute = 60.0
Foot = 12.0 * Inch
Inch = 0.0254 reference: https://www.nist.gov/pml/owm/si-units-length
"""@EN; 
                 rdfs:subClassOf ddhub:Unit. 
ddhub:MilePerHour a owl:Class; 
                  rdfs:comment """[v] = a * [SI]
where
[v] is the value in mile per hour
[SI] is the value in SI
a = Hour/Mile, i.e., 2.2369362920544025
and
Hour = 60.0 * Minute
Mile = 1760.0 * Yard reference: https://dictionary.cambridge.org/dictionary/english/mile
Minute = 60.0
Yard = 3.0 * Foot
Foot = 12.0 * Inch
Inch = 0.0254 reference: https://www.nist.gov/pml/owm/si-units-length
"""@EN; 
                  rdfs:subClassOf ddhub:Unit. 
ddhub:MilePerHourPerSecond a owl:Class; 
                           rdfs:comment """[v] = a * [SI]
where
[v] is the value in mile per hour per second
[SI] is the value in SI
a = Hour / Mile, i.e., 2.2369362920544025
and
Hour = 60.0 * Minute
Mile = 1760.0 * Yard reference: https://dictionary.cambridge.org/dictionary/english/mile
Minute = 60.0
Yard = 3.0 * Foot
Foot = 12.0 * Inch
Inch = 0.0254 reference: https://www.nist.gov/pml/owm/si-units-length
"""@EN; 
                           rdfs:subClassOf ddhub:Unit. 
ddhub:MilePerMinute a owl:Class; 
                    rdfs:comment """[v] = a * [SI]
where
[v] is the value in mile per minute
[SI] is the value in SI
a = Minute/Mile, i.e., 0.03728227153424004
and
Minute = 60.0
Mile = 1760.0 * Yard reference: https://dictionary.cambridge.org/dictionary/english/mile
Yard = 3.0 * Foot
Foot = 12.0 * Inch
Inch = 0.0254 reference: https://www.nist.gov/pml/owm/si-units-length
"""@EN; 
                    rdfs:subClassOf ddhub:Unit. 
ddhub:MilePerMinutePerSecond a owl:Class; 
                             rdfs:comment """[v] = a * [SI]
where
[v] is the value in mile per minute per second
[SI] is the value in SI
a = Minute /Mile, i.e., 0.03728227153424004
and
Minute = 60.0
Mile = 1760.0 * Yard reference: https://dictionary.cambridge.org/dictionary/english/mile
Yard = 3.0 * Foot
Foot = 12.0 * Inch
Inch = 0.0254 reference: https://www.nist.gov/pml/owm/si-units-length
"""@EN; 
                             rdfs:subClassOf ddhub:Unit. 
ddhub:MilePerSecond a owl:Class; 
                    rdfs:comment """[v] = a * [SI]
where
[v] is the value in mile per second
[SI] is the value in SI
a = Unit/Mile, i.e., 0.000621371192237334
and
Unit = 1.0
Mile = 1760.0 * Yard reference: https://dictionary.cambridge.org/dictionary/english/mile
Yard = 3.0 * Foot
Foot = 12.0 * Inch
Inch = 0.0254 reference: https://www.nist.gov/pml/owm/si-units-length
"""@EN; 
                    rdfs:subClassOf ddhub:Unit. 
ddhub:MilePerSecondSquared a owl:Class; 
                           rdfs:comment """[v] = a * [SI]
where
[v] is the value in mile per second squared
[SI] is the value in SI
a = 1.0/Mile, i.e., 0.000621371192237334
and
Mile = 1760.0 * Yard reference: https://dictionary.cambridge.org/dictionary/english/mile
Yard = 3.0 * Foot
Foot = 12.0 * Inch
Inch = 0.0254 reference: https://www.nist.gov/pml/owm/si-units-length
"""@EN; 
                           rdfs:subClassOf ddhub:Unit. 
ddhub:MillCasingCutting a owl:Class; 
                        rdfs:comment ""@EN; 
                        rdfs:subClassOf ddhub:CasingMillingTools. 
ddhub:MillDress a owl:Class; 
                rdfs:comment ""@EN; 
                rdfs:subClassOf ddhub:CasingMillingTools. 
ddhub:Millenia a owl:Class; 
               rdfs:comment """[v] = a * [SI]
where
[v] is the value in millenia
[SI] is the value in SI
a = 1.0/Millenia, i.e., 3.168808781402895E-11
and
Millenia = 10.0 * Century
Century = 10.0 * Decade
Decade = 10.0 * YearJulian
YearJulian = 365.25 * Day
Day = 24.0 * Hour
Hour = 60.0 * Minute
Minute = 60.0
"""@EN; 
               rdfs:subClassOf ddhub:Unit. 
ddhub:MillFlatBottom a owl:Class; 
                     rdfs:comment ""@EN; 
                     rdfs:subClassOf ddhub:CasingMillingTools. 
ddhub:MillHollow a owl:Class; 
                 rdfs:comment ""@EN; 
                 rdfs:subClassOf ddhub:CasingMillingTools. 
ddhub:Milliampere a owl:Class; 
                  rdfs:comment """[v] = a * [SI]
where
[v] is the value in milliampere
[SI] is the value in SI
a = 1.0/Milli, i.e., 1000
and
Milli = 0.001
"""@EN; 
                  rdfs:subClassOf ddhub:Unit. 
ddhub:Millibar a owl:Class; 
               rdfs:comment """[v] = a * [SI]
where
[v] is the value in millibar
[SI] is the value in SI
a = 1.0/(Milli*Bar), i.e., 0.01
and
Milli = 0.001
Bar = 1e5 reference: https://en.wikipedia.org/wiki/Bar_(unit)
"""@EN; 
               rdfs:subClassOf ddhub:Unit. 
ddhub:MillibarPerHour a owl:Class; 
                      rdfs:comment """[v] = a * [SI]
where
[v] is the value in millibar per hour
[SI] is the value in SI
a = Hour/(Milli*Bar), i.e., 36
and
Hour = 60.0 * Minute
Milli = 0.001
Bar = 1e5 reference: https://en.wikipedia.org/wiki/Bar_(unit)
Minute = 60.0
"""@EN; 
                      rdfs:subClassOf ddhub:Unit. 
ddhub:MillibarPerMinute a owl:Class; 
                        rdfs:comment """[v] = a * [SI]
where
[v] is the value in millibar per minute
[SI] is the value in SI
a = Minute/(Milli*Bar), i.e., 0.6
and
Minute = 60.0
Milli = 0.001
Bar = 1e5 reference: https://en.wikipedia.org/wiki/Bar_(unit)
"""@EN; 
                        rdfs:subClassOf ddhub:Unit. 
ddhub:MillibarPerSecond a owl:Class; 
                        rdfs:comment """[v] = a * [SI]
where
[v] is the value in millibar per second
[SI] is the value in SI
a = 1.0/(Milli*Bar), i.e., 0.01
and
Milli = 0.001
Bar = 1e5 reference: https://en.wikipedia.org/wiki/Bar_(unit)
"""@EN; 
                        rdfs:subClassOf ddhub:Unit. 
ddhub:Millicandela a owl:Class; 
                   rdfs:comment """[v] = a * [SI]
where
[v] is the value in millicandela
[SI] is the value in SI
a = 1.0/Milli, i.e., 1000
and
Milli = 0.001
"""@EN; 
                   rdfs:subClassOf ddhub:Unit. 
ddhub:Millidarcy a owl:Class; 
                 rdfs:comment """[v] = a * [SI]
where
[v] is the value in millidarcy
[SI] is the value in SI
a = 1.0/(Milli*Darcy), i.e., 1013250000000000.1
and
Milli = 0.001
Darcy = 0.0000001 / Atmosphere reference: https://en.wikipedia.org/wiki/Darcy_(unit)
Atmosphere = 101325.0 reference: https://en.wikipedia.org/wiki/Atmospheric_pressure
"""@EN; 
                 rdfs:subClassOf ddhub:Unit. 
ddhub:Millifarad a owl:Class; 
                 rdfs:comment """[v] = a * [SI]
where
[v] is the value in millifarad
[SI] is the value in SI
a = 1.0/Milli, i.e., 1000
and
Milli = 0.001
"""@EN; 
                 rdfs:subClassOf ddhub:Unit. 
ddhub:Milligauss a owl:Class; 
                 rdfs:comment """[v] = a * [SI]
where
[v] is the value in milligauss
[SI] is the value in SI
a = 1.0/(Milli*Gauss), i.e., 10000000
and
Milli = 0.001
Gauss = 1e-4 reference: https://en.wikipedia.org/wiki/Gauss_(unit)
"""@EN; 
                 rdfs:subClassOf ddhub:Unit. 
ddhub:Milligram a owl:Class; 
                rdfs:comment """[v] = a * [SI]
where
[v] is the value in milligram
[SI] is the value in SI
a = 1.0/Micro, i.e., 1000000
and
Micro = 1e-6
"""@EN; 
                rdfs:subClassOf ddhub:Unit. 
ddhub:Millilitre a owl:Class; 
                 rdfs:comment """[v] = a * [SI]
where
[v] is the value in millilitre
[SI] is the value in SI
a = 1.0/(Milli*Milli), i.e., 1000000
and
Milli = 0.001
"""@EN; 
                 rdfs:subClassOf ddhub:Unit. 
ddhub:Millimetre a owl:Class; 
                 rdfs:comment """[v] = a * [SI]
where
[v] is the value in millimetre
[SI] is the value in SI
a = 1.0/Milli, i.e., 1000
and
Milli = 0.001
"""@EN; 
                 rdfs:subClassOf ddhub:Unit. 
ddhub:MillimetreMercuryAtZeroDegreeCelsius a owl:Class; 
                                           rdfs:comment """[v] = a * [SI]
where
[v] is the value in millimetre mercury at zero degree celsius
[SI] is the value in SI
a = 1.0/MillimetreMercury, i.e., 0.007500615758456563
and
MillimetreMercury = 133.322387415 reference: https://en.wikipedia.org/wiki/Millimetre_of_mercury
"""@EN; 
                                           rdfs:subClassOf ddhub:Unit. 
ddhub:MillimetreMercuryAtZeroDegreeCelsiusPerHour a owl:Class; 
                                                  rdfs:comment """[v] = a * [SI]
where
[v] is the value in millimetre mercury at zero degree celsius per hour
[SI] is the value in SI
a = Hour/MillimetreMercury, i.e., 27.002216730443628
and
Hour = 60.0 * Minute
MillimetreMercury = 133.322387415 reference: https://en.wikipedia.org/wiki/Millimetre_of_mercury
Minute = 60.0
"""@EN; 
                                                  rdfs:subClassOf ddhub:Unit. 
ddhub:MillimetreMercuryAtZeroDegreeCelsiusPerMinute a owl:Class; 
                                                    rdfs:comment """[v] = a * [SI]
where
[v] is the value in millimetre mercury at zero degree celsius per minute
[SI] is the value in SI
a = Minute/MillimetreMercury, i.e., 0.45003694550739376
and
Minute = 60.0
MillimetreMercury = 133.322387415 reference: https://en.wikipedia.org/wiki/Millimetre_of_mercury
"""@EN; 
                                                    rdfs:subClassOf ddhub:Unit. 
ddhub:MillimetreMercuryAtZeroDegreeCelsiusPerSecond a owl:Class; 
                                                    rdfs:comment """[v] = a * [SI]
where
[v] is the value in millimetre mercury at zero degree celsius per second
[SI] is the value in SI
a = 1.0/MillimetreMercury, i.e., 0.007500615758456563
and
MillimetreMercury = 133.322387415 reference: https://en.wikipedia.org/wiki/Millimetre_of_mercury
"""@EN; 
                                                    rdfs:subClassOf ddhub:Unit. 
ddhub:MillimetrePerDay a owl:Class; 
                       rdfs:comment """[v] = a * [SI]
where
[v] is the value in millimetre per day
[SI] is the value in SI
a = Day/Milli, i.e., 86400000
and
Day = 24.0 * Hour
Milli = 0.001
Hour = 60.0 * Minute
Minute = 60.0
"""@EN; 
                       rdfs:subClassOf ddhub:Unit. 
ddhub:MillimetrePerHour a owl:Class; 
                        rdfs:comment """[v] = a * [SI]
where
[v] is the value in millimetre per hour
[SI] is the value in SI
a = Hour/Milli, i.e., 3600000
and
Hour = 60.0 * Minute
Milli = 0.001
Minute = 60.0
"""@EN; 
                        rdfs:subClassOf ddhub:Unit. 
ddhub:MillimetrePerKilometre a owl:Class; 
                             rdfs:comment """[v] = a * [SI]
where
[v] is the value in millimetre per kilometre
[SI] is the value in SI
a = Kilo / Milli, i.e., 1000000
and
Kilo = 1000.0
Milli = 0.001
"""@EN; 
                             rdfs:subClassOf ddhub:Unit. 
ddhub:MillimetrePerMetre a owl:Class; 
                         rdfs:comment """[v] = a * [SI]
where
[v] is the value in millimetre per metre
[SI] is the value in SI
a = 1.0/Milli, i.e., 1000
and
Milli = 0.001
"""@EN; 
                         rdfs:subClassOf ddhub:Unit. 
ddhub:MillimetrePerMinute a owl:Class; 
                          rdfs:comment """[v] = a * [SI]
where
[v] is the value in millimetre per minute
[SI] is the value in SI
a = Minute/Milli, i.e., 60000
and
Minute = 60.0
Milli = 0.001
"""@EN; 
                          rdfs:subClassOf ddhub:Unit. 
ddhub:MillimetrePerSecond a owl:Class; 
                          rdfs:comment """[v] = a * [SI]
where
[v] is the value in millimetre per second
[SI] is the value in SI
a = Unit/Milli, i.e., 1000
and
Unit = 1.0
Milli = 0.001
"""@EN; 
                          rdfs:subClassOf ddhub:Unit. 
ddhub:MillimetreWaterAt4DegreeCelsius a owl:Class; 
                                      rdfs:comment """[v] = a * [SI]
where
[v] is the value in millimetre water at 4 degree celsius
[SI] is the value in SI
a = 1.0/MillimetreWater4degC, i.e., 0.10104429276573387
and
MillimetreWater4degC = 9.89665 reference: https://en.wikipedia.org/wiki/Centimetre_or_millimetre_of_water
"""@EN; 
                                      rdfs:subClassOf ddhub:Unit. 
ddhub:MillimetreWaterAt4DegreeCelsiusPerHour a owl:Class; 
                                             rdfs:comment """[v] = a * [SI]
where
[v] is the value in millimetre water at 4 degree celsius per hour
[SI] is the value in SI
a = Hour/MillimetreWater4degC, i.e., 363.75945395664195
and
Hour = 60.0 * Minute
MillimetreWater4degC = 9.89665 reference: https://en.wikipedia.org/wiki/Centimetre_or_millimetre_of_water
Minute = 60.0
"""@EN; 
                                             rdfs:subClassOf ddhub:Unit. 
ddhub:MillimetreWaterAt4DegreeCelsiusPerMinute a owl:Class; 
                                               rdfs:comment """[v] = a * [SI]
where
[v] is the value in millimetre water at 4 degree celsius per minute
[SI] is the value in SI
a = Minute/MillimetreWater4degC, i.e., 6.062657565944032
and
Minute = 60.0
MillimetreWater4degC = 9.89665 reference: https://en.wikipedia.org/wiki/Centimetre_or_millimetre_of_water
"""@EN; 
                                               rdfs:subClassOf ddhub:Unit. 
ddhub:MillimetreWaterAt4DegreeCelsiusPerSecond a owl:Class; 
                                               rdfs:comment """[v] = a * [SI]
where
[v] is the value in millimetre water at 4 degree celsius per second
[SI] is the value in SI
a = 1.0/MillimetreWater4degC, i.e., 0.10104429276573387
and
MillimetreWater4degC = 9.89665 reference: https://en.wikipedia.org/wiki/Centimetre_or_millimetre_of_water
"""@EN; 
                                               rdfs:subClassOf ddhub:Unit. 
ddhub:Millimole a owl:Class; 
                rdfs:comment """[v] = a * [SI]
where
[v] is the value in millimole
[SI] is the value in SI
a = 1.0/Milli, i.e., 1000
and
Milli = 0.001
"""@EN; 
                rdfs:subClassOf ddhub:Unit. 
ddhub:MillinewtonPerMetre a owl:Class; 
                          rdfs:comment """[v] = a * [SI]
where
[v] is the value in millinewton per metre
[SI] is the value in SI
a = 1.0/Milli, i.e., 1000
and
Milli = 0.001
"""@EN; 
                          rdfs:subClassOf ddhub:Unit. 
ddhub:MillionBarrel a owl:Class; 
                    rdfs:comment """[v] = a * [SI]
where
[v] is the value in million barrel
[SI] is the value in SI
a = 1.0/(Mega*Barrel), i.e., 6.289810770432106E-06
and
Mega = 1e6
Barrel = 42.0 * GallonUS reference: https://en.wikipedia.org/wiki/Barrel_(unit)
GallonUS = 231.0 * Inch * Inch * Inch reference: https://en.wikipedia.org/wiki/Gallon
Inch = 0.0254 reference: https://www.nist.gov/pml/owm/si-units-length
"""@EN; 
                    rdfs:subClassOf ddhub:Unit. 
ddhub:MillionCubicMetre a owl:Class; 
                        rdfs:comment """[v] = a * [SI]
where
[v] is the value in million cubic metre
[SI] is the value in SI
a = 1.0/Mega, i.e., 1E-06
and
Mega = 1e6
"""@EN; 
                        rdfs:subClassOf ddhub:Unit. 
ddhub:MillionCubicMetrePerDay a owl:Class; 
                              rdfs:comment """[v] = a * [SI]
where
[v] is the value in million cubic metre per day
[SI] is the value in SI
a = Day / Mega, i.e., 0.0864
and
Day = 24.0 * Hour
Mega = 1e6
Hour = 60.0 * Minute
Minute = 60.0
"""@EN; 
                              rdfs:subClassOf ddhub:Unit. 
ddhub:MillionLiterPerDay a owl:Class; 
                         rdfs:comment """[v] = a * [SI]
where
[v] is the value in million liter per day
[SI] is the value in SI
a = Day / (Mega*Milli), i.e., 86.4
and
Day = 24.0 * Hour
Mega = 1e6
Milli = 0.001
Hour = 60.0 * Minute
Minute = 60.0
"""@EN; 
                         rdfs:subClassOf ddhub:Unit. 
ddhub:MillionLitre a owl:Class; 
                   rdfs:comment """[v] = a * [SI]
where
[v] is the value in million litre
[SI] is the value in SI
a = 1.0/(Mega*Milli), i.e., 0.001
and
Mega = 1e6
Milli = 0.001
"""@EN; 
                   rdfs:subClassOf ddhub:Unit. 
ddhub:MillionStandardCubicFoot a owl:Class; 
                               rdfs:comment """[v] = a * [SI]
where
[v] is the value in million standard cubic foot
[SI] is the value in SI
a = 1.0/(Mega*Foot*Foot*Foot), i.e., 3.531466672148861E-05
and
Mega = 1e6
Foot = 12.0 * Inch
Inch = 0.0254 reference: https://www.nist.gov/pml/owm/si-units-length
"""@EN; 
                               rdfs:subClassOf ddhub:Unit. 
ddhub:MillionStandardCubicFootPerDay a owl:Class; 
                                     rdfs:comment """[v] = a * [SI]
where
[v] is the value in million standard cubic foot per day
[SI] is the value in SI
a = Day / (Mega*Foot*Foot*Foot), i.e., 3.0511872047366158
and
Day = 24.0 * Hour
Mega = 1e6
Foot = 12.0 * Inch
Hour = 60.0 * Minute
Inch = 0.0254 reference: https://www.nist.gov/pml/owm/si-units-length
Minute = 60.0
"""@EN; 
                                     rdfs:subClassOf ddhub:Unit. 
ddhub:MillionUkGallon a owl:Class; 
                      rdfs:comment """[v] = a * [SI]
where
[v] is the value in million UK gallon
[SI] is the value in SI
a = 1.0/(Mega*GallonUK), i.e., 0.0002199692482990878
and
Mega = 1e6
GallonUK = 4.54609e-3 reference: https://en.wikipedia.org/wiki/Gallon
"""@EN; 
                      rdfs:subClassOf ddhub:Unit. 
ddhub:MillionUkGallonPerDay a owl:Class; 
                            rdfs:comment """[v] = a * [SI]
where
[v] is the value in million UK gallon per day
[SI] is the value in SI
a = Day / (Mega*GallonUK), i.e., 19.005343053041184
and
Day = 24.0 * Hour
Mega = 1e6
GallonUK = 4.54609e-3 reference: https://en.wikipedia.org/wiki/Gallon
Hour = 60.0 * Minute
Minute = 60.0
"""@EN; 
                            rdfs:subClassOf ddhub:Unit. 
ddhub:MillionUsGallon a owl:Class; 
                      rdfs:comment """[v] = a * [SI]
where
[v] is the value in million US gallon
[SI] is the value in SI
a = 1.0/(Mega*GallonUS), i.e., 0.00026417205235814843
and
Mega = 1e6
GallonUS = 231.0 * Inch * Inch * Inch reference: https://en.wikipedia.org/wiki/Gallon
Inch = 0.0254 reference: https://www.nist.gov/pml/owm/si-units-length
"""@EN; 
                      rdfs:subClassOf ddhub:Unit. 
ddhub:MillionUsGallonPerDay a owl:Class; 
                            rdfs:comment """[v] = a * [SI]
where
[v] is the value in million US gallon per day
[SI] is the value in SI
a = Day / (Mega*GallonUS), i.e., 22.824465323744025
and
Day = 24.0 * Hour
Mega = 1e6
GallonUS = 231.0 * Inch * Inch * Inch reference: https://en.wikipedia.org/wiki/Gallon
Hour = 60.0 * Minute
Inch = 0.0254 reference: https://www.nist.gov/pml/owm/si-units-length
Minute = 60.0
"""@EN; 
                            rdfs:subClassOf ddhub:Unit. 
ddhub:MillionYear a owl:Class; 
                  rdfs:comment """[v] = a * [SI]
where
[v] is the value in million year
[SI] is the value in SI
a = 1.0/MillionYear, i.e., 3.168808781402895E-14
and
MillionYear = 1000.0 * Millenia
Millenia = 10.0 * Century
Century = 10.0 * Decade
Decade = 10.0 * YearJulian
YearJulian = 365.25 * Day
Day = 24.0 * Hour
Hour = 60.0 * Minute
Minute = 60.0
"""@EN; 
                  rdfs:subClassOf ddhub:Unit. 
ddhub:MillipascalSecond a owl:Class; 
                        rdfs:comment """[v] = a * [SI]
where
[v] is the value in millipascal second
[SI] is the value in SI
a = 1.0/Milli, i.e., 1000
and
Milli = 0.001
"""@EN; 
                        rdfs:subClassOf ddhub:Unit. 
ddhub:Millipoise a owl:Class; 
                 rdfs:comment """[v] = a * [SI]
where
[v] is the value in millipoise
[SI] is the value in SI
a = 1.0/(Milli* Poise), i.e., 10000
and
Milli = 0.001
Poise = 0.1 reference: https://en.wikipedia.org/wiki/Poise_(unit)
"""@EN; 
                 rdfs:subClassOf ddhub:Unit. 
ddhub:Milliradian a owl:Class; 
                  rdfs:comment """[v] = a * [SI]
where
[v] is the value in milliradian
[SI] is the value in SI
a = 1.0/Milli, i.e., 1000
and
Milli = 0.001
"""@EN; 
                  rdfs:subClassOf ddhub:Unit. 
ddhub:Millisecond a owl:Class; 
                  rdfs:comment """[v] = a * [SI]
where
[v] is the value in millisecond
[SI] is the value in SI
a = 1.0/Milli, i.e., 1000
and
Milli = 0.001
"""@EN; 
                  rdfs:subClassOf ddhub:Unit. 
ddhub:Millitesla a owl:Class; 
                 rdfs:comment """[v] = a * [SI]
where
[v] is the value in millitesla
[SI] is the value in SI
a = 1.0/Milli, i.e., 1000
and
Milli = 0.001
"""@EN; 
                 rdfs:subClassOf ddhub:Unit. 
ddhub:Millivolt a owl:Class; 
                rdfs:comment """[v] = a * [SI]
where
[v] is the value in millivolt
[SI] is the value in SI
a = 1.0/Milli, i.e., 1000
and
Milli = 0.001
"""@EN; 
                rdfs:subClassOf ddhub:Unit. 
ddhub:Milliwatt a owl:Class; 
                rdfs:comment """[v] = a * [SI]
where
[v] is the value in milliwatt
[SI] is the value in SI
a = 1.0/Milli, i.e., 1000
and
Milli = 0.001
"""@EN; 
                rdfs:subClassOf ddhub:Unit. 
ddhub:Milliweber a owl:Class; 
                 rdfs:comment """[v] = a * [SI]
where
[v] is the value in milliweber
[SI] is the value in SI
a = 1.0/Milli, i.e., 1000
and
Milli = 0.001
"""@EN; 
                 rdfs:subClassOf ddhub:Unit. 
ddhub:MillPackerPickerAssembly a owl:Class; 
                               rdfs:comment ""@EN; 
                               rdfs:subClassOf ddhub:CasingMillingTools. 
ddhub:MillPilot a owl:Class; 
                rdfs:comment ""@EN; 
                rdfs:subClassOf ddhub:CasingMillingTools. 
ddhub:MillPolish a owl:Class; 
                 rdfs:comment ""@EN; 
                 rdfs:subClassOf ddhub:CasingMillingTools. 
ddhub:MillSection a owl:Class; 
                  rdfs:comment ""@EN; 
                  rdfs:subClassOf ddhub:CasingMillingTools. 
ddhub:MillTaper a owl:Class; 
                rdfs:comment ""@EN; 
                rdfs:subClassOf ddhub:CasingMillingTools. 
ddhub:Milltooth a owl:Class; 
                rdfs:comment ""@EN; 
                rdfs:subClassOf ddhub:RollingCutter. 
ddhub:MillWashover a owl:Class; 
                   rdfs:comment ""@EN; 
                   rdfs:subClassOf ddhub:CasingMillingTools. 
ddhub:MillWatermelon a owl:Class; 
                     rdfs:comment ""@EN; 
                     rdfs:subClassOf ddhub:CasingMillingTools. 
ddhub:MinDrillHeightVerticalLocation a owl:Class; 
                                     rdfs:comment ""@EN; 
                                     rdfs:subClassOf ddhub:VerticalReferenceLocation. 
ddhub:MinFrequency a owl:DatatypeProperty, owl:FunctionalProperty; 
                   rdfs:comment """
"""@EN; 
                   rdfs:domain ddhub:BandPassFilter; 
                   rdfs:range xsd:double. 
ddhub:MinimumHorizontalStress a owl:Class; 
                              rdfs:comment ""@EN; 
                              rdfs:subClassOf ddhub:PrototypeData. 
ddhub:MinimumHorizontalStressGradient a owl:Class; 
                                      rdfs:comment ""@EN; 
                                      rdfs:subClassOf ddhub:PrototypeData. 
ddhub:MinimumLimit a owl:Class; 
                   rdfs:comment ""@EN; 
                   rdfs:subClassOf ddhub:Limit. 
ddhub:MinMaxUncertainty a owl:Class; 
                        rdfs:comment """The uncertainty is represented by a uniform probability distribution between a `Min` and a `Max` value.
"""@EN; 
                        rdfs:subClassOf ddhub:SignalUncertainty. 
ddhub:Minute a owl:Class; 
             rdfs:comment """[v] = a * [SI]
where
[v] is the value in minute
[SI] is the value in SI
a = 1.0/Minute, i.e., 0.016666666666666666
and
Minute = 60.0
"""@EN; 
             rdfs:subClassOf ddhub:Unit. 
ddhub:MiscSubs a owl:Class; 
               rdfs:comment ""@EN; 
               rdfs:subClassOf ddhub:DrillString. 
ddhub:MixingTank a owl:Class; 
                 rdfs:comment ""@EN; 
                 rdfs:subClassOf ddhub:MudPits. 
ddhub:Mnemonic a owl:DatatypeProperty, owl:FunctionalProperty; 
               rdfs:comment """
"""@EN; 
               rdfs:domain ddhub:WitsMLTimeBasedLogEndPoint; 
               rdfs:range xsd:string. 
ddhub:ModelingApproach a owl:Class; 
                       rdfs:comment """A classification of the modeling direction of a model.
"""@EN; 
                       rdfs:subClassOf ddhub:DWISNoun. 
ddhub:ModelingObjective a owl:Class; 
                        rdfs:comment """A classification of the objective/purpose of a model.
"""@EN; 
                        rdfs:subClassOf ddhub:DWISNoun. 
ddhub:ModelingParadigm a owl:Class; 
                       rdfs:comment """A classification of the relationship of the model to data or physical laws.
"""@EN; 
                       rdfs:subClassOf ddhub:DWISNoun. 
ddhub:ModelledDegreeOfFreedom a owl:Class; 
                              rdfs:comment """In physics and chemistry, a degree of freedom is an independent physical parameter in the formal description of the state of a physical system. A model may account for some or all of the degrees of freedom of the physical system.
"""@EN; 
                              rdfs:subClassOf ddhub:DWISNoun. 
ddhub:ModellingDimensions a owl:Class; 
                          rdfs:comment """The number of dimensions that are accounted by the model
"""@EN; 
                          rdfs:subClassOf ddhub:DWISNoun. 
ddhub:ModellingDiscretization a owl:Class; 
                              rdfs:comment """A characteristic of the discretization made by the model.
"""@EN; 
                              rdfs:subClassOf ddhub:DWISNoun. 
ddhub:ModelScope a owl:Class; 
                 rdfs:comment """A classification of a model with regards to its range of applicability.
"""@EN; 
                 rdfs:subClassOf ddhub:DWISNoun. 
ddhub:ModelTransparency a owl:Class; 
                        rdfs:comment """A classification of a model with regards to its transparency or interpretability.
"""@EN; 
                        rdfs:subClassOf ddhub:DWISNoun. 
ddhub:ModelType a owl:Class; 
                rdfs:comment ""@EN; 
                rdfs:subClassOf ddhub:DWISNoun. 
ddhub:Mole a owl:Class; 
           rdfs:comment """No conversion necessary as the unit choice is SI
"""@EN; 
           rdfs:subClassOf ddhub:Unit. 
ddhub:MonthCommon a owl:Class; 
                  rdfs:comment """[v] = a * [SI]
where
[v] is the value in month common
[SI] is the value in SI
a = 1.0/MonthCommon, i.e., 3.802570537683474E-07
and
MonthCommon = YearJulian / 12.0
YearJulian = 365.25 * Day
Day = 24.0 * Hour
Hour = 60.0 * Minute
Minute = 60.0
"""@EN; 
                  rdfs:subClassOf ddhub:Unit. 
ddhub:MonthSideral a owl:Class; 
                   rdfs:comment """[v] = a * [SI]
where
[v] is the value in month sideral
[SI] is the value in SI
a = 1.0/MonthSideral, i.e., 4.2362265228665E-07
and
MonthSideral = 27.32166 * Day reference: https://en.wikipedia.org/wiki/Month
Day = 24.0 * Hour
Hour = 60.0 * Minute
Minute = 60.0
"""@EN; 
                   rdfs:subClassOf ddhub:Unit. 
ddhub:MonthSynodic a owl:Class; 
                   rdfs:comment """[v] = a * [SI]
where
[v] is the value in month synodic
[SI] is the value in SI
a = 1.0/MonthSynodic, i.e., 3.9193507729016165E-07
and
MonthSynodic = 29.53059 * Day reference: https://en.wikipedia.org/wiki/Month
Day = 24.0 * Hour
Hour = 60.0 * Minute
Minute = 60.0
"""@EN; 
                   rdfs:subClassOf ddhub:Unit. 
ddhub:MooringLines a owl:Class; 
                   rdfs:comment ""@EN; 
                   rdfs:subClassOf ddhub:MooringSystem. 
ddhub:MooringSystem a owl:Class; 
                    rdfs:comment ""@EN; 
                    rdfs:subClassOf ddhub:MarineSystem. 
ddhub:MotionType a owl:Class; 
                 rdfs:comment ""@EN; 
                 rdfs:subClassOf ddhub:DWISNoun. 
ddhub:MotorStall a owl:Class; 
                 rdfs:comment """This Noun is used to refer to a situation during which the downhole motor is stalled.
"""@EN; 
                 rdfs:subClassOf ddhub:DrillingIncident. 
ddhub:Mousehole a owl:Class; 
                rdfs:comment ""@EN; 
                rdfs:subClassOf ddhub:DrillFloorStructure. 
ddhub:MovingAverage a owl:Class; 
                    rdfs:comment ""@EN; 
                    rdfs:subClassOf ddhub:Filter. 
ddhub:MovingMax a owl:Class; 
                rdfs:comment ""@EN; 
                rdfs:subClassOf ddhub:Filter. 
ddhub:MovingMin a owl:Class; 
                rdfs:comment ""@EN; 
                rdfs:subClassOf ddhub:Filter. 
ddhub:MovingStandardDeviation a owl:Class; 
                              rdfs:comment ""@EN; 
                              rdfs:subClassOf ddhub:Filter. 
ddhub:MPDAlternateFlowPath a owl:Class; 
                           rdfs:comment ""@EN; 
                           rdfs:subClassOf ddhub:TopsideHydraulicNetwork. 
ddhub:MpdChoke a owl:Class; 
               rdfs:comment ""@EN; 
               rdfs:subClassOf ddhub:WellControlSystem. 
ddhub:MPDChokeOpening a owl:Class; 
                      rdfs:comment ""@EN; 
                      rdfs:subClassOf ddhub:PrototypeData. 
ddhub:MPDChokePressure a owl:Class; 
                       rdfs:comment ""@EN; 
                       rdfs:subClassOf ddhub:PrototypeData. 
ddhub:MPDMainFlowPath a owl:Class; 
                      rdfs:comment ""@EN; 
                      rdfs:subClassOf ddhub:TopsideHydraulicNetwork. 
ddhub:MPDPumpFlowRate a owl:Class; 
                      rdfs:comment ""@EN; 
                      rdfs:subClassOf ddhub:PrototypeData. 
ddhub:MPDPumpRate a owl:Class; 
                  rdfs:comment ""@EN; 
                  rdfs:subClassOf ddhub:PrototypeData. 
ddhub:MudHose a owl:Class; 
              rdfs:comment ""@EN; 
              rdfs:subClassOf ddhub:MudLines. 
ddhub:MudLines a owl:Class; 
               rdfs:comment ""@EN; 
               rdfs:subClassOf ddhub:CirculationSystem. 
ddhub:MudLineSystem a owl:Class; 
                    rdfs:comment ""@EN; 
                    rdfs:subClassOf ddhub:MarineSystem. 
ddhub:MudLoggingEquipment a owl:Class; 
                          rdfs:comment ""@EN; 
                          rdfs:subClassOf ddhub:RigEquipment. 
ddhub:MudLubeBearing a owl:Class; 
                     rdfs:comment ""@EN; 
                     rdfs:subClassOf ddhub:DownholeMotor. 
ddhub:MudMixing a owl:Class; 
                rdfs:comment ""@EN; 
                rdfs:subClassOf ddhub:HydraulicJunction. 
ddhub:MudPits a owl:Class; 
              rdfs:comment ""@EN; 
              rdfs:subClassOf ddhub:CirculationSystem. 
ddhub:MudPulse a owl:Class; 
               rdfs:comment ""@EN; 
               rdfs:subClassOf ddhub:EquipmentTelemetry. 
ddhub:MudPulseTelemetry a owl:Class; 
                        rdfs:comment """A method that allows transfer of downhole data to the surface via pressure pulses sent through the drilling fluid.
"""@EN; 
                        rdfs:subClassOf ddhub:DownHoleTelemetry. 
ddhub:MudPump a owl:Class; 
              rdfs:comment ""@EN; 
              rdfs:subClassOf ddhub:CirculationSystem. 
ddhub:MudStandpipe a owl:Class; 
                   rdfs:comment ""@EN; 
                   rdfs:subClassOf ddhub:MudLines. 
ddhub:MudStandpipeManifold a owl:Class; 
                           rdfs:comment ""@EN; 
                           rdfs:subClassOf ddhub:MudLines. 
ddhub:N a owl:DatatypeProperty, owl:FunctionalProperty; 
        rdfs:comment """Amount of substance exponent.
SI Unit: Mole (N)
"""@EN; 
        rdfs:domain ddhub:Quantity; 
        rdfs:range xsd:double. 
ddhub:Nanoampere a owl:Class; 
                 rdfs:comment """[v] = a * [SI]
where
[v] is the value in nanoampere
[SI] is the value in SI
a = 1.0/Nano, i.e., 999999999.9999999
and
Nano = 1e-9
"""@EN; 
                 rdfs:subClassOf ddhub:Unit. 
ddhub:Nanodarcy a owl:Class; 
                rdfs:comment """[v] = a * [SI]
where
[v] is the value in nanodarcy
[SI] is the value in SI
a = 1.0/(Nano*Darcy), i.e., 1.01325E+21
and
Nano = 1e-9
Darcy = 0.0000001 / Atmosphere reference: https://en.wikipedia.org/wiki/Darcy_(unit)
Atmosphere = 101325.0 reference: https://en.wikipedia.org/wiki/Atmospheric_pressure
"""@EN; 
                rdfs:subClassOf ddhub:Unit. 
ddhub:Nanofarad a owl:Class; 
                rdfs:comment """[v] = a * [SI]
where
[v] is the value in nanofarad
[SI] is the value in SI
a = 1.0/Nano, i.e., 999999999.9999999
and
Nano = 1e-9
"""@EN; 
                rdfs:subClassOf ddhub:Unit. 
ddhub:Nanogram a owl:Class; 
               rdfs:comment """[v] = a * [SI]
where
[v] is the value in nanogram
[SI] is the value in SI
a = 1.0/Pico, i.e., 1000000000000
and
Pico = 1e-12
"""@EN; 
               rdfs:subClassOf ddhub:Unit. 
ddhub:Nanometre a owl:Class; 
                rdfs:comment """[v] = a * [SI]
where
[v] is the value in nanometre
[SI] is the value in SI
a = 1.0/Nano, i.e., 999999999.9999999
and
Nano = 1e-9
"""@EN; 
                rdfs:subClassOf ddhub:Unit. 
ddhub:Nanomole a owl:Class; 
               rdfs:comment """[v] = a * [SI]
where
[v] is the value in nanomole
[SI] is the value in SI
a = 1.0/Nano, i.e., 999999999.9999999
and
Nano = 1e-9
"""@EN; 
               rdfs:subClassOf ddhub:Unit. 
ddhub:Nanosecond a owl:Class; 
                 rdfs:comment """[v] = a * [SI]
where
[v] is the value in nanosecond
[SI] is the value in SI
a = 1.0/Nano, i.e., 999999999.9999999
and
Nano = 1e-9
"""@EN; 
                 rdfs:subClassOf ddhub:Unit. 
ddhub:Nanotesla a owl:Class; 
                rdfs:comment """[v] = a * [SI]
where
[v] is the value in nanotesla
[SI] is the value in SI
a = 1.0/Nano, i.e., 999999999.9999999
and
Nano = 1e-9
"""@EN; 
                rdfs:subClassOf ddhub:Unit. 
ddhub:Nanovolt a owl:Class; 
               rdfs:comment """[v] = a * [SI]
where
[v] is the value in nanovolt
[SI] is the value in SI
a = 1.0/Nano, i.e., 999999999.9999999
and
Nano = 1e-9
"""@EN; 
               rdfs:subClassOf ddhub:Unit. 
ddhub:Nanowatt a owl:Class; 
               rdfs:comment """[v] = a * [SI]
where
[v] is the value in nanowatt
[SI] is the value in SI
a = 1.0/Nano, i.e., 999999999.9999999
and
Nano = 1e-9
"""@EN; 
               rdfs:subClassOf ddhub:Unit. 
ddhub:NearBit a owl:Class; 
              rdfs:comment ""@EN; 
              rdfs:subClassOf ddhub:Stabilizers. 
ddhub:NearbitReamers a owl:Class; 
                     rdfs:comment ""@EN; 
                     rdfs:subClassOf ddhub:Reamers. 
ddhub:NearBitVibrationDampers a owl:Class; 
                              rdfs:comment ""@EN; 
                              rdfs:subClassOf ddhub:ActiveVibrationTools. 
ddhub:NetworkSynchronizationLatencyAverage a owl:DatatypeProperty, owl:FunctionalProperty; 
                                           rdfs:comment """
"""@EN; 
                                           rdfs:domain ddhub:Clock; 
                                           rdfs:range xsd:double. 
ddhub:NetworkSynchronizationLatencyStandardDeviation a owl:DatatypeProperty, owl:FunctionalProperty; 
                                                     rdfs:comment """
"""@EN; 
                                                     rdfs:domain ddhub:Clock; 
                                                     rdfs:range xsd:double. 
ddhub:Newton a owl:Class; 
             rdfs:comment """No conversion necessary as the unit choice is SI
"""@EN; 
             rdfs:subClassOf ddhub:Unit. 
ddhub:NewtonCentimetre a owl:Class; 
                       rdfs:comment """[v] = a * [SI]
where
[v] is the value in newton centimetre
[SI] is the value in SI
a = 1.0/Centi, i.e., 100
and
Centi = 0.01
"""@EN; 
                       rdfs:subClassOf ddhub:Unit. 
ddhub:NewtonCentimetrePerCentimetre a owl:Class; 
                                    rdfs:comment """[v] = a * [SI]
where
[v] is the value in newton centimetre per centimetre
[SI] is the value in SI
a = Centi/Centi, i.e., 1
and
Centi = 0.01
"""@EN; 
                                    rdfs:subClassOf ddhub:Unit. 
ddhub:NewtonCentimetrePerDecimetre a owl:Class; 
                                   rdfs:comment """[v] = a * [SI]
where
[v] is the value in newton centimetre per decimetre
[SI] is the value in SI
a = Deci/(Centi*Unit), i.e., 10
and
Deci = 0.1
Centi = 0.01
Unit = 1.0
"""@EN; 
                                   rdfs:subClassOf ddhub:Unit. 
ddhub:NewtonCentimetrePerFoot a owl:Class; 
                              rdfs:comment """[v] = a * [SI]
where
[v] is the value in newton centimetre per foot
[SI] is the value in SI
a = Foot/Centi, i.e., 30.479999999999997
and
Foot = 12.0 * Inch
Centi = 0.01
Inch = 0.0254 reference: https://www.nist.gov/pml/owm/si-units-length
"""@EN; 
                              rdfs:subClassOf ddhub:Unit. 
ddhub:NewtonCentimetrePerHour a owl:Class; 
                              rdfs:comment """[v] = a * [SI]
where
[v] is the value in newton centimetre per hour
[SI] is the value in SI
a = Hour/Centi, i.e., 360000
and
Hour = 60.0 * Minute
Centi = 0.01
Minute = 60.0
"""@EN; 
                              rdfs:subClassOf ddhub:Unit. 
ddhub:NewtonCentimetrePerInch a owl:Class; 
                              rdfs:comment """[v] = a * [SI]
where
[v] is the value in newton centimetre per inch
[SI] is the value in SI
a = Inch/Centi, i.e., 2.54
and
Inch = 0.0254 reference: https://www.nist.gov/pml/owm/si-units-length
Centi = 0.01
"""@EN; 
                              rdfs:subClassOf ddhub:Unit. 
ddhub:NewtonCentimetrePerMetre a owl:Class; 
                               rdfs:comment """[v] = a * [SI]
where
[v] is the value in newton centimetre per metre
[SI] is the value in SI
a = Unit/Centi, i.e., 100
and
Unit = 1.0
Centi = 0.01
"""@EN; 
                               rdfs:subClassOf ddhub:Unit. 
ddhub:NewtonCentimetrePerMillimetre a owl:Class; 
                                    rdfs:comment """[v] = a * [SI]
where
[v] is the value in newton centimetre per millimetre
[SI] is the value in SI
a = Milli/Centi, i.e., 0.1
and
Milli = 0.001
Centi = 0.01
"""@EN; 
                                    rdfs:subClassOf ddhub:Unit. 
ddhub:NewtonCentimetrePerMinute a owl:Class; 
                                rdfs:comment """[v] = a * [SI]
where
[v] is the value in newton centimetre per minute
[SI] is the value in SI
a = Minute/Centi, i.e., 6000
and
Minute = 60.0
Centi = 0.01
"""@EN; 
                                rdfs:subClassOf ddhub:Unit. 
ddhub:NewtonCentimetrePerSecond a owl:Class; 
                                rdfs:comment """[v] = a * [SI]
where
[v] is the value in newton centimetre per second
[SI] is the value in SI
a = 1.0/Centi, i.e., 100
and
Centi = 0.01
"""@EN; 
                                rdfs:subClassOf ddhub:Unit. 
ddhub:NewtonDecimetre a owl:Class; 
                      rdfs:comment """[v] = a * [SI]
where
[v] is the value in newton decimetre
[SI] is the value in SI
a = 1.0/Deci, i.e., 10
and
Deci = 0.1
"""@EN; 
                      rdfs:subClassOf ddhub:Unit. 
ddhub:NewtonDecimetrePerCentimetre a owl:Class; 
                                   rdfs:comment """[v] = a * [SI]
where
[v] is the value in newton decimetre per centimetre
[SI] is the value in SI
a = Centi/(Deci), i.e., 0.09999999999999999
and
Centi = 0.01
Deci = 0.1
"""@EN; 
                                   rdfs:subClassOf ddhub:Unit. 
ddhub:NewtonDecimetrePerDecimetre a owl:Class; 
                                  rdfs:comment """[v] = a * [SI]
where
[v] is the value in newton decimetre per decimetre
[SI] is the value in SI
a = Deci/(Deci*Unit), i.e., 1
and
Deci = 0.1
Unit = 1.0
"""@EN; 
                                  rdfs:subClassOf ddhub:Unit. 
ddhub:NewtonDecimetrePerFoot a owl:Class; 
                             rdfs:comment """[v] = a * [SI]
where
[v] is the value in newton decimetre per foot
[SI] is the value in SI
a = Foot/(Deci), i.e., 3.0479999999999996
and
Foot = 12.0 * Inch
Deci = 0.1
Inch = 0.0254 reference: https://www.nist.gov/pml/owm/si-units-length
"""@EN; 
                             rdfs:subClassOf ddhub:Unit. 
ddhub:NewtonDecimetrePerHour a owl:Class; 
                             rdfs:comment """[v] = a * [SI]
where
[v] is the value in newton decimetre per hour
[SI] is the value in SI
a = Hour/Deci, i.e., 36000
and
Hour = 60.0 * Minute
Deci = 0.1
Minute = 60.0
"""@EN; 
                             rdfs:subClassOf ddhub:Unit. 
ddhub:NewtonDecimetrePerInch a owl:Class; 
                             rdfs:comment """[v] = a * [SI]
where
[v] is the value in newton decimetre per inch
[SI] is the value in SI
a = Inch/Deci, i.e., 0.25399999999999995
and
Inch = 0.0254 reference: https://www.nist.gov/pml/owm/si-units-length
Deci = 0.1
"""@EN; 
                             rdfs:subClassOf ddhub:Unit. 
ddhub:NewtonDecimetrePerMetre a owl:Class; 
                              rdfs:comment """[v] = a * [SI]
where
[v] is the value in newton decimetre per metre
[SI] is the value in SI
a = Unit/Deci, i.e., 10
and
Unit = 1.0
Deci = 0.1
"""@EN; 
                              rdfs:subClassOf ddhub:Unit. 
ddhub:NewtonDecimetrePerMillimetre a owl:Class; 
                                   rdfs:comment """[v] = a * [SI]
where
[v] is the value in newton decimetre per millimetre
[SI] is the value in SI
a = Milli/(Deci), i.e., 0.01
and
Milli = 0.001
Deci = 0.1
"""@EN; 
                                   rdfs:subClassOf ddhub:Unit. 
ddhub:NewtonDecimetrePerMinute a owl:Class; 
                               rdfs:comment """[v] = a * [SI]
where
[v] is the value in newton decimetre per minute
[SI] is the value in SI
a = Minute/Deci, i.e., 600
and
Minute = 60.0
Deci = 0.1
"""@EN; 
                               rdfs:subClassOf ddhub:Unit. 
ddhub:NewtonDecimetrePerSecond a owl:Class; 
                               rdfs:comment """[v] = a * [SI]
where
[v] is the value in newton decimetre per second
[SI] is the value in SI
a = 1.0/Deci, i.e., 10
and
Deci = 0.1
"""@EN; 
                               rdfs:subClassOf ddhub:Unit. 
ddhub:NewtonMetre a owl:Class; 
                  rdfs:comment """No conversion necessary as the unit choice is SI
"""@EN; 
                  rdfs:subClassOf ddhub:Unit. 
ddhub:NewtonMetrePerCentimetre a owl:Class; 
                               rdfs:comment """[v] = a * [SI]
where
[v] is the value in Newton metre per centimetre
[SI] is the value in SI
a = Centi/(Unit*Unit), i.e., 0.01
and
Centi = 0.01
Unit = 1.0
"""@EN; 
                               rdfs:subClassOf ddhub:Unit. 
ddhub:NewtonMetrePerDecimetre a owl:Class; 
                              rdfs:comment """[v] = a * [SI]
where
[v] is the value in Newton metre per decimetre
[SI] is the value in SI
a = Deci/Unit, i.e., 0.1
and
Deci = 0.1
Unit = 1.0
"""@EN; 
                              rdfs:subClassOf ddhub:Unit. 
ddhub:NewtonMetrePerFoot a owl:Class; 
                         rdfs:comment """[v] = a * [SI]
where
[v] is the value in Newton metre per foot
[SI] is the value in SI
a = Foot/Unit, i.e., 0.30479999999999996
and
Foot = 12.0 * Inch
Unit = 1.0
Inch = 0.0254 reference: https://www.nist.gov/pml/owm/si-units-length
"""@EN; 
                         rdfs:subClassOf ddhub:Unit. 
ddhub:NewtonMetrePerHour a owl:Class; 
                         rdfs:comment """No conversion necessary as the unit choice is SI
"""@EN; 
                         rdfs:subClassOf ddhub:Unit. 
ddhub:NewtonMetrePerInch a owl:Class; 
                         rdfs:comment """[v] = a * [SI]
where
[v] is the value in Newton metre per inch
[SI] is the value in SI
a = Inch/Unit, i.e., 0.0254
and
Inch = 0.0254 reference: https://www.nist.gov/pml/owm/si-units-length
Unit = 1.0
"""@EN; 
                         rdfs:subClassOf ddhub:Unit. 
ddhub:NewtonMetrePerMetre a owl:Class; 
                          rdfs:comment """No conversion necessary as the unit choice is SI
"""@EN; 
                          rdfs:subClassOf ddhub:Unit. 
ddhub:NewtonMetrePerMillimetre a owl:Class; 
                               rdfs:comment """[v] = a * [SI]
where
[v] is the value in Newton metre per millimetre
[SI] is the value in SI
a = Milli/(Unit*Unit), i.e., 0.001
and
Milli = 0.001
Unit = 1.0
"""@EN; 
                               rdfs:subClassOf ddhub:Unit. 
ddhub:NewtonMetrePerMinute a owl:Class; 
                           rdfs:comment """No conversion necessary as the unit choice is SI
"""@EN; 
                           rdfs:subClassOf ddhub:Unit. 
ddhub:NewtonMetrePerSecond a owl:Class; 
                           rdfs:comment """No conversion necessary as the unit choice is SI
"""@EN; 
                           rdfs:subClassOf ddhub:Unit. 
ddhub:NewtonMillimetre a owl:Class; 
                       rdfs:comment """[v] = a * [SI]
where
[v] is the value in newton millimetre
[SI] is the value in SI
a = 1.0/Milli, i.e., 1000
and
Milli = 0.001
"""@EN; 
                       rdfs:subClassOf ddhub:Unit. 
ddhub:NewtonMillimetrePerCentimetre a owl:Class; 
                                    rdfs:comment """[v] = a * [SI]
where
[v] is the value in newton millimetre per centimetre
[SI] is the value in SI
a = Centi/Milli, i.e., 10
and
Centi = 0.01
Milli = 0.001
"""@EN; 
                                    rdfs:subClassOf ddhub:Unit. 
ddhub:NewtonMillimetrePerDecimetre a owl:Class; 
                                   rdfs:comment """[v] = a * [SI]
where
[v] is the value in newton millimetre per decimetre
[SI] is the value in SI
a = Deci/(Milli*Unit), i.e., 100
and
Deci = 0.1
Milli = 0.001
Unit = 1.0
"""@EN; 
                                   rdfs:subClassOf ddhub:Unit. 
ddhub:NewtonMillimetrePerFoot a owl:Class; 
                              rdfs:comment """[v] = a * [SI]
where
[v] is the value in newton millimetre per foot
[SI] is the value in SI
a = Foot/Milli, i.e., 304.79999999999995
and
Foot = 12.0 * Inch
Milli = 0.001
Inch = 0.0254 reference: https://www.nist.gov/pml/owm/si-units-length
"""@EN; 
                              rdfs:subClassOf ddhub:Unit. 
ddhub:NewtonMillimetrePerHour a owl:Class; 
                              rdfs:comment """[v] = a * [SI]
where
[v] is the value in newton millimetre per hour
[SI] is the value in SI
a = Hour/Milli, i.e., 3600000
and
Hour = 60.0 * Minute
Milli = 0.001
Minute = 60.0
"""@EN; 
                              rdfs:subClassOf ddhub:Unit. 
ddhub:NewtonMillimetrePerInch a owl:Class; 
                              rdfs:comment """[v] = a * [SI]
where
[v] is the value in newton millimetre per inch
[SI] is the value in SI
a = Inch/Milli, i.e., 25.4
and
Inch = 0.0254 reference: https://www.nist.gov/pml/owm/si-units-length
Milli = 0.001
"""@EN; 
                              rdfs:subClassOf ddhub:Unit. 
ddhub:NewtonMillimetrePerMetre a owl:Class; 
                               rdfs:comment """[v] = a * [SI]
where
[v] is the value in newton millimetre per metre
[SI] is the value in SI
a = Unit/Milli, i.e., 1000
and
Unit = 1.0
Milli = 0.001
"""@EN; 
                               rdfs:subClassOf ddhub:Unit. 
ddhub:NewtonMillimetrePerMillimetre a owl:Class; 
                                    rdfs:comment """[v] = a * [SI]
where
[v] is the value in newton millimetre per millimetre
[SI] is the value in SI
a = Milli/Milli, i.e., 1
and
Milli = 0.001
"""@EN; 
                                    rdfs:subClassOf ddhub:Unit. 
ddhub:NewtonMillimetrePerMinute a owl:Class; 
                                rdfs:comment """[v] = a * [SI]
where
[v] is the value in newton millimetre per minute
[SI] is the value in SI
a = Minute/Milli, i.e., 60000
and
Minute = 60.0
Milli = 0.001
"""@EN; 
                                rdfs:subClassOf ddhub:Unit. 
ddhub:NewtonMillimetrePerSecond a owl:Class; 
                                rdfs:comment """[v] = a * [SI]
where
[v] is the value in newton millimetre per second
[SI] is the value in SI
a = 1.0/Milli, i.e., 1000
and
Milli = 0.001
"""@EN; 
                                rdfs:subClassOf ddhub:Unit. 
ddhub:NewtonPer10Metre a owl:Class; 
                       rdfs:comment """[v] = a * [SI]
where
[v] is the value in newton per 10 metre
[SI] is the value in SI
a = Deca/Unit, i.e., 10
and
Deca = 10.0
Unit = 1.0
"""@EN; 
                       rdfs:subClassOf ddhub:Unit. 
ddhub:NewtonPer30Metre a owl:Class; 
                       rdfs:comment """[v] = a * [SI]
where
[v] is the value in newton per 30 metre
[SI] is the value in SI
a = 3*Deca/Unit, i.e., 30
and
Deca = 10.0
Unit = 1.0
"""@EN; 
                       rdfs:subClassOf ddhub:Unit. 
ddhub:NewtonPerCentimetre a owl:Class; 
                          rdfs:comment """[v] = a * [SI]
where
[v] is the value in newton per centimetre
[SI] is the value in SI
a = Centi/Unit, i.e., 0.01
and
Centi = 0.01
Unit = 1.0
"""@EN; 
                          rdfs:subClassOf ddhub:Unit. 
ddhub:NewtonPerDecimetre a owl:Class; 
                         rdfs:comment """[v] = a * [SI]
where
[v] is the value in newton per decimetre
[SI] is the value in SI
a = Deci/Unit, i.e., 0.1
and
Deci = 0.1
Unit = 1.0
"""@EN; 
                         rdfs:subClassOf ddhub:Unit. 
ddhub:NewtonPerHour a owl:Class; 
                    rdfs:comment """No conversion necessary as the unit choice is SI
"""@EN; 
                    rdfs:subClassOf ddhub:Unit. 
ddhub:NewtonPerMetre a owl:Class; 
                     rdfs:comment """No conversion necessary as the unit choice is SI
"""@EN; 
                     rdfs:subClassOf ddhub:Unit. 
ddhub:NewtonPerMillimetre a owl:Class; 
                          rdfs:comment """[v] = a * [SI]
where
[v] is the value in newton per millimetre
[SI] is the value in SI
a = Milli/Unit, i.e., 0.001
and
Milli = 0.001
Unit = 1.0
"""@EN; 
                          rdfs:subClassOf ddhub:Unit. 
ddhub:NewtonPerMinute a owl:Class; 
                      rdfs:comment """No conversion necessary as the unit choice is SI
"""@EN; 
                      rdfs:subClassOf ddhub:Unit. 
ddhub:NewtonPerSecond a owl:Class; 
                      rdfs:comment """No conversion necessary as the unit choice is SI
"""@EN; 
                      rdfs:subClassOf ddhub:Unit. 
ddhub:NewtonPerSquareCentimetre a owl:Class; 
                                rdfs:comment """[v] = a * [SI]
where
[v] is the value in newton per square centimetre
[SI] is the value in SI
a = Centi*Centi, i.e., 0.0001
and
Centi = 0.01
"""@EN; 
                                rdfs:subClassOf ddhub:Unit. 
ddhub:NewtonPerSquareCentimetrePerHour a owl:Class; 
                                       rdfs:comment """[v] = a * [SI]
where
[v] is the value in newton per square centimetre per hour
[SI] is the value in SI
a = Hour*Centi*Centi, i.e., 0.36
and
Hour = 60.0 * Minute
Centi = 0.01
Minute = 60.0
"""@EN; 
                                       rdfs:subClassOf ddhub:Unit. 
ddhub:NewtonPerSquareCentimetrePerMinute a owl:Class; 
                                         rdfs:comment """[v] = a * [SI]
where
[v] is the value in newton per square centimetre per minute
[SI] is the value in SI
a = Minute*Centi*Centi, i.e., 0.006
and
Minute = 60.0
Centi = 0.01
"""@EN; 
                                         rdfs:subClassOf ddhub:Unit. 
ddhub:NewtonPerSquareCentimetrePerSecond a owl:Class; 
                                         rdfs:comment """[v] = a * [SI]
where
[v] is the value in newton per square centimetre per second
[SI] is the value in SI
a = Centi*Centi, i.e., 0.0001
and
Centi = 0.01
"""@EN; 
                                         rdfs:subClassOf ddhub:Unit. 
ddhub:NewtonPerSquareMetre a owl:Class; 
                           rdfs:comment """[v] = a * [SI]
where
[v] is the value in newton per square metre
[SI] is the value in SI
a = 1.0/Unit, i.e., 1
and
Unit = 1.0
"""@EN; 
                           rdfs:subClassOf ddhub:Unit. 
ddhub:NewtonPerSquareMetrePerHour a owl:Class; 
                                  rdfs:comment """[v] = a * [SI]
where
[v] is the value in newton per square metre per hour
[SI] is the value in SI
a = Hour/Unit, i.e., 3600
and
Hour = 60.0 * Minute
Unit = 1.0
Minute = 60.0
"""@EN; 
                                  rdfs:subClassOf ddhub:Unit. 
ddhub:NewtonPerSquareMetrePerMinute a owl:Class; 
                                    rdfs:comment """[v] = a * [SI]
where
[v] is the value in newton per square metre per minute
[SI] is the value in SI
a = Minute/Unit, i.e., 60
and
Minute = 60.0
Unit = 1.0
"""@EN; 
                                    rdfs:subClassOf ddhub:Unit. 
ddhub:NewtonPerSquareMetrePerSecond a owl:Class; 
                                    rdfs:comment """[v] = a * [SI]
where
[v] is the value in newton per square metre per second
[SI] is the value in SI
a = 1.0/Unit, i.e., 1
and
Unit = 1.0
"""@EN; 
                                    rdfs:subClassOf ddhub:Unit. 
ddhub:NewtonPerSquareMillimetre a owl:Class; 
                                rdfs:comment """[v] = a * [SI]
where
[v] is the value in newton per square millimetre
[SI] is the value in SI
a = Milli*Milli, i.e., 1E-06
and
Milli = 0.001
"""@EN; 
                                rdfs:subClassOf ddhub:Unit. 
ddhub:NewtonPerSquareMillimetrePerHour a owl:Class; 
                                       rdfs:comment """[v] = a * [SI]
where
[v] is the value in newton per square millimetre per hour
[SI] is the value in SI
a = Hour*Milli*Milli, i.e., 0.0036000000000000003
and
Hour = 60.0 * Minute
Milli = 0.001
Minute = 60.0
"""@EN; 
                                       rdfs:subClassOf ddhub:Unit. 
ddhub:NewtonPerSquareMillimetrePerMinute a owl:Class; 
                                         rdfs:comment """[v] = a * [SI]
where
[v] is the value in newton per square millimetre per minute
[SI] is the value in SI
a = Minute*Milli*Milli, i.e., 6E-05
and
Minute = 60.0
Milli = 0.001
"""@EN; 
                                         rdfs:subClassOf ddhub:Unit. 
ddhub:NewtonPerSquareMillimetrePerSecond a owl:Class; 
                                         rdfs:comment """[v] = a * [SI]
where
[v] is the value in newton per square millimetre per second
[SI] is the value in SI
a = Milli*Milli, i.e., 1E-06
and
Milli = 0.001
"""@EN; 
                                         rdfs:subClassOf ddhub:Unit. 
ddhub:Nonmagnetic a owl:Class; 
                  rdfs:comment ""@EN; 
                  rdfs:subClassOf ddhub:Stabilizers. 
ddhub:NonmagneticCollars a owl:Class; 
                         rdfs:comment ""@EN; 
                         rdfs:subClassOf ddhub:DrillString. 
ddhub:Nonrotating a owl:Class; 
                  rdfs:comment ""@EN; 
                  rdfs:subClassOf ddhub:Stabilizers. 
ddhub:NormalizedDataType a owl:Class; 
                         rdfs:comment """between 0 and 1
"""@EN; 
                         rdfs:subClassOf ddhub:ContinuousDataType. 
ddhub:NorthEastFrame a owl:Class; 
                     rdfs:comment ""@EN; 
                     rdfs:subClassOf ddhub:CartesianTwoDimensionalReferenceFrame. 
ddhub:NorthEastTVDFrame a owl:Class; 
                        rdfs:comment ""@EN; 
                        rdfs:subClassOf ddhub:CartesianThreeDimensionalReferenceFrame. 
ddhub:NozzleDiameterDrillingQuantity a owl:Class; 
                                     rdfs:comment """Length is a measure of distance.
The dimension of length is:
$$[L]$$.
The SI unit for **length** is: metre with the associated unit label $m$
The meaningful precision of small length is typically: 0.0001 m
The meaningful precision of nozzle diameter in the drilling context is typically: 0.0001 m
"""@EN; 
                                     rdfs:subClassOf ddhub:MeasurableQuantity. 
ddhub:Nozzles a owl:Class; 
              rdfs:comment ""@EN; 
              rdfs:subClassOf ddhub:DrillingBit. 
ddhub:NumberOfItems a owl:DatatypeProperty, owl:FunctionalProperty; 
                    rdfs:comment """
"""@EN; 
                    rdfs:domain ddhub:NumberOfItemsRangeExtraction; 
                    rdfs:range xsd:int. 
ddhub:NumberOfItemsRangeExtraction a owl:Class; 
                                   rdfs:comment ""@EN; 
                                   rdfs:subClassOf ddhub:RangeExtraction. 
ddhub:NumberOfRepeaters a owl:DatatypeProperty, owl:FunctionalProperty; 
                        rdfs:comment """The number of repeaters between the source of the signal and the receiver.
"""@EN; 
                        rdfs:domain ddhub:Telemetry; 
                        rdfs:range xsd:int. 
ddhub:NumberOfSampleMovingAverage a owl:Class; 
                                  rdfs:comment ""@EN; 
                                  rdfs:subClassOf ddhub:MovingAverage. 
ddhub:NumberOfSamples a owl:DatatypeProperty, owl:FunctionalProperty; 
                      rdfs:comment """
"""@EN; 
                      rdfs:domain ddhub:NumberOfSampleMovingAverage; 
                      rdfs:range xsd:int. 
ddhub:Octant a owl:Class; 
             rdfs:comment """[v] = a * [SI]
where
[v] is the value in octant
[SI] is the value in SI
a = 4.0/PI, i.e., 1.2732395447351628
"""@EN; 
             rdfs:subClassOf ddhub:Unit. 
ddhub:OhmMetre a owl:Class; 
               rdfs:comment """No conversion necessary as the unit choice is SI
"""@EN; 
               rdfs:subClassOf ddhub:Unit. 
ddhub:OilBasedMudObm a owl:Class; 
                     rdfs:comment ""@EN; 
                     rdfs:subClassOf ddhub:DrillingFluid. 
ddhub:OilBearing a owl:Class; 
                 rdfs:comment ""@EN; 
                 rdfs:subClassOf ddhub:DownholeMotor. 
ddhub:Omega a owl:DatatypeProperty, owl:FunctionalProperty; 
            rdfs:comment """solid angle exponent.
SI Unit: steradian (sr)
"""@EN; 
            rdfs:domain ddhub:Quantity; 
            rdfs:range xsd:double. 
ddhub:OnBottomDrillingFeature a owl:Class; 
                              rdfs:comment """An on bottom drilling feature indicates that something accounts for on bottom drilling.
"""@EN; 
                              rdfs:subClassOf ddhub:DrillingManagementFeature. 
ddhub:OneDimensionalCartesianReferenceFrame a owl:Class; 
                                            rdfs:comment ""@EN; 
                                            rdfs:subClassOf ddhub:OneDimensionalReferenceFrame. 
ddhub:OneDimensionalCurviLinearReferenceFrame a owl:Class; 
                                              rdfs:comment ""@EN; 
                                              rdfs:subClassOf ddhub:OneDimensionalReferenceFrame. 
ddhub:OneDimensionalReferenceFrame a owl:Class; 
                                   rdfs:comment ""@EN; 
                                   rdfs:subClassOf ddhub:ReferenceFrame. 
ddhub:OneDModelling a owl:Class; 
                    rdfs:comment """The model only accounts for one dimension
"""@EN; 
                    rdfs:subClassOf ddhub:ModellingDimensions. 
ddhub:OnlyLimits a owl:Class; 
                 rdfs:comment """This noun states that something works with only limits, for example excluding the relation to set-points, etc.
"""@EN; 
                 rdfs:subClassOf ddhub:DrillingLimit. 
ddhub:OpenChannel a owl:Class; 
                  rdfs:comment ""@EN; 
                  rdfs:subClassOf ddhub:HydraulicBranch. 
ddhub:OpenHole a owl:Class; 
               rdfs:comment ""@EN; 
               rdfs:subClassOf ddhub:Pipe. 
ddhub:OpenholeTools a owl:Class; 
                    rdfs:comment ""@EN; 
                    rdfs:subClassOf ddhub:WirelineLoggingTools. 
ddhub:OperatingCompany a owl:Class; 
                       rdfs:comment """An operating company is an entity that holds the rights to explore, develop, and produce hydrocarbon resources from a particular oil or gas field or lease
"""@EN; 
                       rdfs:subClassOf ddhub:DataProvider. 
ddhub:OperationalPlan a owl:Class; 
                      rdfs:comment """An operational plan is the day-to-day list of activities that shall be performed to contruct a well.
"""@EN; 
                      rdfs:subClassOf ddhub:Plan. 
ddhub:OperationalStep a owl:Class; 
                      rdfs:comment """An operation step is a possible element of a rig action plan.
"""@EN; 
                      rdfs:subClassOf ddhub:ContextualData. 
ddhub:OrdinaryDifferentialEquationModel a owl:Class; 
                                        rdfs:comment """A model that uses ordinary differential equations.
"""@EN; 
                                        rdfs:subClassOf ddhub:MathematicalFormulation. 
ddhub:Ounce a owl:Class; 
            rdfs:comment """[v] = a * [SI]
where
[v] is the value in ounce
[SI] is the value in SI
a = 1.0/Ounce, i.e., 35.27396194958041
and
Ounce = (1.0 / 16.0) * Pound reference: https://en.wikipedia.org/wiki/Ounce
Pound = 0.45359237 reference: https://en.wikipedia.org/wiki/Pound_(mass)
"""@EN; 
            rdfs:subClassOf ddhub:Unit. 
ddhub:OuterBarrel a owl:Class; 
                  rdfs:comment ""@EN; 
                  rdfs:subClassOf ddhub:CoringTool. 
ddhub:OverburdenPressure a owl:Class; 
                         rdfs:comment ""@EN; 
                         rdfs:subClassOf ddhub:PrototypeData. 
ddhub:OverburdenPressureGradient a owl:Class; 
                                 rdfs:comment ""@EN; 
                                 rdfs:subClassOf ddhub:PrototypeData. 
ddhub:Overpull a owl:Class; 
               rdfs:comment """This Noun is used to refer to a situation during which the drill-stem hangs in something in the upward direction.
"""@EN; 
               rdfs:subClassOf ddhub:DrillingIncident. 
ddhub:Overshot a owl:Class; 
               rdfs:comment ""@EN; 
               rdfs:subClassOf ddhub:FishingTools. 
ddhub:OverTorque a owl:Class; 
                 rdfs:comment """This Noun is used to refer to a situation during which the rotation of the drill-stem is impeded.
"""@EN; 
                 rdfs:subClassOf ddhub:DrillingIncident. 
ddhub:PackOff a owl:Class; 
              rdfs:comment """This Noun is used to refer to a situation during which the annulus hydraulic flow-path is partially or fully blocked.
"""@EN; 
              rdfs:subClassOf ddhub:Plugged. 
ddhub:PackOffFeature a owl:Class; 
                     rdfs:comment """A pack-off feature indicates that something accounts for the possibility to pack-off while circulating cuttings.
"""@EN; 
                     rdfs:subClassOf ddhub:CuttingsTransportFeature. 
ddhub:Parsec a owl:Class; 
             rdfs:comment """[v] = a * [SI]
where
[v] is the value in parsec
[SI] is the value in SI
a = 1.0/Parsec, i.e., 3.240779289444365E-17
and
Parsec = (60.0*60.0*180.0 / System.Math.PI) * AstronomicalUnit reference: https://imagine.gsfc.nasa.gov/features/cosmic/milkyway_info.html
AstronomicalUnit = 149597870700.0 reference: https://www.iau.org/static/resolutions/IAU2012_English.pdf
"""@EN; 
             rdfs:subClassOf ddhub:Unit. 
ddhub:PartialDifferentialEquationModel a owl:Class; 
                                       rdfs:comment """A model that uses partial differential equations.
"""@EN; 
                                       rdfs:subClassOf ddhub:MathematicalFormulation. 
ddhub:PartPerMillion a owl:Class; 
                     rdfs:comment """[v] = a * [SI]
where
[v] is the value in part per million
[SI] is the value in SI
a = 1.0/Micro, i.e., 1000000
and
Micro = 1e-6
"""@EN; 
                     rdfs:subClassOf ddhub:Unit. 
ddhub:Pascal a owl:Class; 
             rdfs:comment """No conversion necessary as the unit choice is SI
"""@EN; 
             rdfs:subClassOf ddhub:Unit. 
ddhub:PascalPerHour a owl:Class; 
                    rdfs:comment """No conversion necessary as the unit choice is SI
"""@EN; 
                    rdfs:subClassOf ddhub:Unit. 
ddhub:PascalPerMetre a owl:Class; 
                     rdfs:comment """No conversion necessary as the unit choice is SI
"""@EN; 
                     rdfs:subClassOf ddhub:Unit. 
ddhub:PascalPerMinute a owl:Class; 
                      rdfs:comment """No conversion necessary as the unit choice is SI
"""@EN; 
                      rdfs:subClassOf ddhub:Unit. 
ddhub:PascalPerSecond a owl:Class; 
                      rdfs:comment """No conversion necessary as the unit choice is SI
"""@EN; 
                      rdfs:subClassOf ddhub:Unit. 
ddhub:PascalSecond a owl:Class; 
                   rdfs:comment """No conversion necessary as the unit choice is SI
"""@EN; 
                   rdfs:subClassOf ddhub:Unit. 
ddhub:Pdc a owl:Class; 
          rdfs:comment ""@EN; 
          rdfs:subClassOf ddhub:FixedCutter. 
ddhub:PdcCore a owl:Class; 
              rdfs:comment ""@EN; 
              rdfs:subClassOf ddhub:FixedCutter. 
ddhub:Percent a owl:Class; 
              rdfs:comment """[v] = a * [SI]
where
[v] is the value in percent
[SI] is the value in SI
a = 1.0/Centi, i.e., 100
and
Centi = 0.01
"""@EN; 
              rdfs:subClassOf ddhub:Unit. 
ddhub:PerforatingGuns a owl:Class; 
                      rdfs:comment ""@EN; 
                      rdfs:subClassOf ddhub:CasingEquipment. 
ddhub:PeristalticMudPump a owl:Class; 
                         rdfs:comment ""@EN; 
                         rdfs:subClassOf ddhub:MudPump. 
ddhub:PerThousand a owl:Class; 
                  rdfs:comment """[v] = a * [SI]
where
[v] is the value in per thousand
[SI] is the value in SI
a = 1.0/Milli, i.e., 1000
and
Milli = 0.001
"""@EN; 
                  rdfs:subClassOf ddhub:Unit. 
ddhub:Petawatt a owl:Class; 
               rdfs:comment """[v] = a * [SI]
where
[v] is the value in petawatt
[SI] is the value in SI
a = 1.0/Peta, i.e., 1E-15
and
Peta = 1e15
"""@EN; 
               rdfs:subClassOf ddhub:Unit. 
ddhub:PhaseStep a owl:Class; 
                rdfs:comment """A phase step is at the first level of a rig action plan.
"""@EN; 
                rdfs:subClassOf ddhub:OperationalStep. 
ddhub:PhysicalData a owl:Class; 
                   rdfs:comment ""@EN; 
                   rdfs:subClassOf ddhub:DrillingDataPoint. 
ddhub:PhysicalState a owl:Class; 
                    rdfs:comment ""@EN; 
                    rdfs:subClassOf ddhub:ComputedState. 
ddhub:PhysicsInformedDataDrivenModel a owl:Class; 
                                     rdfs:comment """A hybrid model that uses both physical laws and data.
"""@EN; 
                                     rdfs:subClassOf ddhub:ModelingParadigm. 
ddhub:Picoampere a owl:Class; 
                 rdfs:comment """[v] = a * [SI]
where
[v] is the value in picoampere
[SI] is the value in SI
a = 1.0/Pico, i.e., 1000000000000
and
Pico = 1e-12
"""@EN; 
                 rdfs:subClassOf ddhub:Unit. 
ddhub:Picofarad a owl:Class; 
                rdfs:comment """[v] = a * [SI]
where
[v] is the value in picofarad
[SI] is the value in SI
a = 1.0/Pico, i.e., 1000000000000
and
Pico = 1e-12
"""@EN; 
                rdfs:subClassOf ddhub:Unit. 
ddhub:Picometre a owl:Class; 
                rdfs:comment """[v] = a * [SI]
where
[v] is the value in picometre
[SI] is the value in SI
a = 1.0/Pico, i.e., 1000000000000
and
Pico = 1e-12
"""@EN; 
                rdfs:subClassOf ddhub:Unit. 
ddhub:Picomole a owl:Class; 
               rdfs:comment """[v] = a * [SI]
where
[v] is the value in picomole
[SI] is the value in SI
a = 1.0/Pico, i.e., 1000000000000
and
Pico = 1e-12
"""@EN; 
               rdfs:subClassOf ddhub:Unit. 
ddhub:Picosecond a owl:Class; 
                 rdfs:comment """[v] = a * [SI]
where
[v] is the value in picosecond
[SI] is the value in SI
a = 1.0/Pico, i.e., 1000000000000
and
Pico = 1e-12
"""@EN; 
                 rdfs:subClassOf ddhub:Unit. 
ddhub:Picovolt a owl:Class; 
               rdfs:comment """[v] = a * [SI]
where
[v] is the value in picovolt
[SI] is the value in SI
a = 1.0/Pico, i.e., 1000000000000
and
Pico = 1e-12
"""@EN; 
               rdfs:subClassOf ddhub:Unit. 
ddhub:Picowatt a owl:Class; 
               rdfs:comment """[v] = a * [SI]
where
[v] is the value in picowatt
[SI] is the value in SI
a = 1.0/Pico, i.e., 1000000000000
and
Pico = 1e-12
"""@EN; 
               rdfs:subClassOf ddhub:Unit. 
ddhub:Pin a owl:Class; 
          rdfs:comment ""@EN; 
          rdfs:subClassOf ddhub:Connection. 
ddhub:PinDown a owl:Class; 
              rdfs:comment ""@EN; 
              rdfs:subClassOf ddhub:TubularConfiguration. 
ddhub:Pinpin a owl:Class; 
             rdfs:comment ""@EN; 
             rdfs:subClassOf ddhub:TubularConfiguration. 
ddhub:PinUp a owl:Class; 
            rdfs:comment ""@EN; 
            rdfs:subClassOf ddhub:TubularConfiguration. 
ddhub:Pipe a owl:Class; 
           rdfs:comment ""@EN; 
           rdfs:subClassOf ddhub:HydraulicBranch. 
ddhub:PipeRam a owl:Class; 
              rdfs:comment ""@EN; 
              rdfs:subClassOf ddhub:BopElement. 
ddhub:PipeWashout a owl:Class; 
                  rdfs:comment """This Noun is used to refer to a situation during which there is leak between the inside of the drill-stem and the annulus.
"""@EN; 
                  rdfs:subClassOf ddhub:DrillingIncident. 
ddhub:PipeWashoutLocation a owl:Class; 
                          rdfs:comment ""@EN; 
                          rdfs:subClassOf ddhub:AbscissaReferenceLocation. 
ddhub:Piston a owl:Class; 
             rdfs:comment ""@EN; 
             rdfs:subClassOf ddhub:PistonMudPump. 
ddhub:PistonMudPump a owl:Class; 
                    rdfs:comment ""@EN; 
                    rdfs:subClassOf ddhub:MudPump. 
ddhub:Plan a owl:Class; 
           rdfs:comment """A plan is a description of the actions that shall be undertaken to reach an objective
"""@EN; 
           rdfs:subClassOf ddhub:ContextualData. 
ddhub:PlaneAngleDrillingQuantity a owl:Class; 
                                 rdfs:comment """A plane angle is the angle formed between two intersecting lines or planes in a two-dimensional or three-dimensional space.
The dimension of plane angle is:
$$[{\\theta}]$$.
The SI unit for **plane angle** is: radian with the associated unit label $rad$
The meaningful precision of plane angle in the drilling context is typically: 0.00017453292519943296 rad
"""@EN; 
                                 rdfs:subClassOf ddhub:MeasurableQuantity. 
ddhub:PlaneAngleQuantity a owl:Class; 
                         rdfs:comment """A plane angle is the angle formed between two intersecting lines or planes in a two-dimensional or three-dimensional space.
The dimension of plane angle is:
$$[{\\theta}]$$.
The SI unit for **plane angle** is: radian with the associated unit label $rad$
"""@EN; 
                         rdfs:subClassOf ddhub:Quantity. 
ddhub:Planned a owl:Class; 
              rdfs:comment """Planned characterizes that the wellbore data is described in its planned stage. This applies to wellbore data
that is intended to be constructed.
"""@EN; 
              rdfs:subClassOf ddhub:WellBoreDataCharateristic. 
ddhub:Plugged a owl:Class; 
              rdfs:comment """This Noun is used to refer to a situation during which the hydraulic flow-path is partially or fully blocked.
"""@EN; 
              rdfs:subClassOf ddhub:DrillingIncident. 
ddhub:Plugs a owl:Class; 
            rdfs:comment ""@EN; 
            rdfs:subClassOf ddhub:CasingEquipment. 
ddhub:PlungerFloatValvesF a owl:Class; 
                          rdfs:comment ""@EN; 
                          rdfs:subClassOf ddhub:FloatValveNonreturnValve. 
ddhub:PlungerMudPump a owl:Class; 
                     rdfs:comment ""@EN; 
                     rdfs:subClassOf ddhub:MudPump. 
ddhub:PneumaticSlips a owl:Class; 
                     rdfs:comment ""@EN; 
                     rdfs:subClassOf ddhub:RotarySlips. 
ddhub:Pointthebit a owl:Class; 
                  rdfs:comment ""@EN; 
                  rdfs:subClassOf ddhub:RotarySteerableSystems. 
ddhub:Poise a owl:Class; 
            rdfs:comment """[v] = a * [SI]
where
[v] is the value in poise
[SI] is the value in SI
a = 1.0/Poise, i.e., 10
and
Poise = 0.1 reference: https://en.wikipedia.org/wiki/Poise_(unit)
"""@EN; 
            rdfs:subClassOf ddhub:Unit. 
ddhub:PolarReferenceFrame a owl:Class; 
                          rdfs:comment ""@EN; 
                          rdfs:subClassOf ddhub:TwoDimensionalReferenceFrame. 
ddhub:PorePressure a owl:Class; 
                   rdfs:comment ""@EN; 
                   rdfs:subClassOf ddhub:PrototypeData. 
ddhub:PorePressureGradient a owl:Class; 
                           rdfs:comment ""@EN; 
                           rdfs:subClassOf ddhub:PrototypeData. 
ddhub:PorosityQuantity a owl:Class; 
                       rdfs:comment """A proportion is the ratio of two quantities with the same dimension. It represents how one quantity compares to another in relative terms.
A proportion is dimensionless:
Porosity is the measure of the void spaces or pores within a material, expressed as a fraction or percentage of the total volume.
The meaningful precision of porosity is typically: 0.001 
"""@EN; 
                       rdfs:subClassOf ddhub:MeasurableQuantity. 
ddhub:PorousMediumPermeabilityDrillingQuantity a owl:Class; 
                                               rdfs:comment """The permeability is a property of porous medium that quantifies its ability to allow fluids to pass through it.
The dimension of porous medium permeability is:
$$[L^{2}]$$.
The SI unit for **porous medium permeability** is: square metre with the associated unit label $m^{2}$
The meaningful precision of permeability in the drilling context is typically: 1E-10 m²
"""@EN; 
                                               rdfs:subClassOf ddhub:MeasurableQuantity. 
ddhub:PorousMediumPermeabilityQuantity a owl:Class; 
                                       rdfs:comment """The permeability is a property of porous medium that quantifies its ability to allow fluids to pass through it.
The dimension of porous medium permeability is:
$$[L^{2}]$$.
The SI unit for **porous medium permeability** is: square metre with the associated unit label $m^{2}$
"""@EN; 
                                       rdfs:subClassOf ddhub:Quantity. 
ddhub:PortedPlungerValvesFa a owl:Class; 
                            rdfs:comment ""@EN; 
                            rdfs:subClassOf ddhub:FloatValveNonreturnValve. 
ddhub:PositionDrillingQuantity a owl:Class; 
                               rdfs:comment """Length is a measure of distance.
The dimension of length is:
$$[L]$$.
The SI unit for **length** is: metre with the associated unit label $m$
The meaningful precision of position in the drilling context is typically: 0.01 m
"""@EN; 
                               rdfs:subClassOf ddhub:MeasurableQuantity. 
ddhub:PositionReferenceLocation a owl:Class; 
                                rdfs:comment ""@EN; 
                                rdfs:subClassOf ddhub:Location. 
ddhub:PositiveDisplacementMotor a owl:Class; 
                                rdfs:comment ""@EN; 
                                rdfs:subClassOf ddhub:DownholeMotor. 
ddhub:PostiveUpward a owl:DatatypeProperty, owl:FunctionalProperty; 
                    rdfs:comment """
"""@EN; 
                    rdfs:domain ddhub:OneDimensionalReferenceFrame; 
                    rdfs:range xsd:bool. 
ddhub:PotableWater a owl:Class; 
                   rdfs:comment ""@EN; 
                   rdfs:subClassOf ddhub:DrillingFluid. 
ddhub:Pound a owl:Class; 
            rdfs:comment """[v] = a * [SI]
where
[v] is the value in pound
[SI] is the value in SI
a = 1.0/Pound, i.e., 2.2046226218487757
and
Pound = 0.45359237 reference: https://en.wikipedia.org/wiki/Pound_(mass)
"""@EN; 
            rdfs:subClassOf ddhub:Unit. 
ddhub:PoundForce a owl:Class; 
                 rdfs:comment """[v] = a * [SI]
where
[v] is the value in pound force
[SI] is the value in SI
a = 1.0/PoundForce, i.e., 0.2248089430997105
and
PoundForce = Pound * G reference: https://en.wikipedia.org/wiki/Pound_(force)
Pound = 0.45359237 reference: https://en.wikipedia.org/wiki/Pound_(mass)
G = 9.80665 reference: https://en.wikipedia.org/wiki/Gravity_of_Earth
"""@EN; 
                 rdfs:subClassOf ddhub:Unit. 
ddhub:PoundForcePerHour a owl:Class; 
                        rdfs:comment """[v] = a * [SI]
where
[v] is the value in pound force per hour
[SI] is the value in SI
a = Hour/PoundForce, i.e., 809.3121951589578
and
Hour = 60.0 * Minute
PoundForce = Pound * G reference: https://en.wikipedia.org/wiki/Pound_(force)
Minute = 60.0
Pound = 0.45359237 reference: https://en.wikipedia.org/wiki/Pound_(mass)
G = 9.80665 reference: https://en.wikipedia.org/wiki/Gravity_of_Earth
"""@EN; 
                        rdfs:subClassOf ddhub:Unit. 
ddhub:PoundForcePerMinute a owl:Class; 
                          rdfs:comment """[v] = a * [SI]
where
[v] is the value in pound force per minute
[SI] is the value in SI
a = Minute/PoundForce, i.e., 13.48853658598263
and
Minute = 60.0
PoundForce = Pound * G reference: https://en.wikipedia.org/wiki/Pound_(force)
Pound = 0.45359237 reference: https://en.wikipedia.org/wiki/Pound_(mass)
G = 9.80665 reference: https://en.wikipedia.org/wiki/Gravity_of_Earth
"""@EN; 
                          rdfs:subClassOf ddhub:Unit. 
ddhub:PoundForcePerSecond a owl:Class; 
                          rdfs:comment """[v] = a * [SI]
where
[v] is the value in pound force per second
[SI] is the value in SI
a = 1.0/PoundForce, i.e., 0.2248089430997105
and
PoundForce = Pound * G reference: https://en.wikipedia.org/wiki/Pound_(force)
Pound = 0.45359237 reference: https://en.wikipedia.org/wiki/Pound_(mass)
G = 9.80665 reference: https://en.wikipedia.org/wiki/Gravity_of_Earth
"""@EN; 
                          rdfs:subClassOf ddhub:Unit. 
ddhub:PoundPer100Foot a owl:Class; 
                      rdfs:comment """[v] = a * [SI]
where
[v] is the value in pound per 100 foot
[SI] is the value in SI
a = 100.0*Foot/PoundForce, i.e., 6.852176585679175
and
Foot = 12.0 * Inch
PoundForce = Pound * G reference: https://en.wikipedia.org/wiki/Pound_(force)
Inch = 0.0254 reference: https://www.nist.gov/pml/owm/si-units-length
Pound = 0.45359237 reference: https://en.wikipedia.org/wiki/Pound_(mass)
G = 9.80665 reference: https://en.wikipedia.org/wiki/Gravity_of_Earth
"""@EN; 
                      rdfs:subClassOf ddhub:Unit. 
ddhub:PoundPer100SquareFoot a owl:Class; 
                            rdfs:comment """[v] = a * [SI]
where
[v] is the value in pound per 100 square foot
[SI] is the value in SI
a = 100.0*Foot*Foot/(PoundForce), i.e., 2.0885434233150124
and
Foot = 12.0 * Inch
PoundForce = Pound * G reference: https://en.wikipedia.org/wiki/Pound_(force)
Inch = 0.0254 reference: https://www.nist.gov/pml/owm/si-units-length
Pound = 0.45359237 reference: https://en.wikipedia.org/wiki/Pound_(mass)
G = 9.80665 reference: https://en.wikipedia.org/wiki/Gravity_of_Earth
"""@EN; 
                            rdfs:subClassOf ddhub:Unit. 
ddhub:PoundPer100SquareFootPerHour a owl:Class; 
                                   rdfs:comment """[v] = a * [SI]
where
[v] is the value in pound per 100 square foot per hour
[SI] is the value in SI
a = Hour*100.0*Foot*Foot/PoundForce, i.e., 7518.756323934045
and
Hour = 60.0 * Minute
Foot = 12.0 * Inch
PoundForce = Pound * G reference: https://en.wikipedia.org/wiki/Pound_(force)
Minute = 60.0
Inch = 0.0254 reference: https://www.nist.gov/pml/owm/si-units-length
Pound = 0.45359237 reference: https://en.wikipedia.org/wiki/Pound_(mass)
G = 9.80665 reference: https://en.wikipedia.org/wiki/Gravity_of_Earth
"""@EN; 
                                   rdfs:subClassOf ddhub:Unit. 
ddhub:PoundPer100SquareFootPerMinute a owl:Class; 
                                     rdfs:comment """[v] = a * [SI]
where
[v] is the value in pound per 100 square foot per minute
[SI] is the value in SI
a = Minute*100.0*Foot*Foot/PoundForce, i.e., 125.31260539890074
and
Minute = 60.0
Foot = 12.0 * Inch
PoundForce = Pound * G reference: https://en.wikipedia.org/wiki/Pound_(force)
Inch = 0.0254 reference: https://www.nist.gov/pml/owm/si-units-length
Pound = 0.45359237 reference: https://en.wikipedia.org/wiki/Pound_(mass)
G = 9.80665 reference: https://en.wikipedia.org/wiki/Gravity_of_Earth
"""@EN; 
                                     rdfs:subClassOf ddhub:Unit. 
ddhub:PoundPer100SquareFootPerSecond a owl:Class; 
                                     rdfs:comment """[v] = a * [SI]
where
[v] is the value in pound per 100 square foot per second
[SI] is the value in SI
a = 100.0*Foot*Foot/PoundForce, i.e., 2.0885434233150124
and
Foot = 12.0 * Inch
PoundForce = Pound * G reference: https://en.wikipedia.org/wiki/Pound_(force)
Inch = 0.0254 reference: https://www.nist.gov/pml/owm/si-units-length
Pound = 0.45359237 reference: https://en.wikipedia.org/wiki/Pound_(mass)
G = 9.80665 reference: https://en.wikipedia.org/wiki/Gravity_of_Earth
"""@EN; 
                                     rdfs:subClassOf ddhub:Unit. 
ddhub:PoundPer30Foot a owl:Class; 
                     rdfs:comment """[v] = a * [SI]
where
[v] is the value in pound per 30 foot
[SI] is the value in SI
a = 30.0*Foot/PoundForce, i.e., 2.0556529757037523
and
Foot = 12.0 * Inch
PoundForce = Pound * G reference: https://en.wikipedia.org/wiki/Pound_(force)
Inch = 0.0254 reference: https://www.nist.gov/pml/owm/si-units-length
Pound = 0.45359237 reference: https://en.wikipedia.org/wiki/Pound_(mass)
G = 9.80665 reference: https://en.wikipedia.org/wiki/Gravity_of_Earth
"""@EN; 
                     rdfs:subClassOf ddhub:Unit. 
ddhub:PoundPerCubicFoot a owl:Class; 
                        rdfs:comment """[v] = a * [SI]
where
[v] is the value in pound per cubic foot
[SI] is the value in SI
a = Foot*Foot*Foot/Pound, i.e., 0.06242796057614459
and
Foot = 12.0 * Inch
Pound = 0.45359237 reference: https://en.wikipedia.org/wiki/Pound_(mass)
Inch = 0.0254 reference: https://www.nist.gov/pml/owm/si-units-length
"""@EN; 
                        rdfs:subClassOf ddhub:Unit. 
ddhub:PoundPerCubicFootPer100Foot a owl:Class; 
                                  rdfs:comment """[v] = a * [SI]
where
[v] is the value in pound per cubic foot per 100 foot
[SI] is the value in SI
a = Foot*Foot*Foot*100.0*Foot/Pound, i.e., 1.902804238360887
and
Foot = 12.0 * Inch
Pound = 0.45359237 reference: https://en.wikipedia.org/wiki/Pound_(mass)
Inch = 0.0254 reference: https://www.nist.gov/pml/owm/si-units-length
"""@EN; 
                                  rdfs:subClassOf ddhub:Unit. 
ddhub:PoundPerCubicFootPer30Foot a owl:Class; 
                                 rdfs:comment """[v] = a * [SI]
where
[v] is the value in pound per cubic foot per 30 foot
[SI] is the value in SI
a = Foot*Foot*Foot*30.0*Foot/Pound, i.e., 0.570841271508266
and
Foot = 12.0 * Inch
Pound = 0.45359237 reference: https://en.wikipedia.org/wiki/Pound_(mass)
Inch = 0.0254 reference: https://www.nist.gov/pml/owm/si-units-length
"""@EN; 
                                 rdfs:subClassOf ddhub:Unit. 
ddhub:PoundPerCubicFootPerCelsius a owl:Class; 
                                  rdfs:comment """[v] = a * [SI]
where
[v] is the value in pound per cubic foot per celsius
[SI] is the value in SI
a = Foot*Foot*Foot/Pound, i.e., 0.06242796057614459
and
Foot = 12.0 * Inch
Pound = 0.45359237 reference: https://en.wikipedia.org/wiki/Pound_(mass)
Inch = 0.0254 reference: https://www.nist.gov/pml/owm/si-units-length
"""@EN; 
                                  rdfs:subClassOf ddhub:Unit. 
ddhub:PoundPerCubicFootPerFahrenheit a owl:Class; 
                                     rdfs:comment """[v] = a * [SI]
where
[v] is the value in pound per cubic foot per fahrenheit
[SI] is the value in SI
a = Foot*Foot*Foot*FahrenheitSlope/Pound, i.e., 0.03468220032008033
and
Foot = 12.0 * Inch
FahrenheitSlope = 5.0 / 9.0 reference: https://nn.wikipedia.org/wiki/Fahrenheit
Pound = 0.45359237 reference: https://en.wikipedia.org/wiki/Pound_(mass)
Inch = 0.0254 reference: https://www.nist.gov/pml/owm/si-units-length
"""@EN; 
                                     rdfs:subClassOf ddhub:Unit. 
ddhub:PoundPerCubicFootPerFoot a owl:Class; 
                               rdfs:comment """[v] = a * [SI]
where
[v] is the value in pound per cubic foot per foot
[SI] is the value in SI
a = Foot*Foot*Foot*Foot/Pound, i.e., 0.019028042383608865
and
Foot = 12.0 * Inch
Pound = 0.45359237 reference: https://en.wikipedia.org/wiki/Pound_(mass)
Inch = 0.0254 reference: https://www.nist.gov/pml/owm/si-units-length
"""@EN; 
                               rdfs:subClassOf ddhub:Unit. 
ddhub:PoundPerCubicInch a owl:Class; 
                        rdfs:comment """[v] = a * [SI]
where
[v] is the value in pound per cubic inch
[SI] is the value in SI
a = Inch*Inch*Inch/Pound, i.e., 3.612729200008369E-05
and
Inch = 0.0254 reference: https://www.nist.gov/pml/owm/si-units-length
Pound = 0.45359237 reference: https://en.wikipedia.org/wiki/Pound_(mass)
"""@EN; 
                        rdfs:subClassOf ddhub:Unit. 
ddhub:PoundPerCubicInchPer100Foot a owl:Class; 
                                  rdfs:comment """[v] = a * [SI]
where
[v] is the value in pound per cubic inch per 100 foot
[SI] is the value in SI
a = Inch*Inch*Inch*100.0*Foot/Pound, i.e., 0.0011011598601625506
and
Inch = 0.0254 reference: https://www.nist.gov/pml/owm/si-units-length
Foot = 12.0 * Inch
Pound = 0.45359237 reference: https://en.wikipedia.org/wiki/Pound_(mass)
"""@EN; 
                                  rdfs:subClassOf ddhub:Unit. 
ddhub:PoundPerCubicInchPer30Foot a owl:Class; 
                                 rdfs:comment """[v] = a * [SI]
where
[v] is the value in pound per cubic inch per 30 foot
[SI] is the value in SI
a = Inch*Inch*Inch*30.0*Foot/Pound, i.e., 0.00033034795804876514
and
Inch = 0.0254 reference: https://www.nist.gov/pml/owm/si-units-length
Foot = 12.0 * Inch
Pound = 0.45359237 reference: https://en.wikipedia.org/wiki/Pound_(mass)
"""@EN; 
                                 rdfs:subClassOf ddhub:Unit. 
ddhub:PoundPerCubicInchPerCelsius a owl:Class; 
                                  rdfs:comment """[v] = a * [SI]
where
[v] is the value in pound per cubic inch per celsius
[SI] is the value in SI
a = Inch*Inch*Inch/Pound, i.e., 3.612729200008369E-05
and
Inch = 0.0254 reference: https://www.nist.gov/pml/owm/si-units-length
Pound = 0.45359237 reference: https://en.wikipedia.org/wiki/Pound_(mass)
"""@EN; 
                                  rdfs:subClassOf ddhub:Unit. 
ddhub:PoundPerCubicInchPerFahrenheit a owl:Class; 
                                     rdfs:comment """[v] = a * [SI]
where
[v] is the value in pound per cubic inch per fahrenheit
[SI] is the value in SI
a = Inch*Inch*Inch*FahrenheitSlope/Pound, i.e., 2.0070717777824268E-05
and
Inch = 0.0254 reference: https://www.nist.gov/pml/owm/si-units-length
FahrenheitSlope = 5.0 / 9.0 reference: https://nn.wikipedia.org/wiki/Fahrenheit
Pound = 0.45359237 reference: https://en.wikipedia.org/wiki/Pound_(mass)
"""@EN; 
                                     rdfs:subClassOf ddhub:Unit. 
ddhub:PoundPerCubicInchPerFoot a owl:Class; 
                               rdfs:comment """[v] = a * [SI]
where
[v] is the value in pound per cubic inch per foot
[SI] is the value in SI
a = Inch*Inch*Inch*Foot/Pound, i.e., 1.1011598601625506E-05
and
Inch = 0.0254 reference: https://www.nist.gov/pml/owm/si-units-length
Foot = 12.0 * Inch
Pound = 0.45359237 reference: https://en.wikipedia.org/wiki/Pound_(mass)
"""@EN; 
                               rdfs:subClassOf ddhub:Unit. 
ddhub:PoundPerCubicYard a owl:Class; 
                        rdfs:comment """[v] = a * [SI]
where
[v] is the value in pound per cubic yard
[SI] is the value in SI
a = Yard*Yard*Yard/Pound, i.e., 1.6855549355559039
and
Yard = 3.0 * Foot
Pound = 0.45359237 reference: https://en.wikipedia.org/wiki/Pound_(mass)
Foot = 12.0 * Inch
Inch = 0.0254 reference: https://www.nist.gov/pml/owm/si-units-length
"""@EN; 
                        rdfs:subClassOf ddhub:Unit. 
ddhub:PoundPerCubicYardPer100Foot a owl:Class; 
                                  rdfs:comment """[v] = a * [SI]
where
[v] is the value in pound per cubic yard per 100 foot
[SI] is the value in SI
a = Yard*Yard*Yard*100.0*Foot/Pound, i.e., 51.37571443574393
and
Yard = 3.0 * Foot
Foot = 12.0 * Inch
Pound = 0.45359237 reference: https://en.wikipedia.org/wiki/Pound_(mass)
Inch = 0.0254 reference: https://www.nist.gov/pml/owm/si-units-length
"""@EN; 
                                  rdfs:subClassOf ddhub:Unit. 
ddhub:PoundPerCubicYardPer30Foot a owl:Class; 
                                 rdfs:comment """[v] = a * [SI]
where
[v] is the value in pound per cubic yard per 30 foot
[SI] is the value in SI
a = Yard*Yard*Yard*30.0*Foot/Pound, i.e., 15.412714330723183
and
Yard = 3.0 * Foot
Foot = 12.0 * Inch
Pound = 0.45359237 reference: https://en.wikipedia.org/wiki/Pound_(mass)
Inch = 0.0254 reference: https://www.nist.gov/pml/owm/si-units-length
"""@EN; 
                                 rdfs:subClassOf ddhub:Unit. 
ddhub:PoundPerCubicYardPerCelsius a owl:Class; 
                                  rdfs:comment """[v] = a * [SI]
where
[v] is the value in pound per cubic yard per celsius
[SI] is the value in SI
a = Yard*Yard*Yard/Pound, i.e., 1.6855549355559039
and
Yard = 3.0 * Foot
Pound = 0.45359237 reference: https://en.wikipedia.org/wiki/Pound_(mass)
Foot = 12.0 * Inch
Inch = 0.0254 reference: https://www.nist.gov/pml/owm/si-units-length
"""@EN; 
                                  rdfs:subClassOf ddhub:Unit. 
ddhub:PoundPerCubicYardPerFoot a owl:Class; 
                               rdfs:comment """[v] = a * [SI]
where
[v] is the value in pound per cubic yard per foot
[SI] is the value in SI
a = Yard*Yard*Yard*Foot/Pound, i.e., 0.5137571443574394
and
Yard = 3.0 * Foot
Foot = 12.0 * Inch
Pound = 0.45359237 reference: https://en.wikipedia.org/wiki/Pound_(mass)
Inch = 0.0254 reference: https://www.nist.gov/pml/owm/si-units-length
"""@EN; 
                               rdfs:subClassOf ddhub:Unit. 
ddhub:PoundPerCubicYeardPerFahrenheit a owl:Class; 
                                      rdfs:comment """[v] = a * [SI]
where
[v] is the value in pound per cubic yeard per fahrenheit
[SI] is the value in SI
a = Yard*Yard*Yard*FahrenheitSlope/Pound, i.e., 0.9364194086421688
and
Yard = 3.0 * Foot
FahrenheitSlope = 5.0 / 9.0 reference: https://nn.wikipedia.org/wiki/Fahrenheit
Pound = 0.45359237 reference: https://en.wikipedia.org/wiki/Pound_(mass)
Foot = 12.0 * Inch
Inch = 0.0254 reference: https://www.nist.gov/pml/owm/si-units-length
"""@EN; 
                                      rdfs:subClassOf ddhub:Unit. 
ddhub:PoundPerFoot a owl:Class; 
                   rdfs:comment """[v] = a * [SI]
where
[v] is the value in pound per foot
[SI] is the value in SI
a = Foot/PoundForce, i.e., 0.06852176585679175
and
Foot = 12.0 * Inch
PoundForce = Pound * G reference: https://en.wikipedia.org/wiki/Pound_(force)
Inch = 0.0254 reference: https://www.nist.gov/pml/owm/si-units-length
Pound = 0.45359237 reference: https://en.wikipedia.org/wiki/Pound_(mass)
G = 9.80665 reference: https://en.wikipedia.org/wiki/Gravity_of_Earth
"""@EN; 
                   rdfs:subClassOf ddhub:Unit. 
ddhub:PoundPerGallonUk a owl:Class; 
                       rdfs:comment """[v] = a * [SI]
where
[v] is the value in pound per gallon (UK)
[SI] is the value in SI
a = 1.0/PPGUK, i.e., 0.010022412854960501
and
PPGUK = Pound / GallonUK
Pound = 0.45359237 reference: https://en.wikipedia.org/wiki/Pound_(mass)
GallonUK = 4.54609e-3 reference: https://en.wikipedia.org/wiki/Gallon
"""@EN; 
                       rdfs:subClassOf ddhub:Unit. 
ddhub:PoundPerGallonUkPer100Foot a owl:Class; 
                                 rdfs:comment """[v] = a * [SI]
where
[v] is the value in pound per gallon (UK) per 100 foot
[SI] is the value in SI
a = GallonUK*100.0*Foot/Pound, i.e., 0.305483143819196
and
GallonUK = 4.54609e-3 reference: https://en.wikipedia.org/wiki/Gallon
Foot = 12.0 * Inch
Pound = 0.45359237 reference: https://en.wikipedia.org/wiki/Pound_(mass)
Inch = 0.0254 reference: https://www.nist.gov/pml/owm/si-units-length
"""@EN; 
                                 rdfs:subClassOf ddhub:Unit. 
ddhub:PoundPerGallonUkPer30Foot a owl:Class; 
                                rdfs:comment """[v] = a * [SI]
where
[v] is the value in pound per gallon (UK) per 30 foot
[SI] is the value in SI
a = GallonUK*30.0*Foot/Pound, i.e., 0.0916449431457588
and
GallonUK = 4.54609e-3 reference: https://en.wikipedia.org/wiki/Gallon
Foot = 12.0 * Inch
Pound = 0.45359237 reference: https://en.wikipedia.org/wiki/Pound_(mass)
Inch = 0.0254 reference: https://www.nist.gov/pml/owm/si-units-length
"""@EN; 
                                rdfs:subClassOf ddhub:Unit. 
ddhub:PoundPerGallonUkPerCelsius a owl:Class; 
                                 rdfs:comment """[v] = a * [SI]
where
[v] is the value in pound per gallon (UK) per celsius
[SI] is the value in SI
a = GallonUK/Pound, i.e., 0.010022412854960501
and
GallonUK = 4.54609e-3 reference: https://en.wikipedia.org/wiki/Gallon
Pound = 0.45359237 reference: https://en.wikipedia.org/wiki/Pound_(mass)
"""@EN; 
                                 rdfs:subClassOf ddhub:Unit. 
ddhub:PoundPerGallonUkPerFahrenheit a owl:Class; 
                                    rdfs:comment """[v] = a * [SI]
where
[v] is the value in pound per gallon (UK) per fahrenheit
[SI] is the value in SI
a = GallonUK*FahrenheitSlope/Pound, i.e., 0.005568007141644723
and
GallonUK = 4.54609e-3 reference: https://en.wikipedia.org/wiki/Gallon
FahrenheitSlope = 5.0 / 9.0 reference: https://nn.wikipedia.org/wiki/Fahrenheit
Pound = 0.45359237 reference: https://en.wikipedia.org/wiki/Pound_(mass)
"""@EN; 
                                    rdfs:subClassOf ddhub:Unit. 
ddhub:PoundPerGallonUkPerFoot a owl:Class; 
                              rdfs:comment """[v] = a * [SI]
where
[v] is the value in pound per gallon (UK) per foot
[SI] is the value in SI
a = GallonUK*Foot/Pound, i.e., 0.00305483143819196
and
GallonUK = 4.54609e-3 reference: https://en.wikipedia.org/wiki/Gallon
Foot = 12.0 * Inch
Pound = 0.45359237 reference: https://en.wikipedia.org/wiki/Pound_(mass)
Inch = 0.0254 reference: https://www.nist.gov/pml/owm/si-units-length
"""@EN; 
                              rdfs:subClassOf ddhub:Unit. 
ddhub:PoundPerGallonUkPerHour a owl:Class; 
                              rdfs:comment """[v] = a * [SI]
where
[v] is the value in pound per gallon (UK) per hour
[SI] is the value in SI
a = Hour / PPGUK, i.e., 36.08068627785781
and
Hour = 60.0 * Minute
PPGUK = Pound / GallonUK
Minute = 60.0
Pound = 0.45359237 reference: https://en.wikipedia.org/wiki/Pound_(mass)
GallonUK = 4.54609e-3 reference: https://en.wikipedia.org/wiki/Gallon
"""@EN; 
                              rdfs:subClassOf ddhub:Unit. 
ddhub:PoundPerGallonUkPerMinute a owl:Class; 
                                rdfs:comment """[v] = a * [SI]
where
[v] is the value in pound per gallon (UK) per minute
[SI] is the value in SI
a = Minute / PPGUK, i.e., 0.6013447712976301
and
Minute = 60.0
PPGUK = Pound / GallonUK
Pound = 0.45359237 reference: https://en.wikipedia.org/wiki/Pound_(mass)
GallonUK = 4.54609e-3 reference: https://en.wikipedia.org/wiki/Gallon
"""@EN; 
                                rdfs:subClassOf ddhub:Unit. 
ddhub:PoundPerGallonUkPerSecond a owl:Class; 
                                rdfs:comment """[v] = a * [SI]
where
[v] is the value in pound per gallon (UK) per second
[SI] is the value in SI
a = 1.0 / PPGUK, i.e., 0.010022412854960501
and
PPGUK = Pound / GallonUK
Pound = 0.45359237 reference: https://en.wikipedia.org/wiki/Pound_(mass)
GallonUK = 4.54609e-3 reference: https://en.wikipedia.org/wiki/Gallon
"""@EN; 
                                rdfs:subClassOf ddhub:Unit. 
ddhub:PoundPerGallonUs a owl:Class; 
                       rdfs:comment """[v] = a * [SI]
where
[v] is the value in pound per gallon (US)
[SI] is the value in SI
a = 1.0/PPGUS, i.e., 0.00834540445201933
and
PPGUS = Pound / GallonUS
Pound = 0.45359237 reference: https://en.wikipedia.org/wiki/Pound_(mass)
GallonUS = 231.0 * Inch * Inch * Inch reference: https://en.wikipedia.org/wiki/Gallon
Inch = 0.0254 reference: https://www.nist.gov/pml/owm/si-units-length
"""@EN; 
                       rdfs:subClassOf ddhub:Unit. 
ddhub:PoundPerGallonUsPer100Foot a owl:Class; 
                                 rdfs:comment """[v] = a * [SI]
where
[v] is the value in pound per gallon (US) per 100 foot
[SI] is the value in SI
a = GallonUS*100.0*Foot/Pound, i.e., 0.2543679276975492
and
GallonUS = 231.0 * Inch * Inch * Inch reference: https://en.wikipedia.org/wiki/Gallon
Foot = 12.0 * Inch
Pound = 0.45359237 reference: https://en.wikipedia.org/wiki/Pound_(mass)
Inch = 0.0254 reference: https://www.nist.gov/pml/owm/si-units-length
"""@EN; 
                                 rdfs:subClassOf ddhub:Unit. 
ddhub:PoundPerGallonUsPer30Foot a owl:Class; 
                                rdfs:comment """[v] = a * [SI]
where
[v] is the value in pound per gallon (US) per 30 foot
[SI] is the value in SI
a = GallonUS*30.0*Foot/Pound, i.e., 0.07631037830926475
and
GallonUS = 231.0 * Inch * Inch * Inch reference: https://en.wikipedia.org/wiki/Gallon
Foot = 12.0 * Inch
Pound = 0.45359237 reference: https://en.wikipedia.org/wiki/Pound_(mass)
Inch = 0.0254 reference: https://www.nist.gov/pml/owm/si-units-length
"""@EN; 
                                rdfs:subClassOf ddhub:Unit. 
ddhub:PoundPerGallonUsPerCelsius a owl:Class; 
                                 rdfs:comment """[v] = a * [SI]
where
[v] is the value in pound per gallon (US) per celsius
[SI] is the value in SI
a = GallonUS/Pound, i.e., 0.00834540445201933
and
GallonUS = 231.0 * Inch * Inch * Inch reference: https://en.wikipedia.org/wiki/Gallon
Pound = 0.45359237 reference: https://en.wikipedia.org/wiki/Pound_(mass)
Inch = 0.0254 reference: https://www.nist.gov/pml/owm/si-units-length
"""@EN; 
                                 rdfs:subClassOf ddhub:Unit. 
ddhub:PoundPerGallonUsPerFahrenheit a owl:Class; 
                                    rdfs:comment """[v] = a * [SI]
where
[v] is the value in pound per gallon (US) per fahrenheit
[SI] is the value in SI
a = GallonUS*FahrenheitSlope/Pound, i.e., 0.004636335806677406
and
GallonUS = 231.0 * Inch * Inch * Inch reference: https://en.wikipedia.org/wiki/Gallon
FahrenheitSlope = 5.0 / 9.0 reference: https://nn.wikipedia.org/wiki/Fahrenheit
Pound = 0.45359237 reference: https://en.wikipedia.org/wiki/Pound_(mass)
Inch = 0.0254 reference: https://www.nist.gov/pml/owm/si-units-length
"""@EN; 
                                    rdfs:subClassOf ddhub:Unit. 
ddhub:PoundPerGallonUsPerFoot a owl:Class; 
                              rdfs:comment """[v] = a * [SI]
where
[v] is the value in pound per gallon (US) per foot
[SI] is the value in SI
a = GallonUS*Foot/Pound, i.e., 0.0025436792769754917
and
GallonUS = 231.0 * Inch * Inch * Inch reference: https://en.wikipedia.org/wiki/Gallon
Foot = 12.0 * Inch
Pound = 0.45359237 reference: https://en.wikipedia.org/wiki/Pound_(mass)
Inch = 0.0254 reference: https://www.nist.gov/pml/owm/si-units-length
"""@EN; 
                              rdfs:subClassOf ddhub:Unit. 
ddhub:PoundPerGallonUsPerHour a owl:Class; 
                              rdfs:comment """[v] = a * [SI]
where
[v] is the value in pound per gallon (US) per hour
[SI] is the value in SI
a = Hour / PPGUS, i.e., 30.043456027269592
and
Hour = 60.0 * Minute
PPGUS = Pound / GallonUS
Minute = 60.0
Pound = 0.45359237 reference: https://en.wikipedia.org/wiki/Pound_(mass)
GallonUS = 231.0 * Inch * Inch * Inch reference: https://en.wikipedia.org/wiki/Gallon
Inch = 0.0254 reference: https://www.nist.gov/pml/owm/si-units-length
"""@EN; 
                              rdfs:subClassOf ddhub:Unit. 
ddhub:PoundPerGallonUsPerMinute a owl:Class; 
                                rdfs:comment """[v] = a * [SI]
where
[v] is the value in pound per gallon (US) per minute
[SI] is the value in SI
a = Minute / PPGUS, i.e., 0.5007242671211598
and
Minute = 60.0
PPGUS = Pound / GallonUS
Pound = 0.45359237 reference: https://en.wikipedia.org/wiki/Pound_(mass)
GallonUS = 231.0 * Inch * Inch * Inch reference: https://en.wikipedia.org/wiki/Gallon
Inch = 0.0254 reference: https://www.nist.gov/pml/owm/si-units-length
"""@EN; 
                                rdfs:subClassOf ddhub:Unit. 
ddhub:PoundPerGallonUsPerSecond a owl:Class; 
                                rdfs:comment """[v] = a * [SI]
where
[v] is the value in pound per gallon (US) per second
[SI] is the value in SI
a = 1.0 /PPGUS, i.e., 0.00834540445201933
and
PPGUS = Pound / GallonUS
Pound = 0.45359237 reference: https://en.wikipedia.org/wiki/Pound_(mass)
GallonUS = 231.0 * Inch * Inch * Inch reference: https://en.wikipedia.org/wiki/Gallon
Inch = 0.0254 reference: https://www.nist.gov/pml/owm/si-units-length
"""@EN; 
                                rdfs:subClassOf ddhub:Unit. 
ddhub:PoundPerHour a owl:Class; 
                   rdfs:comment """[v] = a * [SI]
where
[v] is the value in pound per hour
[SI] is the value in SI
a = Hour/Pound, i.e., 7936.6414386555925
and
Hour = 60.0 * Minute
Pound = 0.45359237 reference: https://en.wikipedia.org/wiki/Pound_(mass)
Minute = 60.0
"""@EN; 
                   rdfs:subClassOf ddhub:Unit. 
ddhub:PoundPerInch a owl:Class; 
                   rdfs:comment """[v] = a * [SI]
where
[v] is the value in pound per inch
[SI] is the value in SI
a = Inch/PoundForce, i.e., 0.0057101471547326465
and
Inch = 0.0254 reference: https://www.nist.gov/pml/owm/si-units-length
PoundForce = Pound * G reference: https://en.wikipedia.org/wiki/Pound_(force)
Pound = 0.45359237 reference: https://en.wikipedia.org/wiki/Pound_(mass)
G = 9.80665 reference: https://en.wikipedia.org/wiki/Gravity_of_Earth
"""@EN; 
                   rdfs:subClassOf ddhub:Unit. 
ddhub:PoundPerMinute a owl:Class; 
                     rdfs:comment """[v] = a * [SI]
where
[v] is the value in pound per minute
[SI] is the value in SI
a = Minute/Pound, i.e., 132.27735731092653
and
Minute = 60.0
Pound = 0.45359237 reference: https://en.wikipedia.org/wiki/Pound_(mass)
"""@EN; 
                     rdfs:subClassOf ddhub:Unit. 
ddhub:PoundPerSecond a owl:Class; 
                     rdfs:comment """[v] = a * [SI]
where
[v] is the value in pound per second
[SI] is the value in SI
a = Unit/Pound, i.e., 2.2046226218487757
and
Unit = 1.0
Pound = 0.45359237 reference: https://en.wikipedia.org/wiki/Pound_(mass)
"""@EN; 
                     rdfs:subClassOf ddhub:Unit. 
ddhub:PoundPerSecondSquared a owl:Class; 
                            rdfs:comment """[v] = a * [SI]
where
[v] is the value in pound per second squared
[SI] is the value in SI
a = 1.0/Pound, i.e., 2.2046226218487757
and
Pound = 0.45359237 reference: https://en.wikipedia.org/wiki/Pound_(mass)
"""@EN; 
                            rdfs:subClassOf ddhub:Unit. 
ddhub:PoundPerSquareFoot a owl:Class; 
                         rdfs:comment """[v] = a * [SI]
where
[v] is the value in pound per square foot
[SI] is the value in SI
a = Foot*Foot/PoundForce, i.e., 0.020885434233150126
and
Foot = 12.0 * Inch
PoundForce = Pound * G reference: https://en.wikipedia.org/wiki/Pound_(force)
Inch = 0.0254 reference: https://www.nist.gov/pml/owm/si-units-length
Pound = 0.45359237 reference: https://en.wikipedia.org/wiki/Pound_(mass)
G = 9.80665 reference: https://en.wikipedia.org/wiki/Gravity_of_Earth
"""@EN; 
                         rdfs:subClassOf ddhub:Unit. 
ddhub:PoundPerSquareFootPerHour a owl:Class; 
                                rdfs:comment """[v] = a * [SI]
where
[v] is the value in pound per square foot per hour
[SI] is the value in SI
a = Hour*Foot*Foot/PoundForce, i.e., 75.18756323934043
and
Hour = 60.0 * Minute
Foot = 12.0 * Inch
PoundForce = Pound * G reference: https://en.wikipedia.org/wiki/Pound_(force)
Minute = 60.0
Inch = 0.0254 reference: https://www.nist.gov/pml/owm/si-units-length
Pound = 0.45359237 reference: https://en.wikipedia.org/wiki/Pound_(mass)
G = 9.80665 reference: https://en.wikipedia.org/wiki/Gravity_of_Earth
"""@EN; 
                                rdfs:subClassOf ddhub:Unit. 
ddhub:PoundPerSquareFootPerMinute a owl:Class; 
                                  rdfs:comment """[v] = a * [SI]
where
[v] is the value in pound per square foot per minute
[SI] is the value in SI
a = Minute*Foot*Foot/PoundForce, i.e., 1.2531260539890072
and
Minute = 60.0
Foot = 12.0 * Inch
PoundForce = Pound * G reference: https://en.wikipedia.org/wiki/Pound_(force)
Inch = 0.0254 reference: https://www.nist.gov/pml/owm/si-units-length
Pound = 0.45359237 reference: https://en.wikipedia.org/wiki/Pound_(mass)
G = 9.80665 reference: https://en.wikipedia.org/wiki/Gravity_of_Earth
"""@EN; 
                                  rdfs:subClassOf ddhub:Unit. 
ddhub:PoundPerSquareFootPerSecond a owl:Class; 
                                  rdfs:comment """[v] = a * [SI]
where
[v] is the value in pound per square foot per second
[SI] is the value in SI
a = Foot*Foot/PoundForce, i.e., 0.020885434233150126
and
Foot = 12.0 * Inch
PoundForce = Pound * G reference: https://en.wikipedia.org/wiki/Pound_(force)
Inch = 0.0254 reference: https://www.nist.gov/pml/owm/si-units-length
Pound = 0.45359237 reference: https://en.wikipedia.org/wiki/Pound_(mass)
G = 9.80665 reference: https://en.wikipedia.org/wiki/Gravity_of_Earth
"""@EN; 
                                  rdfs:subClassOf ddhub:Unit. 
ddhub:PoundPerSquareInch a owl:Class; 
                         rdfs:comment """[v] = a * [SI]
where
[v] is the value in pound per square inch
[SI] is the value in SI
a = 1.0/PSI, i.e., 0.00014503773773020924
and
PSI = PoundForce / (Inch * Inch) reference: https://en.wikipedia.org/wiki/Pound_per_square_inch
PoundForce = Pound * G reference: https://en.wikipedia.org/wiki/Pound_(force)
Inch = 0.0254 reference: https://www.nist.gov/pml/owm/si-units-length
Pound = 0.45359237 reference: https://en.wikipedia.org/wiki/Pound_(mass)
G = 9.80665 reference: https://en.wikipedia.org/wiki/Gravity_of_Earth
"""@EN; 
                         rdfs:subClassOf ddhub:Unit. 
ddhub:PoundPerSquareInchPerHour a owl:Class; 
                                rdfs:comment """[v] = a * [SI]
where
[v] is the value in pound per square inch per hour
[SI] is the value in SI
a = Hour/PSI, i.e., 0.5221358558287532
and
Hour = 60.0 * Minute
PSI = PoundForce / (Inch * Inch) reference: https://en.wikipedia.org/wiki/Pound_per_square_inch
Minute = 60.0
PoundForce = Pound * G reference: https://en.wikipedia.org/wiki/Pound_(force)
Inch = 0.0254 reference: https://www.nist.gov/pml/owm/si-units-length
Pound = 0.45359237 reference: https://en.wikipedia.org/wiki/Pound_(mass)
G = 9.80665 reference: https://en.wikipedia.org/wiki/Gravity_of_Earth
"""@EN; 
                                rdfs:subClassOf ddhub:Unit. 
ddhub:PoundPerSquareInchPerMinute a owl:Class; 
                                  rdfs:comment """[v] = a * [SI]
where
[v] is the value in pound per square inch per minute
[SI] is the value in SI
a = Minute/PSI, i.e., 0.008702264263812553
and
Minute = 60.0
PSI = PoundForce / (Inch * Inch) reference: https://en.wikipedia.org/wiki/Pound_per_square_inch
PoundForce = Pound * G reference: https://en.wikipedia.org/wiki/Pound_(force)
Inch = 0.0254 reference: https://www.nist.gov/pml/owm/si-units-length
Pound = 0.45359237 reference: https://en.wikipedia.org/wiki/Pound_(mass)
G = 9.80665 reference: https://en.wikipedia.org/wiki/Gravity_of_Earth
"""@EN; 
                                  rdfs:subClassOf ddhub:Unit. 
ddhub:PoundPerSquareInchPerSecond a owl:Class; 
                                  rdfs:comment """[v] = a * [SI]
where
[v] is the value in pound per square inch per second
[SI] is the value in SI
a = 1.0/PSI, i.e., 0.00014503773773020924
and
PSI = PoundForce / (Inch * Inch) reference: https://en.wikipedia.org/wiki/Pound_per_square_inch
PoundForce = Pound * G reference: https://en.wikipedia.org/wiki/Pound_(force)
Inch = 0.0254 reference: https://www.nist.gov/pml/owm/si-units-length
Pound = 0.45359237 reference: https://en.wikipedia.org/wiki/Pound_(mass)
G = 9.80665 reference: https://en.wikipedia.org/wiki/Gravity_of_Earth
"""@EN; 
                                  rdfs:subClassOf ddhub:Unit. 
ddhub:PoundPerYear a owl:Class; 
                   rdfs:comment """[v] = a * [SI]
where
[v] is the value in pound per year
[SI] is the value in SI
a = YearJulian/Pound, i.e., 69572598.85125493
and
YearJulian = 365.25 * Day
Pound = 0.45359237 reference: https://en.wikipedia.org/wiki/Pound_(mass)
Day = 24.0 * Hour
Hour = 60.0 * Minute
Minute = 60.0
"""@EN; 
                   rdfs:subClassOf ddhub:Unit. 
ddhub:PoundSecondPer100SquareFoot a owl:Class; 
                                  rdfs:comment """[v] = a * [SI]
where
[v] is the value in pound second per 100 square foot
[SI] is the value in SI
a = (100.0*Foot*Foot)/(Pound * G), i.e., 2.0885434233150124
and
Foot = 12.0 * Inch
Pound = 0.45359237 reference: https://en.wikipedia.org/wiki/Pound_(mass)
G = 9.80665 reference: https://en.wikipedia.org/wiki/Gravity_of_Earth
Inch = 0.0254 reference: https://www.nist.gov/pml/owm/si-units-length
"""@EN; 
                                  rdfs:subClassOf ddhub:Unit. 
ddhub:PoundSecondPerSquareFoot a owl:Class; 
                               rdfs:comment """[v] = a * [SI]
where
[v] is the value in pound second per square foot
[SI] is the value in SI
a = (Foot*Foot)/(Pound * G), i.e., 0.020885434233150126
and
Foot = 12.0 * Inch
Pound = 0.45359237 reference: https://en.wikipedia.org/wiki/Pound_(mass)
G = 9.80665 reference: https://en.wikipedia.org/wiki/Gravity_of_Earth
Inch = 0.0254 reference: https://www.nist.gov/pml/owm/si-units-length
"""@EN; 
                               rdfs:subClassOf ddhub:Unit. 
ddhub:PoundSecondPerSquareInch a owl:Class; 
                               rdfs:comment """[v] = a * [SI]
where
[v] is the value in pound second per square inch
[SI] is the value in SI
a = (Inch*Inch)/(Pound * G), i.e., 0.0001450377377302092
and
Inch = 0.0254 reference: https://www.nist.gov/pml/owm/si-units-length
Pound = 0.45359237 reference: https://en.wikipedia.org/wiki/Pound_(mass)
G = 9.80665 reference: https://en.wikipedia.org/wiki/Gravity_of_Earth
"""@EN; 
                               rdfs:subClassOf ddhub:Unit. 
ddhub:PowerDrillingQuantity a owl:Class; 
                            rdfs:comment """Power is the rate at which work is done or energy is transferred over time.
The dimension of power is:
$$[L^{2}MT^{-3}]$$.
The SI unit for **power** is: watt with the associated unit label $W$
The meaningful precision of power in the drilling context is typically: 0.1 W
"""@EN; 
                            rdfs:subClassOf ddhub:MeasurableQuantity. 
ddhub:PowerGenerationSystem a owl:Class; 
                            rdfs:comment ""@EN; 
                            rdfs:subClassOf ddhub:RigEquipment. 
ddhub:PowerGenerators a owl:Class; 
                      rdfs:comment ""@EN; 
                      rdfs:subClassOf ddhub:PowerGenerationSystem. 
ddhub:PowerPipeTongs a owl:Class; 
                     rdfs:comment ""@EN; 
                     rdfs:subClassOf ddhub:DrillPipeTongs. 
ddhub:PowerQuantity a owl:Class; 
                    rdfs:comment """Power is the rate at which work is done or energy is transferred over time.
The dimension of power is:
$$[L^{2}MT^{-3}]$$.
The SI unit for **power** is: watt with the associated unit label $W$
"""@EN; 
                    rdfs:subClassOf ddhub:Quantity. 
ddhub:PowerScrSystem a owl:Class; 
                     rdfs:comment ""@EN; 
                     rdfs:subClassOf ddhub:PowerGenerationSystem. 
ddhub:PowerSlips a owl:Class; 
                 rdfs:comment ""@EN; 
                 rdfs:subClassOf ddhub:RotarySlips. 
ddhub:PowerSupply a owl:Class; 
                  rdfs:comment ""@EN; 
                  rdfs:subClassOf ddhub:CoiledTubingEquipment. 
ddhub:PowerSystems a owl:Class; 
                   rdfs:comment ""@EN; 
                   rdfs:subClassOf ddhub:LoggingEquipment. 
ddhub:Precision a owl:DatatypeProperty, owl:FunctionalProperty; 
                rdfs:comment """The standard deviation of the repetitive error component of the uncertainty of the sensor. The assumed mean value of the attached Gaussian distribution is the measured value. The value is expected to be in the same physical quantity as the sensor value.
"""@EN; 
                rdfs:domain ddhub:SensorUncertainty; 
                rdfs:range xsd:double. 
ddhub:PredictiveModel a owl:Class; 
                      rdfs:comment """A model that aims to forecast future behavior based on current data or conditions.
"""@EN; 
                      rdfs:subClassOf ddhub:ModelingObjective. 
ddhub:PressureDrillingQuantity a owl:Class; 
                               rdfs:comment """Pressure is the force applied per unit area on a surface.
The dimension of pressure is:
$$[ML^{-1}T^{-2}]$$.
The SI unit for **pressure** is: pascal with the associated unit label $Pa$
The meaningful precision of pressure in the drilling context is typically: 10000 Pa
"""@EN; 
                               rdfs:subClassOf ddhub:MeasurableQuantity. 
ddhub:PressureGradientPerLengthDrillingQuantity a owl:Class; 
                                                rdfs:comment """A pressure gradient per length is the first derivative of a pressure compared to a distance: $\\frac{dp}{ds}$, where $p$ is a pressure and $s$ is a distance.
The dimension of pressure gradient per length is:
$$[ML^{-2}T^{-2}]$$.
The SI unit for **pressure gradient per length** is: pascal per metre with the associated unit label $\\frac{Pa}{m}$
The meaningful precision of pressure gradient per length in the drilling context is typically: 10000 Pa/m
"""@EN; 
                                                rdfs:subClassOf ddhub:MeasurableQuantity. 
ddhub:PressureGradientPerLengthQuantity a owl:Class; 
                                        rdfs:comment """A pressure gradient per length is the first derivative of a pressure compared to a distance: $\\frac{dp}{ds}$, where $p$ is a pressure and $s$ is a distance.
The dimension of pressure gradient per length is:
$$[ML^{-2}T^{-2}]$$.
The SI unit for **pressure gradient per length** is: pascal per metre with the associated unit label $\\frac{Pa}{m}$
"""@EN; 
                                        rdfs:subClassOf ddhub:Quantity. 
ddhub:PressureIntegrityTestProcedure a owl:Class; 
                                     rdfs:comment """The pressure integrity test procedure is used to either check that the formation can hold the maximum expected downhole
pressure (formation integrity test) or to test the strength of the formation and the minimum horizontal stress (leak-off test and 
extended leakoff test). 
"""@EN; 
                                     rdfs:subClassOf ddhub:DrillingProcedure. 
ddhub:PressureLoggingTools a owl:Class; 
                           rdfs:comment ""@EN; 
                           rdfs:subClassOf ddhub:WirelineLoggingTools. 
ddhub:PressureLossConstantDrillingQuantity a owl:Class; 
                                           rdfs:comment """The pressure loss constant is a parameter used to quantify the resistance to flow in a system, such as a pipe or more complex tubulars, which leads to a reduction in pressure. It helps in calculating the pressure drop due to friction or other factors in fluid dynamics.
The dimension of pressure loss constant is:
$$[L^{4}]$$.
The SI unit for **pressure loss constant** is: pressure loss constant SI with the associated unit label $(\\frac{m^{3}}{s})^{2} \\cdot \\frac{(\\frac{kg}{m^{3}})}{Pa}$
The meaningful precision of pressure loss constant in the drilling context is typically: 0.1 (m³/s)²•(kg/m³)/Pa
"""@EN; 
                                           rdfs:subClassOf ddhub:MeasurableQuantity. 
ddhub:PressureLossConstantMetric a owl:Class; 
                                 rdfs:comment """[v] = a * [SI]
where
[v] is the value in pressure loss constant metric
[SI] is the value in SI
a = Minute*Minute*Bar*SpecificGavity4degC/(Milli*Milli), i.e., 360010080282.2479
and
Minute = 60.0
Bar = 1e5 reference: https://en.wikipedia.org/wiki/Bar_(unit)
SpecificGavity4degC = 1.0 / WaterDensity4degC1Atm
Milli = 0.001
WaterDensity4degC1Atm = 999.9720 reference: https://en.wikipedia.org/wiki/Relative_density
"""@EN; 
                                 rdfs:subClassOf ddhub:Unit. 
ddhub:PressureLossConstantQuantity a owl:Class; 
                                   rdfs:comment """The pressure loss constant is a parameter used to quantify the resistance to flow in a system, such as a pipe or more complex tubulars, which leads to a reduction in pressure. It helps in calculating the pressure drop due to friction or other factors in fluid dynamics.
The dimension of pressure loss constant is:
$$[L^{4}]$$.
The SI unit for **pressure loss constant** is: pressure loss constant SI with the associated unit label $(\\frac{m^{3}}{s})^{2} \\cdot \\frac{(\\frac{kg}{m^{3}})}{Pa}$
"""@EN; 
                                   rdfs:subClassOf ddhub:Quantity. 
ddhub:PressureLossConstantSi a owl:Class; 
                             rdfs:comment """No conversion necessary as the unit choice is SI
"""@EN; 
                             rdfs:subClassOf ddhub:Unit. 
ddhub:PressureLossConstantUk a owl:Class; 
                             rdfs:comment """[v] = a * [SI]
where
[v] is the value in pressure loss constant UK
[SI] is the value in SI
a = Minute*Minute*PSI/(PPGUK*GallonUK*GallonUK), i.e., 12036984846.853645
and
Minute = 60.0
PSI = PoundForce / (Inch * Inch) reference: https://en.wikipedia.org/wiki/Pound_per_square_inch
PPGUK = Pound / GallonUK
GallonUK = 4.54609e-3 reference: https://en.wikipedia.org/wiki/Gallon
PoundForce = Pound * G reference: https://en.wikipedia.org/wiki/Pound_(force)
Inch = 0.0254 reference: https://www.nist.gov/pml/owm/si-units-length
Pound = 0.45359237 reference: https://en.wikipedia.org/wiki/Pound_(mass)
G = 9.80665 reference: https://en.wikipedia.org/wiki/Gravity_of_Earth
"""@EN; 
                             rdfs:subClassOf ddhub:Unit. 
ddhub:PressureLossConstantUs a owl:Class; 
                             rdfs:comment """[v] = a * [SI]
where
[v] is the value in pressure loss constant US
[SI] is the value in SI
a = Minute*Minute*PSI/(PPGUS*GallonUS*GallonUS), i.e., 14455816055.131952
and
Minute = 60.0
PSI = PoundForce / (Inch * Inch) reference: https://en.wikipedia.org/wiki/Pound_per_square_inch
PPGUS = Pound / GallonUS
GallonUS = 231.0 * Inch * Inch * Inch reference: https://en.wikipedia.org/wiki/Gallon
PoundForce = Pound * G reference: https://en.wikipedia.org/wiki/Pound_(force)
Inch = 0.0254 reference: https://www.nist.gov/pml/owm/si-units-length
Pound = 0.45359237 reference: https://en.wikipedia.org/wiki/Pound_(mass)
G = 9.80665 reference: https://en.wikipedia.org/wiki/Gravity_of_Earth
"""@EN; 
                             rdfs:subClassOf ddhub:Unit. 
ddhub:PressureQuantity a owl:Class; 
                       rdfs:comment """Pressure is the force applied per unit area on a surface.
The dimension of pressure is:
$$[ML^{-1}T^{-2}]$$.
The SI unit for **pressure** is: pascal with the associated unit label $Pa$
"""@EN; 
                       rdfs:subClassOf ddhub:Quantity. 
ddhub:PressureRateOfChangeDrillingQuantity a owl:Class; 
                                           rdfs:comment """A pressure rate of change is the time derivative of a pressure.
The dimension of pressure rate of change is:
$$[ML^{-1}T^{-3}]$$.
The SI unit for **pressure rate of change** is: pascal per second with the associated unit label $\\frac{Pa}{s}$
The meaningful precision of pressure rate of change in the drilling context is typically: 10000 Pa/s
"""@EN; 
                                           rdfs:subClassOf ddhub:MeasurableQuantity. 
ddhub:PressureRateOfChangeQuantity a owl:Class; 
                                   rdfs:comment """A pressure rate of change is the time derivative of a pressure.
The dimension of pressure rate of change is:
$$[ML^{-1}T^{-3}]$$.
The SI unit for **pressure rate of change** is: pascal per second with the associated unit label $\\frac{Pa}{s}$
"""@EN; 
                                   rdfs:subClassOf ddhub:Quantity. 
ddhub:PressureReference a owl:Class; 
                        rdfs:comment ""@EN; 
                        rdfs:subClassOf ddhub:DWISNoun. 
ddhub:PressureToEquivalentDensityTransformation a owl:Class; 
                                                rdfs:comment ""@EN; 
                                                rdfs:subClassOf ddhub:DirectTransformation. 
ddhub:PressureToForceTransformation a owl:Class; 
                                    rdfs:comment ""@EN; 
                                    rdfs:subClassOf ddhub:DirectTransformation. 
ddhub:ProceduralState a owl:Class; 
                      rdfs:comment ""@EN; 
                      rdfs:subClassOf ddhub:ComputedState. 
ddhub:ProcedureFunction a owl:Class; 
                        rdfs:comment """A `ProcedureFunction` is a `RunnableFunction` that executes a finites state automaton, i.e., a graph of
transitions between states. It should be noted that a `ProcedureFunction` may use control algorithms while being in one
state or when transiting from state to state. An example of `ProcedureFunction` is a friction test. A friction test has
at least three states: rotation off bottom, pick-up without rotation, slack-off without rotation. The transitions 
between the different states may depend on the implementation. Each of those states uses a controller, one that controls
the rotational speed and one that controls the axial speed.
"""@EN; 
                        rdfs:subClassOf ddhub:RunnableFunction. 
ddhub:ProcessData a owl:Class; 
                  rdfs:comment ""@EN; 
                  rdfs:subClassOf ddhub:DrillingDataPoint. 
ddhub:ProcessFeature a owl:Class; 
                     rdfs:comment """This Noun is used for signals that describe a process feature, typically assuming that this is a static signal.
"""@EN; 
                     rdfs:subClassOf ddhub:ProcessData. 
ddhub:ProcessState a owl:Class; 
                   rdfs:comment ""@EN; 
                   rdfs:subClassOf ddhub:ComputedState. 
ddhub:ProductionStringDescription a owl:Class; 
                                  rdfs:comment """A production string is a drill-stem that is used to complete a wellbore. It is composed of tubings, expansion joints,
packers, etc.
"""@EN; 
                                  rdfs:subClassOf ddhub:DrillStemDescription. 
ddhub:ProductionTools a owl:Class; 
                      rdfs:comment ""@EN; 
                      rdfs:subClassOf ddhub:WirelineLoggingTools. 
ddhub:Prognosed a owl:Class; 
                rdfs:comment """Prognosed characterizes that the wellbore data is described in its prognosed stage. This applies to wellbore
data that exists from before but that may be associated with uncertainty like the geology.
"""@EN; 
                rdfs:subClassOf ddhub:WellBoreDataCharateristic. 
ddhub:Proportion a owl:Class; 
                 rdfs:comment """No conversion necessary as the unit choice is SI
"""@EN; 
                 rdfs:subClassOf ddhub:Unit. 
ddhub:ProportionError a owl:DatatypeProperty, owl:FunctionalProperty; 
                      rdfs:comment """The proportion error on the signal. The value is expected to be a dimensionless physical quantity between 0 and 1 in SI unit. This proportion is applied to the `Fullscale` to obtain the standard deviation of the Gaussian probability distribution that describes the uncertainty of the signal. The mean value of that Gaussian distribution is the signal value.
"""@EN; 
                      rdfs:domain ddhub:FullScaleUncertainty; 
                      rdfs:range xsd:double. 
ddhub:ProportionQuantity a owl:Class; 
                         rdfs:comment """A proportion is the ratio of two quantities with the same dimension. It represents how one quantity compares to another in relative terms.
A proportion is dimensionless:
"""@EN; 
                         rdfs:subClassOf ddhub:Quantity. 
ddhub:ProportionSmallQuantity a owl:Class; 
                              rdfs:comment """A proportion is the ratio of two quantities with the same dimension. It represents how one quantity compares to another in relative terms.
A proportion is dimensionless:
The meaningful precision of small proportion is typically: 1E-08 
"""@EN; 
                              rdfs:subClassOf ddhub:MeasurableQuantity. 
ddhub:ProportionStandardQuantity a owl:Class; 
                                 rdfs:comment """A proportion is the ratio of two quantities with the same dimension. It represents how one quantity compares to another in relative terms.
A proportion is dimensionless:
The meaningful precision of a standard proportion is typically: 0.001 
"""@EN; 
                                 rdfs:subClassOf ddhub:MeasurableQuantity. 
ddhub:ProtectionFunction a owl:Class; 
                         rdfs:comment """A `ProtectionFunction` is an `ActivableFunction`. It must be activated to have an effect, but the effect
is to protect the drilling process, either by protecting the inputs to the drilling machines to avoid generating 
a drilling incident, or to detect an abnormal drilling process state and react to the situation.
detected.
"""@EN; 
                         rdfs:subClassOf ddhub:ActivableFunction. 
ddhub:PrototypeData a owl:Class; 
                    rdfs:comment ""@EN; 
                    rdfs:subClassOf ddhub:DrillingDataPoint. 
ddhub:ProviderName a owl:DatatypeProperty, owl:FunctionalProperty; 
                   rdfs:comment """
"""@EN; 
                   rdfs:domain ddhub:DataProvider, ddhub:OperatingCompany, ddhub:ServiceCompany, ddhub:DirectionalServiceCompany, ddhub:DrillingFluidProvider, ddhub:LoggingServiceCompany, ddhub:CementingServiceCompany, ddhub:CompletionServiceCompany, ddhub:DataAnalysisServiceCompany, ddhub:DrillingContractor, ddhub:DWISInternalService; 
                   rdfs:range xsd:string. 
ddhub:Psi a owl:Class; 
          rdfs:comment """[v] = a * [SI]
where
[v] is the value in psi
[SI] is the value in SI
a = 1.0/PSI, i.e., 0.00014503773773020924
and
PSI = PoundForce / (Inch * Inch) reference: https://en.wikipedia.org/wiki/Pound_per_square_inch
PoundForce = Pound * G reference: https://en.wikipedia.org/wiki/Pound_(force)
Inch = 0.0254 reference: https://www.nist.gov/pml/owm/si-units-length
Pound = 0.45359237 reference: https://en.wikipedia.org/wiki/Pound_(mass)
G = 9.80665 reference: https://en.wikipedia.org/wiki/Gravity_of_Earth
"""@EN; 
          rdfs:subClassOf ddhub:Unit. 
ddhub:PsiPerFoot a owl:Class; 
                 rdfs:comment """[v] = a * [SI]
where
[v] is the value in psi per foot
[SI] is the value in SI
a = Foot/PSI, i.e., 4.4207502460167764E-05
and
Foot = 12.0 * Inch
PSI = PoundForce / (Inch * Inch) reference: https://en.wikipedia.org/wiki/Pound_per_square_inch
Inch = 0.0254 reference: https://www.nist.gov/pml/owm/si-units-length
PoundForce = Pound * G reference: https://en.wikipedia.org/wiki/Pound_(force)
Pound = 0.45359237 reference: https://en.wikipedia.org/wiki/Pound_(mass)
G = 9.80665 reference: https://en.wikipedia.org/wiki/Gravity_of_Earth
"""@EN; 
                 rdfs:subClassOf ddhub:Unit. 
ddhub:PsiPerMetre a owl:Class; 
                  rdfs:comment """[v] = a * [SI]
where
[v] is the value in psi per metre
[SI] is the value in SI
a = 1.0/PSI, i.e., 0.00014503773773020924
and
PSI = PoundForce / (Inch * Inch) reference: https://en.wikipedia.org/wiki/Pound_per_square_inch
PoundForce = Pound * G reference: https://en.wikipedia.org/wiki/Pound_(force)
Inch = 0.0254 reference: https://www.nist.gov/pml/owm/si-units-length
Pound = 0.45359237 reference: https://en.wikipedia.org/wiki/Pound_(mass)
G = 9.80665 reference: https://en.wikipedia.org/wiki/Gravity_of_Earth
"""@EN; 
                  rdfs:subClassOf ddhub:Unit. 
ddhub:PulsationDampener a owl:Class; 
                        rdfs:comment ""@EN; 
                        rdfs:subClassOf ddhub:PistonMudPump. 
ddhub:PumpRate a owl:Class; 
               rdfs:comment ""@EN; 
               rdfs:subClassOf ddhub:PrototypeData. 
ddhub:PupJoints a owl:Class; 
                rdfs:comment ""@EN; 
                rdfs:subClassOf ddhub:DrillString. 
ddhub:Pushthebit a owl:Class; 
                 rdfs:comment ""@EN; 
                 rdfs:subClassOf ddhub:RotarySteerableSystems. 
ddhub:PwdPressure a owl:Class; 
                  rdfs:comment ""@EN; 
                  rdfs:subClassOf ddhub:MeasurementWhileDrillingTools. 
ddhub:Quadrant a owl:Class; 
               rdfs:comment """[v] = a * [SI]
where
[v] is the value in quadrant
[SI] is the value in SI
a = 2.0/PI, i.e., 0.6366197723675814
"""@EN; 
               rdfs:subClassOf ddhub:Unit. 
ddhub:QuadristandDerrick a owl:Class; 
                         rdfs:comment ""@EN; 
                         rdfs:subClassOf ddhub:Derrick. 
ddhub:Quantity a owl:Class; 
               rdfs:comment """A `Quantity` represents a physical quantity. A `Quantity` is characterized by its physical dimensions as defined in the SI
International System of units. There are typical sub-types of `Quantity` defined in `QuantityTypes`. These types can be used in a sort of singleton pattern, i.e., it is not necessary to create an individual to use them
in a relation. Also, if individuals are created with the same characteristics, they are considered as being 
multiple representations of the same `Noun`. These typical
sub-types are automatically generated from the `PhysicalQuantities` defined in the Open Source Drilling 
Community ([OSDC](https://opensourcedrilling.org/)) project called `UnitConversion` (see [`OSDC UnitConversion`](https://github.com/Open-Source-Drilling-Community/UnitConversion)).
Only the physical quantities for which a `MeaningfulPrecision` is *not* defined are used to generate 
QuantityTypes. It is possible to look at all the physical quantities defined in the `OSDC UnitConversion` project by
using the web application hosted here: [`OSDC Physical Quantity Web App`](https://dev.digiwells.no/UnitConversion/webapp/PhysicalQuantity).
"""@EN; 
               rdfs:subClassOf ddhub:DWISNoun. 
ddhub:QuarterCommon a owl:Class; 
                    rdfs:comment """[v] = a * [SI]
where
[v] is the value in quarter common
[SI] is the value in SI
a = 1.0/QuarterCommon, i.e., 1.267523512561158E-07
and
QuarterCommon = YearJulian / 4.0
YearJulian = 365.25 * Day
Day = 24.0 * Hour
Hour = 60.0 * Minute
Minute = 60.0
"""@EN; 
                    rdfs:subClassOf ddhub:Unit. 
ddhub:Quill a owl:Class; 
            rdfs:comment ""@EN; 
            rdfs:subClassOf ddhub:TopDrive. 
ddhub:RackAndPinionHoistingSystem a owl:Class; 
                                  rdfs:comment ""@EN; 
                                  rdfs:subClassOf ddhub:HoistingSystem. 
ddhub:RadialModelling a owl:Class; 
                      rdfs:comment """The model accounts for the radial movement of some parts of the physical system.
"""@EN; 
                      rdfs:subClassOf ddhub:LateralModelling. 
ddhub:Radian a owl:Class; 
             rdfs:comment """No conversion necessary as the unit choice is SI
"""@EN; 
             rdfs:subClassOf ddhub:Unit. 
ddhub:RadianGauss a owl:Class; 
                  rdfs:comment """[v] = a * [SI]
where
[v] is the value in radian gauss
[SI] is the value in SI
a = 1.0/Gauss, i.e., 10000
and
Gauss = 1e-4 reference: https://en.wikipedia.org/wiki/Gauss_(unit)
"""@EN; 
                  rdfs:subClassOf ddhub:Unit. 
ddhub:RadianMaxwellPerSquareCentimetre a owl:Class; 
                                       rdfs:comment """[v] = a * [SI]
where
[v] is the value in radian maxwell per square centimetre
[SI] is the value in SI
a = 1.0/(Centi*Centi), i.e., 10000
and
Centi = 0.01
"""@EN; 
                                       rdfs:subClassOf ddhub:Unit. 
ddhub:RadianMicrotesla a owl:Class; 
                       rdfs:comment """[v] = a * [SI]
where
[v] is the value in radian microtesla
[SI] is the value in SI
a = 1.0/Micro, i.e., 1000000
and
Micro = 1e-6
"""@EN; 
                       rdfs:subClassOf ddhub:Unit. 
ddhub:RadianMilligauss a owl:Class; 
                       rdfs:comment """[v] = a * [SI]
where
[v] is the value in radian milligauss
[SI] is the value in SI
a = 1.0/(Milli*Gauss), i.e., 10000000
and
Milli = 0.001
Gauss = 1e-4 reference: https://en.wikipedia.org/wiki/Gauss_(unit)
"""@EN; 
                       rdfs:subClassOf ddhub:Unit. 
ddhub:RadianMillitesla a owl:Class; 
                       rdfs:comment """[v] = a * [SI]
where
[v] is the value in radian millitesla
[SI] is the value in SI
a = 1.0/Milli, i.e., 1000
and
Milli = 0.001
"""@EN; 
                       rdfs:subClassOf ddhub:Unit. 
ddhub:RadianNanotesla a owl:Class; 
                      rdfs:comment """[v] = a * [SI]
where
[v] is the value in radian nanotesla
[SI] is the value in SI
a = 1.0/Nano, i.e., 999999999.9999999
and
Nano = 1e-9
"""@EN; 
                      rdfs:subClassOf ddhub:Unit. 
ddhub:RadianPerCentimeter a owl:Class; 
                          rdfs:comment """[v] = a * [SI]
where
[v] is the value in radian per centimeter
[SI] is the value in SI
a = Centi, i.e., 0.01
and
Centi = 0.01
"""@EN; 
                          rdfs:subClassOf ddhub:Unit. 
ddhub:RadianPerCentimetre a owl:Class; 
                          rdfs:comment """[v] = a * [SI]
where
[v] is the value in radian per centimetre
[SI] is the value in SI
a = Centi, i.e., 0.01
and
Centi = 0.01
"""@EN; 
                          rdfs:subClassOf ddhub:Unit. 
ddhub:RadianPerDay a owl:Class; 
                   rdfs:comment """[v] = a * [SI]
where
[v] is the value in radian per day
[SI] is the value in SI
a = Day, i.e., 86400
and
Day = 24.0 * Hour
Hour = 60.0 * Minute
Minute = 60.0
"""@EN; 
                   rdfs:subClassOf ddhub:Unit. 
ddhub:RadianPerDayPerHour a owl:Class; 
                          rdfs:comment """[v] = a * [SI]
where
[v] is the value in radian per day per hour
[SI] is the value in SI
a = Day*Hour, i.e., 311040000
and
Day = 24.0 * Hour
Hour = 60.0 * Minute
Minute = 60.0
"""@EN; 
                          rdfs:subClassOf ddhub:Unit. 
ddhub:RadianPerDayPerMinute a owl:Class; 
                            rdfs:comment """[v] = a * [SI]
where
[v] is the value in radian per day per minute
[SI] is the value in SI
a = Day*Minute, i.e., 5184000
and
Day = 24.0 * Hour
Minute = 60.0
Hour = 60.0 * Minute
"""@EN; 
                            rdfs:subClassOf ddhub:Unit. 
ddhub:RadianPerDayPerSecond a owl:Class; 
                            rdfs:comment """[v] = a * [SI]
where
[v] is the value in radian per day per second
[SI] is the value in SI
a = Day, i.e., 86400
and
Day = 24.0 * Hour
Hour = 60.0 * Minute
Minute = 60.0
"""@EN; 
                            rdfs:subClassOf ddhub:Unit. 
ddhub:RadianPerDaySquared a owl:Class; 
                          rdfs:comment """[v] = a * [SI]
where
[v] is the value in radian per day squared
[SI] is the value in SI
a = Day*Day, i.e., 7464960000
and
Day = 24.0 * Hour
Hour = 60.0 * Minute
Minute = 60.0
"""@EN; 
                          rdfs:subClassOf ddhub:Unit. 
ddhub:RadianPerDecameter a owl:Class; 
                         rdfs:comment """[v] = a * [SI]
where
[v] is the value in radian per decameter
[SI] is the value in SI
a = Deca, i.e., 10
and
Deca = 10.0
"""@EN; 
                         rdfs:subClassOf ddhub:Unit. 
ddhub:RadianPerDecimeter a owl:Class; 
                         rdfs:comment """[v] = a * [SI]
where
[v] is the value in radian per decimeter
[SI] is the value in SI
a = Deci, i.e., 0.1
and
Deci = 0.1
"""@EN; 
                         rdfs:subClassOf ddhub:Unit. 
ddhub:RadianPerDecimetre a owl:Class; 
                         rdfs:comment """[v] = a * [SI]
where
[v] is the value in radian per decimetre
[SI] is the value in SI
a = Deci, i.e., 0.1
and
Deci = 0.1
"""@EN; 
                         rdfs:subClassOf ddhub:Unit. 
ddhub:RadianPerFoot a owl:Class; 
                    rdfs:comment """[v] = a * [SI]
where
[v] is the value in radian per foot
[SI] is the value in SI
a = Foot, i.e., 0.30479999999999996
and
Foot = 12.0 * Inch
Inch = 0.0254 reference: https://www.nist.gov/pml/owm/si-units-length
"""@EN; 
                    rdfs:subClassOf ddhub:Unit. 
ddhub:RadianPerHectometer a owl:Class; 
                          rdfs:comment """[v] = a * [SI]
where
[v] is the value in radian per hectometer
[SI] is the value in SI
a = Hecto, i.e., 100
and
Hecto = 100.0
"""@EN; 
                          rdfs:subClassOf ddhub:Unit. 
ddhub:RadianPerHour a owl:Class; 
                    rdfs:comment """[v] = a * [SI]
where
[v] is the value in radian per hour
[SI] is the value in SI
a = Hour, i.e., 3600
and
Hour = 60.0 * Minute
Minute = 60.0
"""@EN; 
                    rdfs:subClassOf ddhub:Unit. 
ddhub:RadianPerHourPerDay a owl:Class; 
                          rdfs:comment """[v] = a * [SI]
where
[v] is the value in radian per hour per day
[SI] is the value in SI
a = Hour*Day, i.e., 311040000
and
Hour = 60.0 * Minute
Day = 24.0 * Hour
Minute = 60.0
"""@EN; 
                          rdfs:subClassOf ddhub:Unit. 
ddhub:RadianPerHourPerMinute a owl:Class; 
                             rdfs:comment """[v] = a * [SI]
where
[v] is the value in radian per hour per minute
[SI] is the value in SI
a = Hour*Minute, i.e., 216000
and
Hour = 60.0 * Minute
Minute = 60.0
"""@EN; 
                             rdfs:subClassOf ddhub:Unit. 
ddhub:RadianPerHourPerSecond a owl:Class; 
                             rdfs:comment """[v] = a * [SI]
where
[v] is the value in radian per hour per second
[SI] is the value in SI
a = Hour, i.e., 3600
and
Hour = 60.0 * Minute
Minute = 60.0
"""@EN; 
                             rdfs:subClassOf ddhub:Unit. 
ddhub:RadianPerHourSquared a owl:Class; 
                           rdfs:comment """[v] = a * [SI]
where
[v] is the value in radian per hour squared
[SI] is the value in SI
a = Hour*Hour, i.e., 12960000
and
Hour = 60.0 * Minute
Minute = 60.0
"""@EN; 
                           rdfs:subClassOf ddhub:Unit. 
ddhub:RadianPerInch a owl:Class; 
                    rdfs:comment """[v] = a * [SI]
where
[v] is the value in radian per inch
[SI] is the value in SI
a = Inch, i.e., 0.0254
and
Inch = 0.0254 reference: https://www.nist.gov/pml/owm/si-units-length
"""@EN; 
                    rdfs:subClassOf ddhub:Unit. 
ddhub:RadianPerKilometer a owl:Class; 
                         rdfs:comment """[v] = a * [SI]
where
[v] is the value in radian per kilometer
[SI] is the value in SI
a = Kilo, i.e., 1000
and
Kilo = 1000.0
"""@EN; 
                         rdfs:subClassOf ddhub:Unit. 
ddhub:RadianPerMetre a owl:Class; 
                     rdfs:comment """No conversion necessary as the unit choice is SI
"""@EN; 
                     rdfs:subClassOf ddhub:Unit. 
ddhub:RadianPerMicrometer a owl:Class; 
                          rdfs:comment """[v] = a * [SI]
where
[v] is the value in radian per micrometer
[SI] is the value in SI
a = Micro, i.e., 1E-06
and
Micro = 1e-6
"""@EN; 
                          rdfs:subClassOf ddhub:Unit. 
ddhub:RadianPerMile a owl:Class; 
                    rdfs:comment """[v] = a * [SI]
where
[v] is the value in radian per mile
[SI] is the value in SI
a = Mile, i.e., 1609.3439999999998
and
Mile = 1760.0 * Yard reference: https://dictionary.cambridge.org/dictionary/english/mile
Yard = 3.0 * Foot
Foot = 12.0 * Inch
Inch = 0.0254 reference: https://www.nist.gov/pml/owm/si-units-length
"""@EN; 
                    rdfs:subClassOf ddhub:Unit. 
ddhub:RadianPerMillimeter a owl:Class; 
                          rdfs:comment """[v] = a * [SI]
where
[v] is the value in radian per millimeter
[SI] is the value in SI
a = Milli, i.e., 0.001
and
Milli = 0.001
"""@EN; 
                          rdfs:subClassOf ddhub:Unit. 
ddhub:RadianPerMillimetre a owl:Class; 
                          rdfs:comment """[v] = a * [SI]
where
[v] is the value in radian per millimetre
[SI] is the value in SI
a = Milli, i.e., 0.001
and
Milli = 0.001
"""@EN; 
                          rdfs:subClassOf ddhub:Unit. 
ddhub:RadianPerMinute a owl:Class; 
                      rdfs:comment """[v] = a * [SI]
where
[v] is the value in radian per minute
[SI] is the value in SI
a = Minute, i.e., 60
and
Minute = 60.0
"""@EN; 
                      rdfs:subClassOf ddhub:Unit. 
ddhub:RadianPerMinutePerDay a owl:Class; 
                            rdfs:comment """[v] = a * [SI]
where
[v] is the value in radian per minute per day
[SI] is the value in SI
a = Minute*Day, i.e., 5184000
and
Minute = 60.0
Day = 24.0 * Hour
Hour = 60.0 * Minute
"""@EN; 
                            rdfs:subClassOf ddhub:Unit. 
ddhub:RadianPerMinutePerHour a owl:Class; 
                             rdfs:comment """[v] = a * [SI]
where
[v] is the value in radian per minute per hour
[SI] is the value in SI
a = Minute*Hour, i.e., 216000
and
Minute = 60.0
Hour = 60.0 * Minute
"""@EN; 
                             rdfs:subClassOf ddhub:Unit. 
ddhub:RadianPerMinutePerSecond a owl:Class; 
                               rdfs:comment """[v] = a * [SI]
where
[v] is the value in radian per minute per second
[SI] is the value in SI
a = Minute, i.e., 60
and
Minute = 60.0
"""@EN; 
                               rdfs:subClassOf ddhub:Unit. 
ddhub:RadianPerMinuteSquared a owl:Class; 
                             rdfs:comment """[v] = a * [SI]
where
[v] is the value in radian per minute squared
[SI] is the value in SI
a = Minute*Minute, i.e., 3600
and
Minute = 60.0
"""@EN; 
                             rdfs:subClassOf ddhub:Unit. 
ddhub:RadianPerNanometer a owl:Class; 
                         rdfs:comment """[v] = a * [SI]
where
[v] is the value in radian per nanometer
[SI] is the value in SI
a = Nano, i.e., 1E-09
and
Nano = 1e-9
"""@EN; 
                         rdfs:subClassOf ddhub:Unit. 
ddhub:RadianPerSecond a owl:Class; 
                      rdfs:comment """No conversion necessary as the unit choice is SI
"""@EN; 
                      rdfs:subClassOf ddhub:Unit. 
ddhub:RadianPerSecondPerDay a owl:Class; 
                            rdfs:comment """[v] = a * [SI]
where
[v] is the value in radian per second per day
[SI] is the value in SI
a = Unit*Day, i.e., 86400
and
Unit = 1.0
Day = 24.0 * Hour
Hour = 60.0 * Minute
Minute = 60.0
"""@EN; 
                            rdfs:subClassOf ddhub:Unit. 
ddhub:RadianPerSecondPerHour a owl:Class; 
                             rdfs:comment """[v] = a * [SI]
where
[v] is the value in radian per second per hour
[SI] is the value in SI
a = Unit*Hour, i.e., 3600
and
Unit = 1.0
Hour = 60.0 * Minute
Minute = 60.0
"""@EN; 
                             rdfs:subClassOf ddhub:Unit. 
ddhub:RadianPerSecondPerMinute a owl:Class; 
                               rdfs:comment """[v] = a * [SI]
where
[v] is the value in radian per second per minute
[SI] is the value in SI
a = Unit * Minute, i.e., 60
and
Unit = 1.0
Minute = 60.0
"""@EN; 
                               rdfs:subClassOf ddhub:Unit. 
ddhub:RadianPerSecondSquared a owl:Class; 
                             rdfs:comment """No conversion necessary as the unit choice is SI
"""@EN; 
                             rdfs:subClassOf ddhub:Unit. 
ddhub:RadianPerSquareRootDay a owl:Class; 
                             rdfs:comment """[v] = a * [SI]
where
[v] is the value in radian per square root day
[SI] is the value in SI
a = Sqrt(Day), i.e., 293.9387691339814
and
Day = 24.0 * Hour
Hour = 60.0 * Minute
Minute = 60.0
"""@EN; 
                             rdfs:subClassOf ddhub:Unit. 
ddhub:RadianPerSquareRootHour a owl:Class; 
                              rdfs:comment """[v] = a * [SI]
where
[v] is the value in radian per square root hour
[SI] is the value in SI
a = Sqrt(Hour), i.e., 60
and
Hour = 60.0 * Minute
Minute = 60.0
"""@EN; 
                              rdfs:subClassOf ddhub:Unit. 
ddhub:RadianPerSquareRootMinute a owl:Class; 
                                rdfs:comment """[v] = a * [SI]
where
[v] is the value in radian per square root minute
[SI] is the value in SI
a = Sqrt(Minute), i.e., 7.745966692414834
and
Minute = 60.0
"""@EN; 
                                rdfs:subClassOf ddhub:Unit. 
ddhub:RadianPerSquareRootSecond a owl:Class; 
                                rdfs:comment """No conversion necessary as the unit choice is SI
"""@EN; 
                                rdfs:subClassOf ddhub:Unit. 
ddhub:RadianPerYard a owl:Class; 
                    rdfs:comment """[v] = a * [SI]
where
[v] is the value in radian per yard
[SI] is the value in SI
a = Yard, i.e., 0.9143999999999999
and
Yard = 3.0 * Foot
Foot = 12.0 * Inch
Inch = 0.0254 reference: https://www.nist.gov/pml/owm/si-units-length
"""@EN; 
                    rdfs:subClassOf ddhub:Unit. 
ddhub:RadianTesla a owl:Class; 
                  rdfs:comment """No conversion necessary as the unit choice is SI
"""@EN; 
                  rdfs:subClassOf ddhub:Unit. 
ddhub:RadianWeberPerSquareMetre a owl:Class; 
                                rdfs:comment """[v] = a * [SI]
where
[v] is the value in radian weber per square metre
[SI] is the value in SI
a = 1.0/Unit, i.e., 1
and
Unit = 1.0
"""@EN; 
                                rdfs:subClassOf ddhub:Unit. 
ddhub:RamHoistingSystem a owl:Class; 
                        rdfs:comment ""@EN; 
                        rdfs:subClassOf ddhub:HoistingSystem. 
ddhub:RamRig a owl:Class; 
             rdfs:comment ""@EN; 
             rdfs:subClassOf ddhub:Drawworks. 
ddhub:RandomWalkDrillingQuantity a owl:Class; 
                                 rdfs:comment """A random walk is a mathematical concept describing a path consisting of a series of random steps or movements, where each step's direction or magnitude is determined probabilistically. It is used to model various phenomena in fields like physics, finance, and computer science.
The dimension of random walk is:
$$[{\\theta}T^{-0.5}]$$.
The SI unit for **random walk** is: radian per square root second with the associated unit label $\\frac{rad}{\\sqrt{s}}$
The meaningful precision of random walk in the drilling context is typically: 1E-05 rad/√s
"""@EN; 
                                 rdfs:subClassOf ddhub:MeasurableQuantity. 
ddhub:RandomWalkQuantity a owl:Class; 
                         rdfs:comment """A random walk is a mathematical concept describing a path consisting of a series of random steps or movements, where each step's direction or magnitude is determined probabilistically. It is used to model various phenomena in fields like physics, finance, and computer science.
The dimension of random walk is:
$$[{\\theta}T^{-0.5}]$$.
The SI unit for **random walk** is: radian per square root second with the associated unit label $\\frac{rad}{\\sqrt{s}}$
"""@EN; 
                         rdfs:subClassOf ddhub:Quantity. 
ddhub:RangeExtraction a owl:Class; 
                      rdfs:comment ""@EN; 
                      rdfs:subClassOf ddhub:TimeBasedTransformation. 
ddhub:Rankine a owl:Class; 
              rdfs:comment """[v] = a * [SI]
where
[v] is the value in rankine
[SI] is the value in SI
a = 1.0/FahrenheitSlope, i.e., 1.7999999999999998
and
FahrenheitSlope = 5.0 / 9.0 reference: https://nn.wikipedia.org/wiki/Fahrenheit
"""@EN; 
              rdfs:subClassOf ddhub:Unit. 
ddhub:RateOfPenetrationDrillingQuantity a owl:Class; 
                                        rdfs:comment """A velocity is the time derivative of a position or a displacement: $\\frac{dx}{dt}$, where $x$ is a position and $t$ is time.
The dimension of velocity is:
$$[LT^{-1}]$$.
The SI unit for **velocity** is: metre per second with the associated unit label $\\frac{m}{s}$
The meaningful precision of rate of penetration in the drilling context is typically: 2.77778E-05 m/min
"""@EN; 
                                        rdfs:subClassOf ddhub:MeasurableQuantity. 
ddhub:Reamers a owl:Class; 
              rdfs:comment ""@EN; 
              rdfs:subClassOf ddhub:DrillingEquipment. 
ddhub:Réaumur a owl:Class; 
              rdfs:comment """[v] = a * [SI] + b
where
[v] is the value in réaumur
[SI] is the value in SI
a = 1.0/ReaumurSlope, i.e., 0.8
b = -ReaumurBias, i.e., -218.51999999999998
and
ReaumurSlope = 5.0 / 4.0 reference: https://en.wikipedia.org/wiki/R%C3%A9aumur_scale
ReaumurBias = ZeroCelsius / ReaumurSlope
ZeroCelsius = 273.15 reference: https://www.nist.gov/pml/owm/si-units-temperature
"""@EN; 
              rdfs:subClassOf ddhub:Unit. 
ddhub:ReciprocalAangstroem a owl:Class; 
                           rdfs:comment """[v] = a * [SI]
where
[v] is the value in reciprocal ångstrøm
[SI] is the value in SI
a = Angstrom, i.e., 1E-10
and
Angstrom = 1e-10
"""@EN; 
                           rdfs:subClassOf ddhub:Unit. 
ddhub:ReciprocalAstronomicalUnit a owl:Class; 
                                 rdfs:comment """[v] = a * [SI]
where
[v] is the value in reciprocal astronomical unit
[SI] is the value in SI
a = AstronomicalUnit, i.e., 149597870700
and
AstronomicalUnit = 149597870700.0 reference: https://www.iau.org/static/resolutions/IAU2012_English.pdf
"""@EN; 
                                 rdfs:subClassOf ddhub:Unit. 
ddhub:ReciprocalCentimetre a owl:Class; 
                           rdfs:comment """[v] = a * [SI]
where
[v] is the value in reciprocal centimetre
[SI] is the value in SI
a = Centi, i.e., 0.01
and
Centi = 0.01
"""@EN; 
                           rdfs:subClassOf ddhub:Unit. 
ddhub:ReciprocalDecametre a owl:Class; 
                          rdfs:comment """[v] = a * [SI]
where
[v] is the value in reciprocal decametre
[SI] is the value in SI
a = Deca, i.e., 10
and
Deca = 10.0
"""@EN; 
                          rdfs:subClassOf ddhub:Unit. 
ddhub:ReciprocalDecimetre a owl:Class; 
                          rdfs:comment """[v] = a * [SI]
where
[v] is the value in reciprocal decimetre
[SI] is the value in SI
a = Deci, i.e., 0.1
and
Deci = 0.1
"""@EN; 
                          rdfs:subClassOf ddhub:Unit. 
ddhub:ReciprocalFathom a owl:Class; 
                       rdfs:comment """[v] = a * [SI]
where
[v] is the value in reciprocal fathom
[SI] is the value in SI
a = Fathom, i.e., 1.8287999999999998
and
Fathom = 6.0 * Foot reference: https://www.britannica.com/science/fathom
Foot = 12.0 * Inch
Inch = 0.0254 reference: https://www.nist.gov/pml/owm/si-units-length
"""@EN; 
                       rdfs:subClassOf ddhub:Unit. 
ddhub:ReciprocalFoot a owl:Class; 
                     rdfs:comment """[v] = a * [SI]
where
[v] is the value in reciprocal foot
[SI] is the value in SI
a = Foot, i.e., 0.30479999999999996
and
Foot = 12.0 * Inch
Inch = 0.0254 reference: https://www.nist.gov/pml/owm/si-units-length
"""@EN; 
                     rdfs:subClassOf ddhub:Unit. 
ddhub:ReciprocalFurlong a owl:Class; 
                        rdfs:comment """[v] = a * [SI]
where
[v] is the value in reciprocal furlong
[SI] is the value in SI
a = Furlong, i.e., 201.16799999999998
and
Furlong = 660.0 * Foot reference: https://www.britannica.com/science/furlong
Foot = 12.0 * Inch
Inch = 0.0254 reference: https://www.nist.gov/pml/owm/si-units-length
"""@EN; 
                        rdfs:subClassOf ddhub:Unit. 
ddhub:ReciprocalHand a owl:Class; 
                     rdfs:comment """[v] = a * [SI]
where
[v] is the value in reciprocal hand
[SI] is the value in SI
a = Hand, i.e., 0.1016
and
Hand = 4.0 * Inch reference: https://en.wikipedia.org/wiki/Hand_(unit)
Inch = 0.0254 reference: https://www.nist.gov/pml/owm/si-units-length
"""@EN; 
                     rdfs:subClassOf ddhub:Unit. 
ddhub:ReciprocalHectometre a owl:Class; 
                           rdfs:comment """[v] = a * [SI]
where
[v] is the value in reciprocal hectometre
[SI] is the value in SI
a = Hecto, i.e., 100
and
Hecto = 100.0
"""@EN; 
                           rdfs:subClassOf ddhub:Unit. 
ddhub:ReciprocalInch a owl:Class; 
                     rdfs:comment """[v] = a * [SI]
where
[v] is the value in reciprocal inch
[SI] is the value in SI
a = Inch, i.e., 0.0254
and
Inch = 0.0254 reference: https://www.nist.gov/pml/owm/si-units-length
"""@EN; 
                     rdfs:subClassOf ddhub:Unit. 
ddhub:ReciprocalInchPer32 a owl:Class; 
                          rdfs:comment """[v] = a * [SI]
where
[v] is the value in reciprocal inch per 32
[SI] is the value in SI
a = InchPer32, i.e., 0.00079375
and
InchPer32 = Inch / 32.0
Inch = 0.0254 reference: https://www.nist.gov/pml/owm/si-units-length
"""@EN; 
                          rdfs:subClassOf ddhub:Unit. 
ddhub:ReciprocalInternationalNauticalMile a owl:Class; 
                                          rdfs:comment """[v] = a * [SI]
where
[v] is the value in reciprocal international nautical mile
[SI] is the value in SI
a = InternationalNauticalMile, i.e., 1852
and
InternationalNauticalMile = 1852.0 reference: https://www.merriam-webster.com/dictionary/nautical%20mile
"""@EN; 
                                          rdfs:subClassOf ddhub:Unit. 
ddhub:ReciprocalKilometre a owl:Class; 
                          rdfs:comment """[v] = a * [SI]
where
[v] is the value in reciprocal kilometre
[SI] is the value in SI
a = Kilo, i.e., 1000
and
Kilo = 1000.0
"""@EN; 
                          rdfs:subClassOf ddhub:Unit. 
ddhub:ReciprocalLengthSurveyInstrumentDrillingQuantity a owl:Class; 
                                                       rdfs:comment """A wave number is the number of wave lengths per unit distance.
The dimension of wave number is:
$$[L^{-1}]$$.
The SI unit for **wave number** is: reciprocal metre with the associated unit label $\\frac{1}{m}$
The meaningful precision of reciprocal length related to survey instrument performance models in the drilling context is typically: 1E-08 1/m
"""@EN; 
                                                       rdfs:subClassOf ddhub:MeasurableQuantity. 
ddhub:ReciprocalLightYear a owl:Class; 
                          rdfs:comment """[v] = a * [SI]
where
[v] is the value in reciprocal light year
[SI] is the value in SI
a = LightYear, i.e., 9460730472580800
and
LightYear = 9460730472580800.0 reference: https://www.iau.org/public/themes/measuring/
"""@EN; 
                          rdfs:subClassOf ddhub:Unit. 
ddhub:ReciprocalMetre a owl:Class; 
                      rdfs:comment """No conversion necessary as the unit choice is SI
"""@EN; 
                      rdfs:subClassOf ddhub:Unit. 
ddhub:ReciprocalMicrometre a owl:Class; 
                           rdfs:comment """[v] = a * [SI]
where
[v] is the value in reciprocal micrometre
[SI] is the value in SI
a = Micro, i.e., 1E-06
and
Micro = 1e-6
"""@EN; 
                           rdfs:subClassOf ddhub:Unit. 
ddhub:ReciprocalMil a owl:Class; 
                    rdfs:comment """[v] = a * [SI]
where
[v] is the value in reciprocal mil
[SI] is the value in SI
a = Mil, i.e., 2.54E-05
and
Mil = 0.001 * Inch reference: https://en.wikipedia.org/wiki/Thousandth_of_an_inch
Inch = 0.0254 reference: https://www.nist.gov/pml/owm/si-units-length
"""@EN; 
                    rdfs:subClassOf ddhub:Unit. 
ddhub:ReciprocalMile a owl:Class; 
                     rdfs:comment """[v] = a * [SI]
where
[v] is the value in reciprocal mile
[SI] is the value in SI
a = Mile, i.e., 1609.3439999999998
and
Mile = 1760.0 * Yard reference: https://dictionary.cambridge.org/dictionary/english/mile
Yard = 3.0 * Foot
Foot = 12.0 * Inch
Inch = 0.0254 reference: https://www.nist.gov/pml/owm/si-units-length
"""@EN; 
                     rdfs:subClassOf ddhub:Unit. 
ddhub:ReciprocalMillimetre a owl:Class; 
                           rdfs:comment """[v] = a * [SI]
where
[v] is the value in reciprocal millimetre
[SI] is the value in SI
a = Milli, i.e., 0.001
and
Milli = 0.001
"""@EN; 
                           rdfs:subClassOf ddhub:Unit. 
ddhub:ReciprocalNanometre a owl:Class; 
                          rdfs:comment """[v] = a * [SI]
where
[v] is the value in reciprocal nanometre
[SI] is the value in SI
a = Nano, i.e., 1E-09
and
Nano = 1e-9
"""@EN; 
                          rdfs:subClassOf ddhub:Unit. 
ddhub:ReciprocalParsec a owl:Class; 
                       rdfs:comment """[v] = a * [SI]
where
[v] is the value in reciprocal parsec
[SI] is the value in SI
a = Parsec, i.e., 30856775814913670
and
Parsec = (60.0*60.0*180.0 / System.Math.PI) * AstronomicalUnit reference: https://imagine.gsfc.nasa.gov/features/cosmic/milkyway_info.html
AstronomicalUnit = 149597870700.0 reference: https://www.iau.org/static/resolutions/IAU2012_English.pdf
"""@EN; 
                       rdfs:subClassOf ddhub:Unit. 
ddhub:ReciprocalPicometre a owl:Class; 
                          rdfs:comment """[v] = a * [SI]
where
[v] is the value in reciprocal picometre
[SI] is the value in SI
a = Pico, i.e., 1E-12
and
Pico = 1e-12
"""@EN; 
                          rdfs:subClassOf ddhub:Unit. 
ddhub:ReciprocalScandinavianMile a owl:Class; 
                                 rdfs:comment """[v] = a * [SI]
where
[v] is the value in reciprocal scandinavian mile
[SI] is the value in SI
a = ScandinavianMile, i.e., 10000
and
ScandinavianMile = 10000.0
"""@EN; 
                                 rdfs:subClassOf ddhub:Unit. 
ddhub:ReciprocalSecond a owl:Class; 
                       rdfs:comment """[v] = a * [SI]
where
[v] is the value in reciprocal second
[SI] is the value in SI
a = 1.0/Unit, i.e., 1
and
Unit = 1.0
"""@EN; 
                       rdfs:subClassOf ddhub:Unit. 
ddhub:ReciprocalSurveyorsChain a owl:Class; 
                               rdfs:comment """[v] = a * [SI]
where
[v] is the value in reciprocal surveyors chain
[SI] is the value in SI
a = SurveyorChain, i.e., 20.116799999999998
and
SurveyorChain = 22.0 * Yard reference: https://www.britannica.com/technology/surveyors-chain
Yard = 3.0 * Foot
Foot = 12.0 * Inch
Inch = 0.0254 reference: https://www.nist.gov/pml/owm/si-units-length
"""@EN; 
                               rdfs:subClassOf ddhub:Unit. 
ddhub:ReciprocalThou a owl:Class; 
                     rdfs:comment """[v] = a * [SI]
where
[v] is the value in reciprocal thou
[SI] is the value in SI
a = Thou, i.e., 2.54E-05
and
Thou = Mil
Mil = 0.001 * Inch reference: https://en.wikipedia.org/wiki/Thousandth_of_an_inch
Inch = 0.0254 reference: https://www.nist.gov/pml/owm/si-units-length
"""@EN; 
                     rdfs:subClassOf ddhub:Unit. 
ddhub:ReciprocalUkNauticalMile a owl:Class; 
                               rdfs:comment """[v] = a * [SI]
where
[v] is the value in reciprocal UK nautical mile
[SI] is the value in SI
a = UKNauticalMile, i.e., 1853.1839999999997
and
UKNauticalMile = 6080 * Foot reference: https://www.rmg.co.uk/stories/topics/nautical-mile
Foot = 12.0 * Inch
Inch = 0.0254 reference: https://www.nist.gov/pml/owm/si-units-length
"""@EN; 
                               rdfs:subClassOf ddhub:Unit. 
ddhub:ReciprocalUsSurveyFoot a owl:Class; 
                             rdfs:comment """[v] = a * [SI]
where
[v] is the value in reciprocal US survey foot
[SI] is the value in SI
a = USSurveyFoot, i.e., 0.3048006096012192
and
USSurveyFoot = 1200.0 / 3937.0 reference: https://www.nist.gov/pml/us-surveyfoot
"""@EN; 
                             rdfs:subClassOf ddhub:Unit. 
ddhub:ReciprocalYard a owl:Class; 
                     rdfs:comment """[v] = a * [SI]
where
[v] is the value in reciprocal yard
[SI] is the value in SI
a = Yard, i.e., 0.9143999999999999
and
Yard = 3.0 * Foot
Foot = 12.0 * Inch
Inch = 0.0254 reference: https://www.nist.gov/pml/owm/si-units-length
"""@EN; 
                     rdfs:subClassOf ddhub:Unit. 
ddhub:ReciprocationProcedure a owl:Class; 
                             rdfs:comment """The reciprocation procedure is used to ream up and down with the same stand. The main purpose is often to clean the hole
while avoiding to wash out the formation. 
"""@EN; 
                             rdfs:subClassOf ddhub:DrillingProcedure. 
ddhub:Recommendation a owl:Class; 
                     rdfs:comment ""@EN; 
                     rdfs:subClassOf ddhub:ProcessData. 
ddhub:RecommendedMaximum a owl:Class; 
                         rdfs:comment ""@EN; 
                         rdfs:subClassOf ddhub:Recommendation. 
ddhub:RecommendedMinimum a owl:Class; 
                         rdfs:comment ""@EN; 
                         rdfs:subClassOf ddhub:Recommendation. 
ddhub:RecommendedTarget a owl:Class; 
                        rdfs:comment ""@EN; 
                        rdfs:subClassOf ddhub:Recommendation. 
ddhub:RectangularChannel a owl:Class; 
                         rdfs:comment ""@EN; 
                         rdfs:subClassOf ddhub:OpenChannel. 
ddhub:ReferenceFrame a owl:Class; 
                     rdfs:comment """Represents a system of coordinates
"""@EN; 
                     rdfs:subClassOf ddhub:DWISNoun. 
ddhub:RelativeCelsius a owl:Class; 
                      rdfs:comment """[v] = a * [SI]
where
[v] is the value in relative celsius
[SI] is the value in SI
a = 1.0/Unit, i.e., 1
and
Unit = 1.0
"""@EN; 
                      rdfs:subClassOf ddhub:Unit. 
ddhub:RelativePressureReference a owl:Class; 
                                rdfs:comment ""@EN; 
                                rdfs:subClassOf ddhub:PressureReference. 
ddhub:RelativeTemperatureQuantity a owl:Class; 
                                  rdfs:comment """Relative temperature is a measure of temperature expressed in relation to a reference point or baseline, often used to compare temperature differences rather than absolute values.
The dimension of relative temperature is:
$$[K]$$.
The SI unit for **relative temperature** is: kelvin with the associated unit label $K$
"""@EN; 
                                  rdfs:subClassOf ddhub:Quantity. 
ddhub:RelativeTimeReference a owl:Class; 
                            rdfs:comment ""@EN; 
                            rdfs:subClassOf ddhub:TimeReference. 
ddhub:Resampling a owl:Class; 
                 rdfs:comment ""@EN; 
                 rdfs:subClassOf ddhub:TimeBasedTransformation. 
ddhub:ResamplingDelay a owl:DatatypeProperty, owl:FunctionalProperty; 
                      rdfs:comment """
"""@EN; 
                      rdfs:domain ddhub:Resampling; 
                      rdfs:range xsd:double. 
ddhub:ResamplingRate a owl:DatatypeProperty, owl:FunctionalProperty; 
                     rdfs:comment """
"""@EN; 
                     rdfs:domain ddhub:Resampling; 
                     rdfs:range xsd:double. 
ddhub:ReservePit a owl:Class; 
                 rdfs:comment ""@EN; 
                 rdfs:subClassOf ddhub:MudPits. 
ddhub:Resolution a owl:DatatypeProperty, owl:FunctionalProperty; 
                 rdfs:comment """
"""@EN; 
                 rdfs:domain ddhub:Clock; 
                 rdfs:range xsd:double. 
ddhub:ReturnFlowLine a owl:Class; 
                     rdfs:comment ""@EN; 
                     rdfs:subClassOf ddhub:Pipe. 
ddhub:Revolution a owl:Class; 
                 rdfs:comment """[v] = a * [SI]
where
[v] is the value in revolution
[SI] is the value in SI
a = 1.0/(2.0*PI), i.e., 0.15915494309189535
"""@EN; 
                 rdfs:subClassOf ddhub:Unit. 
ddhub:RfidReamers a owl:Class; 
                  rdfs:comment ""@EN; 
                  rdfs:subClassOf ddhub:Reamers. 
ddhub:RiemannianManifoldFourDimensionalReferenceFrame a owl:Class; 
                                                      rdfs:comment ""@EN; 
                                                      rdfs:subClassOf ddhub:FourDimensionalReferenceFrame. 
ddhub:RiemannianManifoldThreeDimensionalReferenceFrame a owl:Class; 
                                                       rdfs:comment ""@EN; 
                                                       rdfs:subClassOf ddhub:ThreeDimensionalReferenceFrame. 
ddhub:RiemannianManifoldTwoDimensionalReferenceFrame a owl:Class; 
                                                     rdfs:comment ""@EN; 
                                                     rdfs:subClassOf ddhub:TwoDimensionalReferenceFrame. 
ddhub:RigActionPlan a owl:Class; 
                    rdfs:comment """A rig action plan is a set of steps and rules that shall be conducted to fulfil a particulat activity when constructing a well.
"""@EN; 
                    rdfs:subClassOf ddhub:Plan. 
ddhub:RigActionPlanFeature a owl:Class; 
                           rdfs:comment """A rig action plan feature indicates that something accounts for the rig action plan.
"""@EN; 
                           rdfs:subClassOf ddhub:DrillingManagementFeature. 
ddhub:RigChokeControlSystem a owl:Class; 
                            rdfs:comment ""@EN; 
                            rdfs:subClassOf ddhub:ControlSystem. 
ddhub:RigDescription a owl:Class; 
                     rdfs:comment """The rig data structure describes the characteristics of the drilling equipment and any additional equipment
associated with non-standard drilling methods, e.g., back-pressure MPD, dual-gradient,...
"""@EN; 
                     rdfs:subClassOf ddhub:WellBoreData. 
ddhub:RigEquipment a owl:Class; 
                   rdfs:comment ""@EN; 
                   rdfs:subClassOf ddhub:Equipment. 
ddhub:RigFloor a owl:Class; 
               rdfs:comment ""@EN; 
               rdfs:subClassOf ddhub:DrillFloorStructure. 
ddhub:RightToLeft a owl:DatatypeProperty, owl:FunctionalProperty; 
                  rdfs:comment """Indicates whether the fluid can flow from the right branch to the left branch though the junction
"""@EN; 
                  rdfs:domain ddhub:HydraulicJunction; 
                  rdfs:range xsd:bool. 
ddhub:RiserLiftPump a owl:Class; 
                    rdfs:comment ""@EN; 
                    rdfs:subClassOf ddhub:CirculationSystem. 
ddhub:RiserRecoilSystem a owl:Class; 
                        rdfs:comment ""@EN; 
                        rdfs:subClassOf ddhub:MarineSystem. 
ddhub:RiserTensioners a owl:Class; 
                      rdfs:comment ""@EN; 
                      rdfs:subClassOf ddhub:MarineSystem. 
ddhub:RollerReamers a owl:Class; 
                    rdfs:comment ""@EN; 
                    rdfs:subClassOf ddhub:Reamers. 
ddhub:RollingCutter a owl:Class; 
                    rdfs:comment ""@EN; 
                    rdfs:subClassOf ddhub:DrillingBit. 
ddhub:ROP a owl:Class; 
          rdfs:comment ""@EN; 
          rdfs:subClassOf ddhub:PrototypeData. 
ddhub:ROPLimit a owl:Class; 
               rdfs:comment """This Noun is used to refer to a rate of penetration limit.
"""@EN; 
               rdfs:subClassOf ddhub:DrillingLimit. 
ddhub:RotarySlips a owl:Class; 
                  rdfs:comment ""@EN; 
                  rdfs:subClassOf ddhub:DrillFloorEquipment. 
ddhub:RotarySteerableSystems a owl:Class; 
                             rdfs:comment ""@EN; 
                             rdfs:subClassOf ddhub:DrillingEquipment. 
ddhub:RotaryTable a owl:Class; 
                  rdfs:comment ""@EN; 
                  rdfs:subClassOf ddhub:SurfaceRotationSystem. 
ddhub:RotaryTableBushings a owl:Class; 
                          rdfs:comment ""@EN; 
                          rdfs:subClassOf ddhub:RotaryTable. 
ddhub:RotaryTableVerticalLocation a owl:Class; 
                                  rdfs:comment ""@EN; 
                                  rdfs:subClassOf ddhub:VerticalReferenceLocation. 
ddhub:RotatingControlDeviceRcd a owl:Class; 
                               rdfs:comment ""@EN; 
                               rdfs:subClassOf ddhub:DrillFloorEquipment. 
ddhub:RotationalFrequencyQuantity a owl:Class; 
                                  rdfs:comment """Rotation frequency is the number of complete rotations or cycles an object makes per unit of time.
The dimension of rotational frequency is:
$$[T^{-1}]$$.
"""@EN; 
                                  rdfs:subClassOf ddhub:MeasurableQuantity. 
ddhub:RotationalFrequencyRateOfChangeDrillingQuantity a owl:Class; 
                                                      rdfs:comment """A frequency rate of change is the time derivative of a frequency: $\\frac{df}{dt}$, where $f$ is a frequency and $t$ is time.
The dimension of frequency rate of change is:
$$[T^{-2}]$$.
The SI unit for **frequency rate of change** is: hertz per second with the associated unit label $\\frac{Hz}{s}$
A rotation frequency rate of change is the time derivative of a rotation frequency.
The meaningful precision of rotational frequency is typically: 0.016666666666666666 Hz/s
The meaningful precision of rotational frequency rate of change in the drilling context is typically: 0.016666666666666666 Hz/s
"""@EN; 
                                                      rdfs:subClassOf ddhub:MeasurableQuantity. 
ddhub:RotationalFrequencyRateOfChangeQuantity a owl:Class; 
                                              rdfs:comment """A frequency rate of change is the time derivative of a frequency: $\\frac{df}{dt}$, where $f$ is a frequency and $t$ is time.
The dimension of frequency rate of change is:
$$[T^{-2}]$$.
The SI unit for **frequency rate of change** is: hertz per second with the associated unit label $\\frac{Hz}{s}$
A rotation frequency rate of change is the time derivative of a rotation frequency.
The meaningful precision of rotational frequency is typically:  Hz/s
"""@EN; 
                                              rdfs:subClassOf ddhub:Quantity. 
ddhub:RotationalFrequencySmallQuantity a owl:Class; 
                                       rdfs:comment """Rotation frequency is the number of complete rotations or cycles an object makes per unit of time.
The dimension of rotational frequency is:
$$[T^{-1}]$$.
The meaningful precision of small rotational frequency is typically: 0.00016666 Hz
"""@EN; 
                                       rdfs:subClassOf ddhub:MeasurableQuantity. 
ddhub:RotationalModelling a owl:Class; 
                          rdfs:comment """The model accounts for the rotational movement of some parts of the physical system.
"""@EN; 
                          rdfs:subClassOf ddhub:ModelledDegreeOfFreedom. 
ddhub:RotationalVelocityLimit a owl:Class; 
                              rdfs:comment """This Noun is used to refer to a rotational velocity limit.
"""@EN; 
                              rdfs:subClassOf ddhub:DrillingLimit. 
ddhub:RotationControlSystem a owl:Class; 
                            rdfs:comment ""@EN; 
                            rdfs:subClassOf ddhub:ControlSystem. 
ddhub:RotationPerHour a owl:Class; 
                      rdfs:comment """[v] = a * [SI]
where
[v] is the value in rotation per hour
[SI] is the value in SI
a = Hour, i.e., 3600
and
Hour = 60.0 * Minute
Minute = 60.0
"""@EN; 
                      rdfs:subClassOf ddhub:Unit. 
ddhub:RotationPerSecond a owl:Class; 
                        rdfs:comment """[v] = a * [SI]
where
[v] is the value in rotation per second
[SI] is the value in SI
a = Unit, i.e., 1
and
Unit = 1.0
"""@EN; 
                        rdfs:subClassOf ddhub:Unit. 
ddhub:RotationStartupProcedure a owl:Class; 
                               rdfs:comment """The rotation startup procedure controls the steps to start the rotation of the drill-stem to reach a target rotational
speed while attempting to avoid having too large torsional oscillations.
"""@EN; 
                               rdfs:subClassOf ddhub:DrillingProcedure. 
ddhub:RotationStopProcedure a owl:Class; 
                            rdfs:comment """The rotation stop procedure controls the path for stopping the rotation of the drill-stem and remove as much torque
along the drill-stem as possible.
"""@EN; 
                            rdfs:subClassOf ddhub:DrillingProcedure. 
ddhub:Rov a owl:Class; 
          rdfs:comment ""@EN; 
          rdfs:subClassOf ddhub:MarineSystem. 
ddhub:Rpm a owl:Class; 
          rdfs:comment """[v] = a * [SI]
where
[v] is the value in rpm
[SI] is the value in SI
a = Minute, i.e., 60
and
Minute = 60.0
"""@EN; 
          rdfs:subClassOf ddhub:Unit. 
ddhub:RpmPerSecond a owl:Class; 
                   rdfs:comment ""@EN; 
                   rdfs:subClassOf ddhub:Unit. 
ddhub:RunnableFunction a owl:Class; 
                       rdfs:comment """A runnable function is a function that starts to run immediately when activated.
"""@EN; 
                       rdfs:subClassOf ddhub:ActivableFunction. 
ddhub:SafetyClamps a owl:Class; 
                   rdfs:comment ""@EN; 
                   rdfs:subClassOf ddhub:DrillFloorEquipment. 
ddhub:SafetyEquipment a owl:Class; 
                      rdfs:comment ""@EN; 
                      rdfs:subClassOf ddhub:RigEquipment. 
ddhub:SamplingRate a owl:DatatypeProperty, owl:FunctionalProperty; 
                   rdfs:comment """
"""@EN; 
                   rdfs:domain ddhub:SynchronizationGroup; 
                   rdfs:range xsd:double. 
ddhub:SandTrap a owl:Class; 
               rdfs:comment ""@EN; 
               rdfs:subClassOf ddhub:MudPits. 
ddhub:ScandinavianMile a owl:Class; 
                       rdfs:comment """[v] = a * [SI]
where
[v] is the value in scandinavian mile
[SI] is the value in SI
a = 1.0/ScandinavianMile, i.e., 0.0001
and
ScandinavianMile = 10000.0
"""@EN; 
                       rdfs:subClassOf ddhub:Unit. 
ddhub:ScreenString a owl:Class; 
                   rdfs:comment ""@EN; 
                   rdfs:subClassOf ddhub:Tubulars. 
ddhub:ScribeLineAngleLocation a owl:Class; 
                              rdfs:comment ""@EN; 
                              rdfs:subClassOf ddhub:AngleReferenceLocation. 
ddhub:SeaFloorVerticalLocation a owl:Class; 
                               rdfs:comment ""@EN; 
                               rdfs:subClassOf ddhub:VerticalReferenceLocation. 
ddhub:SeaWater a owl:Class; 
               rdfs:comment ""@EN; 
               rdfs:subClassOf ddhub:DrillingFluid. 
ddhub:Second a owl:Class; 
             rdfs:comment """No conversion necessary as the unit choice is SI
"""@EN; 
             rdfs:subClassOf ddhub:Unit. 
ddhub:Selfsealingthreaded a owl:Class; 
                          rdfs:comment ""@EN; 
                          rdfs:subClassOf ddhub:Connection. 
ddhub:SemiCircularChannel a owl:Class; 
                          rdfs:comment ""@EN; 
                          rdfs:subClassOf ddhub:OpenChannel. 
ddhub:SensorUncertainty a owl:Class; 
                        rdfs:comment """The uncertainty of the sensor is described by a systematic bias and repetitive error. The systematic bias is referred to as the `Accuracy` while the repetitive error is referred to as the `Precision`. The standard deviation of the overall Gaussian distribution is $\\sqrt{\\sigma^2{_a}+\\sigma^2{_p}}$ where $\\sigma_a$ is the accuracy and $\\sigma_p$ is the precision. The `Accuracy` or the `Precision` can either be defined as attribute values, for example when they have fixed values, or using another facts utilizing the verbs `HasAccuracy` or respectively `HasPrecision` when these values may change through time.
"""@EN; 
                        rdfs:subClassOf ddhub:GaussianUncertainty. 
ddhub:Seperator a owl:Class; 
                rdfs:comment ""@EN; 
                rdfs:subClassOf ddhub:WellTestingEquipment. 
ddhub:ServiceCompany a owl:Class; 
                     rdfs:comment """A service company is an entity that provides services during the well construction.
"""@EN; 
                     rdfs:subClassOf ddhub:DataProvider. 
ddhub:SetPoint a owl:Class; 
               rdfs:comment ""@EN; 
               rdfs:subClassOf ddhub:ProcessData. 
ddhub:Sextant a owl:Class; 
              rdfs:comment """[v] = a * [SI]
where
[v] is the value in sextant
[SI] is the value in SI
a = 3.0/PI, i.e., 0.954929658551372
"""@EN; 
              rdfs:subClassOf ddhub:Unit. 
ddhub:Shake a owl:Class; 
            rdfs:comment """[v] = a * [SI]
where
[v] is the value in shake
[SI] is the value in SI
a = 1.0/(10.0*Nano), i.e., 100000000
and
Nano = 1e-9
"""@EN; 
            rdfs:subClassOf ddhub:Unit. 
ddhub:ShakerCascadeLevels a owl:Class; 
                          rdfs:comment ""@EN; 
                          rdfs:subClassOf ddhub:ShaleShakers. 
ddhub:ShakerDecks a owl:Class; 
                  rdfs:comment ""@EN; 
                  rdfs:subClassOf ddhub:ShaleShakers. 
ddhub:ShakerHopper a owl:Class; 
                   rdfs:comment ""@EN; 
                   rdfs:subClassOf ddhub:ShaleShakers. 
ddhub:ShakerScreenMeshSize a owl:Class; 
                           rdfs:comment ""@EN; 
                           rdfs:subClassOf ddhub:ShakerDecks. 
ddhub:ShakerScreens a owl:Class; 
                    rdfs:comment ""@EN; 
                    rdfs:subClassOf ddhub:ShakerDecks. 
ddhub:ShaleShakers a owl:Class; 
                   rdfs:comment ""@EN; 
                   rdfs:subClassOf ddhub:CirculationSystem. 
ddhub:ShearRam a owl:Class; 
               rdfs:comment ""@EN; 
               rdfs:subClassOf ddhub:BopElement. 
ddhub:ShearRate a owl:Class; 
                rdfs:comment ""@EN; 
                rdfs:subClassOf ddhub:PrototypeData. 
ddhub:ShearStress a owl:Class; 
                  rdfs:comment ""@EN; 
                  rdfs:subClassOf ddhub:PrototypeData. 
ddhub:Shock a owl:Class; 
            rdfs:comment """This Noun is used to refer to lateral shocks.
"""@EN; 
            rdfs:subClassOf ddhub:AbnormalLateralOscillation. 
ddhub:ShockPerHour a owl:Class; 
                   rdfs:comment """[v] = a * [SI]
where
[v] is the value in shock per hour
[SI] is the value in SI
a = Hour, i.e., 3600
and
Hour = 60.0 * Minute
Minute = 60.0
"""@EN; 
                   rdfs:subClassOf ddhub:Unit. 
ddhub:ShockPerMinute a owl:Class; 
                     rdfs:comment """[v] = a * [SI]
where
[v] is the value in shock per minute
[SI] is the value in SI
a = Minute, i.e., 60
and
Minute = 60.0
"""@EN; 
                     rdfs:subClassOf ddhub:Unit. 
ddhub:ShockPerSecond a owl:Class; 
                     rdfs:comment """[v] = a * [SI]
where
[v] is the value in shock per second
[SI] is the value in SI
a = Unit, i.e., 1
and
Unit = 1.0
"""@EN; 
                     rdfs:subClassOf ddhub:Unit. 
ddhub:ShockRateQuantity a owl:Class; 
                        rdfs:comment """A shock rate is the number of shocks per unit time.
The meaningful precision of shock rate is typically: 0.016666666666666666 Hz/s
"""@EN; 
                        rdfs:subClassOf ddhub:MeasurableQuantity. 
ddhub:ShoeTrack a owl:Class; 
                rdfs:comment ""@EN; 
                rdfs:subClassOf ddhub:CasingEquipment. 
ddhub:ShortDc a owl:Class; 
              rdfs:comment ""@EN; 
              rdfs:subClassOf ddhub:DrillString. 
ddhub:SiemensVolt a owl:Class; 
                  rdfs:comment """[v] = a * [SI]
where
[v] is the value in siemens volt
[SI] is the value in SI
a = 1.0/Unit, i.e., 1
and
Unit = 1.0
"""@EN; 
                  rdfs:subClassOf ddhub:Unit. 
ddhub:SignalProcessingUnit a owl:Class; 
                           rdfs:comment """Represent any signal processing applied prior to the distribution of the considered signal. Signal processing refers to e.g. noise removal, filtering,..
"""@EN; 
                           rdfs:subClassOf ddhub:Transformation. 
ddhub:SignalUncertainty a owl:Class; 
                        rdfs:comment """Represent the uncertainty associated to a `DrillingDataPoint`.
"""@EN; 
                        rdfs:subClassOf ddhub:DWISNoun. 
ddhub:Simulator a owl:Class; 
                rdfs:comment """A simulator is a computation unit that tries to replicate the outputs of a process. Its output is typically
a set of ComputedData, i.e., a specialisation of DrillingDataPoint.
"""@EN; 
                rdfs:subClassOf ddhub:ComputationUnit. 
ddhub:SingleActing a owl:Class; 
                   rdfs:comment ""@EN; 
                   rdfs:subClassOf ddhub:Action. 
ddhub:SingleJointDerrick a owl:Class; 
                         rdfs:comment ""@EN; 
                         rdfs:subClassOf ddhub:Derrick. 
ddhub:Singles a owl:Class; 
              rdfs:comment ""@EN; 
              rdfs:subClassOf ddhub:Grouping. 
ddhub:SIUnit a owl:DatatypeProperty, owl:FunctionalProperty; 
             rdfs:comment """
"""@EN; 
             rdfs:domain ddhub:Quantity; 
             rdfs:range xsd:string. 
ddhub:SlantDerrick a owl:Class; 
                   rdfs:comment ""@EN; 
                   rdfs:subClassOf ddhub:Derrick. 
ddhub:Sleeve a owl:Class; 
             rdfs:comment ""@EN; 
             rdfs:subClassOf ddhub:BladeType. 
ddhub:SlickLine a owl:Class; 
                rdfs:comment ""@EN; 
                rdfs:subClassOf ddhub:DrillFloorEquipment. 
ddhub:SlipJoint a owl:Class; 
                rdfs:comment ""@EN; 
                rdfs:subClassOf ddhub:MarineSystem. 
ddhub:SlowCirculationRateProcedure a owl:Class; 
                                   rdfs:comment """The slow circulation rate procedure is used to measure the pressure losses of the drilling system in conditions close
to what would be necessary while circulating out a kick.
"""@EN; 
                                   rdfs:subClassOf ddhub:DrillingProcedure. 
ddhub:SlugSettlingPit a owl:Class; 
                      rdfs:comment ""@EN; 
                      rdfs:subClassOf ddhub:MudPits. 
ddhub:SOEFunction a owl:Class; 
                  rdfs:comment """A `SOEFunction` is a `ProtectionFunction` that limits the commands that are send to the drilling machines
to avoid generating a drilling incident. SOE stands for Safe Operating Envelope. A `SOEFunction` protects the inputs
of the drilling process. An example `SOEFunction` is a swab/surge limits protection. This function limits the axial acceleration
and speed of the drill-stem to avoid generate swabbing pressure below the maximum of the collapse and pore pressure, and
surging pressure above the fracturing pressure.
"""@EN; 
                  rdfs:subClassOf ddhub:ProtectionFunction. 
ddhub:SolarMass a owl:Class; 
                rdfs:comment """[v] = a * [SI]
where
[v] is the value in solar mass
[SI] is the value in SI
a = 1.0/SolarMass, i.e., 5.0291176051105175E-31
and
SolarMass = 332946.0487 * EarthMass reference: https://en.wikipedia.org/wiki/Earth_mass
EarthMass = 5.9722e24 reference: https://en.wikipedia.org/wiki/Earth_mass
"""@EN; 
                rdfs:subClassOf ddhub:Unit. 
ddhub:SolidAngleQuantity a owl:Class; 
                         rdfs:comment """A solid angle is a three-dimensional angle that measures the portion of a sphere's surface subtended by an object. It is the 3D equivalent of a planar angle in two dimensions.
The dimension of solid angle is:
$$[{\\Omega}]$$.
The SI unit for **solid angle** is: steradian with the associated unit label $sr$
"""@EN; 
                         rdfs:subClassOf ddhub:Quantity. 
ddhub:SolidComponent a owl:Class; 
                     rdfs:comment ""@EN; 
                     rdfs:subClassOf ddhub:FluidComponent. 
ddhub:SpacingSpool a owl:Class; 
                   rdfs:comment ""@EN; 
                   rdfs:subClassOf ddhub:WellControlSystem. 
ddhub:Spat a owl:Class; 
           rdfs:comment """[v] = a * [SI]
where
[v] is the value in spat
[SI] is the value in SI
a = 1/(4.0*PI), i.e., 0.07957747154594767
"""@EN; 
           rdfs:subClassOf ddhub:Unit. 
ddhub:Spear a owl:Class; 
            rdfs:comment ""@EN; 
            rdfs:subClassOf ddhub:FishingTools. 
ddhub:SpecializedModel a owl:Class; 
                       rdfs:comment """A model that is tailored to specific systems, scenarios or conditions.
"""@EN; 
                       rdfs:subClassOf ddhub:ModelScope. 
ddhub:SpecificGravity a owl:Class; 
                      rdfs:comment """[v] = a * [SI]
where
[v] is the value in specific gravity
[SI] is the value in SI
a = 1.0/SpecificGavity4degC, i.e., 999.972
and
SpecificGavity4degC = 1.0 / WaterDensity4degC1Atm
WaterDensity4degC1Atm = 999.9720 reference: https://en.wikipedia.org/wiki/Relative_density
"""@EN; 
                      rdfs:subClassOf ddhub:Unit. 
ddhub:SpecificGravityPer100Metre a owl:Class; 
                                 rdfs:comment """[v] = a * [SI]
where
[v] is the value in specific gravity per 100 metre
[SI] is the value in SI
a = Hecto*SpecificGavity4degC, i.e., 0.10000280007840219
and
Hecto = 100.0
SpecificGavity4degC = 1.0 / WaterDensity4degC1Atm
WaterDensity4degC1Atm = 999.9720 reference: https://en.wikipedia.org/wiki/Relative_density
"""@EN; 
                                 rdfs:subClassOf ddhub:Unit. 
ddhub:SpecificGravityPer10Metre a owl:Class; 
                                rdfs:comment """[v] = a * [SI]
where
[v] is the value in specific gravity per 10 metre
[SI] is the value in SI
a = Deca*SpecificGavity4degC, i.e., 0.01000028000784022
and
Deca = 10.0
SpecificGavity4degC = 1.0 / WaterDensity4degC1Atm
WaterDensity4degC1Atm = 999.9720 reference: https://en.wikipedia.org/wiki/Relative_density
"""@EN; 
                                rdfs:subClassOf ddhub:Unit. 
ddhub:SpecificGravityPer30Metre a owl:Class; 
                                rdfs:comment """[v] = a * [SI]
where
[v] is the value in specific gravity per 30 metre
[SI] is the value in SI
a = 3.0*Deca*SpecificGavity4degC, i.e., 0.03000084002352066
and
Deca = 10.0
SpecificGavity4degC = 1.0 / WaterDensity4degC1Atm
WaterDensity4degC1Atm = 999.9720 reference: https://en.wikipedia.org/wiki/Relative_density
"""@EN; 
                                rdfs:subClassOf ddhub:Unit. 
ddhub:SpecificGravityPerCelsius a owl:Class; 
                                rdfs:comment """[v] = a * [SI]
where
[v] is the value in specific gravity per celsius
[SI] is the value in SI
a = SpecificGavity4degC, i.e., 0.001000028000784022
and
SpecificGavity4degC = 1.0 / WaterDensity4degC1Atm
WaterDensity4degC1Atm = 999.9720 reference: https://en.wikipedia.org/wiki/Relative_density
"""@EN; 
                                rdfs:subClassOf ddhub:Unit. 
ddhub:SpecificGravityPerHour a owl:Class; 
                             rdfs:comment """[v] = a * [SI]
where
[v] is the value in specific gravity per hour
[SI] is the value in SI
a = Hour / WaterDensity4degC1Atm, i.e., 3.600100802822479
and
Hour = 60.0 * Minute
WaterDensity4degC1Atm = 999.9720 reference: https://en.wikipedia.org/wiki/Relative_density
Minute = 60.0
"""@EN; 
                             rdfs:subClassOf ddhub:Unit. 
ddhub:SpecificGravityPerMetre a owl:Class; 
                              rdfs:comment """[v] = a * [SI]
where
[v] is the value in specific gravity per metre
[SI] is the value in SI
a = SpecificGavity4degC, i.e., 0.001000028000784022
and
SpecificGavity4degC = 1.0 / WaterDensity4degC1Atm
WaterDensity4degC1Atm = 999.9720 reference: https://en.wikipedia.org/wiki/Relative_density
"""@EN; 
                              rdfs:subClassOf ddhub:Unit. 
ddhub:SpecificGravityPerMinute a owl:Class; 
                               rdfs:comment """[v] = a * [SI]
where
[v] is the value in specific gravity per minute
[SI] is the value in SI
a = Minute / WaterDensity4degC1Atm, i.e., 0.06000168004704132
and
Minute = 60.0
WaterDensity4degC1Atm = 999.9720 reference: https://en.wikipedia.org/wiki/Relative_density
"""@EN; 
                               rdfs:subClassOf ddhub:Unit. 
ddhub:SpecificGravityPerSecond a owl:Class; 
                               rdfs:comment """[v] = a * [SI]
where
[v] is the value in specific gravity per second
[SI] is the value in SI
a = 1.0/WaterDensity4degC1Atm, i.e., 0.001000028000784022
and
WaterDensity4degC1Atm = 999.9720 reference: https://en.wikipedia.org/wiki/Relative_density
"""@EN; 
                               rdfs:subClassOf ddhub:Unit. 
ddhub:SphericalReferenceFrame a owl:Class; 
                              rdfs:comment ""@EN; 
                              rdfs:subClassOf ddhub:ThreeDimensionalReferenceFrame. 
ddhub:SpiderGimbal a owl:Class; 
                   rdfs:comment ""@EN; 
                   rdfs:subClassOf ddhub:MarineSystem. 
ddhub:Spiral a owl:Class; 
             rdfs:comment ""@EN; 
             rdfs:subClassOf ddhub:BladeShape. 
ddhub:Spm a owl:Class; 
          rdfs:comment """[v] = a * [SI]
where
[v] is the value in spm
[SI] is the value in SI
a = Minute, i.e., 60
and
Minute = 60.0
"""@EN; 
          rdfs:subClassOf ddhub:Unit. 
ddhub:SpmPerSecond a owl:Class; 
                   rdfs:comment ""@EN; 
                   rdfs:subClassOf ddhub:Unit. 
ddhub:SpontaneousPotential a owl:Class; 
                           rdfs:comment ""@EN; 
                           rdfs:subClassOf ddhub:WirelineLoggingTools. 
ddhub:SPP a owl:Class; 
          rdfs:comment ""@EN; 
          rdfs:subClassOf ddhub:PrototypeData. 
ddhub:SpudMud a owl:Class; 
              rdfs:comment ""@EN; 
              rdfs:subClassOf ddhub:DrillingFluid. 
ddhub:SquareCentimetre a owl:Class; 
                       rdfs:comment """[v] = a * [SI]
where
[v] is the value in square centimetre
[SI] is the value in SI
a = 1.0/(Centi*Centi), i.e., 10000
and
Centi = 0.01
"""@EN; 
                       rdfs:subClassOf ddhub:Unit. 
ddhub:SquareDecametre a owl:Class; 
                      rdfs:comment """[v] = a * [SI]
where
[v] is the value in square decametre
[SI] is the value in SI
a = 1.0/(Deca*Deca), i.e., 0.01
and
Deca = 10.0
"""@EN; 
                      rdfs:subClassOf ddhub:Unit. 
ddhub:SquareDecimetre a owl:Class; 
                      rdfs:comment """[v] = a * [SI]
where
[v] is the value in square decimetre
[SI] is the value in SI
a = 1.0/(Deci*Deci), i.e., 99.99999999999999
and
Deci = 0.1
"""@EN; 
                      rdfs:subClassOf ddhub:Unit. 
ddhub:SquareFoot a owl:Class; 
                 rdfs:comment """[v] = a * [SI]
where
[v] is the value in square foot
[SI] is the value in SI
a = 1.0/(Foot*Foot), i.e., 10.763910416709725
and
Foot = 12.0 * Inch
Inch = 0.0254 reference: https://www.nist.gov/pml/owm/si-units-length
"""@EN; 
                 rdfs:subClassOf ddhub:Unit. 
ddhub:SquareInch a owl:Class; 
                 rdfs:comment """[v] = a * [SI]
where
[v] is the value in square inch
[SI] is the value in SI
a = 1.0/(Inch*Inch), i.e., 1550.0031000062002
and
Inch = 0.0254 reference: https://www.nist.gov/pml/owm/si-units-length
"""@EN; 
                 rdfs:subClassOf ddhub:Unit. 
ddhub:SquareKilometre a owl:Class; 
                      rdfs:comment """[v] = a * [SI]
where
[v] is the value in square kilometre
[SI] is the value in SI
a = 1.0/(Kilo*Kilo), i.e., 1E-06
and
Kilo = 1000.0
"""@EN; 
                      rdfs:subClassOf ddhub:Unit. 
ddhub:SquareMetre a owl:Class; 
                  rdfs:comment """No conversion necessary as the unit choice is SI
"""@EN; 
                  rdfs:subClassOf ddhub:Unit. 
ddhub:SquareMicrometre a owl:Class; 
                       rdfs:comment """[v] = a * [SI]
where
[v] is the value in square micrometre
[SI] is the value in SI
a = 1.0/(Micro*Micro), i.e., 1000000000000
and
Micro = 1e-6
"""@EN; 
                       rdfs:subClassOf ddhub:Unit. 
ddhub:SquareMile a owl:Class; 
                 rdfs:comment """[v] = a * [SI]
where
[v] is the value in square mile
[SI] is the value in SI
a = 1.0/(Mile*Mile), i.e., 3.861021585424459E-07
and
Mile = 1760.0 * Yard reference: https://dictionary.cambridge.org/dictionary/english/mile
Yard = 3.0 * Foot
Foot = 12.0 * Inch
Inch = 0.0254 reference: https://www.nist.gov/pml/owm/si-units-length
"""@EN; 
                 rdfs:subClassOf ddhub:Unit. 
ddhub:SquareMillimetre a owl:Class; 
                       rdfs:comment """[v] = a * [SI]
where
[v] is the value in square millimetre
[SI] is the value in SI
a = 1.0/(Milli*Milli), i.e., 1000000
and
Milli = 0.001
"""@EN; 
                       rdfs:subClassOf ddhub:Unit. 
ddhub:SquareYard a owl:Class; 
                 rdfs:comment """[v] = a * [SI]
where
[v] is the value in square yard
[SI] is the value in SI
a = 1.0/(Yard*Yard), i.e., 1.1959900463010806
and
Yard = 3.0 * Foot
Foot = 12.0 * Inch
Inch = 0.0254 reference: https://www.nist.gov/pml/owm/si-units-length
"""@EN; 
                 rdfs:subClassOf ddhub:Unit. 
ddhub:StabbingGuide a owl:Class; 
                    rdfs:comment ""@EN; 
                    rdfs:subClassOf ddhub:DrillFloorEquipment. 
ddhub:Stabilizers a owl:Class; 
                  rdfs:comment ""@EN; 
                  rdfs:subClassOf ddhub:DrillString. 
ddhub:StableAxialForceObjective a owl:Class; 
                                rdfs:comment """This Noun is used to refer to the objective of obtaining stable axial force.
"""@EN; 
                                rdfs:subClassOf ddhub:DrillingObjective. 
ddhub:StableAxialVelocityObjective a owl:Class; 
                                   rdfs:comment """This Noun is used to refer to the objective of obtaining stable axial velocity.
"""@EN; 
                                   rdfs:subClassOf ddhub:DrillingObjective. 
ddhub:StableDrillingObjective a owl:Class; 
                              rdfs:comment """This Noun is used to refer to the objective of obtaining stable torque.
"""@EN; 
                              rdfs:subClassOf ddhub:DrillingObjective. 
ddhub:StableFlowrateObjective a owl:Class; 
                              rdfs:comment """This Noun is used to refer to the objective of obtaining stable torque.
"""@EN; 
                              rdfs:subClassOf ddhub:DrillingObjective. 
ddhub:StablePressureObjective a owl:Class; 
                              rdfs:comment """This Noun is used to refer to the objective of obtaining stable pressure.
"""@EN; 
                              rdfs:subClassOf ddhub:DrillingObjective. 
ddhub:StableRotationalVelocityObjective a owl:Class; 
                                        rdfs:comment """This Noun is used to refer to the objective of obtaining stable rotational velocity.
"""@EN; 
                                        rdfs:subClassOf ddhub:DrillingObjective. 
ddhub:StableTorqueObjective a owl:Class; 
                            rdfs:comment """This Noun is used to refer to the objective of obtaining stable torque.
"""@EN; 
                            rdfs:subClassOf ddhub:DrillingObjective. 
ddhub:StandardAtmosphere a owl:Class; 
                         rdfs:comment """[v] = a * [SI]
where
[v] is the value in standard atmosphere
[SI] is the value in SI
a = 1.0/Atmosphere, i.e., 9.869232667160129E-06
and
Atmosphere = 101325.0 reference: https://en.wikipedia.org/wiki/Atmospheric_pressure
"""@EN; 
                         rdfs:subClassOf ddhub:Unit. 
ddhub:StandardAtmospherePerHour a owl:Class; 
                                rdfs:comment """[v] = a * [SI]
where
[v] is the value in standard atmosphere per hour
[SI] is the value in SI
a = Hour/Atmosphere, i.e., 0.03552923760177646
and
Hour = 60.0 * Minute
Atmosphere = 101325.0 reference: https://en.wikipedia.org/wiki/Atmospheric_pressure
Minute = 60.0
"""@EN; 
                                rdfs:subClassOf ddhub:Unit. 
ddhub:StandardAtmospherePerMinute a owl:Class; 
                                  rdfs:comment """[v] = a * [SI]
where
[v] is the value in standard atmosphere per minute
[SI] is the value in SI
a = Minute/Atmosphere, i.e., 0.0005921539600296077
and
Minute = 60.0
Atmosphere = 101325.0 reference: https://en.wikipedia.org/wiki/Atmospheric_pressure
"""@EN; 
                                  rdfs:subClassOf ddhub:Unit. 
ddhub:StandardAtmospherePerSecond a owl:Class; 
                                  rdfs:comment """[v] = a * [SI]
where
[v] is the value in standard atmosphere per second
[SI] is the value in SI
a = 1.0/Atmosphere, i.e., 9.869232667160129E-06
and
Atmosphere = 101325.0 reference: https://en.wikipedia.org/wiki/Atmospheric_pressure
"""@EN; 
                                  rdfs:subClassOf ddhub:Unit. 
ddhub:StandardElectricalDrawworks a owl:Class; 
                                  rdfs:comment ""@EN; 
                                  rdfs:subClassOf ddhub:Drawworks. 
ddhub:Stands a owl:Class; 
             rdfs:comment ""@EN; 
             rdfs:subClassOf ddhub:Grouping. 
ddhub:StartsHydraulicBranchDecomposition a owl:ObjectProperty; 
                                         rdfs:comment ""@EN; 
                                         rdfs:domain ddhub:DWISNoun; 
                                         rdfs:range ddhub:DWISNoun; 
                                         rdfs:subPropertyOf ddhub:DWISVerb. 
ddhub:Statampere a owl:Class; 
                 rdfs:comment """[v] = a * [SI]
where
[v] is the value in statampere
[SI] is the value in SI
a = C_cgs/10.0, i.e., 2997924580
and
C_cgs = 2.99792458e10 reference: https://en.wikipedia.org/wiki/Statampere
"""@EN; 
                 rdfs:subClassOf ddhub:Unit. 
ddhub:SteadyStateModel a owl:Class; 
                       rdfs:comment """A model for which the state variables do not change with time.
"""@EN; 
                       rdfs:subClassOf ddhub:TemporalBehaviorModel. 
ddhub:Steerable a owl:Class; 
                rdfs:comment ""@EN; 
                rdfs:subClassOf ddhub:Stabilizers. 
ddhub:SteerableLinerDrilling a owl:Class; 
                             rdfs:comment ""@EN; 
                             rdfs:subClassOf ddhub:LinerDrilling. 
ddhub:SteerableMotor a owl:Class; 
                     rdfs:comment ""@EN; 
                     rdfs:subClassOf ddhub:DownholeMotor. 
ddhub:Steradian a owl:Class; 
                rdfs:comment """No conversion necessary as the unit choice is SI
"""@EN; 
                rdfs:subClassOf ddhub:Unit. 
ddhub:StickDurationDrillingQuantity a owl:Class; 
                                    rdfs:comment """Time is a continuous, measurable progression in which events occur, from the past through the present to the future.
The dimension of time is:
$$[T]$$.
The SI unit for **time** is: second with the associated unit label $s$
The meaningful precision of stick duration in the drilling context is typically: 0.001 s
"""@EN; 
                                    rdfs:subClassOf ddhub:MeasurableQuantity. 
ddhub:StickSlip a owl:Class; 
                rdfs:comment """This Noun is used to refer to stick-slips.
"""@EN; 
                rdfs:subClassOf ddhub:AbnormalTorsionalOscillation. 
ddhub:StickUpHeightVerticalLocation a owl:Class; 
                                    rdfs:comment ""@EN; 
                                    rdfs:subClassOf ddhub:VerticalReferenceLocation. 
ddhub:StochasticModel a owl:Class; 
                      rdfs:comment ""@EN; 
                      rdfs:subClassOf ddhub:ModelType. 
ddhub:Stone a owl:Class; 
            rdfs:comment """[v] = a * [SI]
where
[v] is the value in stone
[SI] is the value in SI
a = 1.0/ Stone, i.e., 0.1574730444177697
and
Stone = 14.0 * Pound reference: https://simple.wikipedia.org/wiki/Stone_(unit)
Pound = 0.45359237 reference: https://en.wikipedia.org/wiki/Pound_(mass)
"""@EN; 
            rdfs:subClassOf ddhub:Unit. 
ddhub:StorageTank a owl:Class; 
                  rdfs:comment ""@EN; 
                  rdfs:subClassOf ddhub:MudPits. 
ddhub:StormLoop a owl:Class; 
                rdfs:comment ""@EN; 
                rdfs:subClassOf ddhub:MarineSystem. 
ddhub:Straight a owl:Class; 
               rdfs:comment ""@EN; 
               rdfs:subClassOf ddhub:BladeShape. 
ddhub:StrainWaveBasedDiscretization a owl:Class; 
                                    rdfs:comment """A model can properly estimate values at the level of strain wave propagation.
"""@EN; 
                                    rdfs:subClassOf ddhub:ModellingDiscretization. 
ddhub:StratigraphyDescription a owl:Class; 
                              rdfs:comment """The stratigraphy data structure describes the type of rock, the porosity, permeability and fluid saturations
of the formation layers that are encountered along the wellbore.
"""@EN; 
                              rdfs:subClassOf ddhub:WellBoreData. 
ddhub:Stratum a owl:DatatypeProperty, owl:FunctionalProperty; 
              rdfs:comment """
"""@EN; 
              rdfs:domain ddhub:Clock; 
              rdfs:range xsd:int. 
ddhub:StressQuantity a owl:Class; 
                     rdfs:comment """Stress in a material is the internal force per unit area that arises when the material is subjected to external forces or loads. It reflects how much the material is being compressed, stretched, or sheared.
The dimension of stress is:
$$[ML^{-1}T^{-2}]$$.
The SI unit for **stress** is: pascal with the associated unit label $Pa$
"""@EN; 
                     rdfs:subClassOf ddhub:Quantity. 
ddhub:StringDataType a owl:Class; 
                     rdfs:comment ""@EN; 
                     rdfs:subClassOf ddhub:DataType. 
ddhub:StrokeFrequencyQuantity a owl:Class; 
                              rdfs:comment """A stroke frequency is the number of stokes per unit time
The meaningful precision of a stroke frequency is typically: 0.016666666666666666 Hz
"""@EN; 
                              rdfs:subClassOf ddhub:MeasurableQuantity. 
ddhub:StrokePerHour a owl:Class; 
                    rdfs:comment """[v] = a * [SI]
where
[v] is the value in stroke per hour
[SI] is the value in SI
a = Hour, i.e., 3600
and
Hour = 60.0 * Minute
Minute = 60.0
"""@EN; 
                    rdfs:subClassOf ddhub:Unit. 
ddhub:StrokePerSecond a owl:Class; 
                      rdfs:comment """[v] = a * [SI]
where
[v] is the value in stroke per second
[SI] is the value in SI
a = Unit, i.e., 1
and
Unit = 1.0
"""@EN; 
                      rdfs:subClassOf ddhub:Unit. 
ddhub:StuckPipe a owl:Class; 
                rdfs:comment """This Noun is used to refer to a situation during which the drill-stem is impeded to move either axially or rotationally or both.
"""@EN; 
                rdfs:subClassOf ddhub:DrillingIncident. 
ddhub:StuckPipeFeature a owl:Class; 
                       rdfs:comment """A stuck-pipe feature indicates that something accounts for stuck-pipes.
"""@EN; 
                       rdfs:subClassOf ddhub:DrillStemMovementFeature. 
ddhub:Subbent a owl:Class; 
              rdfs:comment ""@EN; 
              rdfs:subClassOf ddhub:MiscSubs. 
ddhub:Subbit a owl:Class; 
             rdfs:comment ""@EN; 
             rdfs:subClassOf ddhub:MiscSubs. 
ddhub:Subbumper a owl:Class; 
                rdfs:comment ""@EN; 
                rdfs:subClassOf ddhub:MiscSubs. 
ddhub:Subcatcher a owl:Class; 
                 rdfs:comment ""@EN; 
                 rdfs:subClassOf ddhub:MiscSubs. 
ddhub:Subcirculation a owl:Class; 
                     rdfs:comment ""@EN; 
                     rdfs:subClassOf ddhub:MiscSubs. 
ddhub:Subcone a owl:Class; 
              rdfs:comment ""@EN; 
              rdfs:subClassOf ddhub:MiscSubs. 
ddhub:Subcrossover a owl:Class; 
                   rdfs:comment ""@EN; 
                   rdfs:subClassOf ddhub:MiscSubs. 
ddhub:Subdart a owl:Class; 
              rdfs:comment ""@EN; 
              rdfs:subClassOf ddhub:MiscSubs. 
ddhub:Subfilter a owl:Class; 
                rdfs:comment ""@EN; 
                rdfs:subClassOf ddhub:MiscSubs. 
ddhub:Subfloat a owl:Class; 
               rdfs:comment ""@EN; 
               rdfs:subClassOf ddhub:MiscSubs. 
ddhub:Subjetting a owl:Class; 
                 rdfs:comment ""@EN; 
                 rdfs:subClassOf ddhub:MiscSubs. 
ddhub:Subjunk a owl:Class; 
              rdfs:comment ""@EN; 
              rdfs:subClassOf ddhub:MiscSubs. 
ddhub:Suborienting a owl:Class; 
                   rdfs:comment ""@EN; 
                   rdfs:subClassOf ddhub:MiscSubs. 
ddhub:Subported a owl:Class; 
                rdfs:comment ""@EN; 
                rdfs:subClassOf ddhub:MiscSubs. 
ddhub:SubpressureRelief a owl:Class; 
                        rdfs:comment ""@EN; 
                        rdfs:subClassOf ddhub:MiscSubs. 
ddhub:SubpumpOut a owl:Class; 
                 rdfs:comment ""@EN; 
                 rdfs:subClassOf ddhub:MiscSubs. 
ddhub:Subrestrictor a owl:Class; 
                    rdfs:comment ""@EN; 
                    rdfs:subClassOf ddhub:MiscSubs. 
ddhub:Subsaver a owl:Class; 
               rdfs:comment ""@EN; 
               rdfs:subClassOf ddhub:MiscSubs. 
ddhub:SubseaBop a owl:Class; 
                rdfs:comment ""@EN; 
                rdfs:subClassOf ddhub:BopStack. 
ddhub:SubseaTestTree a owl:Class; 
                     rdfs:comment ""@EN; 
                     rdfs:subClassOf ddhub:WellTestingEquipment. 
ddhub:Subshock a owl:Class; 
               rdfs:comment ""@EN; 
               rdfs:subClassOf ddhub:MiscSubs. 
ddhub:SubsideEntry a owl:Class; 
                   rdfs:comment ""@EN; 
                   rdfs:subClassOf ddhub:MiscSubs. 
ddhub:Substop a owl:Class; 
              rdfs:comment ""@EN; 
              rdfs:subClassOf ddhub:MiscSubs. 
ddhub:SupportLine a owl:Class; 
                  rdfs:comment ""@EN; 
                  rdfs:subClassOf ddhub:DrillLine. 
ddhub:SurfaceBop a owl:Class; 
                 rdfs:comment ""@EN; 
                 rdfs:subClassOf ddhub:BopStack. 
ddhub:SurfacePoreDrillingQuantity a owl:Class; 
                                  rdfs:comment """Area is the measure of the extent of a surface or the size of a two-dimensional shape.
The dimension of area is:
$$[L^{2}]$$.
The SI unit for **area** is: square metre with the associated unit label $m^{2}$
The meaningful precision of pore surface in the drilling context is typically: 1E-13 m²
"""@EN; 
                                  rdfs:subClassOf ddhub:MeasurableQuantity. 
ddhub:SurfacePower a owl:Class; 
                   rdfs:comment ""@EN; 
                   rdfs:subClassOf ddhub:PowerSystems. 
ddhub:SurfaceRiser a owl:Class; 
                   rdfs:comment ""@EN; 
                   rdfs:subClassOf ddhub:DrillingRiser. 
ddhub:SurfaceRotationSystem a owl:Class; 
                            rdfs:comment ""@EN; 
                            rdfs:subClassOf ddhub:RigEquipment. 
ddhub:SurfaceRPM a owl:Class; 
                 rdfs:comment ""@EN; 
                 rdfs:subClassOf ddhub:PrototypeData. 
ddhub:SurfaceTorque a owl:Class; 
                    rdfs:comment ""@EN; 
                    rdfs:subClassOf ddhub:PrototypeData. 
ddhub:SurgeTank a owl:Class; 
                rdfs:comment ""@EN; 
                rdfs:subClassOf ddhub:MudPits. 
ddhub:SurveyorSChain a owl:Class; 
                     rdfs:comment """[v] = a * [SI]
where
[v] is the value in surveyor's chain
[SI] is the value in SI
a = 1.0/SurveyorChain, i.e., 0.04970969537898672
and
SurveyorChain = 22.0 * Yard reference: https://www.britannica.com/technology/surveyors-chain
Yard = 3.0 * Foot
Foot = 12.0 * Inch
Inch = 0.0254 reference: https://www.nist.gov/pml/owm/si-units-length
"""@EN; 
                     rdfs:subClassOf ddhub:Unit. 
ddhub:SwabSurgeFeature a owl:Class; 
                       rdfs:comment """A swab and surge feature indicates that something accounts for swab and surge pressure variations.
"""@EN; 
                       rdfs:subClassOf ddhub:DownholePressureFeature. 
ddhub:SwivelSub a owl:Class; 
                rdfs:comment ""@EN; 
                rdfs:subClassOf ddhub:TopDrive. 
ddhub:Symbol a owl:DatatypeProperty, owl:FunctionalProperty; 
             rdfs:comment """a typical label for that unit.
"""@EN; 
             rdfs:domain ddhub:Unit; 
             rdfs:range xsd:string. 
ddhub:SynchronizationDelay a owl:DatatypeProperty, owl:FunctionalProperty; 
                           rdfs:comment """
"""@EN; 
                           rdfs:domain ddhub:SynchronizationGroup; 
                           rdfs:range xsd:double. 
ddhub:SynchronizationGroup a owl:Class; 
                           rdfs:comment ""@EN; 
                           rdfs:subClassOf ddhub:DWISNoun. 
ddhub:SyntheticOilBasedMudSobm a owl:Class; 
                               rdfs:comment ""@EN; 
                               rdfs:subClassOf ddhub:DrillingFluid. 
ddhub:T a owl:DatatypeProperty, owl:FunctionalProperty; 
        rdfs:comment """Time exponent.
SI Unit: Second (s)
"""@EN; 
        rdfs:domain ddhub:Quantity; 
        rdfs:range xsd:double. 
ddhub:TagBottomProcedure a owl:Class; 
                         rdfs:comment """The tag bottom procedure is used to tag the bottom hole and establish the drilling parameters.
"""@EN; 
                         rdfs:subClassOf ddhub:DrillingProcedure. 
ddhub:TangencyLength a owl:Class; 
                     rdfs:comment """the position along the drill-string, counted from the bit, from which we can consider that the pipes direction is tangential with the borehole direction.
"""@EN; 
                     rdfs:subClassOf ddhub:DWISNoun. 
ddhub:TangentialModelling a owl:Class; 
                          rdfs:comment """The model accounts for the change of tangential direction of some parts of the physical system.
"""@EN; 
                          rdfs:subClassOf ddhub:LateralModelling. 
ddhub:Tank a owl:Class; 
           rdfs:comment ""@EN; 
           rdfs:subClassOf ddhub:HydraulicLogicalElement. 
ddhub:TaskStep a owl:Class; 
               rdfs:comment """A task step is at the third level of a rig action plan.
"""@EN; 
               rdfs:subClassOf ddhub:OperationalStep. 
ddhub:Telemetry a owl:Class; 
                rdfs:comment """Technology used for transferring the data from its main origin.
"""@EN; 
                rdfs:subClassOf ddhub:DWISNoun. 
ddhub:TemperatureDrillingQuantity a owl:Class; 
                                  rdfs:comment """Temperature is a measure of the average kinetic energy of particles in a substance, indicating how hot or cold the substance is.
The dimension of temperature is:
$$[K]$$.
The SI unit for **temperature** is: kelvin with the associated unit label $K$
The meaningful precision of temperature in the drilling context is typically: 0.01 K
"""@EN; 
                                  rdfs:subClassOf ddhub:MeasurableQuantity. 
ddhub:TemperatureGradientPerLengthDrillingQuantity a owl:Class; 
                                                   rdfs:comment """A temperature gradient per lenth is the first derivative of a temperature compared to a distance: $\\frac{dT}{ds}$, where $T$ is a temperature and $s$ is a distance.
The dimension of temperature gradient per length is:
$$[KL^{-1}]$$.
The SI unit for **temperature gradient per length** is: kelvin per metre with the associated unit label $\\frac{K}{m}$
The meaningful precision of temperature gradient per length in the drilling context is typically: 0.001 K/m
"""@EN; 
                                                   rdfs:subClassOf ddhub:MeasurableQuantity. 
ddhub:TemperatureGradientPerLengthQuantity a owl:Class; 
                                           rdfs:comment """A temperature gradient per lenth is the first derivative of a temperature compared to a distance: $\\frac{dT}{ds}$, where $T$ is a temperature and $s$ is a distance.
The dimension of temperature gradient per length is:
$$[KL^{-1}]$$.
The SI unit for **temperature gradient per length** is: kelvin per metre with the associated unit label $\\frac{K}{m}$
"""@EN; 
                                           rdfs:subClassOf ddhub:Quantity. 
ddhub:TemperatureIn a owl:Class; 
                    rdfs:comment ""@EN; 
                    rdfs:subClassOf ddhub:PrototypeData. 
ddhub:TemperatureOut a owl:Class; 
                     rdfs:comment ""@EN; 
                     rdfs:subClassOf ddhub:PrototypeData. 
ddhub:TemperatureQuantity a owl:Class; 
                          rdfs:comment """Temperature is a measure of the average kinetic energy of particles in a substance, indicating how hot or cold the substance is.
The dimension of temperature is:
$$[K]$$.
The SI unit for **temperature** is: kelvin with the associated unit label $K$
"""@EN; 
                          rdfs:subClassOf ddhub:Quantity. 
ddhub:TemporalBehaviorModel a owl:Class; 
                            rdfs:comment """A classification of a model as a function of its temporal behavior.
"""@EN; 
                            rdfs:subClassOf ddhub:DWISNoun. 
ddhub:TensionDrillingQuantity a owl:Class; 
                              rdfs:comment """Tension is the pulling or stretching force transmitted axially along an object such as a string, rope, chain, rod, truss member, or other object, so as to stretch or pull apart the object. In terms of force, it is the opposite of compression. Tension might also be described as the action-reaction pair of forces acting at each end of an object.
The dimension of tension is:
$$[LMT^{-2}]$$.
The meaningful precision of tension in the drilling context is typically: 100 N
"""@EN; 
                              rdfs:subClassOf ddhub:MeasurableQuantity. 
ddhub:TensionQuantity a owl:Class; 
                      rdfs:comment """Tension is the pulling or stretching force transmitted axially along an object such as a string, rope, chain, rod, truss member, or other object, so as to stretch or pull apart the object. In terms of force, it is the opposite of compression. Tension might also be described as the action-reaction pair of forces acting at each end of an object.
The dimension of tension is:
$$[LMT^{-2}]$$.
"""@EN; 
                      rdfs:subClassOf ddhub:Quantity. 
ddhub:Teraampere a owl:Class; 
                 rdfs:comment """[v] = a * [SI]
where
[v] is the value in teraampere
[SI] is the value in SI
a = 1.0/Tera, i.e., 1E-12
and
Tera = 1e12
"""@EN; 
                 rdfs:subClassOf ddhub:Unit. 
ddhub:Terahertz a owl:Class; 
                rdfs:comment """[v] = a * [SI]
where
[v] is the value in terahertz
[SI] is the value in SI
a = 1.0/Tera, i.e., 1E-12
and
Tera = 1e12
"""@EN; 
                rdfs:subClassOf ddhub:Unit. 
ddhub:Terawatt a owl:Class; 
               rdfs:comment """[v] = a * [SI]
where
[v] is the value in terawatt
[SI] is the value in SI
a = 1.0/Tera, i.e., 1E-12
and
Tera = 1e12
"""@EN; 
               rdfs:subClassOf ddhub:Unit. 
ddhub:Tesla a owl:Class; 
            rdfs:comment """No conversion necessary as the unit choice is SI
"""@EN; 
            rdfs:subClassOf ddhub:Unit. 
ddhub:TeslaSquareCentimetre a owl:Class; 
                            rdfs:comment """[v] = a * [SI]
where
[v] is the value in tesla square centimetre
[SI] is the value in SI
a = 1.0/(Unit *Centi*Centi), i.e., 10000
and
Unit = 1.0
Centi = 0.01
"""@EN; 
                            rdfs:subClassOf ddhub:Unit. 
ddhub:TeslaSquareMetre a owl:Class; 
                       rdfs:comment """[v] = a * [SI]
where
[v] is the value in tesla square metre
[SI] is the value in SI
a = 1.0/Unit, i.e., 1
and
Unit = 1.0
"""@EN; 
                       rdfs:subClassOf ddhub:Unit. 
ddhub:TestingTools a owl:Class; 
                   rdfs:comment ""@EN; 
                   rdfs:subClassOf ddhub:WellTestingEquipment. 
ddhub:TestPlug a owl:Class; 
               rdfs:comment ""@EN; 
               rdfs:subClassOf ddhub:WellTestingEquipment. 
ddhub:TestTools a owl:Class; 
                rdfs:comment ""@EN; 
                rdfs:subClassOf ddhub:WellTestingEquipment. 
ddhub:ThermalConductivityDrillingQuantity a owl:Class; 
                                          rdfs:comment """Thermal conductivity is a material's ability to conduct heat. It measures how efficiently heat is transferred through a material when there is a temperature difference.
The dimension of thermal conductivity is:
$$[LMK^{-1}T^{-3}]$$.
The SI unit for **thermal conductivity** is: watt per metre kelvin with the associated unit label $\\frac{W}{m \\cdot K}$
The meaningful precision of thermal conductivity in the drilling context is typically: 0.01 W/m•K
"""@EN; 
                                          rdfs:subClassOf ddhub:MeasurableQuantity. 
ddhub:ThermalConductivityGradientPerTemperatureDrillingQuantity a owl:Class; 
                                                                rdfs:comment """A thermal conductivity gradient per temperature is the first derivative of a thermal conductivity compared to temperature: $\\frac{dk}{dT}$, where $k$ is a thermal conductivity and $T$ is temperature. 
The dimension of thermal conductivity gradient per temperature is:
$$[LMK^{-2}T^{-3}]$$.
The SI unit for **thermal conductivity gradient per temperature** is: watt per metre kelvin per kelvin with the associated unit label $\\frac{(\\frac{W}{(m \\cdot K)}}{K}$
The meaningful precision of thermal conductivity gradient per temperature in the drilling context is typically: 0.01 (W/(m•K))/K
"""@EN; 
                                                                rdfs:subClassOf ddhub:MeasurableQuantity. 
ddhub:ThermalConductivityGradientPerTemperatureQuantity a owl:Class; 
                                                        rdfs:comment """A thermal conductivity gradient per temperature is the first derivative of a thermal conductivity compared to temperature: $\\frac{dk}{dT}$, where $k$ is a thermal conductivity and $T$ is temperature. 
The dimension of thermal conductivity gradient per temperature is:
$$[LMK^{-2}T^{-3}]$$.
The SI unit for **thermal conductivity gradient per temperature** is: watt per metre kelvin per kelvin with the associated unit label $\\frac{(\\frac{W}{(m \\cdot K)}}{K}$
"""@EN; 
                                                        rdfs:subClassOf ddhub:Quantity. 
ddhub:ThermalConductivityQuantity a owl:Class; 
                                  rdfs:comment """Thermal conductivity is a material's ability to conduct heat. It measures how efficiently heat is transferred through a material when there is a temperature difference.
The dimension of thermal conductivity is:
$$[LMK^{-1}T^{-3}]$$.
The SI unit for **thermal conductivity** is: watt per metre kelvin with the associated unit label $\\frac{W}{m \\cdot K}$
"""@EN; 
                                  rdfs:subClassOf ddhub:Quantity. 
ddhub:Theta a owl:DatatypeProperty, owl:FunctionalProperty; 
            rdfs:comment """plane angle exponent.
SI Unit: radian (rad)
"""@EN; 
            rdfs:domain ddhub:Quantity; 
            rdfs:range xsd:double. 
ddhub:ThirdPartyRigEquipment a owl:Class; 
                             rdfs:comment ""@EN; 
                             rdfs:subClassOf ddhub:RigEquipment. 
ddhub:ThirdPartyTools a owl:Class; 
                      rdfs:comment ""@EN; 
                      rdfs:subClassOf ddhub:ThirdPartyRigEquipment. 
ddhub:Thou a owl:Class; 
           rdfs:comment """[v] = a * [SI]
where
[v] is the value in thou
[SI] is the value in SI
a = 1.0/Thou, i.e., 39370.07874015748
and
Thou = Mil
Mil = 0.001 * Inch reference: https://en.wikipedia.org/wiki/Thousandth_of_an_inch
Inch = 0.0254 reference: https://www.nist.gov/pml/owm/si-units-length
"""@EN; 
           rdfs:subClassOf ddhub:Unit. 
ddhub:ThousandStandardCubicFoot a owl:Class; 
                                rdfs:comment """[v] = a * [SI]
where
[v] is the value in thousand standard cubic foot
[SI] is the value in SI
a = 1.0/(Kilo*Foot*Foot*Foot), i.e., 0.0353146667214886
and
Kilo = 1000.0
Foot = 12.0 * Inch
Inch = 0.0254 reference: https://www.nist.gov/pml/owm/si-units-length
"""@EN; 
                                rdfs:subClassOf ddhub:Unit. 
ddhub:ThousandStandardCubicFootPerDay a owl:Class; 
                                      rdfs:comment """[v] = a * [SI]
where
[v] is the value in thousand standard cubic foot per day
[SI] is the value in SI
a = Day / (1000.0*Foot*Foot*Foot), i.e., 3051.187204736615
and
Day = 24.0 * Hour
Foot = 12.0 * Inch
Hour = 60.0 * Minute
Inch = 0.0254 reference: https://www.nist.gov/pml/owm/si-units-length
Minute = 60.0
"""@EN; 
                                      rdfs:subClassOf ddhub:Unit. 
ddhub:ThreeDimensionalReferenceFrame a owl:Class; 
                                     rdfs:comment ""@EN; 
                                     rdfs:subClassOf ddhub:ReferenceFrame. 
ddhub:ThreeDModelling a owl:Class; 
                      rdfs:comment """The model only accounts for three dimensions
"""@EN; 
                      rdfs:subClassOf ddhub:ModellingDimensions. 
ddhub:ThreeWayManifold a owl:Class; 
                       rdfs:comment ""@EN; 
                       rdfs:subClassOf ddhub:GenericEquipment. 
ddhub:ThreeWayValve a owl:Class; 
                    rdfs:comment ""@EN; 
                    rdfs:subClassOf ddhub:GenericEquipment. 
ddhub:Thruster a owl:Class; 
               rdfs:comment ""@EN; 
               rdfs:subClassOf ddhub:DrillingEquipment. 
ddhub:ThT a owl:DatatypeProperty, owl:FunctionalProperty; 
          rdfs:comment """Thermodynamic temperature exponent.
SI Unit: Kelvin (K)
"""@EN; 
          rdfs:domain ddhub:Quantity; 
          rdfs:range xsd:double. 
ddhub:TimeBasedTransformation a owl:Class; 
                              rdfs:comment """Transformations that apply only to time series: time derivations, time integration, averaging...
"""@EN; 
                              rdfs:subClassOf ddhub:Transformation. 
ddhub:TimeQuantity a owl:Class; 
                   rdfs:comment """Time is a continuous, measurable progression in which events occur, from the past through the present to the future.
The dimension of time is:
$$[T]$$.
The SI unit for **time** is: second with the associated unit label $s$
"""@EN; 
                   rdfs:subClassOf ddhub:Quantity. 
ddhub:TimeReference a owl:Class; 
                    rdfs:comment ""@EN; 
                    rdfs:subClassOf ddhub:DWISNoun. 
ddhub:TimeSpanReference a owl:Class; 
                        rdfs:comment ""@EN; 
                        rdfs:subClassOf ddhub:RelativeTimeReference. 
ddhub:TimeStampAcquisition a owl:DatatypeProperty, owl:FunctionalProperty; 
                           rdfs:comment """this is a UTC date-time value at which the value has been acquired by the data acquisition system.
"""@EN; 
                           rdfs:domain ddhub:DynamicDrillingSignal; 
                           rdfs:range xsd:datetime. 
ddhub:TimeStampAtSource a owl:DatatypeProperty, owl:FunctionalProperty; 
                        rdfs:comment """this is a UTC date-time value corresponding to the time at which the value has been taken.
"""@EN; 
                        rdfs:domain ddhub:DynamicDrillingSignal; 
                        rdfs:range xsd:datetime. 
ddhub:TimeWindow a owl:DatatypeProperty, owl:FunctionalProperty; 
                 rdfs:comment """
"""@EN; 
                 rdfs:domain ddhub:TimeWindowMovingAverage, ddhub:TimeWindowRangeExtraction; 
                 rdfs:range xsd:double. 
ddhub:TimeWindowMovingAverage a owl:Class; 
                              rdfs:comment ""@EN; 
                              rdfs:subClassOf ddhub:MovingAverage. 
ddhub:TimeWindowRangeExtraction a owl:Class; 
                                rdfs:comment ""@EN; 
                                rdfs:subClassOf ddhub:RangeExtraction. 
ddhub:TonneMetric a owl:Class; 
                  rdfs:comment """[v] = a * [SI]
where
[v] is the value in tonne metric
[SI] is the value in SI
a = 1.0/Kilo, i.e., 0.001
and
Kilo = 1000.0
"""@EN; 
                  rdfs:subClassOf ddhub:Unit. 
ddhub:TonUk a owl:Class; 
            rdfs:comment """[v] = a * [SI]
where
[v] is the value in ton UK
[SI] is the value in SI
a = 1.0 / TonUK, i.e., 0.0009842065276110606
and
TonUK = 2240.0 * Pound reference: https://en.wikipedia.org/wiki/Ton
Pound = 0.45359237 reference: https://en.wikipedia.org/wiki/Pound_(mass)
"""@EN; 
            rdfs:subClassOf ddhub:Unit. 
ddhub:TonUs a owl:Class; 
            rdfs:comment """[v] = a * [SI]
where
[v] is the value in ton US
[SI] is the value in SI
a = 1.0/ TonUS, i.e., 0.001102311310924388
and
TonUS = 2000.0 * Pound reference: https://en.wikipedia.org/wiki/Ton
Pound = 0.45359237 reference: https://en.wikipedia.org/wiki/Pound_(mass)
"""@EN; 
            rdfs:subClassOf ddhub:Unit. 
ddhub:ToolfaceOrientationProcedure a owl:Class; 
                                   rdfs:comment """The toolface orientation procedure is used to manipulate the top of string angular position to ensure that the downhole
motor toolface is set to a desired set-point.
"""@EN; 
                                   rdfs:subClassOf ddhub:DrillingProcedure. 
ddhub:ToolJoint1ReferenceLocation a owl:Class; 
                                  rdfs:comment ""@EN; 
                                  rdfs:subClassOf ddhub:AbscissaReferenceLocation. 
ddhub:ToolJoint2ReferenceLocation a owl:Class; 
                                  rdfs:comment ""@EN; 
                                  rdfs:subClassOf ddhub:AbscissaReferenceLocation. 
ddhub:ToolJoint3ReferenceLocation a owl:Class; 
                                  rdfs:comment ""@EN; 
                                  rdfs:subClassOf ddhub:AbscissaReferenceLocation. 
ddhub:ToolJoint4ReferenceLocation a owl:Class; 
                                  rdfs:comment ""@EN; 
                                  rdfs:subClassOf ddhub:AbscissaReferenceLocation. 
ddhub:TopDrive a owl:Class; 
               rdfs:comment ""@EN; 
               rdfs:subClassOf ddhub:SurfaceRotationSystem. 
ddhub:TopOfRatHoleLocation a owl:Class; 
                           rdfs:comment ""@EN; 
                           rdfs:subClassOf ddhub:AbscissaReferenceLocation. 
ddhub:TopOfStringPosition a owl:Class; 
                          rdfs:comment ""@EN; 
                          rdfs:subClassOf ddhub:PrototypeData. 
ddhub:TopOfStringReferenceLocation a owl:Class; 
                                   rdfs:comment ""@EN; 
                                   rdfs:subClassOf ddhub:AbscissaReferenceLocation. 
ddhub:TopShoulderAxialLocation a owl:Class; 
                               rdfs:comment ""@EN; 
                               rdfs:subClassOf ddhub:AxialReferenceLocation. 
ddhub:TopsideHydraulicNetwork a owl:Class; 
                              rdfs:comment ""@EN; 
                              rdfs:subClassOf ddhub:HydraulicNetwork. 
ddhub:TopSideTelemetry a owl:Class; 
                       rdfs:comment """Method that allows transfer of data from surface systems.
"""@EN; 
                       rdfs:subClassOf ddhub:Telemetry. 
ddhub:TorqueBushing a owl:Class; 
                    rdfs:comment ""@EN; 
                    rdfs:subClassOf ddhub:TopDrive. 
ddhub:TorqueDrillingQuantity a owl:Class; 
                             rdfs:comment """A torque is a measure of the rotational force applied to a body around an axis.
The dimension of torque is:
$$[L^{2}MT^{-2}]$$.
The SI unit for **torque** is: newton metre with the associated unit label $N \\cdot m$
The meaningful precision of torque in the drilling context is typically: 0.1 N•m
"""@EN; 
                             rdfs:subClassOf ddhub:MeasurableQuantity. 
ddhub:TorqueGradientPerLengthDrillingQuantity a owl:Class; 
                                              rdfs:comment """A torque gradient per length is the first derivative of torque compared to a distance: $\\frac{d\\tau}{ds}$, where $\\tau$ is a torque and $s$ is a distance.
The dimension of torque gradient per length is:
$$[LMT^{-2}]$$.
The SI unit for **torque gradient per length** is: newton metre per metre with the associated unit label $\\frac{N \\cdot m}{m}$
The meaningful precision of torque gradient per length in the drilling context is typically: 1 N•m/m
"""@EN; 
                                              rdfs:subClassOf ddhub:MeasurableQuantity. 
ddhub:TorqueGradientPerLengthQuantity a owl:Class; 
                                      rdfs:comment """A torque gradient per length is the first derivative of torque compared to a distance: $\\frac{d\\tau}{ds}$, where $\\tau$ is a torque and $s$ is a distance.
The dimension of torque gradient per length is:
$$[LMT^{-2}]$$.
The SI unit for **torque gradient per length** is: newton metre per metre with the associated unit label $\\frac{N \\cdot m}{m}$
"""@EN; 
                                      rdfs:subClassOf ddhub:Quantity. 
ddhub:TorqueLimit a owl:Class; 
                  rdfs:comment """This Noun is used to refer to a torque limit.
"""@EN; 
                  rdfs:subClassOf ddhub:DrillingLimit. 
ddhub:TorqueQuantity a owl:Class; 
                     rdfs:comment """A torque is a measure of the rotational force applied to a body around an axis.
The dimension of torque is:
$$[L^{2}MT^{-2}]$$.
The SI unit for **torque** is: newton metre with the associated unit label $N \\cdot m$
"""@EN; 
                     rdfs:subClassOf ddhub:Quantity. 
ddhub:TorqueRateOfChangeDrillingQuantity a owl:Class; 
                                         rdfs:comment """A torque rate of change is the time derivative of a torque.
The dimension of torque rate of change is:
$$[L^{2}MT^{-3}]$$.
The SI unit for **torque** is: newton metre per second with the associated unit label $\\frac{N \\cdot m}{s}$
The meaningful precision of torque rate of change in the drilling context is typically: 0.1 N•m/s
"""@EN; 
                                         rdfs:subClassOf ddhub:MeasurableQuantity. 
ddhub:TorqueRateOfChangeQuantity a owl:Class; 
                                 rdfs:comment """A torque rate of change is the time derivative of a torque.
The dimension of torque rate of change is:
$$[L^{2}MT^{-3}]$$.
The SI unit for **torque** is: newton metre per second with the associated unit label $\\frac{N \\cdot m}{s}$
"""@EN; 
                                 rdfs:subClassOf ddhub:Quantity. 
ddhub:TorqueSmallQuantity a owl:Class; 
                          rdfs:comment """A torque is a measure of the rotational force applied to a body around an axis.
The dimension of torque is:
$$[L^{2}MT^{-2}]$$.
The SI unit for **torque** is: newton metre with the associated unit label $N \\cdot m$
The meaningful precision of small torque is typically: 1E-05 N•m
"""@EN; 
                          rdfs:subClassOf ddhub:MeasurableQuantity. 
ddhub:TorqueToForceTransformation a owl:Class; 
                                  rdfs:comment ""@EN; 
                                  rdfs:subClassOf ddhub:DirectTransformation. 
ddhub:TorqueTrack a owl:Class; 
                  rdfs:comment ""@EN; 
                  rdfs:subClassOf ddhub:TopDrive. 
ddhub:Torr a owl:Class; 
           rdfs:comment """[v] = a * [SI]
where
[v] is the value in torr
[SI] is the value in SI
a = 1.0/Torr, i.e., 0.007500616827041697
and
Torr = (1.0 / 760.0) * Atmosphere reference: https://en.wikipedia.org/wiki/Torr
Atmosphere = 101325.0 reference: https://en.wikipedia.org/wiki/Atmospheric_pressure
"""@EN; 
           rdfs:subClassOf ddhub:Unit. 
ddhub:TorrPerHour a owl:Class; 
                  rdfs:comment """[v] = a * [SI]
where
[v] is the value in torr per hour
[SI] is the value in SI
a = Hour/Torr, i.e., 27.002220577350112
and
Hour = 60.0 * Minute
Torr = (1.0 / 760.0) * Atmosphere reference: https://en.wikipedia.org/wiki/Torr
Minute = 60.0
Atmosphere = 101325.0 reference: https://en.wikipedia.org/wiki/Atmospheric_pressure
"""@EN; 
                  rdfs:subClassOf ddhub:Unit. 
ddhub:TorrPerMinute a owl:Class; 
                    rdfs:comment """[v] = a * [SI]
where
[v] is the value in torr per minute
[SI] is the value in SI
a = Minute/Torr, i.e., 0.45003700962250187
and
Minute = 60.0
Torr = (1.0 / 760.0) * Atmosphere reference: https://en.wikipedia.org/wiki/Torr
Atmosphere = 101325.0 reference: https://en.wikipedia.org/wiki/Atmospheric_pressure
"""@EN; 
                    rdfs:subClassOf ddhub:Unit. 
ddhub:TorrPerSecond a owl:Class; 
                    rdfs:comment """[v] = a * [SI]
where
[v] is the value in torr per second
[SI] is the value in SI
a = 1.0/Torr, i.e., 0.007500616827041697
and
Torr = (1.0 / 760.0) * Atmosphere reference: https://en.wikipedia.org/wiki/Torr
Atmosphere = 101325.0 reference: https://en.wikipedia.org/wiki/Atmospheric_pressure
"""@EN; 
                    rdfs:subClassOf ddhub:Unit. 
ddhub:TorsionalMotionType a owl:Class; 
                          rdfs:comment ""@EN; 
                          rdfs:subClassOf ddhub:MotionType. 
ddhub:TrajectoryDescription a owl:Class; 
                            rdfs:comment """A trajectory contains information about the position of the wellbore.
"""@EN; 
                            rdfs:subClassOf ddhub:WellBoreData. 
ddhub:Transformation a owl:Class; 
                     rdfs:comment """Represents a transformation applied to some signals that produces other signals
"""@EN; 
                     rdfs:subClassOf ddhub:DataFlowNode. 
ddhub:TransientModel a owl:Class; 
                     rdfs:comment """A model for which the state variables changes with time.
"""@EN; 
                     rdfs:subClassOf ddhub:TemporalBehaviorModel. 
ddhub:TransmissionLine a owl:Class; 
                       rdfs:comment ""@EN; 
                       rdfs:subClassOf ddhub:DataFlowNode. 
ddhub:TravellingBlock a owl:Class; 
                      rdfs:comment ""@EN; 
                      rdfs:subClassOf ddhub:MechanicalBlock. 
ddhub:TripleStandDerrick a owl:Class; 
                         rdfs:comment ""@EN; 
                         rdfs:subClassOf ddhub:Derrick. 
ddhub:TripTank a owl:Class; 
               rdfs:comment ""@EN; 
               rdfs:subClassOf ddhub:MudPits. 
ddhub:TrueNorthAzimuthLocation a owl:Class; 
                               rdfs:comment ""@EN; 
                               rdfs:subClassOf ddhub:AzimuthReferenceLocation. 
ddhub:TubingGuideArch a owl:Class; 
                      rdfs:comment ""@EN; 
                      rdfs:subClassOf ddhub:CoiledTubingEquipment. 
ddhub:TubingHanger a owl:Class; 
                   rdfs:comment ""@EN; 
                   rdfs:subClassOf ddhub:Hangers. 
ddhub:TubingString a owl:Class; 
                   rdfs:comment ""@EN; 
                   rdfs:subClassOf ddhub:Tubulars. 
ddhub:TubularConfiguration a owl:Class; 
                           rdfs:comment ""@EN; 
                           rdfs:subClassOf ddhub:Tubulars. 
ddhub:TubularConnection a owl:Class; 
                        rdfs:comment ""@EN; 
                        rdfs:subClassOf ddhub:Tubulars. 
ddhub:Tubulars a owl:Class; 
               rdfs:comment ""@EN; 
               rdfs:subClassOf ddhub:Equipment. 
ddhub:TurbineMotor a owl:Class; 
                   rdfs:comment ""@EN; 
                   rdfs:subClassOf ddhub:DownholeMotor. 
ddhub:TwistOff a owl:Class; 
               rdfs:comment """This Noun is used to refer to a twist-off situation.
"""@EN; 
               rdfs:subClassOf ddhub:DrillingIncident. 
ddhub:TwoDimensionalReferenceFrame a owl:Class; 
                                   rdfs:comment ""@EN; 
                                   rdfs:subClassOf ddhub:ReferenceFrame. 
ddhub:TwoDModelling a owl:Class; 
                    rdfs:comment """The model only accounts for two dimensions
"""@EN; 
                    rdfs:subClassOf ddhub:ModellingDimensions. 
ddhub:UkGallon a owl:Class; 
               rdfs:comment """[v] = a * [SI]
where
[v] is the value in UK gallon
[SI] is the value in SI
a = 1.0/GallonUK, i.e., 219.96924829908778
and
GallonUK = 4.54609e-3 reference: https://en.wikipedia.org/wiki/Gallon
"""@EN; 
               rdfs:subClassOf ddhub:Unit. 
ddhub:UkGallonPerDay a owl:Class; 
                     rdfs:comment """[v] = a * [SI]
where
[v] is the value in UK gallon per day
[SI] is the value in SI
a = Day / GallonUK, i.e., 19005343.053041186
and
Day = 24.0 * Hour
GallonUK = 4.54609e-3 reference: https://en.wikipedia.org/wiki/Gallon
Hour = 60.0 * Minute
Minute = 60.0
"""@EN; 
                     rdfs:subClassOf ddhub:Unit. 
ddhub:UkGallonPerHour a owl:Class; 
                      rdfs:comment """[v] = a * [SI]
where
[v] is the value in UK gallon per hour
[SI] is the value in SI
a = Hour/ GallonUK, i.e., 791889.293876716
and
Hour = 60.0 * Minute
GallonUK = 4.54609e-3 reference: https://en.wikipedia.org/wiki/Gallon
Minute = 60.0
"""@EN; 
                      rdfs:subClassOf ddhub:Unit. 
ddhub:UkGallonPerMinute a owl:Class; 
                        rdfs:comment """[v] = a * [SI]
where
[v] is the value in UK gallon per minute
[SI] is the value in SI
a = Minute / GallonUK, i.e., 13198.154897945267
and
Minute = 60.0
GallonUK = 4.54609e-3 reference: https://en.wikipedia.org/wiki/Gallon
"""@EN; 
                        rdfs:subClassOf ddhub:Unit. 
ddhub:UkGallonPerMinutePerSecond a owl:Class; 
                                 rdfs:comment """[v] = a * [SI]
where
[v] is the value in UK gallon per minute per second
[SI] is the value in SI
a = Minute*Unit/GallonUK, i.e., 13198.154897945267
and
Minute = 60.0
Unit = 1.0
GallonUK = 4.54609e-3 reference: https://en.wikipedia.org/wiki/Gallon
"""@EN; 
                                 rdfs:subClassOf ddhub:Unit. 
ddhub:UkGallonPerMinuteSquared a owl:Class; 
                               rdfs:comment """[v] = a * [SI]
where
[v] is the value in UK gallon per minute squared
[SI] is the value in SI
a = Minute*Minute/GallonUK, i.e., 791889.293876716
and
Minute = 60.0
GallonUK = 4.54609e-3 reference: https://en.wikipedia.org/wiki/Gallon
"""@EN; 
                               rdfs:subClassOf ddhub:Unit. 
ddhub:UkGallonPerSecond a owl:Class; 
                        rdfs:comment """[v] = a * [SI]
where
[v] is the value in UK gallon per second
[SI] is the value in SI
a = 1.0/GallonUK, i.e., 219.96924829908778
and
GallonUK = 4.54609e-3 reference: https://en.wikipedia.org/wiki/Gallon
"""@EN; 
                        rdfs:subClassOf ddhub:Unit. 
ddhub:UkGallonPerYear a owl:Class; 
                      rdfs:comment """[v] = a * [SI]
where
[v] is the value in UK gallon per year
[SI] is the value in SI
a = YearJulian /GallonUK, i.e., 6941701550.123293
and
YearJulian = 365.25 * Day
GallonUK = 4.54609e-3 reference: https://en.wikipedia.org/wiki/Gallon
Day = 24.0 * Hour
Hour = 60.0 * Minute
Minute = 60.0
"""@EN; 
                      rdfs:subClassOf ddhub:Unit. 
ddhub:UkNauticalMile a owl:Class; 
                     rdfs:comment """[v] = a * [SI]
where
[v] is the value in UK nautical mile
[SI] is the value in SI
a = 1.0/UKNauticalMile, i.e., 0.0005396118248376849
and
UKNauticalMile = 6080 * Foot reference: https://www.rmg.co.uk/stories/topics/nautical-mile
Foot = 12.0 * Inch
Inch = 0.0254 reference: https://www.nist.gov/pml/owm/si-units-length
"""@EN; 
                     rdfs:subClassOf ddhub:Unit. 
ddhub:UnderBalanceFeature a owl:Class; 
                          rdfs:comment """An under-balance feature indicates that something accounts for under-balance conditions.
"""@EN; 
                          rdfs:subClassOf ddhub:DownholePressureFeature. 
ddhub:Underpull a owl:Class; 
                rdfs:comment """This Noun is used to refer to a situation during which the drill-stem hangs in something in the downward direction.
"""@EN; 
                rdfs:subClassOf ddhub:DrillingIncident. 
ddhub:Underreamers a owl:Class; 
                   rdfs:comment ""@EN; 
                   rdfs:subClassOf ddhub:HoleOpener. 
ddhub:UnderReamingFeature a owl:Class; 
                          rdfs:comment """An under-reaming feature indicates that something accounts for under-reaming a borehole.
"""@EN; 
                          rdfs:subClassOf ddhub:HoleOpeningFeature. 
ddhub:Unit a owl:Class; 
           rdfs:comment """Physical quantities, such as length, mass, time, temperature, and
electric current, are described using both a numerical value and a `Unit`. The `Unit` defines what 
standard is being used to measure that quantity. A `Unit` is characterized by two attributes `ConversionFactorA`
and `ConversionFactorB` that are used to convert a SI value to the unit. Typical sub-types are made available. These types
can be used in a sort of singleton pattern, i.e., it is not necessary to create an individual to use them
in a relation. Also, if individuals are created with the same characteristics, they are considered as being 
multiple representations of the same `Noun`. Typical sub-types for the Noun `Unit`
are defined in UnitTypes. These units are automatically generated from the unit conversions of each individual 
`PhysicalQuantities` defined in the Open Source Drilling Community ([OSDC](https://opensourcedrilling.org/)) project called `UnitConversion` 
(see [`OSDC UnitConversion`](https://github.com/Open-Source-Drilling-Community/UnitConversion)).
It is possible to look at all the physical quantities defined in the `OSDC UnitConversion` project by
using the web application hosted here: [`OSDC Physical Quantity Web App`](https://dev.digiwells.no/UnitConversion/webapp/PhysicalQuantity). 
"""@EN; 
           rdfs:subClassOf ddhub:DWISNoun. 
ddhub:UnitPole a owl:Class; 
               rdfs:comment """[v] = a * [SI]
where
[v] is the value in unit pole
[SI] is the value in SI
a = 1e16/(4.0*PI), i.e., 795774715459476.8
"""@EN; 
               rdfs:subClassOf ddhub:Unit. 
ddhub:UnitSystem a owl:Class; 
                 rdfs:comment """A set of associations between measurable quantities and units.
"""@EN; 
                 rdfs:subClassOf ddhub:DWISNoun. 
ddhub:UpperSideAngleLocation a owl:Class; 
                             rdfs:comment ""@EN; 
                             rdfs:subClassOf ddhub:AngleReferenceLocation. 
ddhub:UserInterface a owl:Class; 
                    rdfs:comment ""@EN; 
                    rdfs:subClassOf ddhub:DataFlowNode. 
ddhub:UsGallon a owl:Class; 
               rdfs:comment """[v] = a * [SI]
where
[v] is the value in US gallon
[SI] is the value in SI
a = 1.0/GallonUS, i.e., 264.17205235814845
and
GallonUS = 231.0 * Inch * Inch * Inch reference: https://en.wikipedia.org/wiki/Gallon
Inch = 0.0254 reference: https://www.nist.gov/pml/owm/si-units-length
"""@EN; 
               rdfs:subClassOf ddhub:Unit. 
ddhub:UsGallonPerDay a owl:Class; 
                     rdfs:comment """[v] = a * [SI]
where
[v] is the value in US gallon per day
[SI] is the value in SI
a = Day / GallonUS, i.e., 22824465.323744025
and
Day = 24.0 * Hour
GallonUS = 231.0 * Inch * Inch * Inch reference: https://en.wikipedia.org/wiki/Gallon
Hour = 60.0 * Minute
Inch = 0.0254 reference: https://www.nist.gov/pml/owm/si-units-length
Minute = 60.0
"""@EN; 
                     rdfs:subClassOf ddhub:Unit. 
ddhub:UsGallonPerHour a owl:Class; 
                      rdfs:comment """[v] = a * [SI]
where
[v] is the value in US gallon per hour
[SI] is the value in SI
a = Hour/ GallonUS, i.e., 951019.3884893344
and
Hour = 60.0 * Minute
GallonUS = 231.0 * Inch * Inch * Inch reference: https://en.wikipedia.org/wiki/Gallon
Minute = 60.0
Inch = 0.0254 reference: https://www.nist.gov/pml/owm/si-units-length
"""@EN; 
                      rdfs:subClassOf ddhub:Unit. 
ddhub:UsGallonPerMinute a owl:Class; 
                        rdfs:comment """[v] = a * [SI]
where
[v] is the value in US gallon per minute
[SI] is the value in SI
a = Minute / GallonUS, i.e., 15850.323141488907
and
Minute = 60.0
GallonUS = 231.0 * Inch * Inch * Inch reference: https://en.wikipedia.org/wiki/Gallon
Inch = 0.0254 reference: https://www.nist.gov/pml/owm/si-units-length
"""@EN; 
                        rdfs:subClassOf ddhub:Unit. 
ddhub:UsGallonPerMinutePerSecond a owl:Class; 
                                 rdfs:comment """[v] = a * [SI]
where
[v] is the value in US gallon per minute per second
[SI] is the value in SI
a = Minute*Unit/GallonUS, i.e., 15850.323141488907
and
Minute = 60.0
Unit = 1.0
GallonUS = 231.0 * Inch * Inch * Inch reference: https://en.wikipedia.org/wiki/Gallon
Inch = 0.0254 reference: https://www.nist.gov/pml/owm/si-units-length
"""@EN; 
                                 rdfs:subClassOf ddhub:Unit. 
ddhub:UsGallonPerMinuteSquared a owl:Class; 
                               rdfs:comment """[v] = a * [SI]
where
[v] is the value in US gallon per minute squared
[SI] is the value in SI
a = Minute*Minute/GallonUS, i.e., 951019.3884893344
and
Minute = 60.0
GallonUS = 231.0 * Inch * Inch * Inch reference: https://en.wikipedia.org/wiki/Gallon
Inch = 0.0254 reference: https://www.nist.gov/pml/owm/si-units-length
"""@EN; 
                               rdfs:subClassOf ddhub:Unit. 
ddhub:UsGallonPerSecond a owl:Class; 
                        rdfs:comment """[v] = a * [SI]
where
[v] is the value in US gallon per second
[SI] is the value in SI
a = 1.0/GallonUS, i.e., 264.17205235814845
and
GallonUS = 231.0 * Inch * Inch * Inch reference: https://en.wikipedia.org/wiki/Gallon
Inch = 0.0254 reference: https://www.nist.gov/pml/owm/si-units-length
"""@EN; 
                        rdfs:subClassOf ddhub:Unit. 
ddhub:UsGallonPerYear a owl:Class; 
                      rdfs:comment """[v] = a * [SI]
where
[v] is the value in US gallon per year
[SI] is the value in SI
a = YearJulian /GallonUS, i.e., 8336635959.497505
and
YearJulian = 365.25 * Day
GallonUS = 231.0 * Inch * Inch * Inch reference: https://en.wikipedia.org/wiki/Gallon
Day = 24.0 * Hour
Inch = 0.0254 reference: https://www.nist.gov/pml/owm/si-units-length
Hour = 60.0 * Minute
Minute = 60.0
"""@EN; 
                      rdfs:subClassOf ddhub:Unit. 
ddhub:UsSurveyFoot a owl:Class; 
                   rdfs:comment """[v] = a * [SI]
where
[v] is the value in US survey foot
[SI] is the value in SI
a = 1.0/USSurveyFoot, i.e., 3.2808333333333337
and
USSurveyFoot = 1200.0 / 3937.0 reference: https://www.nist.gov/pml/us-surveyfoot
"""@EN; 
                   rdfs:subClassOf ddhub:Unit. 
ddhub:UTCReference a owl:Class; 
                   rdfs:comment ""@EN; 
                   rdfs:subClassOf ddhub:TimeReference. 
ddhub:VacuumDegasser a owl:Class; 
                     rdfs:comment ""@EN; 
                     rdfs:subClassOf ddhub:Degasser. 
ddhub:Validity a owl:DatatypeProperty, owl:FunctionalProperty; 
               rdfs:comment """
"""@EN; 
               rdfs:domain ddhub:Resampling; 
               rdfs:range xsd:double. 
ddhub:ValidityCondition a owl:Class; 
                        rdfs:comment ""@EN; 
                        rdfs:subClassOf ddhub:DWISNoun. 
ddhub:Value a owl:DatatypeProperty, owl:FunctionalProperty; 
            rdfs:comment """
"""@EN; 
            rdfs:domain ddhub:DrillingSignal, ddhub:HydraulicConnectedState, ddhub:MechanicalElementState; 
            rdfs:range xsd:object, xsd:bool. 
ddhub:ValuesIndices a owl:DatatypeProperty, owl:FunctionalProperty; 
                    rdfs:comment """
"""@EN; 
                    rdfs:domain ddhub:EndPointMapping; 
                    rdfs:range <http://www.w3.org/2001/XMLSchema#int[]>. 
ddhub:Variable a owl:Class; 
               rdfs:comment ""@EN; 
               rdfs:subClassOf ddhub:BladeShape. 
ddhub:VelocityQuantity a owl:Class; 
                       rdfs:comment """A velocity is the time derivative of a position or a displacement: $\\frac{dx}{dt}$, where $x$ is a position and $t$ is time.
The dimension of velocity is:
$$[LT^{-1}]$$.
The SI unit for **velocity** is: metre per second with the associated unit label $\\frac{m}{s}$
"""@EN; 
                       rdfs:subClassOf ddhub:Quantity. 
ddhub:VentOverboardLine a owl:Class; 
                        rdfs:comment ""@EN; 
                        rdfs:subClassOf ddhub:Diverter. 
ddhub:VerticalDepthFrame a owl:Class; 
                         rdfs:comment ""@EN; 
                         rdfs:subClassOf ddhub:OneDimensionalCartesianReferenceFrame. 
ddhub:VerticalOndulationModelling a owl:Class; 
                                  rdfs:comment """The model accounts for the change of inclination of some parts of the physical system.
"""@EN; 
                                  rdfs:subClassOf ddhub:TangentialModelling. 
ddhub:VerticalReferenceLocation a owl:Class; 
                                rdfs:comment ""@EN; 
                                rdfs:subClassOf ddhub:Location. 
ddhub:VibrationIsolators a owl:Class; 
                         rdfs:comment ""@EN; 
                         rdfs:subClassOf ddhub:ActiveVibrationTools. 
ddhub:Violle a owl:Class; 
             rdfs:comment """[v] = a * [SI]
where
[v] is the value in violle
[SI] is the value in SI
a = 1.0/Violle, i.e., 0.016666666666666666
and
Violle = 60.0 reference: https://en.wikipedia.org/wiki/Jules_Violle
"""@EN; 
             rdfs:subClassOf ddhub:Unit. 
ddhub:Volt a owl:Class; 
           rdfs:comment """No conversion necessary as the unit choice is SI
"""@EN; 
           rdfs:subClassOf ddhub:Unit. 
ddhub:VoltPerOhm a owl:Class; 
                 rdfs:comment """[v] = a * [SI]
where
[v] is the value in volt per ohm
[SI] is the value in SI
a = 1.0/Unit, i.e., 1
and
Unit = 1.0
"""@EN; 
                 rdfs:subClassOf ddhub:Unit. 
ddhub:VoltSecond a owl:Class; 
                 rdfs:comment """[v] = a * [SI]
where
[v] is the value in volt second
[SI] is the value in SI
a = 1.0/Unit, i.e., 1
and
Unit = 1.0
"""@EN; 
                 rdfs:subClassOf ddhub:Unit. 
ddhub:VolumeDrillingQuantity a owl:Class; 
                             rdfs:comment """A volume is the amount of three-dimensional space occupied by a body.
The dimension of volume is:
$$[L^{3}]$$.
The SI unit for **volume** is: cubic metre with the associated unit label $m^{3}$
The meaningful precision of volume in the drilling context is typically: 0.0001 m³
"""@EN; 
                             rdfs:subClassOf ddhub:MeasurableQuantity. 
ddhub:VolumeLargeQuantity a owl:Class; 
                          rdfs:comment """A volume is the amount of three-dimensional space occupied by a body.
The dimension of volume is:
$$[L^{3}]$$.
The SI unit for **volume** is: cubic metre with the associated unit label $m^{3}$
The meaningful precision of a large volume is typically: 0.1 m³
"""@EN; 
                          rdfs:subClassOf ddhub:MeasurableQuantity. 
ddhub:VolumeQuantity a owl:Class; 
                     rdfs:comment """A volume is the amount of three-dimensional space occupied by a body.
The dimension of volume is:
$$[L^{3}]$$.
The SI unit for **volume** is: cubic metre with the associated unit label $m^{3}$
"""@EN; 
                     rdfs:subClassOf ddhub:Quantity. 
ddhub:VolumetricFlowrateDrillingQuantity a owl:Class; 
                                         rdfs:comment """A volumetric flowrate is the volume of fluid that passes per unit time: $\\frac{dV}{dt}$, where $V$ is a volume and $t$ is time.
The dimension of volumetric flowrate is:
$$[L^{3}T^{-1}]$$.
The SI unit for **volumetric flow rate** is: cubic metre per second with the associated unit label $\\frac{m^{3}}{s}$
The meaningful precision of volumetric flowrate in the drilling context is typically: 0.0001 ft³/s
"""@EN; 
                                         rdfs:subClassOf ddhub:MeasurableQuantity. 
ddhub:VolumetricFlowRateOfChangeDrillingQuantity a owl:Class; 
                                                 rdfs:comment """A volumetric flow rate of change is the time derivative of a volumetric flowrate: $\\frac{dQ}{dt}$, where $Q$ is a volumetric flowrate and $t$ is time.
The dimension of volumetric flow rate of change is:
$$[L^{3}T^{-2}]$$.
The SI unit for **volumetric flow Rate rate of change** is: cubic metre per second squared with the associated unit label $\\frac{m^{3}}{s^{2}}$
The meaningful precision of volumetric flow rate of change in the drilling context is typically: 1E-06 m³/s²
"""@EN; 
                                                 rdfs:subClassOf ddhub:MeasurableQuantity. 
ddhub:VolumetricFlowRateOfChangeQuantity a owl:Class; 
                                         rdfs:comment """A volumetric flow rate of change is the time derivative of a volumetric flowrate: $\\frac{dQ}{dt}$, where $Q$ is a volumetric flowrate and $t$ is time.
The dimension of volumetric flow rate of change is:
$$[L^{3}T^{-2}]$$.
The SI unit for **volumetric flow Rate rate of change** is: cubic metre per second squared with the associated unit label $\\frac{m^{3}}{s^{2}}$
"""@EN; 
                                         rdfs:subClassOf ddhub:Quantity. 
ddhub:VolumetricFlowRateQuantity a owl:Class; 
                                 rdfs:comment """A volumetric flowrate is the volume of fluid that passes per unit time: $\\frac{dV}{dt}$, where $V$ is a volume and $t$ is time.
The dimension of volumetric flowrate is:
$$[L^{3}T^{-1}]$$.
The SI unit for **volumetric flow rate** is: cubic metre per second with the associated unit label $\\frac{m^{3}}{s}$
"""@EN; 
                                 rdfs:subClassOf ddhub:Quantity. 
ddhub:WaterBasedMudWbm a owl:Class; 
                       rdfs:comment ""@EN; 
                       rdfs:subClassOf ddhub:DrillingFluid. 
ddhub:Watt a owl:Class; 
           rdfs:comment """No conversion necessary as the unit choice is SI
"""@EN; 
           rdfs:subClassOf ddhub:Unit. 
ddhub:WattPerMetreKelvin a owl:Class; 
                         rdfs:comment """No conversion necessary as the unit choice is SI
"""@EN; 
                         rdfs:subClassOf ddhub:Unit. 
ddhub:WattPerMetreKelvinPerKelvin a owl:Class; 
                                  rdfs:comment """No conversion necessary as the unit choice is SI
"""@EN; 
                                  rdfs:subClassOf ddhub:Unit. 
ddhub:WattPerSquareMetrePerKelvin a owl:Class; 
                                  rdfs:comment """No conversion necessary as the unit choice is SI
"""@EN; 
                                  rdfs:subClassOf ddhub:Unit. 
ddhub:WattPerVolt a owl:Class; 
                  rdfs:comment """[v] = a * [SI]
where
[v] is the value in watt per volt
[SI] is the value in SI
a = 1.0/Unit, i.e., 1
and
Unit = 1.0
"""@EN; 
                  rdfs:subClassOf ddhub:Unit. 
ddhub:WaveNumberQuantity a owl:Class; 
                         rdfs:comment """A wave number is the number of wave lengths per unit distance.
The dimension of wave number is:
$$[L^{-1}]$$.
The SI unit for **wave number** is: reciprocal metre with the associated unit label $\\frac{1}{m}$
"""@EN; 
                         rdfs:subClassOf ddhub:Quantity. 
ddhub:Weber a owl:Class; 
            rdfs:comment """No conversion necessary as the unit choice is SI
"""@EN; 
            rdfs:subClassOf ddhub:Unit. 
ddhub:WeberPerHenry a owl:Class; 
                    rdfs:comment """[v] = a * [SI]
where
[v] is the value in weber per henry
[SI] is the value in SI
a = 1.0/Unit, i.e., 1
and
Unit = 1.0
"""@EN; 
                    rdfs:subClassOf ddhub:Unit. 
ddhub:WeberPerSquareMetre a owl:Class; 
                          rdfs:comment """[v] = a * [SI]
where
[v] is the value in weber per square metre
[SI] is the value in SI
a = 1.0/Unit, i.e., 1
and
Unit = 1.0
"""@EN; 
                          rdfs:subClassOf ddhub:Unit. 
ddhub:Week a owl:Class; 
           rdfs:comment """[v] = a * [SI]
where
[v] is the value in week
[SI] is the value in SI
a = 1.0/Week, i.e., 1.6534391534391535E-06
and
Week = 7.0 * Day
Day = 24.0 * Hour
Hour = 60.0 * Minute
Minute = 60.0
"""@EN; 
           rdfs:subClassOf ddhub:Unit. 
ddhub:WeightOnBitDrillingQuantity a owl:Class; 
                                  rdfs:comment """Mass can be experimentally defined as a measure of the body's inertia, meaning the resistance to acceleration (change of velocity) when a net force is applied. The object's mass also determines the strength of its gravitational attraction to other bodies.
The dimension of mass is:
$$[M]$$.
The SI unit for **mass** is: kilogram with the associated unit label $kg$
The meaningful precision of weight on bit in the drilling context is typically: 10 kg
"""@EN; 
                                  rdfs:subClassOf ddhub:MeasurableQuantity. 
ddhub:WeightTransferObjective a owl:Class; 
                              rdfs:comment """This Noun is used to refer to the objective of transferring weight to the bottom of the drill-stem.
"""@EN; 
                              rdfs:subClassOf ddhub:DrillingObjective. 
ddhub:WellboreArchitectureDescription a owl:Class; 
                                      rdfs:comment """The wellbore architecture provides information about the casings and liners in place as well as the current
open hole configuration. Also the surface architecture, i.e., everything above the wellhead, is also described, e.g., BOP, high 
pressure riser, low pressure riser, expansion joint,...
"""@EN; 
                                      rdfs:subClassOf ddhub:WellBoreData. 
ddhub:WellboreCenterLineFrame a owl:Class; 
                              rdfs:comment ""@EN; 
                              rdfs:subClassOf ddhub:OneDimensionalCurviLinearReferenceFrame. 
ddhub:WellBoreData a owl:Class; 
                   rdfs:comment ""@EN; 
                   rdfs:subClassOf ddhub:ContextualData. 
ddhub:WellBoreDataCharateristic a owl:Class; 
                                rdfs:comment """This Noun is used to characterize a piece of wellbore data.
"""@EN; 
                                rdfs:subClassOf ddhub:DWISNoun. 
ddhub:WellboreName a owl:DatatypeProperty, owl:FunctionalProperty; 
                   rdfs:comment """
"""@EN; 
                   rdfs:domain ddhub:WitsMLTimeBasedLogEndPoint; 
                   rdfs:range xsd:string. 
ddhub:WellboreUID a owl:DatatypeProperty, owl:FunctionalProperty; 
                  rdfs:comment """
"""@EN; 
                  rdfs:domain ddhub:WitsMLTimeBasedLogEndPoint; 
                  rdfs:range xsd:string. 
ddhub:WellcontrolStackEquipment a owl:Class; 
                                rdfs:comment ""@EN; 
                                rdfs:subClassOf ddhub:CoiledTubingEquipment. 
ddhub:WellControlSystem a owl:Class; 
                        rdfs:comment ""@EN; 
                        rdfs:subClassOf ddhub:RigEquipment. 
ddhub:WellHeadPositionLocation a owl:Class; 
                               rdfs:comment ""@EN; 
                               rdfs:subClassOf ddhub:PositionReferenceLocation. 
ddhub:WellHeadVerticalLocation a owl:Class; 
                               rdfs:comment ""@EN; 
                               rdfs:subClassOf ddhub:VerticalReferenceLocation. 
ddhub:WellheadXmasTree a owl:Class; 
                       rdfs:comment ""@EN; 
                       rdfs:subClassOf ddhub:WellControlSystem. 
ddhub:WellName a owl:DatatypeProperty, owl:FunctionalProperty; 
               rdfs:comment """
"""@EN; 
               rdfs:domain ddhub:WitsMLTimeBasedLogEndPoint; 
               rdfs:range xsd:string. 
ddhub:WellTestingEquipment a owl:Class; 
                           rdfs:comment ""@EN; 
                           rdfs:subClassOf ddhub:RigEquipment. 
ddhub:WellUID a owl:DatatypeProperty, owl:FunctionalProperty; 
              rdfs:comment """
"""@EN; 
              rdfs:domain ddhub:WitsMLTimeBasedLogEndPoint; 
              rdfs:range xsd:string. 
ddhub:WGS84PositionLocation a owl:Class; 
                            rdfs:comment ""@EN; 
                            rdfs:subClassOf ddhub:PositionReferenceLocation. 
ddhub:WGS84VerticalLocation a owl:Class; 
                            rdfs:comment ""@EN; 
                            rdfs:subClassOf ddhub:VerticalReferenceLocation. 
ddhub:Whipstock a owl:Class; 
                rdfs:comment ""@EN; 
                rdfs:subClassOf ddhub:DrillingEquipment. 
ddhub:Whirling a owl:Class; 
               rdfs:comment """This Noun is used to refer to abnormal lateral oscillations.
"""@EN; 
               rdfs:subClassOf ddhub:AbnormalLateralOscillation. 
ddhub:WhiteBoxModel a owl:Class; 
                    rdfs:comment """The model is fully transparent and interpretable, with all internal mechanisms and assumptions clearly defined.
"""@EN; 
                    rdfs:subClassOf ddhub:ModelTransparency. 
ddhub:WireCable a owl:Class; 
                rdfs:comment ""@EN; 
                rdfs:subClassOf ddhub:EquipmentTelemetry. 
ddhub:WiredPipe a owl:Class; 
                rdfs:comment ""@EN; 
                rdfs:subClassOf ddhub:EquipmentTelemetry. 
ddhub:WiredPipeTelemetry a owl:Class; 
                         rdfs:comment """A method that allows transfer of downhole data to the surface via electrical connections along the drill string.
"""@EN; 
                         rdfs:subClassOf ddhub:DownHoleTelemetry. 
ddhub:WirelineLoggingTools a owl:Class; 
                           rdfs:comment ""@EN; 
                           rdfs:subClassOf ddhub:LoggingEquipment. 
ddhub:WirelineLoggingToolsAcoustictools a owl:Class; 
                                        rdfs:comment ""@EN; 
                                        rdfs:subClassOf ddhub:WirelineLoggingTools. 
ddhub:WirelineLoggingToolsElectricalpropagation a owl:Class; 
                                                rdfs:comment ""@EN; 
                                                rdfs:subClassOf ddhub:WirelineLoggingTools. 
ddhub:WirelineLoggingToolsElectricalresistivity a owl:Class; 
                                                rdfs:comment ""@EN; 
                                                rdfs:subClassOf ddhub:WirelineLoggingTools. 
ddhub:WirelineLoggingToolsNmrtools a owl:Class; 
                                   rdfs:comment ""@EN; 
                                   rdfs:subClassOf ddhub:WirelineLoggingTools. 
ddhub:WirelineLoggingToolsNucleartools a owl:Class; 
                                       rdfs:comment ""@EN; 
                                       rdfs:subClassOf ddhub:WirelineLoggingTools. 
ddhub:WirelineLoggingToolsSeismictools a owl:Class; 
                                       rdfs:comment ""@EN; 
                                       rdfs:subClassOf ddhub:WirelineLoggingTools. 
ddhub:WitsMLTimeBasedLogEndPoint a owl:Class; 
                                 rdfs:comment ""@EN; 
                                 rdfs:subClassOf ddhub:DataEndPoint. 
ddhub:WOB a owl:Class; 
          rdfs:comment ""@EN; 
          rdfs:subClassOf ddhub:PrototypeData. 
ddhub:WOBLimit a owl:Class; 
               rdfs:comment """This Noun is used to refer to a weight on bit limit.
"""@EN; 
               rdfs:subClassOf ddhub:DrillingLimit. 
ddhub:Yard a owl:Class; 
           rdfs:comment """[v] = a * [SI]
where
[v] is the value in yard
[SI] is the value in SI
a = 1.0/Yard, i.e., 1.093613298337708
and
Yard = 3.0 * Foot
Foot = 12.0 * Inch
Inch = 0.0254 reference: https://www.nist.gov/pml/owm/si-units-length
"""@EN; 
           rdfs:subClassOf ddhub:Unit. 
ddhub:YardPerFoot a owl:Class; 
                  rdfs:comment """[v] = a * [SI]
where
[v] is the value in yard per foot
[SI] is the value in SI
a = Foot / Yard, i.e., 0.3333333333333333
and
Foot = 12.0 * Inch
Yard = 3.0 * Foot
Inch = 0.0254 reference: https://www.nist.gov/pml/owm/si-units-length
"""@EN; 
                  rdfs:subClassOf ddhub:Unit. 
ddhub:YardPerMile a owl:Class; 
                  rdfs:comment """[v] = a * [SI]
where
[v] is the value in yard per mile
[SI] is the value in SI
a = Mile / Yard, i.e., 1760
and
Mile = 1760.0 * Yard reference: https://dictionary.cambridge.org/dictionary/english/mile
Yard = 3.0 * Foot
Foot = 12.0 * Inch
Inch = 0.0254 reference: https://www.nist.gov/pml/owm/si-units-length
"""@EN; 
                  rdfs:subClassOf ddhub:Unit. 
ddhub:YardPerYard a owl:Class; 
                  rdfs:comment """[v] = a * [SI]
where
[v] is the value in yard per yard
[SI] is the value in SI
a = Yard / Yard, i.e., 1
and
Yard = 3.0 * Foot
Foot = 12.0 * Inch
Inch = 0.0254 reference: https://www.nist.gov/pml/owm/si-units-length
"""@EN; 
                  rdfs:subClassOf ddhub:Unit. 
ddhub:YearAverageGregorian a owl:Class; 
                           rdfs:comment """[v] = a * [SI]
where
[v] is the value in year average gregorian
[SI] is the value in SI
a = 1.0/YearAverageGregorian, i.e., 3.1709791983764586E-08
and
YearAverageGregorian = (365.0 + 97 / 400) * Day reference: https://en.wikipedia.org/wiki/Gregorian_calendar
Day = 24.0 * Hour
Hour = 60.0 * Minute
Minute = 60.0
"""@EN; 
                           rdfs:subClassOf ddhub:Unit. 
ddhub:YearCommon a owl:Class; 
                 rdfs:comment """[v] = a * [SI]
where
[v] is the value in year common
[SI] is the value in SI
a = 1.0/YearCommon, i.e., 3.1709791983764586E-08
and
YearCommon = 365 * Day
Day = 24.0 * Hour
Hour = 60.0 * Minute
Minute = 60.0
"""@EN; 
                 rdfs:subClassOf ddhub:Unit. 
ddhub:YearJulian a owl:Class; 
                 rdfs:comment """[v] = a * [SI]
where
[v] is the value in year julian
[SI] is the value in SI
a = 1.0/YearJulian, i.e., 3.168808781402895E-08
and
YearJulian = 365.25 * Day
Day = 24.0 * Hour
Hour = 60.0 * Minute
Minute = 60.0
"""@EN; 
                 rdfs:subClassOf ddhub:Unit. 
ddhub:YearLeap a owl:Class; 
               rdfs:comment """[v] = a * [SI]
where
[v] is the value in year leap
[SI] is the value in SI
a = 1.0/YearLeap, i.e., 3.1623153207852664E-08
and
YearLeap = 366 * Day
Day = 24.0 * Hour
Hour = 60.0 * Minute
Minute = 60.0
"""@EN; 
               rdfs:subClassOf ddhub:Unit. 
ddhub:YearTropical a owl:Class; 
                   rdfs:comment """[v] = a * [SI]
where
[v] is the value in year tropical
[SI] is the value in SI
a = 1.0/YearTropical, i.e., 3.1688764535078565E-08
and
YearTropical = 365.2422 * Day reference: https://www.grc.nasa.gov/www/k-12/Numbers/Math/Mathematical_Thinking/calendar_calculations.htm
Day = 24.0 * Hour
Hour = 60.0 * Minute
Minute = 60.0
"""@EN; 
                   rdfs:subClassOf ddhub:Unit. 
