@prefix ddhub: <http://ddhub.no/>.
@prefix owl: <http://www.w3.org/2002/07/owl#>.
@prefix rdf: <http://www.w3.org/1999/02/22-rdf-syntax-ns#>.
@prefix rdfs: <http://www.w3.org/2000/01/rdf-schema#>.
@prefix xsd: <http://www.w3.org/2001/XMLSchema#>.
@base <https://rdfsharp.codeplex.com/>.

ddhub:AbnormalAxialOscillation a owl:Class; 
                               rdfs:comment ""@EN; 
                               rdfs:subClassOf ddhub:AbnormalOscillation. 
ddhub:AbnormalLateralOscillation a owl:Class; 
                                 rdfs:comment ""@EN; 
                                 rdfs:subClassOf ddhub:AbnormalOscillation. 
ddhub:AbnormalOscillation a owl:Class; 
                          rdfs:comment ""@EN; 
                          rdfs:subClassOf ddhub:DrillingIncident. 
ddhub:AbnormalTorsionalOscillation a owl:Class; 
                                   rdfs:comment ""@EN; 
                                   rdfs:subClassOf ddhub:AbnormalOscillation. 
ddhub:AbscissaReferenceLocation a owl:Class; 
                                rdfs:comment ""@EN; 
                                rdfs:subClassOf ddhub:Location. 
ddhub:AbsolutePressureReference a owl:Class; 
                                rdfs:comment ""@EN; 
                                rdfs:subClassOf ddhub:PressureReference. 
ddhub:AbsoluteTimeReference a owl:Class; 
                            rdfs:comment ""@EN; 
                            rdfs:subClassOf ddhub:TimeReference. 
ddhub:AccelerationDrillingQuantity a owl:Class; 
                                   rdfs:comment """**Acceleration** is defined as the rate of change of velocity with respect to time. Velocity itself is the rate of change of displacement (or position) with respect to time. Therefore, acceleration is the rate of change of displacement twice with respect to time.
Let's break this down:
1. **Displacement** (or position) has the dimension of **Length(L)**.
2. **Velocity** is displacement per unit time:
$$\\text{Velocity} = \\frac{\\text{Length}}{\\text{Time}} = \\frac{L}{T}$$
So, the dimension of velocity is **$[L T^{ -1}]$**.
3. **Acceleration** is the rate of change of velocity with respect to time:
$$\\text{Acceleration} = \\frac{\\text{Velocity}}{\\text{Time}} = \\frac{L T^{ -1}}{T} = L T ^{-2}$$
Therefore, the dimension of acceleration is $[LT^{-2}]$.
The SI unit for **acceleration** is: metre per second squared with the associated unit label $\\frac{m}{s^{2}}$
The meaningful precision of acceleration in the drilling context is typically: 0.001 m/s²
"""@EN; 
                                   rdfs:subClassOf ddhub:MeasurableQuantity. 
ddhub:AccelerationQuantity a owl:Class; 
                           rdfs:comment """**Acceleration** is defined as the rate of change of velocity with respect to time. Velocity itself is the rate of change of displacement (or position) with respect to time. Therefore, acceleration is the rate of change of displacement twice with respect to time.
Let's break this down:
1. **Displacement** (or position) has the dimension of **Length(L)**.
2. **Velocity** is displacement per unit time:
$$\\text{Velocity} = \\frac{\\text{Length}}{\\text{Time}} = \\frac{L}{T}$$
So, the dimension of velocity is **$[L T^{ -1}]$**.
3. **Acceleration** is the rate of change of velocity with respect to time:
$$\\text{Acceleration} = \\frac{\\text{Velocity}}{\\text{Time}} = \\frac{L T^{ -1}}{T} = L T ^{-2}$$
Therefore, the dimension of acceleration is $[LT^{-2}]$.
The SI unit for **acceleration** is: metre per second squared with the associated unit label $\\frac{m}{s^{2}}$
"""@EN; 
                           rdfs:subClassOf ddhub:Quantity. 
ddhub:Accelerator a owl:Class; 
                  rdfs:comment ""@EN; 
                  rdfs:subClassOf ddhub:JarringAssembly. 
ddhub:Accumulator a owl:Class; 
                  rdfs:comment ""@EN; 
                  rdfs:subClassOf ddhub:WellControlSystem. 
ddhub:Accuracy a owl:DatatypeProperty, owl:FunctionalProperty; 
               rdfs:comment """The standard deviation of the systematic bias component of the uncertainty of the sensor. The assumed mean value of the attached Gaussian distribution is the measured value. The value is expected to be in the same physical quantity as the sensor value.
"""@EN; 
               rdfs:domain ddhub:SensorUncertainty; 
               rdfs:range xsd:double. 
ddhub:Acoustic a owl:Class; 
               rdfs:comment ""@EN; 
               rdfs:subClassOf ddhub:EquipmentTelemetry. 
ddhub:Action a owl:Class; 
             rdfs:comment ""@EN; 
             rdfs:subClassOf ddhub:PistonMudPump. 
ddhub:ActivableFunction a owl:Class; 
                        rdfs:comment """An `ActivableFunction` is an ADCS function that can be activated. Here activation means that the
function may run immediately or that it is enabled and can trigger if some conditions are respected.
"""@EN; 
                        rdfs:subClassOf ddhub:DWISNoun. 
ddhub:ActiveDrillingSystem a owl:Class; 
                           rdfs:comment ""@EN; 
                           rdfs:subClassOf ddhub:MudPits. 
ddhub:ActiveLine a owl:Class; 
                 rdfs:comment ""@EN; 
                 rdfs:subClassOf ddhub:DrillLine. 
ddhub:ActiveVibrationTools a owl:Class; 
                           rdfs:comment ""@EN; 
                           rdfs:subClassOf ddhub:DrillingEquipment. 
ddhub:ActiveVolume a owl:Class; 
                   rdfs:comment ""@EN; 
                   rdfs:subClassOf ddhub:PrototypeData. 
ddhub:AdapterSpool a owl:Class; 
                   rdfs:comment ""@EN; 
                   rdfs:subClassOf ddhub:WellControlSystem. 
ddhub:AdjustableKickoffSub a owl:Class; 
                           rdfs:comment ""@EN; 
                           rdfs:subClassOf ddhub:DrillingEquipment. 
ddhub:Advice a owl:Class; 
             rdfs:comment ""@EN; 
             rdfs:subClassOf ddhub:ProcessData. 
ddhub:AdviceType a owl:DatatypeProperty, owl:FunctionalProperty; 
                 rdfs:comment """
"""@EN; 
                 rdfs:domain ddhub:Advisor; 
                 rdfs:range xsd:string. 
ddhub:AdvisedMaximum a owl:Class; 
                     rdfs:comment ""@EN; 
                     rdfs:subClassOf ddhub:Advice. 
ddhub:AdvisedMinimum a owl:Class; 
                     rdfs:comment ""@EN; 
                     rdfs:subClassOf ddhub:Advice. 
ddhub:AdvisedTarget a owl:Class; 
                    rdfs:comment ""@EN; 
                    rdfs:subClassOf ddhub:Advice. 
ddhub:Advisor a owl:Class; 
              rdfs:comment ""@EN; 
              rdfs:subClassOf ddhub:ComputationUnit. 
ddhub:AfmAutofluidMeasSkid a owl:Class; 
                           rdfs:comment ""@EN; 
                           rdfs:subClassOf ddhub:CirculationSystem. 
ddhub:Aggregation a owl:Class; 
                  rdfs:comment ""@EN; 
                  rdfs:subClassOf ddhub:DirectTransformation. 
ddhub:AllowEnablementSignalFor a owl:ObjectProperty; 
                               rdfs:comment """This verb is used to define a `DrillingDataPoint` tells if it is allowed or not to enable or
disable an activable function. It is expected that the `DrillingDataPoint` is a Boolean value. If the signal is true,
then it is possible to enable or disable the function using the signal associated with `IsEnablingSignalFor`. If it is
false, it is not allowed to enable or disable the `ActivableFunction`, meaning that the signal associated with `IsEnablingSignalFor`
is ignored.
"""@EN; 
                               rdfs:domain ddhub:DrillingDataPoint; 
                               rdfs:range ddhub:ActivableFunction; 
                               rdfs:subPropertyOf ddhub:DWISVerb. 
ddhub:AmountSubstanceQuantity a owl:Class; 
                              rdfs:comment """The **amount of substance** refers to the quantity of entities (such as atoms, molecules, ions, or other particles) in a system.The standard unit used to measure the amount of substance is the **mole** (mol). One mole corresponds to $6.022×10^{23}$ entities (Avogadro's number) of the given substance.
This is one of the nine fundamental dimensions in the International System of Units (SI).A fundamental quantity does not depend on any combinations of other fundamental dimensions.It is denoted $[N]$.
The SI unit for **amount substance** is: mole with the associated unit label $mol$
"""@EN; 
                              rdfs:subClassOf ddhub:Quantity. 
ddhub:Anchors a owl:Class; 
              rdfs:comment ""@EN; 
              rdfs:subClassOf ddhub:MooringSystem. 
ddhub:AngleGradientPerLengthDrillingQuantity a owl:Class; 
                                             rdfs:comment """Consider a situation where you have a length $L$ along which an angle $\\theta$ changes. The angle variation gradient is defined as the **rate of change of the angle** per unit change in length. Mathematically, it can be expressed as: 
$$\\text{ Angle Variation Gradient} = \\frac{ d\\theta}{ dL}$$
where: 
"""@EN; 
                                             rdfs:subClassOf ddhub:MeasurableQuantity. 
ddhub:AngleGradientPerLengthQuantity a owl:Class; 
                                     rdfs:comment """Consider a situation where you have a length $L$ along which an angle $\\theta$ changes. The angle variation gradient is defined as the **rate of change of the angle** per unit change in length. Mathematically, it can be expressed as: 
$$\\text{ Angle Variation Gradient} = \\frac{ d\\theta}{ dL}$$
where: 
"""@EN; 
                                     rdfs:subClassOf ddhub:Quantity. 
ddhub:AngleMagneticFluxDensityQuantity a owl:Class; 
                                       rdfs:comment """The **angle magnetic flux density** is the product of an angle by a magnetic flux density. Let's break it down step by step:
1. Magnetic Flux Density
The **magnetic flux density** $\\mathbf{B}$ is a measure of the strength and direction of the magnetic field at a particular point in space. It represents the amount of magnetic flux passing through a unit area perpendicular to the direction of the magnetic field. In simpler terms, it describes how dense or concentrated the magnetic field lines are in a given region.It can be expressed in terms of the fundamental dimensions as:
$$[M][T]^{-2}[I]^{-1}$$
Where:
"""@EN; 
                                       rdfs:subClassOf ddhub:Quantity. 
ddhub:AngleMagneticFluxDensitySurveyInstrumentDrillingQuantity a owl:Class; 
                                                               rdfs:comment """The **angle magnetic flux density** is the product of an angle by a magnetic flux density. Let's break it down step by step:
1. Magnetic Flux Density
The **magnetic flux density** $\\mathbf{B}$ is a measure of the strength and direction of the magnetic field at a particular point in space. It represents the amount of magnetic flux passing through a unit area perpendicular to the direction of the magnetic field. In simpler terms, it describes how dense or concentrated the magnetic field lines are in a given region.It can be expressed in terms of the fundamental dimensions as:
$$[M][T]^{-2}[I]^{-1}$$
Where:
"""@EN; 
                                                               rdfs:subClassOf ddhub:MeasurableQuantity. 
ddhub:AngleReferenceFrame a owl:Class; 
                          rdfs:comment ""@EN; 
                          rdfs:subClassOf ddhub:OneDimensionalReferenceFrame. 
ddhub:AngleReferenceLocation a owl:Class; 
                             rdfs:comment ""@EN; 
                             rdfs:subClassOf ddhub:Location. 
ddhub:AngularAccelerationDrillingQuantity a owl:Class; 
                                          rdfs:comment """An angular acceleration is the second derivative compared to time of a plan angle: $\\frac{d^2\\theta}{dt^2}$.
The dimension of angular acceleration is:
$$[{\\theta}T^{-2}]$$.
The SI unit for **angular acceleration** is: radian per second squared with the associated unit label $\\frac{rad}{s^{2}}$
The meaningful precision of angular acceleration in the drilling context is typically: 0.01 rad/s²
"""@EN; 
                                          rdfs:subClassOf ddhub:MeasurableQuantity. 
ddhub:AngularAccelerationQuantity a owl:Class; 
                                  rdfs:comment """An angular acceleration is the second derivative compared to time of a plan angle: $\\frac{d^2\\theta}{dt^2}$.
The dimension of angular acceleration is:
$$[{\\theta}T^{-2}]$$.
The SI unit for **angular acceleration** is: radian per second squared with the associated unit label $\\frac{rad}{s^{2}}$
"""@EN; 
                                  rdfs:subClassOf ddhub:Quantity. 
ddhub:AngularLateralModelling a owl:Class; 
                              rdfs:comment """The model accounts for the angular lateral movement of some parts of the physical system.
"""@EN; 
                              rdfs:subClassOf ddhub:LateralModelling. 
ddhub:AngularVelocityDrillingQuantity a owl:Class; 
                                      rdfs:comment """An angular velocity is the first derivative compared to time of a plan angle: $\\frac{d\\theta}{dt}$.
The dimension of angular velocity is:
$$[{\\theta}T^{-1}]$$.
The SI unit for **angular velocity** is: radian per second with the associated unit label $\\frac{rad}{s}$
The meaningful precision of angular velocity in the drilling context is typically: 0.01 rad/s
"""@EN; 
                                      rdfs:subClassOf ddhub:MeasurableQuantity. 
ddhub:AngularVelocityQuantity a owl:Class; 
                              rdfs:comment """An angular velocity is the first derivative compared to time of a plan angle: $\\frac{d\\theta}{dt}$.
The dimension of angular velocity is:
$$[{\\theta}T^{-1}]$$.
The SI unit for **angular velocity** is: radian per second with the associated unit label $\\frac{rad}{s}$
"""@EN; 
                              rdfs:subClassOf ddhub:Quantity. 
ddhub:AngularVelocitySurveyInstrumentDrillingQuantity a owl:Class; 
                                                      rdfs:comment """An angular velocity is the first derivative compared to time of a plan angle: $\\frac{d\\theta}{dt}$.
The dimension of angular velocity is:
$$[{\\theta}T^{-1}]$$.
The SI unit for **angular velocity** is: radian per second with the associated unit label $\\frac{rad}{s}$
The meaningful precision of angular velocity related to survey instrument performance models in the drilling context is typically: 1E-07 rad•T
"""@EN; 
                                                      rdfs:subClassOf ddhub:MeasurableQuantity. 
ddhub:Annular a owl:Class; 
              rdfs:comment ""@EN; 
              rdfs:subClassOf ddhub:HydraulicBranch. 
ddhub:AnnularPreventer a owl:Class; 
                       rdfs:comment ""@EN; 
                       rdfs:subClassOf ddhub:BopElement. 
ddhub:AreaDrillingQuantity a owl:Class; 
                           rdfs:comment """Area is the measure of the extent of a surface or the size of a two-dimensional shape.
The dimension of area is:
$$[L^{2}]$$.
The SI unit for **area** is: square metre with the associated unit label $m^{2}$
The meaningful precision of area in the drilling context is typically: 1E-06 m²
"""@EN; 
                           rdfs:subClassOf ddhub:MeasurableQuantity. 
ddhub:AreaQuantity a owl:Class; 
                   rdfs:comment """Area is the measure of the extent of a surface or the size of a two-dimensional shape.
The dimension of area is:
$$[L^{2}]$$.
The SI unit for **area** is: square metre with the associated unit label $m^{2}$
"""@EN; 
                   rdfs:subClassOf ddhub:Quantity. 
ddhub:AssociatesMeasurableQuantity a owl:ObjectProperty; 
                                   rdfs:comment ""@EN; 
                                   rdfs:domain ddhub:MeasurableQuantityUnitAssociation; 
                                   rdfs:range ddhub:MeasurableQuantity; 
                                   rdfs:subPropertyOf ddhub:DWISVerb. 
ddhub:AssociatesUnit a owl:ObjectProperty; 
                     rdfs:comment ""@EN; 
                     rdfs:domain ddhub:MeasurableQuantityUnitAssociation; 
                     rdfs:range ddhub:Unit; 
                     rdfs:subPropertyOf ddhub:DWISVerb. 
ddhub:AverageDelayByRepeater a owl:DatatypeProperty, owl:FunctionalProperty; 
                             rdfs:comment """
"""@EN; 
                             rdfs:domain ddhub:Telemetry; 
                             rdfs:range xsd:double. 
ddhub:AxialModelling a owl:Class; 
                     rdfs:comment """The model accounts for the axial movement of some parts of the physical system.
"""@EN; 
                     rdfs:subClassOf ddhub:ModelledDegreeOfFreedom. 
ddhub:AxialMotionType a owl:Class; 
                      rdfs:comment ""@EN; 
                      rdfs:subClassOf ddhub:MotionType. 
ddhub:AxialReferenceLocation a owl:Class; 
                             rdfs:comment ""@EN; 
                             rdfs:subClassOf ddhub:Location. 
ddhub:AxialVelocityDrillingQuantity a owl:Class; 
                                    rdfs:comment """A velocity is the time derivative of a position or a displacement: $\\frac{dx}{dt}$, where $x$ is a position and $t$ is time.
The dimension of velocity is:
$$[LT^{-1}]$$.
The SI unit for **velocity** is: metre per second with the associated unit label $\\frac{m}{s}$
The meaningful precision of velocity in the drilling context is typically: 0.01 m/s
"""@EN; 
                                    rdfs:subClassOf ddhub:MeasurableQuantity. 
ddhub:Azimuth a owl:Class; 
              rdfs:comment ""@EN; 
              rdfs:subClassOf ddhub:PrototypeData. 
ddhub:AzimuthalTools a owl:Class; 
                     rdfs:comment ""@EN; 
                     rdfs:subClassOf ddhub:LoggingWhileDrillingTools. 
ddhub:AzimuthReferenceLocation a owl:Class; 
                               rdfs:comment ""@EN; 
                               rdfs:subClassOf ddhub:Location. 
ddhub:BackPressurePump a owl:Class; 
                       rdfs:comment ""@EN; 
                       rdfs:subClassOf ddhub:CirculationSystem. 
ddhub:BackPressurePumpPressure a owl:Class; 
                               rdfs:comment ""@EN; 
                               rdfs:subClassOf ddhub:PrototypeData. 
ddhub:BackwardWhirl a owl:Class; 
                    rdfs:comment ""@EN; 
                    rdfs:subClassOf ddhub:Whirling. 
ddhub:BallastSystem a owl:Class; 
                    rdfs:comment ""@EN; 
                    rdfs:subClassOf ddhub:MarineSystem. 
ddhub:BallJoint a owl:Class; 
                rdfs:comment ""@EN; 
                rdfs:subClassOf ddhub:DrillingRiser. 
ddhub:BandPassFilter a owl:Class; 
                     rdfs:comment ""@EN; 
                     rdfs:subClassOf ddhub:Filter. 
ddhub:Beacons a owl:Class; 
              rdfs:comment ""@EN; 
              rdfs:subClassOf ddhub:MarineSystem. 
ddhub:BellNipple a owl:Class; 
                 rdfs:comment ""@EN; 
                 rdfs:subClassOf ddhub:WellControlSystem. 
ddhub:BelongsToClass a owl:ObjectProperty; 
                     rdfs:comment """The verb is used between a node and a Noun, i.e., a class. Semantically it can be considered as a synonym to `rdf:type`. It has been introduced to overcome limitations from OPC-UA that does not allow for multiple inheritance. Note that the same node can be in relation using `BelongsToClass` to several classes.
"""@EN; 
                     rdfs:domain ddhub:DWISNoun; 
                     rdfs:range ddhub:DWISNoun; 
                     rdfs:subPropertyOf ddhub:DWISVerb. 
ddhub:BelongsToSynchronizationGroup a owl:ObjectProperty; 
                                    rdfs:comment ""@EN; 
                                    rdfs:domain ddhub:Resampling; 
                                    rdfs:range ddhub:SynchronizationGroup; 
                                    rdfs:subPropertyOf ddhub:DWISVerb. 
ddhub:BHAAnnular a owl:Class; 
                 rdfs:comment ""@EN; 
                 rdfs:subClassOf ddhub:Annular. 
ddhub:BHAInner a owl:Class; 
               rdfs:comment ""@EN; 
               rdfs:subClassOf ddhub:Pipe. 
ddhub:BhaVibrationDampers a owl:Class; 
                          rdfs:comment ""@EN; 
                          rdfs:subClassOf ddhub:ActiveVibrationTools. 
ddhub:BicenterReamerBit a owl:Class; 
                        rdfs:comment ""@EN; 
                        rdfs:subClassOf ddhub:Reamers. 
ddhub:BitDepth a owl:Class; 
               rdfs:comment """Curvilinear abscissa of the bottom of the bit, in the reference frame centered in the wellbore.
"""@EN; 
               rdfs:subClassOf ddhub:PrototypeData. 
ddhub:BladeDiameter a owl:Class; 
                    rdfs:comment ""@EN; 
                    rdfs:subClassOf ddhub:Stabilizers. 
ddhub:BladeLength a owl:Class; 
                  rdfs:comment ""@EN; 
                  rdfs:subClassOf ddhub:Stabilizers. 
ddhub:BladeShape a owl:Class; 
                 rdfs:comment ""@EN; 
                 rdfs:subClassOf ddhub:Stabilizers. 
ddhub:BladeType a owl:Class; 
                rdfs:comment ""@EN; 
                rdfs:subClassOf ddhub:Stabilizers. 
ddhub:BladeTypeWelded a owl:Class; 
                      rdfs:comment ""@EN; 
                      rdfs:subClassOf ddhub:BladeType. 
ddhub:BlindRam a owl:Class; 
               rdfs:comment ""@EN; 
               rdfs:subClassOf ddhub:BopElement. 
ddhub:BlockVelocityDrillingQuantity a owl:Class; 
                                    rdfs:comment """A velocity is the time derivative of a position or a displacement: $\\frac{dx}{dt}$, where $x$ is a position and $t$ is time.
The dimension of velocity is:
$$[LT^{-1}]$$.
The SI unit for **velocity** is: metre per second with the associated unit label $\\frac{m}{s}$
The meaningful precision of block velocity in the drilling context is typically: 0.01 m/s
"""@EN; 
                                    rdfs:subClassOf ddhub:MeasurableQuantity. 
ddhub:BooleanDataType a owl:Class; 
                      rdfs:comment ""@EN; 
                      rdfs:subClassOf ddhub:EnumerationDataType. 
ddhub:BoosterLine a owl:Class; 
                  rdfs:comment ""@EN; 
                  rdfs:subClassOf ddhub:MarineSystem. 
ddhub:BoosterPump a owl:Class; 
                  rdfs:comment ""@EN; 
                  rdfs:subClassOf ddhub:CirculationSystem. 
ddhub:BOPControlSystem a owl:Class; 
                       rdfs:comment ""@EN; 
                       rdfs:subClassOf ddhub:ControlSystem. 
ddhub:BopElement a owl:Class; 
                 rdfs:comment ""@EN; 
                 rdfs:subClassOf ddhub:WellControlSystem. 
ddhub:BOPOpening a owl:Class; 
                 rdfs:comment ""@EN; 
                 rdfs:subClassOf ddhub:PrototypeData. 
ddhub:BOPPressure a owl:Class; 
                  rdfs:comment ""@EN; 
                  rdfs:subClassOf ddhub:PrototypeData. 
ddhub:BopStack a owl:Class; 
               rdfs:comment ""@EN; 
               rdfs:subClassOf ddhub:WellControlSystem. 
ddhub:BottomholeAssembly a owl:Class; 
                         rdfs:comment ""@EN; 
                         rdfs:subClassOf ddhub:DrillString. 
ddhub:BottomOfStringReferenceLocation a owl:Class; 
                                      rdfs:comment ""@EN; 
                                      rdfs:subClassOf ddhub:AbscissaReferenceLocation. 
ddhub:BottomShoulderAxialLocation a owl:Class; 
                                  rdfs:comment ""@EN; 
                                  rdfs:subClassOf ddhub:AxialReferenceLocation. 
ddhub:BoundaryDiscretization a owl:Class; 
                             rdfs:comment """A model only considers the bounds of the physical system and does not apply any intermediate discretization.
"""@EN; 
                             rdfs:subClassOf ddhub:ModellingDiscretization. 
ddhub:Box a owl:Class; 
          rdfs:comment ""@EN; 
          rdfs:subClassOf ddhub:Connection. 
ddhub:Boxbox a owl:Class; 
             rdfs:comment ""@EN; 
             rdfs:subClassOf ddhub:TubularConfiguration. 
ddhub:Buffering a owl:Class; 
                rdfs:comment ""@EN; 
                rdfs:subClassOf ddhub:TimeBasedTransformation. 
ddhub:BufferingInterval a owl:DatatypeProperty, owl:FunctionalProperty; 
                        rdfs:comment """
"""@EN; 
                        rdfs:domain ddhub:Buffering; 
                        rdfs:range xsd:double. 
ddhub:BulkTank a owl:Class; 
               rdfs:comment ""@EN; 
               rdfs:subClassOf ddhub:MudPits. 
ddhub:BullNose a owl:Class; 
               rdfs:comment ""@EN; 
               rdfs:subClassOf ddhub:DrillstemTerminator. 
ddhub:CableDiameterDrillingQuantity a owl:Class; 
                                    rdfs:comment """Length is a measure of distance.
The dimension of length is:
$$[L]$$.
The SI unit for **length** is: metre with the associated unit label $m$
The meaningful precision of small length is typically: 0.0005 m
The meaningful precision of a cable diameter in the drilling context is typically: 0.0005 m
"""@EN; 
                                    rdfs:subClassOf ddhub:MeasurableQuantity. 
ddhub:CapillaryPressureDrillingQuantity a owl:Class; 
                                        rdfs:comment """Pressure is the force applied per unit area on a surface.
The dimension of pressure is:
$$[ML^{-1}T^{-2}]$$.
The SI unit for **pressure** is: pascal with the associated unit label $Pa$
The meaningful precision of capilary pressure in the drilling context is typically: 0.1 Pa
"""@EN; 
                                        rdfs:subClassOf ddhub:MeasurableQuantity. 
ddhub:CartesianFourDimensionalReferenceFrame a owl:Class; 
                                             rdfs:comment ""@EN; 
                                             rdfs:subClassOf ddhub:FourDimensionalReferenceFrame. 
ddhub:CartesianThreeDimensionalReferenceFrame a owl:Class; 
                                              rdfs:comment ""@EN; 
                                              rdfs:subClassOf ddhub:ThreeDimensionalReferenceFrame. 
ddhub:CartesianTwoDimensionalReferenceFrame a owl:Class; 
                                            rdfs:comment ""@EN; 
                                            rdfs:subClassOf ddhub:TwoDimensionalReferenceFrame. 
ddhub:CasedHoleTools a owl:Class; 
                     rdfs:comment ""@EN; 
                     rdfs:subClassOf ddhub:WirelineLoggingTools. 
ddhub:Casing a owl:Class; 
             rdfs:comment ""@EN; 
             rdfs:subClassOf ddhub:CasingString. 
ddhub:CasingCollarLocator a owl:Class; 
                          rdfs:comment ""@EN; 
                          rdfs:subClassOf ddhub:WirelineLoggingTools. 
ddhub:CasingCutter a owl:Class; 
                   rdfs:comment ""@EN; 
                   rdfs:subClassOf ddhub:CasingEquipment. 
ddhub:CasingEquipment a owl:Class; 
                      rdfs:comment ""@EN; 
                      rdfs:subClassOf ddhub:DownholeEquipment. 
ddhub:CasingFlangeVerticalLocation a owl:Class; 
                                   rdfs:comment ""@EN; 
                                   rdfs:subClassOf ddhub:VerticalReferenceLocation. 
ddhub:CasingHanger a owl:Class; 
                   rdfs:comment ""@EN; 
                   rdfs:subClassOf ddhub:Hangers. 
ddhub:CasingHead a owl:Class; 
                 rdfs:comment ""@EN; 
                 rdfs:subClassOf ddhub:CasingEquipment. 
ddhub:CasingLinerEquipment a owl:Class; 
                           rdfs:comment ""@EN; 
                           rdfs:subClassOf ddhub:CasingEquipment. 
ddhub:CasingMillingTools a owl:Class; 
                         rdfs:comment ""@EN; 
                         rdfs:subClassOf ddhub:CasingEquipment. 
ddhub:CasingShoe a owl:Class; 
                 rdfs:comment ""@EN; 
                 rdfs:subClassOf ddhub:CasingEquipment. 
ddhub:CasingString a owl:Class; 
                   rdfs:comment ""@EN; 
                   rdfs:subClassOf ddhub:Tubulars. 
ddhub:CasingTongs a owl:Class; 
                  rdfs:comment ""@EN; 
                  rdfs:subClassOf ddhub:DrillPipeTongs. 
ddhub:Casingwhiledrilling a owl:Class; 
                          rdfs:comment ""@EN; 
                          rdfs:subClassOf ddhub:DrillingEquipment. 
ddhub:CavingsComponent a owl:Class; 
                       rdfs:comment ""@EN; 
                       rdfs:subClassOf ddhub:FormationSolidComponent. 
ddhub:CementBondLoggingTools a owl:Class; 
                             rdfs:comment ""@EN; 
                             rdfs:subClassOf ddhub:WirelineLoggingTools. 
ddhub:CementHead a owl:Class; 
                 rdfs:comment ""@EN; 
                 rdfs:subClassOf ddhub:CementingEquipment. 
ddhub:CementingEquipment a owl:Class; 
                         rdfs:comment ""@EN; 
                         rdfs:subClassOf ddhub:RigEquipment. 
ddhub:CementingServiceCompany a owl:Class; 
                              rdfs:comment ""@EN; 
                              rdfs:subClassOf ddhub:ServiceCompany. 
ddhub:CementLines a owl:Class; 
                  rdfs:comment ""@EN; 
                  rdfs:subClassOf ddhub:CementingEquipment. 
ddhub:CementManifold a owl:Class; 
                     rdfs:comment ""@EN; 
                     rdfs:subClassOf ddhub:CementingEquipment. 
ddhub:CementPump a owl:Class; 
                 rdfs:comment ""@EN; 
                 rdfs:subClassOf ddhub:CementingEquipment. 
ddhub:CementSlurry a owl:Class; 
                   rdfs:comment ""@EN; 
                   rdfs:subClassOf ddhub:CementingEquipment. 
ddhub:CementSpacer a owl:Class; 
                   rdfs:comment ""@EN; 
                   rdfs:subClassOf ddhub:CementingEquipment. 
ddhub:CementStand a owl:Class; 
                  rdfs:comment ""@EN; 
                  rdfs:subClassOf ddhub:CementingEquipment. 
ddhub:CementStinger a owl:Class; 
                    rdfs:comment ""@EN; 
                    rdfs:subClassOf ddhub:CementingEquipment. 
ddhub:CementUnit a owl:Class; 
                 rdfs:comment ""@EN; 
                 rdfs:subClassOf ddhub:CementingEquipment. 
ddhub:Centralizers a owl:Class; 
                   rdfs:comment ""@EN; 
                   rdfs:subClassOf ddhub:CasingString. 
ddhub:CentrifugalDegasser a owl:Class; 
                          rdfs:comment ""@EN; 
                          rdfs:subClassOf ddhub:Degasser. 
ddhub:CentrifugalMudPump a owl:Class; 
                         rdfs:comment ""@EN; 
                         rdfs:subClassOf ddhub:MudPump. 
ddhub:Centrifuge a owl:Class; 
                 rdfs:comment ""@EN; 
                 rdfs:subClassOf ddhub:CirculationSystem. 
ddhub:ChaoticWhirl a owl:Class; 
                   rdfs:comment ""@EN; 
                   rdfs:subClassOf ddhub:Whirling. 
ddhub:ChemicalTank a owl:Class; 
                   rdfs:comment ""@EN; 
                   rdfs:subClassOf ddhub:MudPits. 
ddhub:ChokeLine a owl:Class; 
                rdfs:comment ""@EN; 
                rdfs:subClassOf ddhub:WellControlSystem. 
ddhub:ChokeManifold a owl:Class; 
                    rdfs:comment ""@EN; 
                    rdfs:subClassOf ddhub:WellControlSystem. 
ddhub:ChokeValve a owl:Class; 
                 rdfs:comment ""@EN; 
                 rdfs:subClassOf ddhub:ChokeManifold. 
ddhub:ChokeValveGatevalve a owl:Class; 
                          rdfs:comment ""@EN; 
                          rdfs:subClassOf ddhub:ChokeValve. 
ddhub:CirculationSub a owl:Class; 
                     rdfs:comment ""@EN; 
                     rdfs:subClassOf ddhub:DrillingEquipment. 
ddhub:CirculationSystem a owl:Class; 
                        rdfs:comment ""@EN; 
                        rdfs:subClassOf ddhub:RigEquipment. 
ddhub:Clampon a owl:Class; 
              rdfs:comment ""@EN; 
              rdfs:subClassOf ddhub:BladeType. 
ddhub:Clock a owl:Class; 
            rdfs:comment """Represents a clock
"""@EN; 
            rdfs:subClassOf ddhub:DWISNoun. 
ddhub:ClusterPositionLocation a owl:Class; 
                              rdfs:comment ""@EN; 
                              rdfs:subClassOf ddhub:PositionReferenceLocation. 
ddhub:CoiledTubingEquipment a owl:Class; 
                            rdfs:comment ""@EN; 
                            rdfs:subClassOf ddhub:Equipment. 
ddhub:CoiledTubingReel a owl:Class; 
                       rdfs:comment ""@EN; 
                       rdfs:subClassOf ddhub:CoiledTubingEquipment. 
ddhub:CollapsePressure a owl:Class; 
                       rdfs:comment ""@EN; 
                       rdfs:subClassOf ddhub:PrototypeData. 
ddhub:CollapsePressureGradient a owl:Class; 
                               rdfs:comment ""@EN; 
                               rdfs:subClassOf ddhub:PrototypeData. 
ddhub:Command a owl:Class; 
              rdfs:comment ""@EN; 
              rdfs:subClassOf ddhub:ProcessData. 
ddhub:CompletionWorkoverRiser a owl:Class; 
                              rdfs:comment ""@EN; 
                              rdfs:subClassOf ddhub:MarineSystem. 
ddhub:CompressibilityDrillingQuantity a owl:Class; 
                                      rdfs:comment """Compressibility is the measure of how much a substance's volume decreases under pressure. It indicates how easily a material or fluid can be compressed and is typically expressed as a change in volume per unit change in pressure.
The dimension of compressibility is:
$$[T^{2}LM^{-1}]$$.
The SI unit for **compressibility** is: inverse pascal with the associated unit label $\\frac{1}{Pa}$
The meaningful precision of compressibility in the drilling context is typically: 1E-13 1/Pa
"""@EN; 
                                      rdfs:subClassOf ddhub:MeasurableQuantity. 
ddhub:CompressibilityQuantity a owl:Class; 
                              rdfs:comment """Compressibility is the measure of how much a substance's volume decreases under pressure. It indicates how easily a material or fluid can be compressed and is typically expressed as a change in volume per unit change in pressure.
The dimension of compressibility is:
$$[T^{2}LM^{-1}]$$.
The SI unit for **compressibility** is: inverse pascal with the associated unit label $\\frac{1}{Pa}$
"""@EN; 
                              rdfs:subClassOf ddhub:Quantity. 
ddhub:CompressiveDrillPipe a owl:Class; 
                           rdfs:comment ""@EN; 
                           rdfs:subClassOf ddhub:DrillString. 
ddhub:ComputationUnit a owl:Class; 
                      rdfs:comment """Denotes a complex computation unit, typically based on advanced numerical modeling
"""@EN; 
                      rdfs:subClassOf ddhub:DataFlowNode. 
ddhub:ComputedData a owl:Class; 
                   rdfs:comment ""@EN; 
                   rdfs:subClassOf ddhub:PhysicalData. 
ddhub:ComputedState a owl:Class; 
                    rdfs:comment """A state represents the current configuation of a system.
"""@EN; 
                    rdfs:subClassOf ddhub:ComputationUnit. 
ddhub:ConcernsAFluidComponent a owl:ObjectProperty; 
                              rdfs:comment ""@EN; 
                              rdfs:domain ddhub:DrillingDataPoint; 
                              rdfs:range ddhub:FluidComponent; 
                              rdfs:subPropertyOf ddhub:DWISVerb. 
ddhub:ConductorDrivePipe a owl:Class; 
                         rdfs:comment ""@EN; 
                         rdfs:subClassOf ddhub:CasingString. 
ddhub:ConductorTensioners a owl:Class; 
                          rdfs:comment ""@EN; 
                          rdfs:subClassOf ddhub:MarineSystem. 
ddhub:ConnectedCondition a owl:Class; 
                         rdfs:comment ""@EN; 
                         rdfs:subClassOf ddhub:ValidityCondition. 
ddhub:Connection a owl:Class; 
                 rdfs:comment ""@EN; 
                 rdfs:subClassOf ddhub:CasingString. 
ddhub:ConnectionWelded a owl:Class; 
                       rdfs:comment ""@EN; 
                       rdfs:subClassOf ddhub:Connection. 
ddhub:ConsistencyIndexRheologyQuantity a owl:Class; 
                                       rdfs:comment """Dynamic viscosity is a measure of a fluid's resistance to shear or flow when a force is applied. It quantifies how thick or thin the fluid is.
The dimension of dynamic viscosity is:
$$[ML^{-1}T^{-1}]$$.
The SI unit for **dynamic viscosity** is: pascal second with the associated unit label $Pa \\cdot s$
The consistency index in rheology measures a fluid's resistance to flow; it quantifies the fluid's viscosity and how it changes with shear rate.
The meaningful precision of a consistency index in rheology is typically: 0.0001 Pa•s
"""@EN; 
                                       rdfs:subClassOf ddhub:MeasurableQuantity. 
ddhub:ContinuousDataType a owl:Class; 
                         rdfs:comment ""@EN; 
                         rdfs:subClassOf ddhub:DataType. 
ddhub:ContinuousProportional a owl:Class; 
                             rdfs:comment ""@EN; 
                             rdfs:subClassOf ddhub:RotarySteerableSystems. 
ddhub:ControlAndMonitoringEquipment a owl:Class; 
                                    rdfs:comment ""@EN; 
                                    rdfs:subClassOf ddhub:ControlConsole. 
ddhub:ControlConsole a owl:Class; 
                     rdfs:comment ""@EN; 
                     rdfs:subClassOf ddhub:CoiledTubingEquipment. 
ddhub:Controller a owl:Class; 
                 rdfs:comment ""@EN; 
                 rdfs:subClassOf ddhub:DataFlowNode. 
ddhub:ControllerFunction a owl:Class; 
                         rdfs:comment """A `ControllerFunction` is a `RunnableFunction` that executes a feedback control loop to follow as closely
as possible one or several desired values. A typical example of `ControllerFunction` is the `AutoDriller`. An `AutoDriller` 
follows as closely as possible, for instance, a desired `WOB`.
"""@EN; 
                         rdfs:subClassOf ddhub:RunnableFunction. 
ddhub:ControlLines a owl:Class; 
                   rdfs:comment ""@EN; 
                   rdfs:subClassOf ddhub:WellControlSystem. 
ddhub:ControlManifold a owl:Class; 
                      rdfs:comment ""@EN; 
                      rdfs:subClassOf ddhub:WellControlSystem. 
ddhub:Controls a owl:ObjectProperty; 
               rdfs:comment ""@EN; 
               rdfs:domain ddhub:DWISNoun; 
               rdfs:range ddhub:DWISNoun; 
               rdfs:subPropertyOf ddhub:DWISVerb. 
ddhub:ControlSystem a owl:Class; 
                    rdfs:comment ""@EN; 
                    rdfs:subClassOf ddhub:DataFlowNode. 
ddhub:ConventionalDerrick a owl:Class; 
                          rdfs:comment ""@EN; 
                          rdfs:subClassOf ddhub:Derrick. 
ddhub:ConversionFactorA a owl:DatatypeProperty, owl:FunctionalProperty; 
                        rdfs:comment """Unit conversion from SI unit is performed as:
ConvertedValue = ConversionFactorA + SIValue * ConversionFactorB
"""@EN; 
                        rdfs:domain ddhub:Unit; 
                        rdfs:range xsd:double. 
ddhub:ConversionFactorB a owl:DatatypeProperty, owl:FunctionalProperty; 
                        rdfs:comment """Unit conversion from SI unit is performed as:
ConvertedValue = ConversionFactorA + SIValue * ConversionFactorB
"""@EN; 
                        rdfs:domain ddhub:Unit; 
                        rdfs:range xsd:double. 
ddhub:CoringTool a owl:Class; 
                 rdfs:comment ""@EN; 
                 rdfs:subClassOf ddhub:DrillingEquipment. 
ddhub:CorrectedMeasurement a owl:Class; 
                           rdfs:comment ""@EN; 
                           rdfs:subClassOf ddhub:Measurement. 
ddhub:Crossover a owl:Class; 
                rdfs:comment ""@EN; 
                rdfs:subClassOf ddhub:CasingString. 
ddhub:CrownBlock a owl:Class; 
                 rdfs:comment ""@EN; 
                 rdfs:subClassOf ddhub:MechanicalBlock. 
ddhub:CrownValveVerticalLocation a owl:Class; 
                                 rdfs:comment ""@EN; 
                                 rdfs:subClassOf ddhub:VerticalReferenceLocation. 
ddhub:CtBhaComponents a owl:Class; 
                      rdfs:comment ""@EN; 
                      rdfs:subClassOf ddhub:CoiledTubingEquipment. 
ddhub:CurvatureDrillingQuantity a owl:Class; 
                                rdfs:comment """A curvature is the second derivative of a position compared to the curvilinear abscissa: $\\frac{d^2x}{ds^2}$, where $x$ is the position and $s$ is the curvilinear abscissa.
The dimension of curvature is:
$$[{\\theta}L^{-1}]$$.
The SI unit for **curvature** is: radian per metre with the associated unit label $\\frac{rad}{m}$
The meaningful precision of curvature in the drilling context is typically: 5.817764173314432E-06 rad/m
"""@EN; 
                                rdfs:subClassOf ddhub:MeasurableQuantity. 
ddhub:CurvatureQuantity a owl:Class; 
                        rdfs:comment """A curvature is the second derivative of a position compared to the curvilinear abscissa: $\\frac{d^2x}{ds^2}$, where $x$ is the position and $s$ is the curvilinear abscissa.
The dimension of curvature is:
$$[{\\theta}L^{-1}]$$.
The SI unit for **curvature** is: radian per metre with the associated unit label $\\frac{rad}{m}$
"""@EN; 
                        rdfs:subClassOf ddhub:Quantity. 
ddhub:CutOffFrequency a owl:DatatypeProperty, owl:FunctionalProperty; 
                      rdfs:comment """
"""@EN; 
                      rdfs:domain ddhub:HighPassFilter, ddhub:LowPassFilter; 
                      rdfs:range xsd:double. 
ddhub:CuttingsAnalysisEquipmnet a owl:Class; 
                                rdfs:comment ""@EN; 
                                rdfs:subClassOf ddhub:MudLoggingEquipment. 
ddhub:CuttingsBedLocation a owl:Class; 
                          rdfs:comment ""@EN; 
                          rdfs:subClassOf ddhub:AbscissaReferenceLocation. 
ddhub:CuttingsComponent a owl:Class; 
                        rdfs:comment ""@EN; 
                        rdfs:subClassOf ddhub:FormationSolidComponent. 
ddhub:CuttingsSamplingEquipment a owl:Class; 
                                rdfs:comment ""@EN; 
                                rdfs:subClassOf ddhub:MudLoggingEquipment. 
ddhub:Cylinders a owl:Class; 
                rdfs:comment ""@EN; 
                rdfs:subClassOf ddhub:PistonMudPump. 
ddhub:CylindricalReferenceFrame a owl:Class; 
                                rdfs:comment ""@EN; 
                                rdfs:subClassOf ddhub:ThreeDimensionalReferenceFrame. 
ddhub:DataAnalysisServiceCompany a owl:Class; 
                                 rdfs:comment """A data analysis service company is an entity that analyses measured data and provide new information from these measurements.
"""@EN; 
                                 rdfs:subClassOf ddhub:ServiceCompany. 
ddhub:DataEndPoint a owl:Class; 
                   rdfs:comment ""@EN; 
                   rdfs:subClassOf ddhub:DWISNoun. 
ddhub:DataFlowNode a owl:Class; 
                   rdfs:comment ""@EN; 
                   rdfs:subClassOf ddhub:DWISNoun. 
ddhub:DataProvider a owl:Class; 
                   rdfs:comment """A data provider is any sources for data
"""@EN; 
                   rdfs:subClassOf ddhub:DWISNoun. 
ddhub:DataType a owl:Class; 
               rdfs:comment ""@EN; 
               rdfs:subClassOf ddhub:DWISNoun. 
ddhub:DeadLine a owl:Class; 
               rdfs:comment ""@EN; 
               rdfs:subClassOf ddhub:DrillLine. 
ddhub:DeadLineAnchor a owl:Class; 
                     rdfs:comment ""@EN; 
                     rdfs:subClassOf ddhub:DrillLineFastener. 
ddhub:Degasser a owl:Class; 
               rdfs:comment ""@EN; 
               rdfs:subClassOf ddhub:CirculationSystem. 
ddhub:DensityIn a owl:Class; 
                rdfs:comment ""@EN; 
                rdfs:subClassOf ddhub:PrototypeData. 
ddhub:DensityOut a owl:Class; 
                 rdfs:comment ""@EN; 
                 rdfs:subClassOf ddhub:PrototypeData. 
ddhub:DepthAndAngleFrame a owl:Class; 
                         rdfs:comment ""@EN; 
                         rdfs:subClassOf ddhub:ReferenceFrame. 
ddhub:DepthDrillingQuantity a owl:Class; 
                            rdfs:comment """Length is a measure of distance.
The dimension of length is:
$$[L]$$.
The SI unit for **length** is: metre with the associated unit label $m$
The meaningful precision of depth in the drilling context is typically: 0.001 m
"""@EN; 
                            rdfs:subClassOf ddhub:MeasurableQuantity. 
ddhub:Derivation a owl:Class; 
                 rdfs:comment ""@EN; 
                 rdfs:subClassOf ddhub:TimeBasedTransformation. 
ddhub:DerivedMeasurement a owl:Class; 
                         rdfs:comment ""@EN; 
                         rdfs:subClassOf ddhub:Measurement. 
ddhub:Derrick a owl:Class; 
              rdfs:comment ""@EN; 
              rdfs:subClassOf ddhub:HoistingSystem. 
ddhub:DerrickFloorVerticalLocation a owl:Class; 
                                   rdfs:comment ""@EN; 
                                   rdfs:subClassOf ddhub:VerticalReferenceLocation. 
ddhub:DeterministicModel a owl:Class; 
                         rdfs:comment ""@EN; 
                         rdfs:subClassOf ddhub:ModelType. 
ddhub:DiameterPipeDrillingQuantity a owl:Class; 
                                   rdfs:comment """Length is a measure of distance.
The dimension of length is:
$$[L]$$.
The SI unit for **length** is: metre with the associated unit label $m$
The meaningful precision of small length is typically: 0.0001 m
The meaningful precision of pipe diameter in the drilling context is typically: 0.0001 m
"""@EN; 
                                   rdfs:subClassOf ddhub:MeasurableQuantity. 
ddhub:DiameterPoreDrillingQuantity a owl:Class; 
                                   rdfs:comment """Length is a measure of distance.
The dimension of length is:
$$[L]$$.
The SI unit for **length** is: metre with the associated unit label $m$
The meaningful precision of small length is typically: 1E-07 m
The meaningful precision of pore diameter in the drilling context is typically: 1E-07 m
"""@EN; 
                                   rdfs:subClassOf ddhub:MeasurableQuantity. 
ddhub:DiameterSmallQuantity a owl:Class; 
                            rdfs:comment """Length is a measure of distance.
The dimension of length is:
$$[L]$$.
The SI unit for **length** is: metre with the associated unit label $m$
The meaningful precision of small diameter is typically: 0.0001 m
"""@EN; 
                            rdfs:subClassOf ddhub:MeasurableQuantity. 
ddhub:Diamond a owl:Class; 
              rdfs:comment ""@EN; 
              rdfs:subClassOf ddhub:FixedCutter. 
ddhub:DiamondCore a owl:Class; 
                  rdfs:comment ""@EN; 
                  rdfs:subClassOf ddhub:FixedCutter. 
ddhub:DiaphragmMudPump a owl:Class; 
                       rdfs:comment ""@EN; 
                       rdfs:subClassOf ddhub:MudPump. 
ddhub:DieselElectricalDrawworks a owl:Class; 
                                rdfs:comment ""@EN; 
                                rdfs:subClassOf ddhub:Drawworks. 
ddhub:DifferentialStickingLocation a owl:Class; 
                                   rdfs:comment ""@EN; 
                                   rdfs:subClassOf ddhub:AbscissaReferenceLocation. 
ddhub:DimensionlessQuantity a owl:Class; 
                            rdfs:comment """As its name indicates, a dimensionless quantity has no dimension:
"""@EN; 
                            rdfs:subClassOf ddhub:Quantity. 
ddhub:DimensionLessStandardQuantity a owl:Class; 
                                    rdfs:comment """As its name indicates, a dimensionless quantity has no dimension:
The meaningful precision of standard dimensionless values is typically: 0.001 
"""@EN; 
                                    rdfs:subClassOf ddhub:MeasurableQuantity. 
ddhub:DipmeterAndImagingTools a owl:Class; 
                              rdfs:comment ""@EN; 
                              rdfs:subClassOf ddhub:WirelineLoggingTools. 
ddhub:DirectionalCasingWhileDrilling a owl:Class; 
                                     rdfs:comment ""@EN; 
                                     rdfs:subClassOf ddhub:Casingwhiledrilling. 
ddhub:DirectionalServiceCompany a owl:Class; 
                                rdfs:comment """A directional service company is an entity that provides services for downhole directional drilling and downhole measurements.
"""@EN; 
                                rdfs:subClassOf ddhub:ServiceCompany. 
ddhub:DirectionalTool a owl:Class; 
                      rdfs:comment ""@EN; 
                      rdfs:subClassOf ddhub:MeasurementWhileDrillingTools. 
ddhub:DirectTransformation a owl:Class; 
                           rdfs:comment """Direct transformations are performed using only the current value of their inputs, time is not involved
"""@EN; 
                           rdfs:subClassOf ddhub:Transformation. 
ddhub:DiscreteDataType a owl:Class; 
                       rdfs:comment ""@EN; 
                       rdfs:subClassOf ddhub:DataType. 
ddhub:DistanceBetweenRepeaters a owl:DatatypeProperty, owl:FunctionalProperty; 
                               rdfs:comment """
"""@EN; 
                               rdfs:domain ddhub:Telemetry; 
                               rdfs:range xsd:double. 
ddhub:Diverter a owl:Class; 
               rdfs:comment ""@EN; 
               rdfs:subClassOf ddhub:WellControlSystem. 
ddhub:DiverterLine a owl:Class; 
                   rdfs:comment ""@EN; 
                   rdfs:subClassOf ddhub:Diverter. 
ddhub:DiverterLineHanger a owl:Class; 
                         rdfs:comment ""@EN; 
                         rdfs:subClassOf ddhub:Diverter. 
ddhub:DogHouse a owl:Class; 
               rdfs:comment ""@EN; 
               rdfs:subClassOf ddhub:DrillFloorStructure. 
ddhub:Dolly a owl:Class; 
            rdfs:comment ""@EN; 
            rdfs:subClassOf ddhub:DrillFloorEquipment. 
ddhub:DollyRail a owl:Class; 
                rdfs:comment ""@EN; 
                rdfs:subClassOf ddhub:DrillFloorEquipment. 
ddhub:Doubles a owl:Class; 
              rdfs:comment ""@EN; 
              rdfs:subClassOf ddhub:Grouping. 
ddhub:DoubleStandDerrick a owl:Class; 
                         rdfs:comment ""@EN; 
                         rdfs:subClassOf ddhub:Derrick. 
ddhub:DownholeAlternator a owl:Class; 
                         rdfs:comment ""@EN; 
                         rdfs:subClassOf ddhub:PowerSystems. 
ddhub:DownholeBatteries a owl:Class; 
                        rdfs:comment ""@EN; 
                        rdfs:subClassOf ddhub:PowerSystems. 
ddhub:DownholeCtConnectors a owl:Class; 
                           rdfs:comment ""@EN; 
                           rdfs:subClassOf ddhub:CoiledTubingEquipment. 
ddhub:DownholeECD a owl:Class; 
                  rdfs:comment ""@EN; 
                  rdfs:subClassOf ddhub:PrototypeData. 
ddhub:DownholeEquipment a owl:Class; 
                        rdfs:comment ""@EN; 
                        rdfs:subClassOf ddhub:Equipment. 
ddhub:DownholeHydraulicNetwork a owl:Class; 
                               rdfs:comment ""@EN; 
                               rdfs:subClassOf ddhub:HydraulicNetwork. 
ddhub:DownholeMotor a owl:Class; 
                    rdfs:comment ""@EN; 
                    rdfs:subClassOf ddhub:DrillingEquipment. 
ddhub:DownholePressure a owl:Class; 
                       rdfs:comment ""@EN; 
                       rdfs:subClassOf ddhub:PrototypeData. 
ddhub:DownholeRPM a owl:Class; 
                  rdfs:comment ""@EN; 
                  rdfs:subClassOf ddhub:PrototypeData. 
ddhub:DownHoleTelemetry a owl:Class; 
                        rdfs:comment ""@EN; 
                        rdfs:subClassOf ddhub:Telemetry. 
ddhub:DownholeTemperature a owl:Class; 
                          rdfs:comment ""@EN; 
                          rdfs:subClassOf ddhub:PrototypeData. 
ddhub:DownholeTorque a owl:Class; 
                     rdfs:comment ""@EN; 
                     rdfs:subClassOf ddhub:PrototypeData. 
ddhub:DownholeValveAssembly a owl:Class; 
                            rdfs:comment ""@EN; 
                            rdfs:subClassOf ddhub:CasingEquipment. 
ddhub:Drawworks a owl:Class; 
                rdfs:comment ""@EN; 
                rdfs:subClassOf ddhub:HoistingSystem. 
ddhub:DrawWorksControlSystem a owl:Class; 
                             rdfs:comment ""@EN; 
                             rdfs:subClassOf ddhub:ControlSystem. 
ddhub:DrillCollars a owl:Class; 
                   rdfs:comment ""@EN; 
                   rdfs:subClassOf ddhub:DrillString. 
ddhub:DrillersConsole a owl:Class; 
                      rdfs:comment ""@EN; 
                      rdfs:subClassOf ddhub:DrillFloorEquipment. 
ddhub:DrillFloorEquipment a owl:Class; 
                          rdfs:comment ""@EN; 
                          rdfs:subClassOf ddhub:DrillFloorSystems. 
ddhub:DrillFloorStructure a owl:Class; 
                          rdfs:comment ""@EN; 
                          rdfs:subClassOf ddhub:DrillFloorSystems. 
ddhub:DrillFloorSubstructure a owl:Class; 
                             rdfs:comment ""@EN; 
                             rdfs:subClassOf ddhub:DrillFloorStructure. 
ddhub:DrillFloorSystems a owl:Class; 
                        rdfs:comment ""@EN; 
                        rdfs:subClassOf ddhub:RigEquipment. 
ddhub:DrillingBit a owl:Class; 
                  rdfs:comment ""@EN; 
                  rdfs:subClassOf ddhub:DrillstemTerminator. 
ddhub:DrillingContractor a owl:Class; 
                         rdfs:comment ""@EN; 
                         rdfs:subClassOf ddhub:DataProvider. 
ddhub:DrillingDataPoint a owl:Class; 
                        rdfs:comment """Main type of DDHub data. Represents a drilling signal.
Can be a dynamic signal (linked to a ValueNode) or a static parameter. 
"""@EN; 
                        rdfs:subClassOf ddhub:DWISNoun. 
ddhub:DrillingEquipment a owl:Class; 
                        rdfs:comment ""@EN; 
                        rdfs:subClassOf ddhub:DownholeEquipment. 
ddhub:DrillingFluid a owl:Class; 
                    rdfs:comment ""@EN; 
                    rdfs:subClassOf ddhub:CirculationSystem. 
ddhub:DrillingFluidGasComponent a owl:Class; 
                                rdfs:comment ""@EN; 
                                rdfs:subClassOf ddhub:GasComponent. 
ddhub:DrillingFluidLiquidComponent a owl:Class; 
                                   rdfs:comment ""@EN; 
                                   rdfs:subClassOf ddhub:LiquidComponent. 
ddhub:DrillingFluidOilComponent a owl:Class; 
                                rdfs:comment ""@EN; 
                                rdfs:subClassOf ddhub:DrillingFluidLiquidComponent. 
ddhub:DrillingFluidProvider a owl:Class; 
                            rdfs:comment """A drilling fluid provider is a company that provides and maintains the drilling fluids during well construction.
"""@EN; 
                            rdfs:subClassOf ddhub:ServiceCompany. 
ddhub:DrillingFluidSolidComponent a owl:Class; 
                                  rdfs:comment ""@EN; 
                                  rdfs:subClassOf ddhub:SolidComponent. 
ddhub:DrillingFluidWaterComponent a owl:Class; 
                                  rdfs:comment ""@EN; 
                                  rdfs:subClassOf ddhub:DrillingFluidLiquidComponent. 
ddhub:DrillingIncident a owl:Class; 
                       rdfs:comment ""@EN; 
                       rdfs:subClassOf ddhub:DWISNoun. 
ddhub:DrillingProgram a owl:Class; 
                      rdfs:comment ""@EN; 
                      rdfs:subClassOf ddhub:Plan. 
ddhub:DrillingRiser a owl:Class; 
                    rdfs:comment ""@EN; 
                    rdfs:subClassOf ddhub:MarineSystem. 
ddhub:DrillingSignal a owl:Class; 
                     rdfs:comment """Data structure used to store the streaming drilling data.
"""@EN; 
                     rdfs:subClassOf ddhub:DWISNoun. 
ddhub:DrillLine a owl:Class; 
                rdfs:comment ""@EN; 
                rdfs:subClassOf ddhub:HoistingSystem. 
ddhub:DrillLineFastener a owl:Class; 
                        rdfs:comment ""@EN; 
                        rdfs:subClassOf ddhub:HoistingSystem. 
ddhub:DrillPipe a owl:Class; 
                rdfs:comment ""@EN; 
                rdfs:subClassOf ddhub:DrillString. 
ddhub:DrillPipeElevator a owl:Class; 
                        rdfs:comment ""@EN; 
                        rdfs:subClassOf ddhub:DrillFloorEquipment. 
ddhub:DrillPipesAnnular a owl:Class; 
                        rdfs:comment ""@EN; 
                        rdfs:subClassOf ddhub:Annular. 
ddhub:DrillPipesInner a owl:Class; 
                      rdfs:comment ""@EN; 
                      rdfs:subClassOf ddhub:Pipe. 
ddhub:DrillPipeTongs a owl:Class; 
                     rdfs:comment ""@EN; 
                     rdfs:subClassOf ddhub:DrillFloorEquipment. 
ddhub:DrillStemMaterialStrengthDrillingQuantity a owl:Class; 
                                                rdfs:comment """Material strength refers to the ability of a material to withstand an applied force or load without failing or deforming. It measures how much stress a material can endure before it breaks, bends, or permanently deforms, often categorized into types like tensile, compressive, and shear strength.
The dimension of material strength is:
$$[ML^{-1}T^{-2}]$$.
The SI unit for **material strength** is: pascal with the associated unit label $Pa$
The meaningful precision of drill stem material strength in the drilling context is typically: 10000 Pa
"""@EN; 
                                                rdfs:subClassOf ddhub:MeasurableQuantity. 
ddhub:DrillStemMechanicalModel a owl:Class; 
                               rdfs:comment """A mechanical model for a drill-stem. Another name for drill-stem mechanical models is a torque and drag model.
"""@EN; 
                               rdfs:subClassOf ddhub:MathematicalModel. 
ddhub:DrillstemTerminator a owl:Class; 
                          rdfs:comment ""@EN; 
                          rdfs:subClassOf ddhub:DrillingEquipment. 
ddhub:DrillString a owl:Class; 
                  rdfs:comment ""@EN; 
                  rdfs:subClassOf ddhub:Tubulars. 
ddhub:DrillStringCenterLineFrame a owl:Class; 
                                 rdfs:comment ""@EN; 
                                 rdfs:subClassOf ddhub:OneDimensionalCurviLinearReferenceFrame. 
ddhub:DrillStringMagneticFluxDrillingQuantity a owl:Class; 
                                              rdfs:comment """Magnetic flux is the measure of the total magnetic field passing through a given area. It quantifies the strength and distribution of a magnetic field over a surface.
The dimension of magnetic flux is:
$$[L^{2}MI^{-1}T^{-2}]$$.
The SI unit for **magnetic flux** is: weber with the associated unit label $Wb$
The meaningful precision of magnetic flux in the drilling context is typically: 1E-07 Wb
"""@EN; 
                                              rdfs:subClassOf ddhub:MeasurableQuantity. 
ddhub:DrillWater a owl:Class; 
                 rdfs:comment ""@EN; 
                 rdfs:subClassOf ddhub:DrillingFluid. 
ddhub:DualActing a owl:Class; 
                 rdfs:comment ""@EN; 
                 rdfs:subClassOf ddhub:Action. 
ddhub:DurationDrillingQuantity a owl:Class; 
                               rdfs:comment """Time is a continuous, measurable progression in which events occur, from the past through the present to the future.
The dimension of time is:
$$[T]$$.
The SI unit for **time** is: second with the associated unit label $s$
The meaningful precision of time in the drilling context is typically: 0.001 s
"""@EN; 
                               rdfs:subClassOf ddhub:MeasurableQuantity. 
ddhub:DWISADCSCapabilityDescriptor a owl:Class; 
                                   rdfs:comment ""@EN; 
                                   rdfs:subClassOf ddhub:DWISInternalService. 
ddhub:DWISADCSInterface a owl:Class; 
                        rdfs:comment ""@EN; 
                        rdfs:subClassOf ddhub:DWISInternalService. 
ddhub:DWISAdviceComposer a owl:Class; 
                         rdfs:comment ""@EN; 
                         rdfs:subClassOf ddhub:DWISInternalService. 
ddhub:DWISAttributeCardinalityRestriction a owl:Class, owl:Restriction; 
                                          owl:onClass ddhub:ActivableFunction, ddhub:RunnableFunction, ddhub:Advisor, ddhub:BandPassFilter, ddhub:HighPassFilter, ddhub:LowPassFilter, ddhub:NumberOfSampleMovingAverage, ddhub:TimeWindowMovingAverage, ddhub:Buffering, ddhub:NumberOfItemsRangeExtraction, ddhub:TimeWindowRangeExtraction, ddhub:Resampling, ddhub:DataProvider, ddhub:OperatingCompany, ddhub:ServiceCompany, ddhub:DirectionalServiceCompany, ddhub:DrillingFluidProvider, ddhub:LoggingServiceCompany, ddhub:CementingServiceCompany, ddhub:DataAnalysisServiceCompany, ddhub:DrillingContractor, ddhub:DWISInternalService, ddhub:Telemetry, ddhub:DrillingDataPoint, ddhub:DrillingSignal, ddhub:DynamicDrillingSignal, ddhub:DataEndPoint, ddhub:WitsMLTimeBasedLogEndPoint, ddhub:EndPointMapping, ddhub:HydraulicConnectedState, ddhub:HydraulicJunction, ddhub:MeasurableQuantity, ddhub:MechanicalElementState, ddhub:OneDimensionalReferenceFrame, ddhub:Quantity, ddhub:Unit, ddhub:Clock, ddhub:SynchronizationGroup, ddhub:FullScaleUncertainty, ddhub:SensorUncertainty; 
                                          owl:onProperty ddhub:HasFunction, ddhub:IsAuxiliary, ddhub:AdviceType, ddhub:MinFrequency, ddhub:MaxFrequency, ddhub:CutOffFrequency, ddhub:NumberOfSamples, ddhub:TimeWindow, ddhub:BufferingInterval, ddhub:NumberOfItems, ddhub:ResamplingRate, ddhub:ResamplingDelay, ddhub:Validity, ddhub:ProviderName, ddhub:NumberOfRepeaters, ddhub:DistanceBetweenRepeaters, ddhub:AverageDelayByRepeater, ddhub:IsValid, ddhub:Value, ddhub:TimeStampAtSource, ddhub:TimeStampAcquisition, ddhub:EndPointDescription, ddhub:WellUID, ddhub:WellName, ddhub:WellboreUID, ddhub:WellboreName, ddhub:LogUID, ddhub:LogName, ddhub:Mnemonic, ddhub:FixedIndices, ddhub:ValuesIndices, ddhub:MeasurementIndex, ddhub:LeftToRight, ddhub:RightToLeft, ddhub:MeaningfulPrecision, ddhub:PostiveUpward, ddhub:L, ddhub:M, ddhub:T, ddhub:I, ddhub:ThT, ddhub:N, ddhub:J, ddhub:Theta, ddhub:Omega, ddhub:SIUnit, ddhub:Symbol, ddhub:ConversionFactorA, ddhub:ConversionFactorB, ddhub:LeapSeconds, ddhub:Stratum, ddhub:NetworkSynchronizationLatencyAverage, ddhub:NetworkSynchronizationLatencyStandardDeviation, ddhub:Resolution, ddhub:MaximumFluctuations, ddhub:SynchronizationDelay, ddhub:SamplingRate, ddhub:FullScale, ddhub:ProportionError, ddhub:Accuracy, ddhub:Precision; 
                                          owl:qualifiedCardinality "1"^^xsd:nonNegativeInteger. 
ddhub:DWISContextualDataBuilder a owl:Class; 
                                rdfs:comment ""@EN; 
                                rdfs:subClassOf ddhub:DWISInternalService. 
ddhub:DWISDDHub a owl:Class; 
                rdfs:comment ""@EN; 
                rdfs:subClassOf ddhub:DWISInternalService. 
ddhub:DWISDrillingProcessStateInterpreter a owl:Class; 
                                          rdfs:comment ""@EN; 
                                          rdfs:subClassOf ddhub:DWISInternalService. 
ddhub:DWISInternalService a owl:Class; 
                          rdfs:comment """A DWIS internal service is an internal component of the DWIS infrastructure that generates information that can be used by any systems connected to the DWIS infrastructure.
"""@EN; 
                          rdfs:subClassOf ddhub:DataProvider. 
ddhub:DWISLogger a owl:Class; 
                 rdfs:comment ""@EN; 
                 rdfs:subClassOf ddhub:DWISInternalService. 
ddhub:DWISNoun a owl:Class; 
               rdfs:comment """Nouns refer to the nature of a node in the graph. Implicitely a noun refers to a "is a" relation between the instance node and the noun. This is the root class for all the nouns defined in the DWIS vocabulary.
"""@EN. 
ddhub:DWISScheduler a owl:Class; 
                    rdfs:comment ""@EN; 
                    rdfs:subClassOf ddhub:DWISInternalService. 
ddhub:DWISVerb a owl:ObjectProperty; 
               rdfs:comment """This is the root class for all verbs defined in the DWIS vocabulary. It is used to define a relation between a subject, which can be of any `DWISNoun` and an object, also of any type of `DWISNoun`.
"""@EN; 
               rdfs:domain ddhub:DWISNoun; 
               rdfs:range ddhub:DWISNoun. 
ddhub:DWISVocabulary a owl:Ontology; 
                     rdfs:comment "This is the ontology generated by the D-WIS WG1: Semantics of Real-time signals. It has been automatically generated from the vocabulary defined at https://github.com/D-WIS/DDHub-Semantic-Interoperability/tree/main/docs/vocabulary_development/auto-generated"@EN; 
                     rdfs:isDefinedBy "D-WIS WG1: Semantics of Real-time signals"^^xsd:string; 
                     rdfs:label "D-WIS vocabulary"^^xsd:string; 
                     owl:versionInfo "0.1"^^xsd:string; 
                     owl:versionIRI "https://github.com/D-WIS/DDHub-Semantic-Interoperability/tree/main/docs/vocabulary_development/auto-generated/dwis.owl"^^xsd:anyURI. 
ddhub:Dynamic a owl:Class; 
              rdfs:comment ""@EN; 
              rdfs:subClassOf ddhub:BladeShape. 
ddhub:DynamicDrillingSignal a owl:Class; 
                            rdfs:comment ""@EN; 
                            rdfs:subClassOf ddhub:DrillingSignal. 
ddhub:DynamicViscosityDrillingQuantity a owl:Class; 
                                       rdfs:comment """Dynamic viscosity is a measure of a fluid's resistance to shear or flow when a force is applied. It quantifies how thick or thin the fluid is.
The dimension of dynamic viscosity is:
$$[ML^{-1}T^{-1}]$$.
The SI unit for **dynamic viscosity** is: pascal second with the associated unit label $Pa \\cdot s$
The meaningful precision of dynamic viscosity in the drilling context is typically: 0.0001 Pa•s
"""@EN; 
                                       rdfs:subClassOf ddhub:MeasurableQuantity. 
ddhub:DynamicViscosityQuantity a owl:Class; 
                               rdfs:comment """Dynamic viscosity is a measure of a fluid's resistance to shear or flow when a force is applied. It quantifies how thick or thin the fluid is.
The dimension of dynamic viscosity is:
$$[ML^{-1}T^{-1}]$$.
The SI unit for **dynamic viscosity** is: pascal second with the associated unit label $Pa \\cdot s$
"""@EN; 
                               rdfs:subClassOf ddhub:Quantity. 
ddhub:EarthMagneticFluxDensityQuantity a owl:Class; 
                                       rdfs:comment """Magnetic flux density is the measure of the strength of a magnetic field per unit area through which the magnetic flux passes. It indicates how concentrated the magnetic field is.
The dimension of magnetic flux density is:
$$[MI^{-1}T^{-2}]$$.
The SI unit for **magnetic flux density** is: tesla with the associated unit label $T$
Earth's magnetic flux density refers to the strength and direction of the Earth's magnetic field at a specific location.
The meaningful precision of earth magnetic flux density is: 1E-09 T
"""@EN; 
                                       rdfs:subClassOf ddhub:MeasurableQuantity. 
ddhub:ElasticModulusQuantity a owl:Class; 
                             rdfs:comment """Pressure is the force applied per unit area on a surface.
The dimension of pressure is:
$$[ML^{-1}T^{-2}]$$.
The SI unit for **pressure** is: pascal with the associated unit label $Pa$
Elastic modulus is a measure of a material's ability to resist deformation under stress. It quantifies the ratio of stress to strain in the material's elastic region
The meaningful precision of an elastic modulus is typically: 10000 Pa
"""@EN; 
                             rdfs:subClassOf ddhub:MeasurableQuantity. 
ddhub:ElectricalControlSystem a owl:Class; 
                              rdfs:comment ""@EN; 
                              rdfs:subClassOf ddhub:PowerGenerationSystem. 
ddhub:ElectricCapacitanceQuantity a owl:Class; 
                                  rdfs:comment """lectric capacitance is the ability of a capacitor or a component to store electrical charge per unit voltage applied across it.
The dimension of electric capacitance is:
$$[T^{4}I^{2}M^{-1}L^{-2}]$$.
The SI unit for **electric capacitance** is: farad with the associated unit label $F$
"""@EN; 
                                  rdfs:subClassOf ddhub:Quantity. 
ddhub:ElectricCurrentQuantity a owl:Class; 
                              rdfs:comment """Electric current is the flow of electric charge through a conductor or circuit.
The dimension of electric current is:
$$[I]$$.
The SI unit for **electric current** is: ampere with the associated unit label $A$
"""@EN; 
                              rdfs:subClassOf ddhub:Quantity. 
ddhub:ElectricResistivityQuantity a owl:Class; 
                                  rdfs:comment """Electric resistivity is a material's inherent property that measures how strongly it resists the flow of electric current.
The dimension of resistivity is:
$$[L^{3}MI^{-2}T^{-3}]$$.
The SI unit for **electric resistivity** is: ohm metre with the associated unit label $\\Omega \\cdot m$
"""@EN; 
                                  rdfs:subClassOf ddhub:Quantity. 
ddhub:ElectricTensionQuantity a owl:Class; 
                              rdfs:comment """Electric tension is the difference in electric potential between two points.In a static electric field, it corresponds to the work needed per unit of charge to move a positive test charge from the first point to the second point.
The dimension of electric tension is:
$$[L^{2}MI^{-1}T^{-3}]$$.
The SI unit for **electric tension** is: volt with the associated unit label $V$
"""@EN; 
                              rdfs:subClassOf ddhub:MeasurableQuantity. 
ddhub:Electromagnetic a owl:Class; 
                      rdfs:comment ""@EN; 
                      rdfs:subClassOf ddhub:EquipmentTelemetry. 
ddhub:ElectromagneticTelemetry a owl:Class; 
                               rdfs:comment """A method that allows transfer of downhole data to the surface via electromagnetic waves sent trough the drilling formation.
"""@EN; 
                               rdfs:subClassOf ddhub:DownHoleTelemetry. 
ddhub:ElevatorBailsLinks a owl:Class; 
                         rdfs:comment ""@EN; 
                         rdfs:subClassOf ddhub:DrillFloorEquipment. 
ddhub:ElongationGradientPerLengthDrillingQuantity a owl:Class; 
                                                  rdfs:comment """An elongation gradient per length is the first derivative of an elongation compared to a distance: $\\frac{d\\epsilon}{ds}$, where $\\epsilon$ is an elongation and $s$ is a distance.
It is dimensionless.
The SI unit for **elongation gradient per length** is: metre per metre with the associated unit label $\\frac{m}{m}$
The meaningful precision of elongation gradient per length in the drilling context is typically: 1E-05 m/m
"""@EN; 
                                                  rdfs:subClassOf ddhub:MeasurableQuantity. 
ddhub:ElongationGradientPerLengthQuantity a owl:Class; 
                                          rdfs:comment """An elongation gradient per length is the first derivative of an elongation compared to a distance: $\\frac{d\\epsilon}{ds}$, where $\\epsilon$ is an elongation and $s$ is a distance.
It is dimensionless.
The SI unit for **elongation gradient per length** is: metre per metre with the associated unit label $\\frac{m}{m}$
"""@EN; 
                                          rdfs:subClassOf ddhub:Quantity. 
ddhub:EndPointDescription a owl:DatatypeProperty, owl:FunctionalProperty; 
                          rdfs:comment """
"""@EN; 
                          rdfs:domain ddhub:DataEndPoint; 
                          rdfs:range xsd:string. 
ddhub:EndPointMapping a owl:Class; 
                      rdfs:comment ""@EN; 
                      rdfs:subClassOf ddhub:DWISNoun. 
ddhub:EndsHydraulicBranchDecomposition a owl:ObjectProperty; 
                                       rdfs:comment ""@EN; 
                                       rdfs:domain ddhub:HydraulicBranch; 
                                       rdfs:range ddhub:HydraulicBranch; 
                                       rdfs:subPropertyOf ddhub:DWISVerb. 
ddhub:EnergyDensityDrillingQuantity a owl:Class; 
                                    rdfs:comment """Energy density is the amount of energy stored per unit volume or mass of a substance or system.
The dimension of energy density is:
$$[ML^{-1}T^{-2}]$$.
The SI unit for **energy density** is: joule per cubic metre with the associated unit label $\\frac{J}{m^{3}}$
The meaningful precision of energy density in the drilling context is typically: 0.01 J/m³
"""@EN; 
                                    rdfs:subClassOf ddhub:MeasurableQuantity. 
ddhub:EnergyDensityQuantity a owl:Class; 
                            rdfs:comment """Energy density is the amount of energy stored per unit volume or mass of a substance or system.
The dimension of energy density is:
$$[ML^{-1}T^{-2}]$$.
The SI unit for **energy density** is: joule per cubic metre with the associated unit label $\\frac{J}{m^{3}}$
"""@EN; 
                            rdfs:subClassOf ddhub:Quantity. 
ddhub:EnergyQuantity a owl:Class; 
                     rdfs:comment """Energy is the quantitative property that is transferred to a body or to a physical system, recognizable in the performance of work and in the form of heat and light. Energy is a conserved quantity—the law of conservation of energy states that energy can be converted in form, but not created or destroyed; matter and energy may also be converted to one another.
The dimension of energy is:
$$[L^{2}MT^{-2}]$$.
The SI unit for **energy** is: joule with the associated unit label $J$
"""@EN; 
                     rdfs:subClassOf ddhub:Quantity. 
ddhub:EnumerationDataType a owl:Class; 
                          rdfs:comment ""@EN; 
                          rdfs:subClassOf ddhub:DiscreteDataType. 
ddhub:EQ a owl:Class; 
         rdfs:comment ""@EN; 
         rdfs:subClassOf ddhub:ValidityCondition. 
ddhub:Equipment a owl:Class; 
                rdfs:comment ""@EN; 
                rdfs:subClassOf ddhub:DWISNoun. 
ddhub:EquipmentTelemetry a owl:Class; 
                         rdfs:comment ""@EN; 
                         rdfs:subClassOf ddhub:LoggingEquipment. 
ddhub:ExpandableReamers a owl:Class; 
                        rdfs:comment ""@EN; 
                        rdfs:subClassOf ddhub:Reamers. 
ddhub:Expandables a owl:Class; 
                  rdfs:comment ""@EN; 
                  rdfs:subClassOf ddhub:Tubulars. 
ddhub:ExtendFrame a owl:Class; 
                  rdfs:comment ""@EN; 
                  rdfs:subClassOf ddhub:TopDrive. 
ddhub:FDIRFunction a owl:Class; 
                   rdfs:comment """A `FDIRFunction` is a `ProtectionFunction` that reacts to a particular state of the drilling process. FDIR
"""@EN; 
                   rdfs:subClassOf ddhub:ProtectionFunction. 
ddhub:FillPump a owl:Class; 
               rdfs:comment ""@EN; 
               rdfs:subClassOf ddhub:CirculationSystem. 
ddhub:Filter a owl:Class; 
             rdfs:comment ""@EN; 
             rdfs:subClassOf ddhub:SignalProcessingUnit. 
ddhub:FireSafetySystems a owl:Class; 
                        rdfs:comment ""@EN; 
                        rdfs:subClassOf ddhub:SafetyEquipment. 
ddhub:FishingTools a owl:Class; 
                   rdfs:comment ""@EN; 
                   rdfs:subClassOf ddhub:DrillingEquipment. 
ddhub:FixedBlade a owl:Class; 
                 rdfs:comment ""@EN; 
                 rdfs:subClassOf ddhub:HoleOpener. 
ddhub:FixedBladeReamers a owl:Class; 
                        rdfs:comment ""@EN; 
                        rdfs:subClassOf ddhub:Reamers. 
ddhub:FixedCutter a owl:Class; 
                  rdfs:comment ""@EN; 
                  rdfs:subClassOf ddhub:DrillingBit. 
ddhub:FixedIndices a owl:DatatypeProperty, owl:FunctionalProperty; 
                   rdfs:comment """
"""@EN; 
                   rdfs:domain ddhub:EndPointMapping; 
                   rdfs:range <http://www.w3.org/2001/XMLSchema#int[]>. 
ddhub:Flange a owl:Class; 
             rdfs:comment ""@EN; 
             rdfs:subClassOf ddhub:Connection. 
ddhub:FlapperFloatValvesG a owl:Class; 
                          rdfs:comment ""@EN; 
                          rdfs:subClassOf ddhub:FloatValveNonreturnValve. 
ddhub:FloatCollar a owl:Class; 
                  rdfs:comment ""@EN; 
                  rdfs:subClassOf ddhub:CasingEquipment. 
ddhub:FloatShoe a owl:Class; 
                rdfs:comment ""@EN; 
                rdfs:subClassOf ddhub:CasingEquipment. 
ddhub:FloatValveNonreturnValve a owl:Class; 
                               rdfs:comment ""@EN; 
                               rdfs:subClassOf ddhub:WellControlSystem. 
ddhub:FlowAnalysisEquipment a owl:Class; 
                            rdfs:comment ""@EN; 
                            rdfs:subClassOf ddhub:MudLoggingEquipment. 
ddhub:FlowLine a owl:Class; 
               rdfs:comment ""@EN; 
               rdfs:subClassOf ddhub:MudLines. 
ddhub:FlowmeterTools a owl:Class; 
                     rdfs:comment ""@EN; 
                     rdfs:subClassOf ddhub:WirelineLoggingTools. 
ddhub:FlowRateIn a owl:Class; 
                 rdfs:comment ""@EN; 
                 rdfs:subClassOf ddhub:PrototypeData. 
ddhub:FlowRateOut a owl:Class; 
                  rdfs:comment ""@EN; 
                  rdfs:subClassOf ddhub:PrototypeData. 
ddhub:FluidComponent a owl:Class; 
                     rdfs:comment ""@EN; 
                     rdfs:subClassOf ddhub:DWISNoun. 
ddhub:FluidDensityTools a owl:Class; 
                        rdfs:comment ""@EN; 
                        rdfs:subClassOf ddhub:WirelineLoggingTools. 
ddhub:FluidShearRateQuantity a owl:Class; 
                             rdfs:comment """Frequency is the number of occurrences of a repeating event per unit of time.
The dimension of frequency is:
$$[T^{-1}]$$.
The SI unit for **frequency** is: hertz with the associated unit label $Hz$
Shear rate in a fluid is the rate at which adjacent layers of the fluid move relative to each other, typically expressed as the change in velocity per unit distance between the layers. It measures how quickly the fluid is being deformed by shear stress.
The meaningful precision of a shear rate for a fluid is typically: 0.01 Hz
"""@EN; 
                             rdfs:subClassOf ddhub:MeasurableQuantity. 
ddhub:FluidShearStressQuantity a owl:Class; 
                               rdfs:comment """Pressure is the force applied per unit area on a surface.
The dimension of pressure is:
$$[ML^{-1}T^{-2}]$$.
The SI unit for **pressure** is: pascal with the associated unit label $Pa$
Shear stress in a fluid is the force per unit area exerted parallel to the fluid's surface, causing layers of the fluid to slide relative to each other. It measures the fluid's resistance to this shearing action.
The meaningful precision of a shear stress for a fluid is typically: 0.0001 Pa
"""@EN; 
                               rdfs:subClassOf ddhub:MeasurableQuantity. 
ddhub:FluidVelocityDrillingQuantity a owl:Class; 
                                    rdfs:comment """A velocity is the time derivative of a position or a displacement: $\\frac{dx}{dt}$, where $x$ is a position and $t$ is time.
The dimension of velocity is:
$$[LT^{-1}]$$.
The SI unit for **velocity** is: metre per second with the associated unit label $\\frac{m}{s}$
The meaningful precision of fluid velocity in the drilling context is typically: 0.01 m/s
"""@EN; 
                                    rdfs:subClassOf ddhub:MeasurableQuantity. 
ddhub:ForceDrillingQuantity a owl:Class; 
                            rdfs:comment """A force is an influence that can cause an object to change its velocity unless counterbalanced by other forces.
The dimension of force is:
$$[LMT^{-2}]$$.
The SI unit for **force** is: newton with the associated unit label $N$
The meaningful precision of force in the drilling context is typically: 0.1 N
"""@EN; 
                            rdfs:subClassOf ddhub:MeasurableQuantity. 
ddhub:ForceFromLoadPinsTransformation a owl:Class; 
                                      rdfs:comment ""@EN; 
                                      rdfs:subClassOf ddhub:DirectTransformation. 
ddhub:ForceGradientPerLengthDrillingQuantity a owl:Class; 
                                             rdfs:comment """A force gradient per length is the first derivative compared to a distance of a force: $\\frac{dF}{ds}$ where $F$ is a force and $s$ is a distance.
The dimension of force gradient per length is:
$$[MT^{-2}]$$.
The SI unit for **force gradient per length** is: newton per metre with the associated unit label $\\frac{N}{m}$
The meaningful precision of force gradient per length in the drilling context is typically: 1 N/m
"""@EN; 
                                             rdfs:subClassOf ddhub:MeasurableQuantity. 
ddhub:ForceGradientPerLengthQuantity a owl:Class; 
                                     rdfs:comment """A force gradient per length is the first derivative compared to a distance of a force: $\\frac{dF}{ds}$ where $F$ is a force and $s$ is a distance.
The dimension of force gradient per length is:
$$[MT^{-2}]$$.
The SI unit for **force gradient per length** is: newton per metre with the associated unit label $\\frac{N}{m}$
"""@EN; 
                                     rdfs:subClassOf ddhub:Quantity. 
ddhub:ForceQuantity a owl:Class; 
                    rdfs:comment """A force is an influence that can cause an object to change its velocity unless counterbalanced by other forces.
The dimension of force is:
$$[LMT^{-2}]$$.
The SI unit for **force** is: newton with the associated unit label $N$
"""@EN; 
                    rdfs:subClassOf ddhub:Quantity. 
ddhub:ForceToLoadTransformation a owl:Class; 
                                rdfs:comment ""@EN; 
                                rdfs:subClassOf ddhub:DirectTransformation. 
ddhub:FormationCollapseLocation a owl:Class; 
                                rdfs:comment ""@EN; 
                                rdfs:subClassOf ddhub:AbscissaReferenceLocation. 
ddhub:FormationFluidTransferLocation a owl:Class; 
                                     rdfs:comment ""@EN; 
                                     rdfs:subClassOf ddhub:AbscissaReferenceLocation. 
ddhub:FormationGasComponent a owl:Class; 
                            rdfs:comment ""@EN; 
                            rdfs:subClassOf ddhub:GasComponent. 
ddhub:FormationLiquidComponent a owl:Class; 
                               rdfs:comment ""@EN; 
                               rdfs:subClassOf ddhub:LiquidComponent. 
ddhub:FormationResistivityDrillingQuantity a owl:Class; 
                                           rdfs:comment """Electric resistivity is a material's inherent property that measures how strongly it resists the flow of electric current.
The dimension of resistivity is:
$$[L^{3}MI^{-2}T^{-3}]$$.
The SI unit for **electric resistivity** is: ohm metre with the associated unit label $\\Omega \\cdot m$
The meaningful precision of formation electric resistivity in the drilling context is typically: 0.01 Ω•m
"""@EN; 
                                           rdfs:subClassOf ddhub:MeasurableQuantity. 
ddhub:FormationSolidComponent a owl:Class; 
                              rdfs:comment ""@EN; 
                              rdfs:subClassOf ddhub:SolidComponent. 
ddhub:FormationStrengthDrillingQuantity a owl:Class; 
                                        rdfs:comment """Material strength refers to the ability of a material to withstand an applied force or load without failing or deforming. It measures how much stress a material can endure before it breaks, bends, or permanently deforms, often categorized into types like tensile, compressive, and shear strength.
The dimension of material strength is:
$$[ML^{-1}T^{-2}]$$.
The SI unit for **material strength** is: pascal with the associated unit label $Pa$
The meaningful precision of formation strength in the drilling context is typically: 10000 Pa
"""@EN; 
                                        rdfs:subClassOf ddhub:MeasurableQuantity. 
ddhub:FormationTestingAndSampling a owl:Class; 
                                  rdfs:comment ""@EN; 
                                  rdfs:subClassOf ddhub:WirelineLoggingTools. 
ddhub:FormationTestTools a owl:Class; 
                         rdfs:comment ""@EN; 
                         rdfs:subClassOf ddhub:LoggingWhileDrillingTools. 
ddhub:FormationWashout a owl:Class; 
                       rdfs:comment ""@EN; 
                       rdfs:subClassOf ddhub:DrillingIncident. 
ddhub:FormationWashoutLocation a owl:Class; 
                               rdfs:comment ""@EN; 
                               rdfs:subClassOf ddhub:AbscissaReferenceLocation. 
ddhub:ForwardWhirl a owl:Class; 
                   rdfs:comment ""@EN; 
                   rdfs:subClassOf ddhub:Whirling. 
ddhub:FourDimensionalReferenceFrame a owl:Class; 
                                    rdfs:comment ""@EN; 
                                    rdfs:subClassOf ddhub:ReferenceFrame. 
ddhub:FracturingPressure a owl:Class; 
                         rdfs:comment ""@EN; 
                         rdfs:subClassOf ddhub:PrototypeData. 
ddhub:FracturingPressureGradient a owl:Class; 
                                 rdfs:comment ""@EN; 
                                 rdfs:subClassOf ddhub:PrototypeData. 
ddhub:FrenetSerretReferenceFrame a owl:Class; 
                                 rdfs:comment ""@EN; 
                                 rdfs:subClassOf ddhub:ThreeDimensionalReferenceFrame. 
ddhub:FrequencyQuantity a owl:Class; 
                        rdfs:comment """Frequency is the number of occurrences of a repeating event per unit of time.
The dimension of frequency is:
$$[T^{-1}]$$.
The SI unit for **frequency** is: hertz with the associated unit label $Hz$
"""@EN; 
                        rdfs:subClassOf ddhub:Quantity. 
ddhub:FrequencyRateOfChangeQuantity a owl:Class; 
                                    rdfs:comment """A frequency rate of change is the time derivative of a frequency: $\\frac{df}{dt}$, where $f$ is a frequency and $t$ is time.
The dimension of frequency rate of change is:
$$[T^{-2}]$$.
The SI unit for **frequency rate of change** is: hertz per second with the associated unit label $\\frac{Hz}{s}$
"""@EN; 
                                    rdfs:subClassOf ddhub:Quantity. 
ddhub:FullScale a owl:DatatypeProperty, owl:FunctionalProperty; 
                rdfs:comment """The total range of measurement of the signal, i.e., $\\left| max - min \\right|$. The value is expected to be in the same physical quantity as the sensor value.
"""@EN; 
                rdfs:domain ddhub:FullScaleUncertainty; 
                rdfs:range xsd:double. 
ddhub:FullScaleUncertainty a owl:Class; 
                           rdfs:comment """The uncertainty on the signal is described as a Gaussian distribution with a standard deviation that is calculated using a proportion of the maximum range of the signal. The `Fullscale` or `ProportionError` can either be defined as attribute values, for example when they have fixed values, or using facts utilizing the verbs `HasFullScale` or repectively `HasProportionError` when these values may change through time.
"""@EN; 
                           rdfs:subClassOf ddhub:GaussianUncertainty. 
ddhub:GammaRayIndexDrillingQuantity a owl:Class; 
                                    rdfs:comment """The Gamma Ray API is a unit used in the petroleum industry to measure the natural gamma radiation of formations. Specifically, the Gamma Ray Index (GRI) is used in well logging to measure the gamma ray activity of the rock surrounding the borehole.
Gamma rays are a form of electromagnetic radiation, and in well logging, they are used to assess the radioactive content of the formations, which helps in identifying rock types (shales, sandstones, etc.).
Since the Gamma Ray API is a measure of gamma radiation intensity, let's break down its physical nature:
"""@EN; 
                                    rdfs:subClassOf ddhub:MeasurableQuantity. 
ddhub:GasAnalysisEquipment a owl:Class; 
                           rdfs:comment ""@EN; 
                           rdfs:subClassOf ddhub:MudLoggingEquipment. 
ddhub:GasComponent a owl:Class; 
                   rdfs:comment ""@EN; 
                   rdfs:subClassOf ddhub:FluidComponent. 
ddhub:GasFlowRate a owl:Class; 
                  rdfs:comment ""@EN; 
                  rdfs:subClassOf ddhub:PrototypeData. 
ddhub:GasSafetySystems a owl:Class; 
                       rdfs:comment ""@EN; 
                       rdfs:subClassOf ddhub:SafetyEquipment. 
ddhub:GasShowDrillingQuantity a owl:Class; 
                              rdfs:comment """A proportion is the ratio of two quantities with the same dimension. It represents how one quantity compares to another in relative terms.
A proportion is dimensionless:
The meaningful precision of gas show in the drilling context is typically: 1E-07 
"""@EN; 
                              rdfs:subClassOf ddhub:MeasurableQuantity. 
ddhub:GasVolumetricFlowRateDrillingQuantity a owl:Class; 
                                            rdfs:comment """A volumetric flowrate is the volume of fluid that passes per unit time: $\\frac{dV}{dt}$, where $V$ is a volume and $t$ is time.
The dimension of volumetric flowrate is:
$$[L^{3}T^{-1}]$$.
The SI unit for **volumetric flow rate** is: cubic metre per second with the associated unit label $\\frac{m^{3}}{s}$
The meaningful precision of gas volumetric flowrate in the drilling context is typically: 0.01 m³/s
"""@EN; 
                                            rdfs:subClassOf ddhub:MeasurableQuantity. 
ddhub:GaugePressureReference a owl:Class; 
                             rdfs:comment ""@EN; 
                             rdfs:subClassOf ddhub:RelativePressureReference. 
ddhub:GaussianUncertainty a owl:Class; 
                          rdfs:comment """The uncertainty is represented by a Gaussian distribution, i.e., with a `Mean` and a `StandardDeviation`, $\\mathcal{N}(\\overline{x},{\\sigma_{x}}^2)$ where $\\overline{x}$ is the `Mean` value and $\\sigma_{x}$ is the `StandardDeviation`.
"""@EN; 
                          rdfs:subClassOf ddhub:SignalUncertainty. 
ddhub:GenericEquipment a owl:Class; 
                       rdfs:comment ""@EN; 
                       rdfs:subClassOf ddhub:Equipment. 
ddhub:GenericEquipmentGatevalve a owl:Class; 
                                rdfs:comment ""@EN; 
                                rdfs:subClassOf ddhub:GenericEquipment. 
ddhub:GenericUncertainty a owl:Class; 
                         rdfs:comment """The uncertainty is represented by a `Histogram`.
"""@EN; 
                         rdfs:subClassOf ddhub:SignalUncertainty. 
ddhub:Gooseneck a owl:Class; 
                rdfs:comment ""@EN; 
                rdfs:subClassOf ddhub:MudLines. 
ddhub:GPSReference a owl:Class; 
                   rdfs:comment ""@EN; 
                   rdfs:subClassOf ddhub:TimeReference. 
ddhub:GravitationalLoadQuantity a owl:Class; 
                                rdfs:comment """Mass can be experimentally defined as a measure of the body's inertia, meaning the resistance to acceleration (change of velocity) when a net force is applied. The object's mass also determines the strength of its gravitational attraction to other bodies.
The dimension of mass is:
$$[M]$$.
The SI unit for **mass** is: kilogram with the associated unit label $kg$
"""@EN; 
                                rdfs:subClassOf ddhub:Quantity. 
ddhub:GravityHighSideAngleLocation a owl:Class; 
                                   rdfs:comment ""@EN; 
                                   rdfs:subClassOf ddhub:AngleReferenceLocation. 
ddhub:GridNorthAzimuthLocation a owl:Class; 
                               rdfs:comment ""@EN; 
                               rdfs:subClassOf ddhub:AzimuthReferenceLocation. 
ddhub:GroundLevelVerticalLocation a owl:Class; 
                                  rdfs:comment ""@EN; 
                                  rdfs:subClassOf ddhub:VerticalReferenceLocation. 
ddhub:Grouping a owl:Class; 
               rdfs:comment ""@EN; 
               rdfs:subClassOf ddhub:DrillString. 
ddhub:GT a owl:Class; 
         rdfs:comment ""@EN; 
         rdfs:subClassOf ddhub:ValidityCondition. 
ddhub:HammerAssembly a owl:Class; 
                     rdfs:comment ""@EN; 
                     rdfs:subClassOf ddhub:DrillingEquipment. 
ddhub:Hangers a owl:Class; 
              rdfs:comment ""@EN; 
              rdfs:subClassOf ddhub:CasingEquipment. 
ddhub:HasAcquisitionClock a owl:ObjectProperty; 
                          rdfs:comment ""@EN; 
                          rdfs:domain ddhub:DrillingDataPoint; 
                          rdfs:range ddhub:Clock; 
                          rdfs:subPropertyOf ddhub:DWISVerb. 
ddhub:HasAcquisitionTime a owl:ObjectProperty; 
                         rdfs:comment ""@EN; 
                         rdfs:domain ddhub:DrillingDataPoint; 
                         rdfs:range ddhub:DrillingDataPoint; 
                         rdfs:subPropertyOf ddhub:DWISVerb. 
ddhub:HasBranchComponent a owl:ObjectProperty; 
                         rdfs:comment ""@EN; 
                         rdfs:domain ddhub:HydraulicNetwork; 
                         rdfs:range ddhub:HydraulicBranch; 
                         rdfs:subPropertyOf ddhub:DWISVerb. 
ddhub:HasBranchCoordinateSystem a owl:ObjectProperty; 
                                rdfs:comment ""@EN; 
                                rdfs:domain ddhub:HydraulicBranch; 
                                rdfs:range ddhub:ReferenceFrame; 
                                rdfs:subPropertyOf ddhub:DWISVerb. 
ddhub:HasCoordinates a owl:ObjectProperty; 
                     rdfs:comment ""@EN; 
                     rdfs:domain ddhub:Location; 
                     rdfs:range ddhub:DrillingDataPoint; 
                     rdfs:subPropertyOf ddhub:DWISVerb. 
ddhub:HasDomain a owl:ObjectProperty; 
                rdfs:comment ""@EN; 
                rdfs:domain ddhub:DrillingDataPoint; 
                rdfs:range ddhub:DrillingDataPoint; 
                rdfs:subPropertyOf ddhub:DWISVerb. 
ddhub:HasDynamicValue a owl:ObjectProperty; 
                      rdfs:comment ""@EN; 
                      rdfs:domain ddhub:DrillingDataPoint; 
                      rdfs:range ddhub:DynamicDrillingSignal; 
                      rdfs:subPropertyOf ddhub:HasValue. 
ddhub:HasElevationReference a owl:ObjectProperty; 
                            rdfs:comment """This verb is a specialization of `IsDependentOn` and refers to the specific dependence on an elevation reference.
"""@EN; 
                            rdfs:domain ddhub:DrillingDataPoint; 
                            rdfs:range ddhub:Location; 
                            rdfs:subPropertyOf ddhub:IsDependentOn. 
ddhub:HasEndJunction a owl:ObjectProperty; 
                     rdfs:comment ""@EN; 
                     rdfs:domain ddhub:HydraulicBranch; 
                     rdfs:range ddhub:HydraulicJunction; 
                     rdfs:subPropertyOf ddhub:IsHydraulicConnectedTo. 
ddhub:HasEndPoint a owl:ObjectProperty; 
                  rdfs:comment ""@EN; 
                  rdfs:domain ddhub:DrillingSignal; 
                  rdfs:range ddhub:DataEndPoint; 
                  rdfs:subPropertyOf ddhub:DWISVerb. 
ddhub:HasFullScale a owl:ObjectProperty; 
                   rdfs:comment """This verb is used to associate a `DrillingDataPoint` as the `FullScale` value of a `FullScaleUncertainty`
"""@EN; 
                   rdfs:domain ddhub:FullScaleUncertainty; 
                   rdfs:range ddhub:DrillingDataPoint; 
                   rdfs:subPropertyOf ddhub:DWISVerb. 
ddhub:HasFunction a owl:DatatypeProperty, owl:FunctionalProperty, owl:ObjectProperty; 
                  rdfs:comment """this attribute describes the purpose of the activable function.
"""@EN, ""@EN; 
                  rdfs:domain ddhub:ActivableFunction, ddhub:DrillingDataPoint; 
                  rdfs:range xsd:string, ddhub:DataFlowNode; 
                  rdfs:subPropertyOf ddhub:DWISVerb. 
ddhub:HasHydraulicState a owl:ObjectProperty; 
                        rdfs:comment ""@EN; 
                        rdfs:domain ddhub:HydraulicJunction; 
                        rdfs:range ddhub:HydraulicElementState; 
                        rdfs:subPropertyOf ddhub:DWISVerb. 
ddhub:HasHydraulicStateValueFrom a owl:ObjectProperty; 
                                 rdfs:comment ""@EN; 
                                 rdfs:domain ddhub:DWISNoun; 
                                 rdfs:range ddhub:DWISNoun; 
                                 rdfs:subPropertyOf ddhub:DWISVerb. 
ddhub:HasLeftBranch a owl:ObjectProperty; 
                    rdfs:comment ""@EN; 
                    rdfs:domain ddhub:HydraulicJunction; 
                    rdfs:range ddhub:HydraulicBranch; 
                    rdfs:subPropertyOf ddhub:IsHydraulicConnectedTo. 
ddhub:HasLeftBranchCoordinates a owl:ObjectProperty; 
                               rdfs:comment ""@EN; 
                               rdfs:domain ddhub:HydraulicJunction; 
                               rdfs:range ddhub:DrillingDataPoint; 
                               rdfs:subPropertyOf ddhub:DWISVerb. 
ddhub:HasMechanicalState a owl:ObjectProperty; 
                         rdfs:comment ""@EN; 
                         rdfs:domain ddhub:MechanicalLogicalElement; 
                         rdfs:range ddhub:MechanicalElementState; 
                         rdfs:subPropertyOf ddhub:DWISVerb. 
ddhub:HasMechanicalStateValueFrom a owl:ObjectProperty; 
                                  rdfs:comment ""@EN; 
                                  rdfs:domain ddhub:MechanicalElementState; 
                                  rdfs:range ddhub:DrillingDataPoint; 
                                  rdfs:subPropertyOf ddhub:DWISVerb. 
ddhub:HasMotionType a owl:ObjectProperty; 
                    rdfs:comment ""@EN; 
                    rdfs:domain ddhub:MechanicalLogicalElement; 
                    rdfs:range ddhub:MotionType; 
                    rdfs:subPropertyOf ddhub:DWISVerb. 
ddhub:HasPressureReference a owl:ObjectProperty; 
                           rdfs:comment """This verb is a specialization of `IsDependentOn` and refers to the specific dependence on a pressure reference.
"""@EN; 
                           rdfs:domain ddhub:DrillingDataPoint; 
                           rdfs:range ddhub:DrillingDataPoint; 
                           rdfs:subPropertyOf ddhub:IsDependentOn. 
ddhub:HasPressureReferenceType a owl:ObjectProperty; 
                               rdfs:comment ""@EN; 
                               rdfs:domain ddhub:DrillingDataPoint; 
                               rdfs:range ddhub:PressureReference; 
                               rdfs:subPropertyOf ddhub:DWISVerb. 
ddhub:HasProportionError a owl:ObjectProperty; 
                         rdfs:comment """This verb is used to associate a `DrillingDataPoint` as the `ProportionError` value of a `FullScaleUncertainty`
"""@EN; 
                         rdfs:domain ddhub:FullScaleUncertainty; 
                         rdfs:range ddhub:DrillingDataPoint; 
                         rdfs:subPropertyOf ddhub:DWISVerb. 
ddhub:HasReferenceFrame a owl:ObjectProperty; 
                        rdfs:comment ""@EN; 
                        rdfs:domain ddhub:DrillingDataPoint; 
                        rdfs:range ddhub:ReferenceFrame; 
                        rdfs:subPropertyOf ddhub:DWISVerb. 
ddhub:HasReferenceFrameOrigin a owl:ObjectProperty; 
                              rdfs:comment ""@EN; 
                              rdfs:domain ddhub:ReferenceFrame; 
                              rdfs:range ddhub:Location; 
                              rdfs:subPropertyOf ddhub:DWISVerb. 
ddhub:HasRightBranch a owl:ObjectProperty; 
                     rdfs:comment ""@EN; 
                     rdfs:domain ddhub:HydraulicJunction; 
                     rdfs:range ddhub:HydraulicBranch; 
                     rdfs:subPropertyOf ddhub:IsHydraulicConnectedTo. 
ddhub:HasRightBranchCoordinates a owl:ObjectProperty; 
                                rdfs:comment ""@EN; 
                                rdfs:domain ddhub:HydraulicJunction; 
                                rdfs:range ddhub:DrillingDataPoint; 
                                rdfs:subPropertyOf ddhub:DWISVerb. 
ddhub:HasSIUnit a owl:ObjectProperty; 
                rdfs:comment ""@EN; 
                rdfs:domain ddhub:Quantity; 
                rdfs:range ddhub:Unit; 
                rdfs:subPropertyOf ddhub:DWISVerb. 
ddhub:HasSourceClock a owl:ObjectProperty; 
                     rdfs:comment ""@EN; 
                     rdfs:domain ddhub:DrillingDataPoint; 
                     rdfs:range ddhub:Clock; 
                     rdfs:subPropertyOf ddhub:DWISVerb. 
ddhub:HasSourceTime a owl:ObjectProperty; 
                    rdfs:comment ""@EN; 
                    rdfs:domain ddhub:DrillingDataPoint; 
                    rdfs:range ddhub:DrillingDataPoint; 
                    rdfs:subPropertyOf ddhub:DWISVerb. 
ddhub:HasStartJunction a owl:ObjectProperty; 
                       rdfs:comment ""@EN; 
                       rdfs:domain ddhub:HydraulicBranch; 
                       rdfs:range ddhub:HydraulicJunction; 
                       rdfs:subPropertyOf ddhub:IsHydraulicConnectedTo. 
ddhub:HasStaticValue a owl:ObjectProperty; 
                     rdfs:comment ""@EN; 
                     rdfs:domain ddhub:DrillingDataPoint; 
                     rdfs:range ddhub:DrillingSignal; 
                     rdfs:subPropertyOf ddhub:HasValue. 
ddhub:HasTemperatureReference a owl:ObjectProperty; 
                              rdfs:comment """This verb is a specialization of `IsDependentOn` and refers to the specific dependence on a temperature reference.
"""@EN; 
                              rdfs:domain ddhub:DrillingDataPoint; 
                              rdfs:range ddhub:DrillingDataPoint; 
                              rdfs:subPropertyOf ddhub:IsDependentOn. 
ddhub:HasTimeIntervalDomain a owl:ObjectProperty; 
                            rdfs:comment ""@EN; 
                            rdfs:domain ddhub:DrillingDataPoint; 
                            rdfs:range ddhub:DrillingDataPoint; 
                            rdfs:subPropertyOf ddhub:HasDomain. 
ddhub:HasTimeReference a owl:ObjectProperty; 
                       rdfs:comment ""@EN; 
                       rdfs:domain ddhub:DrillingDataPoint; 
                       rdfs:range ddhub:TimeReference; 
                       rdfs:subPropertyOf ddhub:DWISVerb. 
ddhub:HasTransmissionDelay a owl:ObjectProperty; 
                           rdfs:comment ""@EN; 
                           rdfs:domain ddhub:DrillingDataPoint; 
                           rdfs:range ddhub:DrillingDataPoint; 
                           rdfs:subPropertyOf ddhub:DWISVerb. 
ddhub:HasUncertainty a owl:ObjectProperty; 
                     rdfs:comment """This verb allows to associate a `SignalUncertainty` to a `DrillingDataPoint`.
"""@EN; 
                     rdfs:domain ddhub:DrillingDataPoint; 
                     rdfs:range ddhub:SignalUncertainty; 
                     rdfs:subPropertyOf ddhub:DWISVerb. 
ddhub:HasUncertaintyAccuracy a owl:ObjectProperty; 
                             rdfs:comment """This verb allows to associate a `DrillingDataPoint` as the `Accuracy` of a `SensorUncertainty`
"""@EN; 
                             rdfs:domain ddhub:SensorUncertainty; 
                             rdfs:range ddhub:DrillingDataPoint; 
                             rdfs:subPropertyOf ddhub:DWISVerb. 
ddhub:HasUncertaintyHistogram a owl:ObjectProperty; 
                              rdfs:comment """This verb is used to associated a `DrillingDataPoint` as the `Histogram` value of a `GenericUncertainty`
"""@EN; 
                              rdfs:domain ddhub:GenericUncertainty; 
                              rdfs:range ddhub:DrillingDataPoint; 
                              rdfs:subPropertyOf ddhub:DWISVerb. 
ddhub:HasUncertaintyMax a owl:ObjectProperty; 
                        rdfs:comment """This verb is used to associate a `DrillingDataPoint` as the `Max` value of a `MinMaxUncertainty`
"""@EN; 
                        rdfs:domain ddhub:MinMaxUncertainty; 
                        rdfs:range ddhub:DrillingDataPoint; 
                        rdfs:subPropertyOf ddhub:DWISVerb. 
ddhub:HasUncertaintyMean a owl:ObjectProperty; 
                         rdfs:comment """This verb is used to associate a `DrillingDataPoint` as the `Mean` value of a `GaussianUncertainty`
"""@EN; 
                         rdfs:domain ddhub:GaussianUncertainty; 
                         rdfs:range ddhub:DrillingDataPoint; 
                         rdfs:subPropertyOf ddhub:DWISVerb. 
ddhub:HasUncertaintyMin a owl:ObjectProperty; 
                        rdfs:comment """This verb is used to associate a `DrillingDataPoint` as the `Min` value of `MinMaxUncertainty`
"""@EN; 
                        rdfs:domain ddhub:MinMaxUncertainty; 
                        rdfs:range ddhub:DrillingDataPoint; 
                        rdfs:subPropertyOf ddhub:DWISVerb. 
ddhub:HasUncertaintyPrecision a owl:ObjectProperty; 
                              rdfs:comment """This verb is used to associate a `DrillingDataPoint` as the `Precision` of a `SensorUncertainty`
"""@EN; 
                              rdfs:domain ddhub:SensorUncertainty; 
                              rdfs:range ddhub:DrillingDataPoint; 
                              rdfs:subPropertyOf ddhub:DWISVerb. 
ddhub:HasUncertaintyStandardDeviation a owl:ObjectProperty; 
                                      rdfs:comment """This verb is used to associate a `DrillingDataPoint` as the `StandardDeviation` value of a `GaussianUncertainty`
"""@EN; 
                                      rdfs:domain ddhub:GaussianUncertainty; 
                                      rdfs:range ddhub:DrillingDataPoint; 
                                      rdfs:subPropertyOf ddhub:DWISVerb. 
ddhub:HasUnitAssociation a owl:ObjectProperty; 
                         rdfs:comment ""@EN; 
                         rdfs:domain ddhub:UnitSystem; 
                         rdfs:range ddhub:MeasurableQuantityUnitAssociation; 
                         rdfs:subPropertyOf ddhub:DWISVerb. 
ddhub:HasUnitOfMeasure a owl:ObjectProperty; 
                       rdfs:comment ""@EN; 
                       rdfs:domain ddhub:DrillingSignal; 
                       rdfs:range ddhub:Unit; 
                       rdfs:subPropertyOf ddhub:DWISVerb. 
ddhub:HasValue a owl:ObjectProperty; 
               rdfs:comment ""@EN; 
               rdfs:domain ddhub:DrillingDataPoint; 
               rdfs:range ddhub:DrillingSignal; 
               rdfs:subPropertyOf ddhub:DWISVerb. 
ddhub:HeatTransferCoefficientDrillingQuantity a owl:Class; 
                                              rdfs:comment """Heat transfer coefficient is a measure of the efficiency with which heat is transferred between a solid surface and a fluid (or between two fluids) per unit area and temperature difference.
The dimension of heat transfer coefficient is:
$$[MK^{-1}T^{-3}]$$.
The SI unit for **heat transfer coefficient** is: watt per square metre per kelvin with the associated unit label $\\frac{W}{m^{2} \\cdot K}$
The meaningful precision of heat transfer coefficient in the drilling context is typically: 0.0001 W/m²/K
"""@EN; 
                                              rdfs:subClassOf ddhub:MeasurableQuantity. 
ddhub:HeatTransferCoefficientQuantity a owl:Class; 
                                      rdfs:comment """Heat transfer coefficient is a measure of the efficiency with which heat is transferred between a solid surface and a fluid (or between two fluids) per unit area and temperature difference.
The dimension of heat transfer coefficient is:
$$[MK^{-1}T^{-3}]$$.
The SI unit for **heat transfer coefficient** is: watt per square metre per kelvin with the associated unit label $\\frac{W}{m^{2} \\cdot K}$
"""@EN; 
                                      rdfs:subClassOf ddhub:Quantity. 
ddhub:HeaveCompensationSystem a owl:Class; 
                              rdfs:comment ""@EN; 
                              rdfs:subClassOf ddhub:MarineSystem. 
ddhub:Heavyweight a owl:Class; 
                  rdfs:comment ""@EN; 
                  rdfs:subClassOf ddhub:DrillString. 
ddhub:HeightDrillingQuantity a owl:Class; 
                             rdfs:comment """Length is a measure of distance.
The dimension of length is:
$$[L]$$.
The SI unit for **length** is: metre with the associated unit label $m$
The meaningful precision of height in the drilling context is typically: 0.001 m
"""@EN; 
                             rdfs:subClassOf ddhub:MeasurableQuantity. 
ddhub:HFTO a owl:Class; 
           rdfs:comment ""@EN; 
           rdfs:subClassOf ddhub:AbnormalTorsionalOscillation. 
ddhub:HighGravitySolidComponent a owl:Class; 
                                rdfs:comment ""@EN; 
                                rdfs:subClassOf ddhub:DrillingFluidSolidComponent. 
ddhub:HighPassFilter a owl:Class; 
                     rdfs:comment ""@EN; 
                     rdfs:subClassOf ddhub:Filter. 
ddhub:HighPressureRiser a owl:Class; 
                        rdfs:comment ""@EN; 
                        rdfs:subClassOf ddhub:SurfaceRiser. 
ddhub:HoistingSystem a owl:Class; 
                     rdfs:comment ""@EN; 
                     rdfs:subClassOf ddhub:RigEquipment. 
ddhub:HoleBottomLocation a owl:Class; 
                         rdfs:comment ""@EN; 
                         rdfs:subClassOf ddhub:AbscissaReferenceLocation. 
ddhub:HoleCollapse a owl:Class; 
                   rdfs:comment ""@EN; 
                   rdfs:subClassOf ddhub:DrillingIncident. 
ddhub:HoleDepth a owl:Class; 
                rdfs:comment ""@EN; 
                rdfs:subClassOf ddhub:PrototypeData. 
ddhub:HoleOpener a owl:Class; 
                 rdfs:comment ""@EN; 
                 rdfs:subClassOf ddhub:DrillingEquipment. 
ddhub:Hook a owl:Class; 
           rdfs:comment ""@EN; 
           rdfs:subClassOf ddhub:HoistingSystem. 
ddhub:HookLoad a owl:Class; 
               rdfs:comment ""@EN; 
               rdfs:subClassOf ddhub:PrototypeData. 
ddhub:HookLoadDrillingQuantity a owl:Class; 
                               rdfs:comment """Mass can be experimentally defined as a measure of the body's inertia, meaning the resistance to acceleration (change of velocity) when a net force is applied. The object's mass also determines the strength of its gravitational attraction to other bodies.
The dimension of mass is:
$$[M]$$.
The SI unit for **mass** is: kilogram with the associated unit label $kg$
The meaningful precision of hook load in the drilling context is typically: 100 kg
"""@EN; 
                               rdfs:subClassOf ddhub:MeasurableQuantity. 
ddhub:HookPosition a owl:Class; 
                   rdfs:comment ""@EN; 
                   rdfs:subClassOf ddhub:PrototypeData. 
ddhub:HookVelocity a owl:Class; 
                   rdfs:comment ""@EN; 
                   rdfs:subClassOf ddhub:PrototypeData. 
ddhub:HorizontalOndulationModelling a owl:Class; 
                                    rdfs:comment """The model accounts for the change of azimuth of some parts of the physical system.
"""@EN; 
                                    rdfs:subClassOf ddhub:TangentialModelling. 
ddhub:Hybrid a owl:Class; 
             rdfs:comment ""@EN; 
             rdfs:subClassOf ddhub:EquipmentTelemetry. 
ddhub:HybridKymera a owl:Class; 
                   rdfs:comment ""@EN; 
                   rdfs:subClassOf ddhub:DrillingBit. 
ddhub:HydraulicBranch a owl:Class; 
                      rdfs:comment ""@EN; 
                      rdfs:subClassOf ddhub:HydraulicLogicalElement. 
ddhub:HydraulicConductivityDrillingQuantity a owl:Class; 
                                            rdfs:comment """A velocity is the time derivative of a position or a displacement: $\\frac{dx}{dt}$, where $x$ is a position and $t$ is time.
The dimension of velocity is:
$$[LT^{-1}]$$.
The SI unit for **velocity** is: metre per second with the associated unit label $\\frac{m}{s}$
The meaningful precision of hydraulic conductivity in the drilling context is typically: 0.001 m/s
"""@EN; 
                                            rdfs:subClassOf ddhub:MeasurableQuantity. 
ddhub:HydraulicConductivityQuantity a owl:Class; 
                                    rdfs:comment """A velocity is the time derivative of a position or a displacement: $\\frac{dx}{dt}$, where $x$ is a position and $t$ is time.
The dimension of velocity is:
$$[LT^{-1}]$$.
The SI unit for **velocity** is: metre per second with the associated unit label $\\frac{m}{s}$
"""@EN; 
                                    rdfs:subClassOf ddhub:Quantity. 
ddhub:HydraulicConnectedState a owl:Class; 
                              rdfs:comment ""@EN; 
                              rdfs:subClassOf ddhub:HydraulicElementState. 
ddhub:HydraulicElementState a owl:Class; 
                            rdfs:comment ""@EN; 
                            rdfs:subClassOf ddhub:DWISNoun. 
ddhub:HydraulicJar a owl:Class; 
                   rdfs:comment ""@EN; 
                   rdfs:subClassOf ddhub:JarringAssembly. 
ddhub:HydraulicJunction a owl:Class; 
                        rdfs:comment ""@EN; 
                        rdfs:subClassOf ddhub:HydraulicLogicalElement. 
ddhub:HydraulicLogicalElement a owl:Class; 
                              rdfs:comment ""@EN; 
                              rdfs:subClassOf ddhub:DWISNoun. 
ddhub:HydraulicMudPump a owl:Class; 
                       rdfs:comment ""@EN; 
                       rdfs:subClassOf ddhub:MudPump. 
ddhub:HydraulicNetwork a owl:Class; 
                       rdfs:comment ""@EN; 
                       rdfs:subClassOf ddhub:HydraulicLogicalElement. 
ddhub:Hydrocyclones a owl:Class; 
                    rdfs:comment ""@EN; 
                    rdfs:subClassOf ddhub:CirculationSystem. 
ddhub:HydromechanicalJar a owl:Class; 
                         rdfs:comment ""@EN; 
                         rdfs:subClassOf ddhub:JarringAssembly. 
ddhub:I a owl:DatatypeProperty, owl:FunctionalProperty; 
        rdfs:comment """Electric current exponent.
SI Unit: Ampere (A)
"""@EN; 
        rdfs:domain ddhub:Quantity; 
        rdfs:range xsd:double. 
ddhub:Ibop a owl:Class; 
           rdfs:comment ""@EN; 
           rdfs:subClassOf ddhub:WellControlSystem. 
ddhub:ImageScaleQuantity a owl:Class; 
                         rdfs:comment """Image scale refers to the resolution or level of detail in an image.
The dimension of image scale is:
$$[L^{-1}]$$.
The SI unit for **image scale** is: dot per metre with the associated unit label $dpm$
"""@EN; 
                         rdfs:subClassOf ddhub:MeasurableQuantity. 
ddhub:ImagingTools a owl:Class; 
                   rdfs:comment ""@EN; 
                   rdfs:subClassOf ddhub:LoggingWhileDrillingTools. 
ddhub:Inclination a owl:Class; 
                  rdfs:comment ""@EN; 
                  rdfs:subClassOf ddhub:PrototypeData. 
ddhub:Influx a owl:Class; 
             rdfs:comment ""@EN; 
             rdfs:subClassOf ddhub:DrillingIncident. 
ddhub:InjectorHead a owl:Class; 
                   rdfs:comment ""@EN; 
                   rdfs:subClassOf ddhub:CoiledTubingEquipment. 
ddhub:InnerBarrel a owl:Class; 
                  rdfs:comment ""@EN; 
                  rdfs:subClassOf ddhub:CoringTool. 
ddhub:InnerString a owl:Class; 
                  rdfs:comment ""@EN; 
                  rdfs:subClassOf ddhub:CasingEquipment. 
ddhub:InsertTci a owl:Class; 
                rdfs:comment ""@EN; 
                rdfs:subClassOf ddhub:RollingCutter. 
ddhub:InstrumentedMotor a owl:Class; 
                        rdfs:comment ""@EN; 
                        rdfs:subClassOf ddhub:DownholeMotor. 
ddhub:Integral a owl:Class; 
               rdfs:comment ""@EN; 
               rdfs:subClassOf ddhub:BladeType. 
ddhub:Integration a owl:Class; 
                  rdfs:comment ""@EN; 
                  rdfs:subClassOf ddhub:TimeBasedTransformation. 
ddhub:InterfacialTensionDrillingQuantity a owl:Class; 
                                         rdfs:comment """Interfacial tension is the force per unit length acting along the boundary between two immiscible liquids, resisting their mixing.
The dimension of interfacial tension is:
$$[MT^{-2}]$$.
The SI unit for **interfacial tension** is: newton per metre with the associated unit label $\\frac{N}{m}$
The meaningful precision of interfacial tension in the drilling context is typically: 0.0001 N/m
"""@EN; 
                                         rdfs:subClassOf ddhub:MeasurableQuantity. 
ddhub:InterfacialTensionQuantity a owl:Class; 
                                 rdfs:comment """Interfacial tension is the force per unit length acting along the boundary between two immiscible liquids, resisting their mixing.
The dimension of interfacial tension is:
$$[MT^{-2}]$$.
The SI unit for **interfacial tension** is: newton per metre with the associated unit label $\\frac{N}{m}$
"""@EN; 
                                 rdfs:subClassOf ddhub:Quantity. 
ddhub:IronRoughneck a owl:Class; 
                    rdfs:comment ""@EN; 
                    rdfs:subClassOf ddhub:DrillFloorEquipment. 
ddhub:IsActivatedSignalFor a owl:ObjectProperty; 
                           rdfs:comment """This verb is used to define a `DrillingDataPoint` that indicates if the `ActivableFunction` is activated or
not. It is expected that the `DrillingDataPoint` is a Boolean value.
"""@EN; 
                           rdfs:domain ddhub:DrillingDataPoint; 
                           rdfs:range ddhub:ActivableFunction; 
                           rdfs:subPropertyOf ddhub:DWISVerb. 
ddhub:IsAHydraulicRepresentationFor a owl:ObjectProperty; 
                                    rdfs:comment ""@EN; 
                                    rdfs:domain ddhub:HydraulicLogicalElement; 
                                    rdfs:range ddhub:DrillingEquipment; 
                                    rdfs:subPropertyOf ddhub:DWISVerb. 
ddhub:IsAMechanicalRepresentationFor a owl:ObjectProperty; 
                                     rdfs:comment ""@EN; 
                                     rdfs:domain ddhub:MechanicalLogicalElement; 
                                     rdfs:range ddhub:DrillingEquipment; 
                                     rdfs:subPropertyOf ddhub:DWISVerb. 
ddhub:IsArmedSignalFor a owl:ObjectProperty; 
                       rdfs:comment """This verb is used to indicate a `DrillingDataPoint` used by an `FDIRFunction` tells if the FDIR function is armed and operative.
The signal is supposed to be a Boolean value.
The FDIR function may be active, but the current state of the drilling process may imply that the function cannot be
triggered. For instance, a pack-off FDIR may be active but would react only if the flow is supposed to be steady state.
"""@EN; 
                       rdfs:domain ddhub:DrillingDataPoint; 
                       rdfs:range ddhub:FDIRFunction; 
                       rdfs:subPropertyOf ddhub:DWISVerb. 
ddhub:IsAuxiliary a owl:DatatypeProperty, owl:FunctionalProperty; 
                  rdfs:comment """This attribute specifies if the function is a main or an auxilary one. A main function impacts
substantially the drilling process while an auxiliary function does not impact or only in limited fashion the
drilling process. Example of a main functions are: Hoist, Tag Bottom, Start Circulation, Start Rotation,
Stop Circulation, Stop Rotation, Drill, Pull Out,Run In, Pull Out With Lubrication, Run In With Lubrication, Ream Up,
Ream Down,Test Friction, Reciprocate, Test Pressure Integrity, Place Cement, .... Example of auxiliary functions
are: Boost Riser Flow, Down Link from ADCS, Rock Pipe, ...
"""@EN; 
                  rdfs:domain ddhub:RunnableFunction; 
                  rdfs:range xsd:boolean. 
ddhub:IsBufferingInput a owl:ObjectProperty; 
                       rdfs:comment ""@EN; 
                       rdfs:domain ddhub:DrillingDataPoint; 
                       rdfs:range ddhub:Buffering; 
                       rdfs:subPropertyOf ddhub:IsTransformationInput. 
ddhub:IsBufferingOutput a owl:ObjectProperty; 
                        rdfs:comment ""@EN; 
                        rdfs:domain ddhub:DrillingDataPoint; 
                        rdfs:range ddhub:Buffering; 
                        rdfs:subPropertyOf ddhub:IsTransformationOutput. 
ddhub:IsCommandFor a owl:ObjectProperty; 
                   rdfs:comment ""@EN; 
                   rdfs:domain ddhub:DrillingDataPoint; 
                   rdfs:range ddhub:DWISNoun; 
                   rdfs:subPropertyOf ddhub:HasFunction. 
ddhub:IsComputationInput a owl:ObjectProperty; 
                         rdfs:comment ""@EN; 
                         rdfs:domain ddhub:DrillingDataPoint; 
                         rdfs:range ddhub:ComputationUnit; 
                         rdfs:subPropertyOf ddhub:HasFunction. 
ddhub:IsComputedBy a owl:ObjectProperty; 
                   rdfs:comment ""@EN; 
                   rdfs:domain ddhub:DWISNoun; 
                   rdfs:range ddhub:DWISNoun; 
                   rdfs:subPropertyOf ddhub:IsGeneratedBy. 
ddhub:IsConditionedBy a owl:ObjectProperty; 
                      rdfs:comment ""@EN; 
                      rdfs:domain ddhub:DrillingDataPoint; 
                      rdfs:range ddhub:ValidityCondition; 
                      rdfs:subPropertyOf ddhub:DWISVerb. 
ddhub:IsConditionInput a owl:ObjectProperty; 
                       rdfs:comment ""@EN; 
                       rdfs:domain ddhub:DrillingDataPoint; 
                       rdfs:range ddhub:ValidityCondition; 
                       rdfs:subPropertyOf ddhub:DWISVerb. 
ddhub:IsConditionLeft a owl:ObjectProperty; 
                      rdfs:comment ""@EN; 
                      rdfs:domain ddhub:DWISNoun; 
                      rdfs:range ddhub:DWISNoun; 
                      rdfs:subPropertyOf ddhub:IsConditionInput. 
ddhub:IsConditionRight a owl:ObjectProperty; 
                       rdfs:comment ""@EN; 
                       rdfs:domain ddhub:DWISNoun; 
                       rdfs:range ddhub:DWISNoun; 
                       rdfs:subPropertyOf ddhub:IsConditionInput. 
ddhub:IsDependentOn a owl:ObjectProperty; 
                    rdfs:comment """This verb is used to describe a general dependence relationship between a `DrillingDataPoint` and something else.
"""@EN; 
                    rdfs:domain ddhub:DrillingDataPoint; 
                    rdfs:range ddhub:DWISNoun; 
                    rdfs:subPropertyOf ddhub:DWISVerb. 
ddhub:IsDerivationInput a owl:ObjectProperty; 
                        rdfs:comment ""@EN; 
                        rdfs:domain ddhub:DWISNoun; 
                        rdfs:range ddhub:DWISNoun; 
                        rdfs:subPropertyOf ddhub:IsTransformationInput. 
ddhub:IsDerivedFrom a owl:ObjectProperty; 
                    rdfs:comment ""@EN; 
                    rdfs:domain ddhub:DWISNoun; 
                    rdfs:range ddhub:DWISNoun; 
                    rdfs:subPropertyOf ddhub:IsTransformationOutput. 
ddhub:IsEnablingSignalFor a owl:ObjectProperty; 
                          rdfs:comment """This verb is used to define a `DrillingDataPoint` that is used to enable or disable an `ActivableFunction`.
It is expected that the `DrillingDataPoint` is a Boolean value.
"""@EN; 
                          rdfs:domain ddhub:DrillingDataPoint; 
                          rdfs:range ddhub:ActivableFunction; 
                          rdfs:subPropertyOf ddhub:DWISVerb. 
ddhub:IsEquivalentCirculationDensityAt a owl:ObjectProperty; 
                                       rdfs:comment ""@EN; 
                                       rdfs:domain ddhub:DrillingDataPoint; 
                                       rdfs:range ddhub:HydraulicLogicalElement; 
                                       rdfs:subPropertyOf ddhub:IsHydraulicallyLocatedAt. 
ddhub:IsFluidDensityAt a owl:ObjectProperty; 
                       rdfs:comment ""@EN; 
                       rdfs:domain ddhub:DrillingDataPoint; 
                       rdfs:range ddhub:HydraulicLogicalElement; 
                       rdfs:subPropertyOf ddhub:IsHydraulicallyLocatedAt. 
ddhub:IsFluidTemperatureAt a owl:ObjectProperty; 
                           rdfs:comment ""@EN; 
                           rdfs:domain ddhub:DrillingDataPoint; 
                           rdfs:range ddhub:HydraulicLogicalElement; 
                           rdfs:subPropertyOf ddhub:IsHydraulicallyLocatedAt. 
ddhub:IsFluidVelocityAt a owl:ObjectProperty; 
                        rdfs:comment ""@EN; 
                        rdfs:domain ddhub:DrillingDataPoint; 
                        rdfs:range ddhub:HydraulicLogicalElement; 
                        rdfs:subPropertyOf ddhub:IsHydraulicallyLocatedAt. 
ddhub:IsForMotionType a owl:ObjectProperty; 
                      rdfs:comment ""@EN; 
                      rdfs:domain ddhub:DrillingDataPoint; 
                      rdfs:range ddhub:MotionType; 
                      rdfs:subPropertyOf ddhub:DWISVerb. 
ddhub:IsGeneratedBy a owl:ObjectProperty; 
                    rdfs:comment ""@EN; 
                    rdfs:domain ddhub:DrillingDataPoint; 
                    rdfs:range ddhub:DataFlowNode; 
                    rdfs:subPropertyOf ddhub:DWISVerb. 
ddhub:IsHydraulicallyLocatedAt a owl:ObjectProperty; 
                               rdfs:comment ""@EN; 
                               rdfs:domain ddhub:DrillingDataPoint; 
                               rdfs:range ddhub:HydraulicLogicalElement; 
                               rdfs:subPropertyOf ddhub:DWISVerb. 
ddhub:IsHydraulicConnectedTo a owl:ObjectProperty; 
                             rdfs:comment ""@EN; 
                             rdfs:domain ddhub:HydraulicLogicalElement; 
                             rdfs:range ddhub:HydraulicLogicalElement; 
                             rdfs:subPropertyOf ddhub:DWISVerb. 
ddhub:IsHydraulicEstimationAt a owl:ObjectProperty; 
                              rdfs:comment ""@EN; 
                              rdfs:domain ddhub:DrillingDataPoint; 
                              rdfs:range ddhub:HydraulicLogicalElement; 
                              rdfs:subPropertyOf ddhub:IsHydraulicallyLocatedAt. 
ddhub:IsHydraulicMaximumAllowedRateOfChangeAt a owl:ObjectProperty; 
                                              rdfs:comment ""@EN; 
                                              rdfs:domain ddhub:DrillingDataPoint; 
                                              rdfs:range ddhub:HydraulicLogicalElement; 
                                              rdfs:subPropertyOf ddhub:IsHydraulicallyLocatedAt. 
ddhub:IsHydraulicMaximumAllowedValueAt a owl:ObjectProperty; 
                                       rdfs:comment ""@EN; 
                                       rdfs:domain ddhub:DrillingDataPoint; 
                                       rdfs:range ddhub:HydraulicLogicalElement; 
                                       rdfs:subPropertyOf ddhub:IsHydraulicallyLocatedAt. 
ddhub:IsHydraulicMeasurementAt a owl:ObjectProperty; 
                               rdfs:comment ""@EN; 
                               rdfs:domain ddhub:DrillingDataPoint; 
                               rdfs:range ddhub:HydraulicLogicalElement; 
                               rdfs:subPropertyOf ddhub:IsHydraulicallyLocatedAt. 
ddhub:IsIdlingAfterTriggeredSignalFor a owl:ObjectProperty; 
                                      rdfs:comment """This verb is used to indicate that a `DrillingDataPoint` tells whether the isolation or the recovery
"""@EN; 
                                      rdfs:domain ddhub:DrillingDataPoint; 
                                      rdfs:range ddhub:FDIRFunction; 
                                      rdfs:subPropertyOf ddhub:DWISVerb. 
ddhub:IsIdlingSignalFor a owl:ObjectProperty; 
                        rdfs:comment """This verb is used to indicate a `DrillingDataPoint` that tells if the function is in an idle state.
A function that is idle must be enabled but does not perform any particular control on the machines. For instance, a 
`ProcedureFunction` that has reached its terminal state or a `ControllerFunction` that cannot control anymore its 
parameter because a limit is reached, e.g., autodriller when reaching the `MinDrillHeightVerticalLocation`, or an FDIR
function when there are no incidents that is detected. A SOE function is in idle state, if the used set-points are
within the limits, but if the limits are applied then the idle state is false, because the function acts on the set-points.
"""@EN; 
                        rdfs:domain ddhub:DrillingDataPoint; 
                        rdfs:range ddhub:RunnableFunction; 
                        rdfs:subPropertyOf ddhub:DWISVerb. 
ddhub:IsImpactDescriptionSignalFor a owl:ObjectProperty; 
                                   rdfs:comment """This verbs is used to indicate that a `DrillingDataPoint` used by an `FDIRFunction` can be used to
describe the impact of the function on the drilling process. This signal is supposed to be string value.
"""@EN; 
                                   rdfs:domain ddhub:DrillingDataPoint; 
                                   rdfs:range ddhub:FDIRFunction; 
                                   rdfs:subPropertyOf ddhub:DWISVerb. 
ddhub:IsIntegratedFrom a owl:ObjectProperty; 
                       rdfs:comment ""@EN; 
                       rdfs:domain ddhub:DWISNoun; 
                       rdfs:range ddhub:DWISNoun; 
                       rdfs:subPropertyOf ddhub:IsTransformationOutput. 
ddhub:IsLimitFor a owl:ObjectProperty; 
                 rdfs:comment ""@EN; 
                 rdfs:domain ddhub:DrillingDataPoint; 
                 rdfs:range ddhub:DWISNoun; 
                 rdfs:subPropertyOf ddhub:HasFunction. 
ddhub:IsMassFlowRateAt a owl:ObjectProperty; 
                       rdfs:comment ""@EN; 
                       rdfs:domain ddhub:DrillingDataPoint; 
                       rdfs:range ddhub:HydraulicLogicalElement; 
                       rdfs:subPropertyOf ddhub:IsHydraulicallyLocatedAt. 
ddhub:IsMaximumLimitFor a owl:ObjectProperty; 
                        rdfs:comment ""@EN; 
                        rdfs:domain ddhub:DrillingDataPoint; 
                        rdfs:range ddhub:DWISNoun; 
                        rdfs:subPropertyOf ddhub:IsLimitFor. 
ddhub:IsMeasuredBy a owl:ObjectProperty; 
                   rdfs:comment ""@EN; 
                   rdfs:domain ddhub:DWISNoun; 
                   rdfs:range ddhub:DWISNoun; 
                   rdfs:subPropertyOf ddhub:IsGeneratedBy. 
ddhub:IsMechanicallyConnectedTo a owl:ObjectProperty; 
                                rdfs:comment ""@EN; 
                                rdfs:domain ddhub:MechanicalLogicalElement; 
                                rdfs:range ddhub:MechanicalLogicalElement; 
                                rdfs:subPropertyOf ddhub:DWISVerb. 
ddhub:IsMechanicallyLocatedAt a owl:ObjectProperty; 
                              rdfs:comment ""@EN; 
                              rdfs:domain ddhub:DrillingDataPoint; 
                              rdfs:range ddhub:MechanicalLogicalElement; 
                              rdfs:subPropertyOf ddhub:DWISVerb. 
ddhub:IsMinimumLimitFor a owl:ObjectProperty; 
                        rdfs:comment ""@EN; 
                        rdfs:domain ddhub:DrillingDataPoint; 
                        rdfs:range ddhub:DWISNoun; 
                        rdfs:subPropertyOf ddhub:IsLimitFor. 
ddhub:IsobaricSpecificHeatCapacityDrillingQuantity a owl:Class; 
                                                   rdfs:comment """Isobaric specific heat capacity is the amount of heat required to raise the temperature of one unit mass of a substance by one unit of temperature at constant pressure. It indicates how much heat energy a material can store.
The dimension of specific heat capacity is:
$$[L^{2}K^{-1}T^{-2}]$$.
The SI unit for **isobaric specific heat capacity** is: joule per kilogram kelvin with the associated unit label $\\frac{J}{kg \\cdot K}$
The meaningful precision of specific heat capacity in the drilling context is typically: 0.01 J/kg•K
"""@EN; 
                                                   rdfs:subClassOf ddhub:MeasurableQuantity. 
ddhub:IsobaricSpecificHeatCapacityGradientPerTemperatureDrillingQuantity a owl:Class; 
                                                                         rdfs:comment """An isobaric specific heat capacity gradient per temperature is the first derivative of an isobaric specific heat capacity compared to temperature: $\\frac{dC_p}{dT}$, where $C_p$ is a isobaric specific heat capacity and $T$ is a temperature.
The dimension of specific heat capacity gradient per temperature is:
$$[L^{2}T^{-2}K^{-2}]$$.
The SI unit for **isobaric specific heat capacity gradient per temperature** is: joule per kilogram squared kelvin with the associated unit label $\\frac{J}{kg \\cdot K^{2}}$
The meaningful precision of isobaric specific heat capacity gradient per temperature in the drilling context is typically: 0.01 J/kg•K²
"""@EN; 
                                                                         rdfs:subClassOf ddhub:MeasurableQuantity. 
ddhub:IsobaricSpecificHeatCapacityGradientPerTemperatureQuantity a owl:Class; 
                                                                 rdfs:comment """An isobaric specific heat capacity gradient per temperature is the first derivative of an isobaric specific heat capacity compared to temperature: $\\frac{dC_p}{dT}$, where $C_p$ is a isobaric specific heat capacity and $T$ is a temperature.
The dimension of specific heat capacity gradient per temperature is:
$$[L^{2}T^{-2}K^{-2}]$$.
The SI unit for **isobaric specific heat capacity gradient per temperature** is: joule per kilogram squared kelvin with the associated unit label $\\frac{J}{kg \\cdot K^{2}}$
"""@EN; 
                                                                 rdfs:subClassOf ddhub:Quantity. 
ddhub:IsobaricSpecificHeatCapacityQuantity a owl:Class; 
                                           rdfs:comment """Isobaric specific heat capacity is the amount of heat required to raise the temperature of one unit mass of a substance by one unit of temperature at constant pressure. It indicates how much heat energy a material can store.
The dimension of specific heat capacity is:
$$[L^{2}K^{-1}T^{-2}]$$.
The SI unit for **isobaric specific heat capacity** is: joule per kilogram kelvin with the associated unit label $\\frac{J}{kg \\cdot K}$
"""@EN; 
                                           rdfs:subClassOf ddhub:Quantity. 
ddhub:IsObservableFrom a owl:ObjectProperty; 
                       rdfs:comment ""@EN; 
                       rdfs:domain ddhub:DWISNoun; 
                       rdfs:range ddhub:DWISNoun; 
                       rdfs:subPropertyOf ddhub:DWISVerb. 
ddhub:IsOfBaseQuantity a owl:ObjectProperty; 
                       rdfs:comment ""@EN; 
                       rdfs:domain ddhub:MeasurableQuantity; 
                       rdfs:range ddhub:Quantity; 
                       rdfs:subPropertyOf ddhub:DWISVerb. 
ddhub:IsOfMeasurableQuantity a owl:ObjectProperty; 
                             rdfs:comment ""@EN; 
                             rdfs:domain ddhub:DrillingSignal; 
                             rdfs:range ddhub:MeasurableQuantity; 
                             rdfs:subPropertyOf ddhub:DWISVerb. 
ddhub:IsOfMechanicalStiffnessType a owl:ObjectProperty; 
                                  rdfs:comment """A relation to describe how the drill-stem mechanical model manage stiffness.
"""@EN; 
                                  rdfs:domain ddhub:DrillStemMechanicalModel; 
                                  rdfs:range ddhub:MechanicalStiffnessType; 
                                  rdfs:subPropertyOf ddhub:DWISVerb. 
ddhub:IsolationSeal a owl:Class; 
                    rdfs:comment ""@EN; 
                    rdfs:subClassOf ddhub:DrillingEquipment. 
ddhub:IsOpeningRatioAt a owl:ObjectProperty; 
                       rdfs:comment ""@EN; 
                       rdfs:domain ddhub:DrillingDataPoint; 
                       rdfs:range ddhub:HydraulicLogicalElement; 
                       rdfs:subPropertyOf ddhub:IsHydraulicallyLocatedAt. 
ddhub:IsPhysicallyLocatedAt a owl:ObjectProperty; 
                            rdfs:comment ""@EN; 
                            rdfs:domain ddhub:DrillingDataPoint; 
                            rdfs:range ddhub:Location; 
                            rdfs:subPropertyOf ddhub:DWISVerb. 
ddhub:IsPressureAt a owl:ObjectProperty; 
                   rdfs:comment ""@EN; 
                   rdfs:domain ddhub:DrillingDataPoint; 
                   rdfs:range ddhub:HydraulicLogicalElement; 
                   rdfs:subPropertyOf ddhub:IsHydraulicallyLocatedAt. 
ddhub:IsPressureGradientAt a owl:ObjectProperty; 
                           rdfs:comment ""@EN; 
                           rdfs:domain ddhub:DrillingDataPoint; 
                           rdfs:range ddhub:HydraulicLogicalElement; 
                           rdfs:subPropertyOf ddhub:IsHydraulicallyLocatedAt. 
ddhub:IsProcessedBy a owl:ObjectProperty; 
                    rdfs:comment ""@EN; 
                    rdfs:domain ddhub:DWISNoun; 
                    rdfs:range ddhub:DWISNoun; 
                    rdfs:subPropertyOf ddhub:DWISVerb. 
ddhub:IsProvidedBy a owl:ObjectProperty; 
                   rdfs:comment ""@EN; 
                   rdfs:domain ddhub:DWISNoun; 
                   rdfs:range ddhub:DataProvider; 
                   rdfs:subPropertyOf ddhub:DWISVerb. 
ddhub:IsProvidedTo a owl:ObjectProperty; 
                   rdfs:comment ""@EN; 
                   rdfs:domain ddhub:DWISNoun; 
                   rdfs:range ddhub:DataProvider; 
                   rdfs:subPropertyOf ddhub:DWISVerb. 
ddhub:IsRecordedFrom a owl:ObjectProperty; 
                     rdfs:comment ""@EN; 
                     rdfs:domain ddhub:DWISNoun; 
                     rdfs:range ddhub:DWISNoun; 
                     rdfs:subPropertyOf ddhub:IsGeneratedBy. 
ddhub:IsRelatedToDrillingIncident a owl:ObjectProperty; 
                                  rdfs:comment ""@EN; 
                                  rdfs:domain ddhub:DrillingDataPoint; 
                                  rdfs:range ddhub:DrillingIncident; 
                                  rdfs:subPropertyOf ddhub:DWISVerb. 
ddhub:IsResampledBy a owl:ObjectProperty; 
                    rdfs:comment ""@EN; 
                    rdfs:domain ddhub:DrillingDataPoint; 
                    rdfs:range ddhub:Resampling; 
                    rdfs:subPropertyOf ddhub:IsTransformationOutput. 
ddhub:IsResamplingInput a owl:ObjectProperty; 
                        rdfs:comment ""@EN; 
                        rdfs:domain ddhub:DrillingDataPoint; 
                        rdfs:range ddhub:Resampling; 
                        rdfs:subPropertyOf ddhub:IsTransformationInput. 
ddhub:IsSetPointAdviceFor a owl:ObjectProperty; 
                          rdfs:comment ""@EN; 
                          rdfs:domain ddhub:DrillingDataPoint; 
                          rdfs:range ddhub:ControlSystem; 
                          rdfs:subPropertyOf ddhub:HasFunction. 
ddhub:IsSetPointFor a owl:ObjectProperty; 
                    rdfs:comment ""@EN; 
                    rdfs:domain ddhub:DrillingDataPoint; 
                    rdfs:range ddhub:Controller; 
                    rdfs:subPropertyOf ddhub:HasFunction. 
ddhub:IsSetPointMaximumAdviceFor a owl:ObjectProperty; 
                                 rdfs:comment ""@EN; 
                                 rdfs:domain ddhub:DrillingDataPoint; 
                                 rdfs:range ddhub:ControlSystem; 
                                 rdfs:subPropertyOf ddhub:HasFunction. 
ddhub:IsSetPointMaximumRecommendationFor a owl:ObjectProperty; 
                                         rdfs:comment ""@EN; 
                                         rdfs:domain ddhub:DrillingDataPoint; 
                                         rdfs:range ddhub:ControlSystem; 
                                         rdfs:subPropertyOf ddhub:HasFunction. 
ddhub:IsSetPointMinimumAdviceFor a owl:ObjectProperty; 
                                 rdfs:comment ""@EN; 
                                 rdfs:domain ddhub:DrillingDataPoint; 
                                 rdfs:range ddhub:ControlSystem; 
                                 rdfs:subPropertyOf ddhub:HasFunction. 
ddhub:IsSetPointMinimumRecommendationFor a owl:ObjectProperty; 
                                         rdfs:comment ""@EN; 
                                         rdfs:domain ddhub:DrillingDataPoint; 
                                         rdfs:range ddhub:ControlSystem; 
                                         rdfs:subPropertyOf ddhub:HasFunction. 
ddhub:IsSetPointRecommendationFor a owl:ObjectProperty; 
                                  rdfs:comment ""@EN; 
                                  rdfs:domain ddhub:DrillingDataPoint; 
                                  rdfs:range ddhub:ControlSystem; 
                                  rdfs:subPropertyOf ddhub:HasFunction. 
ddhub:IsSubPartOf a owl:ObjectProperty; 
                  rdfs:comment ""@EN; 
                  rdfs:domain ddhub:DrillingEquipment; 
                  rdfs:range ddhub:DrillingEquipment; 
                  rdfs:subPropertyOf ddhub:DWISVerb. 
ddhub:IsSynchronizationGroupInput a owl:ObjectProperty; 
                                  rdfs:comment ""@EN; 
                                  rdfs:domain ddhub:DrillingDataPoint; 
                                  rdfs:range ddhub:SynchronizationGroup; 
                                  rdfs:subPropertyOf ddhub:DWISVerb. 
ddhub:IsSynchronizationGroupOutput a owl:ObjectProperty; 
                                   rdfs:comment ""@EN; 
                                   rdfs:domain ddhub:DrillingDataPoint; 
                                   rdfs:range ddhub:SynchronizationGroup; 
                                   rdfs:subPropertyOf ddhub:DWISVerb. 
ddhub:IsToBeComparedWith a owl:ObjectProperty; 
                         rdfs:comment ""@EN; 
                         rdfs:domain ddhub:DrillingDataPoint; 
                         rdfs:range ddhub:DrillingDataPoint; 
                         rdfs:subPropertyOf ddhub:DWISVerb. 
ddhub:IsToBeDifferentFrom a owl:ObjectProperty; 
                          rdfs:comment ""@EN; 
                          rdfs:domain ddhub:DrillingDataPoint; 
                          rdfs:range ddhub:DrillingDataPoint; 
                          rdfs:subPropertyOf ddhub:IsToBeComparedWith. 
ddhub:IsToBeEqualTo a owl:ObjectProperty; 
                    rdfs:comment ""@EN; 
                    rdfs:domain ddhub:DrillingDataPoint; 
                    rdfs:range ddhub:DrillingDataPoint; 
                    rdfs:subPropertyOf ddhub:IsToBeComparedWith. 
ddhub:IsToBeGreaterOrEqualThan a owl:ObjectProperty; 
                               rdfs:comment ""@EN; 
                               rdfs:domain ddhub:DrillingDataPoint; 
                               rdfs:range ddhub:DrillingDataPoint; 
                               rdfs:subPropertyOf ddhub:IsToBeGreaterThan. 
ddhub:IsToBeGreaterThan a owl:ObjectProperty; 
                        rdfs:comment ""@EN; 
                        rdfs:domain ddhub:DrillingDataPoint; 
                        rdfs:range ddhub:DrillingDataPoint; 
                        rdfs:subPropertyOf ddhub:IsToBeComparedWith. 
ddhub:IsToBeSmallerOrEqualThan a owl:ObjectProperty; 
                               rdfs:comment ""@EN; 
                               rdfs:domain ddhub:DrillingDataPoint; 
                               rdfs:range ddhub:DrillingDataPoint; 
                               rdfs:subPropertyOf ddhub:IsToBeSmallerThan. 
ddhub:IsToBeSmallerThan a owl:ObjectProperty; 
                        rdfs:comment ""@EN; 
                        rdfs:domain ddhub:DrillingDataPoint; 
                        rdfs:range ddhub:DrillingDataPoint; 
                        rdfs:subPropertyOf ddhub:IsToBeComparedWith. 
ddhub:IsToBeStrictlyGreaterThan a owl:ObjectProperty; 
                                rdfs:comment ""@EN; 
                                rdfs:domain ddhub:DrillingDataPoint; 
                                rdfs:range ddhub:DrillingDataPoint; 
                                rdfs:subPropertyOf ddhub:IsToBeGreaterThan. 
ddhub:IsToBeStrictlySmallerThan a owl:ObjectProperty; 
                                rdfs:comment ""@EN; 
                                rdfs:domain ddhub:DrillingDataPoint; 
                                rdfs:range ddhub:DrillingDataPoint; 
                                rdfs:subPropertyOf ddhub:IsToBeSmallerThan. 
ddhub:IsTransformationInput a owl:ObjectProperty; 
                            rdfs:comment ""@EN; 
                            rdfs:domain ddhub:DrillingDataPoint; 
                            rdfs:range ddhub:Transformation; 
                            rdfs:subPropertyOf ddhub:HasFunction. 
ddhub:IsTransformationOutput a owl:ObjectProperty; 
                             rdfs:comment ""@EN; 
                             rdfs:domain ddhub:DrillingDataPoint; 
                             rdfs:range ddhub:DataFlowNode; 
                             rdfs:subPropertyOf ddhub:IsGeneratedBy. 
ddhub:IsTransmissionInput a owl:ObjectProperty; 
                          rdfs:comment ""@EN; 
                          rdfs:domain ddhub:DrillingDataPoint; 
                          rdfs:range ddhub:TransmissionLine; 
                          rdfs:subPropertyOf ddhub:HasFunction. 
ddhub:IsTransmissionOutput a owl:ObjectProperty; 
                           rdfs:comment ""@EN; 
                           rdfs:domain ddhub:DrillingDataPoint; 
                           rdfs:range ddhub:TransmissionLine; 
                           rdfs:subPropertyOf ddhub:IsGeneratedBy. 
ddhub:IsTransmittedBy a owl:ObjectProperty; 
                      rdfs:comment """Expresses that a signal is transmitted by some given telemetry system
"""@EN; 
                      rdfs:domain ddhub:DrillingDataPoint; 
                      rdfs:range ddhub:Telemetry; 
                      rdfs:subPropertyOf ddhub:DWISVerb. 
ddhub:IsTriggeredSignalFor a owl:ObjectProperty; 
                           rdfs:comment """This verb is used to indicate a `DrillingDataPoint` tells whether an `FDIRFunction` has been triggered
or not. This signal is expected to be a Boolean value. The signal is expected to be true from the moment the FDIR has triggered
to the moment it has recovered from the incident, if it has a recovery procedure, or to the moment the control is given
back to the end-user, in case of failure of the recovery procedure or at the end of the isolation procedure.
"""@EN; 
                           rdfs:domain ddhub:DrillingDataPoint; 
                           rdfs:range ddhub:FDIRFunction; 
                           rdfs:subPropertyOf ddhub:DWISVerb. 
ddhub:IsUnitForQuantity a owl:ObjectProperty; 
                        rdfs:comment ""@EN; 
                        rdfs:domain ddhub:Unit; 
                        rdfs:range ddhub:Quantity; 
                        rdfs:subPropertyOf ddhub:DWISVerb. 
ddhub:IsUsedExtraMarginSignalFor a owl:ObjectProperty; 
                                 rdfs:comment """This verb is used to indicate a `DrillingDataPoint` used by an `FDIRFunction` tells whether the
extra margin signal is used or not by the FDIR function. This signal is expected to be a boolean value.
"""@EN; 
                                 rdfs:domain ddhub:DrillingDataPoint; 
                                 rdfs:range ddhub:FDIRFunction; 
                                 rdfs:subPropertyOf ddhub:DWISVerb. 
ddhub:IsUserControllableExtraMarginSignalFor a owl:ObjectProperty; 
                                             rdfs:comment """This verb is used to indicate that a `DrillingDataPoint` used by an `FDIRFunction`, extends the calculated
threshold value for the fault detection by a user-defined amount. The value of this signal is supposed to be interpreted
in absolute value. If it is negative, then it is its magnitude that is used. This allows the end-user to increase the margin for
detection of an incident. 
"""@EN; 
                                             rdfs:domain ddhub:DrillingDataPoint; 
                                             rdfs:range ddhub:FDIRFunction; 
                                             rdfs:subPropertyOf ddhub:DWISVerb. 
ddhub:IsValid a owl:DatatypeProperty, owl:FunctionalProperty; 
              rdfs:comment """
"""@EN; 
              rdfs:domain ddhub:DrillingDataPoint; 
              rdfs:range xsd:bool. 
ddhub:IsValidBy a owl:ObjectProperty; 
                rdfs:comment ""@EN; 
                rdfs:domain ddhub:DWISNoun; 
                rdfs:range ddhub:DWISNoun; 
                rdfs:subPropertyOf ddhub:DWISVerb. 
ddhub:IsVolumeAt a owl:ObjectProperty; 
                 rdfs:comment ""@EN; 
                 rdfs:domain ddhub:DrillingDataPoint; 
                 rdfs:range ddhub:Tank; 
                 rdfs:subPropertyOf ddhub:IsHydraulicallyLocatedAt. 
ddhub:IsVolumetricFlowRateAt a owl:ObjectProperty; 
                             rdfs:comment ""@EN; 
                             rdfs:domain ddhub:DrillingDataPoint; 
                             rdfs:range ddhub:HydraulicLogicalElement; 
                             rdfs:subPropertyOf ddhub:IsHydraulicallyLocatedAt. 
ddhub:J a owl:DatatypeProperty, owl:FunctionalProperty; 
        rdfs:comment """Luminous intensity exponent.
SI Unit: Candela (cd)
"""@EN; 
        rdfs:domain ddhub:Quantity; 
        rdfs:range xsd:double. 
ddhub:JackupLegs a owl:Class; 
                 rdfs:comment ""@EN; 
                 rdfs:subClassOf ddhub:MarineSystem. 
ddhub:JarAction a owl:Class; 
                rdfs:comment ""@EN; 
                rdfs:subClassOf ddhub:JarringAssembly. 
ddhub:JarringAssembly a owl:Class; 
                      rdfs:comment ""@EN; 
                      rdfs:subClassOf ddhub:DrillingEquipment. 
ddhub:JettingAssembly a owl:Class; 
                      rdfs:comment ""@EN; 
                      rdfs:subClassOf ddhub:DrillingEquipment. 
ddhub:JunkBasket a owl:Class; 
                 rdfs:comment ""@EN; 
                 rdfs:subClassOf ddhub:FishingTools. 
ddhub:Kelly a owl:Class; 
            rdfs:comment ""@EN; 
            rdfs:subClassOf ddhub:RotaryTable. 
ddhub:KellyBushing a owl:Class; 
                   rdfs:comment ""@EN; 
                   rdfs:subClassOf ddhub:Kelly. 
ddhub:KellyBushingVerticalLocation a owl:Class; 
                                   rdfs:comment ""@EN; 
                                   rdfs:subClassOf ddhub:VerticalReferenceLocation. 
ddhub:KellyHose a owl:Class; 
                rdfs:comment ""@EN; 
                rdfs:subClassOf ddhub:Kelly. 
ddhub:KellyJoint a owl:Class; 
                 rdfs:comment ""@EN; 
                 rdfs:subClassOf ddhub:Kelly. 
ddhub:KellySwivel a owl:Class; 
                  rdfs:comment ""@EN; 
                  rdfs:subClassOf ddhub:Kelly. 
ddhub:KellyValve a owl:Class; 
                 rdfs:comment ""@EN; 
                 rdfs:subClassOf ddhub:WellControlSystem. 
ddhub:KickOffVerticalLocation a owl:Class; 
                              rdfs:comment ""@EN; 
                              rdfs:subClassOf ddhub:VerticalReferenceLocation. 
ddhub:KillLine a owl:Class; 
               rdfs:comment ""@EN; 
               rdfs:subClassOf ddhub:WellControlSystem. 
ddhub:L a owl:DatatypeProperty, owl:FunctionalProperty; 
        rdfs:comment """Length exponent.
SI Unit: meter (m)
"""@EN; 
        rdfs:domain ddhub:Quantity; 
        rdfs:range xsd:double. 
ddhub:LandBop a owl:Class; 
              rdfs:comment ""@EN; 
              rdfs:subClassOf ddhub:BopStack. 
ddhub:LandingJoint a owl:Class; 
                   rdfs:comment ""@EN; 
                   rdfs:subClassOf ddhub:MarineSystem. 
ddhub:LandingString a owl:Class; 
                    rdfs:comment ""@EN; 
                    rdfs:subClassOf ddhub:CasingEquipment. 
ddhub:LastCasingShoeReferenceLocation a owl:Class; 
                                      rdfs:comment ""@EN; 
                                      rdfs:subClassOf ddhub:AbscissaReferenceLocation. 
ddhub:LateralModelling a owl:Class; 
                       rdfs:comment """The model accounts for the lateral movement of some parts of the physical system.
"""@EN; 
                       rdfs:subClassOf ddhub:ModelledDegreeOfFreedom. 
ddhub:LateralMotionType a owl:Class; 
                        rdfs:comment ""@EN; 
                        rdfs:subClassOf ddhub:MotionType. 
ddhub:LeapSeconds a owl:DatatypeProperty, owl:FunctionalProperty; 
                  rdfs:comment """
"""@EN; 
                  rdfs:domain ddhub:Clock; 
                  rdfs:range xsd:int. 
ddhub:LeaseLinePositionLocation a owl:Class; 
                                rdfs:comment ""@EN; 
                                rdfs:subClassOf ddhub:PositionReferenceLocation. 
ddhub:LedgeLocation a owl:Class; 
                    rdfs:comment ""@EN; 
                    rdfs:subClassOf ddhub:AbscissaReferenceLocation. 
ddhub:LeftToRight a owl:DatatypeProperty, owl:FunctionalProperty; 
                  rdfs:comment """Indicates whether the fluid can flow from the left branch to the right branch though the junction
"""@EN; 
                  rdfs:domain ddhub:HydraulicJunction; 
                  rdfs:range xsd:bool. 
ddhub:LengthQuantity a owl:Class; 
                     rdfs:comment """Length is a measure of distance.
The dimension of length is:
$$[L]$$.
The SI unit for **length** is: metre with the associated unit label $m$
"""@EN; 
                     rdfs:subClassOf ddhub:Quantity. 
ddhub:LengthSmallQuantity a owl:Class; 
                          rdfs:comment """Length is a measure of distance.
The dimension of length is:
$$[L]$$.
The SI unit for **length** is: metre with the associated unit label $m$
The meaningful precision of small length is typically: 1E-05 m
"""@EN; 
                          rdfs:subClassOf ddhub:MeasurableQuantity. 
ddhub:LengthStandardQuantity a owl:Class; 
                             rdfs:comment """Length is a measure of distance.
The dimension of length is:
$$[L]$$.
The SI unit for **length** is: metre with the associated unit label $m$
The meaningful precision of a standard length is typically: 0.001 m
"""@EN; 
                             rdfs:subClassOf ddhub:MeasurableQuantity. 
ddhub:Limit a owl:Class; 
            rdfs:comment ""@EN; 
            rdfs:subClassOf ddhub:ProcessData. 
ddhub:Liner a owl:Class; 
            rdfs:comment ""@EN; 
            rdfs:subClassOf ddhub:PistonMudPump. 
ddhub:LinerDrilling a owl:Class; 
                    rdfs:comment ""@EN; 
                    rdfs:subClassOf ddhub:DrillingEquipment. 
ddhub:LinerHanger a owl:Class; 
                  rdfs:comment ""@EN; 
                  rdfs:subClassOf ddhub:Hangers. 
ddhub:LinerPacker a owl:Class; 
                  rdfs:comment ""@EN; 
                  rdfs:subClassOf ddhub:CasingEquipment. 
ddhub:Liners a owl:Class; 
             rdfs:comment ""@EN; 
             rdfs:subClassOf ddhub:CasingString. 
ddhub:LiquidComponent a owl:Class; 
                      rdfs:comment ""@EN; 
                      rdfs:subClassOf ddhub:FluidComponent. 
ddhub:LoadNut a owl:Class; 
              rdfs:comment ""@EN; 
              rdfs:subClassOf ddhub:TopDrive. 
ddhub:LocalTimeReference a owl:Class; 
                         rdfs:comment ""@EN; 
                         rdfs:subClassOf ddhub:RelativeTimeReference. 
ddhub:Location a owl:Class; 
               rdfs:comment """Physical location for a signal. Refers to: 1) a reference frame (via the HasReferenceFrame relation), that works as a system of coordinates 2) an origin (of type Location) via the HasReferenceFrameOrigin relation.
 - some coordinates
"""@EN; 
               rdfs:subClassOf ddhub:DWISNoun. 
ddhub:LoggingEquipment a owl:Class; 
                       rdfs:comment ""@EN; 
                       rdfs:subClassOf ddhub:DownholeEquipment. 
ddhub:LoggingServiceCompany a owl:Class; 
                            rdfs:comment """A logging service company is an entity that gathers measured information during well construction.
"""@EN; 
                            rdfs:subClassOf ddhub:ServiceCompany. 
ddhub:LoggingWhileDrillingTools a owl:Class; 
                                rdfs:comment ""@EN; 
                                rdfs:subClassOf ddhub:LoggingEquipment. 
ddhub:LoggingWhileDrillingToolsAcoustictools a owl:Class; 
                                             rdfs:comment ""@EN; 
                                             rdfs:subClassOf ddhub:LoggingWhileDrillingTools. 
ddhub:LoggingWhileDrillingToolsElectricalpropagation a owl:Class; 
                                                     rdfs:comment ""@EN; 
                                                     rdfs:subClassOf ddhub:LoggingWhileDrillingTools. 
ddhub:LoggingWhileDrillingToolsElectricalresistivity a owl:Class; 
                                                     rdfs:comment ""@EN; 
                                                     rdfs:subClassOf ddhub:LoggingWhileDrillingTools. 
ddhub:LoggingWhileDrillingToolsNmrtools a owl:Class; 
                                        rdfs:comment ""@EN; 
                                        rdfs:subClassOf ddhub:LoggingWhileDrillingTools. 
ddhub:LoggingWhileDrillingToolsNucleartools a owl:Class; 
                                            rdfs:comment ""@EN; 
                                            rdfs:subClassOf ddhub:LoggingWhileDrillingTools. 
ddhub:LoggingWhileDrillingToolsSeismictools a owl:Class; 
                                            rdfs:comment ""@EN; 
                                            rdfs:subClassOf ddhub:LoggingWhileDrillingTools. 
ddhub:LogName a owl:DatatypeProperty, owl:FunctionalProperty; 
              rdfs:comment """
"""@EN; 
              rdfs:domain ddhub:WitsMLTimeBasedLogEndPoint; 
              rdfs:range xsd:string. 
ddhub:LogUID a owl:DatatypeProperty, owl:FunctionalProperty; 
             rdfs:comment """
"""@EN; 
             rdfs:domain ddhub:WitsMLTimeBasedLogEndPoint; 
             rdfs:range xsd:string. 
ddhub:LossCirculation a owl:Class; 
                      rdfs:comment ""@EN; 
                      rdfs:subClassOf ddhub:DrillingIncident. 
ddhub:LowerMarineRiserPackageLmrp a owl:Class; 
                                  rdfs:comment ""@EN; 
                                  rdfs:subClassOf ddhub:MarineSystem. 
ddhub:LowestAstronomicalTideVerticalLocation a owl:Class; 
                                             rdfs:comment ""@EN; 
                                             rdfs:subClassOf ddhub:VerticalReferenceLocation. 
ddhub:LowGravitySolidComponent a owl:Class; 
                               rdfs:comment ""@EN; 
                               rdfs:subClassOf ddhub:DrillingFluidSolidComponent. 
ddhub:LowPassFilter a owl:Class; 
                    rdfs:comment ""@EN; 
                    rdfs:subClassOf ddhub:Filter. 
ddhub:LowPressureRiser a owl:Class; 
                       rdfs:comment ""@EN; 
                       rdfs:subClassOf ddhub:SurfaceRiser. 
ddhub:LT a owl:Class; 
         rdfs:comment ""@EN; 
         rdfs:subClassOf ddhub:ValidityCondition. 
ddhub:LuminousIntensityQuantity a owl:Class; 
                                rdfs:comment """Luminous intensity is the measure of the amount of visible light emitted by a source in a particular direction.
The dimension of luminous intensity is:
$$[J]$$.
The SI unit for **luminous intensity** is: candela with the associated unit label $cd$
"""@EN; 
                                rdfs:subClassOf ddhub:Quantity. 
ddhub:M a owl:DatatypeProperty, owl:FunctionalProperty; 
        rdfs:comment """Mass exponent.
SI Unit: Kilogram (kg)
"""@EN; 
        rdfs:domain ddhub:Quantity; 
        rdfs:range xsd:double. 
ddhub:MagneticFluxDensityQuantity a owl:Class; 
                                  rdfs:comment """Magnetic flux density is the measure of the strength of a magnetic field per unit area through which the magnetic flux passes. It indicates how concentrated the magnetic field is.
The dimension of magnetic flux density is:
$$[MI^{-1}T^{-2}]$$.
The SI unit for **magnetic flux density** is: tesla with the associated unit label $T$
"""@EN; 
                                  rdfs:subClassOf ddhub:Quantity. 
ddhub:MagneticFluxQuantity a owl:Class; 
                           rdfs:comment """Magnetic flux is the measure of the total magnetic field passing through a given area. It quantifies the strength and distribution of a magnetic field over a surface.
The dimension of magnetic flux is:
$$[L^{2}MI^{-1}T^{-2}]$$.
The SI unit for **magnetic flux** is: weber with the associated unit label $Wb$
"""@EN; 
                           rdfs:subClassOf ddhub:Quantity. 
ddhub:MagneticHighSideAngleLocation a owl:Class; 
                                    rdfs:comment ""@EN; 
                                    rdfs:subClassOf ddhub:AngleReferenceLocation. 
ddhub:MagneticNorthAzimuthLocation a owl:Class; 
                                   rdfs:comment ""@EN; 
                                   rdfs:subClassOf ddhub:AzimuthReferenceLocation. 
ddhub:MainframeAssembly a owl:Class; 
                        rdfs:comment ""@EN; 
                        rdfs:subClassOf ddhub:TopDrive. 
ddhub:Mandrel a owl:Class; 
              rdfs:comment ""@EN; 
              rdfs:subClassOf ddhub:Connection. 
ddhub:ManualPipeTongs a owl:Class; 
                      rdfs:comment ""@EN; 
                      rdfs:subClassOf ddhub:DrillPipeTongs. 
ddhub:ManualSlips a owl:Class; 
                  rdfs:comment ""@EN; 
                  rdfs:subClassOf ddhub:RotarySlips. 
ddhub:MarineFuel a owl:Class; 
                 rdfs:comment ""@EN; 
                 rdfs:subClassOf ddhub:MarineSystem. 
ddhub:MarineRiser a owl:Class; 
                  rdfs:comment ""@EN; 
                  rdfs:subClassOf ddhub:DrillingRiser. 
ddhub:MarineRiserTensionerMrtRing a owl:Class; 
                                  rdfs:comment ""@EN; 
                                  rdfs:subClassOf ddhub:MarineSystem. 
ddhub:MarineSystem a owl:Class; 
                   rdfs:comment ""@EN; 
                   rdfs:subClassOf ddhub:RigEquipment. 
ddhub:MassDensityDrillingQuantity a owl:Class; 
                                  rdfs:comment """Mass density is the amount of mass per unit volume of a substance.
The dimension of mass density is:
$$[ML^{-3}]$$.
The SI unit for **mass density** is: kilogram per cubic metre with the associated unit label $\\frac{kg}{m^{3}}$
The meaningful precision of mass density in the drilling context is typically: 1 kg/m³
"""@EN; 
                                  rdfs:subClassOf ddhub:MeasurableQuantity. 
ddhub:MassDensityGradientPerLengthDrillingQuantity a owl:Class; 
                                                   rdfs:comment """A mass density gradient per length is the first derivative of a mass density compared to a distance: $\\frac{d\\rho}{ds}$, where $\\rho$ is the mass density and $s$ is a distance.
The dimension of mass density gradient per length is:
$$[ML^{-4}]$$.
The SI unit for **mass density gradient per length** is: kilogram per cubic metre per metre with the associated unit label $\\frac{\\frac{kg}{m^{3}}}{m}$
The meaningful precision of mass density gradient per length in the drilling context is typically: 0.001 kg/m³/m
"""@EN; 
                                                   rdfs:subClassOf ddhub:MeasurableQuantity. 
ddhub:MassDensityGradientPerLengthQuantity a owl:Class; 
                                           rdfs:comment """A mass density gradient per length is the first derivative of a mass density compared to a distance: $\\frac{d\\rho}{ds}$, where $\\rho$ is the mass density and $s$ is a distance.
The dimension of mass density gradient per length is:
$$[ML^{-4}]$$.
The SI unit for **mass density gradient per length** is: kilogram per cubic metre per metre with the associated unit label $\\frac{\\frac{kg}{m^{3}}}{m}$
"""@EN; 
                                           rdfs:subClassOf ddhub:Quantity. 
ddhub:MassDensityGradientPerTemperatureDrillingQuantity a owl:Class; 
                                                        rdfs:comment """A mass density gradient per temperature is the first derivative of a mass density compared to temperature: $\\frac{d\\rho}{dT}$, where $\\rho$ is a mass density and $T$ is temperature.
The dimension of mass density gradient per temperature is:
$$[MK^{-1}L^{-3}]$$.
The SI unit for **mass density gradient per temperature** is: kilogram per cubic metre per kelvin with the associated unit label $\\frac{\\frac{kg}{m^{3}}}{K}$
The meaningful precision of mass density gradient per temperature in the drilling context is typically: 0.001 kg/m³/K
"""@EN; 
                                                        rdfs:subClassOf ddhub:MeasurableQuantity. 
ddhub:MassDensityGradientPerTemperatureQuantity a owl:Class; 
                                                rdfs:comment """A mass density gradient per temperature is the first derivative of a mass density compared to temperature: $\\frac{d\\rho}{dT}$, where $\\rho$ is a mass density and $T$ is temperature.
The dimension of mass density gradient per temperature is:
$$[MK^{-1}L^{-3}]$$.
The SI unit for **mass density gradient per temperature** is: kilogram per cubic metre per kelvin with the associated unit label $\\frac{\\frac{kg}{m^{3}}}{K}$
"""@EN; 
                                                rdfs:subClassOf ddhub:Quantity. 
ddhub:MassDensityQuantity a owl:Class; 
                          rdfs:comment """Mass density is the amount of mass per unit volume of a substance.
The dimension of mass density is:
$$[ML^{-3}]$$.
The SI unit for **mass density** is: kilogram per cubic metre with the associated unit label $\\frac{kg}{m^{3}}$
"""@EN; 
                          rdfs:subClassOf ddhub:Quantity. 
ddhub:MassDensityRateOfChangeDrillingQuantity a owl:Class; 
                                              rdfs:comment """A mass density rate of change is the time derivative of a mass density: $\\frac{d\\rho}{dt}$, where $\\rho$ is the mass density and $t$ is time.
The dimension of mass density rate of change is:
$$[MT^{-1}L^{-3}]$$.
The SI unit for **mass density rate of change** is: kilogram per cubic metre per second with the associated unit label $\\frac{\\frac{kg}{m^{3}}}{s}$
The meaningful precision of mass density rate of change in the drilling context is typically: 0.001 kg/m³/s
"""@EN; 
                                              rdfs:subClassOf ddhub:MeasurableQuantity. 
ddhub:MassDensityRateOfChangeQuantity a owl:Class; 
                                      rdfs:comment """A mass density rate of change is the time derivative of a mass density: $\\frac{d\\rho}{dt}$, where $\\rho$ is the mass density and $t$ is time.
The dimension of mass density rate of change is:
$$[MT^{-1}L^{-3}]$$.
The SI unit for **mass density rate of change** is: kilogram per cubic metre per second with the associated unit label $\\frac{\\frac{kg}{m^{3}}}{s}$
"""@EN; 
                                      rdfs:subClassOf ddhub:Quantity. 
ddhub:MassDrillingQuantity a owl:Class; 
                           rdfs:comment """Mass can be experimentally defined as a measure of the body's inertia, meaning the resistance to acceleration (change of velocity) when a net force is applied. The object's mass also determines the strength of its gravitational attraction to other bodies.
The dimension of mass is:
$$[M]$$.
The SI unit for **mass** is: kilogram with the associated unit label $kg$
The meaningful precision of mass density in the drilling context is typically: 0.1 kg
"""@EN; 
                           rdfs:subClassOf ddhub:MeasurableQuantity. 
ddhub:MassGradientPerLengthDrillingQuantity a owl:Class; 
                                            rdfs:comment """A mass gradient per length is the first derivative of a mass compared to a distance: $\\frac{dm}{ds}$, where $m$ is a mass and $s$ is a distance.
The dimension of mass gradient per length is:
$$[ML^{-1}]$$.
The SI unit for **mass gradient per length** is: kilogram per metre with the associated unit label $\\frac{kg}{m}$
The meaningful precision of mass gradient per length in the drilling context is typically: 0.05 kg/m
"""@EN; 
                                            rdfs:subClassOf ddhub:MeasurableQuantity. 
ddhub:MassGradientPerLengthQuantity a owl:Class; 
                                    rdfs:comment """A mass gradient per length is the first derivative of a mass compared to a distance: $\\frac{dm}{ds}$, where $m$ is a mass and $s$ is a distance.
The dimension of mass gradient per length is:
$$[ML^{-1}]$$.
The SI unit for **mass gradient per length** is: kilogram per metre with the associated unit label $\\frac{kg}{m}$
"""@EN; 
                                    rdfs:subClassOf ddhub:Quantity. 
ddhub:MassQuantity a owl:Class; 
                   rdfs:comment """Mass can be experimentally defined as a measure of the body's inertia, meaning the resistance to acceleration (change of velocity) when a net force is applied. The object's mass also determines the strength of its gravitational attraction to other bodies.
The dimension of mass is:
$$[M]$$.
The SI unit for **mass** is: kilogram with the associated unit label $kg$
"""@EN; 
                   rdfs:subClassOf ddhub:Quantity. 
ddhub:MassRateDrillingQuantity a owl:Class; 
                               rdfs:comment """A mass rate is the time derivative of a mass: $\\frac{dm}{dt}$, where $m$ is a mass and $t$ is time.
The dimension of mass rate is:
$$[MT^{-1}]$$.
The SI unit for **mass rate** is: kilogram per second with the associated unit label $\\frac{kg}{s}$
The meaningful precision of mass rate in the drilling context is typically: 0.0001 kg/s
"""@EN; 
                               rdfs:subClassOf ddhub:MeasurableQuantity. 
ddhub:MassRateQuantity a owl:Class; 
                       rdfs:comment """A mass rate is the time derivative of a mass: $\\frac{dm}{dt}$, where $m$ is a mass and $t$ is time.
The dimension of mass rate is:
$$[MT^{-1}]$$.
The SI unit for **mass rate** is: kilogram per second with the associated unit label $\\frac{kg}{s}$
"""@EN; 
                       rdfs:subClassOf ddhub:Quantity. 
ddhub:MassTransferBasedDiscretization a owl:Class; 
                                      rdfs:comment """A model can properly estimate values at the level of mass transfer propagation.
"""@EN; 
                                      rdfs:subClassOf ddhub:ModellingDiscretization. 
ddhub:MaterialStrengthQuantity a owl:Class; 
                               rdfs:comment """Material strength refers to the ability of a material to withstand an applied force or load without failing or deforming. It measures how much stress a material can endure before it breaks, bends, or permanently deforms, often categorized into types like tensile, compressive, and shear strength.
The dimension of material strength is:
$$[ML^{-1}T^{-2}]$$.
The SI unit for **material strength** is: pascal with the associated unit label $Pa$
"""@EN; 
                               rdfs:subClassOf ddhub:Quantity. 
ddhub:MathematicalModel a owl:Class; 
                        rdfs:comment """A model for which the state variables do not change with time.
"""@EN; 
                        rdfs:subClassOf ddhub:DWISNoun. 
ddhub:MaxFrequency a owl:DatatypeProperty, owl:FunctionalProperty; 
                   rdfs:comment """
"""@EN; 
                   rdfs:domain ddhub:BandPassFilter; 
                   rdfs:range xsd:double. 
ddhub:MaximumFluctuations a owl:DatatypeProperty, owl:FunctionalProperty; 
                          rdfs:comment """
"""@EN; 
                          rdfs:domain ddhub:Clock; 
                          rdfs:range xsd:double. 
ddhub:MaximumLimit a owl:Class; 
                   rdfs:comment ""@EN; 
                   rdfs:subClassOf ddhub:Limit. 
ddhub:MeanHigherHighWaterVerticalLocation a owl:Class; 
                                          rdfs:comment ""@EN; 
                                          rdfs:subClassOf ddhub:VerticalReferenceLocation. 
ddhub:MeanHighWaterVerticalLocation a owl:Class; 
                                    rdfs:comment ""@EN; 
                                    rdfs:subClassOf ddhub:VerticalReferenceLocation. 
ddhub:MeaningfulPrecision a owl:DatatypeProperty, owl:FunctionalProperty; 
                          rdfs:comment """
"""@EN; 
                          rdfs:domain ddhub:MeasurableQuantity; 
                          rdfs:range xsd:double. 
ddhub:MeanLowerLowWaterVerticalLocation a owl:Class; 
                                        rdfs:comment ""@EN; 
                                        rdfs:subClassOf ddhub:VerticalReferenceLocation. 
ddhub:MeanLowWaterVerticalLocation a owl:Class; 
                                   rdfs:comment ""@EN; 
                                   rdfs:subClassOf ddhub:VerticalReferenceLocation. 
ddhub:MeanSeaLevelVerticalLocation a owl:Class; 
                                   rdfs:comment ""@EN; 
                                   rdfs:subClassOf ddhub:VerticalReferenceLocation. 
ddhub:MeanTideLevelVerticalLocation a owl:Class; 
                                    rdfs:comment ""@EN; 
                                    rdfs:subClassOf ddhub:VerticalReferenceLocation. 
ddhub:MeasurableQuantity a owl:Class; 
                         rdfs:comment """Represents a quantity that allows meaningful comparisons.
Are related by a Quantity via the "IsObservableFrom" relation. 
Context dependent: for example, Fluid density and Equivalent Circulating Density are represented as two different "Measurable quantities", although they both refer to the same base SI quantities. 
"""@EN; 
                         rdfs:subClassOf ddhub:DWISNoun. 
ddhub:MeasurableQuantityUnitAssociation a owl:Class; 
                                        rdfs:comment ""@EN; 
                                        rdfs:subClassOf ddhub:DWISNoun. 
ddhub:MeasuredDepth a owl:Class; 
                    rdfs:comment ""@EN; 
                    rdfs:subClassOf ddhub:PrototypeData. 
ddhub:MeasuredDepthToTrueVerticalDepthTransformation a owl:Class; 
                                                     rdfs:comment ""@EN; 
                                                     rdfs:subClassOf ddhub:DirectTransformation. 
ddhub:MeasuredDepthTranslation a owl:Class; 
                               rdfs:comment ""@EN; 
                               rdfs:subClassOf ddhub:DirectTransformation. 
ddhub:Measurement a owl:Class; 
                  rdfs:comment """The noun Measurement represents individuals that are measured by some instrument and which value can be compared with another measurement.
"""@EN; 
                  rdfs:subClassOf ddhub:PhysicalData. 
ddhub:MeasurementDevice a owl:Class; 
                        rdfs:comment """Denotes a physical sensor
"""@EN; 
                        rdfs:subClassOf ddhub:DataFlowNode. 
ddhub:MeasurementIndex a owl:DatatypeProperty, owl:FunctionalProperty; 
                       rdfs:comment """
"""@EN; 
                       rdfs:domain ddhub:EndPointMapping; 
                       rdfs:range xsd:int. 
ddhub:MeasurementWhileDrillingTools a owl:Class; 
                                    rdfs:comment ""@EN; 
                                    rdfs:subClassOf ddhub:LoggingEquipment. 
ddhub:MechanicalBlock a owl:Class; 
                      rdfs:comment ""@EN; 
                      rdfs:subClassOf ddhub:HoistingSystem. 
ddhub:MechanicalDrawworks a owl:Class; 
                          rdfs:comment ""@EN; 
                          rdfs:subClassOf ddhub:Drawworks. 
ddhub:MechanicalElementState a owl:Class; 
                             rdfs:comment ""@EN; 
                             rdfs:subClassOf ddhub:DWISNoun. 
ddhub:MechanicalJar a owl:Class; 
                    rdfs:comment ""@EN; 
                    rdfs:subClassOf ddhub:JarringAssembly. 
ddhub:MechanicalLogicalElement a owl:Class; 
                               rdfs:comment ""@EN; 
                               rdfs:subClassOf ddhub:DWISNoun. 
ddhub:MechanicallyActiveState a owl:Class; 
                              rdfs:comment ""@EN; 
                              rdfs:subClassOf ddhub:MechanicalElementState. 
ddhub:MechanicallyClosedState a owl:Class; 
                              rdfs:comment ""@EN; 
                              rdfs:subClassOf ddhub:MechanicalElementState. 
ddhub:MechanicallyConnectedState a owl:Class; 
                                 rdfs:comment ""@EN; 
                                 rdfs:subClassOf ddhub:MechanicalElementState. 
ddhub:MechanicallyInactiveState a owl:Class; 
                                rdfs:comment ""@EN; 
                                rdfs:subClassOf ddhub:MechanicalElementState. 
ddhub:MechanicallyOpenState a owl:Class; 
                            rdfs:comment ""@EN; 
                            rdfs:subClassOf ddhub:MechanicalElementState. 
ddhub:MechanicalSoftModel a owl:Class; 
                          rdfs:comment """An infinitively soft model assumes that the drill-stem deforms without any resistance when compressive loads are applied.
"""@EN; 
                          rdfs:subClassOf ddhub:MechanicalStiffnessType. 
ddhub:MechanicalSpecificEnergy a owl:Class; 
                               rdfs:comment ""@EN; 
                               rdfs:subClassOf ddhub:PrototypeData. 
ddhub:MechanicalStiffModel a owl:Class; 
                           rdfs:comment """A stiff mechanical model considers that the drill-stem can deform laterally when put in compression.
"""@EN; 
                           rdfs:subClassOf ddhub:MechanicalStiffnessType. 
ddhub:MechanicalStiffModelAssumedContacts a owl:Class; 
                                          rdfs:comment """Such a stiff mechanical model presuposes the position of the contact points.
"""@EN; 
                                          rdfs:subClassOf ddhub:MechanicalStiffModel. 
ddhub:MechanicalStiffModelEstimatedContacts a owl:Class; 
                                            rdfs:comment """Such a stiff mechanical model estimates the position of the contact points.
"""@EN; 
                                            rdfs:subClassOf ddhub:MechanicalStiffModel. 
ddhub:MechanicalStiffnessType a owl:Class; 
                              rdfs:comment """A description of how the drill-stem stiffness is modelled.
"""@EN; 
                              rdfs:subClassOf ddhub:DWISNoun. 
ddhub:MechanicsAndVibrationTools a owl:Class; 
                                 rdfs:comment ""@EN; 
                                 rdfs:subClassOf ddhub:MeasurementWhileDrillingTools. 
ddhub:Melon a owl:Class; 
            rdfs:comment ""@EN; 
            rdfs:subClassOf ddhub:BladeShape. 
ddhub:MillCasingCutting a owl:Class; 
                        rdfs:comment ""@EN; 
                        rdfs:subClassOf ddhub:CasingMillingTools. 
ddhub:MillDress a owl:Class; 
                rdfs:comment ""@EN; 
                rdfs:subClassOf ddhub:CasingMillingTools. 
ddhub:MillFlatBottom a owl:Class; 
                     rdfs:comment ""@EN; 
                     rdfs:subClassOf ddhub:CasingMillingTools. 
ddhub:MillHollow a owl:Class; 
                 rdfs:comment ""@EN; 
                 rdfs:subClassOf ddhub:CasingMillingTools. 
ddhub:MillPackerPickerAssembly a owl:Class; 
                               rdfs:comment ""@EN; 
                               rdfs:subClassOf ddhub:CasingMillingTools. 
ddhub:MillPilot a owl:Class; 
                rdfs:comment ""@EN; 
                rdfs:subClassOf ddhub:CasingMillingTools. 
ddhub:MillPolish a owl:Class; 
                 rdfs:comment ""@EN; 
                 rdfs:subClassOf ddhub:CasingMillingTools. 
ddhub:MillSection a owl:Class; 
                  rdfs:comment ""@EN; 
                  rdfs:subClassOf ddhub:CasingMillingTools. 
ddhub:MillTaper a owl:Class; 
                rdfs:comment ""@EN; 
                rdfs:subClassOf ddhub:CasingMillingTools. 
ddhub:Milltooth a owl:Class; 
                rdfs:comment ""@EN; 
                rdfs:subClassOf ddhub:RollingCutter. 
ddhub:MillWashover a owl:Class; 
                   rdfs:comment ""@EN; 
                   rdfs:subClassOf ddhub:CasingMillingTools. 
ddhub:MillWatermelon a owl:Class; 
                     rdfs:comment ""@EN; 
                     rdfs:subClassOf ddhub:CasingMillingTools. 
ddhub:MinDrillHeightVerticalLocation a owl:Class; 
                                     rdfs:comment ""@EN; 
                                     rdfs:subClassOf ddhub:VerticalReferenceLocation. 
ddhub:MinFrequency a owl:DatatypeProperty, owl:FunctionalProperty; 
                   rdfs:comment """
"""@EN; 
                   rdfs:domain ddhub:BandPassFilter; 
                   rdfs:range xsd:double. 
ddhub:MinimumHorizontalStress a owl:Class; 
                              rdfs:comment ""@EN; 
                              rdfs:subClassOf ddhub:PrototypeData. 
ddhub:MinimumHorizontalStressGradient a owl:Class; 
                                      rdfs:comment ""@EN; 
                                      rdfs:subClassOf ddhub:PrototypeData. 
ddhub:MinimumLimit a owl:Class; 
                   rdfs:comment ""@EN; 
                   rdfs:subClassOf ddhub:Limit. 
ddhub:MinMaxUncertainty a owl:Class; 
                        rdfs:comment """The uncertainty is represented by a uniform probability distribution between a `Min` and a `Max` value.
"""@EN; 
                        rdfs:subClassOf ddhub:SignalUncertainty. 
ddhub:MiscSubs a owl:Class; 
               rdfs:comment ""@EN; 
               rdfs:subClassOf ddhub:DrillString. 
ddhub:MixingTank a owl:Class; 
                 rdfs:comment ""@EN; 
                 rdfs:subClassOf ddhub:MudPits. 
ddhub:Mnemonic a owl:DatatypeProperty, owl:FunctionalProperty; 
               rdfs:comment """
"""@EN; 
               rdfs:domain ddhub:WitsMLTimeBasedLogEndPoint; 
               rdfs:range xsd:string. 
ddhub:ModelledDegreeOfFreedom a owl:Class; 
                              rdfs:comment """In physics and chemistry, a degree of freedom is an independent physical parameter in the formal description of the state of a physical system. A model may account for some or all of the degrees of freedom of the physical system.
"""@EN; 
                              rdfs:subClassOf ddhub:DWISNoun. 
ddhub:ModellingDimensions a owl:Class; 
                          rdfs:comment """The number of dimensions that are accounted by the model
"""@EN; 
                          rdfs:subClassOf ddhub:DWISNoun. 
ddhub:ModellingDiscretization a owl:Class; 
                              rdfs:comment """A characteristic of the discretization made by the model.
"""@EN; 
                              rdfs:subClassOf ddhub:DWISNoun. 
ddhub:ModelType a owl:Class; 
                rdfs:comment ""@EN; 
                rdfs:subClassOf ddhub:DWISNoun. 
ddhub:MooringLines a owl:Class; 
                   rdfs:comment ""@EN; 
                   rdfs:subClassOf ddhub:MooringSystem. 
ddhub:MooringSystem a owl:Class; 
                    rdfs:comment ""@EN; 
                    rdfs:subClassOf ddhub:MarineSystem. 
ddhub:MotionType a owl:Class; 
                 rdfs:comment ""@EN; 
                 rdfs:subClassOf ddhub:DWISNoun. 
ddhub:Mousehole a owl:Class; 
                rdfs:comment ""@EN; 
                rdfs:subClassOf ddhub:DrillFloorStructure. 
ddhub:MovingAverage a owl:Class; 
                    rdfs:comment ""@EN; 
                    rdfs:subClassOf ddhub:Filter. 
ddhub:MovingMax a owl:Class; 
                rdfs:comment ""@EN; 
                rdfs:subClassOf ddhub:Filter. 
ddhub:MovingMin a owl:Class; 
                rdfs:comment ""@EN; 
                rdfs:subClassOf ddhub:Filter. 
ddhub:MovingStandardDeviation a owl:Class; 
                              rdfs:comment ""@EN; 
                              rdfs:subClassOf ddhub:Filter. 
ddhub:MPDAlternateFlowPath a owl:Class; 
                           rdfs:comment ""@EN; 
                           rdfs:subClassOf ddhub:TopsideHydraulicNetwork. 
ddhub:MpdChoke a owl:Class; 
               rdfs:comment ""@EN; 
               rdfs:subClassOf ddhub:WellControlSystem. 
ddhub:MPDChokeOpening a owl:Class; 
                      rdfs:comment ""@EN; 
                      rdfs:subClassOf ddhub:PrototypeData. 
ddhub:MPDChokePressure a owl:Class; 
                       rdfs:comment ""@EN; 
                       rdfs:subClassOf ddhub:PrototypeData. 
ddhub:MPDMainFlowPath a owl:Class; 
                      rdfs:comment ""@EN; 
                      rdfs:subClassOf ddhub:TopsideHydraulicNetwork. 
ddhub:MPDPumpFlowRate a owl:Class; 
                      rdfs:comment ""@EN; 
                      rdfs:subClassOf ddhub:PrototypeData. 
ddhub:MPDPumpRate a owl:Class; 
                  rdfs:comment ""@EN; 
                  rdfs:subClassOf ddhub:PrototypeData. 
ddhub:MudHose a owl:Class; 
              rdfs:comment ""@EN; 
              rdfs:subClassOf ddhub:MudLines. 
ddhub:MudLines a owl:Class; 
               rdfs:comment ""@EN; 
               rdfs:subClassOf ddhub:CirculationSystem. 
ddhub:MudLineSystem a owl:Class; 
                    rdfs:comment ""@EN; 
                    rdfs:subClassOf ddhub:MarineSystem. 
ddhub:MudLoggingEquipment a owl:Class; 
                          rdfs:comment ""@EN; 
                          rdfs:subClassOf ddhub:RigEquipment. 
ddhub:MudLubeBearing a owl:Class; 
                     rdfs:comment ""@EN; 
                     rdfs:subClassOf ddhub:DownholeMotor. 
ddhub:MudMixing a owl:Class; 
                rdfs:comment ""@EN; 
                rdfs:subClassOf ddhub:HydraulicJunction. 
ddhub:MudPits a owl:Class; 
              rdfs:comment ""@EN; 
              rdfs:subClassOf ddhub:CirculationSystem. 
ddhub:MudPulse a owl:Class; 
               rdfs:comment ""@EN; 
               rdfs:subClassOf ddhub:EquipmentTelemetry. 
ddhub:MudPulseTelemetry a owl:Class; 
                        rdfs:comment """A method that allows transfer of downhole data to the surface via pressure pulses sent trough the drilling fluid.
"""@EN; 
                        rdfs:subClassOf ddhub:DownHoleTelemetry. 
ddhub:MudPump a owl:Class; 
              rdfs:comment ""@EN; 
              rdfs:subClassOf ddhub:CirculationSystem. 
ddhub:MudPumpsControlSystem a owl:Class; 
                            rdfs:comment ""@EN; 
                            rdfs:subClassOf ddhub:ControlSystem. 
ddhub:MudStandpipe a owl:Class; 
                   rdfs:comment ""@EN; 
                   rdfs:subClassOf ddhub:MudLines. 
ddhub:MudStandpipeManifold a owl:Class; 
                           rdfs:comment ""@EN; 
                           rdfs:subClassOf ddhub:MudLines. 
ddhub:N a owl:DatatypeProperty, owl:FunctionalProperty; 
        rdfs:comment """Amount of substance exponent.
SI Unit: Mole (N)
"""@EN; 
        rdfs:domain ddhub:Quantity; 
        rdfs:range xsd:double. 
ddhub:NearBit a owl:Class; 
              rdfs:comment ""@EN; 
              rdfs:subClassOf ddhub:Stabilizers. 
ddhub:NearbitReamers a owl:Class; 
                     rdfs:comment ""@EN; 
                     rdfs:subClassOf ddhub:Reamers. 
ddhub:NearBitVibrationDampers a owl:Class; 
                              rdfs:comment ""@EN; 
                              rdfs:subClassOf ddhub:ActiveVibrationTools. 
ddhub:NetworkSynchronizationLatencyAverage a owl:DatatypeProperty, owl:FunctionalProperty; 
                                           rdfs:comment """
"""@EN; 
                                           rdfs:domain ddhub:Clock; 
                                           rdfs:range xsd:double. 
ddhub:NetworkSynchronizationLatencyStandardDeviation a owl:DatatypeProperty, owl:FunctionalProperty; 
                                                     rdfs:comment """
"""@EN; 
                                                     rdfs:domain ddhub:Clock; 
                                                     rdfs:range xsd:double. 
ddhub:Nonmagnetic a owl:Class; 
                  rdfs:comment ""@EN; 
                  rdfs:subClassOf ddhub:Stabilizers. 
ddhub:NonmagneticCollars a owl:Class; 
                         rdfs:comment ""@EN; 
                         rdfs:subClassOf ddhub:DrillString. 
ddhub:Nonrotating a owl:Class; 
                  rdfs:comment ""@EN; 
                  rdfs:subClassOf ddhub:Stabilizers. 
ddhub:NormalizedDataType a owl:Class; 
                         rdfs:comment """between 0 and 1
"""@EN; 
                         rdfs:subClassOf ddhub:ContinuousDataType. 
ddhub:NorthEastFrame a owl:Class; 
                     rdfs:comment ""@EN; 
                     rdfs:subClassOf ddhub:CartesianTwoDimensionalReferenceFrame. 
ddhub:NorthEastTVDFrame a owl:Class; 
                        rdfs:comment ""@EN; 
                        rdfs:subClassOf ddhub:CartesianThreeDimensionalReferenceFrame. 
ddhub:NozzleDiameterDrillingQuantity a owl:Class; 
                                     rdfs:comment """Length is a measure of distance.
The dimension of length is:
$$[L]$$.
The SI unit for **length** is: metre with the associated unit label $m$
The meaningful precision of small length is typically: 0.0001 m
The meaningful precision of nozzle diameter in the drilling context is typically: 0.0001 m
"""@EN; 
                                     rdfs:subClassOf ddhub:MeasurableQuantity. 
ddhub:Nozzles a owl:Class; 
              rdfs:comment ""@EN; 
              rdfs:subClassOf ddhub:DrillingBit. 
ddhub:NumberOfItems a owl:DatatypeProperty, owl:FunctionalProperty; 
                    rdfs:comment """
"""@EN; 
                    rdfs:domain ddhub:NumberOfItemsRangeExtraction; 
                    rdfs:range xsd:int. 
ddhub:NumberOfItemsRangeExtraction a owl:Class; 
                                   rdfs:comment ""@EN; 
                                   rdfs:subClassOf ddhub:RangeExtraction. 
ddhub:NumberOfRepeaters a owl:DatatypeProperty, owl:FunctionalProperty; 
                        rdfs:comment """
"""@EN; 
                        rdfs:domain ddhub:Telemetry; 
                        rdfs:range xsd:int. 
ddhub:NumberOfSampleMovingAverage a owl:Class; 
                                  rdfs:comment ""@EN; 
                                  rdfs:subClassOf ddhub:MovingAverage. 
ddhub:NumberOfSamples a owl:DatatypeProperty, owl:FunctionalProperty; 
                      rdfs:comment """
"""@EN; 
                      rdfs:domain ddhub:NumberOfSampleMovingAverage; 
                      rdfs:range xsd:int. 
ddhub:OilBasedMudObm a owl:Class; 
                     rdfs:comment ""@EN; 
                     rdfs:subClassOf ddhub:DrillingFluid. 
ddhub:OilBearing a owl:Class; 
                 rdfs:comment ""@EN; 
                 rdfs:subClassOf ddhub:DownholeMotor. 
ddhub:Omega a owl:DatatypeProperty, owl:FunctionalProperty; 
            rdfs:comment """solid angle exponent.
SI Unit: steradian (sr)
"""@EN; 
            rdfs:domain ddhub:Quantity; 
            rdfs:range xsd:double. 
ddhub:OneDimensionalCartesianReferenceFrame a owl:Class; 
                                            rdfs:comment ""@EN; 
                                            rdfs:subClassOf ddhub:OneDimensionalReferenceFrame. 
ddhub:OneDimensionalCurviLinearReferenceFrame a owl:Class; 
                                              rdfs:comment ""@EN; 
                                              rdfs:subClassOf ddhub:OneDimensionalReferenceFrame. 
ddhub:OneDimensionalReferenceFrame a owl:Class; 
                                   rdfs:comment ""@EN; 
                                   rdfs:subClassOf ddhub:ReferenceFrame. 
ddhub:OneDModelling a owl:Class; 
                    rdfs:comment """The model only accounts for one dimension
"""@EN; 
                    rdfs:subClassOf ddhub:ModellingDimensions. 
ddhub:OpenChannel a owl:Class; 
                  rdfs:comment ""@EN; 
                  rdfs:subClassOf ddhub:HydraulicBranch. 
ddhub:OpenHole a owl:Class; 
               rdfs:comment ""@EN; 
               rdfs:subClassOf ddhub:Pipe. 
ddhub:OpenholeTools a owl:Class; 
                    rdfs:comment ""@EN; 
                    rdfs:subClassOf ddhub:WirelineLoggingTools. 
ddhub:OperatingCompany a owl:Class; 
                       rdfs:comment """An operating company is an entity that holds the rights to explore, develop, and produce hydrocarbon resources from a particular oil or gas field or lease
"""@EN; 
                       rdfs:subClassOf ddhub:DataProvider. 
ddhub:OperationalPlan a owl:Class; 
                      rdfs:comment ""@EN; 
                      rdfs:subClassOf ddhub:Plan. 
ddhub:OuterBarrel a owl:Class; 
                  rdfs:comment ""@EN; 
                  rdfs:subClassOf ddhub:CoringTool. 
ddhub:OverburdenPressure a owl:Class; 
                         rdfs:comment ""@EN; 
                         rdfs:subClassOf ddhub:PrototypeData. 
ddhub:OverburdenPressureGradient a owl:Class; 
                                 rdfs:comment ""@EN; 
                                 rdfs:subClassOf ddhub:PrototypeData. 
ddhub:Overpull a owl:Class; 
               rdfs:comment ""@EN; 
               rdfs:subClassOf ddhub:DrillingIncident. 
ddhub:Overshot a owl:Class; 
               rdfs:comment ""@EN; 
               rdfs:subClassOf ddhub:FishingTools. 
ddhub:OverTorque a owl:Class; 
                 rdfs:comment ""@EN; 
                 rdfs:subClassOf ddhub:DrillingIncident. 
ddhub:Pdc a owl:Class; 
          rdfs:comment ""@EN; 
          rdfs:subClassOf ddhub:FixedCutter. 
ddhub:PdcCore a owl:Class; 
              rdfs:comment ""@EN; 
              rdfs:subClassOf ddhub:FixedCutter. 
ddhub:PerforatingGuns a owl:Class; 
                      rdfs:comment ""@EN; 
                      rdfs:subClassOf ddhub:CasingEquipment. 
ddhub:PeristalticMudPump a owl:Class; 
                         rdfs:comment ""@EN; 
                         rdfs:subClassOf ddhub:MudPump. 
ddhub:PhysicalData a owl:Class; 
                   rdfs:comment ""@EN; 
                   rdfs:subClassOf ddhub:DrillingDataPoint. 
ddhub:PhysicalState a owl:Class; 
                    rdfs:comment ""@EN; 
                    rdfs:subClassOf ddhub:ComputedState. 
ddhub:Pin a owl:Class; 
          rdfs:comment ""@EN; 
          rdfs:subClassOf ddhub:Connection. 
ddhub:PinDown a owl:Class; 
              rdfs:comment ""@EN; 
              rdfs:subClassOf ddhub:TubularConfiguration. 
ddhub:Pinpin a owl:Class; 
             rdfs:comment ""@EN; 
             rdfs:subClassOf ddhub:TubularConfiguration. 
ddhub:PinUp a owl:Class; 
            rdfs:comment ""@EN; 
            rdfs:subClassOf ddhub:TubularConfiguration. 
ddhub:Pipe a owl:Class; 
           rdfs:comment ""@EN; 
           rdfs:subClassOf ddhub:HydraulicBranch. 
ddhub:PipeRam a owl:Class; 
              rdfs:comment ""@EN; 
              rdfs:subClassOf ddhub:BopElement. 
ddhub:PipeWashout a owl:Class; 
                  rdfs:comment ""@EN; 
                  rdfs:subClassOf ddhub:DrillingIncident. 
ddhub:PipeWashoutLocation a owl:Class; 
                          rdfs:comment ""@EN; 
                          rdfs:subClassOf ddhub:AbscissaReferenceLocation. 
ddhub:Piston a owl:Class; 
             rdfs:comment ""@EN; 
             rdfs:subClassOf ddhub:PistonMudPump. 
ddhub:PistonMudPump a owl:Class; 
                    rdfs:comment ""@EN; 
                    rdfs:subClassOf ddhub:MudPump. 
ddhub:Plan a owl:Class; 
           rdfs:comment ""@EN; 
           rdfs:subClassOf ddhub:DataFlowNode. 
ddhub:PlaneAngleDrillingQuantity a owl:Class; 
                                 rdfs:comment """A plane angle is the angle formed between two intersecting lines or planes in a two-dimensional or three-dimensional space.
The dimension of plane angle is:
$$[{\\theta}]$$.
The SI unit for **plane angle** is: radian with the associated unit label $rad$
The meaningful precision of plane angle in the drilling context is typically: 0.00017453292519943296 rad
"""@EN; 
                                 rdfs:subClassOf ddhub:MeasurableQuantity. 
ddhub:PlaneAngleQuantity a owl:Class; 
                         rdfs:comment """A plane angle is the angle formed between two intersecting lines or planes in a two-dimensional or three-dimensional space.
The dimension of plane angle is:
$$[{\\theta}]$$.
The SI unit for **plane angle** is: radian with the associated unit label $rad$
"""@EN; 
                         rdfs:subClassOf ddhub:Quantity. 
ddhub:Plugged a owl:Class; 
              rdfs:comment ""@EN; 
              rdfs:subClassOf ddhub:DrillingIncident. 
ddhub:Plugs a owl:Class; 
            rdfs:comment ""@EN; 
            rdfs:subClassOf ddhub:CasingEquipment. 
ddhub:PlungerFloatValvesF a owl:Class; 
                          rdfs:comment ""@EN; 
                          rdfs:subClassOf ddhub:FloatValveNonreturnValve. 
ddhub:PlungerMudPump a owl:Class; 
                     rdfs:comment ""@EN; 
                     rdfs:subClassOf ddhub:MudPump. 
ddhub:PneumaticSlips a owl:Class; 
                     rdfs:comment ""@EN; 
                     rdfs:subClassOf ddhub:RotarySlips. 
ddhub:Pointthebit a owl:Class; 
                  rdfs:comment ""@EN; 
                  rdfs:subClassOf ddhub:RotarySteerableSystems. 
ddhub:PolarReferenceFrame a owl:Class; 
                          rdfs:comment ""@EN; 
                          rdfs:subClassOf ddhub:TwoDimensionalReferenceFrame. 
ddhub:PorePressure a owl:Class; 
                   rdfs:comment ""@EN; 
                   rdfs:subClassOf ddhub:PrototypeData. 
ddhub:PorePressureGradient a owl:Class; 
                           rdfs:comment ""@EN; 
                           rdfs:subClassOf ddhub:PrototypeData. 
ddhub:PorosityQuantity a owl:Class; 
                       rdfs:comment """A proportion is the ratio of two quantities with the same dimension. It represents how one quantity compares to another in relative terms.
A proportion is dimensionless:
Porosity is the measure of the void spaces or pores within a material, expressed as a fraction or percentage of the total volume.
The meaningful precision of porosity is typically: 0.001 
"""@EN; 
                       rdfs:subClassOf ddhub:MeasurableQuantity. 
ddhub:PorousMediumPermeabilityDrillingQuantity a owl:Class; 
                                               rdfs:comment """The permeability is a property of porous medium that quantifies its ability to allow fluids to pass through it.
The dimension of porous medium permeability is:
$$[L^{2}]$$.
The SI unit for **porous medium permeability** is: square metre with the associated unit label $m^{2}$
The meaningful precision of permeability in the drilling context is typically: 1E-10 m²
"""@EN; 
                                               rdfs:subClassOf ddhub:MeasurableQuantity. 
ddhub:PorousMediumPermeabilityQuantity a owl:Class; 
                                       rdfs:comment """The permeability is a property of porous medium that quantifies its ability to allow fluids to pass through it.
The dimension of porous medium permeability is:
$$[L^{2}]$$.
The SI unit for **porous medium permeability** is: square metre with the associated unit label $m^{2}$
"""@EN; 
                                       rdfs:subClassOf ddhub:Quantity. 
ddhub:PortedPlungerValvesFa a owl:Class; 
                            rdfs:comment ""@EN; 
                            rdfs:subClassOf ddhub:FloatValveNonreturnValve. 
ddhub:PositionDrillingQuantity a owl:Class; 
                               rdfs:comment """Length is a measure of distance.
The dimension of length is:
$$[L]$$.
The SI unit for **length** is: metre with the associated unit label $m$
The meaningful precision of position in the drilling context is typically: 0.01 m
"""@EN; 
                               rdfs:subClassOf ddhub:MeasurableQuantity. 
ddhub:PositionReferenceLocation a owl:Class; 
                                rdfs:comment ""@EN; 
                                rdfs:subClassOf ddhub:Location. 
ddhub:PositiveDisplacementMotor a owl:Class; 
                                rdfs:comment ""@EN; 
                                rdfs:subClassOf ddhub:DownholeMotor. 
ddhub:PostiveUpward a owl:DatatypeProperty, owl:FunctionalProperty; 
                    rdfs:comment """
"""@EN; 
                    rdfs:domain ddhub:OneDimensionalReferenceFrame; 
                    rdfs:range xsd:bool. 
ddhub:PotableWater a owl:Class; 
                   rdfs:comment ""@EN; 
                   rdfs:subClassOf ddhub:DrillingFluid. 
ddhub:PowerDrillingQuantity a owl:Class; 
                            rdfs:comment """Power is the rate at which work is done or energy is transferred over time.
The dimension of power is:
$$[L^{2}MT^{-3}]$$.
The SI unit for **power** is: watt with the associated unit label $W$
The meaningful precision of power in the drilling context is typically: 0.1 W
"""@EN; 
                            rdfs:subClassOf ddhub:MeasurableQuantity. 
ddhub:PowerGenerationSystem a owl:Class; 
                            rdfs:comment ""@EN; 
                            rdfs:subClassOf ddhub:RigEquipment. 
ddhub:PowerGenerators a owl:Class; 
                      rdfs:comment ""@EN; 
                      rdfs:subClassOf ddhub:PowerGenerationSystem. 
ddhub:PowerPipeTongs a owl:Class; 
                     rdfs:comment ""@EN; 
                     rdfs:subClassOf ddhub:DrillPipeTongs. 
ddhub:PowerQuantity a owl:Class; 
                    rdfs:comment """Power is the rate at which work is done or energy is transferred over time.
The dimension of power is:
$$[L^{2}MT^{-3}]$$.
The SI unit for **power** is: watt with the associated unit label $W$
"""@EN; 
                    rdfs:subClassOf ddhub:Quantity. 
ddhub:PowerScrSystem a owl:Class; 
                     rdfs:comment ""@EN; 
                     rdfs:subClassOf ddhub:PowerGenerationSystem. 
ddhub:PowerSlips a owl:Class; 
                 rdfs:comment ""@EN; 
                 rdfs:subClassOf ddhub:RotarySlips. 
ddhub:PowerSupply a owl:Class; 
                  rdfs:comment ""@EN; 
                  rdfs:subClassOf ddhub:CoiledTubingEquipment. 
ddhub:PowerSystems a owl:Class; 
                   rdfs:comment ""@EN; 
                   rdfs:subClassOf ddhub:LoggingEquipment. 
ddhub:Precision a owl:DatatypeProperty, owl:FunctionalProperty; 
                rdfs:comment """The standard deviation of the repetitive error component of the uncertainty of the sensor. The assumed mean value of the attached Gaussian distribution is the measured value. The value is expected to be in the same physical quantity as the sensor value.
"""@EN; 
                rdfs:domain ddhub:SensorUncertainty; 
                rdfs:range xsd:double. 
ddhub:PressureDrillingQuantity a owl:Class; 
                               rdfs:comment """Pressure is the force applied per unit area on a surface.
The dimension of pressure is:
$$[ML^{-1}T^{-2}]$$.
The SI unit for **pressure** is: pascal with the associated unit label $Pa$
The meaningful precision of pressure in the drilling context is typically: 10000 Pa
"""@EN; 
                               rdfs:subClassOf ddhub:MeasurableQuantity. 
ddhub:PressureGradientPerLengthDrillingQuantity a owl:Class; 
                                                rdfs:comment """A pressure gradient per length is the first derivative of a pressure compared to a distance: $\\frac{dp}{ds}$, where $p$ is a pressure and $s$ is a distance.
The dimension of pressure gradient per length is:
$$[ML^{-2}T^{-2}]$$.
The SI unit for **pressure gradient per length** is: pascal per metre with the associated unit label $\\frac{Pa}{m}$
The meaningful precision of pressure gradient per length in the drilling context is typically: 10000 Pa/m
"""@EN; 
                                                rdfs:subClassOf ddhub:MeasurableQuantity. 
ddhub:PressureGradientPerLengthQuantity a owl:Class; 
                                        rdfs:comment """A pressure gradient per length is the first derivative of a pressure compared to a distance: $\\frac{dp}{ds}$, where $p$ is a pressure and $s$ is a distance.
The dimension of pressure gradient per length is:
$$[ML^{-2}T^{-2}]$$.
The SI unit for **pressure gradient per length** is: pascal per metre with the associated unit label $\\frac{Pa}{m}$
"""@EN; 
                                        rdfs:subClassOf ddhub:Quantity. 
ddhub:PressureLoggingTools a owl:Class; 
                           rdfs:comment ""@EN; 
                           rdfs:subClassOf ddhub:WirelineLoggingTools. 
ddhub:PressureLossConstantDrillingQuantity a owl:Class; 
                                           rdfs:comment """The pressure loss constant is a parameter used to quantify the resistance to flow in a system, such as a pipe or more complex tubulars, which leads to a reduction in pressure. It helps in calculating the pressure drop due to friction or other factors in fluid dynamics.
The dimension of pressure loss constant is:
$$[L^{4}]$$.
The SI unit for **pressure loss constant** is: pressure loss constant SI with the associated unit label $(\\frac{m^{3}}{s})^{2} \\cdot \\frac{(\\frac{kg}{m^{3}})}{Pa}$
The meaningful precision of pressure loss constant in the drilling context is typically: 0.1 (m³/s)²•(kg/m³)/Pa
"""@EN; 
                                           rdfs:subClassOf ddhub:MeasurableQuantity. 
ddhub:PressureLossConstantQuantity a owl:Class; 
                                   rdfs:comment """The pressure loss constant is a parameter used to quantify the resistance to flow in a system, such as a pipe or more complex tubulars, which leads to a reduction in pressure. It helps in calculating the pressure drop due to friction or other factors in fluid dynamics.
The dimension of pressure loss constant is:
$$[L^{4}]$$.
The SI unit for **pressure loss constant** is: pressure loss constant SI with the associated unit label $(\\frac{m^{3}}{s})^{2} \\cdot \\frac{(\\frac{kg}{m^{3}})}{Pa}$
"""@EN; 
                                   rdfs:subClassOf ddhub:Quantity. 
ddhub:PressureQuantity a owl:Class; 
                       rdfs:comment """Pressure is the force applied per unit area on a surface.
The dimension of pressure is:
$$[ML^{-1}T^{-2}]$$.
The SI unit for **pressure** is: pascal with the associated unit label $Pa$
"""@EN; 
                       rdfs:subClassOf ddhub:Quantity. 
ddhub:PressureReference a owl:Class; 
                        rdfs:comment ""@EN; 
                        rdfs:subClassOf ddhub:DWISNoun. 
ddhub:PressureToEquivalentDensityTransformation a owl:Class; 
                                                rdfs:comment ""@EN; 
                                                rdfs:subClassOf ddhub:DirectTransformation. 
ddhub:PressureToForceTransformation a owl:Class; 
                                    rdfs:comment ""@EN; 
                                    rdfs:subClassOf ddhub:DirectTransformation. 
ddhub:ProceduralState a owl:Class; 
                      rdfs:comment ""@EN; 
                      rdfs:subClassOf ddhub:ComputedState. 
ddhub:ProcedureFunction a owl:Class; 
                        rdfs:comment """A `ProcedureFunction` is a `RunnableFunction` that executes a finites state automaton, i.e., a graph of
transitions between states. It should be noted that a `ProcedureFunction` may use control algorithms while being in one
state or when transiting from state to state. An example of `ProcedureFunction` is a friction test. A friction test has
at least three states: rotation off bottom, pick-up without rotation, slack-off without rotation. The transitions 
between the different states may depend on the implementation. Each of those states uses a controller, one that controls
the rotational speed and one that controls the axial speed.
"""@EN; 
                        rdfs:subClassOf ddhub:RunnableFunction. 
ddhub:ProcessData a owl:Class; 
                  rdfs:comment ""@EN; 
                  rdfs:subClassOf ddhub:DrillingDataPoint. 
ddhub:ProcessState a owl:Class; 
                   rdfs:comment ""@EN; 
                   rdfs:subClassOf ddhub:ComputedState. 
ddhub:ProductionTools a owl:Class; 
                      rdfs:comment ""@EN; 
                      rdfs:subClassOf ddhub:WirelineLoggingTools. 
ddhub:ProportionError a owl:DatatypeProperty, owl:FunctionalProperty; 
                      rdfs:comment """The proportion error on the signal. The value is expected to be a dimensionless physical quantity between 0 and 1 in SI unit. This proportion is applied to the `Fullscale` to obtain the standard deviation of the Gaussian probability distribution that describes the uncertainty of the signal. The mean value of that Gaussian distribution is the signal value.
"""@EN; 
                      rdfs:domain ddhub:FullScaleUncertainty; 
                      rdfs:range xsd:double. 
ddhub:ProportionQuantity a owl:Class; 
                         rdfs:comment """A proportion is the ratio of two quantities with the same dimension. It represents how one quantity compares to another in relative terms.
A proportion is dimensionless:
"""@EN; 
                         rdfs:subClassOf ddhub:Quantity. 
ddhub:ProportionSmallQuantity a owl:Class; 
                              rdfs:comment """A proportion is the ratio of two quantities with the same dimension. It represents how one quantity compares to another in relative terms.
A proportion is dimensionless:
The meaningful precision of small proportion is typically: 1E-08 
"""@EN; 
                              rdfs:subClassOf ddhub:MeasurableQuantity. 
ddhub:ProportionStandardQuantity a owl:Class; 
                                 rdfs:comment """A proportion is the ratio of two quantities with the same dimension. It represents how one quantity compares to another in relative terms.
A proportion is dimensionless:
The meaningful precision of a standard proportion is typically: 0.001 
"""@EN; 
                                 rdfs:subClassOf ddhub:MeasurableQuantity. 
ddhub:ProtectionFunction a owl:Class; 
                         rdfs:comment """A `ProtectionFunction` is an `ActivableFunction`. It must be activated to have an effect, but the effect
is to protect the drilling process, either by protecting the inputs to the drilling machines to avoid generating 
a drilling incident, or to detect an abnormal drilling process state and react to the situation.
detected.
"""@EN; 
                         rdfs:subClassOf ddhub:ActivableFunction. 
ddhub:PrototypeData a owl:Class; 
                    rdfs:comment ""@EN; 
                    rdfs:subClassOf ddhub:DrillingDataPoint. 
ddhub:ProviderName a owl:DatatypeProperty, owl:FunctionalProperty; 
                   rdfs:comment """
"""@EN; 
                   rdfs:domain ddhub:DataProvider, ddhub:OperatingCompany, ddhub:ServiceCompany, ddhub:DirectionalServiceCompany, ddhub:DrillingFluidProvider, ddhub:LoggingServiceCompany, ddhub:CementingServiceCompany, ddhub:DataAnalysisServiceCompany, ddhub:DrillingContractor, ddhub:DWISInternalService; 
                   rdfs:range xsd:string. 
ddhub:PulsationDampener a owl:Class; 
                        rdfs:comment ""@EN; 
                        rdfs:subClassOf ddhub:PistonMudPump. 
ddhub:PumpRate a owl:Class; 
               rdfs:comment ""@EN; 
               rdfs:subClassOf ddhub:PrototypeData. 
ddhub:PupJoints a owl:Class; 
                rdfs:comment ""@EN; 
                rdfs:subClassOf ddhub:DrillString. 
ddhub:Pushthebit a owl:Class; 
                 rdfs:comment ""@EN; 
                 rdfs:subClassOf ddhub:RotarySteerableSystems. 
ddhub:PwdPressure a owl:Class; 
                  rdfs:comment ""@EN; 
                  rdfs:subClassOf ddhub:MeasurementWhileDrillingTools. 
ddhub:QuadristandDerrick a owl:Class; 
                         rdfs:comment ""@EN; 
                         rdfs:subClassOf ddhub:Derrick. 
ddhub:Quantity a owl:Class; 
               rdfs:comment ""@EN; 
               rdfs:subClassOf ddhub:DWISNoun. 
ddhub:Quill a owl:Class; 
            rdfs:comment ""@EN; 
            rdfs:subClassOf ddhub:TopDrive. 
ddhub:RackAndPinionHoistingSystem a owl:Class; 
                                  rdfs:comment ""@EN; 
                                  rdfs:subClassOf ddhub:HoistingSystem. 
ddhub:RadialModelling a owl:Class; 
                      rdfs:comment """The model accounts for the radial movement of some parts of the physical system.
"""@EN; 
                      rdfs:subClassOf ddhub:LateralModelling. 
ddhub:RamHoistingSystem a owl:Class; 
                        rdfs:comment ""@EN; 
                        rdfs:subClassOf ddhub:HoistingSystem. 
ddhub:RamRig a owl:Class; 
             rdfs:comment ""@EN; 
             rdfs:subClassOf ddhub:Drawworks. 
ddhub:RandomWalkDrillingQuantity a owl:Class; 
                                 rdfs:comment """A random walk is a mathematical concept describing a path consisting of a series of random steps or movements, where each step's direction or magnitude is determined probabilistically. It is used to model various phenomena in fields like physics, finance, and computer science.
The dimension of random walk is:
$$[{\\theta}T^{-0.5}]$$.
The SI unit for **random walk** is: radian per square root second with the associated unit label $\\frac{rad}{\\sqrt{s}}$
The meaningful precision of random walk in the drilling context is typically: 1E-05 rad/√s
"""@EN; 
                                 rdfs:subClassOf ddhub:MeasurableQuantity. 
ddhub:RandomWalkQuantity a owl:Class; 
                         rdfs:comment """A random walk is a mathematical concept describing a path consisting of a series of random steps or movements, where each step's direction or magnitude is determined probabilistically. It is used to model various phenomena in fields like physics, finance, and computer science.
The dimension of random walk is:
$$[{\\theta}T^{-0.5}]$$.
The SI unit for **random walk** is: radian per square root second with the associated unit label $\\frac{rad}{\\sqrt{s}}$
"""@EN; 
                         rdfs:subClassOf ddhub:Quantity. 
ddhub:RangeExtraction a owl:Class; 
                      rdfs:comment ""@EN; 
                      rdfs:subClassOf ddhub:TimeBasedTransformation. 
ddhub:RateOfPenetrationDrillingQuantity a owl:Class; 
                                        rdfs:comment """A velocity is the time derivative of a position or a displacement: $\\frac{dx}{dt}$, where $x$ is a position and $t$ is time.
The dimension of velocity is:
$$[LT^{-1}]$$.
The SI unit for **velocity** is: metre per second with the associated unit label $\\frac{m}{s}$
The meaningful precision of rate of penetration in the drilling context is typically: 2.77778E-05 m/min
"""@EN; 
                                        rdfs:subClassOf ddhub:MeasurableQuantity. 
ddhub:Reamers a owl:Class; 
              rdfs:comment ""@EN; 
              rdfs:subClassOf ddhub:DrillingEquipment. 
ddhub:ReciprocalLengthSurveyInstrumentDrillingQuantity a owl:Class; 
                                                       rdfs:comment """A wave number is the number of wave lengths per unit distance.
The dimension of wave number is:
$$[L^{-1}]$$.
The SI unit for **wave number** is: reciprocal metre with the associated unit label $\\frac{1}{m}$
The meaningful precision of reciprocal length related to survey instrument performance models in the drilling context is typically: 1E-08 1/m
"""@EN; 
                                                       rdfs:subClassOf ddhub:MeasurableQuantity. 
ddhub:Recommendation a owl:Class; 
                     rdfs:comment ""@EN; 
                     rdfs:subClassOf ddhub:ProcessData. 
ddhub:RecommendedMaximum a owl:Class; 
                         rdfs:comment ""@EN; 
                         rdfs:subClassOf ddhub:Recommendation. 
ddhub:RecommendedMinimum a owl:Class; 
                         rdfs:comment ""@EN; 
                         rdfs:subClassOf ddhub:Recommendation. 
ddhub:RecommendedTarget a owl:Class; 
                        rdfs:comment ""@EN; 
                        rdfs:subClassOf ddhub:Recommendation. 
ddhub:RectangularChannel a owl:Class; 
                         rdfs:comment ""@EN; 
                         rdfs:subClassOf ddhub:OpenChannel. 
ddhub:ReferenceFrame a owl:Class; 
                     rdfs:comment """Represents a system of coordinates
"""@EN; 
                     rdfs:subClassOf ddhub:DWISNoun. 
ddhub:RelativePressureReference a owl:Class; 
                                rdfs:comment ""@EN; 
                                rdfs:subClassOf ddhub:PressureReference. 
ddhub:RelativeTemperatureQuantity a owl:Class; 
                                  rdfs:comment """Relative temperature is a measure of temperature expressed in relation to a reference point or baseline, often used to compare temperature differences rather than absolute values.
The dimension of relative temperature is:
$$[K]$$.
The SI unit for **relative temperature** is: kelvin with the associated unit label $K$
"""@EN; 
                                  rdfs:subClassOf ddhub:Quantity. 
ddhub:RelativeTimeReference a owl:Class; 
                            rdfs:comment ""@EN; 
                            rdfs:subClassOf ddhub:TimeReference. 
ddhub:Resampling a owl:Class; 
                 rdfs:comment ""@EN; 
                 rdfs:subClassOf ddhub:TimeBasedTransformation. 
ddhub:ResamplingDelay a owl:DatatypeProperty, owl:FunctionalProperty; 
                      rdfs:comment """
"""@EN; 
                      rdfs:domain ddhub:Resampling; 
                      rdfs:range xsd:double. 
ddhub:ResamplingRate a owl:DatatypeProperty, owl:FunctionalProperty; 
                     rdfs:comment """
"""@EN; 
                     rdfs:domain ddhub:Resampling; 
                     rdfs:range xsd:double. 
ddhub:ReservePit a owl:Class; 
                 rdfs:comment ""@EN; 
                 rdfs:subClassOf ddhub:MudPits. 
ddhub:Resolution a owl:DatatypeProperty, owl:FunctionalProperty; 
                 rdfs:comment """
"""@EN; 
                 rdfs:domain ddhub:Clock; 
                 rdfs:range xsd:double. 
ddhub:ReturnFlowLine a owl:Class; 
                     rdfs:comment ""@EN; 
                     rdfs:subClassOf ddhub:Pipe. 
ddhub:RfidReamers a owl:Class; 
                  rdfs:comment ""@EN; 
                  rdfs:subClassOf ddhub:Reamers. 
ddhub:RiemannianManifoldFourDimensionalReferenceFrame a owl:Class; 
                                                      rdfs:comment ""@EN; 
                                                      rdfs:subClassOf ddhub:FourDimensionalReferenceFrame. 
ddhub:RiemannianManifoldThreeDimensionalReferenceFrame a owl:Class; 
                                                       rdfs:comment ""@EN; 
                                                       rdfs:subClassOf ddhub:ThreeDimensionalReferenceFrame. 
ddhub:RiemannianManifoldTwoDimensionalReferenceFrame a owl:Class; 
                                                     rdfs:comment ""@EN; 
                                                     rdfs:subClassOf ddhub:TwoDimensionalReferenceFrame. 
ddhub:RigActionPlan a owl:Class; 
                    rdfs:comment ""@EN; 
                    rdfs:subClassOf ddhub:Plan. 
ddhub:RigChokeControlSystem a owl:Class; 
                            rdfs:comment ""@EN; 
                            rdfs:subClassOf ddhub:ControlSystem. 
ddhub:RigEquipment a owl:Class; 
                   rdfs:comment ""@EN; 
                   rdfs:subClassOf ddhub:Equipment. 
ddhub:RigFloor a owl:Class; 
               rdfs:comment ""@EN; 
               rdfs:subClassOf ddhub:DrillFloorStructure. 
ddhub:RightToLeft a owl:DatatypeProperty, owl:FunctionalProperty; 
                  rdfs:comment """Indicates whether the fluid can flow from the right branch to the left branch though the junction
"""@EN; 
                  rdfs:domain ddhub:HydraulicJunction; 
                  rdfs:range xsd:bool. 
ddhub:RiserLiftPump a owl:Class; 
                    rdfs:comment ""@EN; 
                    rdfs:subClassOf ddhub:CirculationSystem. 
ddhub:RiserRecoilSystem a owl:Class; 
                        rdfs:comment ""@EN; 
                        rdfs:subClassOf ddhub:MarineSystem. 
ddhub:RiserTensioners a owl:Class; 
                      rdfs:comment ""@EN; 
                      rdfs:subClassOf ddhub:MarineSystem. 
ddhub:RollerReamers a owl:Class; 
                    rdfs:comment ""@EN; 
                    rdfs:subClassOf ddhub:Reamers. 
ddhub:RollingCutter a owl:Class; 
                    rdfs:comment ""@EN; 
                    rdfs:subClassOf ddhub:DrillingBit. 
ddhub:ROP a owl:Class; 
          rdfs:comment ""@EN; 
          rdfs:subClassOf ddhub:PrototypeData. 
ddhub:RotarySlips a owl:Class; 
                  rdfs:comment ""@EN; 
                  rdfs:subClassOf ddhub:DrillFloorEquipment. 
ddhub:RotarySteerableSystems a owl:Class; 
                             rdfs:comment ""@EN; 
                             rdfs:subClassOf ddhub:DrillingEquipment. 
ddhub:RotaryTable a owl:Class; 
                  rdfs:comment ""@EN; 
                  rdfs:subClassOf ddhub:SurfaceRotationSystem. 
ddhub:RotaryTableBushings a owl:Class; 
                          rdfs:comment ""@EN; 
                          rdfs:subClassOf ddhub:RotaryTable. 
ddhub:RotaryTableVerticalLocation a owl:Class; 
                                  rdfs:comment ""@EN; 
                                  rdfs:subClassOf ddhub:VerticalReferenceLocation. 
ddhub:RotatingControlDeviceRcd a owl:Class; 
                               rdfs:comment ""@EN; 
                               rdfs:subClassOf ddhub:DrillFloorEquipment. 
ddhub:RotationalFrequencyQuantity a owl:Class; 
                                  rdfs:comment """Rotation frequency is the number of complete rotations or cycles an object makes per unit of time.
The dimension of rotational frequency is:
$$[T^{-1}]$$.
"""@EN; 
                                  rdfs:subClassOf ddhub:MeasurableQuantity. 
ddhub:RotationalFrequencyRateOfChangeDrillingQuantity a owl:Class; 
                                                      rdfs:comment """A frequency rate of change is the time derivative of a frequency: $\\frac{df}{dt}$, where $f$ is a frequency and $t$ is time.
The dimension of frequency rate of change is:
$$[T^{-2}]$$.
The SI unit for **frequency rate of change** is: hertz per second with the associated unit label $\\frac{Hz}{s}$
A rotation frequency rate of change is the time derivative of a rotation frequency.
The meaningful precision of rotational frequency is typically: 0.016666666666666666 Hz/s
The meaningful precision of rotational frequency rate of change in the drilling context is typically: 0.016666666666666666 Hz/s
"""@EN; 
                                                      rdfs:subClassOf ddhub:MeasurableQuantity. 
ddhub:RotationalFrequencyRateOfChangeQuantity a owl:Class; 
                                              rdfs:comment """A frequency rate of change is the time derivative of a frequency: $\\frac{df}{dt}$, where $f$ is a frequency and $t$ is time.
The dimension of frequency rate of change is:
$$[T^{-2}]$$.
The SI unit for **frequency rate of change** is: hertz per second with the associated unit label $\\frac{Hz}{s}$
A rotation frequency rate of change is the time derivative of a rotation frequency.
The meaningful precision of rotational frequency is typically:  Hz/s
"""@EN; 
                                              rdfs:subClassOf ddhub:Quantity. 
ddhub:RotationalFrequencySmallQuantity a owl:Class; 
                                       rdfs:comment """Rotation frequency is the number of complete rotations or cycles an object makes per unit of time.
The dimension of rotational frequency is:
$$[T^{-1}]$$.
The meaningful precision of small rotational frequency is typically: 0.00016666 Hz
"""@EN; 
                                       rdfs:subClassOf ddhub:MeasurableQuantity. 
ddhub:RotationalModelling a owl:Class; 
                          rdfs:comment """The model accounts for the rotational movement of some parts of the physical system.
"""@EN; 
                          rdfs:subClassOf ddhub:ModelledDegreeOfFreedom. 
ddhub:Rov a owl:Class; 
          rdfs:comment ""@EN; 
          rdfs:subClassOf ddhub:MarineSystem. 
ddhub:RunnableFunction a owl:Class; 
                       rdfs:comment """A runnable function is a function that starts to run immediately when activated.
"""@EN; 
                       rdfs:subClassOf ddhub:ActivableFunction. 
ddhub:SafetyClamps a owl:Class; 
                   rdfs:comment ""@EN; 
                   rdfs:subClassOf ddhub:DrillFloorEquipment. 
ddhub:SafetyEquipment a owl:Class; 
                      rdfs:comment ""@EN; 
                      rdfs:subClassOf ddhub:RigEquipment. 
ddhub:SamplingRate a owl:DatatypeProperty, owl:FunctionalProperty; 
                   rdfs:comment """
"""@EN; 
                   rdfs:domain ddhub:SynchronizationGroup; 
                   rdfs:range xsd:double. 
ddhub:SandTrap a owl:Class; 
               rdfs:comment ""@EN; 
               rdfs:subClassOf ddhub:MudPits. 
ddhub:ScreenString a owl:Class; 
                   rdfs:comment ""@EN; 
                   rdfs:subClassOf ddhub:Tubulars. 
ddhub:ScribeLineAngleLocation a owl:Class; 
                              rdfs:comment ""@EN; 
                              rdfs:subClassOf ddhub:AngleReferenceLocation. 
ddhub:SeaFloorVerticalLocation a owl:Class; 
                               rdfs:comment ""@EN; 
                               rdfs:subClassOf ddhub:VerticalReferenceLocation. 
ddhub:SeaWater a owl:Class; 
               rdfs:comment ""@EN; 
               rdfs:subClassOf ddhub:DrillingFluid. 
ddhub:Selfsealingthreaded a owl:Class; 
                          rdfs:comment ""@EN; 
                          rdfs:subClassOf ddhub:Connection. 
ddhub:SemiCircularChannel a owl:Class; 
                          rdfs:comment ""@EN; 
                          rdfs:subClassOf ddhub:OpenChannel. 
ddhub:SensorUncertainty a owl:Class; 
                        rdfs:comment """The uncertainty of the sensor is described by a systematic bias and repetitive error. The systematic bias is referred to as the `Accuracy` while the repetitive error is referred to as the `Precision`. The standard deviation of the overall Gaussian distribution is $\\sqrt{\\sigma^2{_a}+\\sigma^2{_p}}$ where $\\sigma_a$ is the accuracy and $\\sigma_p$ is the precision. The `Accuracy` or the `Precision` can either be defined as attribute values, for example when they have fixed values, or using another facts utilizing the verbs `HasAccuracy` or respectively `HasPrecision` when these values may change through time.
"""@EN; 
                        rdfs:subClassOf ddhub:GaussianUncertainty. 
ddhub:Seperator a owl:Class; 
                rdfs:comment ""@EN; 
                rdfs:subClassOf ddhub:WellTestingEquipment. 
ddhub:ServiceCompany a owl:Class; 
                     rdfs:comment """A service company is an entity that provides services during the well construction.
"""@EN; 
                     rdfs:subClassOf ddhub:DataProvider. 
ddhub:SetPoint a owl:Class; 
               rdfs:comment ""@EN; 
               rdfs:subClassOf ddhub:ProcessData. 
ddhub:ShakerCascadeLevels a owl:Class; 
                          rdfs:comment ""@EN; 
                          rdfs:subClassOf ddhub:ShaleShakers. 
ddhub:ShakerDecks a owl:Class; 
                  rdfs:comment ""@EN; 
                  rdfs:subClassOf ddhub:ShaleShakers. 
ddhub:ShakerHopper a owl:Class; 
                   rdfs:comment ""@EN; 
                   rdfs:subClassOf ddhub:ShaleShakers. 
ddhub:ShakerScreenMeshSize a owl:Class; 
                           rdfs:comment ""@EN; 
                           rdfs:subClassOf ddhub:ShakerDecks. 
ddhub:ShakerScreens a owl:Class; 
                    rdfs:comment ""@EN; 
                    rdfs:subClassOf ddhub:ShakerDecks. 
ddhub:ShaleShakers a owl:Class; 
                   rdfs:comment ""@EN; 
                   rdfs:subClassOf ddhub:CirculationSystem. 
ddhub:ShearRam a owl:Class; 
               rdfs:comment ""@EN; 
               rdfs:subClassOf ddhub:BopElement. 
ddhub:ShearRate a owl:Class; 
                rdfs:comment ""@EN; 
                rdfs:subClassOf ddhub:PrototypeData. 
ddhub:ShearStress a owl:Class; 
                  rdfs:comment ""@EN; 
                  rdfs:subClassOf ddhub:PrototypeData. 
ddhub:Shock a owl:Class; 
            rdfs:comment ""@EN; 
            rdfs:subClassOf ddhub:AbnormalLateralOscillation. 
ddhub:ShockRateQuantity a owl:Class; 
                        rdfs:comment """A shock rate is the number of shocks per unit time.
The meaningful precision of shock rate is typically: 0.016666666666666666 Hz/s
"""@EN; 
                        rdfs:subClassOf ddhub:MeasurableQuantity. 
ddhub:ShoeTrack a owl:Class; 
                rdfs:comment ""@EN; 
                rdfs:subClassOf ddhub:CasingEquipment. 
ddhub:ShortDc a owl:Class; 
              rdfs:comment ""@EN; 
              rdfs:subClassOf ddhub:DrillString. 
ddhub:SignalProcessingUnit a owl:Class; 
                           rdfs:comment """Represent any signal processing applied prior to the distribution of the considered signal. Signal processing refers to e.g. noise removal, filtering,..
"""@EN; 
                           rdfs:subClassOf ddhub:Transformation. 
ddhub:SignalUncertainty a owl:Class; 
                        rdfs:comment """Represent the uncertainty associated to a `DrillingDataPoint`.
"""@EN; 
                        rdfs:subClassOf ddhub:DWISNoun. 
ddhub:Simulator a owl:Class; 
                rdfs:comment ""@EN; 
                rdfs:subClassOf ddhub:ComputationUnit. 
ddhub:SingleActing a owl:Class; 
                   rdfs:comment ""@EN; 
                   rdfs:subClassOf ddhub:Action. 
ddhub:SingleJointDerrick a owl:Class; 
                         rdfs:comment ""@EN; 
                         rdfs:subClassOf ddhub:Derrick. 
ddhub:Singles a owl:Class; 
              rdfs:comment ""@EN; 
              rdfs:subClassOf ddhub:Grouping. 
ddhub:SIUnit a owl:DatatypeProperty, owl:FunctionalProperty; 
             rdfs:comment """
"""@EN; 
             rdfs:domain ddhub:Quantity; 
             rdfs:range xsd:string. 
ddhub:SlantDerrick a owl:Class; 
                   rdfs:comment ""@EN; 
                   rdfs:subClassOf ddhub:Derrick. 
ddhub:Sleeve a owl:Class; 
             rdfs:comment ""@EN; 
             rdfs:subClassOf ddhub:BladeType. 
ddhub:SlickLine a owl:Class; 
                rdfs:comment ""@EN; 
                rdfs:subClassOf ddhub:DrillFloorEquipment. 
ddhub:SlipJoint a owl:Class; 
                rdfs:comment ""@EN; 
                rdfs:subClassOf ddhub:MarineSystem. 
ddhub:SlugSettlingPit a owl:Class; 
                      rdfs:comment ""@EN; 
                      rdfs:subClassOf ddhub:MudPits. 
ddhub:SOEFunction a owl:Class; 
                  rdfs:comment """A `SOEFunction` is a `ProtectionFunction` that limits the commands that are send to the drilling machines
to avoid generating a drilling incident. SOE stands for Safe Operating Envelope. A `SOEFunction` protects the inputs
of the drilling process. An example `SOEFunction` is a swab/surge limits protection. This function limits the axial acceleration
and speed of the drill-stem to avoid generate swabbing pressure below the maximum of the collapse and pore pressure, and
surging pressure above the fracturing pressure.
"""@EN; 
                  rdfs:subClassOf ddhub:ProtectionFunction. 
ddhub:SolidAngleQuantity a owl:Class; 
                         rdfs:comment """A solid angle is a three-dimensional angle that measures the portion of a sphere's surface subtended by an object. It is the 3D equivalent of a planar angle in two dimensions.
The dimension of solid angle is:
$$[{\\Omega}]$$.
The SI unit for **solid angle** is: steradian with the associated unit label $sr$
"""@EN; 
                         rdfs:subClassOf ddhub:Quantity. 
ddhub:SolidComponent a owl:Class; 
                     rdfs:comment ""@EN; 
                     rdfs:subClassOf ddhub:FluidComponent. 
ddhub:SpacingSpool a owl:Class; 
                   rdfs:comment ""@EN; 
                   rdfs:subClassOf ddhub:WellControlSystem. 
ddhub:Spear a owl:Class; 
            rdfs:comment ""@EN; 
            rdfs:subClassOf ddhub:FishingTools. 
ddhub:SphericalReferenceFrame a owl:Class; 
                              rdfs:comment ""@EN; 
                              rdfs:subClassOf ddhub:ThreeDimensionalReferenceFrame. 
ddhub:SpiderGimbal a owl:Class; 
                   rdfs:comment ""@EN; 
                   rdfs:subClassOf ddhub:MarineSystem. 
ddhub:Spiral a owl:Class; 
             rdfs:comment ""@EN; 
             rdfs:subClassOf ddhub:BladeShape. 
ddhub:SpontaneousPotential a owl:Class; 
                           rdfs:comment ""@EN; 
                           rdfs:subClassOf ddhub:WirelineLoggingTools. 
ddhub:SPP a owl:Class; 
          rdfs:comment ""@EN; 
          rdfs:subClassOf ddhub:PrototypeData. 
ddhub:SpudMud a owl:Class; 
              rdfs:comment ""@EN; 
              rdfs:subClassOf ddhub:DrillingFluid. 
ddhub:StabbingGuide a owl:Class; 
                    rdfs:comment ""@EN; 
                    rdfs:subClassOf ddhub:DrillFloorEquipment. 
ddhub:Stabilizers a owl:Class; 
                  rdfs:comment ""@EN; 
                  rdfs:subClassOf ddhub:DrillString. 
ddhub:StandardElectricalDrawworks a owl:Class; 
                                  rdfs:comment ""@EN; 
                                  rdfs:subClassOf ddhub:Drawworks. 
ddhub:Stands a owl:Class; 
             rdfs:comment ""@EN; 
             rdfs:subClassOf ddhub:Grouping. 
ddhub:StartsHydraulicBranchDecomposition a owl:ObjectProperty; 
                                         rdfs:comment ""@EN; 
                                         rdfs:domain ddhub:DWISNoun; 
                                         rdfs:range ddhub:DWISNoun; 
                                         rdfs:subPropertyOf ddhub:DWISVerb. 
ddhub:SteadyStateModel a owl:Class; 
                       rdfs:comment """A model for which the state variables do not change with time.
"""@EN; 
                       rdfs:subClassOf ddhub:MathematicalModel. 
ddhub:Steerable a owl:Class; 
                rdfs:comment ""@EN; 
                rdfs:subClassOf ddhub:Stabilizers. 
ddhub:SteerableLinerDrilling a owl:Class; 
                             rdfs:comment ""@EN; 
                             rdfs:subClassOf ddhub:LinerDrilling. 
ddhub:SteerableMotor a owl:Class; 
                     rdfs:comment ""@EN; 
                     rdfs:subClassOf ddhub:DownholeMotor. 
ddhub:StickDurationDrillingQuantity a owl:Class; 
                                    rdfs:comment """Time is a continuous, measurable progression in which events occur, from the past through the present to the future.
The dimension of time is:
$$[T]$$.
The SI unit for **time** is: second with the associated unit label $s$
The meaningful precision of stick duration in the drilling context is typically: 0.001 s
"""@EN; 
                                    rdfs:subClassOf ddhub:MeasurableQuantity. 
ddhub:StickSlip a owl:Class; 
                rdfs:comment ""@EN; 
                rdfs:subClassOf ddhub:AbnormalTorsionalOscillation. 
ddhub:StickUpHeightVerticalLocation a owl:Class; 
                                    rdfs:comment ""@EN; 
                                    rdfs:subClassOf ddhub:VerticalReferenceLocation. 
ddhub:StochasticModel a owl:Class; 
                      rdfs:comment ""@EN; 
                      rdfs:subClassOf ddhub:ModelType. 
ddhub:StorageTank a owl:Class; 
                  rdfs:comment ""@EN; 
                  rdfs:subClassOf ddhub:MudPits. 
ddhub:StormLoop a owl:Class; 
                rdfs:comment ""@EN; 
                rdfs:subClassOf ddhub:MarineSystem. 
ddhub:Straight a owl:Class; 
               rdfs:comment ""@EN; 
               rdfs:subClassOf ddhub:BladeShape. 
ddhub:StrainWaveBasedDiscretization a owl:Class; 
                                    rdfs:comment """A model can properly estimate values at the level of strain wave propagation.
"""@EN; 
                                    rdfs:subClassOf ddhub:ModellingDiscretization. 
ddhub:Stratum a owl:DatatypeProperty, owl:FunctionalProperty; 
              rdfs:comment """
"""@EN; 
              rdfs:domain ddhub:Clock; 
              rdfs:range xsd:int. 
ddhub:StressQuantity a owl:Class; 
                     rdfs:comment """Stress in a material is the internal force per unit area that arises when the material is subjected to external forces or loads. It reflects how much the material is being compressed, stretched, or sheared.
The dimension of stress is:
$$[ML^{-1}T^{-2}]$$.
The SI unit for **stress** is: pascal with the associated unit label $Pa$
"""@EN; 
                     rdfs:subClassOf ddhub:Quantity. 
ddhub:StringDataType a owl:Class; 
                     rdfs:comment ""@EN; 
                     rdfs:subClassOf ddhub:DataType. 
ddhub:StrokeFrequencyQuantity a owl:Class; 
                              rdfs:comment """A stroke frequency is the number of stokes per unit time
The meaningful precision of a stroke frequency is typically: 0.016666666666666666 Hz
"""@EN; 
                              rdfs:subClassOf ddhub:MeasurableQuantity. 
ddhub:StuckPipe a owl:Class; 
                rdfs:comment ""@EN; 
                rdfs:subClassOf ddhub:DrillingIncident. 
ddhub:Subbent a owl:Class; 
              rdfs:comment ""@EN; 
              rdfs:subClassOf ddhub:MiscSubs. 
ddhub:Subbit a owl:Class; 
             rdfs:comment ""@EN; 
             rdfs:subClassOf ddhub:MiscSubs. 
ddhub:Subbumper a owl:Class; 
                rdfs:comment ""@EN; 
                rdfs:subClassOf ddhub:MiscSubs. 
ddhub:Subcatcher a owl:Class; 
                 rdfs:comment ""@EN; 
                 rdfs:subClassOf ddhub:MiscSubs. 
ddhub:Subcirculation a owl:Class; 
                     rdfs:comment ""@EN; 
                     rdfs:subClassOf ddhub:MiscSubs. 
ddhub:Subcone a owl:Class; 
              rdfs:comment ""@EN; 
              rdfs:subClassOf ddhub:MiscSubs. 
ddhub:Subcrossover a owl:Class; 
                   rdfs:comment ""@EN; 
                   rdfs:subClassOf ddhub:MiscSubs. 
ddhub:Subdart a owl:Class; 
              rdfs:comment ""@EN; 
              rdfs:subClassOf ddhub:MiscSubs. 
ddhub:Subfilter a owl:Class; 
                rdfs:comment ""@EN; 
                rdfs:subClassOf ddhub:MiscSubs. 
ddhub:Subfloat a owl:Class; 
               rdfs:comment ""@EN; 
               rdfs:subClassOf ddhub:MiscSubs. 
ddhub:Subjetting a owl:Class; 
                 rdfs:comment ""@EN; 
                 rdfs:subClassOf ddhub:MiscSubs. 
ddhub:Subjunk a owl:Class; 
              rdfs:comment ""@EN; 
              rdfs:subClassOf ddhub:MiscSubs. 
ddhub:Suborienting a owl:Class; 
                   rdfs:comment ""@EN; 
                   rdfs:subClassOf ddhub:MiscSubs. 
ddhub:Subported a owl:Class; 
                rdfs:comment ""@EN; 
                rdfs:subClassOf ddhub:MiscSubs. 
ddhub:SubpressureRelief a owl:Class; 
                        rdfs:comment ""@EN; 
                        rdfs:subClassOf ddhub:MiscSubs. 
ddhub:SubpumpOut a owl:Class; 
                 rdfs:comment ""@EN; 
                 rdfs:subClassOf ddhub:MiscSubs. 
ddhub:Subrestrictor a owl:Class; 
                    rdfs:comment ""@EN; 
                    rdfs:subClassOf ddhub:MiscSubs. 
ddhub:Subsaver a owl:Class; 
               rdfs:comment ""@EN; 
               rdfs:subClassOf ddhub:MiscSubs. 
ddhub:SubseaBop a owl:Class; 
                rdfs:comment ""@EN; 
                rdfs:subClassOf ddhub:BopStack. 
ddhub:SubseaTestTree a owl:Class; 
                     rdfs:comment ""@EN; 
                     rdfs:subClassOf ddhub:WellTestingEquipment. 
ddhub:Subshock a owl:Class; 
               rdfs:comment ""@EN; 
               rdfs:subClassOf ddhub:MiscSubs. 
ddhub:SubsideEntry a owl:Class; 
                   rdfs:comment ""@EN; 
                   rdfs:subClassOf ddhub:MiscSubs. 
ddhub:Substop a owl:Class; 
              rdfs:comment ""@EN; 
              rdfs:subClassOf ddhub:MiscSubs. 
ddhub:SupportLine a owl:Class; 
                  rdfs:comment ""@EN; 
                  rdfs:subClassOf ddhub:DrillLine. 
ddhub:SurfaceBop a owl:Class; 
                 rdfs:comment ""@EN; 
                 rdfs:subClassOf ddhub:BopStack. 
ddhub:SurfacePoreDrillingQuantity a owl:Class; 
                                  rdfs:comment """Area is the measure of the extent of a surface or the size of a two-dimensional shape.
The dimension of area is:
$$[L^{2}]$$.
The SI unit for **area** is: square metre with the associated unit label $m^{2}$
The meaningful precision of pore surface in the drilling context is typically: 1E-13 m²
"""@EN; 
                                  rdfs:subClassOf ddhub:MeasurableQuantity. 
ddhub:SurfacePower a owl:Class; 
                   rdfs:comment ""@EN; 
                   rdfs:subClassOf ddhub:PowerSystems. 
ddhub:SurfaceRiser a owl:Class; 
                   rdfs:comment ""@EN; 
                   rdfs:subClassOf ddhub:DrillingRiser. 
ddhub:SurfaceRotationSystem a owl:Class; 
                            rdfs:comment ""@EN; 
                            rdfs:subClassOf ddhub:RigEquipment. 
ddhub:SurfaceRPM a owl:Class; 
                 rdfs:comment ""@EN; 
                 rdfs:subClassOf ddhub:PrototypeData. 
ddhub:SurfaceTorque a owl:Class; 
                    rdfs:comment ""@EN; 
                    rdfs:subClassOf ddhub:PrototypeData. 
ddhub:SurgeTank a owl:Class; 
                rdfs:comment ""@EN; 
                rdfs:subClassOf ddhub:MudPits. 
ddhub:SwivelSub a owl:Class; 
                rdfs:comment ""@EN; 
                rdfs:subClassOf ddhub:TopDrive. 
ddhub:Symbol a owl:DatatypeProperty, owl:FunctionalProperty; 
             rdfs:comment """
"""@EN; 
             rdfs:domain ddhub:Unit; 
             rdfs:range xsd:string. 
ddhub:SynchronizationDelay a owl:DatatypeProperty, owl:FunctionalProperty; 
                           rdfs:comment """
"""@EN; 
                           rdfs:domain ddhub:SynchronizationGroup; 
                           rdfs:range xsd:double. 
ddhub:SynchronizationGroup a owl:Class; 
                           rdfs:comment ""@EN; 
                           rdfs:subClassOf ddhub:DWISNoun. 
ddhub:SyntheticOilBasedMudSobm a owl:Class; 
                               rdfs:comment ""@EN; 
                               rdfs:subClassOf ddhub:DrillingFluid. 
ddhub:T a owl:DatatypeProperty, owl:FunctionalProperty; 
        rdfs:comment """Time exponent.
SI Unit: Second (s)
"""@EN; 
        rdfs:domain ddhub:Quantity; 
        rdfs:range xsd:double. 
ddhub:TangencyLength a owl:Class; 
                     rdfs:comment """the position along the drill-string, counted from the bit, from which we can consider that the pipes direction is tangential with the borehole direction.
"""@EN; 
                     rdfs:subClassOf ddhub:DWISNoun. 
ddhub:TangentialModelling a owl:Class; 
                          rdfs:comment """The model accounts for the change of tangential direction of some parts of the physical system.
"""@EN; 
                          rdfs:subClassOf ddhub:LateralModelling. 
ddhub:Tank a owl:Class; 
           rdfs:comment ""@EN; 
           rdfs:subClassOf ddhub:HydraulicLogicalElement. 
ddhub:Telemetry a owl:Class; 
                rdfs:comment """Technology used for transferring the data from its main origin.
"""@EN; 
                rdfs:subClassOf ddhub:DWISNoun. 
ddhub:TemperatureDrillingQuantity a owl:Class; 
                                  rdfs:comment """Temperature is a measure of the average kinetic energy of particles in a substance, indicating how hot or cold the substance is.
The dimension of temperature is:
$$[K]$$.
The SI unit for **temperature** is: kelvin with the associated unit label $K$
The meaningful precision of temperature in the drilling context is typically: 0.01 K
"""@EN; 
                                  rdfs:subClassOf ddhub:MeasurableQuantity. 
ddhub:TemperatureGradientPerLengthDrillingQuantity a owl:Class; 
                                                   rdfs:comment """A temperature gradient per lenth is the first derivative of a temperature compared to a distance: $\\frac{dT}{ds}$, where $T$ is a temperature and $s$ is a distance.
The dimension of temperature gradient per length is:
$$[KL^{-1}]$$.
The SI unit for **temperature gradient per length** is: kelvin per metre with the associated unit label $\\frac{K}{m}$
The meaningful precision of temperature gradient per length in the drilling context is typically: 0.001 K/m
"""@EN; 
                                                   rdfs:subClassOf ddhub:MeasurableQuantity. 
ddhub:TemperatureGradientPerLengthQuantity a owl:Class; 
                                           rdfs:comment """A temperature gradient per lenth is the first derivative of a temperature compared to a distance: $\\frac{dT}{ds}$, where $T$ is a temperature and $s$ is a distance.
The dimension of temperature gradient per length is:
$$[KL^{-1}]$$.
The SI unit for **temperature gradient per length** is: kelvin per metre with the associated unit label $\\frac{K}{m}$
"""@EN; 
                                           rdfs:subClassOf ddhub:Quantity. 
ddhub:TemperatureIn a owl:Class; 
                    rdfs:comment ""@EN; 
                    rdfs:subClassOf ddhub:PrototypeData. 
ddhub:TemperatureOut a owl:Class; 
                     rdfs:comment ""@EN; 
                     rdfs:subClassOf ddhub:PrototypeData. 
ddhub:TemperatureQuantity a owl:Class; 
                          rdfs:comment """Temperature is a measure of the average kinetic energy of particles in a substance, indicating how hot or cold the substance is.
The dimension of temperature is:
$$[K]$$.
The SI unit for **temperature** is: kelvin with the associated unit label $K$
"""@EN; 
                          rdfs:subClassOf ddhub:Quantity. 
ddhub:TensionDrillingQuantity a owl:Class; 
                              rdfs:comment """Tension is the pulling or stretching force transmitted axially along an object such as a string, rope, chain, rod, truss member, or other object, so as to stretch or pull apart the object. In terms of force, it is the opposite of compression. Tension might also be described as the action-reaction pair of forces acting at each end of an object.
The dimension of tension is:
$$[LMT^{-2}]$$.
The meaningful precision of tension in the drilling context is typically: 100 N
"""@EN; 
                              rdfs:subClassOf ddhub:MeasurableQuantity. 
ddhub:TensionQuantity a owl:Class; 
                      rdfs:comment """Tension is the pulling or stretching force transmitted axially along an object such as a string, rope, chain, rod, truss member, or other object, so as to stretch or pull apart the object. In terms of force, it is the opposite of compression. Tension might also be described as the action-reaction pair of forces acting at each end of an object.
The dimension of tension is:
$$[LMT^{-2}]$$.
"""@EN; 
                      rdfs:subClassOf ddhub:Quantity. 
ddhub:TestingTools a owl:Class; 
                   rdfs:comment ""@EN; 
                   rdfs:subClassOf ddhub:WellTestingEquipment. 
ddhub:TestPlug a owl:Class; 
               rdfs:comment ""@EN; 
               rdfs:subClassOf ddhub:WellTestingEquipment. 
ddhub:TestTools a owl:Class; 
                rdfs:comment ""@EN; 
                rdfs:subClassOf ddhub:WellTestingEquipment. 
ddhub:ThermalConductivityDrillingQuantity a owl:Class; 
                                          rdfs:comment """Thermal conductivity is a material's ability to conduct heat. It measures how efficiently heat is transferred through a material when there is a temperature difference.
The dimension of thermal conductivity is:
$$[LMK^{-1}T^{-3}]$$.
The SI unit for **thermal conductivity** is: watt per metre kelvin with the associated unit label $\\frac{W}{m \\cdot K}$
The meaningful precision of thermal conductivity in the drilling context is typically: 0.01 W/m•K
"""@EN; 
                                          rdfs:subClassOf ddhub:MeasurableQuantity. 
ddhub:ThermalConductivityGradientPerTemperatureDrillingQuantity a owl:Class; 
                                                                rdfs:comment """A thermal conductivity gradient per temperature is the first derivative of a thermal conductivity compared to temperature: $\\frac{dk}{dT}$, where $k$ is a thermal conductivity and $T$ is temperature. 
The dimension of thermal conductivity gradient per temperature is:
$$[LMK^{-2}T^{-3}]$$.
The SI unit for **thermal conductivity gradient per temperature** is: watt per metre kelvin per kelvin with the associated unit label $\\frac{(\\frac{W}{(m \\cdot K)}}{K}$
The meaningful precision of thermal conductivity gradient per temperature in the drilling context is typically: 0.01 (W/(m•K))/K
"""@EN; 
                                                                rdfs:subClassOf ddhub:MeasurableQuantity. 
ddhub:ThermalConductivityGradientPerTemperatureQuantity a owl:Class; 
                                                        rdfs:comment """A thermal conductivity gradient per temperature is the first derivative of a thermal conductivity compared to temperature: $\\frac{dk}{dT}$, where $k$ is a thermal conductivity and $T$ is temperature. 
The dimension of thermal conductivity gradient per temperature is:
$$[LMK^{-2}T^{-3}]$$.
The SI unit for **thermal conductivity gradient per temperature** is: watt per metre kelvin per kelvin with the associated unit label $\\frac{(\\frac{W}{(m \\cdot K)}}{K}$
"""@EN; 
                                                        rdfs:subClassOf ddhub:Quantity. 
ddhub:ThermalConductivityQuantity a owl:Class; 
                                  rdfs:comment """Thermal conductivity is a material's ability to conduct heat. It measures how efficiently heat is transferred through a material when there is a temperature difference.
The dimension of thermal conductivity is:
$$[LMK^{-1}T^{-3}]$$.
The SI unit for **thermal conductivity** is: watt per metre kelvin with the associated unit label $\\frac{W}{m \\cdot K}$
"""@EN; 
                                  rdfs:subClassOf ddhub:Quantity. 
ddhub:Theta a owl:DatatypeProperty, owl:FunctionalProperty; 
            rdfs:comment """plane angle exponent.
SI Unit: radian (rad)
"""@EN; 
            rdfs:domain ddhub:Quantity; 
            rdfs:range xsd:double. 
ddhub:ThirdPartyRigEquipment a owl:Class; 
                             rdfs:comment ""@EN; 
                             rdfs:subClassOf ddhub:RigEquipment. 
ddhub:ThirdPartyTools a owl:Class; 
                      rdfs:comment ""@EN; 
                      rdfs:subClassOf ddhub:ThirdPartyRigEquipment. 
ddhub:ThreeDimensionalReferenceFrame a owl:Class; 
                                     rdfs:comment ""@EN; 
                                     rdfs:subClassOf ddhub:ReferenceFrame. 
ddhub:ThreeDModelling a owl:Class; 
                      rdfs:comment """The model only accounts for three dimensions
"""@EN; 
                      rdfs:subClassOf ddhub:ModellingDimensions. 
ddhub:ThreeWayManifold a owl:Class; 
                       rdfs:comment ""@EN; 
                       rdfs:subClassOf ddhub:GenericEquipment. 
ddhub:ThreeWayValve a owl:Class; 
                    rdfs:comment ""@EN; 
                    rdfs:subClassOf ddhub:GenericEquipment. 
ddhub:Thruster a owl:Class; 
               rdfs:comment ""@EN; 
               rdfs:subClassOf ddhub:DrillingEquipment. 
ddhub:ThT a owl:DatatypeProperty, owl:FunctionalProperty; 
          rdfs:comment """Thermodynamic temperature exponent.
SI Unit: Kelvin (K)
"""@EN; 
          rdfs:domain ddhub:Quantity; 
          rdfs:range xsd:double. 
ddhub:TimeBasedTransformation a owl:Class; 
                              rdfs:comment """Transformations that apply only to time series: time derivations, time integration, averaging...
"""@EN; 
                              rdfs:subClassOf ddhub:Transformation. 
ddhub:TimeQuantity a owl:Class; 
                   rdfs:comment """Time is a continuous, measurable progression in which events occur, from the past through the present to the future.
The dimension of time is:
$$[T]$$.
The SI unit for **time** is: second with the associated unit label $s$
"""@EN; 
                   rdfs:subClassOf ddhub:Quantity. 
ddhub:TimeReference a owl:Class; 
                    rdfs:comment ""@EN; 
                    rdfs:subClassOf ddhub:DWISNoun. 
ddhub:TimeSpanReference a owl:Class; 
                        rdfs:comment ""@EN; 
                        rdfs:subClassOf ddhub:RelativeTimeReference. 
ddhub:TimeStampAcquisition a owl:DatatypeProperty, owl:FunctionalProperty; 
                           rdfs:comment """this is a UTC date-time value at which the value has been acquired by the data acquisition system.
"""@EN; 
                           rdfs:domain ddhub:DynamicDrillingSignal; 
                           rdfs:range xsd:datetime. 
ddhub:TimeStampAtSource a owl:DatatypeProperty, owl:FunctionalProperty; 
                        rdfs:comment """this is a UTC date-time value corresponding to the time at which the value has been taken.
"""@EN; 
                        rdfs:domain ddhub:DynamicDrillingSignal; 
                        rdfs:range xsd:datetime. 
ddhub:TimeWindow a owl:DatatypeProperty, owl:FunctionalProperty; 
                 rdfs:comment """
"""@EN; 
                 rdfs:domain ddhub:TimeWindowMovingAverage, ddhub:TimeWindowRangeExtraction; 
                 rdfs:range xsd:double. 
ddhub:TimeWindowMovingAverage a owl:Class; 
                              rdfs:comment ""@EN; 
                              rdfs:subClassOf ddhub:MovingAverage. 
ddhub:TimeWindowRangeExtraction a owl:Class; 
                                rdfs:comment ""@EN; 
                                rdfs:subClassOf ddhub:RangeExtraction. 
ddhub:ToolJoint1ReferenceLocation a owl:Class; 
                                  rdfs:comment ""@EN; 
                                  rdfs:subClassOf ddhub:AbscissaReferenceLocation. 
ddhub:ToolJoint2ReferenceLocation a owl:Class; 
                                  rdfs:comment ""@EN; 
                                  rdfs:subClassOf ddhub:AbscissaReferenceLocation. 
ddhub:ToolJoint3ReferenceLocation a owl:Class; 
                                  rdfs:comment ""@EN; 
                                  rdfs:subClassOf ddhub:AbscissaReferenceLocation. 
ddhub:ToolJoint4ReferenceLocation a owl:Class; 
                                  rdfs:comment ""@EN; 
                                  rdfs:subClassOf ddhub:AbscissaReferenceLocation. 
ddhub:TopDrive a owl:Class; 
               rdfs:comment ""@EN; 
               rdfs:subClassOf ddhub:SurfaceRotationSystem. 
ddhub:TopDriveControlSystem a owl:Class; 
                            rdfs:comment ""@EN; 
                            rdfs:subClassOf ddhub:ControlSystem. 
ddhub:TopOfRatHoleLocation a owl:Class; 
                           rdfs:comment ""@EN; 
                           rdfs:subClassOf ddhub:AbscissaReferenceLocation. 
ddhub:TopOfStringPosition a owl:Class; 
                          rdfs:comment ""@EN; 
                          rdfs:subClassOf ddhub:PrototypeData. 
ddhub:TopOfStringReferenceLocation a owl:Class; 
                                   rdfs:comment ""@EN; 
                                   rdfs:subClassOf ddhub:AbscissaReferenceLocation. 
ddhub:TopShoulderAxialLocation a owl:Class; 
                               rdfs:comment ""@EN; 
                               rdfs:subClassOf ddhub:AxialReferenceLocation. 
ddhub:TopsideHydraulicNetwork a owl:Class; 
                              rdfs:comment ""@EN; 
                              rdfs:subClassOf ddhub:HydraulicNetwork. 
ddhub:TopSideTelemetry a owl:Class; 
                       rdfs:comment """Method that allows transfer of data from surface systems.
"""@EN; 
                       rdfs:subClassOf ddhub:Telemetry. 
ddhub:TorqueBushing a owl:Class; 
                    rdfs:comment ""@EN; 
                    rdfs:subClassOf ddhub:TopDrive. 
ddhub:TorqueDrillingQuantity a owl:Class; 
                             rdfs:comment """A torque is a measure of the rotational force applied to a body around an axis.
The dimension of torque is:
$$[L^{2}MT^{-2}]$$.
The SI unit for **torque** is: newton metre with the associated unit label $N \\cdot m$
The meaningful precision of torque in the drilling context is typically: 0.1 N•m
"""@EN; 
                             rdfs:subClassOf ddhub:MeasurableQuantity. 
ddhub:TorqueGradientPerLengthDrillingQuantity a owl:Class; 
                                              rdfs:comment """A torque gradient per length is the first derivative of torque compared to a distance: $\\frac{d\\tau}{ds}$, where $\\tau$ is a torque and $s$ is a distance.
The dimension of torque gradient per length is:
$$[LMT^{-2}]$$.
The SI unit for **torque gradient per length** is: newton metre per metre with the associated unit label $\\frac{N \\cdot m}{m}$
The meaningful precision of torque gradient per length in the drilling context is typically: 1 N•m/m
"""@EN; 
                                              rdfs:subClassOf ddhub:MeasurableQuantity. 
ddhub:TorqueGradientPerLengthQuantity a owl:Class; 
                                      rdfs:comment """A torque gradient per length is the first derivative of torque compared to a distance: $\\frac{d\\tau}{ds}$, where $\\tau$ is a torque and $s$ is a distance.
The dimension of torque gradient per length is:
$$[LMT^{-2}]$$.
The SI unit for **torque gradient per length** is: newton metre per metre with the associated unit label $\\frac{N \\cdot m}{m}$
"""@EN; 
                                      rdfs:subClassOf ddhub:Quantity. 
ddhub:TorqueQuantity a owl:Class; 
                     rdfs:comment """A torque is a measure of the rotational force applied to a body around an axis.
The dimension of torque is:
$$[L^{2}MT^{-2}]$$.
The SI unit for **torque** is: newton metre with the associated unit label $N \\cdot m$
"""@EN; 
                     rdfs:subClassOf ddhub:Quantity. 
ddhub:TorqueSmallQuantity a owl:Class; 
                          rdfs:comment """A torque is a measure of the rotational force applied to a body around an axis.
The dimension of torque is:
$$[L^{2}MT^{-2}]$$.
The SI unit for **torque** is: newton metre with the associated unit label $N \\cdot m$
The meaningful precision of small torque is typically: 1E-05 N•m
"""@EN; 
                          rdfs:subClassOf ddhub:MeasurableQuantity. 
ddhub:TorqueToForceTransformation a owl:Class; 
                                  rdfs:comment ""@EN; 
                                  rdfs:subClassOf ddhub:DirectTransformation. 
ddhub:TorqueTrack a owl:Class; 
                  rdfs:comment ""@EN; 
                  rdfs:subClassOf ddhub:TopDrive. 
ddhub:TorsionalMotionType a owl:Class; 
                          rdfs:comment ""@EN; 
                          rdfs:subClassOf ddhub:MotionType. 
ddhub:Transformation a owl:Class; 
                     rdfs:comment """Represents a transformation applied to some signals that produces other signals
"""@EN; 
                     rdfs:subClassOf ddhub:DataFlowNode. 
ddhub:TransientModel a owl:Class; 
                     rdfs:comment """A model for which the state variables changes with time.
"""@EN; 
                     rdfs:subClassOf ddhub:MathematicalModel. 
ddhub:TransmissionLine a owl:Class; 
                       rdfs:comment ""@EN; 
                       rdfs:subClassOf ddhub:DataFlowNode. 
ddhub:TravellingBlock a owl:Class; 
                      rdfs:comment ""@EN; 
                      rdfs:subClassOf ddhub:MechanicalBlock. 
ddhub:TripleStandDerrick a owl:Class; 
                         rdfs:comment ""@EN; 
                         rdfs:subClassOf ddhub:Derrick. 
ddhub:TripTank a owl:Class; 
               rdfs:comment ""@EN; 
               rdfs:subClassOf ddhub:MudPits. 
ddhub:TrueNorthAzimuthLocation a owl:Class; 
                               rdfs:comment ""@EN; 
                               rdfs:subClassOf ddhub:AzimuthReferenceLocation. 
ddhub:TubingGuideArch a owl:Class; 
                      rdfs:comment ""@EN; 
                      rdfs:subClassOf ddhub:CoiledTubingEquipment. 
ddhub:TubingHanger a owl:Class; 
                   rdfs:comment ""@EN; 
                   rdfs:subClassOf ddhub:Hangers. 
ddhub:TubingString a owl:Class; 
                   rdfs:comment ""@EN; 
                   rdfs:subClassOf ddhub:Tubulars. 
ddhub:TubularConfiguration a owl:Class; 
                           rdfs:comment ""@EN; 
                           rdfs:subClassOf ddhub:Tubulars. 
ddhub:TubularConnection a owl:Class; 
                        rdfs:comment ""@EN; 
                        rdfs:subClassOf ddhub:Tubulars. 
ddhub:Tubulars a owl:Class; 
               rdfs:comment ""@EN; 
               rdfs:subClassOf ddhub:Equipment. 
ddhub:TurbineMotor a owl:Class; 
                   rdfs:comment ""@EN; 
                   rdfs:subClassOf ddhub:DownholeMotor. 
ddhub:TwistOff a owl:Class; 
               rdfs:comment ""@EN; 
               rdfs:subClassOf ddhub:DrillingIncident. 
ddhub:TwoDimensionalReferenceFrame a owl:Class; 
                                   rdfs:comment ""@EN; 
                                   rdfs:subClassOf ddhub:ReferenceFrame. 
ddhub:TwoDModelling a owl:Class; 
                    rdfs:comment """The model only accounts for two dimensions
"""@EN; 
                    rdfs:subClassOf ddhub:ModellingDimensions. 
ddhub:Underpull a owl:Class; 
                rdfs:comment ""@EN; 
                rdfs:subClassOf ddhub:DrillingIncident. 
ddhub:Underreamers a owl:Class; 
                   rdfs:comment ""@EN; 
                   rdfs:subClassOf ddhub:HoleOpener. 
ddhub:Unit a owl:Class; 
           rdfs:comment ""@EN; 
           rdfs:subClassOf ddhub:DWISNoun. 
ddhub:UnitSystem a owl:Class; 
                 rdfs:comment """A set of associations between measurable quantities and units
"""@EN; 
                 rdfs:subClassOf ddhub:DWISNoun. 
ddhub:UpperSideAngleLocation a owl:Class; 
                             rdfs:comment ""@EN; 
                             rdfs:subClassOf ddhub:AngleReferenceLocation. 
ddhub:UserInterface a owl:Class; 
                    rdfs:comment ""@EN; 
                    rdfs:subClassOf ddhub:DataFlowNode. 
ddhub:UTCReference a owl:Class; 
                   rdfs:comment ""@EN; 
                   rdfs:subClassOf ddhub:TimeReference. 
ddhub:VacuumDegasser a owl:Class; 
                     rdfs:comment ""@EN; 
                     rdfs:subClassOf ddhub:Degasser. 
ddhub:Validity a owl:DatatypeProperty, owl:FunctionalProperty; 
               rdfs:comment """
"""@EN; 
               rdfs:domain ddhub:Resampling; 
               rdfs:range xsd:double. 
ddhub:ValidityCondition a owl:Class; 
                        rdfs:comment ""@EN; 
                        rdfs:subClassOf ddhub:DWISNoun. 
ddhub:Value a owl:DatatypeProperty, owl:FunctionalProperty; 
            rdfs:comment """
"""@EN; 
            rdfs:domain ddhub:DrillingSignal, ddhub:HydraulicConnectedState, ddhub:MechanicalElementState; 
            rdfs:range xsd:object, xsd:bool. 
ddhub:ValuesIndices a owl:DatatypeProperty, owl:FunctionalProperty; 
                    rdfs:comment """
"""@EN; 
                    rdfs:domain ddhub:EndPointMapping; 
                    rdfs:range <http://www.w3.org/2001/XMLSchema#int[]>. 
ddhub:Variable a owl:Class; 
               rdfs:comment ""@EN; 
               rdfs:subClassOf ddhub:BladeShape. 
ddhub:VelocityQuantity a owl:Class; 
                       rdfs:comment """A velocity is the time derivative of a position or a displacement: $\\frac{dx}{dt}$, where $x$ is a position and $t$ is time.
The dimension of velocity is:
$$[LT^{-1}]$$.
The SI unit for **velocity** is: metre per second with the associated unit label $\\frac{m}{s}$
"""@EN; 
                       rdfs:subClassOf ddhub:Quantity. 
ddhub:VentOverboardLine a owl:Class; 
                        rdfs:comment ""@EN; 
                        rdfs:subClassOf ddhub:Diverter. 
ddhub:VerticalDepthFrame a owl:Class; 
                         rdfs:comment ""@EN; 
                         rdfs:subClassOf ddhub:OneDimensionalCartesianReferenceFrame. 
ddhub:VerticalOndulationModelling a owl:Class; 
                                  rdfs:comment """The model accounts for the change of inclination of some parts of the physical system.
"""@EN; 
                                  rdfs:subClassOf ddhub:TangentialModelling. 
ddhub:VerticalReferenceLocation a owl:Class; 
                                rdfs:comment ""@EN; 
                                rdfs:subClassOf ddhub:Location. 
ddhub:VibrationIsolators a owl:Class; 
                         rdfs:comment ""@EN; 
                         rdfs:subClassOf ddhub:ActiveVibrationTools. 
ddhub:VolumeDrillingQuantity a owl:Class; 
                             rdfs:comment """A volume is the amount of three-dimensional space occupied by a body.
The dimension of volume is:
$$[L^{3}]$$.
The SI unit for **volume** is: cubic metre with the associated unit label $m^{3}$
The meaningful precision of volume in the drilling context is typically: 0.0001 m³
"""@EN; 
                             rdfs:subClassOf ddhub:MeasurableQuantity. 
ddhub:VolumeLargeQuantity a owl:Class; 
                          rdfs:comment """A volume is the amount of three-dimensional space occupied by a body.
The dimension of volume is:
$$[L^{3}]$$.
The SI unit for **volume** is: cubic metre with the associated unit label $m^{3}$
The meaningful precision of a large volume is typically: 0.1 m³
"""@EN; 
                          rdfs:subClassOf ddhub:MeasurableQuantity. 
ddhub:VolumeQuantity a owl:Class; 
                     rdfs:comment """A volume is the amount of three-dimensional space occupied by a body.
The dimension of volume is:
$$[L^{3}]$$.
The SI unit for **volume** is: cubic metre with the associated unit label $m^{3}$
"""@EN; 
                     rdfs:subClassOf ddhub:Quantity. 
ddhub:VolumetricFlowrateDrillingQuantity a owl:Class; 
                                         rdfs:comment """A volumetric flowrate is the volume of fluid that passes per unit time: $\\frac{dV}{dt}$, where $V$ is a volume and $t$ is time.
The dimension of volumetric flowrate is:
$$[L^{3}T^{-1}]$$.
The SI unit for **volumetric flow rate** is: cubic metre per second with the associated unit label $\\frac{m^{3}}{s}$
The meaningful precision of volumetric flowrate in the drilling context is typically: 0.0001 ft³/s
"""@EN; 
                                         rdfs:subClassOf ddhub:MeasurableQuantity. 
ddhub:VolumetricFlowRateOfChangeDrillingQuantity a owl:Class; 
                                                 rdfs:comment """A volumetric flow rate of change is the time derivative of a volumetric flowrate: $\\frac{dQ}{dt}$, where $Q$ is a volumetric flowrate and $t$ is time.
The dimension of volumetric flow rate of change is:
$$[L^{3}T^{-2}]$$.
The SI unit for **volumetric flow Rate rate of change** is: cubic metre per second squared with the associated unit label $\\frac{m^{3}}{s^{2}}$
The meaningful precision of volumetric flow rate of change in the drilling context is typically: 1E-06 m³/s²
"""@EN; 
                                                 rdfs:subClassOf ddhub:MeasurableQuantity. 
ddhub:VolumetricFlowRateOfChangeQuantity a owl:Class; 
                                         rdfs:comment """A volumetric flow rate of change is the time derivative of a volumetric flowrate: $\\frac{dQ}{dt}$, where $Q$ is a volumetric flowrate and $t$ is time.
The dimension of volumetric flow rate of change is:
$$[L^{3}T^{-2}]$$.
The SI unit for **volumetric flow Rate rate of change** is: cubic metre per second squared with the associated unit label $\\frac{m^{3}}{s^{2}}$
"""@EN; 
                                         rdfs:subClassOf ddhub:Quantity. 
ddhub:VolumetricFlowRateQuantity a owl:Class; 
                                 rdfs:comment """A volumetric flowrate is the volume of fluid that passes per unit time: $\\frac{dV}{dt}$, where $V$ is a volume and $t$ is time.
The dimension of volumetric flowrate is:
$$[L^{3}T^{-1}]$$.
The SI unit for **volumetric flow rate** is: cubic metre per second with the associated unit label $\\frac{m^{3}}{s}$
"""@EN; 
                                 rdfs:subClassOf ddhub:Quantity. 
ddhub:WaterBasedMudWbm a owl:Class; 
                       rdfs:comment ""@EN; 
                       rdfs:subClassOf ddhub:DrillingFluid. 
ddhub:WaveNumberQuantity a owl:Class; 
                         rdfs:comment """A wave number is the number of wave lengths per unit distance.
The dimension of wave number is:
$$[L^{-1}]$$.
The SI unit for **wave number** is: reciprocal metre with the associated unit label $\\frac{1}{m}$
"""@EN; 
                         rdfs:subClassOf ddhub:Quantity. 
ddhub:WeightOnBitDrillingQuantity a owl:Class; 
                                  rdfs:comment """Mass can be experimentally defined as a measure of the body's inertia, meaning the resistance to acceleration (change of velocity) when a net force is applied. The object's mass also determines the strength of its gravitational attraction to other bodies.
The dimension of mass is:
$$[M]$$.
The SI unit for **mass** is: kilogram with the associated unit label $kg$
The meaningful precision of weight on bit in the drilling context is typically: 10 kg
"""@EN; 
                                  rdfs:subClassOf ddhub:MeasurableQuantity. 
ddhub:WellboreCenterLineFrame a owl:Class; 
                              rdfs:comment ""@EN; 
                              rdfs:subClassOf ddhub:OneDimensionalCurviLinearReferenceFrame. 
ddhub:WellboreName a owl:DatatypeProperty, owl:FunctionalProperty; 
                   rdfs:comment """
"""@EN; 
                   rdfs:domain ddhub:WitsMLTimeBasedLogEndPoint; 
                   rdfs:range xsd:string. 
ddhub:WellboreUID a owl:DatatypeProperty, owl:FunctionalProperty; 
                  rdfs:comment """
"""@EN; 
                  rdfs:domain ddhub:WitsMLTimeBasedLogEndPoint; 
                  rdfs:range xsd:string. 
ddhub:WellcontrolStackEquipment a owl:Class; 
                                rdfs:comment ""@EN; 
                                rdfs:subClassOf ddhub:CoiledTubingEquipment. 
ddhub:WellControlSystem a owl:Class; 
                        rdfs:comment ""@EN; 
                        rdfs:subClassOf ddhub:RigEquipment. 
ddhub:WellHeadPositionLocation a owl:Class; 
                               rdfs:comment ""@EN; 
                               rdfs:subClassOf ddhub:PositionReferenceLocation. 
ddhub:WellHeadVerticalLocation a owl:Class; 
                               rdfs:comment ""@EN; 
                               rdfs:subClassOf ddhub:VerticalReferenceLocation. 
ddhub:WellheadXmasTree a owl:Class; 
                       rdfs:comment ""@EN; 
                       rdfs:subClassOf ddhub:WellControlSystem. 
ddhub:WellName a owl:DatatypeProperty, owl:FunctionalProperty; 
               rdfs:comment """
"""@EN; 
               rdfs:domain ddhub:WitsMLTimeBasedLogEndPoint; 
               rdfs:range xsd:string. 
ddhub:WellTestingEquipment a owl:Class; 
                           rdfs:comment ""@EN; 
                           rdfs:subClassOf ddhub:RigEquipment. 
ddhub:WellUID a owl:DatatypeProperty, owl:FunctionalProperty; 
              rdfs:comment """
"""@EN; 
              rdfs:domain ddhub:WitsMLTimeBasedLogEndPoint; 
              rdfs:range xsd:string. 
ddhub:WGS84PositionLocation a owl:Class; 
                            rdfs:comment ""@EN; 
                            rdfs:subClassOf ddhub:PositionReferenceLocation. 
ddhub:WGS84VerticalLocation a owl:Class; 
                            rdfs:comment ""@EN; 
                            rdfs:subClassOf ddhub:VerticalReferenceLocation. 
ddhub:Whipstock a owl:Class; 
                rdfs:comment ""@EN; 
                rdfs:subClassOf ddhub:DrillingEquipment. 
ddhub:Whirling a owl:Class; 
               rdfs:comment ""@EN; 
               rdfs:subClassOf ddhub:AbnormalLateralOscillation. 
ddhub:WireCable a owl:Class; 
                rdfs:comment ""@EN; 
                rdfs:subClassOf ddhub:EquipmentTelemetry. 
ddhub:WiredPipe a owl:Class; 
                rdfs:comment ""@EN; 
                rdfs:subClassOf ddhub:EquipmentTelemetry. 
ddhub:WiredPipeTelemetry a owl:Class; 
                         rdfs:comment """A method that allows transfer of downhole data to the surface via electrical connections through the drill string.
"""@EN; 
                         rdfs:subClassOf ddhub:DownHoleTelemetry. 
ddhub:WirelineLoggingTools a owl:Class; 
                           rdfs:comment ""@EN; 
                           rdfs:subClassOf ddhub:LoggingEquipment. 
ddhub:WirelineLoggingToolsAcoustictools a owl:Class; 
                                        rdfs:comment ""@EN; 
                                        rdfs:subClassOf ddhub:WirelineLoggingTools. 
ddhub:WirelineLoggingToolsElectricalpropagation a owl:Class; 
                                                rdfs:comment ""@EN; 
                                                rdfs:subClassOf ddhub:WirelineLoggingTools. 
ddhub:WirelineLoggingToolsElectricalresistivity a owl:Class; 
                                                rdfs:comment ""@EN; 
                                                rdfs:subClassOf ddhub:WirelineLoggingTools. 
ddhub:WirelineLoggingToolsNmrtools a owl:Class; 
                                   rdfs:comment ""@EN; 
                                   rdfs:subClassOf ddhub:WirelineLoggingTools. 
ddhub:WirelineLoggingToolsNucleartools a owl:Class; 
                                       rdfs:comment ""@EN; 
                                       rdfs:subClassOf ddhub:WirelineLoggingTools. 
ddhub:WirelineLoggingToolsSeismictools a owl:Class; 
                                       rdfs:comment ""@EN; 
                                       rdfs:subClassOf ddhub:WirelineLoggingTools. 
ddhub:WitsMLTimeBasedLogEndPoint a owl:Class; 
                                 rdfs:comment ""@EN; 
                                 rdfs:subClassOf ddhub:DataEndPoint. 
ddhub:WOB a owl:Class; 
          rdfs:comment ""@EN; 
          rdfs:subClassOf ddhub:PrototypeData. 
