@prefix ddhub: <http://ddhub.no/>.
@prefix owl: <http://www.w3.org/2002/07/owl#>.
@prefix rdf: <http://www.w3.org/1999/02/22-rdf-syntax-ns#>.
@prefix rdfs: <http://www.w3.org/2000/01/rdf-schema#>.
@prefix xsd: <http://www.w3.org/2001/XMLSchema#>.
@base <https://rdfsharp.codeplex.com/>.

<http://ddhub.no/<equipment>> a owl:Class; 
                              rdfs:comment """
"""@EN; 
                              rdfs:subClassOf ddhub:DWISNoun. 
<http://ddhub.no/<Tubulars>> a owl:Class; 
                             rdfs:comment """
"""@EN; 
                             rdfs:subClassOf <http://ddhub.no/<equipment>>. 
ddhub:AbscissaReferenceLocation a owl:Class; 
                                rdfs:comment """
"""@EN; 
                                rdfs:subClassOf ddhub:Location. 
ddhub:AbsolutePressureReference a owl:Class; 
                                rdfs:comment """
"""@EN; 
                                rdfs:subClassOf ddhub:PressureReference. 
ddhub:AbsoluteTimeReference a owl:Class; 
                            rdfs:comment """
"""@EN; 
                            rdfs:subClassOf ddhub:TimeReference. 
ddhub:AccelerationQuantity a owl:Class; 
                           rdfs:comment """
"""@EN; 
                           rdfs:subClassOf ddhub:Quantity. 
ddhub:Accelerator a owl:Class; 
                  rdfs:comment """
"""@EN; 
                  rdfs:subClassOf ddhub:JarringAssembly. 
ddhub:Accumulator a owl:Class; 
                  rdfs:comment """
"""@EN; 
                  rdfs:subClassOf ddhub:WellControlSystem. 
ddhub:Accuracy a owl:DatatypeProperty, owl:FunctionalProperty; 
               rdfs:comment """The standard deviation of the systematic bias component of the uncertainty of the sensor. The assumed mean value of the attached Gaussian distribution is the measured value. The value is expected to be in the same physical quantity as the sensor value.
"""@EN; 
               rdfs:domain ddhub:SensorUncertainty; 
               rdfs:range xsd:double. 
ddhub:Acoustic a owl:Class; 
               rdfs:comment """
"""@EN; 
               rdfs:subClassOf ddhub:EquipmentTelemetry. 
ddhub:Action a owl:Class; 
             rdfs:comment """
"""@EN; 
             rdfs:subClassOf ddhub:PistonMudPump. 
ddhub:ActivableFunction a owl:Class; 
                        rdfs:comment """An `ActivableFunction` is an ADCS function that can be activated. Here activation means that the
function may run immediately or that it is enabled and can trigger if some conditions are respected.
"""@EN; 
                        rdfs:subClassOf ddhub:DWISNoun. 
ddhub:ActiveDrillingSystem a owl:Class; 
                           rdfs:comment """
"""@EN; 
                           rdfs:subClassOf ddhub:MudPits. 
ddhub:ActiveLine a owl:Class; 
                 rdfs:comment """
"""@EN; 
                 rdfs:subClassOf ddhub:DrillLine. 
ddhub:ActiveVibrationTools a owl:Class; 
                           rdfs:comment """
"""@EN; 
                           rdfs:subClassOf ddhub:DrillingEquipment. 
ddhub:ActiveVolume a owl:Class; 
                   rdfs:comment """
"""@EN; 
                   rdfs:subClassOf ddhub:PrototypeData. 
ddhub:AdapterSpool a owl:Class; 
                   rdfs:comment """
"""@EN; 
                   rdfs:subClassOf ddhub:WellControlSystem. 
ddhub:AdjustableKickoffSub a owl:Class; 
                           rdfs:comment """
"""@EN; 
                           rdfs:subClassOf ddhub:DrillingEquipment. 
ddhub:Advice a owl:Class; 
             rdfs:comment """
"""@EN; 
             rdfs:subClassOf ddhub:ProcessData. 
ddhub:AdviceType a owl:DatatypeProperty, owl:FunctionalProperty; 
                 rdfs:comment """
"""@EN; 
                 rdfs:domain ddhub:Advisor; 
                 rdfs:range xsd:string. 
ddhub:AdvisedMaximum a owl:Class; 
                     rdfs:comment """
"""@EN; 
                     rdfs:subClassOf ddhub:Advice. 
ddhub:AdvisedMinimum a owl:Class; 
                     rdfs:comment """
"""@EN; 
                     rdfs:subClassOf ddhub:Advice. 
ddhub:AdvisedTarget a owl:Class; 
                    rdfs:comment """
"""@EN; 
                    rdfs:subClassOf ddhub:Advice. 
ddhub:Advisor a owl:Class; 
              rdfs:comment """
"""@EN; 
              rdfs:subClassOf ddhub:ComputationUnit. 
ddhub:AfmAutofluidMeasSkid a owl:Class; 
                           rdfs:comment """
"""@EN; 
                           rdfs:subClassOf ddhub:CirculationSystem. 
ddhub:Aggregation a owl:Class; 
                  rdfs:comment """
"""@EN; 
                  rdfs:subClassOf ddhub:DirectTransformation. 
ddhub:AllowEnablementSignalFor a owl:ObjectProperty; 
                               rdfs:comment """This verb is used to define a `DrillingDataPoint` tells if it is allowed or not to enable or
disable an activable function. It is expected that the `DrillingDataPoint` is a Boolean value. If the signal is true,
then it is possible to enable or disable the function using the signal associated with `IsEnablingSignalFor`. If it is
false, it is not allowed to enable or disable the `ActivableFunction`, meaning that the signal associated with `IsEnablingSignalFor`
is ignored.
"""@EN; 
                               rdfs:domain ddhub:DrillingDataPoint; 
                               rdfs:range ddhub:ActivableFunction; 
                               rdfs:subPropertyOf ddhub:DWISVerb. 
ddhub:AmountSubstanceQuantity a owl:Class; 
                              rdfs:comment """
"""@EN; 
                              rdfs:subClassOf ddhub:Quantity. 
ddhub:Anchors a owl:Class; 
              rdfs:comment """
"""@EN; 
              rdfs:subClassOf ddhub:MooringSystem. 
ddhub:AngleMagneticFluxDensityQuantity a owl:Class; 
                                       rdfs:comment """
"""@EN; 
                                       rdfs:subClassOf ddhub:Quantity. 
ddhub:AngleReferenceFrame a owl:Class; 
                          rdfs:comment """
"""@EN; 
                          rdfs:subClassOf ddhub:OneDimensionalReferenceFrame. 
ddhub:AngleReferenceLocation a owl:Class; 
                             rdfs:comment """
"""@EN; 
                             rdfs:subClassOf ddhub:Location. 
ddhub:AngleVariationGradientQuantity a owl:Class; 
                                     rdfs:comment """
"""@EN; 
                                     rdfs:subClassOf ddhub:Quantity. 
ddhub:AngularLateralModelling a owl:Class; 
                              rdfs:comment """The model accounts for the angular lateral movement of some parts of the physical system.
"""@EN; 
                              rdfs:subClassOf ddhub:LateralModelling. 
ddhub:AngularVelocityQuantity a owl:Class; 
                              rdfs:comment """
"""@EN; 
                              rdfs:subClassOf ddhub:Quantity. 
ddhub:Annular a owl:Class; 
              rdfs:comment """
"""@EN; 
              rdfs:subClassOf ddhub:HydraulicBranch. 
ddhub:AnnularPreventer a owl:Class; 
                       rdfs:comment """
"""@EN; 
                       rdfs:subClassOf ddhub:BopElement. 
ddhub:AreaQuantity a owl:Class; 
                   rdfs:comment """
"""@EN; 
                   rdfs:subClassOf ddhub:Quantity. 
ddhub:AssociatesMeasurableQuantity a owl:ObjectProperty; 
                                   rdfs:comment """
"""@EN; 
                                   rdfs:domain ddhub:MeasurableQuantityUnitAssociation; 
                                   rdfs:range ddhub:MeasurableQuantity; 
                                   rdfs:subPropertyOf ddhub:DWISVerb. 
ddhub:AssociatesUnit a owl:ObjectProperty; 
                     rdfs:comment """
"""@EN; 
                     rdfs:domain ddhub:MeasurableQuantityUnitAssociation; 
                     rdfs:range ddhub:Unit; 
                     rdfs:subPropertyOf ddhub:DWISVerb. 
ddhub:AverageDelayByRepeater a owl:DatatypeProperty, owl:FunctionalProperty; 
                             rdfs:comment """
"""@EN; 
                             rdfs:domain ddhub:Telemetry; 
                             rdfs:range xsd:double. 
ddhub:AxialModelling a owl:Class; 
                     rdfs:comment """The model accounts for the axial movement of some parts of the physical system.
"""@EN; 
                     rdfs:subClassOf ddhub:ModelledDegreeOfFreedom. 
ddhub:AxialMotionType a owl:Class; 
                      rdfs:comment """
"""@EN; 
                      rdfs:subClassOf ddhub:MotionType. 
ddhub:AxialReferenceLocation a owl:Class; 
                             rdfs:comment """
"""@EN; 
                             rdfs:subClassOf ddhub:Location. 
ddhub:Azimuth a owl:Class; 
              rdfs:comment """
"""@EN; 
              rdfs:subClassOf ddhub:PrototypeData. 
ddhub:AzimuthalTools a owl:Class; 
                     rdfs:comment """
"""@EN; 
                     rdfs:subClassOf ddhub:LoggingWhileDrillingTools. 
ddhub:AzimuthReferenceLocation a owl:Class; 
                               rdfs:comment """
"""@EN; 
                               rdfs:subClassOf ddhub:Location. 
ddhub:BackPressurePump a owl:Class; 
                       rdfs:comment """
"""@EN; 
                       rdfs:subClassOf ddhub:CirculationSystem. 
ddhub:BackPressurePumpPressure a owl:Class; 
                               rdfs:comment """
"""@EN; 
                               rdfs:subClassOf ddhub:PrototypeData. 
ddhub:BallastSystem a owl:Class; 
                    rdfs:comment """
"""@EN; 
                    rdfs:subClassOf ddhub:MarineSystem. 
ddhub:BallJoint a owl:Class; 
                rdfs:comment """
"""@EN; 
                rdfs:subClassOf ddhub:DrillingRiser. 
ddhub:BandPassFilter a owl:Class; 
                     rdfs:comment """
"""@EN; 
                     rdfs:subClassOf ddhub:Filter. 
ddhub:Beacons a owl:Class; 
              rdfs:comment """
"""@EN; 
              rdfs:subClassOf ddhub:MarineSystem. 
ddhub:BellNipple a owl:Class; 
                 rdfs:comment """
"""@EN; 
                 rdfs:subClassOf ddhub:WellControlSystem. 
ddhub:BelongsToClass a owl:ObjectProperty; 
                     rdfs:comment """The verb is used between a node and a Noun, i.e., a class. Semantically it can be considered as a synonym to `rdf:type`. It has been introduced to overcome limitations from OPC-UA that does not allow for multiple inheritance. Note that the same node can be in relation using `BelongsToClass` to several classes.
"""@EN; 
                     rdfs:domain ddhub:DWISNoun; 
                     rdfs:range ddhub:DWISNoun; 
                     rdfs:subPropertyOf ddhub:DWISVerb. 
ddhub:BelongsToSynchronizationGroup a owl:ObjectProperty; 
                                    rdfs:comment """
"""@EN; 
                                    rdfs:domain ddhub:Resampling; 
                                    rdfs:range ddhub:SynchronizationGroup; 
                                    rdfs:subPropertyOf ddhub:DWISVerb. 
ddhub:BHAAnnular a owl:Class; 
                 rdfs:comment """
"""@EN; 
                 rdfs:subClassOf ddhub:Annular. 
ddhub:BHAInner a owl:Class; 
               rdfs:comment """
"""@EN; 
               rdfs:subClassOf ddhub:Pipe. 
ddhub:BhaVibrationDampers a owl:Class; 
                          rdfs:comment """
"""@EN; 
                          rdfs:subClassOf ddhub:ActiveVibrationTools. 
ddhub:BicenterReamerBit a owl:Class; 
                        rdfs:comment """
"""@EN; 
                        rdfs:subClassOf ddhub:Reamers. 
ddhub:BitDepth a owl:Class; 
               rdfs:comment """Curvilinear abscissa of the bottom of the bit, in the reference frame centered in the wellbore.
"""@EN; 
               rdfs:subClassOf ddhub:PrototypeData. 
ddhub:BladeDiameter a owl:Class; 
                    rdfs:comment """
"""@EN; 
                    rdfs:subClassOf ddhub:Stabilizers. 
ddhub:BladeLength a owl:Class; 
                  rdfs:comment """
"""@EN; 
                  rdfs:subClassOf ddhub:Stabilizers. 
ddhub:BladeShape a owl:Class; 
                 rdfs:comment """
"""@EN; 
                 rdfs:subClassOf ddhub:Stabilizers. 
ddhub:BladeType a owl:Class; 
                rdfs:comment """
"""@EN; 
                rdfs:subClassOf ddhub:Stabilizers. 
ddhub:BladeTypeWelded a owl:Class; 
                      rdfs:comment """
"""@EN; 
                      rdfs:subClassOf ddhub:BladeType. 
ddhub:BlindRam a owl:Class; 
               rdfs:comment """
"""@EN; 
               rdfs:subClassOf ddhub:BopElement. 
ddhub:BlockVelocityQuantity a owl:Class; 
                            rdfs:comment """
"""@EN; 
                            rdfs:subClassOf ddhub:MeasurableQuantity. 
ddhub:BooleanDataType a owl:Class; 
                      rdfs:comment """
"""@EN; 
                      rdfs:subClassOf ddhub:EnumerationDataType. 
ddhub:BoosterLine a owl:Class; 
                  rdfs:comment """
"""@EN; 
                  rdfs:subClassOf ddhub:MarineSystem. 
ddhub:BoosterPump a owl:Class; 
                  rdfs:comment """
"""@EN; 
                  rdfs:subClassOf ddhub:CirculationSystem. 
ddhub:BOPControlSystem a owl:Class; 
                       rdfs:comment """
"""@EN; 
                       rdfs:subClassOf ddhub:ControlSystem. 
ddhub:BopElement a owl:Class; 
                 rdfs:comment """
"""@EN; 
                 rdfs:subClassOf ddhub:WellControlSystem. 
ddhub:BOPOpening a owl:Class; 
                 rdfs:comment """
"""@EN; 
                 rdfs:subClassOf ddhub:PrototypeData. 
ddhub:BOPPressure a owl:Class; 
                  rdfs:comment """
"""@EN; 
                  rdfs:subClassOf ddhub:PrototypeData. 
ddhub:BopStack a owl:Class; 
               rdfs:comment """
"""@EN; 
               rdfs:subClassOf ddhub:WellControlSystem. 
ddhub:BottomholeAssembly a owl:Class; 
                         rdfs:comment """
"""@EN; 
                         rdfs:subClassOf ddhub:DrillString. 
ddhub:BottomOfStringReferenceLocation a owl:Class; 
                                      rdfs:comment """
"""@EN; 
                                      rdfs:subClassOf ddhub:AbscissaReferenceLocation. 
ddhub:BottomShoulderAxialLocation a owl:Class; 
                                  rdfs:comment """
"""@EN; 
                                  rdfs:subClassOf ddhub:AxialReferenceLocation. 
ddhub:BoundaryDiscretization a owl:Class; 
                             rdfs:comment """A model only considers the bounds of the physical system and does not apply any intermediate discretization.
"""@EN; 
                             rdfs:subClassOf ddhub:ModellingDiscretization. 
ddhub:box a owl:Class; 
          rdfs:comment """
"""@EN; 
          rdfs:subClassOf ddhub:Connection. 
ddhub:Box-Box a owl:Class; 
              rdfs:comment """
"""@EN; 
              rdfs:subClassOf ddhub:TubularConfiguration. 
ddhub:Buffering a owl:Class; 
                rdfs:comment """
"""@EN; 
                rdfs:subClassOf ddhub:TimeBasedTransformation. 
ddhub:BufferingInterval a owl:DatatypeProperty, owl:FunctionalProperty; 
                        rdfs:comment """
"""@EN; 
                        rdfs:domain ddhub:Buffering; 
                        rdfs:range xsd:double. 
ddhub:BulkTank a owl:Class; 
               rdfs:comment """
"""@EN; 
               rdfs:subClassOf ddhub:MudPits. 
ddhub:BullNose a owl:Class; 
               rdfs:comment """
"""@EN; 
               rdfs:subClassOf ddhub:DrillstemTerminator. 
ddhub:CableDiameterQuantity a owl:Class; 
                            rdfs:comment """
"""@EN; 
                            rdfs:subClassOf ddhub:MeasurableQuantity. 
ddhub:CapillaryPressureQuantity a owl:Class; 
                                rdfs:comment """
"""@EN; 
                                rdfs:subClassOf ddhub:MeasurableQuantity. 
ddhub:CartesianFourDimensionalReferenceFrame a owl:Class; 
                                             rdfs:comment """
"""@EN; 
                                             rdfs:subClassOf ddhub:FourDimensionalReferenceFrame. 
ddhub:CartesianThreeDimensionalReferenceFrame a owl:Class; 
                                              rdfs:comment """
"""@EN; 
                                              rdfs:subClassOf ddhub:ThreeDimensionalReferenceFrame. 
ddhub:CartesianTwoDimensionalReferenceFrame a owl:Class; 
                                            rdfs:comment """
"""@EN; 
                                            rdfs:subClassOf ddhub:TwoDimensionalReferenceFrame. 
ddhub:CasedHoleTools a owl:Class; 
                     rdfs:comment """
"""@EN; 
                     rdfs:subClassOf ddhub:WirelineLoggingTools. 
ddhub:Casing a owl:Class; 
             rdfs:comment """
"""@EN; 
             rdfs:subClassOf ddhub:CasingString. 
ddhub:Casing-While-Drilling a owl:Class; 
                            rdfs:comment """
"""@EN; 
                            rdfs:subClassOf ddhub:DrillingEquipment. 
ddhub:CasingCollarLocator a owl:Class; 
                          rdfs:comment """
"""@EN; 
                          rdfs:subClassOf ddhub:WirelineLoggingTools. 
ddhub:CasingCutter a owl:Class; 
                   rdfs:comment """
"""@EN; 
                   rdfs:subClassOf ddhub:CasingEquipment. 
ddhub:CasingEquipment a owl:Class; 
                      rdfs:comment """
"""@EN; 
                      rdfs:subClassOf ddhub:DownholeEquipment. 
ddhub:CasingFlangeVerticalLocation a owl:Class; 
                                   rdfs:comment """
"""@EN; 
                                   rdfs:subClassOf ddhub:VerticalReferenceLocation. 
ddhub:CasingHanger a owl:Class; 
                   rdfs:comment """
"""@EN; 
                   rdfs:subClassOf ddhub:Hangers. 
ddhub:CasingHead a owl:Class; 
                 rdfs:comment """
"""@EN; 
                 rdfs:subClassOf ddhub:CasingEquipment. 
ddhub:CasingLinerEquipment a owl:Class; 
                           rdfs:comment """
"""@EN; 
                           rdfs:subClassOf ddhub:CasingEquipment. 
ddhub:CasingMillingTools a owl:Class; 
                         rdfs:comment """
"""@EN; 
                         rdfs:subClassOf ddhub:CasingEquipment. 
ddhub:CasingShoe a owl:Class; 
                 rdfs:comment """
"""@EN; 
                 rdfs:subClassOf ddhub:CasingEquipment. 
ddhub:CasingString a owl:Class; 
                   rdfs:comment """
"""@EN; 
                   rdfs:subClassOf <http://ddhub.no/<Tubulars>>. 
ddhub:CasingTongs a owl:Class; 
                  rdfs:comment """
"""@EN; 
                  rdfs:subClassOf ddhub:DrillPipeTongs. 
ddhub:CavingsComponent a owl:Class; 
                       rdfs:comment """
"""@EN; 
                       rdfs:subClassOf ddhub:FormationSolidComponent. 
ddhub:CementBondLoggingTools a owl:Class; 
                             rdfs:comment """
"""@EN; 
                             rdfs:subClassOf ddhub:WirelineLoggingTools. 
ddhub:CementHead a owl:Class; 
                 rdfs:comment """
"""@EN; 
                 rdfs:subClassOf ddhub:CementingEquipment. 
ddhub:CementingEquipment a owl:Class; 
                         rdfs:comment """
"""@EN; 
                         rdfs:subClassOf ddhub:RigEquipment. 
ddhub:CementingServiceCompany a owl:Class; 
                              rdfs:comment """
"""@EN; 
                              rdfs:subClassOf ddhub:ServiceCompany. 
ddhub:CementLines a owl:Class; 
                  rdfs:comment """
"""@EN; 
                  rdfs:subClassOf ddhub:CementingEquipment. 
ddhub:CementManifold a owl:Class; 
                     rdfs:comment """
"""@EN; 
                     rdfs:subClassOf ddhub:CementingEquipment. 
ddhub:CementPump a owl:Class; 
                 rdfs:comment """
"""@EN; 
                 rdfs:subClassOf ddhub:CementingEquipment. 
ddhub:CementSlurry a owl:Class; 
                   rdfs:comment """
"""@EN; 
                   rdfs:subClassOf ddhub:CementingEquipment. 
ddhub:CementSpacer a owl:Class; 
                   rdfs:comment """
"""@EN; 
                   rdfs:subClassOf ddhub:CementingEquipment. 
ddhub:CementStand a owl:Class; 
                  rdfs:comment """
"""@EN; 
                  rdfs:subClassOf ddhub:CementingEquipment. 
ddhub:CementStinger a owl:Class; 
                    rdfs:comment """
"""@EN; 
                    rdfs:subClassOf ddhub:CementingEquipment. 
ddhub:CementUnit a owl:Class; 
                 rdfs:comment """
"""@EN; 
                 rdfs:subClassOf ddhub:CementingEquipment. 
ddhub:Centralizers a owl:Class; 
                   rdfs:comment """
"""@EN; 
                   rdfs:subClassOf ddhub:CasingString. 
ddhub:CentrifugalDegasser a owl:Class; 
                          rdfs:comment """
"""@EN; 
                          rdfs:subClassOf ddhub:Degasser. 
ddhub:CentrifugalMudPump a owl:Class; 
                         rdfs:comment """
"""@EN; 
                         rdfs:subClassOf ddhub:MudPump. 
ddhub:Centrifuge a owl:Class; 
                 rdfs:comment """
"""@EN; 
                 rdfs:subClassOf ddhub:CirculationSystem. 
ddhub:ChemicalTank a owl:Class; 
                   rdfs:comment """
"""@EN; 
                   rdfs:subClassOf ddhub:MudPits. 
ddhub:ChokeLine a owl:Class; 
                rdfs:comment """
"""@EN; 
                rdfs:subClassOf ddhub:WellControlSystem. 
ddhub:ChokeManifold a owl:Class; 
                    rdfs:comment """
"""@EN; 
                    rdfs:subClassOf ddhub:WellControlSystem. 
ddhub:ChokeValve a owl:Class; 
                 rdfs:comment """
"""@EN; 
                 rdfs:subClassOf ddhub:ChokeManifold. 
ddhub:ChokeValveGatevalve a owl:Class; 
                          rdfs:comment """
"""@EN; 
                          rdfs:subClassOf ddhub:ChokeValve. 
ddhub:CirculationSub a owl:Class; 
                     rdfs:comment """
"""@EN; 
                     rdfs:subClassOf ddhub:DrillingEquipment. 
ddhub:CirculationSystem a owl:Class; 
                        rdfs:comment """
"""@EN; 
                        rdfs:subClassOf ddhub:RigEquipment. 
ddhub:clamp-on a owl:Class; 
               rdfs:comment """
"""@EN; 
               rdfs:subClassOf ddhub:BladeType. 
ddhub:Clock a owl:Class; 
            rdfs:comment """Represents a clock
"""@EN; 
            rdfs:subClassOf ddhub:DWISNoun. 
ddhub:ClusterPositionLocation a owl:Class; 
                              rdfs:comment """
"""@EN; 
                              rdfs:subClassOf ddhub:PositionReferenceLocation. 
ddhub:CoiledTubingEquipment a owl:Class; 
                            rdfs:comment """
"""@EN; 
                            rdfs:subClassOf <http://ddhub.no/<equipment>>. 
ddhub:CoiledTubingReel a owl:Class; 
                       rdfs:comment """
"""@EN; 
                       rdfs:subClassOf ddhub:CoiledTubingEquipment. 
ddhub:CollapsePressure a owl:Class; 
                       rdfs:comment """
"""@EN; 
                       rdfs:subClassOf ddhub:PrototypeData. 
ddhub:CollapsePressureGradient a owl:Class; 
                               rdfs:comment """
"""@EN; 
                               rdfs:subClassOf ddhub:PrototypeData. 
ddhub:Command a owl:Class; 
              rdfs:comment """
"""@EN; 
              rdfs:subClassOf ddhub:ProcessData. 
ddhub:CompletionWorkoverRiser a owl:Class; 
                              rdfs:comment """
"""@EN; 
                              rdfs:subClassOf ddhub:MarineSystem. 
ddhub:CompressibilityQuantity a owl:Class; 
                              rdfs:comment """
"""@EN; 
                              rdfs:subClassOf ddhub:Quantity. 
ddhub:CompressiveDrillPipe a owl:Class; 
                           rdfs:comment """
"""@EN; 
                           rdfs:subClassOf ddhub:DrillString. 
ddhub:ComputationUnit a owl:Class; 
                      rdfs:comment """Denotes a complex computation unit, typically based on advanced numerical modeling
"""@EN; 
                      rdfs:subClassOf ddhub:DataFlowNode. 
ddhub:ComputedData a owl:Class; 
                   rdfs:comment """
"""@EN; 
                   rdfs:subClassOf ddhub:PhysicalData. 
ddhub:ComputedState a owl:Class; 
                    rdfs:comment """A state represents the current configuation of a system.
"""@EN; 
                    rdfs:subClassOf ddhub:ComputationUnit. 
ddhub:ConcernsAFluidComponent a owl:ObjectProperty; 
                              rdfs:comment """
"""@EN; 
                              rdfs:domain ddhub:DrillingDataPoint; 
                              rdfs:range ddhub:FluidComponent; 
                              rdfs:subPropertyOf ddhub:DWISVerb. 
ddhub:ConductorDrivePipe a owl:Class; 
                         rdfs:comment """
"""@EN; 
                         rdfs:subClassOf ddhub:CasingString. 
ddhub:ConductorTensioners a owl:Class; 
                          rdfs:comment """
"""@EN; 
                          rdfs:subClassOf ddhub:MarineSystem. 
ddhub:ConnectedCondition a owl:Class; 
                         rdfs:comment """
"""@EN; 
                         rdfs:subClassOf ddhub:ValidityCondition. 
ddhub:Connection a owl:Class; 
                 rdfs:comment """
"""@EN; 
                 rdfs:subClassOf ddhub:CasingString. 
ddhub:ConnectionWelded a owl:Class; 
                       rdfs:comment """
"""@EN; 
                       rdfs:subClassOf ddhub:Connection. 
ddhub:ContinuousDataType a owl:Class; 
                         rdfs:comment """
"""@EN; 
                         rdfs:subClassOf ddhub:DataType. 
ddhub:ContinuousProportional a owl:Class; 
                             rdfs:comment """
"""@EN; 
                             rdfs:subClassOf ddhub:RotarySteerableSystems. 
ddhub:ControlAndMonitoringEquipment a owl:Class; 
                                    rdfs:comment """
"""@EN; 
                                    rdfs:subClassOf ddhub:ControlConsole. 
ddhub:ControlConsole a owl:Class; 
                     rdfs:comment """
"""@EN; 
                     rdfs:subClassOf ddhub:CoiledTubingEquipment. 
ddhub:Controller a owl:Class; 
                 rdfs:comment """
"""@EN; 
                 rdfs:subClassOf ddhub:DataFlowNode. 
ddhub:ControllerFunction a owl:Class; 
                         rdfs:comment """A `ControllerFunction` is a `RunnableFunction` that executes a feedback control loop to follow as closely
as possible one or several desired values. A typical example of `ControllerFunction` is the `AutoDriller`. An `AutoDriller` 
follows as closely as possible, for instance, a desired `WOB`.
"""@EN; 
                         rdfs:subClassOf ddhub:RunnableFunction. 
ddhub:ControlLines a owl:Class; 
                   rdfs:comment """
"""@EN; 
                   rdfs:subClassOf ddhub:WellControlSystem. 
ddhub:ControlManifold a owl:Class; 
                      rdfs:comment """
"""@EN; 
                      rdfs:subClassOf ddhub:WellControlSystem. 
ddhub:Controls a owl:ObjectProperty; 
               rdfs:comment """
"""@EN; 
               rdfs:domain ddhub:DWISNoun; 
               rdfs:range ddhub:DWISNoun; 
               rdfs:subPropertyOf ddhub:DWISVerb. 
ddhub:ControlSystem a owl:Class; 
                    rdfs:comment """
"""@EN; 
                    rdfs:subClassOf ddhub:DataFlowNode. 
ddhub:ConventionalDerrick a owl:Class; 
                          rdfs:comment """
"""@EN; 
                          rdfs:subClassOf ddhub:Derrick. 
ddhub:ConversionFactorA a owl:DatatypeProperty, owl:FunctionalProperty; 
                        rdfs:comment """Unit conversion from SI unit is performed as:
ConvertedValue = ConversionFactorA + SIValue * ConversionFactorB
"""@EN; 
                        rdfs:domain ddhub:Unit; 
                        rdfs:range xsd:double. 
ddhub:ConversionFactorB a owl:DatatypeProperty, owl:FunctionalProperty; 
                        rdfs:comment """Unit conversion from SI unit is performed as:
ConvertedValue = ConversionFactorA + SIValue * ConversionFactorB
"""@EN; 
                        rdfs:domain ddhub:Unit; 
                        rdfs:range xsd:double. 
ddhub:CoringTool a owl:Class; 
                 rdfs:comment """
"""@EN; 
                 rdfs:subClassOf ddhub:DrillingEquipment. 
ddhub:CorrectedMeasurement a owl:Class; 
                           rdfs:comment """
"""@EN; 
                           rdfs:subClassOf ddhub:Measurement. 
ddhub:Crossover a owl:Class; 
                rdfs:comment """
"""@EN; 
                rdfs:subClassOf ddhub:CasingString. 
ddhub:CrownBlock a owl:Class; 
                 rdfs:comment """
"""@EN; 
                 rdfs:subClassOf ddhub:MechanicalBlock. 
ddhub:CrownValveVerticalLocation a owl:Class; 
                                 rdfs:comment """
"""@EN; 
                                 rdfs:subClassOf ddhub:VerticalReferenceLocation. 
ddhub:CtBhaComponents a owl:Class; 
                      rdfs:comment """
"""@EN; 
                      rdfs:subClassOf ddhub:CoiledTubingEquipment. 
ddhub:CurvatureQuantity a owl:Class; 
                        rdfs:comment """
"""@EN; 
                        rdfs:subClassOf ddhub:Quantity. 
ddhub:CutOffFrequency a owl:DatatypeProperty, owl:FunctionalProperty; 
                      rdfs:comment """
"""@EN; 
                      rdfs:domain ddhub:HighPassFilter, ddhub:LowPassFilter; 
                      rdfs:range xsd:double. 
ddhub:CuttingsAnalysisEquipmnet a owl:Class; 
                                rdfs:comment """
"""@EN; 
                                rdfs:subClassOf ddhub:MudLoggingEquipment. 
ddhub:CuttingsBedLocation a owl:Class; 
                          rdfs:comment """
"""@EN; 
                          rdfs:subClassOf ddhub:AbscissaReferenceLocation. 
ddhub:CuttingsComponent a owl:Class; 
                        rdfs:comment """
"""@EN; 
                        rdfs:subClassOf ddhub:FormationSolidComponent. 
ddhub:CuttingsSamplingEquipment a owl:Class; 
                                rdfs:comment """
"""@EN; 
                                rdfs:subClassOf ddhub:MudLoggingEquipment. 
ddhub:Cylinders a owl:Class; 
                rdfs:comment """
"""@EN; 
                rdfs:subClassOf ddhub:PistonMudPump. 
ddhub:CylindricalReferenceFrame a owl:Class; 
                                rdfs:comment """
"""@EN; 
                                rdfs:subClassOf ddhub:ThreeDimensionalReferenceFrame. 
ddhub:DataAnalysisServiceCompany a owl:Class; 
                                 rdfs:comment """A data analysis service company is an entity that analyses measured data and provide new information from these measurements.
"""@EN; 
                                 rdfs:subClassOf ddhub:ServiceCompany. 
ddhub:DataEndPoint a owl:Class; 
                   rdfs:comment """
"""@EN; 
                   rdfs:subClassOf ddhub:DWISNoun. 
ddhub:DataFlowNode a owl:Class; 
                   rdfs:comment """
"""@EN; 
                   rdfs:subClassOf ddhub:DWISNoun. 
ddhub:DataProvider a owl:Class; 
                   rdfs:comment """A data provider is any sources for data
"""@EN; 
                   rdfs:subClassOf ddhub:DWISNoun. 
ddhub:DataType a owl:Class; 
               rdfs:comment """
"""@EN; 
               rdfs:subClassOf ddhub:DWISNoun. 
ddhub:DeadLine a owl:Class; 
               rdfs:comment """
"""@EN; 
               rdfs:subClassOf ddhub:DrillLine. 
ddhub:DeadLineAnchor a owl:Class; 
                     rdfs:comment """
"""@EN; 
                     rdfs:subClassOf ddhub:DrillLineFastener. 
ddhub:Degasser a owl:Class; 
               rdfs:comment """
"""@EN; 
               rdfs:subClassOf ddhub:CirculationSystem. 
ddhub:DensityGradientDepthQuantity a owl:Class; 
                                   rdfs:comment """
"""@EN; 
                                   rdfs:subClassOf ddhub:Quantity. 
ddhub:DensityGradientTemperatureQuantity a owl:Class; 
                                         rdfs:comment """
"""@EN; 
                                         rdfs:subClassOf ddhub:Quantity. 
ddhub:DensityIn a owl:Class; 
                rdfs:comment """
"""@EN; 
                rdfs:subClassOf ddhub:PrototypeData. 
ddhub:DensityOut a owl:Class; 
                 rdfs:comment """
"""@EN; 
                 rdfs:subClassOf ddhub:PrototypeData. 
ddhub:DensityQuantity a owl:Class; 
                      rdfs:comment """
"""@EN; 
                      rdfs:subClassOf ddhub:Quantity. 
ddhub:DensityRateOfChangeQuantity a owl:Class; 
                                  rdfs:comment """
"""@EN; 
                                  rdfs:subClassOf ddhub:Quantity. 
ddhub:DepthAndAngleFrame a owl:Class; 
                         rdfs:comment """
"""@EN; 
                         rdfs:subClassOf ddhub:ReferenceFrame. 
ddhub:DepthQuantity a owl:Class; 
                    rdfs:comment """
"""@EN; 
                    rdfs:subClassOf ddhub:MeasurableQuantity. 
ddhub:Derivation a owl:Class; 
                 rdfs:comment """
"""@EN; 
                 rdfs:subClassOf ddhub:TimeBasedTransformation. 
ddhub:DerivedMeasurement a owl:Class; 
                         rdfs:comment """
"""@EN; 
                         rdfs:subClassOf ddhub:Measurement. 
ddhub:Derrick a owl:Class; 
              rdfs:comment """
"""@EN; 
              rdfs:subClassOf ddhub:HoistingSystem. 
ddhub:DerrickFloorVerticalLocation a owl:Class; 
                                   rdfs:comment """
"""@EN; 
                                   rdfs:subClassOf ddhub:VerticalReferenceLocation. 
ddhub:DeterministicModel a owl:Class; 
                         rdfs:comment """
"""@EN; 
                         rdfs:subClassOf ddhub:ModelType. 
ddhub:Diamond a owl:Class; 
              rdfs:comment """
"""@EN; 
              rdfs:subClassOf ddhub:FixedCutter. 
ddhub:DiamondCore a owl:Class; 
                  rdfs:comment """
"""@EN; 
                  rdfs:subClassOf ddhub:FixedCutter. 
ddhub:DiaphragmMudPump a owl:Class; 
                       rdfs:comment """
"""@EN; 
                       rdfs:subClassOf ddhub:MudPump. 
ddhub:DieselElectricalDrawworks a owl:Class; 
                                rdfs:comment """
"""@EN; 
                                rdfs:subClassOf ddhub:Drawworks. 
ddhub:DifferentialStickingLocation a owl:Class; 
                                   rdfs:comment """
"""@EN; 
                                   rdfs:subClassOf ddhub:AbscissaReferenceLocation. 
ddhub:DimensionlessQuantity a owl:Class; 
                            rdfs:comment """
"""@EN; 
                            rdfs:subClassOf ddhub:Quantity. 
ddhub:DipmeterAndImagingTools a owl:Class; 
                              rdfs:comment """
"""@EN; 
                              rdfs:subClassOf ddhub:WirelineLoggingTools. 
ddhub:DirectionalCasingWhileDrilling a owl:Class; 
                                     rdfs:comment """
"""@EN; 
                                     rdfs:subClassOf ddhub:Casing-While-Drilling. 
ddhub:DirectionalServiceCompany a owl:Class; 
                                rdfs:comment """A directional service company is an entity that provides services for downhole directional drilling and downhole measurements.
"""@EN; 
                                rdfs:subClassOf ddhub:ServiceCompany. 
ddhub:DirectionalTool a owl:Class; 
                      rdfs:comment """
"""@EN; 
                      rdfs:subClassOf ddhub:MeasurementWhileDrillingTools. 
ddhub:DirectTransformation a owl:Class; 
                           rdfs:comment """Direct transformations are performed using only the current value of their inputs, time is not involved
"""@EN; 
                           rdfs:subClassOf ddhub:Transformation. 
ddhub:DiscreteDataType a owl:Class; 
                       rdfs:comment """
"""@EN; 
                       rdfs:subClassOf ddhub:DataType. 
ddhub:DistanceBetweenRepeaters a owl:DatatypeProperty, owl:FunctionalProperty; 
                               rdfs:comment """
"""@EN; 
                               rdfs:domain ddhub:Telemetry; 
                               rdfs:range xsd:double. 
ddhub:Diverter a owl:Class; 
               rdfs:comment """
"""@EN; 
               rdfs:subClassOf ddhub:WellControlSystem. 
ddhub:DiverterLine a owl:Class; 
                   rdfs:comment """
"""@EN; 
                   rdfs:subClassOf ddhub:Diverter. 
ddhub:DiverterLineHanger a owl:Class; 
                         rdfs:comment """
"""@EN; 
                         rdfs:subClassOf ddhub:Diverter. 
ddhub:DogHouse a owl:Class; 
               rdfs:comment """
"""@EN; 
               rdfs:subClassOf ddhub:DrillFloorStructure. 
ddhub:Dolly a owl:Class; 
            rdfs:comment """
"""@EN; 
            rdfs:subClassOf ddhub:DrillFloorEquipment. 
ddhub:DollyRail a owl:Class; 
                rdfs:comment """
"""@EN; 
                rdfs:subClassOf ddhub:DrillFloorEquipment. 
ddhub:Doubles a owl:Class; 
              rdfs:comment """
"""@EN; 
              rdfs:subClassOf ddhub:Grouping. 
ddhub:DoubleStandDerrick a owl:Class; 
                         rdfs:comment """
"""@EN; 
                         rdfs:subClassOf ddhub:Derrick. 
ddhub:DownholeAlternator a owl:Class; 
                         rdfs:comment """
"""@EN; 
                         rdfs:subClassOf ddhub:PowerSystems. 
ddhub:DownholeBatteries a owl:Class; 
                        rdfs:comment """
"""@EN; 
                        rdfs:subClassOf ddhub:PowerSystems. 
ddhub:DownholeCtConnectors a owl:Class; 
                           rdfs:comment """
"""@EN; 
                           rdfs:subClassOf ddhub:CoiledTubingEquipment. 
ddhub:DownholeECD a owl:Class; 
                  rdfs:comment """
"""@EN; 
                  rdfs:subClassOf ddhub:PrototypeData. 
ddhub:DownholeEquipment a owl:Class; 
                        rdfs:comment """
"""@EN; 
                        rdfs:subClassOf <http://ddhub.no/<equipment>>. 
ddhub:DownholeHydraulicNetwork a owl:Class; 
                               rdfs:comment """
"""@EN; 
                               rdfs:subClassOf ddhub:HydraulicNetwork. 
ddhub:DownholeMotor a owl:Class; 
                    rdfs:comment """
"""@EN; 
                    rdfs:subClassOf ddhub:DrillingEquipment. 
ddhub:DownholePressure a owl:Class; 
                       rdfs:comment """
"""@EN; 
                       rdfs:subClassOf ddhub:PrototypeData. 
ddhub:DownholeRPM a owl:Class; 
                  rdfs:comment """
"""@EN; 
                  rdfs:subClassOf ddhub:PrototypeData. 
ddhub:DownHoleTelemetry a owl:Class; 
                        rdfs:comment """
"""@EN; 
                        rdfs:subClassOf ddhub:Telemetry. 
ddhub:DownholeTemperature a owl:Class; 
                          rdfs:comment """
"""@EN; 
                          rdfs:subClassOf ddhub:PrototypeData. 
ddhub:DownholeTorque a owl:Class; 
                     rdfs:comment """
"""@EN; 
                     rdfs:subClassOf ddhub:PrototypeData. 
ddhub:DownholeValveAssembly a owl:Class; 
                            rdfs:comment """
"""@EN; 
                            rdfs:subClassOf ddhub:CasingEquipment. 
ddhub:Drawworks a owl:Class; 
                rdfs:comment """
"""@EN; 
                rdfs:subClassOf ddhub:HoistingSystem. 
ddhub:DrawWorksControlSystem a owl:Class; 
                             rdfs:comment """
"""@EN; 
                             rdfs:subClassOf ddhub:ControlSystem. 
ddhub:DrillCollars a owl:Class; 
                   rdfs:comment """
"""@EN; 
                   rdfs:subClassOf ddhub:DrillString. 
ddhub:DrillersConsole a owl:Class; 
                      rdfs:comment """
"""@EN; 
                      rdfs:subClassOf ddhub:DrillFloorEquipment. 
ddhub:DrillFloorEquipment a owl:Class; 
                          rdfs:comment """
"""@EN; 
                          rdfs:subClassOf ddhub:DrillFloorSystems. 
ddhub:DrillFloorStructure a owl:Class; 
                          rdfs:comment """
"""@EN; 
                          rdfs:subClassOf ddhub:DrillFloorSystems. 
ddhub:DrillFloorSubstructure a owl:Class; 
                             rdfs:comment """
"""@EN; 
                             rdfs:subClassOf ddhub:DrillFloorStructure. 
ddhub:DrillFloorSystems a owl:Class; 
                        rdfs:comment """
"""@EN; 
                        rdfs:subClassOf ddhub:RigEquipment. 
ddhub:DrillingAccelerationQuantity a owl:Class; 
                                   rdfs:comment """
"""@EN; 
                                   rdfs:subClassOf ddhub:MeasurableQuantity. 
ddhub:DrillingAngleVariationGradientQuantity a owl:Class; 
                                             rdfs:comment """
"""@EN; 
                                             rdfs:subClassOf ddhub:MeasurableQuantity. 
ddhub:DrillingAngularVelocityQuantity a owl:Class; 
                                      rdfs:comment """
"""@EN; 
                                      rdfs:subClassOf ddhub:MeasurableQuantity. 
ddhub:DrillingAreaQuantity a owl:Class; 
                           rdfs:comment """
"""@EN; 
                           rdfs:subClassOf ddhub:MeasurableQuantity. 
ddhub:DrillingAxialVelocityQuantity a owl:Class; 
                                    rdfs:comment """
"""@EN; 
                                    rdfs:subClassOf ddhub:MeasurableQuantity. 
ddhub:DrillingBit a owl:Class; 
                  rdfs:comment """
"""@EN; 
                  rdfs:subClassOf ddhub:DrillstemTerminator. 
ddhub:DrillingCompressibilityQuantity a owl:Class; 
                                      rdfs:comment """
"""@EN; 
                                      rdfs:subClassOf ddhub:MeasurableQuantity. 
ddhub:DrillingContractor a owl:Class; 
                         rdfs:comment """
"""@EN; 
                         rdfs:subClassOf ddhub:DataProvider. 
ddhub:DrillingCurvatureQuantity a owl:Class; 
                                rdfs:comment """
"""@EN; 
                                rdfs:subClassOf ddhub:MeasurableQuantity. 
ddhub:DrillingDataPoint a owl:Class; 
                        rdfs:comment """Main type of DDHub data. Represents a drilling signal.
Can be a dynamic signal (linked to a ValueNode) or a static parameter. 
"""@EN; 
                        rdfs:subClassOf ddhub:DWISNoun. 
ddhub:DrillingDensityGradientDepthQuantity a owl:Class; 
                                           rdfs:comment """
"""@EN; 
                                           rdfs:subClassOf ddhub:MeasurableQuantity. 
ddhub:DrillingDensityGradientTemperatureQuantity a owl:Class; 
                                                 rdfs:comment """
"""@EN; 
                                                 rdfs:subClassOf ddhub:MeasurableQuantity. 
ddhub:DrillingDensityQuantity a owl:Class; 
                              rdfs:comment """
"""@EN; 
                              rdfs:subClassOf ddhub:MeasurableQuantity. 
ddhub:DrillingDensityRateOfChangeQuantity a owl:Class; 
                                          rdfs:comment """
"""@EN; 
                                          rdfs:subClassOf ddhub:MeasurableQuantity. 
ddhub:DrillingDrillStringMagneticFluxQuantity a owl:Class; 
                                              rdfs:comment """
"""@EN; 
                                              rdfs:subClassOf ddhub:MeasurableQuantity. 
ddhub:DrillingDurationQuantity a owl:Class; 
                               rdfs:comment """
"""@EN; 
                               rdfs:subClassOf ddhub:MeasurableQuantity. 
ddhub:DrillingDynamicViscosityQuantity a owl:Class; 
                                       rdfs:comment """
"""@EN; 
                                       rdfs:subClassOf ddhub:MeasurableQuantity. 
ddhub:DrillingElongationGradientQuantity a owl:Class; 
                                         rdfs:comment """
"""@EN; 
                                         rdfs:subClassOf ddhub:MeasurableQuantity. 
ddhub:DrillingEquipment a owl:Class; 
                        rdfs:comment """
"""@EN; 
                        rdfs:subClassOf ddhub:DownholeEquipment. 
ddhub:DrillingFluid a owl:Class; 
                    rdfs:comment """
"""@EN; 
                    rdfs:subClassOf ddhub:CirculationSystem. 
ddhub:DrillingFluidGasComponent a owl:Class; 
                                rdfs:comment """
"""@EN; 
                                rdfs:subClassOf ddhub:GasComponent. 
ddhub:DrillingFluidLiquidComponent a owl:Class; 
                                   rdfs:comment """
"""@EN; 
                                   rdfs:subClassOf ddhub:LiquidComponent. 
ddhub:DrillingFluidOilComponent a owl:Class; 
                                rdfs:comment """
"""@EN; 
                                rdfs:subClassOf ddhub:DrillingFluidLiquidComponent. 
ddhub:DrillingFluidProvider a owl:Class; 
                            rdfs:comment """A drilling fluid provider is a company that provides and maintains the drilling fluids during well construction.
"""@EN; 
                            rdfs:subClassOf ddhub:ServiceCompany. 
ddhub:DrillingFluidSolidComponent a owl:Class; 
                                  rdfs:comment """
"""@EN; 
                                  rdfs:subClassOf ddhub:SolidComponent. 
ddhub:DrillingFluidVelocityQuantity a owl:Class; 
                                    rdfs:comment """
"""@EN; 
                                    rdfs:subClassOf ddhub:MeasurableQuantity. 
ddhub:DrillingFluidWaterComponent a owl:Class; 
                                  rdfs:comment """
"""@EN; 
                                  rdfs:subClassOf ddhub:DrillingFluidLiquidComponent. 
ddhub:DrillingForceGradientQuantity a owl:Class; 
                                    rdfs:comment """
"""@EN; 
                                    rdfs:subClassOf ddhub:MeasurableQuantity. 
ddhub:DrillingForceQuantity a owl:Class; 
                            rdfs:comment """
"""@EN; 
                            rdfs:subClassOf ddhub:MeasurableQuantity. 
ddhub:DrillingHeatTransferCoefficientQuantity a owl:Class; 
                                              rdfs:comment """
"""@EN; 
                                              rdfs:subClassOf ddhub:MeasurableQuantity. 
ddhub:DrillingHydraulicConductivityQuantity a owl:Class; 
                                            rdfs:comment """
"""@EN; 
                                            rdfs:subClassOf ddhub:MeasurableQuantity. 
ddhub:DrillingIncident a owl:Class; 
                       rdfs:comment """
"""@EN; 
                       rdfs:subClassOf ddhub:DWISNoun. 
ddhub:DrillingInterfacialTensionQuantity a owl:Class; 
                                         rdfs:comment """
"""@EN; 
                                         rdfs:subClassOf ddhub:MeasurableQuantity. 
ddhub:DrillingMassGradientQuantity a owl:Class; 
                                   rdfs:comment """
"""@EN; 
                                   rdfs:subClassOf ddhub:MeasurableQuantity. 
ddhub:DrillingMassQuantity a owl:Class; 
                           rdfs:comment """
"""@EN; 
                           rdfs:subClassOf ddhub:MeasurableQuantity. 
ddhub:DrillingMassRateQuantity a owl:Class; 
                               rdfs:comment """
"""@EN; 
                               rdfs:subClassOf ddhub:MeasurableQuantity. 
ddhub:DrillingPlaneAngleQuantity a owl:Class; 
                                 rdfs:comment """
"""@EN; 
                                 rdfs:subClassOf ddhub:MeasurableQuantity. 
ddhub:DrillingPressureGradientQuantity a owl:Class; 
                                       rdfs:comment """
"""@EN; 
                                       rdfs:subClassOf ddhub:MeasurableQuantity. 
ddhub:DrillingPressureLossConstantQuantity a owl:Class; 
                                           rdfs:comment """
"""@EN; 
                                           rdfs:subClassOf ddhub:MeasurableQuantity. 
ddhub:DrillingPressureQuantity a owl:Class; 
                               rdfs:comment """
"""@EN; 
                               rdfs:subClassOf ddhub:MeasurableQuantity. 
ddhub:DrillingProgram a owl:Class; 
                      rdfs:comment """
"""@EN; 
                      rdfs:subClassOf ddhub:Plan. 
ddhub:DrillingRandomWalkQuantity a owl:Class; 
                                 rdfs:comment """
"""@EN; 
                                 rdfs:subClassOf ddhub:MeasurableQuantity. 
ddhub:DrillingRiser a owl:Class; 
                    rdfs:comment """
"""@EN; 
                    rdfs:subClassOf ddhub:MarineSystem. 
ddhub:DrillingRotationFrequencyRateOfChangeQuantity a owl:Class; 
                                                    rdfs:comment """
"""@EN; 
                                                    rdfs:subClassOf ddhub:MeasurableQuantity. 
ddhub:DrillingSignal a owl:Class; 
                     rdfs:comment """Data structure used to store the streaming drilling data.
"""@EN; 
                     rdfs:subClassOf ddhub:DWISNoun. 
ddhub:DrillingSpecificHeatCapacityQuantity a owl:Class; 
                                           rdfs:comment """
"""@EN; 
                                           rdfs:subClassOf ddhub:MeasurableQuantity. 
ddhub:DrillingSpecificHeatCapacityTemperatureGradientQuantity a owl:Class; 
                                                              rdfs:comment """
"""@EN; 
                                                              rdfs:subClassOf ddhub:MeasurableQuantity. 
ddhub:DrillingSurveyInstrumentAngleMagneticFluxDensityQuantity a owl:Class; 
                                                               rdfs:comment """
"""@EN; 
                                                               rdfs:subClassOf ddhub:MeasurableQuantity. 
ddhub:DrillingSurveyInstrumentAngularVelocityQuantity a owl:Class; 
                                                      rdfs:comment """
"""@EN; 
                                                      rdfs:subClassOf ddhub:MeasurableQuantity. 
ddhub:DrillingSurveyInstrumentReciprocalLengthQuantity a owl:Class; 
                                                       rdfs:comment """
"""@EN; 
                                                       rdfs:subClassOf ddhub:MeasurableQuantity. 
ddhub:DrillingTemperatureGradientQuantity a owl:Class; 
                                          rdfs:comment """
"""@EN; 
                                          rdfs:subClassOf ddhub:MeasurableQuantity. 
ddhub:DrillingTemperatureQuantity a owl:Class; 
                                  rdfs:comment """
"""@EN; 
                                  rdfs:subClassOf ddhub:MeasurableQuantity. 
ddhub:DrillingTensionQuantity a owl:Class; 
                              rdfs:comment """
"""@EN; 
                              rdfs:subClassOf ddhub:MeasurableQuantity. 
ddhub:DrillingThermalConductivityQuantity a owl:Class; 
                                          rdfs:comment """
"""@EN; 
                                          rdfs:subClassOf ddhub:MeasurableQuantity. 
ddhub:DrillingThermalConductivityTemperatureGradientQuantity a owl:Class; 
                                                             rdfs:comment """
"""@EN; 
                                                             rdfs:subClassOf ddhub:MeasurableQuantity. 
ddhub:DrillingTorqueQuantity a owl:Class; 
                             rdfs:comment """
"""@EN; 
                             rdfs:subClassOf ddhub:MeasurableQuantity. 
ddhub:DrillingVolumeQuantity a owl:Class; 
                             rdfs:comment """
"""@EN; 
                             rdfs:subClassOf ddhub:MeasurableQuantity. 
ddhub:DrillingVolumetricFlowRateOfChangeQuantity a owl:Class; 
                                                 rdfs:comment """
"""@EN; 
                                                 rdfs:subClassOf ddhub:MeasurableQuantity. 
ddhub:DrillingVolumetricFlowrateQuantity a owl:Class; 
                                         rdfs:comment """
"""@EN; 
                                         rdfs:subClassOf ddhub:MeasurableQuantity. 
ddhub:DrillLine a owl:Class; 
                rdfs:comment """
"""@EN; 
                rdfs:subClassOf ddhub:HoistingSystem. 
ddhub:DrillLineFastener a owl:Class; 
                        rdfs:comment """
"""@EN; 
                        rdfs:subClassOf ddhub:HoistingSystem. 
ddhub:DrillPipe a owl:Class; 
                rdfs:comment """
"""@EN; 
                rdfs:subClassOf ddhub:DrillString. 
ddhub:DrillPipeElevator a owl:Class; 
                        rdfs:comment """
"""@EN; 
                        rdfs:subClassOf ddhub:DrillFloorEquipment. 
ddhub:DrillPipesAnnular a owl:Class; 
                        rdfs:comment """
"""@EN; 
                        rdfs:subClassOf ddhub:Annular. 
ddhub:DrillPipesInner a owl:Class; 
                      rdfs:comment """
"""@EN; 
                      rdfs:subClassOf ddhub:Pipe. 
ddhub:DrillPipeTongs a owl:Class; 
                     rdfs:comment """
"""@EN; 
                     rdfs:subClassOf ddhub:DrillFloorEquipment. 
ddhub:DrillStemMaterialStrengthQuantity a owl:Class; 
                                        rdfs:comment """
"""@EN; 
                                        rdfs:subClassOf ddhub:MeasurableQuantity. 
ddhub:DrillStemMechanicalModel a owl:Class; 
                               rdfs:comment """A mechanical model for a drill-stem. Another name for drill-stem mechanical models is a torque and drag model.
"""@EN; 
                               rdfs:subClassOf ddhub:MathematicalModel. 
ddhub:DrillstemTerminator a owl:Class; 
                          rdfs:comment """
"""@EN; 
                          rdfs:subClassOf ddhub:DrillingEquipment. 
ddhub:DrillString a owl:Class; 
                  rdfs:comment """
"""@EN; 
                  rdfs:subClassOf <http://ddhub.no/<Tubulars>>. 
ddhub:DrillStringCenterLineFrame a owl:Class; 
                                 rdfs:comment """
"""@EN; 
                                 rdfs:subClassOf ddhub:OneDimensionalCurviLinearReferenceFrame. 
ddhub:DrillWater a owl:Class; 
                 rdfs:comment """
"""@EN; 
                 rdfs:subClassOf ddhub:DrillingFluid. 
ddhub:DualActing a owl:Class; 
                 rdfs:comment """
"""@EN; 
                 rdfs:subClassOf ddhub:Action. 
ddhub:DWISADCSCapabilityDescriptor a owl:Class; 
                                   rdfs:comment """
"""@EN; 
                                   rdfs:subClassOf ddhub:DWISInternalService. 
ddhub:DWISADCSInterface a owl:Class; 
                        rdfs:comment """
"""@EN; 
                        rdfs:subClassOf ddhub:DWISInternalService. 
ddhub:DWISAdviceComposer a owl:Class; 
                         rdfs:comment """
"""@EN; 
                         rdfs:subClassOf ddhub:DWISInternalService. 
ddhub:DWISAttributeCardinalityRestriction a owl:Class, owl:Restriction; 
                                          owl:onClass ddhub:ActivableFunction, ddhub:RunnableFunction, ddhub:Advisor, ddhub:BandPassFilter, ddhub:HighPassFilter, ddhub:LowPassFilter, ddhub:NumberOfSampleMovingAverage, ddhub:TimeWindowMovingAverage, ddhub:Buffering, ddhub:NumberOfItemsRangeExtraction, ddhub:TimeWindowRangeExtraction, ddhub:Resampling, ddhub:DataProvider, ddhub:OperatingCompany, ddhub:ServiceCompany, ddhub:DirectionalServiceCompany, ddhub:DrillingFluidProvider, ddhub:LoggingServiceCompany, ddhub:CementingServiceCompany, ddhub:DataAnalysisServiceCompany, ddhub:DrillingContractor, ddhub:DWISInternalService, ddhub:Telemetry, ddhub:DrillingDataPoint, ddhub:DrillingSignal, ddhub:DynamicDrillingSignal, ddhub:DataEndPoint, ddhub:WitsMLTimeBasedLogEndPoint, ddhub:EndPointMapping, ddhub:HydraulicConnectedState, ddhub:HydraulicJunction, ddhub:MeasurableQuantity, ddhub:MechanicalElementState, ddhub:OneDimensionalReferenceFrame, ddhub:Quantity, ddhub:Unit, ddhub:Clock, ddhub:SynchronizationGroup, ddhub:FullScaleUncertainty, ddhub:SensorUncertainty; 
                                          owl:onProperty ddhub:HasFunction, ddhub:IsAuxiliary, ddhub:AdviceType, ddhub:MinFrequency, ddhub:MaxFrequency, ddhub:CutOffFrequency, ddhub:NumberOfSamples, ddhub:TimeWindow, ddhub:BufferingInterval, ddhub:NumberOfItems, ddhub:ResamplingRate, ddhub:ResamplingDelay, ddhub:Validity, ddhub:ProviderName, ddhub:NumberOfRepeaters, ddhub:DistanceBetweenRepeaters, ddhub:AverageDelayByRepeater, ddhub:IsValid, ddhub:Value, ddhub:TimeStampAtSource, ddhub:TimeStampAcquisition, ddhub:EndPointDescription, ddhub:WellUID, ddhub:WellName, ddhub:WellboreUID, ddhub:WellboreName, ddhub:LogUID, ddhub:LogName, ddhub:Mnemonic, ddhub:FixedIndices, ddhub:ValuesIndices, ddhub:MeasurementIndex, ddhub:LeftToRight, ddhub:RightToLeft, ddhub:MeaningfulPrecision, ddhub:PostiveUpward, ddhub:L, ddhub:M, ddhub:T, ddhub:I, ddhub:ThT, ddhub:N, ddhub:J, ddhub:SIUnit, ddhub:Symbol, ddhub:ConversionFactorA, ddhub:ConversionFactorB, ddhub:LeapSeconds, ddhub:Stratum, ddhub:NetworkSynchronizationLatencyAverage, ddhub:NetworkSynchronizationLatencyStandardDeviation, ddhub:Resolution, ddhub:MaximumFluctuations, ddhub:SynchronizationDelay, ddhub:SamplingRate, ddhub:FullScale, ddhub:ProportionError, ddhub:Accuracy, ddhub:Precision; 
                                          owl:qualifiedCardinality "1"^^xsd:nonNegativeInteger. 
ddhub:DWISContextualDataBuilder a owl:Class; 
                                rdfs:comment """
"""@EN; 
                                rdfs:subClassOf ddhub:DWISInternalService. 
ddhub:DWISDDHub a owl:Class; 
                rdfs:comment """
"""@EN; 
                rdfs:subClassOf ddhub:DWISInternalService. 
ddhub:DWISDrillingProcessStateInterpreter a owl:Class; 
                                          rdfs:comment """
"""@EN; 
                                          rdfs:subClassOf ddhub:DWISInternalService. 
ddhub:DWISInternalService a owl:Class; 
                          rdfs:comment """A DWIS internal service is an internal component of the DWIS infrastructure that generates information that can be used by any systems connected to the DWIS infrastructure.
"""@EN; 
                          rdfs:subClassOf ddhub:DataProvider. 
ddhub:DWISLogger a owl:Class; 
                 rdfs:comment """
"""@EN; 
                 rdfs:subClassOf ddhub:DWISInternalService. 
ddhub:DWISNoun a owl:Class; 
               rdfs:comment """Nouns refer to the nature of a node in the graph. Implicitely a noun refers to a "is a" relation between the instance node and the noun. This is the root class for all the nouns defined in the DWIS vocabulary.
"""@EN. 
ddhub:DWISScheduler a owl:Class; 
                    rdfs:comment """
"""@EN; 
                    rdfs:subClassOf ddhub:DWISInternalService. 
ddhub:DWISVerb a owl:ObjectProperty; 
               rdfs:comment """This is the root class for all verbs defined in the DWIS vocabulary. It is used to define a relation between a subject, which can be of any `DWISNoun` and an object, also of any type of `DWISNoun`.
"""@EN; 
               rdfs:domain ddhub:DWISNoun; 
               rdfs:range ddhub:DWISNoun. 
ddhub:DWISVocabulary a owl:Ontology; 
                     rdfs:comment "This is the ontology generated by the D-WIS WG1: Semantics of Real-time signals. It has been automatically generated from the vocabulary defined at https://github.com/D-WIS/DDHub-Semantic-Interoperability/tree/main/docs/vocabulary_development/auto-generated"@EN; 
                     rdfs:isDefinedBy "D-WIS WG1: Semantics of Real-time signals"^^xsd:string; 
                     rdfs:label "D-WIS vocabulary"^^xsd:string; 
                     owl:versionInfo "0.1"^^xsd:string; 
                     owl:versionIRI "https://github.com/D-WIS/DDHub-Semantic-Interoperability/tree/main/docs/vocabulary_development/auto-generated/dwis.owl"^^xsd:anyURI. 
ddhub:dynamic a owl:Class; 
              rdfs:comment """
"""@EN; 
              rdfs:subClassOf ddhub:BladeShape. 
ddhub:DynamicDrillingSignal a owl:Class; 
                            rdfs:comment """
"""@EN; 
                            rdfs:subClassOf ddhub:DrillingSignal. 
ddhub:DynamicViscosityQuantity a owl:Class; 
                               rdfs:comment """
"""@EN; 
                               rdfs:subClassOf ddhub:Quantity. 
ddhub:EarthMagneticFluxDensityQuantity a owl:Class; 
                                       rdfs:comment """
"""@EN; 
                                       rdfs:subClassOf ddhub:MeasurableQuantity. 
ddhub:ElectricalCapacitanceQuantity a owl:Class; 
                                    rdfs:comment """
"""@EN; 
                                    rdfs:subClassOf ddhub:Quantity. 
ddhub:ElectricalControlSystem a owl:Class; 
                              rdfs:comment """
"""@EN; 
                              rdfs:subClassOf ddhub:PowerGenerationSystem. 
ddhub:ElectricCurrentQuantity a owl:Class; 
                              rdfs:comment """
"""@EN; 
                              rdfs:subClassOf ddhub:Quantity. 
ddhub:ElectricTensionQuantity a owl:Class; 
                              rdfs:comment """
"""@EN; 
                              rdfs:subClassOf ddhub:MeasurableQuantity. 
ddhub:Electro-Magnetic a owl:Class; 
                       rdfs:comment """
"""@EN; 
                       rdfs:subClassOf ddhub:EquipmentTelemetry. 
ddhub:ElectromagneticTelemetry a owl:Class; 
                               rdfs:comment """A method that allows transfer of downhole data to the surface via electromagnetic waves sent trough the drilling formation.
"""@EN; 
                               rdfs:subClassOf ddhub:DownHoleTelemetry. 
ddhub:ElevatorBailsLinks a owl:Class; 
                         rdfs:comment """
"""@EN; 
                         rdfs:subClassOf ddhub:DrillFloorEquipment. 
ddhub:ElongationGradientQuantity a owl:Class; 
                                 rdfs:comment """
"""@EN; 
                                 rdfs:subClassOf ddhub:Quantity. 
ddhub:EndPointDescription a owl:DatatypeProperty, owl:FunctionalProperty; 
                          rdfs:comment """
"""@EN; 
                          rdfs:domain ddhub:DataEndPoint; 
                          rdfs:range xsd:string. 
ddhub:EndPointMapping a owl:Class; 
                      rdfs:comment """
"""@EN; 
                      rdfs:subClassOf ddhub:DWISNoun. 
ddhub:EndsHydraulicBranchDecomposition a owl:ObjectProperty; 
                                       rdfs:comment """
"""@EN; 
                                       rdfs:domain ddhub:HydraulicBranch; 
                                       rdfs:range ddhub:HydraulicBranch; 
                                       rdfs:subPropertyOf ddhub:DWISVerb. 
ddhub:EnergyQuantity a owl:Class; 
                     rdfs:comment """
"""@EN; 
                     rdfs:subClassOf ddhub:Quantity. 
ddhub:EnumerationDataType a owl:Class; 
                          rdfs:comment """
"""@EN; 
                          rdfs:subClassOf ddhub:DiscreteDataType. 
ddhub:EQ a owl:Class; 
         rdfs:comment """
"""@EN; 
         rdfs:subClassOf ddhub:ValidityCondition. 
ddhub:EquipmentTelemetry a owl:Class; 
                         rdfs:comment """
"""@EN; 
                         rdfs:subClassOf ddhub:LoggingEquipment. 
ddhub:ExpandableReamers a owl:Class; 
                        rdfs:comment """
"""@EN; 
                        rdfs:subClassOf ddhub:Reamers. 
ddhub:Expandables a owl:Class; 
                  rdfs:comment """
"""@EN; 
                  rdfs:subClassOf <http://ddhub.no/<Tubulars>>. 
ddhub:ExtendFrame a owl:Class; 
                  rdfs:comment """
"""@EN; 
                  rdfs:subClassOf ddhub:TopDrive. 
ddhub:FDIRFunction a owl:Class; 
                   rdfs:comment """A `FDIRFunction` is a `ProtectionFunction` that reacts to a particular state of the drilling process. FDIR
"""@EN; 
                   rdfs:subClassOf ddhub:ProtectionFunction. 
ddhub:FillPump a owl:Class; 
               rdfs:comment """
"""@EN; 
               rdfs:subClassOf ddhub:CirculationSystem. 
ddhub:Filter a owl:Class; 
             rdfs:comment """
"""@EN; 
             rdfs:subClassOf ddhub:SignalProcessingUnit. 
ddhub:FireSafetySystems a owl:Class; 
                        rdfs:comment """
"""@EN; 
                        rdfs:subClassOf ddhub:SafetyEquipment. 
ddhub:FishingTools a owl:Class; 
                   rdfs:comment """
"""@EN; 
                   rdfs:subClassOf ddhub:DrillingEquipment. 
ddhub:FixedBlade a owl:Class; 
                 rdfs:comment """
"""@EN; 
                 rdfs:subClassOf ddhub:HoleOpener. 
ddhub:FixedBladeReamers a owl:Class; 
                        rdfs:comment """
"""@EN; 
                        rdfs:subClassOf ddhub:Reamers. 
ddhub:FixedCutter a owl:Class; 
                  rdfs:comment """
"""@EN; 
                  rdfs:subClassOf ddhub:DrillingBit. 
ddhub:FixedIndices a owl:DatatypeProperty, owl:FunctionalProperty; 
                   rdfs:comment """
"""@EN; 
                   rdfs:domain ddhub:EndPointMapping; 
                   rdfs:range <http://www.w3.org/2001/XMLSchema#int[]>. 
ddhub:flange a owl:Class; 
             rdfs:comment """
"""@EN; 
             rdfs:subClassOf ddhub:Connection. 
ddhub:FlapperFloatValvesG a owl:Class; 
                          rdfs:comment """
"""@EN; 
                          rdfs:subClassOf ddhub:FloatValveNonreturnValve. 
ddhub:FloatCollar a owl:Class; 
                  rdfs:comment """
"""@EN; 
                  rdfs:subClassOf ddhub:CasingEquipment. 
ddhub:FloatShoe a owl:Class; 
                rdfs:comment """
"""@EN; 
                rdfs:subClassOf ddhub:CasingEquipment. 
ddhub:FloatValveNonreturnValve a owl:Class; 
                               rdfs:comment """
"""@EN; 
                               rdfs:subClassOf ddhub:WellControlSystem. 
ddhub:FlowAnalysisEquipment a owl:Class; 
                            rdfs:comment """
"""@EN; 
                            rdfs:subClassOf ddhub:MudLoggingEquipment. 
ddhub:FlowLine a owl:Class; 
               rdfs:comment """
"""@EN; 
               rdfs:subClassOf ddhub:MudLines. 
ddhub:FlowmeterTools a owl:Class; 
                     rdfs:comment """
"""@EN; 
                     rdfs:subClassOf ddhub:WirelineLoggingTools. 
ddhub:FlowRateIn a owl:Class; 
                 rdfs:comment """
"""@EN; 
                 rdfs:subClassOf ddhub:PrototypeData. 
ddhub:FlowRateOut a owl:Class; 
                  rdfs:comment """
"""@EN; 
                  rdfs:subClassOf ddhub:PrototypeData. 
ddhub:FluidComponent a owl:Class; 
                     rdfs:comment """
"""@EN; 
                     rdfs:subClassOf ddhub:DWISNoun. 
ddhub:FluidDensityTools a owl:Class; 
                        rdfs:comment """
"""@EN; 
                        rdfs:subClassOf ddhub:WirelineLoggingTools. 
ddhub:FluidShearRateQuantity a owl:Class; 
                             rdfs:comment """
"""@EN; 
                             rdfs:subClassOf ddhub:MeasurableQuantity. 
ddhub:FluidShearStressQuantity a owl:Class; 
                               rdfs:comment """
"""@EN; 
                               rdfs:subClassOf ddhub:MeasurableQuantity. 
ddhub:ForceFromLoadPinsTransformation a owl:Class; 
                                      rdfs:comment """
"""@EN; 
                                      rdfs:subClassOf ddhub:DirectTransformation. 
ddhub:ForceGradientQuantity a owl:Class; 
                            rdfs:comment """
"""@EN; 
                            rdfs:subClassOf ddhub:Quantity. 
ddhub:ForceQuantity a owl:Class; 
                    rdfs:comment """
"""@EN; 
                    rdfs:subClassOf ddhub:Quantity. 
ddhub:ForceToLoadTransformation a owl:Class; 
                                rdfs:comment """
"""@EN; 
                                rdfs:subClassOf ddhub:DirectTransformation. 
ddhub:FormationCollapseLocation a owl:Class; 
                                rdfs:comment """
"""@EN; 
                                rdfs:subClassOf ddhub:AbscissaReferenceLocation. 
ddhub:FormationFluidTransferLocation a owl:Class; 
                                     rdfs:comment """
"""@EN; 
                                     rdfs:subClassOf ddhub:AbscissaReferenceLocation. 
ddhub:FormationGasComponent a owl:Class; 
                            rdfs:comment """
"""@EN; 
                            rdfs:subClassOf ddhub:GasComponent. 
ddhub:FormationLiquidComponent a owl:Class; 
                               rdfs:comment """
"""@EN; 
                               rdfs:subClassOf ddhub:LiquidComponent. 
ddhub:FormationResistivityQuantity a owl:Class; 
                                   rdfs:comment """
"""@EN; 
                                   rdfs:subClassOf ddhub:MeasurableQuantity. 
ddhub:FormationSolidComponent a owl:Class; 
                              rdfs:comment """
"""@EN; 
                              rdfs:subClassOf ddhub:SolidComponent. 
ddhub:FormationStrengthQuantity a owl:Class; 
                                rdfs:comment """
"""@EN; 
                                rdfs:subClassOf ddhub:MeasurableQuantity. 
ddhub:FormationTestingAndSampling a owl:Class; 
                                  rdfs:comment """
"""@EN; 
                                  rdfs:subClassOf ddhub:WirelineLoggingTools. 
ddhub:FormationTestTools a owl:Class; 
                         rdfs:comment """
"""@EN; 
                         rdfs:subClassOf ddhub:LoggingWhileDrillingTools. 
ddhub:FormationWashout a owl:Class; 
                       rdfs:comment """
"""@EN; 
                       rdfs:subClassOf ddhub:DrillingIncident. 
ddhub:FormationWashoutLocation a owl:Class; 
                               rdfs:comment """
"""@EN; 
                               rdfs:subClassOf ddhub:AbscissaReferenceLocation. 
ddhub:FourDimensionalReferenceFrame a owl:Class; 
                                    rdfs:comment """
"""@EN; 
                                    rdfs:subClassOf ddhub:ReferenceFrame. 
ddhub:FracturingPressure a owl:Class; 
                         rdfs:comment """
"""@EN; 
                         rdfs:subClassOf ddhub:PrototypeData. 
ddhub:FracturingPressureGradient a owl:Class; 
                                 rdfs:comment """
"""@EN; 
                                 rdfs:subClassOf ddhub:PrototypeData. 
ddhub:FrenetSerretReferenceFrame a owl:Class; 
                                 rdfs:comment """
"""@EN; 
                                 rdfs:subClassOf ddhub:ThreeDimensionalReferenceFrame. 
ddhub:FrequencyQuantity a owl:Class; 
                        rdfs:comment """
"""@EN; 
                        rdfs:subClassOf ddhub:Quantity. 
ddhub:FrequencyRateOfChangeQuantity a owl:Class; 
                                    rdfs:comment """
"""@EN; 
                                    rdfs:subClassOf ddhub:Quantity. 
ddhub:FullScale a owl:DatatypeProperty, owl:FunctionalProperty; 
                rdfs:comment """The total range of measurement of the signal, i.e., $\\left| max - min \\right|$. The value is expected to be in the same physical quantity as the sensor value.
"""@EN; 
                rdfs:domain ddhub:FullScaleUncertainty; 
                rdfs:range xsd:double. 
ddhub:FullScaleUncertainty a owl:Class; 
                           rdfs:comment """The uncertainty on the signal is described as a Gaussian distribution with a standard deviation that is calculated using a proportion of the maximum range of the signal. The `Fullscale` or `ProportionError` can either be defined as attribute values, for example when they have fixed values, or using facts utilizing the verbs `HasFullScale` or repectively `HasProportionError` when these values may change through time.
"""@EN; 
                           rdfs:subClassOf ddhub:GaussianUncertainty. 
ddhub:GammaRayQuantity a owl:Class; 
                       rdfs:comment """
"""@EN; 
                       rdfs:subClassOf ddhub:MeasurableQuantity. 
ddhub:GasAnalysisEquipment a owl:Class; 
                           rdfs:comment """
"""@EN; 
                           rdfs:subClassOf ddhub:MudLoggingEquipment. 
ddhub:GasComponent a owl:Class; 
                   rdfs:comment """
"""@EN; 
                   rdfs:subClassOf ddhub:FluidComponent. 
ddhub:GasFlowRate a owl:Class; 
                  rdfs:comment """
"""@EN; 
                  rdfs:subClassOf ddhub:PrototypeData. 
ddhub:GasSafetySystems a owl:Class; 
                       rdfs:comment """
"""@EN; 
                       rdfs:subClassOf ddhub:SafetyEquipment. 
ddhub:GasShowQuantity a owl:Class; 
                      rdfs:comment """
"""@EN; 
                      rdfs:subClassOf ddhub:MeasurableQuantity. 
ddhub:GasVolumetricFlowRateQuantity a owl:Class; 
                                    rdfs:comment """
"""@EN; 
                                    rdfs:subClassOf ddhub:MeasurableQuantity. 
ddhub:GaugePressureReference a owl:Class; 
                             rdfs:comment """
"""@EN; 
                             rdfs:subClassOf ddhub:RelativePressureReference. 
ddhub:GaussianUncertainty a owl:Class; 
                          rdfs:comment """The uncertainty is represented by a Gaussian distribution, i.e., with a `Mean` and a `StandardDeviation`, $\\mathcal{N}(\\overline{x},{\\sigma_{x}}^2)$ where $\\overline{x}$ is the `Mean` value and $\\sigma_{x}$ is the `StandardDeviation`.
"""@EN; 
                          rdfs:subClassOf ddhub:SignalUncertainty. 
ddhub:GenericEquipment a owl:Class; 
                       rdfs:comment """
"""@EN; 
                       rdfs:subClassOf <http://ddhub.no/<equipment>>. 
ddhub:GenericEquipmentGatevalve a owl:Class; 
                                rdfs:comment """
"""@EN; 
                                rdfs:subClassOf ddhub:GenericEquipment. 
ddhub:GenericUncertainty a owl:Class; 
                         rdfs:comment """The uncertainty is represented by a `Histogram`.
"""@EN; 
                         rdfs:subClassOf ddhub:SignalUncertainty. 
ddhub:Gooseneck a owl:Class; 
                rdfs:comment """
"""@EN; 
                rdfs:subClassOf ddhub:MudLines. 
ddhub:GPSReference a owl:Class; 
                   rdfs:comment """
"""@EN; 
                   rdfs:subClassOf ddhub:TimeReference. 
ddhub:GravitationalLoadQuantity a owl:Class; 
                                rdfs:comment """
"""@EN; 
                                rdfs:subClassOf ddhub:Quantity. 
ddhub:GravityHighSideAngleLocation a owl:Class; 
                                   rdfs:comment """
"""@EN; 
                                   rdfs:subClassOf ddhub:AngleReferenceLocation. 
ddhub:GridNorthAzimuthLocation a owl:Class; 
                               rdfs:comment """
"""@EN; 
                               rdfs:subClassOf ddhub:AzimuthReferenceLocation. 
ddhub:GroundLevelVerticalLocation a owl:Class; 
                                  rdfs:comment """
"""@EN; 
                                  rdfs:subClassOf ddhub:VerticalReferenceLocation. 
ddhub:Grouping a owl:Class; 
               rdfs:comment """
"""@EN; 
               rdfs:subClassOf ddhub:DrillString. 
ddhub:GT a owl:Class; 
         rdfs:comment """
"""@EN; 
         rdfs:subClassOf ddhub:ValidityCondition. 
ddhub:HammerAssembly a owl:Class; 
                     rdfs:comment """
"""@EN; 
                     rdfs:subClassOf ddhub:DrillingEquipment. 
ddhub:Hangers a owl:Class; 
              rdfs:comment """
"""@EN; 
              rdfs:subClassOf ddhub:CasingEquipment. 
ddhub:HasAcquisitionClock a owl:ObjectProperty; 
                          rdfs:comment """
"""@EN; 
                          rdfs:domain ddhub:DrillingDataPoint; 
                          rdfs:range ddhub:Clock; 
                          rdfs:subPropertyOf ddhub:DWISVerb. 
ddhub:HasBranchComponent a owl:ObjectProperty; 
                         rdfs:comment """
"""@EN; 
                         rdfs:domain ddhub:HydraulicNetwork; 
                         rdfs:range ddhub:HydraulicBranch; 
                         rdfs:subPropertyOf ddhub:DWISVerb. 
ddhub:HasBranchCoordinateSystem a owl:ObjectProperty; 
                                rdfs:comment """
"""@EN; 
                                rdfs:domain ddhub:HydraulicBranch; 
                                rdfs:range ddhub:ReferenceFrame; 
                                rdfs:subPropertyOf ddhub:DWISVerb. 
ddhub:HasCoordinates a owl:ObjectProperty; 
                     rdfs:comment """
"""@EN; 
                     rdfs:domain ddhub:Location; 
                     rdfs:range ddhub:DrillingDataPoint; 
                     rdfs:subPropertyOf ddhub:DWISVerb. 
ddhub:HasDomain a owl:ObjectProperty; 
                rdfs:comment """
"""@EN; 
                rdfs:domain ddhub:DrillingDataPoint; 
                rdfs:range ddhub:DrillingDataPoint; 
                rdfs:subPropertyOf ddhub:DWISVerb. 
ddhub:HasDynamicValue a owl:ObjectProperty; 
                      rdfs:comment """
"""@EN; 
                      rdfs:domain ddhub:DrillingDataPoint; 
                      rdfs:range ddhub:DynamicDrillingSignal; 
                      rdfs:subPropertyOf ddhub:HasValue. 
ddhub:HasElevationReference a owl:ObjectProperty; 
                            rdfs:comment """This verb is a specialization of `IsDependentOn` and refers to the specific dependence on an elevation reference.
"""@EN; 
                            rdfs:domain ddhub:DrillingDataPoint; 
                            rdfs:range ddhub:Location; 
                            rdfs:subPropertyOf ddhub:IsDependentOn. 
ddhub:HasEndJunction a owl:ObjectProperty; 
                     rdfs:comment """
"""@EN; 
                     rdfs:domain ddhub:HydraulicBranch; 
                     rdfs:range ddhub:HydraulicJunction; 
                     rdfs:subPropertyOf ddhub:IsHydraulicConnectedTo. 
ddhub:HasEndPoint a owl:ObjectProperty; 
                  rdfs:comment """
"""@EN; 
                  rdfs:domain ddhub:DrillingSignal; 
                  rdfs:range ddhub:DataEndPoint; 
                  rdfs:subPropertyOf ddhub:DWISVerb. 
ddhub:HasFullScale a owl:ObjectProperty; 
                   rdfs:comment """This verb is used to associate a `DrillingDataPoint` as the `FullScale` value of a `FullScaleUncertainty`
"""@EN; 
                   rdfs:domain ddhub:FullScaleUncertainty; 
                   rdfs:range ddhub:DrillingDataPoint; 
                   rdfs:subPropertyOf ddhub:DWISVerb. 
ddhub:HasFunction a owl:DatatypeProperty, owl:FunctionalProperty, owl:ObjectProperty; 
                  rdfs:comment """this attribute describes the purpose of the activable function.
"""@EN, """
"""@EN; 
                  rdfs:domain ddhub:ActivableFunction, ddhub:DrillingDataPoint; 
                  rdfs:range xsd:string, ddhub:DataFlowNode; 
                  rdfs:subPropertyOf ddhub:DWISVerb. 
ddhub:HasHydraulicState a owl:ObjectProperty; 
                        rdfs:comment """
"""@EN; 
                        rdfs:domain ddhub:HydraulicJunction; 
                        rdfs:range ddhub:HydraulicElementState; 
                        rdfs:subPropertyOf ddhub:DWISVerb. 
ddhub:HasHydraulicStateValueFrom a owl:ObjectProperty; 
                                 rdfs:comment """
"""@EN; 
                                 rdfs:domain ddhub:DWISNoun; 
                                 rdfs:range ddhub:DWISNoun; 
                                 rdfs:subPropertyOf ddhub:DWISVerb. 
ddhub:HasLeftBranch a owl:ObjectProperty; 
                    rdfs:comment """
"""@EN; 
                    rdfs:domain ddhub:HydraulicJunction; 
                    rdfs:range ddhub:HydraulicBranch; 
                    rdfs:subPropertyOf ddhub:IsHydraulicConnectedTo. 
ddhub:HasLeftBranchCoordinates a owl:ObjectProperty; 
                               rdfs:comment """
"""@EN; 
                               rdfs:domain ddhub:HydraulicJunction; 
                               rdfs:range ddhub:DrillingDataPoint; 
                               rdfs:subPropertyOf ddhub:DWISVerb. 
ddhub:HasMechanicalState a owl:ObjectProperty; 
                         rdfs:comment """
"""@EN; 
                         rdfs:domain ddhub:MechanicalLogicalElement; 
                         rdfs:range ddhub:MechanicalElementState; 
                         rdfs:subPropertyOf ddhub:DWISVerb. 
ddhub:HasMechanicalStateValueFrom a owl:ObjectProperty; 
                                  rdfs:comment """
"""@EN; 
                                  rdfs:domain ddhub:MechanicalElementState; 
                                  rdfs:range ddhub:DrillingDataPoint; 
                                  rdfs:subPropertyOf ddhub:DWISVerb. 
ddhub:HasMotionType a owl:ObjectProperty; 
                    rdfs:comment """
"""@EN; 
                    rdfs:domain ddhub:MechanicalLogicalElement; 
                    rdfs:range ddhub:MotionType; 
                    rdfs:subPropertyOf ddhub:DWISVerb. 
ddhub:HasPressureReference a owl:ObjectProperty; 
                           rdfs:comment """This verb is a specialization of `IsDependentOn` and refers to the specific dependence on a pressure reference.
"""@EN; 
                           rdfs:domain ddhub:DrillingDataPoint; 
                           rdfs:range ddhub:DrillingDataPoint; 
                           rdfs:subPropertyOf ddhub:IsDependentOn. 
ddhub:HasPressureReferenceType a owl:ObjectProperty; 
                               rdfs:comment """
"""@EN; 
                               rdfs:domain ddhub:DrillingDataPoint; 
                               rdfs:range ddhub:PressureReference; 
                               rdfs:subPropertyOf ddhub:DWISVerb. 
ddhub:HasProportionError a owl:ObjectProperty; 
                         rdfs:comment """This verb is used to associate a `DrillingDataPoint` as the `ProportionError` value of a `FullScaleUncertainty`
"""@EN; 
                         rdfs:domain ddhub:FullScaleUncertainty; 
                         rdfs:range ddhub:DrillingDataPoint; 
                         rdfs:subPropertyOf ddhub:DWISVerb. 
ddhub:HasReferenceFrame a owl:ObjectProperty; 
                        rdfs:comment """
"""@EN; 
                        rdfs:domain ddhub:DrillingDataPoint; 
                        rdfs:range ddhub:ReferenceFrame; 
                        rdfs:subPropertyOf ddhub:DWISVerb. 
ddhub:HasReferenceFrameOrigin a owl:ObjectProperty; 
                              rdfs:comment """
"""@EN; 
                              rdfs:domain ddhub:ReferenceFrame; 
                              rdfs:range ddhub:Location; 
                              rdfs:subPropertyOf ddhub:DWISVerb. 
ddhub:HasRightBranch a owl:ObjectProperty; 
                     rdfs:comment """
"""@EN; 
                     rdfs:domain ddhub:HydraulicJunction; 
                     rdfs:range ddhub:HydraulicBranch; 
                     rdfs:subPropertyOf ddhub:IsHydraulicConnectedTo. 
ddhub:HasRightBranchCoordinates a owl:ObjectProperty; 
                                rdfs:comment """
"""@EN; 
                                rdfs:domain ddhub:HydraulicJunction; 
                                rdfs:range ddhub:DrillingDataPoint; 
                                rdfs:subPropertyOf ddhub:DWISVerb. 
ddhub:HasSIUnit a owl:ObjectProperty; 
                rdfs:comment """
"""@EN; 
                rdfs:domain ddhub:Quantity; 
                rdfs:range ddhub:Unit; 
                rdfs:subPropertyOf ddhub:DWISVerb. 
ddhub:HasSourceClock a owl:ObjectProperty; 
                     rdfs:comment """
"""@EN; 
                     rdfs:domain ddhub:DrillingDataPoint; 
                     rdfs:range ddhub:Clock; 
                     rdfs:subPropertyOf ddhub:DWISVerb. 
ddhub:HasStartJunction a owl:ObjectProperty; 
                       rdfs:comment """
"""@EN; 
                       rdfs:domain ddhub:HydraulicBranch; 
                       rdfs:range ddhub:HydraulicJunction; 
                       rdfs:subPropertyOf ddhub:IsHydraulicConnectedTo. 
ddhub:HasStaticValue a owl:ObjectProperty; 
                     rdfs:comment """
"""@EN; 
                     rdfs:domain ddhub:DrillingDataPoint; 
                     rdfs:range ddhub:DrillingSignal; 
                     rdfs:subPropertyOf ddhub:HasValue. 
ddhub:HasTemperatureReference a owl:ObjectProperty; 
                              rdfs:comment """This verb is a specialization of `IsDependentOn` and refers to the specific dependence on a temperature reference.
"""@EN; 
                              rdfs:domain ddhub:DrillingDataPoint; 
                              rdfs:range ddhub:DrillingDataPoint; 
                              rdfs:subPropertyOf ddhub:IsDependentOn. 
ddhub:HasTimeIntervalDomain a owl:ObjectProperty; 
                            rdfs:comment """
"""@EN; 
                            rdfs:domain ddhub:DrillingDataPoint; 
                            rdfs:range ddhub:DrillingDataPoint; 
                            rdfs:subPropertyOf ddhub:HasDomain. 
ddhub:HasTimeReference a owl:ObjectProperty; 
                       rdfs:comment """
"""@EN; 
                       rdfs:domain ddhub:DrillingDataPoint; 
                       rdfs:range ddhub:TimeReference; 
                       rdfs:subPropertyOf ddhub:DWISVerb. 
ddhub:HasTransmissionDelay a owl:ObjectProperty; 
                           rdfs:comment """
"""@EN; 
                           rdfs:domain ddhub:DrillingDataPoint; 
                           rdfs:range ddhub:DrillingDataPoint; 
                           rdfs:subPropertyOf ddhub:DWISVerb. 
ddhub:HasUncertainty a owl:ObjectProperty; 
                     rdfs:comment """This verb allows to associate a `SignalUncertainty` to a `DrillingDataPoint`.
"""@EN; 
                     rdfs:domain ddhub:DrillingDataPoint; 
                     rdfs:range ddhub:SignalUncertainty; 
                     rdfs:subPropertyOf ddhub:DWISVerb. 
ddhub:HasUncertaintyAccuracy a owl:ObjectProperty; 
                             rdfs:comment """This verb allows to associate a `DrillingDataPoint` as the `Accuracy` of a `SensorUncertainty`
"""@EN; 
                             rdfs:domain ddhub:SensorUncertainty; 
                             rdfs:range ddhub:DrillingDataPoint; 
                             rdfs:subPropertyOf ddhub:DWISVerb. 
ddhub:HasUncertaintyHistogram a owl:ObjectProperty; 
                              rdfs:comment """This verb is used to associated a `DrillingDataPoint` as the `Histogram` value of a `GenericUncertainty`
"""@EN; 
                              rdfs:domain ddhub:GenericUncertainty; 
                              rdfs:range ddhub:DrillingDataPoint; 
                              rdfs:subPropertyOf ddhub:DWISVerb. 
ddhub:HasUncertaintyMax a owl:ObjectProperty; 
                        rdfs:comment """This verb is used to associate a `DrillingDataPoint` as the `Max` value of a `MinMaxUncertainty`
"""@EN; 
                        rdfs:domain ddhub:MinMaxUncertainty; 
                        rdfs:range ddhub:DrillingDataPoint; 
                        rdfs:subPropertyOf ddhub:DWISVerb. 
ddhub:HasUncertaintyMean a owl:ObjectProperty; 
                         rdfs:comment """This verb is used to associate a `DrillingDataPoint` as the `Mean` value of a `GaussianUncertainty`
"""@EN; 
                         rdfs:domain ddhub:GaussianUncertainty; 
                         rdfs:range ddhub:DrillingDataPoint; 
                         rdfs:subPropertyOf ddhub:DWISVerb. 
ddhub:HasUncertaintyMin a owl:ObjectProperty; 
                        rdfs:comment """This verb is used to associate a `DrillingDataPoint` as the `Min` value of `MinMaxUncertainty`
"""@EN; 
                        rdfs:domain ddhub:MinMaxUncertainty; 
                        rdfs:range ddhub:DrillingDataPoint; 
                        rdfs:subPropertyOf ddhub:DWISVerb. 
ddhub:HasUncertaintyPrecision a owl:ObjectProperty; 
                              rdfs:comment """This verb is used to associate a `DrillingDataPoint` as the `Precision` of a `SensorUncertainty`
"""@EN; 
                              rdfs:domain ddhub:SensorUncertainty; 
                              rdfs:range ddhub:DrillingDataPoint; 
                              rdfs:subPropertyOf ddhub:DWISVerb. 
ddhub:HasUncertaintyStandardDeviation a owl:ObjectProperty; 
                                      rdfs:comment """This verb is used to associate a `DrillingDataPoint` as the `StandardDeviation` value of a `GaussianUncertainty`
"""@EN; 
                                      rdfs:domain ddhub:GaussianUncertainty; 
                                      rdfs:range ddhub:DrillingDataPoint; 
                                      rdfs:subPropertyOf ddhub:DWISVerb. 
ddhub:HasUnitAssociation a owl:ObjectProperty; 
                         rdfs:comment """
"""@EN; 
                         rdfs:domain ddhub:UnitSystem; 
                         rdfs:range ddhub:MeasurableQuantityUnitAssociation; 
                         rdfs:subPropertyOf ddhub:DWISVerb. 
ddhub:HasUnitOfMeasure a owl:ObjectProperty; 
                       rdfs:comment """
"""@EN; 
                       rdfs:domain ddhub:DrillingSignal; 
                       rdfs:range ddhub:Unit; 
                       rdfs:subPropertyOf ddhub:DWISVerb. 
ddhub:HasValue a owl:ObjectProperty; 
               rdfs:comment """
"""@EN; 
               rdfs:domain ddhub:DrillingDataPoint; 
               rdfs:range ddhub:DrillingSignal; 
               rdfs:subPropertyOf ddhub:DWISVerb. 
ddhub:HeatTransferCoefficientQuantity a owl:Class; 
                                      rdfs:comment """
"""@EN; 
                                      rdfs:subClassOf ddhub:Quantity. 
ddhub:HeaveCompensationSystem a owl:Class; 
                              rdfs:comment """
"""@EN; 
                              rdfs:subClassOf ddhub:MarineSystem. 
ddhub:Heavyweight a owl:Class; 
                  rdfs:comment """
"""@EN; 
                  rdfs:subClassOf ddhub:DrillString. 
ddhub:HeightQuantity a owl:Class; 
                     rdfs:comment """
"""@EN; 
                     rdfs:subClassOf ddhub:MeasurableQuantity. 
ddhub:HighGravitySolidComponent a owl:Class; 
                                rdfs:comment """
"""@EN; 
                                rdfs:subClassOf ddhub:DrillingFluidSolidComponent. 
ddhub:HighPassFilter a owl:Class; 
                     rdfs:comment """
"""@EN; 
                     rdfs:subClassOf ddhub:Filter. 
ddhub:HighPressureRiser a owl:Class; 
                        rdfs:comment """
"""@EN; 
                        rdfs:subClassOf ddhub:SurfaceRiser. 
ddhub:HoistingSystem a owl:Class; 
                     rdfs:comment """
"""@EN; 
                     rdfs:subClassOf ddhub:RigEquipment. 
ddhub:HoleBottomLocation a owl:Class; 
                         rdfs:comment """
"""@EN; 
                         rdfs:subClassOf ddhub:AbscissaReferenceLocation. 
ddhub:HoleCollapse a owl:Class; 
                   rdfs:comment """
"""@EN; 
                   rdfs:subClassOf ddhub:DrillingIncident. 
ddhub:HoleDepth a owl:Class; 
                rdfs:comment """
"""@EN; 
                rdfs:subClassOf ddhub:PrototypeData. 
ddhub:HoleOpener a owl:Class; 
                 rdfs:comment """
"""@EN; 
                 rdfs:subClassOf ddhub:DrillingEquipment. 
ddhub:Hook a owl:Class; 
           rdfs:comment """
"""@EN; 
           rdfs:subClassOf ddhub:HoistingSystem. 
ddhub:HookLoad a owl:Class; 
               rdfs:comment """
"""@EN; 
               rdfs:subClassOf ddhub:PrototypeData. 
ddhub:HookLoadQuantity a owl:Class; 
                       rdfs:comment """
"""@EN; 
                       rdfs:subClassOf ddhub:MeasurableQuantity. 
ddhub:HookPosition a owl:Class; 
                   rdfs:comment """
"""@EN; 
                   rdfs:subClassOf ddhub:PrototypeData. 
ddhub:HookVelocity a owl:Class; 
                   rdfs:comment """
"""@EN; 
                   rdfs:subClassOf ddhub:PrototypeData. 
ddhub:HorizontalOndulationModelling a owl:Class; 
                                    rdfs:comment """The model accounts for the change of azimuth of some parts of the physical system.
"""@EN; 
                                    rdfs:subClassOf ddhub:TangentialModelling. 
ddhub:Hybrid a owl:Class; 
             rdfs:comment """
"""@EN; 
             rdfs:subClassOf ddhub:EquipmentTelemetry. 
ddhub:HybridKymera a owl:Class; 
                   rdfs:comment """
"""@EN; 
                   rdfs:subClassOf ddhub:DrillingBit. 
ddhub:HydraulicBranch a owl:Class; 
                      rdfs:comment """
"""@EN; 
                      rdfs:subClassOf ddhub:HydraulicLogicalElement. 
ddhub:HydraulicConductivityQuantity a owl:Class; 
                                    rdfs:comment """
"""@EN; 
                                    rdfs:subClassOf ddhub:Quantity. 
ddhub:HydraulicConnectedState a owl:Class; 
                              rdfs:comment """
"""@EN; 
                              rdfs:subClassOf ddhub:HydraulicElementState. 
ddhub:HydraulicElementState a owl:Class; 
                            rdfs:comment """
"""@EN; 
                            rdfs:subClassOf ddhub:DWISNoun. 
ddhub:HydraulicJar a owl:Class; 
                   rdfs:comment """
"""@EN; 
                   rdfs:subClassOf ddhub:JarringAssembly. 
ddhub:HydraulicJunction a owl:Class; 
                        rdfs:comment """
"""@EN; 
                        rdfs:subClassOf ddhub:HydraulicLogicalElement. 
ddhub:HydraulicLogicalElement a owl:Class; 
                              rdfs:comment """
"""@EN; 
                              rdfs:subClassOf ddhub:DWISNoun. 
ddhub:HydraulicMudPump a owl:Class; 
                       rdfs:comment """
"""@EN; 
                       rdfs:subClassOf ddhub:MudPump. 
ddhub:HydraulicNetwork a owl:Class; 
                       rdfs:comment """
"""@EN; 
                       rdfs:subClassOf ddhub:HydraulicLogicalElement. 
ddhub:Hydrocyclones a owl:Class; 
                    rdfs:comment """
"""@EN; 
                    rdfs:subClassOf ddhub:CirculationSystem. 
ddhub:HydromechanicalJar a owl:Class; 
                         rdfs:comment """
"""@EN; 
                         rdfs:subClassOf ddhub:JarringAssembly. 
ddhub:I a owl:DatatypeProperty, owl:FunctionalProperty; 
        rdfs:comment """Electric current exponent.
SI Unit: Ampere (A)
"""@EN; 
        rdfs:domain ddhub:Quantity; 
        rdfs:range xsd:int. 
ddhub:IBOP a owl:Class; 
           rdfs:comment """
"""@EN; 
           rdfs:subClassOf ddhub:WellControlSystem. 
ddhub:ImageScaleQuantity a owl:Class; 
                         rdfs:comment """
"""@EN; 
                         rdfs:subClassOf ddhub:MeasurableQuantity. 
ddhub:ImagingTools a owl:Class; 
                   rdfs:comment """
"""@EN; 
                   rdfs:subClassOf ddhub:LoggingWhileDrillingTools. 
ddhub:Inclination a owl:Class; 
                  rdfs:comment """
"""@EN; 
                  rdfs:subClassOf ddhub:PrototypeData. 
ddhub:Influx a owl:Class; 
             rdfs:comment """
"""@EN; 
             rdfs:subClassOf ddhub:DrillingIncident. 
ddhub:InjectorHead a owl:Class; 
                   rdfs:comment """
"""@EN; 
                   rdfs:subClassOf ddhub:CoiledTubingEquipment. 
ddhub:InnerBarrel a owl:Class; 
                  rdfs:comment """
"""@EN; 
                  rdfs:subClassOf ddhub:CoringTool. 
ddhub:InnerString a owl:Class; 
                  rdfs:comment """
"""@EN; 
                  rdfs:subClassOf ddhub:CasingEquipment. 
ddhub:InsertTci a owl:Class; 
                rdfs:comment """
"""@EN; 
                rdfs:subClassOf ddhub:RollingCutter. 
ddhub:InstrumentedMotor a owl:Class; 
                        rdfs:comment """
"""@EN; 
                        rdfs:subClassOf ddhub:DownholeMotor. 
ddhub:integral a owl:Class; 
               rdfs:comment """
"""@EN; 
               rdfs:subClassOf ddhub:BladeType. 
ddhub:Integration a owl:Class; 
                  rdfs:comment """
"""@EN; 
                  rdfs:subClassOf ddhub:TimeBasedTransformation. 
ddhub:InterfacialTensionQuantity a owl:Class; 
                                 rdfs:comment """
"""@EN; 
                                 rdfs:subClassOf ddhub:Quantity. 
ddhub:IronRoughneck a owl:Class; 
                    rdfs:comment """
"""@EN; 
                    rdfs:subClassOf ddhub:DrillFloorEquipment. 
ddhub:IsActivatedSignalFor a owl:ObjectProperty; 
                           rdfs:comment """This verb is used to define a `DrillingDataPoint` that indicates if the `ActivableFunction` is activated or
not. It is expected that the `DrillingDataPoint` is a Boolean value.
"""@EN; 
                           rdfs:domain ddhub:DrillingDataPoint; 
                           rdfs:range ddhub:ActivableFunction; 
                           rdfs:subPropertyOf ddhub:DWISVerb. 
ddhub:IsAHydraulicRepresentationFor a owl:ObjectProperty; 
                                    rdfs:comment """
"""@EN; 
                                    rdfs:domain ddhub:HydraulicLogicalElement; 
                                    rdfs:range ddhub:DrillingEquipment; 
                                    rdfs:subPropertyOf ddhub:DWISVerb. 
ddhub:IsAMechanicalRepresentationFor a owl:ObjectProperty; 
                                     rdfs:comment """
"""@EN; 
                                     rdfs:domain ddhub:MechanicalLogicalElement; 
                                     rdfs:range ddhub:DrillingEquipment; 
                                     rdfs:subPropertyOf ddhub:DWISVerb. 
ddhub:IsArmedSignalFor a owl:ObjectProperty; 
                       rdfs:comment """This verb is used to indicate a `DrillingDataPoint` used by an `FDIRFunction` tells if the FDIR function is armed and operative.
The signal is supposed to be a Boolean value.
The FDIR function may be active, but the current state of the drilling process may imply that the function cannot be
triggered. For instance, a pack-off FDIR may be active but would react only if the flow is supposed to be steady state.
"""@EN; 
                       rdfs:domain ddhub:DrillingDataPoint; 
                       rdfs:range ddhub:FDIRFunction; 
                       rdfs:subPropertyOf ddhub:DWISVerb. 
ddhub:IsAuxiliary a owl:DatatypeProperty, owl:FunctionalProperty; 
                  rdfs:comment """This attribute specifies if the function is a main or an auxilary one. A main function impacts
    substantially the drilling process while an auxiliary function does not impact or only in limited fashion the
    drilling process. Example of a main functions are: Hoist, Tag Bottom, Start Circulation, Start Rotation, 
    Stop Circulation, Stop Rotation, Drill, Pull Out,Run In, Pull Out With Lubrication, Run In With Lubrication, Ream Up, 
    Ream Down,Test Friction, Reciprocate, Test Pressure Integrity, Place Cement, .... Example of auxiliary functions
    are: Boost Riser Flow, Down Link from ADCS, Rock Pipe, ...
"""@EN; 
                  rdfs:domain ddhub:RunnableFunction; 
                  rdfs:range xsd:boolean. 
ddhub:IsBufferingInput a owl:ObjectProperty; 
                       rdfs:comment """
"""@EN; 
                       rdfs:domain ddhub:DrillingDataPoint; 
                       rdfs:range ddhub:Buffering; 
                       rdfs:subPropertyOf ddhub:IsTransformationInput. 
ddhub:IsBufferingOutput a owl:ObjectProperty; 
                        rdfs:comment """
"""@EN; 
                        rdfs:domain ddhub:DrillingDataPoint; 
                        rdfs:range ddhub:Buffering; 
                        rdfs:subPropertyOf ddhub:IsTransformationOutput. 
ddhub:IsCommandFor a owl:ObjectProperty; 
                   rdfs:comment """
"""@EN; 
                   rdfs:domain ddhub:DrillingDataPoint; 
                   rdfs:range ddhub:DWISNoun; 
                   rdfs:subPropertyOf ddhub:HasFunction. 
ddhub:IsComputationInput a owl:ObjectProperty; 
                         rdfs:comment """
"""@EN; 
                         rdfs:domain ddhub:DrillingDataPoint; 
                         rdfs:range ddhub:ComputationUnit; 
                         rdfs:subPropertyOf ddhub:HasFunction. 
ddhub:IsComputedBy a owl:ObjectProperty; 
                   rdfs:comment """
"""@EN; 
                   rdfs:domain ddhub:DWISNoun; 
                   rdfs:range ddhub:DWISNoun; 
                   rdfs:subPropertyOf ddhub:IsGeneratedBy. 
ddhub:IsConditionedBy a owl:ObjectProperty; 
                      rdfs:comment """
"""@EN; 
                      rdfs:domain ddhub:DrillingDataPoint; 
                      rdfs:range ddhub:ValidityCondition; 
                      rdfs:subPropertyOf ddhub:DWISVerb. 
ddhub:IsConditionInput a owl:ObjectProperty; 
                       rdfs:comment """
"""@EN; 
                       rdfs:domain ddhub:DrillingDataPoint; 
                       rdfs:range ddhub:ValidityCondition; 
                       rdfs:subPropertyOf ddhub:DWISVerb. 
ddhub:IsConditionLeft a owl:ObjectProperty; 
                      rdfs:comment """
"""@EN; 
                      rdfs:domain ddhub:DWISNoun; 
                      rdfs:range ddhub:DWISNoun; 
                      rdfs:subPropertyOf ddhub:IsConditionInput. 
ddhub:IsConditionRight a owl:ObjectProperty; 
                       rdfs:comment """
"""@EN; 
                       rdfs:domain ddhub:DWISNoun; 
                       rdfs:range ddhub:DWISNoun; 
                       rdfs:subPropertyOf ddhub:IsConditionInput. 
ddhub:IsDependentOn a owl:ObjectProperty; 
                    rdfs:comment """This verb is used to describe a general dependence relationship between a `DrillingDataPoint` and something else.
"""@EN; 
                    rdfs:domain ddhub:DrillingDataPoint; 
                    rdfs:range ddhub:DWISNoun; 
                    rdfs:subPropertyOf ddhub:DWISVerb. 
ddhub:IsDerivationInput a owl:ObjectProperty; 
                        rdfs:comment """
"""@EN; 
                        rdfs:domain ddhub:DWISNoun; 
                        rdfs:range ddhub:DWISNoun; 
                        rdfs:subPropertyOf ddhub:IsTransformationInput. 
ddhub:IsDerivedFrom a owl:ObjectProperty; 
                    rdfs:comment """
"""@EN; 
                    rdfs:domain ddhub:DWISNoun; 
                    rdfs:range ddhub:DWISNoun; 
                    rdfs:subPropertyOf ddhub:IsTransformationOutput. 
ddhub:IsEnablingSignalFor a owl:ObjectProperty; 
                          rdfs:comment """This verb is used to define a `DrillingDataPoint` that is used to enable or disable an `ActivableFunction`.
It is expected that the `DrillingDataPoint` is a Boolean value.
"""@EN; 
                          rdfs:domain ddhub:DrillingDataPoint; 
                          rdfs:range ddhub:ActivableFunction; 
                          rdfs:subPropertyOf ddhub:DWISVerb. 
ddhub:IsEquivalentCirculationDensityAt a owl:ObjectProperty; 
                                       rdfs:comment """
"""@EN; 
                                       rdfs:domain ddhub:DrillingDataPoint; 
                                       rdfs:range ddhub:HydraulicLogicalElement; 
                                       rdfs:subPropertyOf ddhub:IsHydraulicallyLocatedAt. 
ddhub:IsFluidDensityAt a owl:ObjectProperty; 
                       rdfs:comment """
"""@EN; 
                       rdfs:domain ddhub:DrillingDataPoint; 
                       rdfs:range ddhub:HydraulicLogicalElement; 
                       rdfs:subPropertyOf ddhub:IsHydraulicallyLocatedAt. 
ddhub:IsFluidTemperatureAt a owl:ObjectProperty; 
                           rdfs:comment """
"""@EN; 
                           rdfs:domain ddhub:DrillingDataPoint; 
                           rdfs:range ddhub:HydraulicLogicalElement; 
                           rdfs:subPropertyOf ddhub:IsHydraulicallyLocatedAt. 
ddhub:IsFluidVelocityAt a owl:ObjectProperty; 
                        rdfs:comment """
"""@EN; 
                        rdfs:domain ddhub:DrillingDataPoint; 
                        rdfs:range ddhub:HydraulicLogicalElement; 
                        rdfs:subPropertyOf ddhub:IsHydraulicallyLocatedAt. 
ddhub:IsForMotionType a owl:ObjectProperty; 
                      rdfs:comment """
"""@EN; 
                      rdfs:domain ddhub:DrillingDataPoint; 
                      rdfs:range ddhub:MotionType; 
                      rdfs:subPropertyOf ddhub:DWISVerb. 
ddhub:IsGeneratedBy a owl:ObjectProperty; 
                    rdfs:comment """
"""@EN; 
                    rdfs:domain ddhub:DrillingDataPoint; 
                    rdfs:range ddhub:DataFlowNode; 
                    rdfs:subPropertyOf ddhub:DWISVerb. 
ddhub:IsHydraulicallyLocatedAt a owl:ObjectProperty; 
                               rdfs:comment """
"""@EN; 
                               rdfs:domain ddhub:DrillingDataPoint; 
                               rdfs:range ddhub:HydraulicLogicalElement; 
                               rdfs:subPropertyOf ddhub:DWISVerb. 
ddhub:IsHydraulicConnectedTo a owl:ObjectProperty; 
                             rdfs:comment """
"""@EN; 
                             rdfs:domain ddhub:HydraulicLogicalElement; 
                             rdfs:range ddhub:HydraulicLogicalElement; 
                             rdfs:subPropertyOf ddhub:DWISVerb. 
ddhub:IsHydraulicEstimationAt a owl:ObjectProperty; 
                              rdfs:comment """
"""@EN; 
                              rdfs:domain ddhub:DrillingDataPoint; 
                              rdfs:range ddhub:HydraulicLogicalElement; 
                              rdfs:subPropertyOf ddhub:IsHydraulicallyLocatedAt. 
ddhub:IsHydraulicMaximumAllowedRateOfChangeAt a owl:ObjectProperty; 
                                              rdfs:comment """
"""@EN; 
                                              rdfs:domain ddhub:DrillingDataPoint; 
                                              rdfs:range ddhub:HydraulicLogicalElement; 
                                              rdfs:subPropertyOf ddhub:IsHydraulicallyLocatedAt. 
ddhub:IsHydraulicMaximumAllowedValueAt a owl:ObjectProperty; 
                                       rdfs:comment """
"""@EN; 
                                       rdfs:domain ddhub:DrillingDataPoint; 
                                       rdfs:range ddhub:HydraulicLogicalElement; 
                                       rdfs:subPropertyOf ddhub:IsHydraulicallyLocatedAt. 
ddhub:IsHydraulicMeasurementAt a owl:ObjectProperty; 
                               rdfs:comment """
"""@EN; 
                               rdfs:domain ddhub:DrillingDataPoint; 
                               rdfs:range ddhub:HydraulicLogicalElement; 
                               rdfs:subPropertyOf ddhub:IsHydraulicallyLocatedAt. 
ddhub:IsIdlingAfterTriggeredSignalFor a owl:ObjectProperty; 
                                      rdfs:comment """This verb is used to indicate that a `DrillingDataPoint` tells whether the isolation or the recovery
"""@EN; 
                                      rdfs:domain ddhub:DrillingDataPoint; 
                                      rdfs:range ddhub:FDIRFunction; 
                                      rdfs:subPropertyOf ddhub:DWISVerb. 
ddhub:IsIdlingSignalFor a owl:ObjectProperty; 
                        rdfs:comment """This verb is used to indicate a `DrillingDataPoint` that tells if the function is in an idle state.
A function that is idle must be enabled but does not perform any particular control on the machines. For instance, a 
`ProcedureFunction` that has reached its terminal state or a `ControllerFunction` that cannot control anymore its 
parameter because a limit is reached, e.g., autodriller when reaching the `MinDrillHeightVerticalLocation`, or an FDIR
function when there are no incidents that is detected. A SOE function is in idle state, if the used set-points are
within the limits, but if the limits are applied then the idle state is false, because the function acts on the set-points.
"""@EN; 
                        rdfs:domain ddhub:DrillingDataPoint; 
                        rdfs:range ddhub:RunnableFunction; 
                        rdfs:subPropertyOf ddhub:DWISVerb. 
ddhub:IsImpactDescriptionSignalFor a owl:ObjectProperty; 
                                   rdfs:comment """This verbs is used to indicate that a `DrillingDataPoint` used by an `FDIRFunction` can be used to
describe the impact of the function on the drilling process. This signal is supposed to be string value.
"""@EN; 
                                   rdfs:domain ddhub:DrillingDataPoint; 
                                   rdfs:range ddhub:FDIRFunction; 
                                   rdfs:subPropertyOf ddhub:DWISVerb. 
ddhub:IsIntegratedFrom a owl:ObjectProperty; 
                       rdfs:comment """
"""@EN; 
                       rdfs:domain ddhub:DWISNoun; 
                       rdfs:range ddhub:DWISNoun; 
                       rdfs:subPropertyOf ddhub:IsTransformationOutput. 
ddhub:IsLimitFor a owl:ObjectProperty; 
                 rdfs:comment """
"""@EN; 
                 rdfs:domain ddhub:DrillingDataPoint; 
                 rdfs:range ddhub:DWISNoun; 
                 rdfs:subPropertyOf ddhub:HasFunction. 
ddhub:IsMassFlowRateAt a owl:ObjectProperty; 
                       rdfs:comment """
"""@EN; 
                       rdfs:domain ddhub:DrillingDataPoint; 
                       rdfs:range ddhub:HydraulicLogicalElement; 
                       rdfs:subPropertyOf ddhub:IsHydraulicallyLocatedAt. 
ddhub:IsMaximumLimitFor a owl:ObjectProperty; 
                        rdfs:comment """
"""@EN; 
                        rdfs:domain ddhub:DrillingDataPoint; 
                        rdfs:range ddhub:DWISNoun; 
                        rdfs:subPropertyOf ddhub:IsLimitFor. 
ddhub:IsMeasuredBy a owl:ObjectProperty; 
                   rdfs:comment """
"""@EN; 
                   rdfs:domain ddhub:DWISNoun; 
                   rdfs:range ddhub:DWISNoun; 
                   rdfs:subPropertyOf ddhub:IsGeneratedBy. 
ddhub:IsMechanicallyConnectedTo a owl:ObjectProperty; 
                                rdfs:comment """
"""@EN; 
                                rdfs:domain ddhub:MechanicalLogicalElement; 
                                rdfs:range ddhub:MechanicalLogicalElement; 
                                rdfs:subPropertyOf ddhub:DWISVerb. 
ddhub:IsMechanicallyLocatedAt a owl:ObjectProperty; 
                              rdfs:comment """
"""@EN; 
                              rdfs:domain ddhub:DrillingDataPoint; 
                              rdfs:range ddhub:MechanicalLogicalElement; 
                              rdfs:subPropertyOf ddhub:DWISVerb. 
ddhub:IsMinimumLimitFor a owl:ObjectProperty; 
                        rdfs:comment """
"""@EN; 
                        rdfs:domain ddhub:DrillingDataPoint; 
                        rdfs:range ddhub:DWISNoun; 
                        rdfs:subPropertyOf ddhub:IsLimitFor. 
ddhub:IsObservableFrom a owl:ObjectProperty; 
                       rdfs:comment """
"""@EN; 
                       rdfs:domain ddhub:DWISNoun; 
                       rdfs:range ddhub:DWISNoun; 
                       rdfs:subPropertyOf ddhub:DWISVerb. 
ddhub:IsOfBaseQuantity a owl:ObjectProperty; 
                       rdfs:comment """
"""@EN; 
                       rdfs:domain ddhub:MeasurableQuantity; 
                       rdfs:range ddhub:Quantity; 
                       rdfs:subPropertyOf ddhub:DWISVerb. 
ddhub:IsOfMeasurableQuantity a owl:ObjectProperty; 
                             rdfs:comment """
"""@EN; 
                             rdfs:domain ddhub:DrillingSignal; 
                             rdfs:range ddhub:MeasurableQuantity; 
                             rdfs:subPropertyOf ddhub:DWISVerb. 
ddhub:IsOfMechanicalStiffnessType a owl:ObjectProperty; 
                                  rdfs:comment """A relation to describe how the drill-stem mechanical model manage stiffness.
"""@EN; 
                                  rdfs:domain ddhub:DrillStemMechanicalModel; 
                                  rdfs:range ddhub:MechanicalStiffnessType; 
                                  rdfs:subPropertyOf ddhub:DWISVerb. 
ddhub:IsolationSeal a owl:Class; 
                    rdfs:comment """
"""@EN; 
                    rdfs:subClassOf ddhub:DrillingEquipment. 
ddhub:IsOpeningRatioAt a owl:ObjectProperty; 
                       rdfs:comment """
"""@EN; 
                       rdfs:domain ddhub:DrillingDataPoint; 
                       rdfs:range ddhub:HydraulicLogicalElement; 
                       rdfs:subPropertyOf ddhub:IsHydraulicallyLocatedAt. 
ddhub:IsPhysicallyLocatedAt a owl:ObjectProperty; 
                            rdfs:comment """
"""@EN; 
                            rdfs:domain ddhub:DrillingDataPoint; 
                            rdfs:range ddhub:Location; 
                            rdfs:subPropertyOf ddhub:DWISVerb. 
ddhub:IsPressureAt a owl:ObjectProperty; 
                   rdfs:comment """
"""@EN; 
                   rdfs:domain ddhub:DrillingDataPoint; 
                   rdfs:range ddhub:HydraulicLogicalElement; 
                   rdfs:subPropertyOf ddhub:IsHydraulicallyLocatedAt. 
ddhub:IsPressureGradientAt a owl:ObjectProperty; 
                           rdfs:comment """
"""@EN; 
                           rdfs:domain ddhub:DrillingDataPoint; 
                           rdfs:range ddhub:HydraulicLogicalElement; 
                           rdfs:subPropertyOf ddhub:IsHydraulicallyLocatedAt. 
ddhub:IsProcessedBy a owl:ObjectProperty; 
                    rdfs:comment """
"""@EN; 
                    rdfs:domain ddhub:DWISNoun; 
                    rdfs:range ddhub:DWISNoun; 
                    rdfs:subPropertyOf ddhub:DWISVerb. 
ddhub:IsProvidedBy a owl:ObjectProperty; 
                   rdfs:comment """
"""@EN; 
                   rdfs:domain ddhub:DWISNoun; 
                   rdfs:range ddhub:DataProvider; 
                   rdfs:subPropertyOf ddhub:DWISVerb. 
ddhub:IsProvidedTo a owl:ObjectProperty; 
                   rdfs:comment """
"""@EN; 
                   rdfs:domain ddhub:DWISNoun; 
                   rdfs:range ddhub:DataProvider; 
                   rdfs:subPropertyOf ddhub:DWISVerb. 
ddhub:IsRecordedFrom a owl:ObjectProperty; 
                     rdfs:comment """
"""@EN; 
                     rdfs:domain ddhub:DWISNoun; 
                     rdfs:range ddhub:DWISNoun; 
                     rdfs:subPropertyOf ddhub:IsGeneratedBy. 
ddhub:IsRelatedToDrillingIncident a owl:ObjectProperty; 
                                  rdfs:comment """
"""@EN; 
                                  rdfs:domain ddhub:DrillingDataPoint; 
                                  rdfs:range ddhub:DrillingIncident; 
                                  rdfs:subPropertyOf ddhub:DWISVerb. 
ddhub:IsResampledBy a owl:ObjectProperty; 
                    rdfs:comment """
"""@EN; 
                    rdfs:domain ddhub:DrillingDataPoint; 
                    rdfs:range ddhub:Resampling; 
                    rdfs:subPropertyOf ddhub:IsTransformationOutput. 
ddhub:IsResamplingInput a owl:ObjectProperty; 
                        rdfs:comment """
"""@EN; 
                        rdfs:domain ddhub:DrillingDataPoint; 
                        rdfs:range ddhub:Resampling; 
                        rdfs:subPropertyOf ddhub:IsTransformationInput. 
ddhub:IsSetPointAdviceFor a owl:ObjectProperty; 
                          rdfs:comment """
"""@EN; 
                          rdfs:domain ddhub:DrillingDataPoint; 
                          rdfs:range ddhub:ControlSystem; 
                          rdfs:subPropertyOf ddhub:HasFunction. 
ddhub:IsSetPointFor a owl:ObjectProperty; 
                    rdfs:comment """
"""@EN; 
                    rdfs:domain ddhub:DrillingDataPoint; 
                    rdfs:range ddhub:Controller; 
                    rdfs:subPropertyOf ddhub:HasFunction. 
ddhub:IsSetPointMaximumAdviceFor a owl:ObjectProperty; 
                                 rdfs:comment """
"""@EN; 
                                 rdfs:domain ddhub:DrillingDataPoint; 
                                 rdfs:range ddhub:ControlSystem; 
                                 rdfs:subPropertyOf ddhub:HasFunction. 
ddhub:IsSetPointMaximumRecommendationFor a owl:ObjectProperty; 
                                         rdfs:comment """
"""@EN; 
                                         rdfs:domain ddhub:DrillingDataPoint; 
                                         rdfs:range ddhub:ControlSystem; 
                                         rdfs:subPropertyOf ddhub:HasFunction. 
ddhub:IsSetPointMinimumAdviceFor a owl:ObjectProperty; 
                                 rdfs:comment """
"""@EN; 
                                 rdfs:domain ddhub:DrillingDataPoint; 
                                 rdfs:range ddhub:ControlSystem; 
                                 rdfs:subPropertyOf ddhub:HasFunction. 
ddhub:IsSetPointMinimumRecommendationFor a owl:ObjectProperty; 
                                         rdfs:comment """
"""@EN; 
                                         rdfs:domain ddhub:DrillingDataPoint; 
                                         rdfs:range ddhub:ControlSystem; 
                                         rdfs:subPropertyOf ddhub:HasFunction. 
ddhub:IsSetPointRecommendationFor a owl:ObjectProperty; 
                                  rdfs:comment """
"""@EN; 
                                  rdfs:domain ddhub:DrillingDataPoint; 
                                  rdfs:range ddhub:ControlSystem; 
                                  rdfs:subPropertyOf ddhub:HasFunction. 
ddhub:IsSubPartOf a owl:ObjectProperty; 
                  rdfs:comment """
"""@EN; 
                  rdfs:domain ddhub:DrillingEquipment; 
                  rdfs:range ddhub:DrillingEquipment; 
                  rdfs:subPropertyOf ddhub:DWISVerb. 
ddhub:IsSynchronizationGroupInput a owl:ObjectProperty; 
                                  rdfs:comment """
"""@EN; 
                                  rdfs:domain ddhub:DrillingDataPoint; 
                                  rdfs:range ddhub:SynchronizationGroup; 
                                  rdfs:subPropertyOf ddhub:DWISVerb. 
ddhub:IsSynchronizationGroupOutput a owl:ObjectProperty; 
                                   rdfs:comment """
"""@EN; 
                                   rdfs:domain ddhub:DrillingDataPoint; 
                                   rdfs:range ddhub:SynchronizationGroup; 
                                   rdfs:subPropertyOf ddhub:DWISVerb. 
ddhub:IsToBeComparedWith a owl:ObjectProperty; 
                         rdfs:comment """
"""@EN; 
                         rdfs:domain ddhub:DrillingDataPoint; 
                         rdfs:range ddhub:DrillingDataPoint; 
                         rdfs:subPropertyOf ddhub:DWISVerb. 
ddhub:IsToBeDifferentFrom a owl:ObjectProperty; 
                          rdfs:comment """
"""@EN; 
                          rdfs:domain ddhub:DrillingDataPoint; 
                          rdfs:range ddhub:DrillingDataPoint; 
                          rdfs:subPropertyOf ddhub:IsToBeComparedWith. 
ddhub:IsToBeEqualTo a owl:ObjectProperty; 
                    rdfs:comment """
"""@EN; 
                    rdfs:domain ddhub:DrillingDataPoint; 
                    rdfs:range ddhub:DrillingDataPoint; 
                    rdfs:subPropertyOf ddhub:IsToBeComparedWith. 
ddhub:IsToBeGreaterOrEqualThan a owl:ObjectProperty; 
                               rdfs:comment """
"""@EN; 
                               rdfs:domain ddhub:DrillingDataPoint; 
                               rdfs:range ddhub:DrillingDataPoint; 
                               rdfs:subPropertyOf ddhub:IsToBeGreaterThan. 
ddhub:IsToBeGreaterThan a owl:ObjectProperty; 
                        rdfs:comment """
"""@EN; 
                        rdfs:domain ddhub:DrillingDataPoint; 
                        rdfs:range ddhub:DrillingDataPoint; 
                        rdfs:subPropertyOf ddhub:IsToBeComparedWith. 
ddhub:IsToBeSmallerOrEqualThan a owl:ObjectProperty; 
                               rdfs:comment """
"""@EN; 
                               rdfs:domain ddhub:DrillingDataPoint; 
                               rdfs:range ddhub:DrillingDataPoint; 
                               rdfs:subPropertyOf ddhub:IsToBeSmallerThan. 
ddhub:IsToBeSmallerThan a owl:ObjectProperty; 
                        rdfs:comment """
"""@EN; 
                        rdfs:domain ddhub:DrillingDataPoint; 
                        rdfs:range ddhub:DrillingDataPoint; 
                        rdfs:subPropertyOf ddhub:IsToBeComparedWith. 
ddhub:IsToBeStrictlyGreaterThan a owl:ObjectProperty; 
                                rdfs:comment """
"""@EN; 
                                rdfs:domain ddhub:DrillingDataPoint; 
                                rdfs:range ddhub:DrillingDataPoint; 
                                rdfs:subPropertyOf ddhub:IsToBeGreaterThan. 
ddhub:IsToBeStrictlySmallerThan a owl:ObjectProperty; 
                                rdfs:comment """
"""@EN; 
                                rdfs:domain ddhub:DrillingDataPoint; 
                                rdfs:range ddhub:DrillingDataPoint; 
                                rdfs:subPropertyOf ddhub:IsToBeSmallerThan. 
ddhub:IsTransformationInput a owl:ObjectProperty; 
                            rdfs:comment """
"""@EN; 
                            rdfs:domain ddhub:DrillingDataPoint; 
                            rdfs:range ddhub:Transformation; 
                            rdfs:subPropertyOf ddhub:HasFunction. 
ddhub:IsTransformationOutput a owl:ObjectProperty; 
                             rdfs:comment """
"""@EN; 
                             rdfs:domain ddhub:DrillingDataPoint; 
                             rdfs:range ddhub:DataFlowNode; 
                             rdfs:subPropertyOf ddhub:IsGeneratedBy. 
ddhub:IsTransmissionInput a owl:ObjectProperty; 
                          rdfs:comment """
"""@EN; 
                          rdfs:domain ddhub:DrillingDataPoint; 
                          rdfs:range ddhub:TransmissionLine; 
                          rdfs:subPropertyOf ddhub:HasFunction. 
ddhub:IsTransmissionOutput a owl:ObjectProperty; 
                           rdfs:comment """
"""@EN; 
                           rdfs:domain ddhub:DrillingDataPoint; 
                           rdfs:range ddhub:TransmissionLine; 
                           rdfs:subPropertyOf ddhub:IsGeneratedBy. 
ddhub:IsTransmittedBy a owl:ObjectProperty; 
                      rdfs:comment """Expresses that a signal is transmitted by some given telemetry system
"""@EN; 
                      rdfs:domain ddhub:DrillingDataPoint; 
                      rdfs:range ddhub:Telemetry; 
                      rdfs:subPropertyOf ddhub:DWISVerb. 
ddhub:IsTriggeredSignalFor a owl:ObjectProperty; 
                           rdfs:comment """This verb is used to indicate a `DrillingDataPoint` tells whether an `FDIRFunction` has been triggered
or not. This signal is expected to be a Boolean value. The signal is expected to be true from the moment the FDIR has triggered
to the moment it has recovered from the incident, if it has a recovery procedure, or to the moment the control is given
back to the end-user, in case of failure of the recovery procedure or at the end of the isolation procedure.
"""@EN; 
                           rdfs:domain ddhub:DrillingDataPoint; 
                           rdfs:range ddhub:FDIRFunction; 
                           rdfs:subPropertyOf ddhub:DWISVerb. 
ddhub:IsUnitForQuantity a owl:ObjectProperty; 
                        rdfs:comment """
"""@EN; 
                        rdfs:domain ddhub:Unit; 
                        rdfs:range ddhub:Quantity; 
                        rdfs:subPropertyOf ddhub:DWISVerb. 
ddhub:IsUsedExtraMarginSignalFor a owl:ObjectProperty; 
                                 rdfs:comment """This verb is used to indicate a `DrillingDataPoint` used by an `FDIRFunction` tells whether the
extra margin signal is used or not by the FDIR function. This signal is expected to be a boolean value.
"""@EN; 
                                 rdfs:domain ddhub:DrillingDataPoint; 
                                 rdfs:range ddhub:FDIRFunction; 
                                 rdfs:subPropertyOf ddhub:DWISVerb. 
ddhub:IsUserControllableExtraMarginSignalFor a owl:ObjectProperty; 
                                             rdfs:comment """This verb is used to indicate that a `DrillingDataPoint` used by an `FDIRFunction`, extends the calculated
threshold value for the fault detection by a user-defined amount. The value of this signal is supposed to be interpreted
in absolute value. If it is negative, then it is its magnitude that is used. This allows the end-user to increase the margin for
detection of an incident. 
"""@EN; 
                                             rdfs:domain ddhub:DrillingDataPoint; 
                                             rdfs:range ddhub:FDIRFunction; 
                                             rdfs:subPropertyOf ddhub:DWISVerb. 
ddhub:IsValid a owl:DatatypeProperty, owl:FunctionalProperty; 
              rdfs:comment """
"""@EN; 
              rdfs:domain ddhub:DrillingDataPoint; 
              rdfs:range xsd:bool. 
ddhub:IsValidBy a owl:ObjectProperty; 
                rdfs:comment """
"""@EN; 
                rdfs:domain ddhub:DWISNoun; 
                rdfs:range ddhub:DWISNoun; 
                rdfs:subPropertyOf ddhub:DWISVerb. 
ddhub:IsVolumeAt a owl:ObjectProperty; 
                 rdfs:comment """
"""@EN; 
                 rdfs:domain ddhub:DrillingDataPoint; 
                 rdfs:range ddhub:Tank; 
                 rdfs:subPropertyOf ddhub:IsHydraulicallyLocatedAt. 
ddhub:IsVolumetricFlowRateAt a owl:ObjectProperty; 
                             rdfs:comment """
"""@EN; 
                             rdfs:domain ddhub:DrillingDataPoint; 
                             rdfs:range ddhub:HydraulicLogicalElement; 
                             rdfs:subPropertyOf ddhub:IsHydraulicallyLocatedAt. 
ddhub:J a owl:DatatypeProperty, owl:FunctionalProperty; 
        rdfs:comment """Luminous intensity exponent.
SI Unit: Candela (cd)
"""@EN; 
        rdfs:domain ddhub:Quantity; 
        rdfs:range xsd:int. 
ddhub:JackupLegs a owl:Class; 
                 rdfs:comment """
"""@EN; 
                 rdfs:subClassOf ddhub:MarineSystem. 
ddhub:JarAction a owl:Class; 
                rdfs:comment """
"""@EN; 
                rdfs:subClassOf ddhub:JarringAssembly. 
ddhub:JarringAssembly a owl:Class; 
                      rdfs:comment """
"""@EN; 
                      rdfs:subClassOf ddhub:DrillingEquipment. 
ddhub:JettingAssembly a owl:Class; 
                      rdfs:comment """
"""@EN; 
                      rdfs:subClassOf ddhub:DrillingEquipment. 
ddhub:JunkBasket a owl:Class; 
                 rdfs:comment """
"""@EN; 
                 rdfs:subClassOf ddhub:FishingTools. 
ddhub:Kelly a owl:Class; 
            rdfs:comment """
"""@EN; 
            rdfs:subClassOf ddhub:RotaryTable. 
ddhub:KellyBushing a owl:Class; 
                   rdfs:comment """
"""@EN; 
                   rdfs:subClassOf ddhub:Kelly. 
ddhub:KellyBushingVerticalLocation a owl:Class; 
                                   rdfs:comment """
"""@EN; 
                                   rdfs:subClassOf ddhub:VerticalReferenceLocation. 
ddhub:KellyHose a owl:Class; 
                rdfs:comment """
"""@EN; 
                rdfs:subClassOf ddhub:Kelly. 
ddhub:KellyJoint a owl:Class; 
                 rdfs:comment """
"""@EN; 
                 rdfs:subClassOf ddhub:Kelly. 
ddhub:KellySwivel a owl:Class; 
                  rdfs:comment """
"""@EN; 
                  rdfs:subClassOf ddhub:Kelly. 
ddhub:KellyValve a owl:Class; 
                 rdfs:comment """
"""@EN; 
                 rdfs:subClassOf ddhub:WellControlSystem. 
ddhub:KickOffVerticalLocation a owl:Class; 
                              rdfs:comment """
"""@EN; 
                              rdfs:subClassOf ddhub:VerticalReferenceLocation. 
ddhub:KillLine a owl:Class; 
               rdfs:comment """
"""@EN; 
               rdfs:subClassOf ddhub:WellControlSystem. 
ddhub:L a owl:DatatypeProperty, owl:FunctionalProperty; 
        rdfs:comment """Length exponent.
SI Unit: meter (m)
"""@EN; 
        rdfs:domain ddhub:Quantity; 
        rdfs:range xsd:int. 
ddhub:LandBop a owl:Class; 
              rdfs:comment """
"""@EN; 
              rdfs:subClassOf ddhub:BopStack. 
ddhub:LandingJoint a owl:Class; 
                   rdfs:comment """
"""@EN; 
                   rdfs:subClassOf ddhub:MarineSystem. 
ddhub:LandingString a owl:Class; 
                    rdfs:comment """
"""@EN; 
                    rdfs:subClassOf ddhub:CasingEquipment. 
ddhub:LargeVolumeQuantity a owl:Class; 
                          rdfs:comment """
"""@EN; 
                          rdfs:subClassOf ddhub:MeasurableQuantity. 
ddhub:LastCasingShoeReferenceLocation a owl:Class; 
                                      rdfs:comment """
"""@EN; 
                                      rdfs:subClassOf ddhub:AbscissaReferenceLocation. 
ddhub:LateralModelling a owl:Class; 
                       rdfs:comment """The model accounts for the lateral movement of some parts of the physical system.
"""@EN; 
                       rdfs:subClassOf ddhub:ModelledDegreeOfFreedom. 
ddhub:LateralMotionType a owl:Class; 
                        rdfs:comment """
"""@EN; 
                        rdfs:subClassOf ddhub:MotionType. 
ddhub:LeapSeconds a owl:DatatypeProperty, owl:FunctionalProperty; 
                  rdfs:comment """
"""@EN; 
                  rdfs:domain ddhub:Clock; 
                  rdfs:range xsd:int. 
ddhub:LeaseLinePositionLocation a owl:Class; 
                                rdfs:comment """
"""@EN; 
                                rdfs:subClassOf ddhub:PositionReferenceLocation. 
ddhub:LedgeLocation a owl:Class; 
                    rdfs:comment """
"""@EN; 
                    rdfs:subClassOf ddhub:AbscissaReferenceLocation. 
ddhub:LeftToRight a owl:DatatypeProperty, owl:FunctionalProperty; 
                  rdfs:comment """Indicates whether the fluid can flow from the left branch to the right branch though the junction
"""@EN; 
                  rdfs:domain ddhub:HydraulicJunction; 
                  rdfs:range xsd:bool. 
ddhub:LengthQuantity a owl:Class; 
                     rdfs:comment """
"""@EN; 
                     rdfs:subClassOf ddhub:Quantity. 
ddhub:Limit a owl:Class; 
            rdfs:comment """
"""@EN; 
            rdfs:subClassOf ddhub:ProcessData. 
ddhub:Liner a owl:Class; 
            rdfs:comment """
"""@EN; 
            rdfs:subClassOf ddhub:PistonMudPump. 
ddhub:LinerDrilling a owl:Class; 
                    rdfs:comment """
"""@EN; 
                    rdfs:subClassOf ddhub:DrillingEquipment. 
ddhub:LinerHanger a owl:Class; 
                  rdfs:comment """
"""@EN; 
                  rdfs:subClassOf ddhub:Hangers. 
ddhub:LinerPacker a owl:Class; 
                  rdfs:comment """
"""@EN; 
                  rdfs:subClassOf ddhub:CasingEquipment. 
ddhub:Liners a owl:Class; 
             rdfs:comment """
"""@EN; 
             rdfs:subClassOf ddhub:CasingString. 
ddhub:LiquidComponent a owl:Class; 
                      rdfs:comment """
"""@EN; 
                      rdfs:subClassOf ddhub:FluidComponent. 
ddhub:LoadNut a owl:Class; 
              rdfs:comment """
"""@EN; 
              rdfs:subClassOf ddhub:TopDrive. 
ddhub:LocalTimeReference a owl:Class; 
                         rdfs:comment """
"""@EN; 
                         rdfs:subClassOf ddhub:RelativeTimeReference. 
ddhub:Location a owl:Class; 
               rdfs:comment """Physical location for a signal. Refers to: 1) a reference frame (via the HasReferenceFrame relation), that works as a system of coordinates 2) an origin (of type Location) via the HasReferenceFrameOrigin relation.
 - some coordinates
"""@EN; 
               rdfs:subClassOf ddhub:DWISNoun. 
ddhub:LoggingEquipment a owl:Class; 
                       rdfs:comment """
"""@EN; 
                       rdfs:subClassOf ddhub:DownholeEquipment. 
ddhub:LoggingServiceCompany a owl:Class; 
                            rdfs:comment """A logging service company is an entity that gathers measured information during well construction.
"""@EN; 
                            rdfs:subClassOf ddhub:ServiceCompany. 
ddhub:LoggingWhileDrillingTools a owl:Class; 
                                rdfs:comment """
"""@EN; 
                                rdfs:subClassOf ddhub:LoggingEquipment. 
ddhub:LoggingWhileDrillingToolsAcoustictools a owl:Class; 
                                             rdfs:comment """
"""@EN; 
                                             rdfs:subClassOf ddhub:LoggingWhileDrillingTools. 
ddhub:LoggingWhileDrillingToolsElectricalpropagation a owl:Class; 
                                                     rdfs:comment """
"""@EN; 
                                                     rdfs:subClassOf ddhub:LoggingWhileDrillingTools. 
ddhub:LoggingWhileDrillingToolsElectricalresistivity a owl:Class; 
                                                     rdfs:comment """
"""@EN; 
                                                     rdfs:subClassOf ddhub:LoggingWhileDrillingTools. 
ddhub:LoggingWhileDrillingToolsNmrtools a owl:Class; 
                                        rdfs:comment """
"""@EN; 
                                        rdfs:subClassOf ddhub:LoggingWhileDrillingTools. 
ddhub:LoggingWhileDrillingToolsNucleartools a owl:Class; 
                                            rdfs:comment """
"""@EN; 
                                            rdfs:subClassOf ddhub:LoggingWhileDrillingTools. 
ddhub:LoggingWhileDrillingToolsSeismictools a owl:Class; 
                                            rdfs:comment """
"""@EN; 
                                            rdfs:subClassOf ddhub:LoggingWhileDrillingTools. 
ddhub:LogName a owl:DatatypeProperty, owl:FunctionalProperty; 
              rdfs:comment """
"""@EN; 
              rdfs:domain ddhub:WitsMLTimeBasedLogEndPoint; 
              rdfs:range xsd:string. 
ddhub:LogUID a owl:DatatypeProperty, owl:FunctionalProperty; 
             rdfs:comment """
"""@EN; 
             rdfs:domain ddhub:WitsMLTimeBasedLogEndPoint; 
             rdfs:range xsd:string. 
ddhub:LossCirculation a owl:Class; 
                      rdfs:comment """
"""@EN; 
                      rdfs:subClassOf ddhub:DrillingIncident. 
ddhub:LowerMarineRiserPackageLmrp a owl:Class; 
                                  rdfs:comment """
"""@EN; 
                                  rdfs:subClassOf ddhub:MarineSystem. 
ddhub:LowestAstronomicalTideVerticalLocation a owl:Class; 
                                             rdfs:comment """
"""@EN; 
                                             rdfs:subClassOf ddhub:VerticalReferenceLocation. 
ddhub:LowGravitySolidComponent a owl:Class; 
                               rdfs:comment """
"""@EN; 
                               rdfs:subClassOf ddhub:DrillingFluidSolidComponent. 
ddhub:LowPassFilter a owl:Class; 
                    rdfs:comment """
"""@EN; 
                    rdfs:subClassOf ddhub:Filter. 
ddhub:LowPressureRiser a owl:Class; 
                       rdfs:comment """
"""@EN; 
                       rdfs:subClassOf ddhub:SurfaceRiser. 
ddhub:LT a owl:Class; 
         rdfs:comment """
"""@EN; 
         rdfs:subClassOf ddhub:ValidityCondition. 
ddhub:LuminousIntensityQuantity a owl:Class; 
                                rdfs:comment """
"""@EN; 
                                rdfs:subClassOf ddhub:Quantity. 
ddhub:M a owl:DatatypeProperty, owl:FunctionalProperty; 
        rdfs:comment """Mass exponent.
SI Unit: Kilogram (kg)
"""@EN; 
        rdfs:domain ddhub:Quantity; 
        rdfs:range xsd:int. 
ddhub:MagneticFluxDensityQuantity a owl:Class; 
                                  rdfs:comment """
"""@EN; 
                                  rdfs:subClassOf ddhub:Quantity. 
ddhub:MagneticFluxQuantity a owl:Class; 
                           rdfs:comment """
"""@EN; 
                           rdfs:subClassOf ddhub:Quantity. 
ddhub:MagneticHighSideAngleLocation a owl:Class; 
                                    rdfs:comment """
"""@EN; 
                                    rdfs:subClassOf ddhub:AngleReferenceLocation. 
ddhub:MagneticNorthAzimuthLocation a owl:Class; 
                                   rdfs:comment """
"""@EN; 
                                   rdfs:subClassOf ddhub:AzimuthReferenceLocation. 
ddhub:MainframeAssembly a owl:Class; 
                        rdfs:comment """
"""@EN; 
                        rdfs:subClassOf ddhub:TopDrive. 
ddhub:mandrel a owl:Class; 
              rdfs:comment """
"""@EN; 
              rdfs:subClassOf ddhub:Connection. 
ddhub:ManualPipeTongs a owl:Class; 
                      rdfs:comment """
"""@EN; 
                      rdfs:subClassOf ddhub:DrillPipeTongs. 
ddhub:ManualSlips a owl:Class; 
                  rdfs:comment """
"""@EN; 
                  rdfs:subClassOf ddhub:RotarySlips. 
ddhub:MarineFuel a owl:Class; 
                 rdfs:comment """
"""@EN; 
                 rdfs:subClassOf ddhub:MarineSystem. 
ddhub:MarineRiser a owl:Class; 
                  rdfs:comment """
"""@EN; 
                  rdfs:subClassOf ddhub:DrillingRiser. 
ddhub:MarineRiserTensionerMrtRing a owl:Class; 
                                  rdfs:comment """
"""@EN; 
                                  rdfs:subClassOf ddhub:MarineSystem. 
ddhub:MarineSystem a owl:Class; 
                   rdfs:comment """
"""@EN; 
                   rdfs:subClassOf ddhub:RigEquipment. 
ddhub:MassGradientQuantity a owl:Class; 
                           rdfs:comment """
"""@EN; 
                           rdfs:subClassOf ddhub:Quantity. 
ddhub:MassQuantity a owl:Class; 
                   rdfs:comment """
"""@EN; 
                   rdfs:subClassOf ddhub:Quantity. 
ddhub:MassRateQuantity a owl:Class; 
                       rdfs:comment """
"""@EN; 
                       rdfs:subClassOf ddhub:Quantity. 
ddhub:MassTransferBasedDiscretization a owl:Class; 
                                      rdfs:comment """A model can properly estimate values at the level of mass transfer propagation.
"""@EN; 
                                      rdfs:subClassOf ddhub:ModellingDiscretization. 
ddhub:MaterialStrengthQuantity a owl:Class; 
                               rdfs:comment """
"""@EN; 
                               rdfs:subClassOf ddhub:Quantity. 
ddhub:MathematicalModel a owl:Class; 
                        rdfs:comment """A model for which the state variables do not change with time.
"""@EN; 
                        rdfs:subClassOf ddhub:DWISNoun. 
ddhub:MaxFrequency a owl:DatatypeProperty, owl:FunctionalProperty; 
                   rdfs:comment """
"""@EN; 
                   rdfs:domain ddhub:BandPassFilter; 
                   rdfs:range xsd:double. 
ddhub:MaximumFluctuations a owl:DatatypeProperty, owl:FunctionalProperty; 
                          rdfs:comment """
"""@EN; 
                          rdfs:domain ddhub:Clock; 
                          rdfs:range xsd:double. 
ddhub:MaximumLimit a owl:Class; 
                   rdfs:comment """
"""@EN; 
                   rdfs:subClassOf ddhub:Limit. 
ddhub:MeanHigherHighWaterVerticalLocation a owl:Class; 
                                          rdfs:comment """
"""@EN; 
                                          rdfs:subClassOf ddhub:VerticalReferenceLocation. 
ddhub:MeanHighWaterVerticalLocation a owl:Class; 
                                    rdfs:comment """
"""@EN; 
                                    rdfs:subClassOf ddhub:VerticalReferenceLocation. 
ddhub:MeaningfulPrecision a owl:DatatypeProperty, owl:FunctionalProperty; 
                          rdfs:comment """
"""@EN; 
                          rdfs:domain ddhub:MeasurableQuantity; 
                          rdfs:range xsd:double. 
ddhub:MeanLowerLowWaterVerticalLocation a owl:Class; 
                                        rdfs:comment """
"""@EN; 
                                        rdfs:subClassOf ddhub:VerticalReferenceLocation. 
ddhub:MeanLowWaterVerticalLocation a owl:Class; 
                                   rdfs:comment """
"""@EN; 
                                   rdfs:subClassOf ddhub:VerticalReferenceLocation. 
ddhub:MeanSeaLevelVerticalLocation a owl:Class; 
                                   rdfs:comment """
"""@EN; 
                                   rdfs:subClassOf ddhub:VerticalReferenceLocation. 
ddhub:MeanTideLevelVerticalLocation a owl:Class; 
                                    rdfs:comment """
"""@EN; 
                                    rdfs:subClassOf ddhub:VerticalReferenceLocation. 
ddhub:MeasurableQuantity a owl:Class; 
                         rdfs:comment """Represents a quantity that allows meaningful comparisons.
Are related by a Quantity via the "IsObservableFrom" relation. 
Context dependent: for example, Fluid density and Equivalent Circulating Density are represented as two different "Measurable quantities", although they both refer to the same base SI quantities. 
"""@EN; 
                         rdfs:subClassOf ddhub:DWISNoun. 
ddhub:MeasurableQuantityUnitAssociation a owl:Class; 
                                        rdfs:comment """
"""@EN; 
                                        rdfs:subClassOf ddhub:DWISNoun. 
ddhub:MeasuredDepth a owl:Class; 
                    rdfs:comment """
"""@EN; 
                    rdfs:subClassOf ddhub:PrototypeData. 
ddhub:MeasuredDepthToTrueVerticalDepthTransformation a owl:Class; 
                                                     rdfs:comment """
"""@EN; 
                                                     rdfs:subClassOf ddhub:DirectTransformation. 
ddhub:MeasuredDepthTranslation a owl:Class; 
                               rdfs:comment """
"""@EN; 
                               rdfs:subClassOf ddhub:DirectTransformation. 
ddhub:Measurement a owl:Class; 
                  rdfs:comment """The noun Measurement represents individuals that are measured by some instrument and which value can be compared with another measurement.
"""@EN; 
                  rdfs:subClassOf ddhub:PhysicalData. 
ddhub:MeasurementDevice a owl:Class; 
                        rdfs:comment """Denotes a physical sensor
"""@EN; 
                        rdfs:subClassOf ddhub:DataFlowNode. 
ddhub:MeasurementIndex a owl:DatatypeProperty, owl:FunctionalProperty; 
                       rdfs:comment """
"""@EN; 
                       rdfs:domain ddhub:EndPointMapping; 
                       rdfs:range xsd:int. 
ddhub:MeasurementWhileDrillingTools a owl:Class; 
                                    rdfs:comment """
"""@EN; 
                                    rdfs:subClassOf ddhub:LoggingEquipment. 
ddhub:MechanicalBlock a owl:Class; 
                      rdfs:comment """
"""@EN; 
                      rdfs:subClassOf ddhub:HoistingSystem. 
ddhub:MechanicalDrawworks a owl:Class; 
                          rdfs:comment """
"""@EN; 
                          rdfs:subClassOf ddhub:Drawworks. 
ddhub:MechanicalElementState a owl:Class; 
                             rdfs:comment """
"""@EN; 
                             rdfs:subClassOf ddhub:DWISNoun. 
ddhub:MechanicalJar a owl:Class; 
                    rdfs:comment """
"""@EN; 
                    rdfs:subClassOf ddhub:JarringAssembly. 
ddhub:MechanicalLogicalElement a owl:Class; 
                               rdfs:comment """
"""@EN; 
                               rdfs:subClassOf ddhub:DWISNoun. 
ddhub:MechanicallyActiveState a owl:Class; 
                              rdfs:comment """
"""@EN; 
                              rdfs:subClassOf ddhub:MechanicalElementState. 
ddhub:MechanicallyClosedState a owl:Class; 
                              rdfs:comment """
"""@EN; 
                              rdfs:subClassOf ddhub:MechanicalElementState. 
ddhub:MechanicallyConnectedState a owl:Class; 
                                 rdfs:comment """
"""@EN; 
                                 rdfs:subClassOf ddhub:MechanicalElementState. 
ddhub:MechanicallyInactiveState a owl:Class; 
                                rdfs:comment """
"""@EN; 
                                rdfs:subClassOf ddhub:MechanicalElementState. 
ddhub:MechanicallyOpenState a owl:Class; 
                            rdfs:comment """
"""@EN; 
                            rdfs:subClassOf ddhub:MechanicalElementState. 
ddhub:MechanicalSoftModel a owl:Class; 
                          rdfs:comment """An infinitively soft model assumes that the drill-stem deforms without any resistance when compressive loads are applied.
"""@EN; 
                          rdfs:subClassOf ddhub:MechanicalStiffnessType. 
ddhub:MechanicalSpecificEnergy a owl:Class; 
                               rdfs:comment """
"""@EN; 
                               rdfs:subClassOf ddhub:PrototypeData. 
ddhub:MechanicalStiffModel a owl:Class; 
                           rdfs:comment """A stiff mechanical model considers that the drill-stem can deform laterally when put in compression.
"""@EN; 
                           rdfs:subClassOf ddhub:MechanicalStiffnessType. 
ddhub:MechanicalStiffModelAssumedContacts a owl:Class; 
                                          rdfs:comment """Such a stiff mechanical model presuposes the position of the contact points.
"""@EN; 
                                          rdfs:subClassOf ddhub:MechanicalStiffModel. 
ddhub:MechanicalStiffModelEstimatedContacts a owl:Class; 
                                            rdfs:comment """Such a stiff mechanical model estimates the position of the contact points.
"""@EN; 
                                            rdfs:subClassOf ddhub:MechanicalStiffModel. 
ddhub:MechanicalStiffnessType a owl:Class; 
                              rdfs:comment """A description of how the drill-stem stiffness is modelled.
"""@EN; 
                              rdfs:subClassOf ddhub:DWISNoun. 
ddhub:MechanicsAndVibrationTools a owl:Class; 
                                 rdfs:comment """
"""@EN; 
                                 rdfs:subClassOf ddhub:MeasurementWhileDrillingTools. 
ddhub:melon a owl:Class; 
            rdfs:comment """
"""@EN; 
            rdfs:subClassOf ddhub:BladeShape. 
ddhub:MillCasingCutting a owl:Class; 
                        rdfs:comment """
"""@EN; 
                        rdfs:subClassOf ddhub:CasingMillingTools. 
ddhub:MillDress a owl:Class; 
                rdfs:comment """
"""@EN; 
                rdfs:subClassOf ddhub:CasingMillingTools. 
ddhub:MillFlatBottom a owl:Class; 
                     rdfs:comment """
"""@EN; 
                     rdfs:subClassOf ddhub:CasingMillingTools. 
ddhub:MillHollow a owl:Class; 
                 rdfs:comment """
"""@EN; 
                 rdfs:subClassOf ddhub:CasingMillingTools. 
ddhub:MillPackerPickerAssembly a owl:Class; 
                               rdfs:comment """
"""@EN; 
                               rdfs:subClassOf ddhub:CasingMillingTools. 
ddhub:MillPilot a owl:Class; 
                rdfs:comment """
"""@EN; 
                rdfs:subClassOf ddhub:CasingMillingTools. 
ddhub:MillPolish a owl:Class; 
                 rdfs:comment """
"""@EN; 
                 rdfs:subClassOf ddhub:CasingMillingTools. 
ddhub:MillSection a owl:Class; 
                  rdfs:comment """
"""@EN; 
                  rdfs:subClassOf ddhub:CasingMillingTools. 
ddhub:MillTaper a owl:Class; 
                rdfs:comment """
"""@EN; 
                rdfs:subClassOf ddhub:CasingMillingTools. 
ddhub:MillTooth a owl:Class; 
                rdfs:comment """
"""@EN; 
                rdfs:subClassOf ddhub:RollingCutter. 
ddhub:MillWashover a owl:Class; 
                   rdfs:comment """
"""@EN; 
                   rdfs:subClassOf ddhub:CasingMillingTools. 
ddhub:MillWatermelon a owl:Class; 
                     rdfs:comment """
"""@EN; 
                     rdfs:subClassOf ddhub:CasingMillingTools. 
ddhub:MinDrillHeightVerticalLocation a owl:Class; 
                                     rdfs:comment """
"""@EN; 
                                     rdfs:subClassOf ddhub:VerticalReferenceLocation. 
ddhub:MinFrequency a owl:DatatypeProperty, owl:FunctionalProperty; 
                   rdfs:comment """
"""@EN; 
                   rdfs:domain ddhub:BandPassFilter; 
                   rdfs:range xsd:double. 
ddhub:MinimumHorizontalStress a owl:Class; 
                              rdfs:comment """
"""@EN; 
                              rdfs:subClassOf ddhub:PrototypeData. 
ddhub:MinimumHorizontalStressGradient a owl:Class; 
                                      rdfs:comment """
"""@EN; 
                                      rdfs:subClassOf ddhub:PrototypeData. 
ddhub:MinimumLimit a owl:Class; 
                   rdfs:comment """
"""@EN; 
                   rdfs:subClassOf ddhub:Limit. 
ddhub:MinMaxUncertainty a owl:Class; 
                        rdfs:comment """The uncertainty is represented by a uniform probability distribution between a `Min` and a `Max` value.
"""@EN; 
                        rdfs:subClassOf ddhub:SignalUncertainty. 
ddhub:MiscSubs a owl:Class; 
               rdfs:comment """
"""@EN; 
               rdfs:subClassOf ddhub:DrillString. 
ddhub:MixingTank a owl:Class; 
                 rdfs:comment """
"""@EN; 
                 rdfs:subClassOf ddhub:MudPits. 
ddhub:Mnemonic a owl:DatatypeProperty, owl:FunctionalProperty; 
               rdfs:comment """
"""@EN; 
               rdfs:domain ddhub:WitsMLTimeBasedLogEndPoint; 
               rdfs:range xsd:string. 
ddhub:ModelledDegreeOfFreedom a owl:Class; 
                              rdfs:comment """In physics and chemistry, a degree of freedom is an independent physical parameter in the formal description of the state of a physical system. A model may account for some or all of the degrees of freedom of the physical system.
"""@EN; 
                              rdfs:subClassOf ddhub:DWISNoun. 
ddhub:ModellingDimensions a owl:Class; 
                          rdfs:comment """The number of dimensions that are accounted by the model
"""@EN; 
                          rdfs:subClassOf ddhub:DWISNoun. 
ddhub:ModellingDiscretization a owl:Class; 
                              rdfs:comment """A characteristic of the discretization made by the model.
"""@EN; 
                              rdfs:subClassOf ddhub:DWISNoun. 
ddhub:ModelType a owl:Class; 
                rdfs:comment """
"""@EN; 
                rdfs:subClassOf ddhub:DWISNoun. 
ddhub:MooringLines a owl:Class; 
                   rdfs:comment """
"""@EN; 
                   rdfs:subClassOf ddhub:MooringSystem. 
ddhub:MooringSystem a owl:Class; 
                    rdfs:comment """
"""@EN; 
                    rdfs:subClassOf ddhub:MarineSystem. 
ddhub:MotionType a owl:Class; 
                 rdfs:comment """
"""@EN; 
                 rdfs:subClassOf ddhub:DWISNoun. 
ddhub:Mousehole a owl:Class; 
                rdfs:comment """
"""@EN; 
                rdfs:subClassOf ddhub:DrillFloorStructure. 
ddhub:MovingAverage a owl:Class; 
                    rdfs:comment """
"""@EN; 
                    rdfs:subClassOf ddhub:Filter. 
ddhub:MovingMax a owl:Class; 
                rdfs:comment """
"""@EN; 
                rdfs:subClassOf ddhub:Filter. 
ddhub:MovingMin a owl:Class; 
                rdfs:comment """
"""@EN; 
                rdfs:subClassOf ddhub:Filter. 
ddhub:MovingStandardDeviation a owl:Class; 
                              rdfs:comment """
"""@EN; 
                              rdfs:subClassOf ddhub:Filter. 
ddhub:MPDAlternateFlowPath a owl:Class; 
                           rdfs:comment """
"""@EN; 
                           rdfs:subClassOf ddhub:TopsideHydraulicNetwork. 
ddhub:MpdChoke a owl:Class; 
               rdfs:comment """
"""@EN; 
               rdfs:subClassOf ddhub:WellControlSystem. 
ddhub:MPDChokeOpening a owl:Class; 
                      rdfs:comment """
"""@EN; 
                      rdfs:subClassOf ddhub:PrototypeData. 
ddhub:MPDChokePressure a owl:Class; 
                       rdfs:comment """
"""@EN; 
                       rdfs:subClassOf ddhub:PrototypeData. 
ddhub:MPDMainFlowPath a owl:Class; 
                      rdfs:comment """
"""@EN; 
                      rdfs:subClassOf ddhub:TopsideHydraulicNetwork. 
ddhub:MPDPumpFlowRate a owl:Class; 
                      rdfs:comment """
"""@EN; 
                      rdfs:subClassOf ddhub:PrototypeData. 
ddhub:MPDPumpRate a owl:Class; 
                  rdfs:comment """
"""@EN; 
                  rdfs:subClassOf ddhub:PrototypeData. 
ddhub:MudHose a owl:Class; 
              rdfs:comment """
"""@EN; 
              rdfs:subClassOf ddhub:MudLines. 
ddhub:MudLines a owl:Class; 
               rdfs:comment """
"""@EN; 
               rdfs:subClassOf ddhub:CirculationSystem. 
ddhub:MudLineSystem a owl:Class; 
                    rdfs:comment """
"""@EN; 
                    rdfs:subClassOf ddhub:MarineSystem. 
ddhub:MudLoggingEquipment a owl:Class; 
                          rdfs:comment """
"""@EN; 
                          rdfs:subClassOf ddhub:RigEquipment. 
ddhub:MudLubeBearing a owl:Class; 
                     rdfs:comment """
"""@EN; 
                     rdfs:subClassOf ddhub:DownholeMotor. 
ddhub:MudMixing a owl:Class; 
                rdfs:comment """
"""@EN; 
                rdfs:subClassOf ddhub:HydraulicJunction. 
ddhub:MudPits a owl:Class; 
              rdfs:comment """
"""@EN; 
              rdfs:subClassOf ddhub:CirculationSystem. 
ddhub:MudPulse a owl:Class; 
               rdfs:comment """
"""@EN; 
               rdfs:subClassOf ddhub:EquipmentTelemetry. 
ddhub:MudPulseTelemetry a owl:Class; 
                        rdfs:comment """A method that allows transfer of downhole data to the surface via pressure pulses sent trough the drilling fluid.
"""@EN; 
                        rdfs:subClassOf ddhub:DownHoleTelemetry. 
ddhub:MudPump a owl:Class; 
              rdfs:comment """
"""@EN; 
              rdfs:subClassOf ddhub:CirculationSystem. 
ddhub:MudPumpsControlSystem a owl:Class; 
                            rdfs:comment """
"""@EN; 
                            rdfs:subClassOf ddhub:ControlSystem. 
ddhub:MudStandpipe a owl:Class; 
                   rdfs:comment """
"""@EN; 
                   rdfs:subClassOf ddhub:MudLines. 
ddhub:MudStandpipeManifold a owl:Class; 
                           rdfs:comment """
"""@EN; 
                           rdfs:subClassOf ddhub:MudLines. 
ddhub:N a owl:DatatypeProperty, owl:FunctionalProperty; 
        rdfs:comment """Amount of substance exponent.
SI Unit: Mole (N)
"""@EN; 
        rdfs:domain ddhub:Quantity; 
        rdfs:range xsd:int. 
ddhub:NearBit a owl:Class; 
              rdfs:comment """
"""@EN; 
              rdfs:subClassOf ddhub:Stabilizers. 
ddhub:NearbitReamers a owl:Class; 
                     rdfs:comment """
"""@EN; 
                     rdfs:subClassOf ddhub:Reamers. 
ddhub:NearBitVibrationDampers a owl:Class; 
                              rdfs:comment """
"""@EN; 
                              rdfs:subClassOf ddhub:ActiveVibrationTools. 
ddhub:NetworkSynchronizationLatencyAverage a owl:DatatypeProperty, owl:FunctionalProperty; 
                                           rdfs:comment """
"""@EN; 
                                           rdfs:domain ddhub:Clock; 
                                           rdfs:range xsd:double. 
ddhub:NetworkSynchronizationLatencyStandardDeviation a owl:DatatypeProperty, owl:FunctionalProperty; 
                                                     rdfs:comment """
"""@EN; 
                                                     rdfs:domain ddhub:Clock; 
                                                     rdfs:range xsd:double. 
ddhub:Non-Magnetic a owl:Class; 
                   rdfs:comment """
"""@EN; 
                   rdfs:subClassOf ddhub:Stabilizers. 
ddhub:Non-Rotating a owl:Class; 
                   rdfs:comment """
"""@EN; 
                   rdfs:subClassOf ddhub:Stabilizers. 
ddhub:NonmagneticCollars a owl:Class; 
                         rdfs:comment """
"""@EN; 
                         rdfs:subClassOf ddhub:DrillString. 
ddhub:NormalizedDataType a owl:Class; 
                         rdfs:comment """between 0 and 1
"""@EN; 
                         rdfs:subClassOf ddhub:ContinuousDataType. 
ddhub:NorthEastFrame a owl:Class; 
                     rdfs:comment """
"""@EN; 
                     rdfs:subClassOf ddhub:CartesianTwoDimensionalReferenceFrame. 
ddhub:NorthEastTVDFrame a owl:Class; 
                        rdfs:comment """
"""@EN; 
                        rdfs:subClassOf ddhub:CartesianThreeDimensionalReferenceFrame. 
ddhub:NozzleDiameterQuantity a owl:Class; 
                             rdfs:comment """
"""@EN; 
                             rdfs:subClassOf ddhub:MeasurableQuantity. 
ddhub:Nozzles a owl:Class; 
              rdfs:comment """
"""@EN; 
              rdfs:subClassOf ddhub:DrillingBit. 
ddhub:NumberOfItems a owl:DatatypeProperty, owl:FunctionalProperty; 
                    rdfs:comment """
"""@EN; 
                    rdfs:domain ddhub:NumberOfItemsRangeExtraction; 
                    rdfs:range xsd:int. 
ddhub:NumberOfItemsRangeExtraction a owl:Class; 
                                   rdfs:comment """
"""@EN; 
                                   rdfs:subClassOf ddhub:RangeExtraction. 
ddhub:NumberOfRepeaters a owl:DatatypeProperty, owl:FunctionalProperty; 
                        rdfs:comment """
"""@EN; 
                        rdfs:domain ddhub:Telemetry; 
                        rdfs:range xsd:int. 
ddhub:NumberOfSampleMovingAverage a owl:Class; 
                                  rdfs:comment """
"""@EN; 
                                  rdfs:subClassOf ddhub:MovingAverage. 
ddhub:NumberOfSamples a owl:DatatypeProperty, owl:FunctionalProperty; 
                      rdfs:comment """
"""@EN; 
                      rdfs:domain ddhub:NumberOfSampleMovingAverage; 
                      rdfs:range xsd:int. 
ddhub:OilBasedMudObm a owl:Class; 
                     rdfs:comment """
"""@EN; 
                     rdfs:subClassOf ddhub:DrillingFluid. 
ddhub:OilBearing a owl:Class; 
                 rdfs:comment """
"""@EN; 
                 rdfs:subClassOf ddhub:DownholeMotor. 
ddhub:OneDimensionalCartesianReferenceFrame a owl:Class; 
                                            rdfs:comment """
"""@EN; 
                                            rdfs:subClassOf ddhub:OneDimensionalReferenceFrame. 
ddhub:OneDimensionalCurviLinearReferenceFrame a owl:Class; 
                                              rdfs:comment """
"""@EN; 
                                              rdfs:subClassOf ddhub:OneDimensionalReferenceFrame. 
ddhub:OneDimensionalReferenceFrame a owl:Class; 
                                   rdfs:comment """
"""@EN; 
                                   rdfs:subClassOf ddhub:ReferenceFrame. 
ddhub:OneDModelling a owl:Class; 
                    rdfs:comment """The model only accounts for one dimension
"""@EN; 
                    rdfs:subClassOf ddhub:ModellingDimensions. 
ddhub:OpenChannel a owl:Class; 
                  rdfs:comment """
"""@EN; 
                  rdfs:subClassOf ddhub:HydraulicBranch. 
ddhub:OpenHole a owl:Class; 
               rdfs:comment """
"""@EN; 
               rdfs:subClassOf ddhub:Pipe. 
ddhub:OpenholeTools a owl:Class; 
                    rdfs:comment """
"""@EN; 
                    rdfs:subClassOf ddhub:WirelineLoggingTools. 
ddhub:OperatingCompany a owl:Class; 
                       rdfs:comment """An operating company is an entity that holds the rights to explore, develop, and produce hydrocarbon resources from a particular oil or gas field or lease
"""@EN; 
                       rdfs:subClassOf ddhub:DataProvider. 
ddhub:OperationalPlan a owl:Class; 
                      rdfs:comment """
"""@EN; 
                      rdfs:subClassOf ddhub:Plan. 
ddhub:OuterBarrel a owl:Class; 
                  rdfs:comment """
"""@EN; 
                  rdfs:subClassOf ddhub:CoringTool. 
ddhub:OverburdenPressure a owl:Class; 
                         rdfs:comment """
"""@EN; 
                         rdfs:subClassOf ddhub:PrototypeData. 
ddhub:OverburdenPressureGradient a owl:Class; 
                                 rdfs:comment """
"""@EN; 
                                 rdfs:subClassOf ddhub:PrototypeData. 
ddhub:Overpull a owl:Class; 
               rdfs:comment """
"""@EN; 
               rdfs:subClassOf ddhub:DrillingIncident. 
ddhub:Overshot a owl:Class; 
               rdfs:comment """
"""@EN; 
               rdfs:subClassOf ddhub:FishingTools. 
ddhub:OverTorque a owl:Class; 
                 rdfs:comment """
"""@EN; 
                 rdfs:subClassOf ddhub:DrillingIncident. 
ddhub:PDC a owl:Class; 
          rdfs:comment """
"""@EN; 
          rdfs:subClassOf ddhub:FixedCutter. 
ddhub:PdcCore a owl:Class; 
              rdfs:comment """
"""@EN; 
              rdfs:subClassOf ddhub:FixedCutter. 
ddhub:PerforatingGuns a owl:Class; 
                      rdfs:comment """
"""@EN; 
                      rdfs:subClassOf ddhub:CasingEquipment. 
ddhub:PeristalticMudPump a owl:Class; 
                         rdfs:comment """
"""@EN; 
                         rdfs:subClassOf ddhub:MudPump. 
ddhub:PermeabilityQuantity a owl:Class; 
                           rdfs:comment """
"""@EN; 
                           rdfs:subClassOf ddhub:MeasurableQuantity. 
ddhub:PhysicalData a owl:Class; 
                   rdfs:comment """
"""@EN; 
                   rdfs:subClassOf ddhub:DrillingDataPoint. 
ddhub:PhysicalState a owl:Class; 
                    rdfs:comment """
"""@EN; 
                    rdfs:subClassOf ddhub:ComputedState. 
ddhub:pin a owl:Class; 
          rdfs:comment """
"""@EN; 
          rdfs:subClassOf ddhub:Connection. 
ddhub:Pin-Pin a owl:Class; 
              rdfs:comment """
"""@EN; 
              rdfs:subClassOf ddhub:TubularConfiguration. 
ddhub:PinDown a owl:Class; 
              rdfs:comment """
"""@EN; 
              rdfs:subClassOf ddhub:TubularConfiguration. 
ddhub:PinUp a owl:Class; 
            rdfs:comment """
"""@EN; 
            rdfs:subClassOf ddhub:TubularConfiguration. 
ddhub:Pipe a owl:Class; 
           rdfs:comment """
"""@EN; 
           rdfs:subClassOf ddhub:HydraulicBranch. 
ddhub:PipeDiameterQuantity a owl:Class; 
                           rdfs:comment """
"""@EN; 
                           rdfs:subClassOf ddhub:MeasurableQuantity. 
ddhub:PipeRam a owl:Class; 
              rdfs:comment """
"""@EN; 
              rdfs:subClassOf ddhub:BopElement. 
ddhub:PipeWashout a owl:Class; 
                  rdfs:comment """
"""@EN; 
                  rdfs:subClassOf ddhub:DrillingIncident. 
ddhub:PipeWashoutLocation a owl:Class; 
                          rdfs:comment """
"""@EN; 
                          rdfs:subClassOf ddhub:AbscissaReferenceLocation. 
ddhub:Piston a owl:Class; 
             rdfs:comment """
"""@EN; 
             rdfs:subClassOf ddhub:PistonMudPump. 
ddhub:PistonMudPump a owl:Class; 
                    rdfs:comment """
"""@EN; 
                    rdfs:subClassOf ddhub:MudPump. 
ddhub:Plan a owl:Class; 
           rdfs:comment """
"""@EN; 
           rdfs:subClassOf ddhub:DataFlowNode. 
ddhub:PlaneAngleQuantity a owl:Class; 
                         rdfs:comment """
"""@EN; 
                         rdfs:subClassOf ddhub:Quantity. 
ddhub:Plugged a owl:Class; 
              rdfs:comment """
"""@EN; 
              rdfs:subClassOf ddhub:DrillingIncident. 
ddhub:Plugs a owl:Class; 
            rdfs:comment """
"""@EN; 
            rdfs:subClassOf ddhub:CasingEquipment. 
ddhub:PlungerFloatValvesF a owl:Class; 
                          rdfs:comment """
"""@EN; 
                          rdfs:subClassOf ddhub:FloatValveNonreturnValve. 
ddhub:PlungerMudPump a owl:Class; 
                     rdfs:comment """
"""@EN; 
                     rdfs:subClassOf ddhub:MudPump. 
ddhub:PneumaticSlips a owl:Class; 
                     rdfs:comment """
"""@EN; 
                     rdfs:subClassOf ddhub:RotarySlips. 
ddhub:Point-The-Bit a owl:Class; 
                    rdfs:comment """
"""@EN; 
                    rdfs:subClassOf ddhub:RotarySteerableSystems. 
ddhub:PolarReferenceFrame a owl:Class; 
                          rdfs:comment """
"""@EN; 
                          rdfs:subClassOf ddhub:TwoDimensionalReferenceFrame. 
ddhub:PoreDiameterQuantity a owl:Class; 
                           rdfs:comment """
"""@EN; 
                           rdfs:subClassOf ddhub:MeasurableQuantity. 
ddhub:PorePressure a owl:Class; 
                   rdfs:comment """
"""@EN; 
                   rdfs:subClassOf ddhub:PrototypeData. 
ddhub:PorePressureGradient a owl:Class; 
                           rdfs:comment """
"""@EN; 
                           rdfs:subClassOf ddhub:PrototypeData. 
ddhub:PoreSurfaceQuantity a owl:Class; 
                          rdfs:comment """
"""@EN; 
                          rdfs:subClassOf ddhub:MeasurableQuantity. 
ddhub:PorosityQuantity a owl:Class; 
                       rdfs:comment """
"""@EN; 
                       rdfs:subClassOf ddhub:MeasurableQuantity. 
ddhub:PortedPlungerValvesFa a owl:Class; 
                            rdfs:comment """
"""@EN; 
                            rdfs:subClassOf ddhub:FloatValveNonreturnValve. 
ddhub:PositionQuantity a owl:Class; 
                       rdfs:comment """
"""@EN; 
                       rdfs:subClassOf ddhub:MeasurableQuantity. 
ddhub:PositionReferenceLocation a owl:Class; 
                                rdfs:comment """
"""@EN; 
                                rdfs:subClassOf ddhub:Location. 
ddhub:PositiveDisplacementMotor a owl:Class; 
                                rdfs:comment """
"""@EN; 
                                rdfs:subClassOf ddhub:DownholeMotor. 
ddhub:PostiveUpward a owl:DatatypeProperty, owl:FunctionalProperty; 
                    rdfs:comment """
"""@EN; 
                    rdfs:domain ddhub:OneDimensionalReferenceFrame; 
                    rdfs:range xsd:bool. 
ddhub:PotableWater a owl:Class; 
                   rdfs:comment """
"""@EN; 
                   rdfs:subClassOf ddhub:DrillingFluid. 
ddhub:PowerGenerationSystem a owl:Class; 
                            rdfs:comment """
"""@EN; 
                            rdfs:subClassOf ddhub:RigEquipment. 
ddhub:PowerGenerators a owl:Class; 
                      rdfs:comment """
"""@EN; 
                      rdfs:subClassOf ddhub:PowerGenerationSystem. 
ddhub:PowerPipeTongs a owl:Class; 
                     rdfs:comment """
"""@EN; 
                     rdfs:subClassOf ddhub:DrillPipeTongs. 
ddhub:PowerScrSystem a owl:Class; 
                     rdfs:comment """
"""@EN; 
                     rdfs:subClassOf ddhub:PowerGenerationSystem. 
ddhub:PowerSlips a owl:Class; 
                 rdfs:comment """
"""@EN; 
                 rdfs:subClassOf ddhub:RotarySlips. 
ddhub:PowerSupply a owl:Class; 
                  rdfs:comment """
"""@EN; 
                  rdfs:subClassOf ddhub:CoiledTubingEquipment. 
ddhub:PowerSystems a owl:Class; 
                   rdfs:comment """
"""@EN; 
                   rdfs:subClassOf ddhub:LoggingEquipment. 
ddhub:Precision a owl:DatatypeProperty, owl:FunctionalProperty; 
                rdfs:comment """The standard deviation of the repetitive error component of the uncertainty of the sensor. The assumed mean value of the attached Gaussian distribution is the measured value. The value is expected to be in the same physical quantity as the sensor value.
"""@EN; 
                rdfs:domain ddhub:SensorUncertainty; 
                rdfs:range xsd:double. 
ddhub:PressureGradientQuantity a owl:Class; 
                               rdfs:comment """
"""@EN; 
                               rdfs:subClassOf ddhub:Quantity. 
ddhub:PressureLoggingTools a owl:Class; 
                           rdfs:comment """
"""@EN; 
                           rdfs:subClassOf ddhub:WirelineLoggingTools. 
ddhub:PressureLossConstantQuantity a owl:Class; 
                                   rdfs:comment """
"""@EN; 
                                   rdfs:subClassOf ddhub:Quantity. 
ddhub:PressureQuantity a owl:Class; 
                       rdfs:comment """
"""@EN; 
                       rdfs:subClassOf ddhub:Quantity. 
ddhub:PressureReference a owl:Class; 
                        rdfs:comment """
"""@EN; 
                        rdfs:subClassOf ddhub:DWISNoun. 
ddhub:PressureToEquivalentDensityTransformation a owl:Class; 
                                                rdfs:comment """
"""@EN; 
                                                rdfs:subClassOf ddhub:DirectTransformation. 
ddhub:PressureToForceTransformation a owl:Class; 
                                    rdfs:comment """
"""@EN; 
                                    rdfs:subClassOf ddhub:DirectTransformation. 
ddhub:ProceduralState a owl:Class; 
                      rdfs:comment """
"""@EN; 
                      rdfs:subClassOf ddhub:ComputedState. 
ddhub:ProcedureFunction a owl:Class; 
                        rdfs:comment """A `ProcedureFunction` is a `RunnableFunction` that executes a finites state automaton, i.e., a graph of
transitions between states. It should be noted that a `ProcedureFunction` may use control algorithms while being in one
state or when transiting from state to state. An example of `ProcedureFunction` is a friction test. A friction test has
at least three states: rotation off bottom, pick-up without rotation, slack-off without rotation. The transitions 
between the different states may depend on the implementation. Each of those states uses a controller, one that controls
the rotational speed and one that controls the axial speed.
"""@EN; 
                        rdfs:subClassOf ddhub:RunnableFunction. 
ddhub:ProcessData a owl:Class; 
                  rdfs:comment """
"""@EN; 
                  rdfs:subClassOf ddhub:DrillingDataPoint. 
ddhub:ProcessState a owl:Class; 
                   rdfs:comment """
"""@EN; 
                   rdfs:subClassOf ddhub:ComputedState. 
ddhub:ProductionTools a owl:Class; 
                      rdfs:comment """
"""@EN; 
                      rdfs:subClassOf ddhub:WirelineLoggingTools. 
ddhub:ProportionError a owl:DatatypeProperty, owl:FunctionalProperty; 
                      rdfs:comment """The proportion error on the signal. The value is expected to be a dimensionless physical quantity between 0 and 1 in SI unit. This proportion is applied to the `Fullscale` to obtain the standard deviation of the Gaussian probability distribution that describes the uncertainty of the signal. The mean value of that Gaussian distribution is the signal value.
"""@EN; 
                      rdfs:domain ddhub:FullScaleUncertainty; 
                      rdfs:range xsd:double. 
ddhub:ProportionQuantity a owl:Class; 
                         rdfs:comment """
"""@EN; 
                         rdfs:subClassOf ddhub:Quantity. 
ddhub:ProtectionFunction a owl:Class; 
                         rdfs:comment """A `ProtectionFunction` is an `ActivableFunction`. It must be activated to have an effect, but the effect
is to protect the drilling process, either by protecting the inputs to the drilling machines to avoid generating 
a drilling incident, or to detect an abnormal drilling process state and react to the situation.
detected.
"""@EN; 
                         rdfs:subClassOf ddhub:ActivableFunction. 
ddhub:PrototypeData a owl:Class; 
                    rdfs:comment """
"""@EN; 
                    rdfs:subClassOf ddhub:DrillingDataPoint. 
ddhub:ProviderName a owl:DatatypeProperty, owl:FunctionalProperty; 
                   rdfs:comment """
"""@EN; 
                   rdfs:domain ddhub:DataProvider, ddhub:OperatingCompany, ddhub:ServiceCompany, ddhub:DirectionalServiceCompany, ddhub:DrillingFluidProvider, ddhub:LoggingServiceCompany, ddhub:CementingServiceCompany, ddhub:DataAnalysisServiceCompany, ddhub:DrillingContractor, ddhub:DWISInternalService; 
                   rdfs:range xsd:string. 
ddhub:PulsationDampener a owl:Class; 
                        rdfs:comment """
"""@EN; 
                        rdfs:subClassOf ddhub:PistonMudPump. 
ddhub:PumpRate a owl:Class; 
               rdfs:comment """
"""@EN; 
               rdfs:subClassOf ddhub:PrototypeData. 
ddhub:PupJoints a owl:Class; 
                rdfs:comment """
"""@EN; 
                rdfs:subClassOf ddhub:DrillString. 
ddhub:Push-The-Bit a owl:Class; 
                   rdfs:comment """
"""@EN; 
                   rdfs:subClassOf ddhub:RotarySteerableSystems. 
ddhub:PwdPressure a owl:Class; 
                  rdfs:comment """
"""@EN; 
                  rdfs:subClassOf ddhub:MeasurementWhileDrillingTools. 
ddhub:QuadristandDerrick a owl:Class; 
                         rdfs:comment """
"""@EN; 
                         rdfs:subClassOf ddhub:Derrick. 
ddhub:Quantity a owl:Class; 
               rdfs:comment """
"""@EN; 
               rdfs:subClassOf ddhub:DWISNoun. 
ddhub:Quill a owl:Class; 
            rdfs:comment """
"""@EN; 
            rdfs:subClassOf ddhub:TopDrive. 
ddhub:RackAndPinionHoistingSystem a owl:Class; 
                                  rdfs:comment """
"""@EN; 
                                  rdfs:subClassOf ddhub:HoistingSystem. 
ddhub:RadialModelling a owl:Class; 
                      rdfs:comment """The model accounts for the radial movement of some parts of the physical system.
"""@EN; 
                      rdfs:subClassOf ddhub:LateralModelling. 
ddhub:RamHoistingSystem a owl:Class; 
                        rdfs:comment """
"""@EN; 
                        rdfs:subClassOf ddhub:HoistingSystem. 
ddhub:RamRig a owl:Class; 
             rdfs:comment """
"""@EN; 
             rdfs:subClassOf ddhub:Drawworks. 
ddhub:RandomWalkQuantity a owl:Class; 
                         rdfs:comment """
"""@EN; 
                         rdfs:subClassOf ddhub:Quantity. 
ddhub:RangeExtraction a owl:Class; 
                      rdfs:comment """
"""@EN; 
                      rdfs:subClassOf ddhub:TimeBasedTransformation. 
ddhub:RateOfPenetrationQuantity a owl:Class; 
                                rdfs:comment """
"""@EN; 
                                rdfs:subClassOf ddhub:MeasurableQuantity. 
ddhub:Reamers a owl:Class; 
              rdfs:comment """
"""@EN; 
              rdfs:subClassOf ddhub:DrillingEquipment. 
ddhub:Recommendation a owl:Class; 
                     rdfs:comment """
"""@EN; 
                     rdfs:subClassOf ddhub:ProcessData. 
ddhub:RecommendedMaximum a owl:Class; 
                         rdfs:comment """
"""@EN; 
                         rdfs:subClassOf ddhub:Recommendation. 
ddhub:RecommendedMinimum a owl:Class; 
                         rdfs:comment """
"""@EN; 
                         rdfs:subClassOf ddhub:Recommendation. 
ddhub:RecommendedTarget a owl:Class; 
                        rdfs:comment """
"""@EN; 
                        rdfs:subClassOf ddhub:Recommendation. 
ddhub:RectangularChannel a owl:Class; 
                         rdfs:comment """
"""@EN; 
                         rdfs:subClassOf ddhub:OpenChannel. 
ddhub:ReferenceFrame a owl:Class; 
                     rdfs:comment """Represents a system of coordinates
"""@EN; 
                     rdfs:subClassOf ddhub:DWISNoun. 
ddhub:RelativePressureReference a owl:Class; 
                                rdfs:comment """
"""@EN; 
                                rdfs:subClassOf ddhub:PressureReference. 
ddhub:RelativeTemperatureQuantity a owl:Class; 
                                  rdfs:comment """
"""@EN; 
                                  rdfs:subClassOf ddhub:Quantity. 
ddhub:RelativeTimeReference a owl:Class; 
                            rdfs:comment """
"""@EN; 
                            rdfs:subClassOf ddhub:TimeReference. 
ddhub:Resampling a owl:Class; 
                 rdfs:comment """
"""@EN; 
                 rdfs:subClassOf ddhub:TimeBasedTransformation. 
ddhub:ResamplingDelay a owl:DatatypeProperty, owl:FunctionalProperty; 
                      rdfs:comment """
"""@EN; 
                      rdfs:domain ddhub:Resampling; 
                      rdfs:range xsd:double. 
ddhub:ResamplingRate a owl:DatatypeProperty, owl:FunctionalProperty; 
                     rdfs:comment """
"""@EN; 
                     rdfs:domain ddhub:Resampling; 
                     rdfs:range xsd:double. 
ddhub:ReservePit a owl:Class; 
                 rdfs:comment """
"""@EN; 
                 rdfs:subClassOf ddhub:MudPits. 
ddhub:ResistivityQuantity a owl:Class; 
                          rdfs:comment """
"""@EN; 
                          rdfs:subClassOf ddhub:Quantity. 
ddhub:Resolution a owl:DatatypeProperty, owl:FunctionalProperty; 
                 rdfs:comment """
"""@EN; 
                 rdfs:domain ddhub:Clock; 
                 rdfs:range xsd:double. 
ddhub:ReturnFlowLine a owl:Class; 
                     rdfs:comment """
"""@EN; 
                     rdfs:subClassOf ddhub:Pipe. 
ddhub:RfidReamers a owl:Class; 
                  rdfs:comment """
"""@EN; 
                  rdfs:subClassOf ddhub:Reamers. 
ddhub:RheologyConsistencyIndexQuantity a owl:Class; 
                                       rdfs:comment """
"""@EN; 
                                       rdfs:subClassOf ddhub:MeasurableQuantity. 
ddhub:RiemannianManifoldFourDimensionalReferenceFrame a owl:Class; 
                                                      rdfs:comment """
"""@EN; 
                                                      rdfs:subClassOf ddhub:FourDimensionalReferenceFrame. 
ddhub:RiemannianManifoldThreeDimensionalReferenceFrame a owl:Class; 
                                                       rdfs:comment """
"""@EN; 
                                                       rdfs:subClassOf ddhub:ThreeDimensionalReferenceFrame. 
ddhub:RiemannianManifoldTwoDimensionalReferenceFrame a owl:Class; 
                                                     rdfs:comment """
"""@EN; 
                                                     rdfs:subClassOf ddhub:TwoDimensionalReferenceFrame. 
ddhub:RigActionPlan a owl:Class; 
                    rdfs:comment """
"""@EN; 
                    rdfs:subClassOf ddhub:Plan. 
ddhub:RigChokeControlSystem a owl:Class; 
                            rdfs:comment """
"""@EN; 
                            rdfs:subClassOf ddhub:ControlSystem. 
ddhub:RigEquipment a owl:Class; 
                   rdfs:comment """
"""@EN; 
                   rdfs:subClassOf <http://ddhub.no/<equipment>>. 
ddhub:RigFloor a owl:Class; 
               rdfs:comment """
"""@EN; 
               rdfs:subClassOf ddhub:DrillFloorStructure. 
ddhub:RightToLeft a owl:DatatypeProperty, owl:FunctionalProperty; 
                  rdfs:comment """Indicates whether the fluid can flow from the right branch to the left branch though the junction
"""@EN; 
                  rdfs:domain ddhub:HydraulicJunction; 
                  rdfs:range xsd:bool. 
ddhub:RiserLiftPump a owl:Class; 
                    rdfs:comment """
"""@EN; 
                    rdfs:subClassOf ddhub:CirculationSystem. 
ddhub:RiserRecoilSystem a owl:Class; 
                        rdfs:comment """
"""@EN; 
                        rdfs:subClassOf ddhub:MarineSystem. 
ddhub:RiserTensioners a owl:Class; 
                      rdfs:comment """
"""@EN; 
                      rdfs:subClassOf ddhub:MarineSystem. 
ddhub:RollerReamers a owl:Class; 
                    rdfs:comment """
"""@EN; 
                    rdfs:subClassOf ddhub:Reamers. 
ddhub:RollingCutter a owl:Class; 
                    rdfs:comment """
"""@EN; 
                    rdfs:subClassOf ddhub:DrillingBit. 
ddhub:ROP a owl:Class; 
          rdfs:comment """
"""@EN; 
          rdfs:subClassOf ddhub:PrototypeData. 
ddhub:RotarySlips a owl:Class; 
                  rdfs:comment """
"""@EN; 
                  rdfs:subClassOf ddhub:DrillFloorEquipment. 
ddhub:RotarySteerableSystems a owl:Class; 
                             rdfs:comment """
"""@EN; 
                             rdfs:subClassOf ddhub:DrillingEquipment. 
ddhub:RotaryTable a owl:Class; 
                  rdfs:comment """
"""@EN; 
                  rdfs:subClassOf ddhub:SurfaceRotationSystem. 
ddhub:RotaryTableBushings a owl:Class; 
                          rdfs:comment """
"""@EN; 
                          rdfs:subClassOf ddhub:RotaryTable. 
ddhub:RotaryTableVerticalLocation a owl:Class; 
                                  rdfs:comment """
"""@EN; 
                                  rdfs:subClassOf ddhub:VerticalReferenceLocation. 
ddhub:RotatingControlDeviceRcd a owl:Class; 
                               rdfs:comment """
"""@EN; 
                               rdfs:subClassOf ddhub:DrillFloorEquipment. 
ddhub:RotationalModelling a owl:Class; 
                          rdfs:comment """The model accounts for the rotational movement of some parts of the physical system.
"""@EN; 
                          rdfs:subClassOf ddhub:ModelledDegreeOfFreedom. 
ddhub:RotationFrequencyQuantity a owl:Class; 
                                rdfs:comment """
"""@EN; 
                                rdfs:subClassOf ddhub:MeasurableQuantity. 
ddhub:RotationFrequencyRateOfChangeQuantity a owl:Class; 
                                            rdfs:comment """
"""@EN; 
                                            rdfs:subClassOf ddhub:Quantity. 
ddhub:ROV a owl:Class; 
          rdfs:comment """
"""@EN; 
          rdfs:subClassOf ddhub:MarineSystem. 
ddhub:RunnableFunction a owl:Class; 
                       rdfs:comment """A runnable function is a function that starts to run immediately when activated.
"""@EN; 
                       rdfs:subClassOf ddhub:ActivableFunction. 
ddhub:SafetyClamps a owl:Class; 
                   rdfs:comment """
"""@EN; 
                   rdfs:subClassOf ddhub:DrillFloorEquipment. 
ddhub:SafetyEquipment a owl:Class; 
                      rdfs:comment """
"""@EN; 
                      rdfs:subClassOf ddhub:RigEquipment. 
ddhub:SamplingRate a owl:DatatypeProperty, owl:FunctionalProperty; 
                   rdfs:comment """
"""@EN; 
                   rdfs:domain ddhub:SynchronizationGroup; 
                   rdfs:range xsd:double. 
ddhub:SandTrap a owl:Class; 
               rdfs:comment """
"""@EN; 
               rdfs:subClassOf ddhub:MudPits. 
ddhub:ScreenString a owl:Class; 
                   rdfs:comment """
"""@EN; 
                   rdfs:subClassOf <http://ddhub.no/<Tubulars>>. 
ddhub:ScribeLineAngleLocation a owl:Class; 
                              rdfs:comment """
"""@EN; 
                              rdfs:subClassOf ddhub:AngleReferenceLocation. 
ddhub:SeaFloorVerticalLocation a owl:Class; 
                               rdfs:comment """
"""@EN; 
                               rdfs:subClassOf ddhub:VerticalReferenceLocation. 
ddhub:SeaWater a owl:Class; 
               rdfs:comment """
"""@EN; 
               rdfs:subClassOf ddhub:DrillingFluid. 
ddhub:self-sealing-threaded a owl:Class; 
                            rdfs:comment """
"""@EN; 
                            rdfs:subClassOf ddhub:Connection. 
ddhub:SemiCircularChannel a owl:Class; 
                          rdfs:comment """
"""@EN; 
                          rdfs:subClassOf ddhub:OpenChannel. 
ddhub:SensorUncertainty a owl:Class; 
                        rdfs:comment """The uncertainty of the sensor is described by a systematic bias and repetitive error. The systematic bias is referred to as the `Accuracy` while the repetitive error is referred to as the `Precision`. The standard deviation of the overall Gaussian distribution is $\\sqrt{\\sigma^2{_a}+\\sigma^2{_p}}$ where $\\sigma_a$ is the accuracy and $\\sigma_p$ is the precision. The `Accuracy` or the `Precision` can either be defined as attribute values, for example when they have fixed values, or using another facts utilizing the verbs `HasAccuracy` or respectively `HasPrecision` when these values may change through time.
"""@EN; 
                        rdfs:subClassOf ddhub:GaussianUncertainty. 
ddhub:Seperator a owl:Class; 
                rdfs:comment """
"""@EN; 
                rdfs:subClassOf ddhub:WellTestingEquipment. 
ddhub:ServiceCompany a owl:Class; 
                     rdfs:comment """A service company is an entity that provides services during the well construction.
"""@EN; 
                     rdfs:subClassOf ddhub:DataProvider. 
ddhub:SetPoint a owl:Class; 
               rdfs:comment """
"""@EN; 
               rdfs:subClassOf ddhub:ProcessData. 
ddhub:ShakerCascadeLevels a owl:Class; 
                          rdfs:comment """
"""@EN; 
                          rdfs:subClassOf ddhub:ShaleShakers. 
ddhub:ShakerDecks a owl:Class; 
                  rdfs:comment """
"""@EN; 
                  rdfs:subClassOf ddhub:ShaleShakers. 
ddhub:ShakerHopper a owl:Class; 
                   rdfs:comment """
"""@EN; 
                   rdfs:subClassOf ddhub:ShaleShakers. 
ddhub:ShakerScreenMeshSize a owl:Class; 
                           rdfs:comment """
"""@EN; 
                           rdfs:subClassOf ddhub:ShakerDecks. 
ddhub:ShakerScreens a owl:Class; 
                    rdfs:comment """
"""@EN; 
                    rdfs:subClassOf ddhub:ShakerDecks. 
ddhub:ShaleShakers a owl:Class; 
                   rdfs:comment """
"""@EN; 
                   rdfs:subClassOf ddhub:CirculationSystem. 
ddhub:ShearRam a owl:Class; 
               rdfs:comment """
"""@EN; 
               rdfs:subClassOf ddhub:BopElement. 
ddhub:ShearRate a owl:Class; 
                rdfs:comment """
"""@EN; 
                rdfs:subClassOf ddhub:PrototypeData. 
ddhub:ShearStress a owl:Class; 
                  rdfs:comment """
"""@EN; 
                  rdfs:subClassOf ddhub:PrototypeData. 
ddhub:ShoeTrack a owl:Class; 
                rdfs:comment """
"""@EN; 
                rdfs:subClassOf ddhub:CasingEquipment. 
ddhub:ShortDc a owl:Class; 
              rdfs:comment """
"""@EN; 
              rdfs:subClassOf ddhub:DrillString. 
ddhub:SignalProcessingUnit a owl:Class; 
                           rdfs:comment """Represent any signal processing applied prior to the distribution of the considered signal. Signal processing refers to e.g. noise removal, filtering,..
"""@EN; 
                           rdfs:subClassOf ddhub:Transformation. 
ddhub:SignalUncertainty a owl:Class; 
                        rdfs:comment """Represent the uncertainty associated to a `DrillingDataPoint`.
"""@EN; 
                        rdfs:subClassOf ddhub:DWISNoun. 
ddhub:Simulator a owl:Class; 
                rdfs:comment """
"""@EN; 
                rdfs:subClassOf ddhub:ComputationUnit. 
ddhub:SingleActing a owl:Class; 
                   rdfs:comment """
"""@EN; 
                   rdfs:subClassOf ddhub:Action. 
ddhub:SingleJointDerrick a owl:Class; 
                         rdfs:comment """
"""@EN; 
                         rdfs:subClassOf ddhub:Derrick. 
ddhub:Singles a owl:Class; 
              rdfs:comment """
"""@EN; 
              rdfs:subClassOf ddhub:Grouping. 
ddhub:SIUnit a owl:DatatypeProperty, owl:FunctionalProperty; 
             rdfs:comment """
"""@EN; 
             rdfs:domain ddhub:Quantity; 
             rdfs:range xsd:string. 
ddhub:SlantDerrick a owl:Class; 
                   rdfs:comment """
"""@EN; 
                   rdfs:subClassOf ddhub:Derrick. 
ddhub:sleeve a owl:Class; 
             rdfs:comment """
"""@EN; 
             rdfs:subClassOf ddhub:BladeType. 
ddhub:SlickLine a owl:Class; 
                rdfs:comment """
"""@EN; 
                rdfs:subClassOf ddhub:DrillFloorEquipment. 
ddhub:SlipJoint a owl:Class; 
                rdfs:comment """
"""@EN; 
                rdfs:subClassOf ddhub:MarineSystem. 
ddhub:SlugSettlingPit a owl:Class; 
                      rdfs:comment """
"""@EN; 
                      rdfs:subClassOf ddhub:MudPits. 
ddhub:SmallDiameterQuantity a owl:Class; 
                            rdfs:comment """
"""@EN; 
                            rdfs:subClassOf ddhub:MeasurableQuantity. 
ddhub:SmallLengthQuantity a owl:Class; 
                          rdfs:comment """
"""@EN; 
                          rdfs:subClassOf ddhub:MeasurableQuantity. 
ddhub:SmallProportionQuantity a owl:Class; 
                              rdfs:comment """
"""@EN; 
                              rdfs:subClassOf ddhub:MeasurableQuantity. 
ddhub:SmallRotationFrequencyQuantity a owl:Class; 
                                     rdfs:comment """
"""@EN; 
                                     rdfs:subClassOf ddhub:MeasurableQuantity. 
ddhub:SmallTorqueQuantity a owl:Class; 
                          rdfs:comment """
"""@EN; 
                          rdfs:subClassOf ddhub:MeasurableQuantity. 
ddhub:SOEFunction a owl:Class; 
                  rdfs:comment """A `SOEFunction` is a `ProtectionFunction` that limits the commands that are send to the drilling machines
to avoid generating a drilling incident. SOE stands for Safe Operating Envelope. A `SOEFunction` protects the inputs
of the drilling process. An example `SOEFunction` is a swab/surge limits protection. This function limits the axial acceleration
and speed of the drill-stem to avoid generate swabbing pressure below the maximum of the collapse and pore pressure, and
surging pressure above the fracturing pressure.
"""@EN; 
                  rdfs:subClassOf ddhub:ProtectionFunction. 
ddhub:SolidAngleQuantity a owl:Class; 
                         rdfs:comment """
"""@EN; 
                         rdfs:subClassOf ddhub:Quantity. 
ddhub:SolidComponent a owl:Class; 
                     rdfs:comment """
"""@EN; 
                     rdfs:subClassOf ddhub:FluidComponent. 
ddhub:SpacingSpool a owl:Class; 
                   rdfs:comment """
"""@EN; 
                   rdfs:subClassOf ddhub:WellControlSystem. 
ddhub:Spear a owl:Class; 
            rdfs:comment """
"""@EN; 
            rdfs:subClassOf ddhub:FishingTools. 
ddhub:SpecificHeatCapacityQuantity a owl:Class; 
                                   rdfs:comment """
"""@EN; 
                                   rdfs:subClassOf ddhub:Quantity. 
ddhub:SpecificHeatCapacityTemperatureGradientQuantity a owl:Class; 
                                                      rdfs:comment """
"""@EN; 
                                                      rdfs:subClassOf ddhub:Quantity. 
ddhub:SphericalReferenceFrame a owl:Class; 
                              rdfs:comment """
"""@EN; 
                              rdfs:subClassOf ddhub:ThreeDimensionalReferenceFrame. 
ddhub:SpiderGimbal a owl:Class; 
                   rdfs:comment """
"""@EN; 
                   rdfs:subClassOf ddhub:MarineSystem. 
ddhub:spiral a owl:Class; 
             rdfs:comment """
"""@EN; 
             rdfs:subClassOf ddhub:BladeShape. 
ddhub:SpontaneousPotential a owl:Class; 
                           rdfs:comment """
"""@EN; 
                           rdfs:subClassOf ddhub:WirelineLoggingTools. 
ddhub:SPP a owl:Class; 
          rdfs:comment """
"""@EN; 
          rdfs:subClassOf ddhub:PrototypeData. 
ddhub:SpudMud a owl:Class; 
              rdfs:comment """
"""@EN; 
              rdfs:subClassOf ddhub:DrillingFluid. 
ddhub:StabbingGuide a owl:Class; 
                    rdfs:comment """
"""@EN; 
                    rdfs:subClassOf ddhub:DrillFloorEquipment. 
ddhub:Stabilizers a owl:Class; 
                  rdfs:comment """
"""@EN; 
                  rdfs:subClassOf ddhub:DrillString. 
ddhub:StandardDimensionlessQuantity a owl:Class; 
                                    rdfs:comment """
"""@EN; 
                                    rdfs:subClassOf ddhub:MeasurableQuantity. 
ddhub:StandardElectricalDrawworks a owl:Class; 
                                  rdfs:comment """
"""@EN; 
                                  rdfs:subClassOf ddhub:Drawworks. 
ddhub:StandardLengthQuantity a owl:Class; 
                             rdfs:comment """
"""@EN; 
                             rdfs:subClassOf ddhub:MeasurableQuantity. 
ddhub:StandardProportionQuantity a owl:Class; 
                                 rdfs:comment """
"""@EN; 
                                 rdfs:subClassOf ddhub:MeasurableQuantity. 
ddhub:Stands a owl:Class; 
             rdfs:comment """
"""@EN; 
             rdfs:subClassOf ddhub:Grouping. 
ddhub:StartsHydraulicBranchDecomposition a owl:ObjectProperty; 
                                         rdfs:comment """
"""@EN; 
                                         rdfs:domain ddhub:DWISNoun; 
                                         rdfs:range ddhub:DWISNoun; 
                                         rdfs:subPropertyOf ddhub:DWISVerb. 
ddhub:SteadyStateModel a owl:Class; 
                       rdfs:comment """A model for which the state variables do not change with time.
"""@EN; 
                       rdfs:subClassOf ddhub:MathematicalModel. 
ddhub:Steerable a owl:Class; 
                rdfs:comment """
"""@EN; 
                rdfs:subClassOf ddhub:Stabilizers. 
ddhub:SteerableLinerDrilling a owl:Class; 
                             rdfs:comment """
"""@EN; 
                             rdfs:subClassOf ddhub:LinerDrilling. 
ddhub:SteerableMotor a owl:Class; 
                     rdfs:comment """
"""@EN; 
                     rdfs:subClassOf ddhub:DownholeMotor. 
ddhub:StickUpHeightVerticalLocation a owl:Class; 
                                    rdfs:comment """
"""@EN; 
                                    rdfs:subClassOf ddhub:VerticalReferenceLocation. 
ddhub:StochasticModel a owl:Class; 
                      rdfs:comment """
"""@EN; 
                      rdfs:subClassOf ddhub:ModelType. 
ddhub:StorageTank a owl:Class; 
                  rdfs:comment """
"""@EN; 
                  rdfs:subClassOf ddhub:MudPits. 
ddhub:StormLoop a owl:Class; 
                rdfs:comment """
"""@EN; 
                rdfs:subClassOf ddhub:MarineSystem. 
ddhub:straight a owl:Class; 
               rdfs:comment """
"""@EN; 
               rdfs:subClassOf ddhub:BladeShape. 
ddhub:StrainWaveBasedDiscretization a owl:Class; 
                                    rdfs:comment """A model can properly estimate values at the level of strain wave propagation.
"""@EN; 
                                    rdfs:subClassOf ddhub:ModellingDiscretization. 
ddhub:Stratum a owl:DatatypeProperty, owl:FunctionalProperty; 
              rdfs:comment """
"""@EN; 
              rdfs:domain ddhub:Clock; 
              rdfs:range xsd:int. 
ddhub:StringDataType a owl:Class; 
                     rdfs:comment """
"""@EN; 
                     rdfs:subClassOf ddhub:DataType. 
ddhub:StuckPipe a owl:Class; 
                rdfs:comment """
"""@EN; 
                rdfs:subClassOf ddhub:DrillingIncident. 
ddhub:sub-bent a owl:Class; 
               rdfs:comment """
"""@EN; 
               rdfs:subClassOf ddhub:MiscSubs. 
ddhub:sub-bit a owl:Class; 
              rdfs:comment """
"""@EN; 
              rdfs:subClassOf ddhub:MiscSubs. 
ddhub:sub-bumper a owl:Class; 
                 rdfs:comment """
"""@EN; 
                 rdfs:subClassOf ddhub:MiscSubs. 
ddhub:sub-catcher a owl:Class; 
                  rdfs:comment """
"""@EN; 
                  rdfs:subClassOf ddhub:MiscSubs. 
ddhub:sub-circulation a owl:Class; 
                      rdfs:comment """
"""@EN; 
                      rdfs:subClassOf ddhub:MiscSubs. 
ddhub:sub-cone a owl:Class; 
               rdfs:comment """
"""@EN; 
               rdfs:subClassOf ddhub:MiscSubs. 
ddhub:sub-crossover a owl:Class; 
                    rdfs:comment """
"""@EN; 
                    rdfs:subClassOf ddhub:MiscSubs. 
ddhub:sub-dart a owl:Class; 
               rdfs:comment """
"""@EN; 
               rdfs:subClassOf ddhub:MiscSubs. 
ddhub:sub-filter a owl:Class; 
                 rdfs:comment """
"""@EN; 
                 rdfs:subClassOf ddhub:MiscSubs. 
ddhub:sub-float a owl:Class; 
                rdfs:comment """
"""@EN; 
                rdfs:subClassOf ddhub:MiscSubs. 
ddhub:sub-jetting a owl:Class; 
                  rdfs:comment """
"""@EN; 
                  rdfs:subClassOf ddhub:MiscSubs. 
ddhub:sub-junk a owl:Class; 
               rdfs:comment """
"""@EN; 
               rdfs:subClassOf ddhub:MiscSubs. 
ddhub:sub-orienting a owl:Class; 
                    rdfs:comment """
"""@EN; 
                    rdfs:subClassOf ddhub:MiscSubs. 
ddhub:sub-ported a owl:Class; 
                 rdfs:comment """
"""@EN; 
                 rdfs:subClassOf ddhub:MiscSubs. 
ddhub:sub-restrictor a owl:Class; 
                     rdfs:comment """
"""@EN; 
                     rdfs:subClassOf ddhub:MiscSubs. 
ddhub:sub-saver a owl:Class; 
                rdfs:comment """
"""@EN; 
                rdfs:subClassOf ddhub:MiscSubs. 
ddhub:sub-shock a owl:Class; 
                rdfs:comment """
"""@EN; 
                rdfs:subClassOf ddhub:MiscSubs. 
ddhub:sub-stop a owl:Class; 
               rdfs:comment """
"""@EN; 
               rdfs:subClassOf ddhub:MiscSubs. 
ddhub:SubpressureRelief a owl:Class; 
                        rdfs:comment """
"""@EN; 
                        rdfs:subClassOf ddhub:MiscSubs. 
ddhub:SubpumpOut a owl:Class; 
                 rdfs:comment """
"""@EN; 
                 rdfs:subClassOf ddhub:MiscSubs. 
ddhub:SubseaBop a owl:Class; 
                rdfs:comment """
"""@EN; 
                rdfs:subClassOf ddhub:BopStack. 
ddhub:SubseaTestTree a owl:Class; 
                     rdfs:comment """
"""@EN; 
                     rdfs:subClassOf ddhub:WellTestingEquipment. 
ddhub:SubsideEntry a owl:Class; 
                   rdfs:comment """
"""@EN; 
                   rdfs:subClassOf ddhub:MiscSubs. 
ddhub:SupportLine a owl:Class; 
                  rdfs:comment """
"""@EN; 
                  rdfs:subClassOf ddhub:DrillLine. 
ddhub:SurfaceBop a owl:Class; 
                 rdfs:comment """
"""@EN; 
                 rdfs:subClassOf ddhub:BopStack. 
ddhub:SurfacePower a owl:Class; 
                   rdfs:comment """
"""@EN; 
                   rdfs:subClassOf ddhub:PowerSystems. 
ddhub:SurfaceRiser a owl:Class; 
                   rdfs:comment """
"""@EN; 
                   rdfs:subClassOf ddhub:DrillingRiser. 
ddhub:SurfaceRotationSystem a owl:Class; 
                            rdfs:comment """
"""@EN; 
                            rdfs:subClassOf ddhub:RigEquipment. 
ddhub:SurfaceRPM a owl:Class; 
                 rdfs:comment """
"""@EN; 
                 rdfs:subClassOf ddhub:PrototypeData. 
ddhub:SurfaceTorque a owl:Class; 
                    rdfs:comment """
"""@EN; 
                    rdfs:subClassOf ddhub:PrototypeData. 
ddhub:SurgeTank a owl:Class; 
                rdfs:comment """
"""@EN; 
                rdfs:subClassOf ddhub:MudPits. 
ddhub:SwivelSub a owl:Class; 
                rdfs:comment """
"""@EN; 
                rdfs:subClassOf ddhub:TopDrive. 
ddhub:Symbol a owl:DatatypeProperty, owl:FunctionalProperty; 
             rdfs:comment """
"""@EN; 
             rdfs:domain ddhub:Unit; 
             rdfs:range xsd:string. 
ddhub:SynchronizationDelay a owl:DatatypeProperty, owl:FunctionalProperty; 
                           rdfs:comment """
"""@EN; 
                           rdfs:domain ddhub:SynchronizationGroup; 
                           rdfs:range xsd:double. 
ddhub:SynchronizationGroup a owl:Class; 
                           rdfs:comment """
"""@EN; 
                           rdfs:subClassOf ddhub:DWISNoun. 
ddhub:SyntheticOilBasedMudSobm a owl:Class; 
                               rdfs:comment """
"""@EN; 
                               rdfs:subClassOf ddhub:DrillingFluid. 
ddhub:T a owl:DatatypeProperty, owl:FunctionalProperty; 
        rdfs:comment """Time exponent.
SI Unit: Second (s)
"""@EN; 
        rdfs:domain ddhub:Quantity; 
        rdfs:range xsd:int. 
ddhub:TangencyLength a owl:Class; 
                     rdfs:comment """the position along the drill-string, counted from the bit, from which we can consider that the pipes direction is tangential with the borehole direction.
"""@EN; 
                     rdfs:subClassOf ddhub:DWISNoun. 
ddhub:TangentialModelling a owl:Class; 
                          rdfs:comment """The model accounts for the change of tangential direction of some parts of the physical system.
"""@EN; 
                          rdfs:subClassOf ddhub:LateralModelling. 
ddhub:Tank a owl:Class; 
           rdfs:comment """
"""@EN; 
           rdfs:subClassOf ddhub:HydraulicLogicalElement. 
ddhub:Telemetry a owl:Class; 
                rdfs:comment """Technology used for transferring the data from its main origin.
"""@EN; 
                rdfs:subClassOf ddhub:DWISNoun. 
ddhub:TemperatureGradientQuantity a owl:Class; 
                                  rdfs:comment """
"""@EN; 
                                  rdfs:subClassOf ddhub:Quantity. 
ddhub:TemperatureIn a owl:Class; 
                    rdfs:comment """
"""@EN; 
                    rdfs:subClassOf ddhub:PrototypeData. 
ddhub:TemperatureOut a owl:Class; 
                     rdfs:comment """
"""@EN; 
                     rdfs:subClassOf ddhub:PrototypeData. 
ddhub:TemperatureQuantity a owl:Class; 
                          rdfs:comment """
"""@EN; 
                          rdfs:subClassOf ddhub:Quantity. 
ddhub:TensionQuantity a owl:Class; 
                      rdfs:comment """
"""@EN; 
                      rdfs:subClassOf ddhub:Quantity. 
ddhub:TestingTools a owl:Class; 
                   rdfs:comment """
"""@EN; 
                   rdfs:subClassOf ddhub:WellTestingEquipment. 
ddhub:TestPlug a owl:Class; 
               rdfs:comment """
"""@EN; 
               rdfs:subClassOf ddhub:WellTestingEquipment. 
ddhub:TestTools a owl:Class; 
                rdfs:comment """
"""@EN; 
                rdfs:subClassOf ddhub:WellTestingEquipment. 
ddhub:ThermalConductivityQuantity a owl:Class; 
                                  rdfs:comment """
"""@EN; 
                                  rdfs:subClassOf ddhub:Quantity. 
ddhub:ThermalConductivityTemperatureGradientQuantity a owl:Class; 
                                                     rdfs:comment """
"""@EN; 
                                                     rdfs:subClassOf ddhub:Quantity. 
ddhub:ThirdPartyRigEquipment a owl:Class; 
                             rdfs:comment """
"""@EN; 
                             rdfs:subClassOf ddhub:RigEquipment. 
ddhub:ThirdPartyTools a owl:Class; 
                      rdfs:comment """
"""@EN; 
                      rdfs:subClassOf ddhub:ThirdPartyRigEquipment. 
ddhub:ThreeDimensionalReferenceFrame a owl:Class; 
                                     rdfs:comment """
"""@EN; 
                                     rdfs:subClassOf ddhub:ReferenceFrame. 
ddhub:ThreeDModelling a owl:Class; 
                      rdfs:comment """The model only accounts for three dimensions
"""@EN; 
                      rdfs:subClassOf ddhub:ModellingDimensions. 
ddhub:ThreeWayManifold a owl:Class; 
                       rdfs:comment """
"""@EN; 
                       rdfs:subClassOf ddhub:GenericEquipment. 
ddhub:ThreeWayValve a owl:Class; 
                    rdfs:comment """
"""@EN; 
                    rdfs:subClassOf ddhub:GenericEquipment. 
ddhub:Thruster a owl:Class; 
               rdfs:comment """
"""@EN; 
               rdfs:subClassOf ddhub:DrillingEquipment. 
ddhub:ThT a owl:DatatypeProperty, owl:FunctionalProperty; 
          rdfs:comment """Thermodynamic temperature exponent.
SI Unit: Kelvin (K)
"""@EN; 
          rdfs:domain ddhub:Quantity; 
          rdfs:range xsd:int. 
ddhub:TimeBasedTransformation a owl:Class; 
                              rdfs:comment """Transformations that apply only to time series: time derivations, time integration, averaging...
"""@EN; 
                              rdfs:subClassOf ddhub:Transformation. 
ddhub:TimeQuantity a owl:Class; 
                   rdfs:comment """
"""@EN; 
                   rdfs:subClassOf ddhub:Quantity. 
ddhub:TimeReference a owl:Class; 
                    rdfs:comment """
"""@EN; 
                    rdfs:subClassOf ddhub:DWISNoun. 
ddhub:TimeSpanReference a owl:Class; 
                        rdfs:comment """
"""@EN; 
                        rdfs:subClassOf ddhub:RelativeTimeReference. 
ddhub:TimeStampAcquisition a owl:DatatypeProperty, owl:FunctionalProperty; 
                           rdfs:comment """this is a UTC date-time value at which the value has been acquired by the data acquisition system.
"""@EN; 
                           rdfs:domain ddhub:DynamicDrillingSignal; 
                           rdfs:range xsd:datetime. 
ddhub:TimeStampAtSource a owl:DatatypeProperty, owl:FunctionalProperty; 
                        rdfs:comment """this is a UTC date-time value corresponding to the time at which the value has been taken.
"""@EN; 
                        rdfs:domain ddhub:DynamicDrillingSignal; 
                        rdfs:range xsd:datetime. 
ddhub:TimeWindow a owl:DatatypeProperty, owl:FunctionalProperty; 
                 rdfs:comment """
"""@EN; 
                 rdfs:domain ddhub:TimeWindowMovingAverage, ddhub:TimeWindowRangeExtraction; 
                 rdfs:range xsd:double. 
ddhub:TimeWindowMovingAverage a owl:Class; 
                              rdfs:comment """
"""@EN; 
                              rdfs:subClassOf ddhub:MovingAverage. 
ddhub:TimeWindowRangeExtraction a owl:Class; 
                                rdfs:comment """
"""@EN; 
                                rdfs:subClassOf ddhub:RangeExtraction. 
ddhub:ToolJoint1ReferenceLocation a owl:Class; 
                                  rdfs:comment """
"""@EN; 
                                  rdfs:subClassOf ddhub:AbscissaReferenceLocation. 
ddhub:ToolJoint2ReferenceLocation a owl:Class; 
                                  rdfs:comment """
"""@EN; 
                                  rdfs:subClassOf ddhub:AbscissaReferenceLocation. 
ddhub:ToolJoint3ReferenceLocation a owl:Class; 
                                  rdfs:comment """
"""@EN; 
                                  rdfs:subClassOf ddhub:AbscissaReferenceLocation. 
ddhub:ToolJoint4ReferenceLocation a owl:Class; 
                                  rdfs:comment """
"""@EN; 
                                  rdfs:subClassOf ddhub:AbscissaReferenceLocation. 
ddhub:TopDrive a owl:Class; 
               rdfs:comment """
"""@EN; 
               rdfs:subClassOf ddhub:SurfaceRotationSystem. 
ddhub:TopDriveControlSystem a owl:Class; 
                            rdfs:comment """
"""@EN; 
                            rdfs:subClassOf ddhub:ControlSystem. 
ddhub:TopOfRatHoleLocation a owl:Class; 
                           rdfs:comment """
"""@EN; 
                           rdfs:subClassOf ddhub:AbscissaReferenceLocation. 
ddhub:TopOfStringPosition a owl:Class; 
                          rdfs:comment """
"""@EN; 
                          rdfs:subClassOf ddhub:PrototypeData. 
ddhub:TopOfStringReferenceLocation a owl:Class; 
                                   rdfs:comment """
"""@EN; 
                                   rdfs:subClassOf ddhub:AbscissaReferenceLocation. 
ddhub:TopShoulderAxialLocation a owl:Class; 
                               rdfs:comment """
"""@EN; 
                               rdfs:subClassOf ddhub:AxialReferenceLocation. 
ddhub:TopsideHydraulicNetwork a owl:Class; 
                              rdfs:comment """
"""@EN; 
                              rdfs:subClassOf ddhub:HydraulicNetwork. 
ddhub:TopSideTelemetry a owl:Class; 
                       rdfs:comment """Method that allows transfer of data from surface systems.
"""@EN; 
                       rdfs:subClassOf ddhub:Telemetry. 
ddhub:TorqueBushing a owl:Class; 
                    rdfs:comment """
"""@EN; 
                    rdfs:subClassOf ddhub:TopDrive. 
ddhub:TorqueQuantity a owl:Class; 
                     rdfs:comment """
"""@EN; 
                     rdfs:subClassOf ddhub:Quantity. 
ddhub:TorqueToForceTransformation a owl:Class; 
                                  rdfs:comment """
"""@EN; 
                                  rdfs:subClassOf ddhub:DirectTransformation. 
ddhub:TorqueTrack a owl:Class; 
                  rdfs:comment """
"""@EN; 
                  rdfs:subClassOf ddhub:TopDrive. 
ddhub:TorsionalMotionType a owl:Class; 
                          rdfs:comment """
"""@EN; 
                          rdfs:subClassOf ddhub:MotionType. 
ddhub:Transformation a owl:Class; 
                     rdfs:comment """Represents a transformation applied to some signals that produces other signals
"""@EN; 
                     rdfs:subClassOf ddhub:DataFlowNode. 
ddhub:TransientModel a owl:Class; 
                     rdfs:comment """A model for which the state variables changes with time.
"""@EN; 
                     rdfs:subClassOf ddhub:MathematicalModel. 
ddhub:TransmissionLine a owl:Class; 
                       rdfs:comment """
"""@EN; 
                       rdfs:subClassOf ddhub:DataFlowNode. 
ddhub:TravellingBlock a owl:Class; 
                      rdfs:comment """
"""@EN; 
                      rdfs:subClassOf ddhub:MechanicalBlock. 
ddhub:TripleStandDerrick a owl:Class; 
                         rdfs:comment """
"""@EN; 
                         rdfs:subClassOf ddhub:Derrick. 
ddhub:TripTank a owl:Class; 
               rdfs:comment """
"""@EN; 
               rdfs:subClassOf ddhub:MudPits. 
ddhub:TrueNorthAzimuthLocation a owl:Class; 
                               rdfs:comment """
"""@EN; 
                               rdfs:subClassOf ddhub:AzimuthReferenceLocation. 
ddhub:TubingGuideArch a owl:Class; 
                      rdfs:comment """
"""@EN; 
                      rdfs:subClassOf ddhub:CoiledTubingEquipment. 
ddhub:TubingHanger a owl:Class; 
                   rdfs:comment """
"""@EN; 
                   rdfs:subClassOf ddhub:Hangers. 
ddhub:TubingString a owl:Class; 
                   rdfs:comment """
"""@EN; 
                   rdfs:subClassOf <http://ddhub.no/<Tubulars>>. 
ddhub:TubularConfiguration a owl:Class; 
                           rdfs:comment """
"""@EN; 
                           rdfs:subClassOf <http://ddhub.no/<Tubulars>>. 
ddhub:TubularConnection a owl:Class; 
                        rdfs:comment """
"""@EN; 
                        rdfs:subClassOf <http://ddhub.no/<Tubulars>>. 
ddhub:TurbineMotor a owl:Class; 
                   rdfs:comment """
"""@EN; 
                   rdfs:subClassOf ddhub:DownholeMotor. 
ddhub:TwistOff a owl:Class; 
               rdfs:comment """
"""@EN; 
               rdfs:subClassOf ddhub:DrillingIncident. 
ddhub:TwoDimensionalReferenceFrame a owl:Class; 
                                   rdfs:comment """
"""@EN; 
                                   rdfs:subClassOf ddhub:ReferenceFrame. 
ddhub:TwoDModelling a owl:Class; 
                    rdfs:comment """The model only accounts for two dimensions
"""@EN; 
                    rdfs:subClassOf ddhub:ModellingDimensions. 
ddhub:Underpull a owl:Class; 
                rdfs:comment """
"""@EN; 
                rdfs:subClassOf ddhub:DrillingIncident. 
ddhub:Underreamers a owl:Class; 
                   rdfs:comment """
"""@EN; 
                   rdfs:subClassOf ddhub:HoleOpener. 
ddhub:Unit a owl:Class; 
           rdfs:comment """
"""@EN; 
           rdfs:subClassOf ddhub:DWISNoun. 
ddhub:UnitSystem a owl:Class; 
                 rdfs:comment """A set of associations between measurable quantities and units
"""@EN; 
                 rdfs:subClassOf ddhub:DWISNoun. 
ddhub:UpperSideAngleLocation a owl:Class; 
                             rdfs:comment """
"""@EN; 
                             rdfs:subClassOf ddhub:AngleReferenceLocation. 
ddhub:UserInterface a owl:Class; 
                    rdfs:comment """
"""@EN; 
                    rdfs:subClassOf ddhub:DataFlowNode. 
ddhub:UTCReference a owl:Class; 
                   rdfs:comment """
"""@EN; 
                   rdfs:subClassOf ddhub:TimeReference. 
ddhub:VacuumDegasser a owl:Class; 
                     rdfs:comment """
"""@EN; 
                     rdfs:subClassOf ddhub:Degasser. 
ddhub:Validity a owl:DatatypeProperty, owl:FunctionalProperty; 
               rdfs:comment """
"""@EN; 
               rdfs:domain ddhub:Resampling; 
               rdfs:range xsd:double. 
ddhub:ValidityCondition a owl:Class; 
                        rdfs:comment """
"""@EN; 
                        rdfs:subClassOf ddhub:DWISNoun. 
ddhub:Value a owl:DatatypeProperty, owl:FunctionalProperty; 
            rdfs:comment """
"""@EN; 
            rdfs:domain ddhub:DrillingSignal, ddhub:HydraulicConnectedState, ddhub:MechanicalElementState; 
            rdfs:range xsd:object, xsd:bool. 
ddhub:ValuesIndices a owl:DatatypeProperty, owl:FunctionalProperty; 
                    rdfs:comment """
"""@EN; 
                    rdfs:domain ddhub:EndPointMapping; 
                    rdfs:range <http://www.w3.org/2001/XMLSchema#int[]>. 
ddhub:variable a owl:Class; 
               rdfs:comment """
"""@EN; 
               rdfs:subClassOf ddhub:BladeShape. 
ddhub:VelocityQuantity a owl:Class; 
                       rdfs:comment """
"""@EN; 
                       rdfs:subClassOf ddhub:Quantity. 
ddhub:VentOverboardLine a owl:Class; 
                        rdfs:comment """
"""@EN; 
                        rdfs:subClassOf ddhub:Diverter. 
ddhub:VerticalDepthFrame a owl:Class; 
                         rdfs:comment """
"""@EN; 
                         rdfs:subClassOf ddhub:OneDimensionalCartesianReferenceFrame. 
ddhub:VerticalOndulationModelling a owl:Class; 
                                  rdfs:comment """The model accounts for the change of inclination of some parts of the physical system.
"""@EN; 
                                  rdfs:subClassOf ddhub:TangentialModelling. 
ddhub:VerticalReferenceLocation a owl:Class; 
                                rdfs:comment """
"""@EN; 
                                rdfs:subClassOf ddhub:Location. 
ddhub:VibrationIsolators a owl:Class; 
                         rdfs:comment """
"""@EN; 
                         rdfs:subClassOf ddhub:ActiveVibrationTools. 
ddhub:VolumeQuantity a owl:Class; 
                     rdfs:comment """
"""@EN; 
                     rdfs:subClassOf ddhub:Quantity. 
ddhub:VolumetricFlowRateOfChangeQuantity a owl:Class; 
                                         rdfs:comment """
"""@EN; 
                                         rdfs:subClassOf ddhub:Quantity. 
ddhub:VolumetricFlowRateQuantity a owl:Class; 
                                 rdfs:comment """
"""@EN; 
                                 rdfs:subClassOf ddhub:Quantity. 
ddhub:WaterBasedMudWbm a owl:Class; 
                       rdfs:comment """
"""@EN; 
                       rdfs:subClassOf ddhub:DrillingFluid. 
ddhub:WaveNumberQuantity a owl:Class; 
                         rdfs:comment """
"""@EN; 
                         rdfs:subClassOf ddhub:Quantity. 
ddhub:WeightOnBitQuantity a owl:Class; 
                          rdfs:comment """
"""@EN; 
                          rdfs:subClassOf ddhub:MeasurableQuantity. 
ddhub:WellboreCenterLineFrame a owl:Class; 
                              rdfs:comment """
"""@EN; 
                              rdfs:subClassOf ddhub:OneDimensionalCurviLinearReferenceFrame. 
ddhub:WellboreName a owl:DatatypeProperty, owl:FunctionalProperty; 
                   rdfs:comment """
"""@EN; 
                   rdfs:domain ddhub:WitsMLTimeBasedLogEndPoint; 
                   rdfs:range xsd:string. 
ddhub:WellboreUID a owl:DatatypeProperty, owl:FunctionalProperty; 
                  rdfs:comment """
"""@EN; 
                  rdfs:domain ddhub:WitsMLTimeBasedLogEndPoint; 
                  rdfs:range xsd:string. 
ddhub:WellcontrolStackEquipment a owl:Class; 
                                rdfs:comment """
"""@EN; 
                                rdfs:subClassOf ddhub:CoiledTubingEquipment. 
ddhub:WellControlSystem a owl:Class; 
                        rdfs:comment """
"""@EN; 
                        rdfs:subClassOf ddhub:RigEquipment. 
ddhub:WellHeadPositionLocation a owl:Class; 
                               rdfs:comment """
"""@EN; 
                               rdfs:subClassOf ddhub:PositionReferenceLocation. 
ddhub:WellHeadVerticalLocation a owl:Class; 
                               rdfs:comment """
"""@EN; 
                               rdfs:subClassOf ddhub:VerticalReferenceLocation. 
ddhub:WellheadXmasTree a owl:Class; 
                       rdfs:comment """
"""@EN; 
                       rdfs:subClassOf ddhub:WellControlSystem. 
ddhub:WellName a owl:DatatypeProperty, owl:FunctionalProperty; 
               rdfs:comment """
"""@EN; 
               rdfs:domain ddhub:WitsMLTimeBasedLogEndPoint; 
               rdfs:range xsd:string. 
ddhub:WellTestingEquipment a owl:Class; 
                           rdfs:comment """
"""@EN; 
                           rdfs:subClassOf ddhub:RigEquipment. 
ddhub:WellUID a owl:DatatypeProperty, owl:FunctionalProperty; 
              rdfs:comment """
"""@EN; 
              rdfs:domain ddhub:WitsMLTimeBasedLogEndPoint; 
              rdfs:range xsd:string. 
ddhub:WGS84PositionLocation a owl:Class; 
                            rdfs:comment """
"""@EN; 
                            rdfs:subClassOf ddhub:PositionReferenceLocation. 
ddhub:WGS84VerticalLocation a owl:Class; 
                            rdfs:comment """
"""@EN; 
                            rdfs:subClassOf ddhub:VerticalReferenceLocation. 
ddhub:Whipstock a owl:Class; 
                rdfs:comment """
"""@EN; 
                rdfs:subClassOf ddhub:DrillingEquipment. 
ddhub:WireCable a owl:Class; 
                rdfs:comment """
"""@EN; 
                rdfs:subClassOf ddhub:EquipmentTelemetry. 
ddhub:WiredPipe a owl:Class; 
                rdfs:comment """
"""@EN; 
                rdfs:subClassOf ddhub:EquipmentTelemetry. 
ddhub:WiredPipeTelemetry a owl:Class; 
                         rdfs:comment """A method that allows transfer of downhole data to the surface via electrical connections through the drill string.
"""@EN; 
                         rdfs:subClassOf ddhub:DownHoleTelemetry. 
ddhub:WirelineLoggingTools a owl:Class; 
                           rdfs:comment """
"""@EN; 
                           rdfs:subClassOf ddhub:LoggingEquipment. 
ddhub:WirelineLoggingToolsAcoustictools a owl:Class; 
                                        rdfs:comment """
"""@EN; 
                                        rdfs:subClassOf ddhub:WirelineLoggingTools. 
ddhub:WirelineLoggingToolsElectricalpropagation a owl:Class; 
                                                rdfs:comment """
"""@EN; 
                                                rdfs:subClassOf ddhub:WirelineLoggingTools. 
ddhub:WirelineLoggingToolsElectricalresistivity a owl:Class; 
                                                rdfs:comment """
"""@EN; 
                                                rdfs:subClassOf ddhub:WirelineLoggingTools. 
ddhub:WirelineLoggingToolsNmrtools a owl:Class; 
                                   rdfs:comment """
"""@EN; 
                                   rdfs:subClassOf ddhub:WirelineLoggingTools. 
ddhub:WirelineLoggingToolsNucleartools a owl:Class; 
                                       rdfs:comment """
"""@EN; 
                                       rdfs:subClassOf ddhub:WirelineLoggingTools. 
ddhub:WirelineLoggingToolsSeismictools a owl:Class; 
                                       rdfs:comment """
"""@EN; 
                                       rdfs:subClassOf ddhub:WirelineLoggingTools. 
ddhub:WitsMLTimeBasedLogEndPoint a owl:Class; 
                                 rdfs:comment """
"""@EN; 
                                 rdfs:subClassOf ddhub:DataEndPoint. 
ddhub:WOB a owl:Class; 
          rdfs:comment """
"""@EN; 
          rdfs:subClassOf ddhub:PrototypeData. 
ddhub:YoungModulusQuantity a owl:Class; 
                           rdfs:comment """
"""@EN; 
                           rdfs:subClassOf ddhub:MeasurableQuantity. 
